<?xml version="1.0"?>
<rdf:RDF xmlns:dc="http://purl.org/dc/elements/1.1/" xmlns:owl="http://www.w3.org/2002/07/owl#" xmlns:skosxl="http://www.w3.org/2008/05/skos-xl#" xmlns:rdfs="http://www.w3.org/2000/01/rdf-schema#" xmlns:dcterms="http://purl.org/dc/terms/" xmlns:xsd="http://www.w3.org/2001/XMLSchema#" xmlns:rdf="http://www.w3.org/1999/02/22-rdf-syntax-ns#" xmlns:cc="http://creativecommons.org/ns#" xmlns:skos="http://www.w3.org/2004/02/skos/core#" xml:base="http://stellar/">
	<skos:ConceptScheme rdf:about="http://purl.org/heritagedata/schemes/eh_tmc">
		<dcterms:identifier>http://purl.org/heritagedata/schemes/eh_tmc</dcterms:identifier>
		<cc:license rdf:resource="http://creativecommons.org/licenses/by/3.0" />
		<cc:attributionURL rdf:resource="http://www.english-heritage.org.uk" />
		<cc:attributionName xml:lang="en">English Heritage</cc:attributionName>
		<dcterms:title xml:lang="en">MARITIME CRAFT TYPE (EH)</dcterms:title>
		<rdfs:label xml:lang="en">MARITIME CRAFT TYPE (EH)</rdfs:label>
		<dcterms:description xml:lang="en">A thesaurus of craft types which survive as wrecks in English Heritage�s maritime record</dcterms:description>
		<dcterms:coverage rdf:resource="http://data.ordnancesurvey.co.uk/id/country/england" />
		<dcterms:publisher rdf:resource="http://www.english-heritage.org.uk" />
		<dcterms:issued rdf:datatype="http://www.w3.org/2001/XMLSchema#dateTime">2013-07-17T09:01:42</dcterms:issued>
		<skos:hasTopConcept>
			<skos:Concept rdf:about="http://purl.org/heritagedata/schemes/eh_tmc/concepts/100394">
				<skos:topConceptOf rdf:resource="http://purl.org/heritagedata/schemes/eh_tmc" />
				<skos:inScheme rdf:resource="http://purl.org/heritagedata/schemes/eh_tmc" />
				<dcterms:identifier>http://purl.org/heritagedata/schemes/eh_tmc/concepts/100394</dcterms:identifier>
				<skos:prefLabel xml:lang="en">MARITIME CRAFT</skos:prefLabel>
				<dcterms:issued rdf:datatype="http://www.w3.org/2001/XMLSchema#dateTime">2013-07-17T09:01:43</dcterms:issued>
				<skos:narrower rdf:resource="http://purl.org/heritagedata/schemes/eh_tmc/concepts/100260" />
				<skos:narrower>
					<skos:Concept rdf:about="http://purl.org/heritagedata/schemes/eh_tmc/concepts/162933">
						<skos:inScheme rdf:resource="http://purl.org/heritagedata/schemes/eh_tmc" />
						<dcterms:identifier>http://purl.org/heritagedata/schemes/eh_tmc/concepts/162933</dcterms:identifier>
						<skos:prefLabel xml:lang="en">AMPHIBIOUS VEHICLE</skos:prefLabel>
						<dcterms:issued rdf:datatype="http://www.w3.org/2001/XMLSchema#dateTime">2013-07-17T09:01:43</dcterms:issued>
						<skos:broader rdf:resource="http://purl.org/heritagedata/schemes/eh_tmc/concepts/100394" />
						<skos:scopeNote xml:lang="en">Vehicle either adapted, or purpose-built, to operate on both land and sea, for example a tank or DUKW.</skos:scopeNote>
						<cc:license rdf:resource="http://creativecommons.org/licenses/by/3.0" />
						<cc:attributionURL rdf:resource="http://www.english-heritage.org.uk" />
						<cc:attributionName xml:lang="en">English Heritage</cc:attributionName>
						<dcterms:publisher rdf:resource="http://www.english-heritage.org.uk" />
					</skos:Concept>
				</skos:narrower>
				<skos:narrower>
					<skos:Concept rdf:about="http://purl.org/heritagedata/schemes/eh_tmc/concepts/100281">
						<skos:inScheme rdf:resource="http://purl.org/heritagedata/schemes/eh_tmc" />
						<dcterms:identifier>http://purl.org/heritagedata/schemes/eh_tmc/concepts/100281</dcterms:identifier>
						<skos:prefLabel xml:lang="en">BLOCK SHIP</skos:prefLabel>
						<dcterms:issued rdf:datatype="http://www.w3.org/2001/XMLSchema#dateTime">2013-07-17T09:01:43</dcterms:issued>
						<skos:broader rdf:resource="http://purl.org/heritagedata/schemes/eh_tmc/concepts/100394" />
						<skos:scopeNote xml:lang="en">A hulk or obsolete vessel filled with cement or similar material and scuttled to block an entrance to a port or anchorage, usually as a defensive measure.</skos:scopeNote>
						<cc:license rdf:resource="http://creativecommons.org/licenses/by/3.0" />
						<cc:attributionURL rdf:resource="http://www.english-heritage.org.uk" />
						<cc:attributionName xml:lang="en">English Heritage</cc:attributionName>
						<dcterms:publisher rdf:resource="http://www.english-heritage.org.uk" />
					</skos:Concept>
				</skos:narrower>
				<skos:narrower>
					<skos:Concept rdf:about="http://purl.org/heritagedata/schemes/eh_tmc/concepts/100291">
						<skos:inScheme rdf:resource="http://purl.org/heritagedata/schemes/eh_tmc" />
						<dcterms:identifier>http://purl.org/heritagedata/schemes/eh_tmc/concepts/100291</dcterms:identifier>
						<skos:prefLabel xml:lang="en">CABLE LAYER</skos:prefLabel>
						<dcterms:issued rdf:datatype="http://www.w3.org/2001/XMLSchema#dateTime">2013-07-17T09:01:43</dcterms:issued>
						<skos:broader rdf:resource="http://purl.org/heritagedata/schemes/eh_tmc/concepts/100394" />
						<skos:scopeNote xml:lang="en">A ship used for laying cables (often telephone cables) along the sea bed.</skos:scopeNote>
						<cc:license rdf:resource="http://creativecommons.org/licenses/by/3.0" />
						<cc:attributionURL rdf:resource="http://www.english-heritage.org.uk" />
						<cc:attributionName xml:lang="en">English Heritage</cc:attributionName>
						<dcterms:publisher rdf:resource="http://www.english-heritage.org.uk" />
					</skos:Concept>
				</skos:narrower>
				<skos:narrower rdf:resource="http://purl.org/heritagedata/schemes/eh_tmc/concepts/100307" />
				<skos:narrower rdf:resource="http://purl.org/heritagedata/schemes/eh_tmc/concepts/145105" />
				<skos:narrower rdf:resource="http://purl.org/heritagedata/schemes/eh_tmc/concepts/100322" />
				<skos:narrower>
					<skos:Concept rdf:about="http://purl.org/heritagedata/schemes/eh_tmc/concepts/100334">
						<skos:inScheme rdf:resource="http://purl.org/heritagedata/schemes/eh_tmc" />
						<dcterms:identifier>http://purl.org/heritagedata/schemes/eh_tmc/concepts/100334</dcterms:identifier>
						<skos:prefLabel xml:lang="en">EXPERIMENTAL CRAFT</skos:prefLabel>
						<dcterms:issued rdf:datatype="http://www.w3.org/2001/XMLSchema#dateTime">2013-07-17T09:01:43</dcterms:issued>
						<skos:broader rdf:resource="http://purl.org/heritagedata/schemes/eh_tmc/concepts/100394" />
						<skos:scopeNote xml:lang="en">A craft built with the intention of demonstrating or advertising a novel design feature.</skos:scopeNote>
						<cc:license rdf:resource="http://creativecommons.org/licenses/by/3.0" />
						<cc:attributionURL rdf:resource="http://www.english-heritage.org.uk" />
						<cc:attributionName xml:lang="en">English Heritage</cc:attributionName>
						<dcterms:publisher rdf:resource="http://www.english-heritage.org.uk" />
					</skos:Concept>
				</skos:narrower>
				<skos:narrower rdf:resource="http://purl.org/heritagedata/schemes/eh_tmc/concepts/100335" />
				<skos:narrower rdf:resource="http://purl.org/heritagedata/schemes/eh_tmc/concepts/100342" />
				<skos:narrower rdf:resource="http://purl.org/heritagedata/schemes/eh_tmc/concepts/100355" />
				<skos:narrower>
					<skos:Concept rdf:about="http://purl.org/heritagedata/schemes/eh_tmc/concepts/100367">
						<skos:inScheme rdf:resource="http://purl.org/heritagedata/schemes/eh_tmc" />
						<dcterms:identifier>http://purl.org/heritagedata/schemes/eh_tmc/concepts/100367</dcterms:identifier>
						<skos:prefLabel xml:lang="en">HOUSE BOAT</skos:prefLabel>
						<dcterms:issued rdf:datatype="http://www.w3.org/2001/XMLSchema#dateTime">2013-07-17T09:01:43</dcterms:issued>
						<skos:broader rdf:resource="http://purl.org/heritagedata/schemes/eh_tmc/concepts/100394" />
						<skos:scopeNote xml:lang="en">A boat used as private or domestic living accomodation.</skos:scopeNote>
						<cc:license rdf:resource="http://creativecommons.org/licenses/by/3.0" />
						<cc:attributionURL rdf:resource="http://www.english-heritage.org.uk" />
						<cc:attributionName xml:lang="en">English Heritage</cc:attributionName>
						<dcterms:publisher rdf:resource="http://www.english-heritage.org.uk" />
					</skos:Concept>
				</skos:narrower>
				<skos:narrower rdf:resource="http://purl.org/heritagedata/schemes/eh_tmc/concepts/100369" />
				<skos:narrower>
					<skos:Concept rdf:about="http://purl.org/heritagedata/schemes/eh_tmc/concepts/100520">
						<skos:inScheme rdf:resource="http://purl.org/heritagedata/schemes/eh_tmc" />
						<dcterms:identifier>http://purl.org/heritagedata/schemes/eh_tmc/concepts/100520</dcterms:identifier>
						<skos:prefLabel xml:lang="en">LAUNCH</skos:prefLabel>
						<dcterms:issued rdf:datatype="http://www.w3.org/2001/XMLSchema#dateTime">2013-07-17T09:01:43</dcterms:issued>
						<skos:broader rdf:resource="http://purl.org/heritagedata/schemes/eh_tmc/concepts/100394" />
						<skos:scopeNote xml:lang="en">A large ship's boat powered by oars and or an engine.</skos:scopeNote>
						<cc:license rdf:resource="http://creativecommons.org/licenses/by/3.0" />
						<cc:attributionURL rdf:resource="http://www.english-heritage.org.uk" />
						<cc:attributionName xml:lang="en">English Heritage</cc:attributionName>
						<dcterms:publisher rdf:resource="http://www.english-heritage.org.uk" />
					</skos:Concept>
				</skos:narrower>
				<skos:narrower rdf:resource="http://purl.org/heritagedata/schemes/eh_tmc/concepts/100382" />
				<skos:narrower>
					<skos:Concept rdf:about="http://purl.org/heritagedata/schemes/eh_tmc/concepts/159157">
						<skos:inScheme rdf:resource="http://purl.org/heritagedata/schemes/eh_tmc" />
						<dcterms:identifier>http://purl.org/heritagedata/schemes/eh_tmc/concepts/159157</dcterms:identifier>
						<skos:prefLabel xml:lang="en">LONG BOAT</skos:prefLabel>
						<dcterms:issued rdf:datatype="http://www.w3.org/2001/XMLSchema#dateTime">2013-07-17T09:01:43</dcterms:issued>
						<skos:broader rdf:resource="http://purl.org/heritagedata/schemes/eh_tmc/concepts/100394" />
						<skos:scopeNote xml:lang="en">The largest boat belonging to a sailing vessel, and usually the means of escape from a sinking ship; powered by oars.</skos:scopeNote>
						<cc:license rdf:resource="http://creativecommons.org/licenses/by/3.0" />
						<cc:attributionURL rdf:resource="http://www.english-heritage.org.uk" />
						<cc:attributionName xml:lang="en">English Heritage</cc:attributionName>
						<dcterms:publisher rdf:resource="http://www.english-heritage.org.uk" />
					</skos:Concept>
				</skos:narrower>
				<skos:narrower>
					<skos:Concept rdf:about="http://purl.org/heritagedata/schemes/eh_tmc/concepts/100405">
						<skos:inScheme rdf:resource="http://purl.org/heritagedata/schemes/eh_tmc" />
						<dcterms:identifier>http://purl.org/heritagedata/schemes/eh_tmc/concepts/100405</dcterms:identifier>
						<skos:prefLabel xml:lang="en">MOTOR LAUNCH</skos:prefLabel>
						<dcterms:issued rdf:datatype="http://www.w3.org/2001/XMLSchema#dateTime">2013-07-17T09:01:43</dcterms:issued>
						<skos:altLabel xml:lang="en">B Class Motor Launch</skos:altLabel>
						<skos:broader rdf:resource="http://purl.org/heritagedata/schemes/eh_tmc/concepts/100394" />
						<skos:scopeNote xml:lang="en">Generic name for a small steam or power boat often carried on board a larger vessel.</skos:scopeNote>
						<cc:license rdf:resource="http://creativecommons.org/licenses/by/3.0" />
						<cc:attributionURL rdf:resource="http://www.english-heritage.org.uk" />
						<cc:attributionName xml:lang="en">English Heritage</cc:attributionName>
						<dcterms:publisher rdf:resource="http://www.english-heritage.org.uk" />
					</skos:Concept>
				</skos:narrower>
				<skos:narrower rdf:resource="http://purl.org/heritagedata/schemes/eh_tmc/concepts/100409" />
				<skos:narrower rdf:resource="http://purl.org/heritagedata/schemes/eh_tmc/concepts/100410" />
				<skos:narrower rdf:resource="http://purl.org/heritagedata/schemes/eh_tmc/concepts/100418" />
				<skos:narrower rdf:resource="http://purl.org/heritagedata/schemes/eh_tmc/concepts/139837" />
				<skos:narrower>
					<skos:Concept rdf:about="http://purl.org/heritagedata/schemes/eh_tmc/concepts/100428">
						<skos:inScheme rdf:resource="http://purl.org/heritagedata/schemes/eh_tmc" />
						<dcterms:identifier>http://purl.org/heritagedata/schemes/eh_tmc/concepts/100428</dcterms:identifier>
						<skos:prefLabel xml:lang="en">PONTOON</skos:prefLabel>
						<dcterms:issued rdf:datatype="http://www.w3.org/2001/XMLSchema#dateTime">2013-07-17T09:01:43</dcterms:issued>
						<skos:broader rdf:resource="http://purl.org/heritagedata/schemes/eh_tmc/concepts/100394" />
						<skos:scopeNote xml:lang="en">A flat bottomed boat or hollow float of which a number are used to support a temporary bridge over a river.</skos:scopeNote>
						<cc:license rdf:resource="http://creativecommons.org/licenses/by/3.0" />
						<cc:attributionURL rdf:resource="http://www.english-heritage.org.uk" />
						<cc:attributionName xml:lang="en">English Heritage</cc:attributionName>
						<dcterms:publisher rdf:resource="http://www.english-heritage.org.uk" />
					</skos:Concept>
				</skos:narrower>
				<skos:narrower rdf:resource="http://purl.org/heritagedata/schemes/eh_tmc/concepts/100432" />
				<skos:narrower>
					<skos:Concept rdf:about="http://purl.org/heritagedata/schemes/eh_tmc/concepts/144621">
						<skos:inScheme rdf:resource="http://purl.org/heritagedata/schemes/eh_tmc" />
						<dcterms:identifier>http://purl.org/heritagedata/schemes/eh_tmc/concepts/144621</dcterms:identifier>
						<skos:prefLabel xml:lang="en">PRIZE VESSEL</skos:prefLabel>
						<dcterms:issued rdf:datatype="http://www.w3.org/2001/XMLSchema#dateTime">2013-07-17T09:01:43</dcterms:issued>
						<skos:broader rdf:resource="http://purl.org/heritagedata/schemes/eh_tmc/concepts/100394" />
						<skos:scopeNote xml:lang="en">Cargo vessel or warship captured by a warship or privateer of a hostile nation in time of war, usually taken into that nation¿s mercantile, privateering or naval service.</skos:scopeNote>
						<cc:license rdf:resource="http://creativecommons.org/licenses/by/3.0" />
						<cc:attributionURL rdf:resource="http://www.english-heritage.org.uk" />
						<cc:attributionName xml:lang="en">English Heritage</cc:attributionName>
						<dcterms:publisher rdf:resource="http://www.english-heritage.org.uk" />
					</skos:Concept>
				</skos:narrower>
				<skos:narrower>
					<skos:Concept rdf:about="http://purl.org/heritagedata/schemes/eh_tmc/concepts/152385">
						<skos:inScheme rdf:resource="http://purl.org/heritagedata/schemes/eh_tmc" />
						<dcterms:identifier>http://purl.org/heritagedata/schemes/eh_tmc/concepts/152385</dcterms:identifier>
						<skos:prefLabel xml:lang="en">RADIO SHIP</skos:prefLabel>
						<dcterms:issued rdf:datatype="http://www.w3.org/2001/XMLSchema#dateTime">2013-07-17T09:01:43</dcterms:issued>
						<skos:broader rdf:resource="http://purl.org/heritagedata/schemes/eh_tmc/concepts/100394" />
						<skos:scopeNote xml:lang="en">Vessel fitted with broadcasting equipment and used for off-shore radio programme transmission.</skos:scopeNote>
						<cc:license rdf:resource="http://creativecommons.org/licenses/by/3.0" />
						<cc:attributionURL rdf:resource="http://www.english-heritage.org.uk" />
						<cc:attributionName xml:lang="en">English Heritage</cc:attributionName>
						<dcterms:publisher rdf:resource="http://www.english-heritage.org.uk" />
					</skos:Concept>
				</skos:narrower>
				<skos:narrower>
					<skos:Concept rdf:about="http://purl.org/heritagedata/schemes/eh_tmc/concepts/100436">
						<skos:inScheme rdf:resource="http://purl.org/heritagedata/schemes/eh_tmc" />
						<dcterms:identifier>http://purl.org/heritagedata/schemes/eh_tmc/concepts/100436</dcterms:identifier>
						<skos:prefLabel xml:lang="en">RAFT</skos:prefLabel>
						<dcterms:issued rdf:datatype="http://www.w3.org/2001/XMLSchema#dateTime">2013-07-17T09:01:43</dcterms:issued>
						<skos:broader rdf:resource="http://purl.org/heritagedata/schemes/eh_tmc/concepts/100394" />
						<skos:scopeNote xml:lang="en">A flat floating framework of planks or other materials used for supporting or carrying persons or goods.</skos:scopeNote>
						<cc:license rdf:resource="http://creativecommons.org/licenses/by/3.0" />
						<cc:attributionURL rdf:resource="http://www.english-heritage.org.uk" />
						<cc:attributionName xml:lang="en">English Heritage</cc:attributionName>
						<dcterms:publisher rdf:resource="http://www.english-heritage.org.uk" />
					</skos:Concept>
				</skos:narrower>
				<skos:narrower>
					<skos:Concept rdf:about="http://purl.org/heritagedata/schemes/eh_tmc/concepts/100526">
						<skos:inScheme rdf:resource="http://purl.org/heritagedata/schemes/eh_tmc" />
						<dcterms:identifier>http://purl.org/heritagedata/schemes/eh_tmc/concepts/100526</dcterms:identifier>
						<skos:prefLabel xml:lang="en">REFUGE BUOY</skos:prefLabel>
						<dcterms:issued rdf:datatype="http://www.w3.org/2001/XMLSchema#dateTime">2013-07-17T09:01:43</dcterms:issued>
						<skos:broader rdf:resource="http://purl.org/heritagedata/schemes/eh_tmc/concepts/100394" />
						<skos:scopeNote xml:lang="en">A buoy with a compartment into which shipwrecked mariners could climb to await rescue.</skos:scopeNote>
						<cc:license rdf:resource="http://creativecommons.org/licenses/by/3.0" />
						<cc:attributionURL rdf:resource="http://www.english-heritage.org.uk" />
						<cc:attributionName xml:lang="en">English Heritage</cc:attributionName>
						<dcterms:publisher rdf:resource="http://www.english-heritage.org.uk" />
					</skos:Concept>
				</skos:narrower>
				<skos:narrower rdf:resource="http://purl.org/heritagedata/schemes/eh_tmc/concepts/100443" />
				<skos:narrower rdf:resource="http://purl.org/heritagedata/schemes/eh_tmc/concepts/100444" />
				<skos:narrower rdf:resource="http://purl.org/heritagedata/schemes/eh_tmc/concepts/159232" />
				<skos:narrower rdf:resource="http://purl.org/heritagedata/schemes/eh_tmc/concepts/100450" />
				<skos:narrower>
					<skos:Concept rdf:about="http://purl.org/heritagedata/schemes/eh_tmc/concepts/100451">
						<skos:inScheme rdf:resource="http://purl.org/heritagedata/schemes/eh_tmc" />
						<dcterms:identifier>http://purl.org/heritagedata/schemes/eh_tmc/concepts/100451</dcterms:identifier>
						<skos:prefLabel xml:lang="en">SEWAGE DUMPING VESSEL</skos:prefLabel>
						<dcterms:issued rdf:datatype="http://www.w3.org/2001/XMLSchema#dateTime">2013-07-17T09:01:43</dcterms:issued>
						<skos:broader rdf:resource="http://purl.org/heritagedata/schemes/eh_tmc/concepts/100394" />
						<skos:scopeNote xml:lang="en">A vessel equipped with sealed tanks for transporting sewage and dumping it in deep water.</skos:scopeNote>
						<cc:license rdf:resource="http://creativecommons.org/licenses/by/3.0" />
						<cc:attributionURL rdf:resource="http://www.english-heritage.org.uk" />
						<cc:attributionName xml:lang="en">English Heritage</cc:attributionName>
						<dcterms:publisher rdf:resource="http://www.english-heritage.org.uk" />
					</skos:Concept>
				</skos:narrower>
				<skos:narrower>
					<skos:Concept rdf:about="http://purl.org/heritagedata/schemes/eh_tmc/concepts/100468">
						<skos:inScheme rdf:resource="http://purl.org/heritagedata/schemes/eh_tmc" />
						<dcterms:identifier>http://purl.org/heritagedata/schemes/eh_tmc/concepts/100468</dcterms:identifier>
						<skos:prefLabel xml:lang="en">SURVEY VESSEL</skos:prefLabel>
						<dcterms:issued rdf:datatype="http://www.w3.org/2001/XMLSchema#dateTime">2013-07-17T09:01:43</dcterms:issued>
						<skos:broader rdf:resource="http://purl.org/heritagedata/schemes/eh_tmc/concepts/100394" />
						<skos:scopeNote xml:lang="en">A craft which is equipped for and performs hydrographic surveys.</skos:scopeNote>
						<cc:license rdf:resource="http://creativecommons.org/licenses/by/3.0" />
						<cc:attributionURL rdf:resource="http://www.english-heritage.org.uk" />
						<cc:attributionName xml:lang="en">English Heritage</cc:attributionName>
						<dcterms:publisher rdf:resource="http://www.english-heritage.org.uk" />
					</skos:Concept>
				</skos:narrower>
				<skos:narrower rdf:resource="http://purl.org/heritagedata/schemes/eh_tmc/concepts/100479" />
				<skos:narrower rdf:resource="http://purl.org/heritagedata/schemes/eh_tmc/concepts/100480" />
				<skos:narrower rdf:resource="http://purl.org/heritagedata/schemes/eh_tmc/concepts/100482" />
				<skos:narrower rdf:resource="http://purl.org/heritagedata/schemes/eh_tmc/concepts/100485" />
				<skos:narrower rdf:resource="http://purl.org/heritagedata/schemes/eh_tmc/concepts/100490" />
				<skos:narrower>
					<skos:Concept rdf:about="http://purl.org/heritagedata/schemes/eh_tmc/concepts/152407">
						<skos:inScheme rdf:resource="http://purl.org/heritagedata/schemes/eh_tmc" />
						<dcterms:identifier>http://purl.org/heritagedata/schemes/eh_tmc/concepts/152407</dcterms:identifier>
						<skos:prefLabel xml:lang="en">WORK BOAT</skos:prefLabel>
						<dcterms:issued rdf:datatype="http://www.w3.org/2001/XMLSchema#dateTime">2013-07-17T09:01:43</dcterms:issued>
						<skos:broader rdf:resource="http://purl.org/heritagedata/schemes/eh_tmc/concepts/100394" />
						<skos:scopeNote xml:lang="en">Generic name for a vessel used for work rather than for recreation, transportation, or military purposes. The vessels include tugs, barges, landing craft, dredgers and standby safety vessels. Use only were the exact type of vessel is unknown.</skos:scopeNote>
						<cc:license rdf:resource="http://creativecommons.org/licenses/by/3.0" />
						<cc:attributionURL rdf:resource="http://www.english-heritage.org.uk" />
						<cc:attributionName xml:lang="en">English Heritage</cc:attributionName>
						<dcterms:publisher rdf:resource="http://www.english-heritage.org.uk" />
					</skos:Concept>
				</skos:narrower>
				<skos:scopeNote xml:lang="en">The class term, use more specific terms.</skos:scopeNote>
				<cc:license rdf:resource="http://creativecommons.org/licenses/by/3.0" />
				<cc:attributionURL rdf:resource="http://www.english-heritage.org.uk" />
				<cc:attributionName xml:lang="en">English Heritage</cc:attributionName>
				<dcterms:publisher rdf:resource="http://www.english-heritage.org.uk" />
			</skos:Concept>
		</skos:hasTopConcept>
	</skos:ConceptScheme>
	<skos:Concept rdf:about="http://purl.org/heritagedata/schemes/eh_tmc/concepts/100496">
		<skos:inScheme rdf:resource="http://purl.org/heritagedata/schemes/eh_tmc" />
		<dcterms:identifier>http://purl.org/heritagedata/schemes/eh_tmc/concepts/100496</dcterms:identifier>
		<skos:prefLabel xml:lang="en">WHALE UNIT</skos:prefLabel>
		<dcterms:issued rdf:datatype="http://www.w3.org/2001/XMLSchema#dateTime">2013-07-17T09:01:43</dcterms:issued>
		<skos:narrower>
			<skos:Concept rdf:about="http://purl.org/heritagedata/schemes/eh_tmc/concepts/146361">
				<skos:inScheme rdf:resource="http://purl.org/heritagedata/schemes/eh_tmc" />
				<dcterms:identifier>http://purl.org/heritagedata/schemes/eh_tmc/concepts/146361</dcterms:identifier>
				<skos:prefLabel xml:lang="en">BEETLE UNIT</skos:prefLabel>
				<dcterms:issued rdf:datatype="http://www.w3.org/2001/XMLSchema#dateTime">2013-07-17T09:01:43</dcterms:issued>
				<skos:broader rdf:resource="http://purl.org/heritagedata/schemes/eh_tmc/concepts/100496" />
				<skos:scopeNote xml:lang="en">Concrete or steel pontoons that supported the Whale piers. They were moored in position using wires attsched to Kite anchors.</skos:scopeNote>
				<cc:license rdf:resource="http://creativecommons.org/licenses/by/3.0" />
				<cc:attributionURL rdf:resource="http://www.english-heritage.org.uk" />
				<cc:attributionName xml:lang="en">English Heritage</cc:attributionName>
				<dcterms:publisher rdf:resource="http://www.english-heritage.org.uk" />
			</skos:Concept>
		</skos:narrower>
		<skos:broader rdf:resource="http://purl.org/heritagedata/schemes/eh_tmc/concepts/100409" />
		<skos:scopeNote xml:lang="en">A floating pier, comprised of a floating pierhead (SPUD) and a roadway resting on pontoons (BEETLES). The pierhead and roadway were capable of rising and falling with the tide enabling unloading of troops and equipment to occur at any state of the tide.</skos:scopeNote>
		<cc:license rdf:resource="http://creativecommons.org/licenses/by/3.0" />
		<cc:attributionURL rdf:resource="http://www.english-heritage.org.uk" />
		<cc:attributionName xml:lang="en">English Heritage</cc:attributionName>
		<dcterms:publisher rdf:resource="http://www.english-heritage.org.uk" />
	</skos:Concept>
	<skos:Concept rdf:about="http://purl.org/heritagedata/schemes/eh_tmc/concepts/100319">
		<skos:inScheme rdf:resource="http://purl.org/heritagedata/schemes/eh_tmc" />
		<dcterms:identifier>http://purl.org/heritagedata/schemes/eh_tmc/concepts/100319</dcterms:identifier>
		<skos:prefLabel xml:lang="en">DESTROYER</skos:prefLabel>
		<dcterms:issued rdf:datatype="http://www.w3.org/2001/XMLSchema#dateTime">2013-07-17T09:01:43</dcterms:issued>
		<skos:altLabel xml:lang="en">Hunt Class Destroyer</skos:altLabel>
		<skos:altLabel xml:lang="en">R Class Destroyer</skos:altLabel>
		<skos:altLabel xml:lang="en">Scott Class Destroyer</skos:altLabel>
		<skos:altLabel xml:lang="en">Basilisk Class Destroyer</skos:altLabel>
		<skos:altLabel xml:lang="en">C Class Destroyer</skos:altLabel>
		<skos:altLabel xml:lang="en">D Class Destroyer</skos:altLabel>
		<skos:broader rdf:resource="http://purl.org/heritagedata/schemes/eh_tmc/concepts/100490" />
		<skos:narrower>
			<skos:Concept rdf:about="http://purl.org/heritagedata/schemes/eh_tmc/concepts/100477">
				<skos:inScheme rdf:resource="http://purl.org/heritagedata/schemes/eh_tmc" />
				<dcterms:identifier>http://purl.org/heritagedata/schemes/eh_tmc/concepts/100477</dcterms:identifier>
				<skos:prefLabel xml:lang="en">TORPEDO BOAT DESTROYER</skos:prefLabel>
				<dcterms:issued rdf:datatype="http://www.w3.org/2001/XMLSchema#dateTime">2013-07-17T09:01:43</dcterms:issued>
				<skos:altLabel xml:lang="en">Dryad Class Torpedo Boat</skos:altLabel>
				<skos:broader rdf:resource="http://purl.org/heritagedata/schemes/eh_tmc/concepts/100319" />
				<skos:scopeNote xml:lang="en">A small fast warship developed in the late nineteenth century. Armed principally with quick firing guns to destroy enemy torpedo boats.</skos:scopeNote>
				<cc:license rdf:resource="http://creativecommons.org/licenses/by/3.0" />
				<cc:attributionURL rdf:resource="http://www.english-heritage.org.uk" />
				<cc:attributionName xml:lang="en">English Heritage</cc:attributionName>
				<dcterms:publisher rdf:resource="http://www.english-heritage.org.uk" />
			</skos:Concept>
		</skos:narrower>
		<skos:scopeNote xml:lang="en">A very fast small warship, armed with small calibre guns and torpedoes. Used for attacking enemy vessels, escort duties and anti submarine duties.</skos:scopeNote>
		<cc:license rdf:resource="http://creativecommons.org/licenses/by/3.0" />
		<cc:attributionURL rdf:resource="http://www.english-heritage.org.uk" />
		<cc:attributionName xml:lang="en">English Heritage</cc:attributionName>
		<dcterms:publisher rdf:resource="http://www.english-heritage.org.uk" />
	</skos:Concept>
	<skos:Concept rdf:about="http://purl.org/heritagedata/schemes/eh_tmc/concepts/100322">
		<skos:inScheme rdf:resource="http://purl.org/heritagedata/schemes/eh_tmc" />
		<dcterms:identifier>http://purl.org/heritagedata/schemes/eh_tmc/concepts/100322</dcterms:identifier>
		<skos:prefLabel xml:lang="en">DREDGER</skos:prefLabel>
		<dcterms:issued rdf:datatype="http://www.w3.org/2001/XMLSchema#dateTime">2013-07-17T09:01:43</dcterms:issued>
		<skos:narrower>
			<skos:Concept rdf:about="http://purl.org/heritagedata/schemes/eh_tmc/concepts/100286">
				<skos:inScheme rdf:resource="http://purl.org/heritagedata/schemes/eh_tmc" />
				<dcterms:identifier>http://purl.org/heritagedata/schemes/eh_tmc/concepts/100286</dcterms:identifier>
				<skos:prefLabel xml:lang="en">BUCKET DREDGER</skos:prefLabel>
				<dcterms:issued rdf:datatype="http://www.w3.org/2001/XMLSchema#dateTime">2013-07-17T09:01:43</dcterms:issued>
				<skos:broader rdf:resource="http://purl.org/heritagedata/schemes/eh_tmc/concepts/100322" />
				<skos:scopeNote xml:lang="en">A self propelled vessel for deepening harbours using a continuous chain of buckets</skos:scopeNote>
				<cc:license rdf:resource="http://creativecommons.org/licenses/by/3.0" />
				<cc:attributionURL rdf:resource="http://www.english-heritage.org.uk" />
				<cc:attributionName xml:lang="en">English Heritage</cc:attributionName>
				<dcterms:publisher rdf:resource="http://www.english-heritage.org.uk" />
			</skos:Concept>
		</skos:narrower>
		<skos:broader rdf:resource="http://purl.org/heritagedata/schemes/eh_tmc/concepts/100361" />
		<skos:broader rdf:resource="http://purl.org/heritagedata/schemes/eh_tmc/concepts/100394" />
		<skos:narrower>
			<skos:Concept rdf:about="http://purl.org/heritagedata/schemes/eh_tmc/concepts/100357">
				<skos:inScheme rdf:resource="http://purl.org/heritagedata/schemes/eh_tmc" />
				<dcterms:identifier>http://purl.org/heritagedata/schemes/eh_tmc/concepts/100357</dcterms:identifier>
				<skos:prefLabel xml:lang="en">GRAB DREDGER</skos:prefLabel>
				<dcterms:issued rdf:datatype="http://www.w3.org/2001/XMLSchema#dateTime">2013-07-17T09:01:43</dcterms:issued>
				<skos:broader rdf:resource="http://purl.org/heritagedata/schemes/eh_tmc/concepts/100322" />
				<skos:scopeNote xml:lang="en">A dredger with a grab hung on ropes or chains giving it unlimited depth of excavation. they can lift solids or pieces of wreckages and can work close to ships or to a dock wall.</skos:scopeNote>
				<cc:license rdf:resource="http://creativecommons.org/licenses/by/3.0" />
				<cc:attributionURL rdf:resource="http://www.english-heritage.org.uk" />
				<cc:attributionName xml:lang="en">English Heritage</cc:attributionName>
				<dcterms:publisher rdf:resource="http://www.english-heritage.org.uk" />
			</skos:Concept>
		</skos:narrower>
		<skos:narrower>
			<skos:Concept rdf:about="http://purl.org/heritagedata/schemes/eh_tmc/concepts/100365">
				<skos:inScheme rdf:resource="http://purl.org/heritagedata/schemes/eh_tmc" />
				<dcterms:identifier>http://purl.org/heritagedata/schemes/eh_tmc/concepts/100365</dcterms:identifier>
				<skos:prefLabel xml:lang="en">HOPPER DREDGER</skos:prefLabel>
				<dcterms:issued rdf:datatype="http://www.w3.org/2001/XMLSchema#dateTime">2013-07-17T09:01:43</dcterms:issued>
				<skos:broader rdf:resource="http://purl.org/heritagedata/schemes/eh_tmc/concepts/100322" />
				<skos:scopeNote xml:lang="en">A dredger which can act as its own hopper and can thus transport the mud which it picks up to dump it at the desired place.</skos:scopeNote>
				<cc:license rdf:resource="http://creativecommons.org/licenses/by/3.0" />
				<cc:attributionURL rdf:resource="http://www.english-heritage.org.uk" />
				<cc:attributionName xml:lang="en">English Heritage</cc:attributionName>
				<dcterms:publisher rdf:resource="http://www.english-heritage.org.uk" />
			</skos:Concept>
		</skos:narrower>
		<skos:narrower rdf:resource="http://purl.org/heritagedata/schemes/eh_tmc/concepts/100416" />
		<skos:narrower>
			<skos:Concept rdf:about="http://purl.org/heritagedata/schemes/eh_tmc/concepts/100467">
				<skos:inScheme rdf:resource="http://purl.org/heritagedata/schemes/eh_tmc" />
				<dcterms:identifier>http://purl.org/heritagedata/schemes/eh_tmc/concepts/100467</dcterms:identifier>
				<skos:prefLabel xml:lang="en">SUCTION DREDGER</skos:prefLabel>
				<dcterms:issued rdf:datatype="http://www.w3.org/2001/XMLSchema#dateTime">2013-07-17T09:01:43</dcterms:issued>
				<skos:broader rdf:resource="http://purl.org/heritagedata/schemes/eh_tmc/concepts/100322" />
				<skos:scopeNote xml:lang="en">A dredger that works by the use of suction.</skos:scopeNote>
				<cc:license rdf:resource="http://creativecommons.org/licenses/by/3.0" />
				<cc:attributionURL rdf:resource="http://www.english-heritage.org.uk" />
				<cc:attributionName xml:lang="en">English Heritage</cc:attributionName>
				<dcterms:publisher rdf:resource="http://www.english-heritage.org.uk" />
			</skos:Concept>
		</skos:narrower>
		<skos:scopeNote xml:lang="en">A craft used to deepen shipping channels, harbours and other water courses.</skos:scopeNote>
		<cc:license rdf:resource="http://creativecommons.org/licenses/by/3.0" />
		<cc:attributionURL rdf:resource="http://www.english-heritage.org.uk" />
		<cc:attributionName xml:lang="en">English Heritage</cc:attributionName>
		<dcterms:publisher rdf:resource="http://www.english-heritage.org.uk" />
	</skos:Concept>
	<skos:Concept rdf:about="http://purl.org/heritagedata/schemes/eh_tmc/concepts/100331">
		<skos:inScheme rdf:resource="http://purl.org/heritagedata/schemes/eh_tmc" />
		<dcterms:identifier>http://purl.org/heritagedata/schemes/eh_tmc/concepts/100331</dcterms:identifier>
		<skos:prefLabel xml:lang="en">ESCORT VESSEL</skos:prefLabel>
		<dcterms:issued rdf:datatype="http://www.w3.org/2001/XMLSchema#dateTime">2013-07-17T09:01:43</dcterms:issued>
		<skos:narrower>
			<skos:Concept rdf:about="http://purl.org/heritagedata/schemes/eh_tmc/concepts/100263">
				<skos:inScheme rdf:resource="http://purl.org/heritagedata/schemes/eh_tmc" />
				<dcterms:identifier>http://purl.org/heritagedata/schemes/eh_tmc/concepts/100263</dcterms:identifier>
				<skos:prefLabel xml:lang="en">ANTI SUBMARINE VESSEL</skos:prefLabel>
				<dcterms:issued rdf:datatype="http://www.w3.org/2001/XMLSchema#dateTime">2013-07-17T09:01:43</dcterms:issued>
				<skos:broader rdf:resource="http://purl.org/heritagedata/schemes/eh_tmc/concepts/100331" />
				<skos:scopeNote xml:lang="en">A small warship (often adapted from a trawler or drifter) used to hunt enemy submarines.</skos:scopeNote>
				<cc:license rdf:resource="http://creativecommons.org/licenses/by/3.0" />
				<cc:attributionURL rdf:resource="http://www.english-heritage.org.uk" />
				<cc:attributionName xml:lang="en">English Heritage</cc:attributionName>
				<dcterms:publisher rdf:resource="http://www.english-heritage.org.uk" />
			</skos:Concept>
		</skos:narrower>
		<skos:narrower>
			<skos:Concept rdf:about="http://purl.org/heritagedata/schemes/eh_tmc/concepts/100305">
				<skos:inScheme rdf:resource="http://purl.org/heritagedata/schemes/eh_tmc" />
				<dcterms:identifier>http://purl.org/heritagedata/schemes/eh_tmc/concepts/100305</dcterms:identifier>
				<skos:prefLabel xml:lang="en">CORVETTE (NON SAIL)</skos:prefLabel>
				<dcterms:issued rdf:datatype="http://www.w3.org/2001/XMLSchema#dateTime">2013-07-17T09:01:43</dcterms:issued>
				<skos:broader rdf:resource="http://purl.org/heritagedata/schemes/eh_tmc/concepts/100331" />
				<skos:scopeNote xml:lang="en">A small anti submarine escort vessel built in World War II</skos:scopeNote>
				<cc:license rdf:resource="http://creativecommons.org/licenses/by/3.0" />
				<cc:attributionURL rdf:resource="http://www.english-heritage.org.uk" />
				<cc:attributionName xml:lang="en">English Heritage</cc:attributionName>
				<dcterms:publisher rdf:resource="http://www.english-heritage.org.uk" />
			</skos:Concept>
		</skos:narrower>
		<skos:narrower>
			<skos:Concept rdf:about="http://purl.org/heritagedata/schemes/eh_tmc/concepts/100306">
				<skos:inScheme rdf:resource="http://purl.org/heritagedata/schemes/eh_tmc" />
				<dcterms:identifier>http://purl.org/heritagedata/schemes/eh_tmc/concepts/100306</dcterms:identifier>
				<skos:prefLabel xml:lang="en">CORVETTE (SAIL)</skos:prefLabel>
				<dcterms:issued rdf:datatype="http://www.w3.org/2001/XMLSchema#dateTime">2013-07-17T09:01:43</dcterms:issued>
				<skos:broader rdf:resource="http://purl.org/heritagedata/schemes/eh_tmc/concepts/100331" />
				<skos:scopeNote xml:lang="en">A flush decked sailing warship with a single tier of guns.</skos:scopeNote>
				<cc:license rdf:resource="http://creativecommons.org/licenses/by/3.0" />
				<cc:attributionURL rdf:resource="http://www.english-heritage.org.uk" />
				<cc:attributionName xml:lang="en">English Heritage</cc:attributionName>
				<dcterms:publisher rdf:resource="http://www.english-heritage.org.uk" />
			</skos:Concept>
		</skos:narrower>
		<skos:broader rdf:resource="http://purl.org/heritagedata/schemes/eh_tmc/concepts/100490" />
		<skos:narrower>
			<skos:Concept rdf:about="http://purl.org/heritagedata/schemes/eh_tmc/concepts/100349">
				<skos:inScheme rdf:resource="http://purl.org/heritagedata/schemes/eh_tmc" />
				<dcterms:identifier>http://purl.org/heritagedata/schemes/eh_tmc/concepts/100349</dcterms:identifier>
				<skos:prefLabel xml:lang="en">FRIGATE (NON SAIL)</skos:prefLabel>
				<dcterms:issued rdf:datatype="http://www.w3.org/2001/XMLSchema#dateTime">2013-07-17T09:01:43</dcterms:issued>
				<skos:altLabel xml:lang="en">Captain Class Frigate</skos:altLabel>
				<skos:broader rdf:resource="http://purl.org/heritagedata/schemes/eh_tmc/concepts/100331" />
				<skos:scopeNote xml:lang="en">A medium speed anti submarine escort vessel built from World War II</skos:scopeNote>
				<cc:license rdf:resource="http://creativecommons.org/licenses/by/3.0" />
				<cc:attributionURL rdf:resource="http://www.english-heritage.org.uk" />
				<cc:attributionName xml:lang="en">English Heritage</cc:attributionName>
				<dcterms:publisher rdf:resource="http://www.english-heritage.org.uk" />
			</skos:Concept>
		</skos:narrower>
		<skos:narrower>
			<skos:Concept rdf:about="http://purl.org/heritagedata/schemes/eh_tmc/concepts/100350">
				<skos:inScheme rdf:resource="http://purl.org/heritagedata/schemes/eh_tmc" />
				<dcterms:identifier>http://purl.org/heritagedata/schemes/eh_tmc/concepts/100350</dcterms:identifier>
				<skos:prefLabel xml:lang="en">FRIGATE (SAIL)</skos:prefLabel>
				<dcterms:issued rdf:datatype="http://www.w3.org/2001/XMLSchema#dateTime">2013-07-17T09:01:43</dcterms:issued>
				<skos:broader rdf:resource="http://purl.org/heritagedata/schemes/eh_tmc/concepts/100331" />
				<skos:scopeNote xml:lang="en">A three masted fully rigged warship armed with 24 to 38 guns on a single gundeck.</skos:scopeNote>
				<cc:license rdf:resource="http://creativecommons.org/licenses/by/3.0" />
				<cc:attributionURL rdf:resource="http://www.english-heritage.org.uk" />
				<cc:attributionName xml:lang="en">English Heritage</cc:attributionName>
				<dcterms:publisher rdf:resource="http://www.english-heritage.org.uk" />
			</skos:Concept>
		</skos:narrower>
		<skos:scopeNote xml:lang="en">A warship used to provide an escort to other warships or merchant ships against attack.</skos:scopeNote>
		<cc:license rdf:resource="http://creativecommons.org/licenses/by/3.0" />
		<cc:attributionURL rdf:resource="http://www.english-heritage.org.uk" />
		<cc:attributionName xml:lang="en">English Heritage</cc:attributionName>
		<dcterms:publisher rdf:resource="http://www.english-heritage.org.uk" />
	</skos:Concept>
	<skos:Concept rdf:about="http://purl.org/heritagedata/schemes/eh_tmc/concepts/100335">
		<skos:inScheme rdf:resource="http://purl.org/heritagedata/schemes/eh_tmc" />
		<dcterms:identifier>http://purl.org/heritagedata/schemes/eh_tmc/concepts/100335</dcterms:identifier>
		<skos:prefLabel xml:lang="en">FACTORY SHIP</skos:prefLabel>
		<dcterms:issued rdf:datatype="http://www.w3.org/2001/XMLSchema#dateTime">2013-07-17T09:01:43</dcterms:issued>
		<skos:broader rdf:resource="http://purl.org/heritagedata/schemes/eh_tmc/concepts/100394" />
		<skos:narrower>
			<skos:Concept rdf:about="http://purl.org/heritagedata/schemes/eh_tmc/concepts/100495">
				<skos:inScheme rdf:resource="http://purl.org/heritagedata/schemes/eh_tmc" />
				<dcterms:identifier>http://purl.org/heritagedata/schemes/eh_tmc/concepts/100495</dcterms:identifier>
				<skos:prefLabel xml:lang="en">WHALE PROCESSING SHIP</skos:prefLabel>
				<dcterms:issued rdf:datatype="http://www.w3.org/2001/XMLSchema#dateTime">2013-07-17T09:01:43</dcterms:issued>
				<skos:broader rdf:resource="http://purl.org/heritagedata/schemes/eh_tmc/concepts/100335" />
				<skos:scopeNote xml:lang="en">A ship used to process whales into saleable products.</skos:scopeNote>
				<cc:license rdf:resource="http://creativecommons.org/licenses/by/3.0" />
				<cc:attributionURL rdf:resource="http://www.english-heritage.org.uk" />
				<cc:attributionName xml:lang="en">English Heritage</cc:attributionName>
				<dcterms:publisher rdf:resource="http://www.english-heritage.org.uk" />
			</skos:Concept>
		</skos:narrower>
		<skos:scopeNote xml:lang="en">A vessel with equipment for processing dead marine life whilst still at sea.</skos:scopeNote>
		<cc:license rdf:resource="http://creativecommons.org/licenses/by/3.0" />
		<cc:attributionURL rdf:resource="http://www.english-heritage.org.uk" />
		<cc:attributionName xml:lang="en">English Heritage</cc:attributionName>
		<dcterms:publisher rdf:resource="http://www.english-heritage.org.uk" />
	</skos:Concept>
	<skos:Concept rdf:about="http://purl.org/heritagedata/schemes/eh_tmc/concepts/100336">
		<skos:inScheme rdf:resource="http://purl.org/heritagedata/schemes/eh_tmc" />
		<dcterms:identifier>http://purl.org/heritagedata/schemes/eh_tmc/concepts/100336</dcterms:identifier>
		<skos:prefLabel xml:lang="en">FERRY</skos:prefLabel>
		<dcterms:issued rdf:datatype="http://www.w3.org/2001/XMLSchema#dateTime">2013-07-17T09:01:43</dcterms:issued>
		<skos:narrower>
			<skos:Concept rdf:about="http://purl.org/heritagedata/schemes/eh_tmc/concepts/151872">
				<skos:inScheme rdf:resource="http://purl.org/heritagedata/schemes/eh_tmc" />
				<dcterms:identifier>http://purl.org/heritagedata/schemes/eh_tmc/concepts/151872</dcterms:identifier>
				<skos:prefLabel xml:lang="en">CHAIN FERRY</skos:prefLabel>
				<dcterms:issued rdf:datatype="http://www.w3.org/2001/XMLSchema#dateTime">2013-07-17T09:01:43</dcterms:issued>
				<skos:broader rdf:resource="http://purl.org/heritagedata/schemes/eh_tmc/concepts/100336" />
				<skos:scopeNote xml:lang="en">A small ferry powered by steam or diesel engine, which pull vessel from one side of a river crossing along submerged chains.</skos:scopeNote>
				<cc:license rdf:resource="http://creativecommons.org/licenses/by/3.0" />
				<cc:attributionURL rdf:resource="http://www.english-heritage.org.uk" />
				<cc:attributionName xml:lang="en">English Heritage</cc:attributionName>
				<dcterms:publisher rdf:resource="http://www.english-heritage.org.uk" />
			</skos:Concept>
		</skos:narrower>
		<skos:broader rdf:resource="http://purl.org/heritagedata/schemes/eh_tmc/concepts/100419" />
		<skos:narrower>
			<skos:Concept rdf:about="http://purl.org/heritagedata/schemes/eh_tmc/concepts/152408">
				<skos:inScheme rdf:resource="http://purl.org/heritagedata/schemes/eh_tmc" />
				<dcterms:identifier>http://purl.org/heritagedata/schemes/eh_tmc/concepts/152408</dcterms:identifier>
				<skos:prefLabel xml:lang="en">ROLL ON ROLL OFF FERRY</skos:prefLabel>
				<dcterms:issued rdf:datatype="http://www.w3.org/2001/XMLSchema#dateTime">2013-07-17T09:01:43</dcterms:issued>
				<skos:altLabel xml:lang="en">Roro Ferry</skos:altLabel>
				<skos:broader rdf:resource="http://purl.org/heritagedata/schemes/eh_tmc/concepts/100336" />
				<skos:scopeNote xml:lang="en">A type of ferry that is designed to carry wheeled vehicles that can be driven on to and off the vessel.</skos:scopeNote>
				<cc:license rdf:resource="http://creativecommons.org/licenses/by/3.0" />
				<cc:attributionURL rdf:resource="http://www.english-heritage.org.uk" />
				<cc:attributionName xml:lang="en">English Heritage</cc:attributionName>
				<dcterms:publisher rdf:resource="http://www.english-heritage.org.uk" />
			</skos:Concept>
		</skos:narrower>
		<skos:scopeNote xml:lang="en">A vessel designed for the transport of persons and goods from one place to another an a regular schedule of sailings. Use specific type were known.</skos:scopeNote>
		<cc:license rdf:resource="http://creativecommons.org/licenses/by/3.0" />
		<cc:attributionURL rdf:resource="http://www.english-heritage.org.uk" />
		<cc:attributionName xml:lang="en">English Heritage</cc:attributionName>
		<dcterms:publisher rdf:resource="http://www.english-heritage.org.uk" />
	</skos:Concept>
	<skos:Concept rdf:about="http://purl.org/heritagedata/schemes/eh_tmc/concepts/100337">
		<skos:inScheme rdf:resource="http://purl.org/heritagedata/schemes/eh_tmc" />
		<dcterms:identifier>http://purl.org/heritagedata/schemes/eh_tmc/concepts/100337</dcterms:identifier>
		<skos:prefLabel xml:lang="en">FIRE FIGHTING TUG</skos:prefLabel>
		<dcterms:issued rdf:datatype="http://www.w3.org/2001/XMLSchema#dateTime">2013-07-17T09:01:43</dcterms:issued>
		<skos:broader rdf:resource="http://purl.org/heritagedata/schemes/eh_tmc/concepts/100485" />
		<skos:broader rdf:resource="http://purl.org/heritagedata/schemes/eh_tmc/concepts/100338" />
		<skos:scopeNote xml:lang="en">A tug equipped with water tanks and pumps for fighting fires at sea or on the shore line.</skos:scopeNote>
		<cc:license rdf:resource="http://creativecommons.org/licenses/by/3.0" />
		<cc:attributionURL rdf:resource="http://www.english-heritage.org.uk" />
		<cc:attributionName xml:lang="en">English Heritage</cc:attributionName>
		<dcterms:publisher rdf:resource="http://www.english-heritage.org.uk" />
	</skos:Concept>
	<skos:Concept rdf:about="http://purl.org/heritagedata/schemes/eh_tmc/concepts/100338">
		<skos:inScheme rdf:resource="http://purl.org/heritagedata/schemes/eh_tmc" />
		<dcterms:identifier>http://purl.org/heritagedata/schemes/eh_tmc/concepts/100338</dcterms:identifier>
		<skos:prefLabel xml:lang="en">FIRE FIGHTING VESSEL</skos:prefLabel>
		<dcterms:issued rdf:datatype="http://www.w3.org/2001/XMLSchema#dateTime">2013-07-17T09:01:43</dcterms:issued>
		<skos:narrower rdf:resource="http://purl.org/heritagedata/schemes/eh_tmc/concepts/100337" />
		<skos:broader rdf:resource="http://purl.org/heritagedata/schemes/eh_tmc/concepts/100450" />
		<skos:scopeNote xml:lang="en">A vessel equipped with water tanks and pumps for fighting fires at sea or on the shore line.</skos:scopeNote>
		<cc:license rdf:resource="http://creativecommons.org/licenses/by/3.0" />
		<cc:attributionURL rdf:resource="http://www.english-heritage.org.uk" />
		<cc:attributionName xml:lang="en">English Heritage</cc:attributionName>
		<dcterms:publisher rdf:resource="http://www.english-heritage.org.uk" />
	</skos:Concept>
	<skos:Concept rdf:about="http://purl.org/heritagedata/schemes/eh_tmc/concepts/100342">
		<skos:inScheme rdf:resource="http://purl.org/heritagedata/schemes/eh_tmc" />
		<dcterms:identifier>http://purl.org/heritagedata/schemes/eh_tmc/concepts/100342</dcterms:identifier>
		<skos:prefLabel xml:lang="en">FISHING VESSEL</skos:prefLabel>
		<dcterms:issued rdf:datatype="http://www.w3.org/2001/XMLSchema#dateTime">2013-07-17T09:01:43</dcterms:issued>
		<skos:altLabel xml:lang="en">Fishing Boat</skos:altLabel>
		<skos:narrower>
			<skos:Concept rdf:about="http://purl.org/heritagedata/schemes/eh_tmc/concepts/100271">
				<skos:inScheme rdf:resource="http://purl.org/heritagedata/schemes/eh_tmc" />
				<dcterms:identifier>http://purl.org/heritagedata/schemes/eh_tmc/concepts/100271</dcterms:identifier>
				<skos:prefLabel xml:lang="en">BANKER</skos:prefLabel>
				<dcterms:issued rdf:datatype="http://www.w3.org/2001/XMLSchema#dateTime">2013-07-17T09:01:43</dcterms:issued>
				<skos:broader rdf:resource="http://purl.org/heritagedata/schemes/eh_tmc/concepts/100342" />
				<skos:scopeNote xml:lang="en">A fishing vessel employed exclusively on the Grand Banks cod fisheries.</skos:scopeNote>
				<cc:license rdf:resource="http://creativecommons.org/licenses/by/3.0" />
				<cc:attributionURL rdf:resource="http://www.english-heritage.org.uk" />
				<cc:attributionName xml:lang="en">English Heritage</cc:attributionName>
				<dcterms:publisher rdf:resource="http://www.english-heritage.org.uk" />
			</skos:Concept>
		</skos:narrower>
		<skos:narrower>
			<skos:Concept rdf:about="http://purl.org/heritagedata/schemes/eh_tmc/concepts/100323">
				<skos:inScheme rdf:resource="http://purl.org/heritagedata/schemes/eh_tmc" />
				<dcterms:identifier>http://purl.org/heritagedata/schemes/eh_tmc/concepts/100323</dcterms:identifier>
				<skos:prefLabel xml:lang="en">DRIFTER</skos:prefLabel>
				<dcterms:issued rdf:datatype="http://www.w3.org/2001/XMLSchema#dateTime">2013-07-17T09:01:43</dcterms:issued>
				<skos:altLabel xml:lang="en">Admiralty Drifter</skos:altLabel>
				<skos:broader rdf:resource="http://purl.org/heritagedata/schemes/eh_tmc/concepts/100342" />
				<skos:scopeNote xml:lang="en">A fishing boat using nets which are free to move with the tides and currents.</skos:scopeNote>
				<cc:license rdf:resource="http://creativecommons.org/licenses/by/3.0" />
				<cc:attributionURL rdf:resource="http://www.english-heritage.org.uk" />
				<cc:attributionName xml:lang="en">English Heritage</cc:attributionName>
				<dcterms:publisher rdf:resource="http://www.english-heritage.org.uk" />
			</skos:Concept>
		</skos:narrower>
		<skos:broader rdf:resource="http://purl.org/heritagedata/schemes/eh_tmc/concepts/100394" />
		<skos:narrower rdf:resource="http://purl.org/heritagedata/schemes/eh_tmc/concepts/140478" />
		<skos:narrower>
			<skos:Concept rdf:about="http://purl.org/heritagedata/schemes/eh_tmc/concepts/164184">
				<skos:inScheme rdf:resource="http://purl.org/heritagedata/schemes/eh_tmc" />
				<dcterms:identifier>http://purl.org/heritagedata/schemes/eh_tmc/concepts/164184</dcterms:identifier>
				<skos:prefLabel xml:lang="en">LANCASHIRE NOBBY</skos:prefLabel>
				<dcterms:issued rdf:datatype="http://www.w3.org/2001/XMLSchema#dateTime">2013-07-17T09:01:43</dcterms:issued>
				<skos:broader rdf:resource="http://purl.org/heritagedata/schemes/eh_tmc/concepts/100342" />
				<skos:scopeNote xml:lang="en">Fishing smack specialised both for working shoal water and for trawling for shrimp, predominantly in and around Morecambe Bay.</skos:scopeNote>
				<cc:license rdf:resource="http://creativecommons.org/licenses/by/3.0" />
				<cc:attributionURL rdf:resource="http://www.english-heritage.org.uk" />
				<cc:attributionName xml:lang="en">English Heritage</cc:attributionName>
				<dcterms:publisher rdf:resource="http://www.english-heritage.org.uk" />
			</skos:Concept>
		</skos:narrower>
		<skos:narrower rdf:resource="http://purl.org/heritagedata/schemes/eh_tmc/concepts/100416" />
		<skos:narrower>
			<skos:Concept rdf:about="http://purl.org/heritagedata/schemes/eh_tmc/concepts/152411">
				<skos:inScheme rdf:resource="http://purl.org/heritagedata/schemes/eh_tmc" />
				<dcterms:identifier>http://purl.org/heritagedata/schemes/eh_tmc/concepts/152411</dcterms:identifier>
				<skos:prefLabel xml:lang="en">SEINER</skos:prefLabel>
				<dcterms:issued rdf:datatype="http://www.w3.org/2001/XMLSchema#dateTime">2013-07-17T09:01:43</dcterms:issued>
				<skos:broader rdf:resource="http://purl.org/heritagedata/schemes/eh_tmc/concepts/100342" />
				<skos:scopeNote xml:lang="en">A fishing vessel that catches fish by using a Seining net, that is a large net that is made to hang in the water by attaching weights along the bottom edge and counteracting floats along the top.</skos:scopeNote>
				<cc:license rdf:resource="http://creativecommons.org/licenses/by/3.0" />
				<cc:attributionURL rdf:resource="http://www.english-heritage.org.uk" />
				<cc:attributionName xml:lang="en">English Heritage</cc:attributionName>
				<dcterms:publisher rdf:resource="http://www.english-heritage.org.uk" />
			</skos:Concept>
		</skos:narrower>
		<skos:narrower>
			<skos:Concept rdf:about="http://purl.org/heritagedata/schemes/eh_tmc/concepts/147522">
				<skos:inScheme rdf:resource="http://purl.org/heritagedata/schemes/eh_tmc" />
				<dcterms:identifier>http://purl.org/heritagedata/schemes/eh_tmc/concepts/147522</dcterms:identifier>
				<skos:prefLabel xml:lang="en">TERRE NEUVA</skos:prefLabel>
				<dcterms:issued rdf:datatype="http://www.w3.org/2001/XMLSchema#dateTime">2013-07-17T09:01:43</dcterms:issued>
				<skos:broader rdf:resource="http://purl.org/heritagedata/schemes/eh_tmc/concepts/100342" />
				<skos:scopeNote xml:lang="en">French Banker, fishing vessel for the Grand Banks of Newfoundland, generally three-masted or of brig type, from the late 19th and 20th centuries.</skos:scopeNote>
				<cc:license rdf:resource="http://creativecommons.org/licenses/by/3.0" />
				<cc:attributionURL rdf:resource="http://www.english-heritage.org.uk" />
				<cc:attributionName xml:lang="en">English Heritage</cc:attributionName>
				<dcterms:publisher rdf:resource="http://www.english-heritage.org.uk" />
			</skos:Concept>
		</skos:narrower>
		<skos:narrower>
			<skos:Concept rdf:about="http://purl.org/heritagedata/schemes/eh_tmc/concepts/100481">
				<skos:inScheme rdf:resource="http://purl.org/heritagedata/schemes/eh_tmc" />
				<dcterms:identifier>http://purl.org/heritagedata/schemes/eh_tmc/concepts/100481</dcterms:identifier>
				<skos:prefLabel xml:lang="en">TRAWLER</skos:prefLabel>
				<dcterms:issued rdf:datatype="http://www.w3.org/2001/XMLSchema#dateTime">2013-07-17T09:01:43</dcterms:issued>
				<skos:altLabel xml:lang="en">Admiralty Trawler</skos:altLabel>
				<skos:altLabel xml:lang="en">Auxiliary Trawler</skos:altLabel>
				<skos:broader rdf:resource="http://purl.org/heritagedata/schemes/eh_tmc/concepts/100342" />
				<skos:scopeNote xml:lang="en">A fishing vessel specially designed to operate and trawl for the catching of bottom lying fish. Use with power where known.</skos:scopeNote>
				<cc:license rdf:resource="http://creativecommons.org/licenses/by/3.0" />
				<cc:attributionURL rdf:resource="http://www.english-heritage.org.uk" />
				<cc:attributionName xml:lang="en">English Heritage</cc:attributionName>
				<dcterms:publisher rdf:resource="http://www.english-heritage.org.uk" />
			</skos:Concept>
		</skos:narrower>
		<skos:narrower rdf:resource="http://purl.org/heritagedata/schemes/eh_tmc/concepts/100497" />
		<skos:scopeNote xml:lang="en">A vessel or craft used for catching or harvesting marine life by a variety of methods, use specific method where known.</skos:scopeNote>
		<cc:license rdf:resource="http://creativecommons.org/licenses/by/3.0" />
		<cc:attributionURL rdf:resource="http://www.english-heritage.org.uk" />
		<cc:attributionName xml:lang="en">English Heritage</cc:attributionName>
		<dcterms:publisher rdf:resource="http://www.english-heritage.org.uk" />
	</skos:Concept>
	<skos:Concept rdf:about="http://purl.org/heritagedata/schemes/eh_tmc/concepts/100355">
		<skos:inScheme rdf:resource="http://purl.org/heritagedata/schemes/eh_tmc" />
		<dcterms:identifier>http://purl.org/heritagedata/schemes/eh_tmc/concepts/100355</dcterms:identifier>
		<skos:prefLabel xml:lang="en">GALLEY</skos:prefLabel>
		<dcterms:issued rdf:datatype="http://www.w3.org/2001/XMLSchema#dateTime">2013-07-17T09:01:43</dcterms:issued>
		<skos:altLabel xml:lang="en">Oared Galley</skos:altLabel>
		<skos:broader rdf:resource="http://purl.org/heritagedata/schemes/eh_tmc/concepts/100394" />
		<skos:related rdf:resource="http://purl.org/heritagedata/schemes/eh_tmc/concepts/146425" />
		<skos:scopeNote xml:lang="en">Oared fighting ship with ancillary sails.</skos:scopeNote>
		<cc:license rdf:resource="http://creativecommons.org/licenses/by/3.0" />
		<cc:attributionURL rdf:resource="http://www.english-heritage.org.uk" />
		<cc:attributionName xml:lang="en">English Heritage</cc:attributionName>
		<dcterms:publisher rdf:resource="http://www.english-heritage.org.uk" />
	</skos:Concept>
	<skos:Concept rdf:about="http://purl.org/heritagedata/schemes/eh_tmc/concepts/100359">
		<skos:inScheme rdf:resource="http://purl.org/heritagedata/schemes/eh_tmc" />
		<dcterms:identifier>http://purl.org/heritagedata/schemes/eh_tmc/concepts/100359</dcterms:identifier>
		<skos:prefLabel xml:lang="en">GUNBOAT</skos:prefLabel>
		<dcterms:issued rdf:datatype="http://www.w3.org/2001/XMLSchema#dateTime">2013-07-17T09:01:43</dcterms:issued>
		<skos:narrower>
			<skos:Concept rdf:about="http://purl.org/heritagedata/schemes/eh_tmc/concepts/100283">
				<skos:inScheme rdf:resource="http://purl.org/heritagedata/schemes/eh_tmc" />
				<dcterms:identifier>http://purl.org/heritagedata/schemes/eh_tmc/concepts/100283</dcterms:identifier>
				<skos:prefLabel xml:lang="en">BOMB VESSEL</skos:prefLabel>
				<dcterms:issued rdf:datatype="http://www.w3.org/2001/XMLSchema#dateTime">2013-07-17T09:01:43</dcterms:issued>
				<skos:broader rdf:resource="http://purl.org/heritagedata/schemes/eh_tmc/concepts/100359" />
				<skos:scopeNote xml:lang="en">A sailing warship armed with one or more heavy howitzers or mortars and used for bombarding shore positions. The modern equivalent is the MONITOR.</skos:scopeNote>
				<cc:license rdf:resource="http://creativecommons.org/licenses/by/3.0" />
				<cc:attributionURL rdf:resource="http://www.english-heritage.org.uk" />
				<cc:attributionName xml:lang="en">English Heritage</cc:attributionName>
				<dcterms:publisher rdf:resource="http://www.english-heritage.org.uk" />
			</skos:Concept>
		</skos:narrower>
		<skos:narrower>
			<skos:Concept rdf:about="http://purl.org/heritagedata/schemes/eh_tmc/concepts/100358">
				<skos:inScheme rdf:resource="http://purl.org/heritagedata/schemes/eh_tmc" />
				<dcterms:identifier>http://purl.org/heritagedata/schemes/eh_tmc/concepts/100358</dcterms:identifier>
				<skos:prefLabel xml:lang="en">GUN BRIG</skos:prefLabel>
				<dcterms:issued rdf:datatype="http://www.w3.org/2001/XMLSchema#dateTime">2013-07-17T09:01:43</dcterms:issued>
				<skos:broader rdf:resource="http://purl.org/heritagedata/schemes/eh_tmc/concepts/100359" />
				<skos:scopeNote xml:lang="en">A small sailing vessel armed with guns.</skos:scopeNote>
				<cc:license rdf:resource="http://creativecommons.org/licenses/by/3.0" />
				<cc:attributionURL rdf:resource="http://www.english-heritage.org.uk" />
				<cc:attributionName xml:lang="en">English Heritage</cc:attributionName>
				<dcterms:publisher rdf:resource="http://www.english-heritage.org.uk" />
			</skos:Concept>
		</skos:narrower>
		<skos:broader rdf:resource="http://purl.org/heritagedata/schemes/eh_tmc/concepts/100490" />
		<skos:narrower>
			<skos:Concept rdf:about="http://purl.org/heritagedata/schemes/eh_tmc/concepts/100404">
				<skos:inScheme rdf:resource="http://purl.org/heritagedata/schemes/eh_tmc" />
				<dcterms:identifier>http://purl.org/heritagedata/schemes/eh_tmc/concepts/100404</dcterms:identifier>
				<skos:prefLabel xml:lang="en">MOTOR GUNBOAT</skos:prefLabel>
				<dcterms:issued rdf:datatype="http://www.w3.org/2001/XMLSchema#dateTime">2013-07-17T09:01:43</dcterms:issued>
				<skos:broader rdf:resource="http://purl.org/heritagedata/schemes/eh_tmc/concepts/100359" />
				<skos:scopeNote xml:lang="en">A small fast warship powered by diesel or petrol engines. Built during World War II for coastal patrol work and anti shipping missions close in shore</skos:scopeNote>
				<cc:license rdf:resource="http://creativecommons.org/licenses/by/3.0" />
				<cc:attributionURL rdf:resource="http://www.english-heritage.org.uk" />
				<cc:attributionName xml:lang="en">English Heritage</cc:attributionName>
				<dcterms:publisher rdf:resource="http://www.english-heritage.org.uk" />
			</skos:Concept>
		</skos:narrower>
		<skos:narrower>
			<skos:Concept rdf:about="http://purl.org/heritagedata/schemes/eh_tmc/concepts/100441">
				<skos:inScheme rdf:resource="http://purl.org/heritagedata/schemes/eh_tmc" />
				<dcterms:identifier>http://purl.org/heritagedata/schemes/eh_tmc/concepts/100441</dcterms:identifier>
				<skos:prefLabel xml:lang="en">RIVER GUNBOAT</skos:prefLabel>
				<dcterms:issued rdf:datatype="http://www.w3.org/2001/XMLSchema#dateTime">2013-07-17T09:01:43</dcterms:issued>
				<skos:broader rdf:resource="http://purl.org/heritagedata/schemes/eh_tmc/concepts/100359" />
				<skos:scopeNote xml:lang="en">A small warship with a shallow draught. Used for patrol duties and shore bombardment on major rivers.</skos:scopeNote>
				<cc:license rdf:resource="http://creativecommons.org/licenses/by/3.0" />
				<cc:attributionURL rdf:resource="http://www.english-heritage.org.uk" />
				<cc:attributionName xml:lang="en">English Heritage</cc:attributionName>
				<dcterms:publisher rdf:resource="http://www.english-heritage.org.uk" />
			</skos:Concept>
		</skos:narrower>
		<skos:narrower>
			<skos:Concept rdf:about="http://purl.org/heritagedata/schemes/eh_tmc/concepts/142055">
				<skos:inScheme rdf:resource="http://purl.org/heritagedata/schemes/eh_tmc" />
				<dcterms:identifier>http://purl.org/heritagedata/schemes/eh_tmc/concepts/142055</dcterms:identifier>
				<skos:prefLabel xml:lang="en">TORPEDO GUNBOAT</skos:prefLabel>
				<dcterms:issued rdf:datatype="http://www.w3.org/2001/XMLSchema#dateTime">2013-07-17T09:01:43</dcterms:issued>
				<skos:broader rdf:resource="http://purl.org/heritagedata/schemes/eh_tmc/concepts/100359" />
				<skos:scopeNote xml:lang="en">Late nineteenth and early twentieth century warship armed with guns and torpedoes.</skos:scopeNote>
				<cc:license rdf:resource="http://creativecommons.org/licenses/by/3.0" />
				<cc:attributionURL rdf:resource="http://www.english-heritage.org.uk" />
				<cc:attributionName xml:lang="en">English Heritage</cc:attributionName>
				<dcterms:publisher rdf:resource="http://www.english-heritage.org.uk" />
			</skos:Concept>
		</skos:narrower>
		<skos:scopeNote xml:lang="en">A small warship built to operate close to the shore or in river estuaries. Used for shore bombardment and patrol duties.</skos:scopeNote>
		<cc:license rdf:resource="http://creativecommons.org/licenses/by/3.0" />
		<cc:attributionURL rdf:resource="http://www.english-heritage.org.uk" />
		<cc:attributionName xml:lang="en">English Heritage</cc:attributionName>
		<dcterms:publisher rdf:resource="http://www.english-heritage.org.uk" />
	</skos:Concept>
	<skos:Concept rdf:about="http://purl.org/heritagedata/schemes/eh_tmc/concepts/100361">
		<skos:inScheme rdf:resource="http://purl.org/heritagedata/schemes/eh_tmc" />
		<dcterms:identifier>http://purl.org/heritagedata/schemes/eh_tmc/concepts/100361</dcterms:identifier>
		<skos:prefLabel xml:lang="en">HARBOUR SERVICE CRAFT</skos:prefLabel>
		<dcterms:issued rdf:datatype="http://www.w3.org/2001/XMLSchema#dateTime">2013-07-17T09:01:43</dcterms:issued>
		<skos:narrower>
			<skos:Concept rdf:about="http://purl.org/heritagedata/schemes/eh_tmc/concepts/100314">
				<skos:inScheme rdf:resource="http://purl.org/heritagedata/schemes/eh_tmc" />
				<dcterms:identifier>http://purl.org/heritagedata/schemes/eh_tmc/concepts/100314</dcterms:identifier>
				<skos:prefLabel xml:lang="en">DAN LAYER</skos:prefLabel>
				<dcterms:issued rdf:datatype="http://www.w3.org/2001/XMLSchema#dateTime">2013-07-17T09:01:43</dcterms:issued>
				<skos:broader rdf:resource="http://purl.org/heritagedata/schemes/eh_tmc/concepts/100361" />
				<skos:scopeNote xml:lang="en">A vessel used for the laying and removal of buoys and other navigational markers.</skos:scopeNote>
				<cc:license rdf:resource="http://creativecommons.org/licenses/by/3.0" />
				<cc:attributionURL rdf:resource="http://www.english-heritage.org.uk" />
				<cc:attributionName xml:lang="en">English Heritage</cc:attributionName>
				<dcterms:publisher rdf:resource="http://www.english-heritage.org.uk" />
			</skos:Concept>
		</skos:narrower>
		<skos:narrower rdf:resource="http://purl.org/heritagedata/schemes/eh_tmc/concepts/100322" />
		<skos:narrower>
			<skos:Concept rdf:about="http://purl.org/heritagedata/schemes/eh_tmc/concepts/100525">
				<skos:inScheme rdf:resource="http://purl.org/heritagedata/schemes/eh_tmc" />
				<dcterms:identifier>http://purl.org/heritagedata/schemes/eh_tmc/concepts/100525</dcterms:identifier>
				<skos:prefLabel xml:lang="en">GRAIN ELEVATOR</skos:prefLabel>
				<dcterms:issued rdf:datatype="http://www.w3.org/2001/XMLSchema#dateTime">2013-07-17T09:01:43</dcterms:issued>
				<skos:broader rdf:resource="http://purl.org/heritagedata/schemes/eh_tmc/concepts/100361" />
				<skos:scopeNote xml:lang="en">A craft on which is a machine for the loading and unloading of grain to and from a warehouse.</skos:scopeNote>
				<cc:license rdf:resource="http://creativecommons.org/licenses/by/3.0" />
				<cc:attributionURL rdf:resource="http://www.english-heritage.org.uk" />
				<cc:attributionName xml:lang="en">English Heritage</cc:attributionName>
				<dcterms:publisher rdf:resource="http://www.english-heritage.org.uk" />
			</skos:Concept>
		</skos:narrower>
		<skos:broader rdf:resource="http://purl.org/heritagedata/schemes/eh_tmc/concepts/100450" />
		<skos:narrower>
			<skos:Concept rdf:about="http://purl.org/heritagedata/schemes/eh_tmc/concepts/100386">
				<skos:inScheme rdf:resource="http://purl.org/heritagedata/schemes/eh_tmc" />
				<dcterms:identifier>http://purl.org/heritagedata/schemes/eh_tmc/concepts/100386</dcterms:identifier>
				<skos:prefLabel xml:lang="en">LIGHTER</skos:prefLabel>
				<dcterms:issued rdf:datatype="http://www.w3.org/2001/XMLSchema#dateTime">2013-07-17T09:01:43</dcterms:issued>
				<skos:altLabel xml:lang="en">Admiralty Lighter</skos:altLabel>
				<skos:broader rdf:resource="http://purl.org/heritagedata/schemes/eh_tmc/concepts/100361" />
				<skos:scopeNote xml:lang="en">Unpowered flat bottomed vessel, used for carrying cargo from ship to shore or as a working platform.</skos:scopeNote>
				<cc:license rdf:resource="http://creativecommons.org/licenses/by/3.0" />
				<cc:attributionURL rdf:resource="http://www.english-heritage.org.uk" />
				<cc:attributionName xml:lang="en">English Heritage</cc:attributionName>
				<dcterms:publisher rdf:resource="http://www.english-heritage.org.uk" />
			</skos:Concept>
		</skos:narrower>
		<skos:narrower>
			<skos:Concept rdf:about="http://purl.org/heritagedata/schemes/eh_tmc/concepts/100403">
				<skos:inScheme rdf:resource="http://purl.org/heritagedata/schemes/eh_tmc" />
				<dcterms:identifier>http://purl.org/heritagedata/schemes/eh_tmc/concepts/100403</dcterms:identifier>
				<skos:prefLabel xml:lang="en">MOORING VESSEL</skos:prefLabel>
				<dcterms:issued rdf:datatype="http://www.w3.org/2001/XMLSchema#dateTime">2013-07-17T09:01:43</dcterms:issued>
				<skos:altLabel xml:lang="en">Auxiliary Mooring Vessel</skos:altLabel>
				<skos:broader rdf:resource="http://purl.org/heritagedata/schemes/eh_tmc/concepts/100361" />
				<skos:scopeNote xml:lang="en">A vessel used to put down and pick up moorings on the sea bed for large vessels.</skos:scopeNote>
				<cc:license rdf:resource="http://creativecommons.org/licenses/by/3.0" />
				<cc:attributionURL rdf:resource="http://www.english-heritage.org.uk" />
				<cc:attributionName xml:lang="en">English Heritage</cc:attributionName>
				<dcterms:publisher rdf:resource="http://www.english-heritage.org.uk" />
			</skos:Concept>
		</skos:narrower>
		<skos:narrower rdf:resource="http://purl.org/heritagedata/schemes/eh_tmc/concepts/100485" />
		<skos:narrower>
			<skos:Concept rdf:about="http://purl.org/heritagedata/schemes/eh_tmc/concepts/100491">
				<skos:inScheme rdf:resource="http://purl.org/heritagedata/schemes/eh_tmc" />
				<dcterms:identifier>http://purl.org/heritagedata/schemes/eh_tmc/concepts/100491</dcterms:identifier>
				<skos:prefLabel xml:lang="en">WATER CARRIER</skos:prefLabel>
				<dcterms:issued rdf:datatype="http://www.w3.org/2001/XMLSchema#dateTime">2013-07-17T09:01:43</dcterms:issued>
				<skos:broader rdf:resource="http://purl.org/heritagedata/schemes/eh_tmc/concepts/100361" />
				<skos:scopeNote xml:lang="en">A small vessel used to carry fresh water to ships at anchor or in harbour.</skos:scopeNote>
				<cc:license rdf:resource="http://creativecommons.org/licenses/by/3.0" />
				<cc:attributionURL rdf:resource="http://www.english-heritage.org.uk" />
				<cc:attributionName xml:lang="en">English Heritage</cc:attributionName>
				<dcterms:publisher rdf:resource="http://www.english-heritage.org.uk" />
			</skos:Concept>
		</skos:narrower>
		<skos:scopeNote xml:lang="en">Craft used to maintain, supply or assist larger vessels whilst in harbour.</skos:scopeNote>
		<cc:license rdf:resource="http://creativecommons.org/licenses/by/3.0" />
		<cc:attributionURL rdf:resource="http://www.english-heritage.org.uk" />
		<cc:attributionName xml:lang="en">English Heritage</cc:attributionName>
		<dcterms:publisher rdf:resource="http://www.english-heritage.org.uk" />
	</skos:Concept>
	<skos:Concept rdf:about="http://purl.org/heritagedata/schemes/eh_tmc/concepts/100366">
		<skos:inScheme rdf:resource="http://purl.org/heritagedata/schemes/eh_tmc" />
		<dcterms:identifier>http://purl.org/heritagedata/schemes/eh_tmc/concepts/100366</dcterms:identifier>
		<skos:prefLabel xml:lang="en">HOSPITAL SHIP</skos:prefLabel>
		<dcterms:issued rdf:datatype="http://www.w3.org/2001/XMLSchema#dateTime">2013-07-17T09:01:43</dcterms:issued>
		<skos:broader rdf:resource="http://purl.org/heritagedata/schemes/eh_tmc/concepts/100419" />
		<skos:broader rdf:resource="http://purl.org/heritagedata/schemes/eh_tmc/concepts/100410" />
		<skos:related rdf:resource="http://purl.org/heritagedata/schemes/eh_tmc/concepts/141858" />
		<skos:scopeNote xml:lang="en">A ship used for treating patients or moving them between a battle zone and a safe area.</skos:scopeNote>
		<cc:license rdf:resource="http://creativecommons.org/licenses/by/3.0" />
		<cc:attributionURL rdf:resource="http://www.english-heritage.org.uk" />
		<cc:attributionName xml:lang="en">English Heritage</cc:attributionName>
		<dcterms:publisher rdf:resource="http://www.english-heritage.org.uk" />
	</skos:Concept>
	<skos:Concept rdf:about="http://purl.org/heritagedata/schemes/eh_tmc/concepts/100369">
		<skos:inScheme rdf:resource="http://purl.org/heritagedata/schemes/eh_tmc" />
		<dcterms:identifier>http://purl.org/heritagedata/schemes/eh_tmc/concepts/100369</dcterms:identifier>
		<skos:prefLabel xml:lang="en">HULK</skos:prefLabel>
		<dcterms:issued rdf:datatype="http://www.w3.org/2001/XMLSchema#dateTime">2013-07-17T09:01:43</dcterms:issued>
		<skos:narrower>
			<skos:Concept rdf:about="http://purl.org/heritagedata/schemes/eh_tmc/concepts/100300">
				<skos:inScheme rdf:resource="http://purl.org/heritagedata/schemes/eh_tmc" />
				<dcterms:identifier>http://purl.org/heritagedata/schemes/eh_tmc/concepts/100300</dcterms:identifier>
				<skos:prefLabel xml:lang="en">COAL HULK</skos:prefLabel>
				<dcterms:issued rdf:datatype="http://www.w3.org/2001/XMLSchema#dateTime">2013-07-17T09:01:43</dcterms:issued>
				<skos:broader rdf:resource="http://purl.org/heritagedata/schemes/eh_tmc/concepts/100369" />
				<skos:scopeNote xml:lang="en">Old ship converted to a floating coal store.</skos:scopeNote>
				<cc:license rdf:resource="http://creativecommons.org/licenses/by/3.0" />
				<cc:attributionURL rdf:resource="http://www.english-heritage.org.uk" />
				<cc:attributionName xml:lang="en">English Heritage</cc:attributionName>
				<dcterms:publisher rdf:resource="http://www.english-heritage.org.uk" />
			</skos:Concept>
		</skos:narrower>
		<skos:broader rdf:resource="http://purl.org/heritagedata/schemes/eh_tmc/concepts/100394" />
		<skos:narrower>
			<skos:Concept rdf:about="http://purl.org/heritagedata/schemes/eh_tmc/concepts/100431">
				<skos:inScheme rdf:resource="http://purl.org/heritagedata/schemes/eh_tmc" />
				<dcterms:identifier>http://purl.org/heritagedata/schemes/eh_tmc/concepts/100431</dcterms:identifier>
				<skos:prefLabel xml:lang="en">PRISON HULK</skos:prefLabel>
				<dcterms:issued rdf:datatype="http://www.w3.org/2001/XMLSchema#dateTime">2013-07-17T09:01:43</dcterms:issued>
				<skos:broader rdf:resource="http://purl.org/heritagedata/schemes/eh_tmc/concepts/100369" />
				<skos:scopeNote xml:lang="en">Demasted old ship used as a floating prison.</skos:scopeNote>
				<cc:license rdf:resource="http://creativecommons.org/licenses/by/3.0" />
				<cc:attributionURL rdf:resource="http://www.english-heritage.org.uk" />
				<cc:attributionName xml:lang="en">English Heritage</cc:attributionName>
				<dcterms:publisher rdf:resource="http://www.english-heritage.org.uk" />
			</skos:Concept>
		</skos:narrower>
		<skos:narrower>
			<skos:Concept rdf:about="http://purl.org/heritagedata/schemes/eh_tmc/concepts/100453">
				<skos:inScheme rdf:resource="http://purl.org/heritagedata/schemes/eh_tmc" />
				<dcterms:identifier>http://purl.org/heritagedata/schemes/eh_tmc/concepts/100453</dcterms:identifier>
				<skos:prefLabel xml:lang="en">SHEER HULK</skos:prefLabel>
				<dcterms:issued rdf:datatype="http://www.w3.org/2001/XMLSchema#dateTime">2013-07-17T09:01:43</dcterms:issued>
				<skos:broader rdf:resource="http://purl.org/heritagedata/schemes/eh_tmc/concepts/100369" />
				<skos:scopeNote xml:lang="en">Old ship with a hull stripped to the water line and used as a platform for mounting the sheers used to lift masts into and out of sailing ships.</skos:scopeNote>
				<cc:license rdf:resource="http://creativecommons.org/licenses/by/3.0" />
				<cc:attributionURL rdf:resource="http://www.english-heritage.org.uk" />
				<cc:attributionName xml:lang="en">English Heritage</cc:attributionName>
				<dcterms:publisher rdf:resource="http://www.english-heritage.org.uk" />
			</skos:Concept>
		</skos:narrower>
		<skos:narrower rdf:resource="http://purl.org/heritagedata/schemes/eh_tmc/concepts/100462" />
		<skos:scopeNote xml:lang="en">An old ship converted for a variety of uses for which it is not required to move under its own power.</skos:scopeNote>
		<cc:license rdf:resource="http://creativecommons.org/licenses/by/3.0" />
		<cc:attributionURL rdf:resource="http://www.english-heritage.org.uk" />
		<cc:attributionName xml:lang="en">English Heritage</cc:attributionName>
		<dcterms:publisher rdf:resource="http://www.english-heritage.org.uk" />
	</skos:Concept>
	<skos:Concept rdf:about="http://purl.org/heritagedata/schemes/eh_tmc/concepts/100372">
		<skos:inScheme rdf:resource="http://purl.org/heritagedata/schemes/eh_tmc" />
		<dcterms:identifier>http://purl.org/heritagedata/schemes/eh_tmc/concepts/100372</dcterms:identifier>
		<skos:prefLabel xml:lang="en">IRONCLAD</skos:prefLabel>
		<dcterms:issued rdf:datatype="http://www.w3.org/2001/XMLSchema#dateTime">2013-07-17T09:01:43</dcterms:issued>
		<skos:broader rdf:resource="http://purl.org/heritagedata/schemes/eh_tmc/concepts/100490" />
		<skos:narrower>
			<skos:Concept rdf:about="http://purl.org/heritagedata/schemes/eh_tmc/concepts/100486">
				<skos:inScheme rdf:resource="http://purl.org/heritagedata/schemes/eh_tmc" />
				<dcterms:identifier>http://purl.org/heritagedata/schemes/eh_tmc/concepts/100486</dcterms:identifier>
				<skos:prefLabel xml:lang="en">TURRET IRONCLAD</skos:prefLabel>
				<dcterms:issued rdf:datatype="http://www.w3.org/2001/XMLSchema#dateTime">2013-07-17T09:01:43</dcterms:issued>
				<skos:broader rdf:resource="http://purl.org/heritagedata/schemes/eh_tmc/concepts/100372" />
				<skos:scopeNote xml:lang="en">A warship constructed of iron plate with its main armament mounted in a revolving turret on deck.</skos:scopeNote>
				<cc:license rdf:resource="http://creativecommons.org/licenses/by/3.0" />
				<cc:attributionURL rdf:resource="http://www.english-heritage.org.uk" />
				<cc:attributionName xml:lang="en">English Heritage</cc:attributionName>
				<dcterms:publisher rdf:resource="http://www.english-heritage.org.uk" />
			</skos:Concept>
		</skos:narrower>
		<skos:scopeNote xml:lang="en">Warships constructed of iron plate or with wooden hulls covered by iron plates. Used as a generic name for the first examples of armour plated warships.</skos:scopeNote>
		<cc:license rdf:resource="http://creativecommons.org/licenses/by/3.0" />
		<cc:attributionURL rdf:resource="http://www.english-heritage.org.uk" />
		<cc:attributionName xml:lang="en">English Heritage</cc:attributionName>
		<dcterms:publisher rdf:resource="http://www.english-heritage.org.uk" />
	</skos:Concept>
	<skos:Concept rdf:about="http://purl.org/heritagedata/schemes/eh_tmc/concepts/100375">
		<skos:inScheme rdf:resource="http://purl.org/heritagedata/schemes/eh_tmc" />
		<dcterms:identifier>http://purl.org/heritagedata/schemes/eh_tmc/concepts/100375</dcterms:identifier>
		<skos:prefLabel xml:lang="en">KETCH</skos:prefLabel>
		<dcterms:issued rdf:datatype="http://www.w3.org/2001/XMLSchema#dateTime">2013-07-17T09:01:43</dcterms:issued>
		<skos:narrower>
			<skos:Concept rdf:about="http://purl.org/heritagedata/schemes/eh_tmc/concepts/100320">
				<skos:inScheme rdf:resource="http://purl.org/heritagedata/schemes/eh_tmc" />
				<dcterms:identifier>http://purl.org/heritagedata/schemes/eh_tmc/concepts/100320</dcterms:identifier>
				<skos:prefLabel xml:lang="en">DOGGER</skos:prefLabel>
				<dcterms:issued rdf:datatype="http://www.w3.org/2001/XMLSchema#dateTime">2013-07-17T09:01:43</dcterms:issued>
				<skos:broader rdf:resource="http://purl.org/heritagedata/schemes/eh_tmc/concepts/100375" />
				<skos:scopeNote xml:lang="en">A short wide-beamed Dutch craft, often used as a fishing vessel or, in the 17th and 18th centuries, a privateer due to its manoeuvrability. Fitted with a ketch rig or variations thereof. Used extensively in the North Sea.</skos:scopeNote>
				<cc:license rdf:resource="http://creativecommons.org/licenses/by/3.0" />
				<cc:attributionURL rdf:resource="http://www.english-heritage.org.uk" />
				<cc:attributionName xml:lang="en">English Heritage</cc:attributionName>
				<dcterms:publisher rdf:resource="http://www.english-heritage.org.uk" />
			</skos:Concept>
		</skos:narrower>
		<skos:broader rdf:resource="http://purl.org/heritagedata/schemes/eh_tmc/concepts/100443" />
		<skos:scopeNote xml:lang="en">A vessel with two masts, rigged as a ketch, used for coastal trading.</skos:scopeNote>
		<cc:license rdf:resource="http://creativecommons.org/licenses/by/3.0" />
		<cc:attributionURL rdf:resource="http://www.english-heritage.org.uk" />
		<cc:attributionName xml:lang="en">English Heritage</cc:attributionName>
		<dcterms:publisher rdf:resource="http://www.english-heritage.org.uk" />
	</skos:Concept>
	<skos:Concept rdf:about="http://purl.org/heritagedata/schemes/eh_tmc/concepts/100377">
		<skos:inScheme rdf:resource="http://purl.org/heritagedata/schemes/eh_tmc" />
		<dcterms:identifier>http://purl.org/heritagedata/schemes/eh_tmc/concepts/100377</dcterms:identifier>
		<skos:prefLabel xml:lang="en">LANDING CRAFT</skos:prefLabel>
		<dcterms:issued rdf:datatype="http://www.w3.org/2001/XMLSchema#dateTime">2013-07-17T09:01:43</dcterms:issued>
		<skos:broader rdf:resource="http://purl.org/heritagedata/schemes/eh_tmc/concepts/100490" />
		<skos:narrower>
			<skos:Concept rdf:about="http://purl.org/heritagedata/schemes/eh_tmc/concepts/100378">
				<skos:inScheme rdf:resource="http://purl.org/heritagedata/schemes/eh_tmc" />
				<dcterms:identifier>http://purl.org/heritagedata/schemes/eh_tmc/concepts/100378</dcterms:identifier>
				<skos:prefLabel xml:lang="en">LANDING CRAFT INFANTRY</skos:prefLabel>
				<dcterms:issued rdf:datatype="http://www.w3.org/2001/XMLSchema#dateTime">2013-07-17T09:01:43</dcterms:issued>
				<skos:broader rdf:resource="http://purl.org/heritagedata/schemes/eh_tmc/concepts/100377" />
				<skos:scopeNote xml:lang="en">Small landing craft often armoured, designed to carry infantrymen and their equipment ashore from larger vessels offshore.</skos:scopeNote>
				<cc:license rdf:resource="http://creativecommons.org/licenses/by/3.0" />
				<cc:attributionURL rdf:resource="http://www.english-heritage.org.uk" />
				<cc:attributionName xml:lang="en">English Heritage</cc:attributionName>
				<dcterms:publisher rdf:resource="http://www.english-heritage.org.uk" />
			</skos:Concept>
		</skos:narrower>
		<skos:narrower>
			<skos:Concept rdf:about="http://purl.org/heritagedata/schemes/eh_tmc/concepts/159170">
				<skos:inScheme rdf:resource="http://purl.org/heritagedata/schemes/eh_tmc" />
				<dcterms:identifier>http://purl.org/heritagedata/schemes/eh_tmc/concepts/159170</dcterms:identifier>
				<skos:prefLabel xml:lang="en">LANDING CRAFT MECHANISED</skos:prefLabel>
				<dcterms:issued rdf:datatype="http://www.w3.org/2001/XMLSchema#dateTime">2013-07-17T09:01:43</dcterms:issued>
				<skos:broader rdf:resource="http://purl.org/heritagedata/schemes/eh_tmc/concepts/100377" />
				<skos:scopeNote xml:lang="en">Landing craft designed for carrying military vehicles and used for beach landings and as a ferry.</skos:scopeNote>
				<cc:license rdf:resource="http://creativecommons.org/licenses/by/3.0" />
				<cc:attributionURL rdf:resource="http://www.english-heritage.org.uk" />
				<cc:attributionName xml:lang="en">English Heritage</cc:attributionName>
				<dcterms:publisher rdf:resource="http://www.english-heritage.org.uk" />
			</skos:Concept>
		</skos:narrower>
		<skos:narrower>
			<skos:Concept rdf:about="http://purl.org/heritagedata/schemes/eh_tmc/concepts/100379">
				<skos:inScheme rdf:resource="http://purl.org/heritagedata/schemes/eh_tmc" />
				<dcterms:identifier>http://purl.org/heritagedata/schemes/eh_tmc/concepts/100379</dcterms:identifier>
				<skos:prefLabel xml:lang="en">LANDING CRAFT TANK</skos:prefLabel>
				<dcterms:issued rdf:datatype="http://www.w3.org/2001/XMLSchema#dateTime">2013-07-17T09:01:43</dcterms:issued>
				<skos:altLabel xml:lang="en">Lct Mk 40</skos:altLabel>
				<skos:broader rdf:resource="http://purl.org/heritagedata/schemes/eh_tmc/concepts/100377" />
				<skos:scopeNote xml:lang="en">Large inshore craft with a retractable loading ramp in the bow. Used to carry tanks ashore for a beach landing or as a tank ferry.</skos:scopeNote>
				<cc:license rdf:resource="http://creativecommons.org/licenses/by/3.0" />
				<cc:attributionURL rdf:resource="http://www.english-heritage.org.uk" />
				<cc:attributionName xml:lang="en">English Heritage</cc:attributionName>
				<dcterms:publisher rdf:resource="http://www.english-heritage.org.uk" />
			</skos:Concept>
		</skos:narrower>
		<skos:scopeNote xml:lang="en">Inshore craft used for carrying troops and military equipment used either for beach landings or as a ferry. Use specific type where known.</skos:scopeNote>
		<cc:license rdf:resource="http://creativecommons.org/licenses/by/3.0" />
		<cc:attributionURL rdf:resource="http://www.english-heritage.org.uk" />
		<cc:attributionName xml:lang="en">English Heritage</cc:attributionName>
		<dcterms:publisher rdf:resource="http://www.english-heritage.org.uk" />
	</skos:Concept>
	<skos:Concept rdf:about="http://purl.org/heritagedata/schemes/eh_tmc/concepts/100382">
		<skos:inScheme rdf:resource="http://purl.org/heritagedata/schemes/eh_tmc" />
		<dcterms:identifier>http://purl.org/heritagedata/schemes/eh_tmc/concepts/100382</dcterms:identifier>
		<skos:prefLabel xml:lang="en">LEISURE CRAFT</skos:prefLabel>
		<dcterms:issued rdf:datatype="http://www.w3.org/2001/XMLSchema#dateTime">2013-07-17T09:01:43</dcterms:issued>
		<skos:narrower rdf:resource="http://purl.org/heritagedata/schemes/eh_tmc/concepts/100290" />
		<skos:narrower rdf:resource="http://purl.org/heritagedata/schemes/eh_tmc/concepts/160144" />
		<skos:broader rdf:resource="http://purl.org/heritagedata/schemes/eh_tmc/concepts/100394" />
		<skos:narrower>
			<skos:Concept rdf:about="http://purl.org/heritagedata/schemes/eh_tmc/concepts/100435">
				<skos:inScheme rdf:resource="http://purl.org/heritagedata/schemes/eh_tmc" />
				<dcterms:identifier>http://purl.org/heritagedata/schemes/eh_tmc/concepts/100435</dcterms:identifier>
				<skos:prefLabel xml:lang="en">RACING CRAFT</skos:prefLabel>
				<dcterms:issued rdf:datatype="http://www.w3.org/2001/XMLSchema#dateTime">2013-07-17T09:01:43</dcterms:issued>
				<skos:broader rdf:resource="http://purl.org/heritagedata/schemes/eh_tmc/concepts/100382" />
				<skos:scopeNote xml:lang="en">Any vessel designed for speed or endurance racing.</skos:scopeNote>
				<cc:license rdf:resource="http://creativecommons.org/licenses/by/3.0" />
				<cc:attributionURL rdf:resource="http://www.english-heritage.org.uk" />
				<cc:attributionName xml:lang="en">English Heritage</cc:attributionName>
				<dcterms:publisher rdf:resource="http://www.english-heritage.org.uk" />
			</skos:Concept>
		</skos:narrower>
		<skos:narrower rdf:resource="http://purl.org/heritagedata/schemes/eh_tmc/concepts/100499" />
		<skos:scopeNote xml:lang="en">Craft intended for recreation and not intended for any commercial use.</skos:scopeNote>
		<cc:license rdf:resource="http://creativecommons.org/licenses/by/3.0" />
		<cc:attributionURL rdf:resource="http://www.english-heritage.org.uk" />
		<cc:attributionName xml:lang="en">English Heritage</cc:attributionName>
		<dcterms:publisher rdf:resource="http://www.english-heritage.org.uk" />
	</skos:Concept>
	<skos:Concept rdf:about="http://purl.org/heritagedata/schemes/eh_tmc/concepts/100383">
		<skos:inScheme rdf:resource="http://purl.org/heritagedata/schemes/eh_tmc" />
		<dcterms:identifier>http://purl.org/heritagedata/schemes/eh_tmc/concepts/100383</dcterms:identifier>
		<skos:prefLabel xml:lang="en">LIBERTY SHIP</skos:prefLabel>
		<dcterms:issued rdf:datatype="http://www.w3.org/2001/XMLSchema#dateTime">2013-07-17T09:01:43</dcterms:issued>
		<skos:broader rdf:resource="http://purl.org/heritagedata/schemes/eh_tmc/concepts/100295" />
		<skos:related rdf:resource="http://purl.org/heritagedata/schemes/eh_tmc/concepts/152307" />
		<skos:scopeNote xml:lang="en">A cargo vessel constructed in the U.S.A. during World War II from prefabricated sections by welding.</skos:scopeNote>
		<cc:license rdf:resource="http://creativecommons.org/licenses/by/3.0" />
		<cc:attributionURL rdf:resource="http://www.english-heritage.org.uk" />
		<cc:attributionName xml:lang="en">English Heritage</cc:attributionName>
		<dcterms:publisher rdf:resource="http://www.english-heritage.org.uk" />
	</skos:Concept>
	<skos:Concept rdf:about="http://purl.org/heritagedata/schemes/eh_tmc/concepts/100392">
		<skos:inScheme rdf:resource="http://purl.org/heritagedata/schemes/eh_tmc" />
		<dcterms:identifier>http://purl.org/heritagedata/schemes/eh_tmc/concepts/100392</dcterms:identifier>
		<skos:prefLabel xml:lang="en">LUGGER</skos:prefLabel>
		<dcterms:issued rdf:datatype="http://www.w3.org/2001/XMLSchema#dateTime">2013-07-17T09:01:43</dcterms:issued>
		<skos:narrower rdf:resource="http://purl.org/heritagedata/schemes/eh_tmc/concepts/140478" />
		<skos:broader rdf:resource="http://purl.org/heritagedata/schemes/eh_tmc/concepts/100443" />
		<skos:scopeNote xml:lang="en">A vessel with a lug sail rig. A lug is a four sided sail set on a lug or yard.</skos:scopeNote>
		<cc:license rdf:resource="http://creativecommons.org/licenses/by/3.0" />
		<cc:attributionURL rdf:resource="http://www.english-heritage.org.uk" />
		<cc:attributionName xml:lang="en">English Heritage</cc:attributionName>
		<dcterms:publisher rdf:resource="http://www.english-heritage.org.uk" />
	</skos:Concept>
	<skos:Concept rdf:about="http://purl.org/heritagedata/schemes/eh_tmc/concepts/100406">
		<skos:inScheme rdf:resource="http://purl.org/heritagedata/schemes/eh_tmc" />
		<dcterms:identifier>http://purl.org/heritagedata/schemes/eh_tmc/concepts/100406</dcterms:identifier>
		<skos:prefLabel xml:lang="en">MOTOR TORPEDO BOAT</skos:prefLabel>
		<dcterms:issued rdf:datatype="http://www.w3.org/2001/XMLSchema#dateTime">2013-07-17T09:01:43</dcterms:issued>
		<skos:narrower>
			<skos:Concept rdf:about="http://purl.org/heritagedata/schemes/eh_tmc/concepts/133093">
				<skos:inScheme rdf:resource="http://purl.org/heritagedata/schemes/eh_tmc" />
				<dcterms:identifier>http://purl.org/heritagedata/schemes/eh_tmc/concepts/133093</dcterms:identifier>
				<skos:prefLabel xml:lang="en">E BOAT</skos:prefLabel>
				<dcterms:issued rdf:datatype="http://www.w3.org/2001/XMLSchema#dateTime">2013-07-17T09:01:43</dcterms:issued>
				<skos:altLabel xml:lang="en">S Boot</skos:altLabel>
				<skos:altLabel xml:lang="en">Schnellboot</skos:altLabel>
				<skos:broader rdf:resource="http://purl.org/heritagedata/schemes/eh_tmc/concepts/100406" />
				<skos:scopeNote xml:lang="en">The name given by the Allies during the Second World War to the German motor torpedo boat. E Boats carried two torpedo tubes and anti aircraft guns. They had a maximum speed of 39 knots and were considered superior to their Allied counterparts.</skos:scopeNote>
				<cc:license rdf:resource="http://creativecommons.org/licenses/by/3.0" />
				<cc:attributionURL rdf:resource="http://www.english-heritage.org.uk" />
				<cc:attributionName xml:lang="en">English Heritage</cc:attributionName>
				<dcterms:publisher rdf:resource="http://www.english-heritage.org.uk" />
			</skos:Concept>
		</skos:narrower>
		<skos:broader rdf:resource="http://purl.org/heritagedata/schemes/eh_tmc/concepts/100490" />
		<skos:scopeNote xml:lang="en">A small warship powered by petrol or diesel engines and armed with torpedo tubes and small guns. Used for coastal anti shipping patrols and warfare in coastal waters.</skos:scopeNote>
		<cc:license rdf:resource="http://creativecommons.org/licenses/by/3.0" />
		<cc:attributionURL rdf:resource="http://www.english-heritage.org.uk" />
		<cc:attributionName xml:lang="en">English Heritage</cc:attributionName>
		<dcterms:publisher rdf:resource="http://www.english-heritage.org.uk" />
	</skos:Concept>
	<skos:Concept rdf:about="http://purl.org/heritagedata/schemes/eh_tmc/concepts/100409">
		<skos:inScheme rdf:resource="http://purl.org/heritagedata/schemes/eh_tmc" />
		<dcterms:identifier>http://purl.org/heritagedata/schemes/eh_tmc/concepts/100409</dcterms:identifier>
		<skos:prefLabel xml:lang="en">MULBERRY HARBOUR</skos:prefLabel>
		<dcterms:issued rdf:datatype="http://www.w3.org/2001/XMLSchema#dateTime">2013-07-17T09:01:43</dcterms:issued>
		<skos:narrower>
			<skos:Concept rdf:about="http://purl.org/heritagedata/schemes/eh_tmc/concepts/131955">
				<skos:inScheme rdf:resource="http://purl.org/heritagedata/schemes/eh_tmc" />
				<dcterms:identifier>http://purl.org/heritagedata/schemes/eh_tmc/concepts/131955</dcterms:identifier>
				<skos:prefLabel xml:lang="en">BOMBARDON</skos:prefLabel>
				<dcterms:issued rdf:datatype="http://www.w3.org/2001/XMLSchema#dateTime">2013-07-17T09:01:43</dcterms:issued>
				<skos:broader rdf:resource="http://purl.org/heritagedata/schemes/eh_tmc/concepts/100409" />
				<skos:scopeNote xml:lang="en">A floating breakwater in the form of a hollow cruciform tube 200 ft long by 25 ft high. Bombardons were designed to reduce the height of waves and formed the outer breakwater of the Mulberry harbours.</skos:scopeNote>
				<cc:license rdf:resource="http://creativecommons.org/licenses/by/3.0" />
				<cc:attributionURL rdf:resource="http://www.english-heritage.org.uk" />
				<cc:attributionName xml:lang="en">English Heritage</cc:attributionName>
				<dcterms:publisher rdf:resource="http://www.english-heritage.org.uk" />
			</skos:Concept>
		</skos:narrower>
		<skos:broader rdf:resource="http://purl.org/heritagedata/schemes/eh_tmc/concepts/100394" />
		<skos:narrower>
			<skos:Concept rdf:about="http://purl.org/heritagedata/schemes/eh_tmc/concepts/131953">
				<skos:inScheme rdf:resource="http://purl.org/heritagedata/schemes/eh_tmc" />
				<dcterms:identifier>http://purl.org/heritagedata/schemes/eh_tmc/concepts/131953</dcterms:identifier>
				<skos:prefLabel xml:lang="en">PHOENIX CAISSON</skos:prefLabel>
				<dcterms:issued rdf:datatype="http://www.w3.org/2001/XMLSchema#dateTime">2013-07-17T09:01:43</dcterms:issued>
				<skos:altLabel xml:lang="en">Phoenix Unit</skos:altLabel>
				<skos:broader rdf:resource="http://purl.org/heritagedata/schemes/eh_tmc/concepts/100409" />
				<skos:scopeNote xml:lang="en">A floatable concrete vessel, numbers of which made up the main breakwater of the Mulberry Harbours used to secure beachheads during the allied invasion of Europe in June 1944.</skos:scopeNote>
				<cc:license rdf:resource="http://creativecommons.org/licenses/by/3.0" />
				<cc:attributionURL rdf:resource="http://www.english-heritage.org.uk" />
				<cc:attributionName xml:lang="en">English Heritage</cc:attributionName>
				<dcterms:publisher rdf:resource="http://www.english-heritage.org.uk" />
			</skos:Concept>
		</skos:narrower>
		<skos:narrower rdf:resource="http://purl.org/heritagedata/schemes/eh_tmc/concepts/100496" />
		<skos:scopeNote xml:lang="en">An artificial harbour, constructed using prefabricated, concrete caissons, floating breakwaters and blockships, which were towed across the channel and assembled off the coast of Normandy to assist the allied forces after the D-Day landings in June 1944.</skos:scopeNote>
		<cc:license rdf:resource="http://creativecommons.org/licenses/by/3.0" />
		<cc:attributionURL rdf:resource="http://www.english-heritage.org.uk" />
		<cc:attributionName xml:lang="en">English Heritage</cc:attributionName>
		<dcterms:publisher rdf:resource="http://www.english-heritage.org.uk" />
	</skos:Concept>
	<skos:Concept rdf:about="http://purl.org/heritagedata/schemes/eh_tmc/concepts/100410">
		<skos:inScheme rdf:resource="http://purl.org/heritagedata/schemes/eh_tmc" />
		<dcterms:identifier>http://purl.org/heritagedata/schemes/eh_tmc/concepts/100410</dcterms:identifier>
		<skos:prefLabel xml:lang="en">NAVAL SUPPORT VESSEL</skos:prefLabel>
		<dcterms:issued rdf:datatype="http://www.w3.org/2001/XMLSchema#dateTime">2013-07-17T09:01:43</dcterms:issued>
		<skos:narrower>
			<skos:Concept rdf:about="http://purl.org/heritagedata/schemes/eh_tmc/concepts/100256">
				<skos:inScheme rdf:resource="http://purl.org/heritagedata/schemes/eh_tmc" />
				<dcterms:identifier>http://purl.org/heritagedata/schemes/eh_tmc/concepts/100256</dcterms:identifier>
				<skos:prefLabel xml:lang="en">ADMIRALTY VESSEL</skos:prefLabel>
				<dcterms:issued rdf:datatype="http://www.w3.org/2001/XMLSchema#dateTime">2013-07-17T09:01:43</dcterms:issued>
				<skos:altLabel xml:lang="en">Admiralty Collier</skos:altLabel>
				<skos:altLabel xml:lang="en">Admiralty Drifter</skos:altLabel>
				<skos:altLabel xml:lang="en">Admiralty Lighter</skos:altLabel>
				<skos:altLabel xml:lang="en">Admiralty Netlayer</skos:altLabel>
				<skos:altLabel xml:lang="en">Admiralty Oiler</skos:altLabel>
				<skos:altLabel xml:lang="en">Admiralty Trawler</skos:altLabel>
				<skos:altLabel xml:lang="en">Admiralty Tug</skos:altLabel>
				<skos:altLabel xml:lang="en">Admiralty Whaler</skos:altLabel>
				<skos:broader rdf:resource="http://purl.org/heritagedata/schemes/eh_tmc/concepts/100410" />
				<skos:scopeNote xml:lang="en">Any vessel which has been hired or impressed for use by the Admiralty.</skos:scopeNote>
				<cc:license rdf:resource="http://creativecommons.org/licenses/by/3.0" />
				<cc:attributionURL rdf:resource="http://www.english-heritage.org.uk" />
				<cc:attributionName xml:lang="en">English Heritage</cc:attributionName>
				<dcterms:publisher rdf:resource="http://www.english-heritage.org.uk" />
			</skos:Concept>
		</skos:narrower>
		<skos:narrower>
			<skos:Concept rdf:about="http://purl.org/heritagedata/schemes/eh_tmc/concepts/100258">
				<skos:inScheme rdf:resource="http://purl.org/heritagedata/schemes/eh_tmc" />
				<dcterms:identifier>http://purl.org/heritagedata/schemes/eh_tmc/concepts/100258</dcterms:identifier>
				<skos:prefLabel xml:lang="en">ADVICE BOAT</skos:prefLabel>
				<dcterms:issued rdf:datatype="http://www.w3.org/2001/XMLSchema#dateTime">2013-07-17T09:01:43</dcterms:issued>
				<skos:broader rdf:resource="http://purl.org/heritagedata/schemes/eh_tmc/concepts/100410" />
				<skos:scopeNote xml:lang="en">A small, fast boat used for carrying orders between sailing vessels.</skos:scopeNote>
				<cc:license rdf:resource="http://creativecommons.org/licenses/by/3.0" />
				<cc:attributionURL rdf:resource="http://www.english-heritage.org.uk" />
				<cc:attributionName xml:lang="en">English Heritage</cc:attributionName>
				<dcterms:publisher rdf:resource="http://www.english-heritage.org.uk" />
			</skos:Concept>
		</skos:narrower>
		<skos:narrower>
			<skos:Concept rdf:about="http://purl.org/heritagedata/schemes/eh_tmc/concepts/100275">
				<skos:inScheme rdf:resource="http://purl.org/heritagedata/schemes/eh_tmc" />
				<dcterms:identifier>http://purl.org/heritagedata/schemes/eh_tmc/concepts/100275</dcterms:identifier>
				<skos:prefLabel xml:lang="en">BARRAGE BALLOON VESSEL</skos:prefLabel>
				<dcterms:issued rdf:datatype="http://www.w3.org/2001/XMLSchema#dateTime">2013-07-17T09:01:43</dcterms:issued>
				<skos:broader rdf:resource="http://purl.org/heritagedata/schemes/eh_tmc/concepts/100410" />
				<skos:scopeNote xml:lang="en">A vessel used as a platform for flying a barrage balloon from.</skos:scopeNote>
				<cc:license rdf:resource="http://creativecommons.org/licenses/by/3.0" />
				<cc:attributionURL rdf:resource="http://www.english-heritage.org.uk" />
				<cc:attributionName xml:lang="en">English Heritage</cc:attributionName>
				<dcterms:publisher rdf:resource="http://www.english-heritage.org.uk" />
			</skos:Concept>
		</skos:narrower>
		<skos:narrower>
			<skos:Concept rdf:about="http://purl.org/heritagedata/schemes/eh_tmc/concepts/100284">
				<skos:inScheme rdf:resource="http://purl.org/heritagedata/schemes/eh_tmc" />
				<dcterms:identifier>http://purl.org/heritagedata/schemes/eh_tmc/concepts/100284</dcterms:identifier>
				<skos:prefLabel xml:lang="en">BOOM DEFENCE VESSEL</skos:prefLabel>
				<dcterms:issued rdf:datatype="http://www.w3.org/2001/XMLSchema#dateTime">2013-07-17T09:01:43</dcterms:issued>
				<skos:broader rdf:resource="http://purl.org/heritagedata/schemes/eh_tmc/concepts/100410" />
				<skos:scopeNote xml:lang="en">A vessel for maintaining the buoys, hawsers and netting of a boom defence.</skos:scopeNote>
				<cc:license rdf:resource="http://creativecommons.org/licenses/by/3.0" />
				<cc:attributionURL rdf:resource="http://www.english-heritage.org.uk" />
				<cc:attributionName xml:lang="en">English Heritage</cc:attributionName>
				<dcterms:publisher rdf:resource="http://www.english-heritage.org.uk" />
			</skos:Concept>
		</skos:narrower>
		<skos:narrower rdf:resource="http://purl.org/heritagedata/schemes/eh_tmc/concepts/100316" />
		<skos:narrower>
			<skos:Concept rdf:about="http://purl.org/heritagedata/schemes/eh_tmc/concepts/100317">
				<skos:inScheme rdf:resource="http://purl.org/heritagedata/schemes/eh_tmc" />
				<dcterms:identifier>http://purl.org/heritagedata/schemes/eh_tmc/concepts/100317</dcterms:identifier>
				<skos:prefLabel xml:lang="en">DEGAUSSING VESSEL</skos:prefLabel>
				<dcterms:issued rdf:datatype="http://www.w3.org/2001/XMLSchema#dateTime">2013-07-17T09:01:43</dcterms:issued>
				<skos:broader rdf:resource="http://purl.org/heritagedata/schemes/eh_tmc/concepts/100410" />
				<skos:scopeNote xml:lang="en">A vessel containing equipment for reducing the magnetic structure of a ship's hull making it immune to magnetic mines.</skos:scopeNote>
				<cc:license rdf:resource="http://creativecommons.org/licenses/by/3.0" />
				<cc:attributionURL rdf:resource="http://www.english-heritage.org.uk" />
				<cc:attributionName xml:lang="en">English Heritage</cc:attributionName>
				<dcterms:publisher rdf:resource="http://www.english-heritage.org.uk" />
			</skos:Concept>
		</skos:narrower>
		<skos:narrower>
			<skos:Concept rdf:about="http://purl.org/heritagedata/schemes/eh_tmc/concepts/100318">
				<skos:inScheme rdf:resource="http://purl.org/heritagedata/schemes/eh_tmc" />
				<dcterms:identifier>http://purl.org/heritagedata/schemes/eh_tmc/concepts/100318</dcterms:identifier>
				<skos:prefLabel xml:lang="en">DEPOT SHIP</skos:prefLabel>
				<dcterms:issued rdf:datatype="http://www.w3.org/2001/XMLSchema#dateTime">2013-07-17T09:01:43</dcterms:issued>
				<skos:broader rdf:resource="http://purl.org/heritagedata/schemes/eh_tmc/concepts/100410" />
				<skos:scopeNote xml:lang="en">A ship acting as a base for smaller vessels and or submarines.</skos:scopeNote>
				<cc:license rdf:resource="http://creativecommons.org/licenses/by/3.0" />
				<cc:attributionURL rdf:resource="http://www.english-heritage.org.uk" />
				<cc:attributionName xml:lang="en">English Heritage</cc:attributionName>
				<dcterms:publisher rdf:resource="http://www.english-heritage.org.uk" />
			</skos:Concept>
		</skos:narrower>
		<skos:narrower>
			<skos:Concept rdf:about="http://purl.org/heritagedata/schemes/eh_tmc/concepts/141981">
				<skos:inScheme rdf:resource="http://purl.org/heritagedata/schemes/eh_tmc" />
				<dcterms:identifier>http://purl.org/heritagedata/schemes/eh_tmc/concepts/141981</dcterms:identifier>
				<skos:prefLabel xml:lang="en">DISTILLING SHIP</skos:prefLabel>
				<dcterms:issued rdf:datatype="http://www.w3.org/2001/XMLSchema#dateTime">2013-07-17T09:01:43</dcterms:issued>
				<skos:broader rdf:resource="http://purl.org/heritagedata/schemes/eh_tmc/concepts/100410" />
				<skos:scopeNote xml:lang="en">World War II naval support vessel usually converted from a mercantile or other warship type and used for the distillation of water by both the Royal Navy and the American Navy.</skos:scopeNote>
				<cc:license rdf:resource="http://creativecommons.org/licenses/by/3.0" />
				<cc:attributionURL rdf:resource="http://www.english-heritage.org.uk" />
				<cc:attributionName xml:lang="en">English Heritage</cc:attributionName>
				<dcterms:publisher rdf:resource="http://www.english-heritage.org.uk" />
			</skos:Concept>
		</skos:narrower>
		<skos:narrower>
			<skos:Concept rdf:about="http://purl.org/heritagedata/schemes/eh_tmc/concepts/100332">
				<skos:inScheme rdf:resource="http://purl.org/heritagedata/schemes/eh_tmc" />
				<dcterms:identifier>http://purl.org/heritagedata/schemes/eh_tmc/concepts/100332</dcterms:identifier>
				<skos:prefLabel xml:lang="en">EXAMINATION SERVICE VESSEL</skos:prefLabel>
				<dcterms:issued rdf:datatype="http://www.w3.org/2001/XMLSchema#dateTime">2013-07-17T09:01:43</dcterms:issued>
				<skos:altLabel xml:lang="en">Examination Vessel</skos:altLabel>
				<skos:broader rdf:resource="http://purl.org/heritagedata/schemes/eh_tmc/concepts/100410" />
				<skos:scopeNote xml:lang="en">A vessel used for inspecting vessels entering port during wartime.</skos:scopeNote>
				<cc:license rdf:resource="http://creativecommons.org/licenses/by/3.0" />
				<cc:attributionURL rdf:resource="http://www.english-heritage.org.uk" />
				<cc:attributionName xml:lang="en">English Heritage</cc:attributionName>
				<dcterms:publisher rdf:resource="http://www.english-heritage.org.uk" />
			</skos:Concept>
		</skos:narrower>
		<skos:narrower>
			<skos:Concept rdf:about="http://purl.org/heritagedata/schemes/eh_tmc/concepts/100341">
				<skos:inScheme rdf:resource="http://purl.org/heritagedata/schemes/eh_tmc" />
				<dcterms:identifier>http://purl.org/heritagedata/schemes/eh_tmc/concepts/100341</dcterms:identifier>
				<skos:prefLabel xml:lang="en">FISHERIES PROTECTION VESSEL</skos:prefLabel>
				<dcterms:issued rdf:datatype="http://www.w3.org/2001/XMLSchema#dateTime">2013-07-17T09:01:43</dcterms:issued>
				<skos:broader rdf:resource="http://purl.org/heritagedata/schemes/eh_tmc/concepts/100410" />
				<skos:scopeNote xml:lang="en">A vessel for policing fishing grounds and fishing vessels.</skos:scopeNote>
				<cc:license rdf:resource="http://creativecommons.org/licenses/by/3.0" />
				<cc:attributionURL rdf:resource="http://www.english-heritage.org.uk" />
				<cc:attributionName xml:lang="en">English Heritage</cc:attributionName>
				<dcterms:publisher rdf:resource="http://www.english-heritage.org.uk" />
			</skos:Concept>
		</skos:narrower>
		<skos:narrower>
			<skos:Concept rdf:about="http://purl.org/heritagedata/schemes/eh_tmc/concepts/100343">
				<skos:inScheme rdf:resource="http://purl.org/heritagedata/schemes/eh_tmc" />
				<dcterms:identifier>http://purl.org/heritagedata/schemes/eh_tmc/concepts/100343</dcterms:identifier>
				<skos:prefLabel xml:lang="en">FLEET MESSENGER</skos:prefLabel>
				<dcterms:issued rdf:datatype="http://www.w3.org/2001/XMLSchema#dateTime">2013-07-17T09:01:43</dcterms:issued>
				<skos:broader rdf:resource="http://purl.org/heritagedata/schemes/eh_tmc/concepts/100410" />
				<skos:scopeNote xml:lang="en">A vessel for carrying messages between warships.</skos:scopeNote>
				<cc:license rdf:resource="http://creativecommons.org/licenses/by/3.0" />
				<cc:attributionURL rdf:resource="http://www.english-heritage.org.uk" />
				<cc:attributionName xml:lang="en">English Heritage</cc:attributionName>
				<dcterms:publisher rdf:resource="http://www.english-heritage.org.uk" />
			</skos:Concept>
		</skos:narrower>
		<skos:narrower rdf:resource="http://purl.org/heritagedata/schemes/eh_tmc/concepts/100366" />
		<skos:narrower>
			<skos:Concept rdf:about="http://purl.org/heritagedata/schemes/eh_tmc/concepts/100397">
				<skos:inScheme rdf:resource="http://purl.org/heritagedata/schemes/eh_tmc" />
				<dcterms:identifier>http://purl.org/heritagedata/schemes/eh_tmc/concepts/100397</dcterms:identifier>
				<skos:prefLabel xml:lang="en">MINE CARRIER</skos:prefLabel>
				<dcterms:issued rdf:datatype="http://www.w3.org/2001/XMLSchema#dateTime">2013-07-17T09:01:43</dcterms:issued>
				<skos:broader rdf:resource="http://purl.org/heritagedata/schemes/eh_tmc/concepts/100410" />
				<skos:scopeNote xml:lang="en">A vessel used for carrying mines between warships and supply depots.</skos:scopeNote>
				<cc:license rdf:resource="http://creativecommons.org/licenses/by/3.0" />
				<cc:attributionURL rdf:resource="http://www.english-heritage.org.uk" />
				<cc:attributionName xml:lang="en">English Heritage</cc:attributionName>
				<dcterms:publisher rdf:resource="http://www.english-heritage.org.uk" />
			</skos:Concept>
		</skos:narrower>
		<skos:broader rdf:resource="http://purl.org/heritagedata/schemes/eh_tmc/concepts/100394" />
		<skos:narrower>
			<skos:Concept rdf:about="http://purl.org/heritagedata/schemes/eh_tmc/concepts/100412">
				<skos:inScheme rdf:resource="http://purl.org/heritagedata/schemes/eh_tmc" />
				<dcterms:identifier>http://purl.org/heritagedata/schemes/eh_tmc/concepts/100412</dcterms:identifier>
				<skos:prefLabel xml:lang="en">OILER</skos:prefLabel>
				<dcterms:issued rdf:datatype="http://www.w3.org/2001/XMLSchema#dateTime">2013-07-17T09:01:43</dcterms:issued>
				<skos:altLabel xml:lang="en">Fueler</skos:altLabel>
				<skos:altLabel xml:lang="en">Admiralty Oiler</skos:altLabel>
				<skos:broader rdf:resource="http://purl.org/heritagedata/schemes/eh_tmc/concepts/100410" />
				<skos:scopeNote xml:lang="en">Generic term for all vessels used to supply warships with any type of fuel.</skos:scopeNote>
				<cc:license rdf:resource="http://creativecommons.org/licenses/by/3.0" />
				<cc:attributionURL rdf:resource="http://www.english-heritage.org.uk" />
				<cc:attributionName xml:lang="en">English Heritage</cc:attributionName>
				<dcterms:publisher rdf:resource="http://www.english-heritage.org.uk" />
			</skos:Concept>
		</skos:narrower>
		<skos:narrower rdf:resource="http://purl.org/heritagedata/schemes/eh_tmc/concepts/100413" />
		<skos:narrower>
			<skos:Concept rdf:about="http://purl.org/heritagedata/schemes/eh_tmc/concepts/100463">
				<skos:inScheme rdf:resource="http://purl.org/heritagedata/schemes/eh_tmc" />
				<dcterms:identifier>http://purl.org/heritagedata/schemes/eh_tmc/concepts/100463</dcterms:identifier>
				<skos:prefLabel xml:lang="en">STORESHIP</skos:prefLabel>
				<dcterms:issued rdf:datatype="http://www.w3.org/2001/XMLSchema#dateTime">2013-07-17T09:01:43</dcterms:issued>
				<skos:broader rdf:resource="http://purl.org/heritagedata/schemes/eh_tmc/concepts/100410" />
				<skos:scopeNote xml:lang="en">A ship in government use, used to carry naval or military stores.</skos:scopeNote>
				<cc:license rdf:resource="http://creativecommons.org/licenses/by/3.0" />
				<cc:attributionURL rdf:resource="http://www.english-heritage.org.uk" />
				<cc:attributionName xml:lang="en">English Heritage</cc:attributionName>
				<dcterms:publisher rdf:resource="http://www.english-heritage.org.uk" />
			</skos:Concept>
		</skos:narrower>
		<skos:narrower>
			<skos:Concept rdf:about="http://purl.org/heritagedata/schemes/eh_tmc/concepts/100473">
				<skos:inScheme rdf:resource="http://purl.org/heritagedata/schemes/eh_tmc" />
				<dcterms:identifier>http://purl.org/heritagedata/schemes/eh_tmc/concepts/100473</dcterms:identifier>
				<skos:prefLabel xml:lang="en">TARGET CRAFT</skos:prefLabel>
				<dcterms:issued rdf:datatype="http://www.w3.org/2001/XMLSchema#dateTime">2013-07-17T09:01:43</dcterms:issued>
				<skos:broader rdf:resource="http://purl.org/heritagedata/schemes/eh_tmc/concepts/100410" />
				<skos:scopeNote xml:lang="en">An obsolete vessel used as a weapons target.</skos:scopeNote>
				<cc:license rdf:resource="http://creativecommons.org/licenses/by/3.0" />
				<cc:attributionURL rdf:resource="http://www.english-heritage.org.uk" />
				<cc:attributionName xml:lang="en">English Heritage</cc:attributionName>
				<dcterms:publisher rdf:resource="http://www.english-heritage.org.uk" />
			</skos:Concept>
		</skos:narrower>
		<skos:narrower rdf:resource="http://purl.org/heritagedata/schemes/eh_tmc/concepts/100474" />
		<skos:narrower>
			<skos:Concept rdf:about="http://purl.org/heritagedata/schemes/eh_tmc/concepts/100478">
				<skos:inScheme rdf:resource="http://purl.org/heritagedata/schemes/eh_tmc" />
				<dcterms:identifier>http://purl.org/heritagedata/schemes/eh_tmc/concepts/100478</dcterms:identifier>
				<skos:prefLabel xml:lang="en">TORPEDO RECOVERY VESSEL</skos:prefLabel>
				<dcterms:issued rdf:datatype="http://www.w3.org/2001/XMLSchema#dateTime">2013-07-17T09:01:43</dcterms:issued>
				<skos:broader rdf:resource="http://purl.org/heritagedata/schemes/eh_tmc/concepts/100410" />
				<skos:scopeNote xml:lang="en">A craft used to retrieve torpedoes after practice firings.</skos:scopeNote>
				<cc:license rdf:resource="http://creativecommons.org/licenses/by/3.0" />
				<cc:attributionURL rdf:resource="http://www.english-heritage.org.uk" />
				<cc:attributionName xml:lang="en">English Heritage</cc:attributionName>
				<dcterms:publisher rdf:resource="http://www.english-heritage.org.uk" />
			</skos:Concept>
		</skos:narrower>
		<skos:narrower rdf:resource="http://purl.org/heritagedata/schemes/eh_tmc/concepts/100483" />
		<skos:narrower>
			<skos:Concept rdf:about="http://purl.org/heritagedata/schemes/eh_tmc/concepts/100489">
				<skos:inScheme rdf:resource="http://purl.org/heritagedata/schemes/eh_tmc" />
				<dcterms:identifier>http://purl.org/heritagedata/schemes/eh_tmc/concepts/100489</dcterms:identifier>
				<skos:prefLabel xml:lang="en">VICTUALLER</skos:prefLabel>
				<dcterms:issued rdf:datatype="http://www.w3.org/2001/XMLSchema#dateTime">2013-07-17T09:01:43</dcterms:issued>
				<skos:broader rdf:resource="http://purl.org/heritagedata/schemes/eh_tmc/concepts/100410" />
				<skos:scopeNote xml:lang="en">A vessel used to carry supplies to warships.</skos:scopeNote>
				<cc:license rdf:resource="http://creativecommons.org/licenses/by/3.0" />
				<cc:attributionURL rdf:resource="http://www.english-heritage.org.uk" />
				<cc:attributionName xml:lang="en">English Heritage</cc:attributionName>
				<dcterms:publisher rdf:resource="http://www.english-heritage.org.uk" />
			</skos:Concept>
		</skos:narrower>
		<skos:scopeNote xml:lang="en">A vessel used to carry essential supplies, such as food and armaments, to naval ships in order to keep them replenished whilst on patrol. Use more specific term.</skos:scopeNote>
		<cc:license rdf:resource="http://creativecommons.org/licenses/by/3.0" />
		<cc:attributionURL rdf:resource="http://www.english-heritage.org.uk" />
		<cc:attributionName xml:lang="en">English Heritage</cc:attributionName>
		<dcterms:publisher rdf:resource="http://www.english-heritage.org.uk" />
	</skos:Concept>
	<skos:Concept rdf:about="http://purl.org/heritagedata/schemes/eh_tmc/concepts/100413">
		<skos:inScheme rdf:resource="http://purl.org/heritagedata/schemes/eh_tmc" />
		<dcterms:identifier>http://purl.org/heritagedata/schemes/eh_tmc/concepts/100413</dcterms:identifier>
		<skos:prefLabel xml:lang="en">ORDNANCE SHIP</skos:prefLabel>
		<dcterms:issued rdf:datatype="http://www.w3.org/2001/XMLSchema#dateTime">2013-07-17T09:01:43</dcterms:issued>
		<skos:broader rdf:resource="http://purl.org/heritagedata/schemes/eh_tmc/concepts/100410" />
		<skos:narrower>
			<skos:Concept rdf:about="http://purl.org/heritagedata/schemes/eh_tmc/concepts/100414">
				<skos:inScheme rdf:resource="http://purl.org/heritagedata/schemes/eh_tmc" />
				<dcterms:identifier>http://purl.org/heritagedata/schemes/eh_tmc/concepts/100414</dcterms:identifier>
				<skos:prefLabel xml:lang="en">ORDNANCE SLOOP</skos:prefLabel>
				<dcterms:issued rdf:datatype="http://www.w3.org/2001/XMLSchema#dateTime">2013-07-17T09:01:43</dcterms:issued>
				<skos:broader rdf:resource="http://purl.org/heritagedata/schemes/eh_tmc/concepts/100413" />
				<skos:scopeNote xml:lang="en">A sloop used for carrying weapons and ammunition to warships.</skos:scopeNote>
				<cc:license rdf:resource="http://creativecommons.org/licenses/by/3.0" />
				<cc:attributionURL rdf:resource="http://www.english-heritage.org.uk" />
				<cc:attributionName xml:lang="en">English Heritage</cc:attributionName>
				<dcterms:publisher rdf:resource="http://www.english-heritage.org.uk" />
			</skos:Concept>
		</skos:narrower>
		<skos:scopeNote xml:lang="en">A vessel used for carrying weapons and ammunition to warships.</skos:scopeNote>
		<cc:license rdf:resource="http://creativecommons.org/licenses/by/3.0" />
		<cc:attributionURL rdf:resource="http://www.english-heritage.org.uk" />
		<cc:attributionName xml:lang="en">English Heritage</cc:attributionName>
		<dcterms:publisher rdf:resource="http://www.english-heritage.org.uk" />
	</skos:Concept>
	<skos:Concept rdf:about="http://purl.org/heritagedata/schemes/eh_tmc/concepts/100416">
		<skos:inScheme rdf:resource="http://purl.org/heritagedata/schemes/eh_tmc" />
		<dcterms:identifier>http://purl.org/heritagedata/schemes/eh_tmc/concepts/100416</dcterms:identifier>
		<skos:prefLabel xml:lang="en">OYSTER DREDGER</skos:prefLabel>
		<dcterms:issued rdf:datatype="http://www.w3.org/2001/XMLSchema#dateTime">2013-07-17T09:01:43</dcterms:issued>
		<skos:broader rdf:resource="http://purl.org/heritagedata/schemes/eh_tmc/concepts/100322" />
		<skos:broader rdf:resource="http://purl.org/heritagedata/schemes/eh_tmc/concepts/100342" />
		<skos:scopeNote xml:lang="en">A fishing vessel which tows a dredger to gather oysters. This is an iron wedge shaped contrivance with a small net attached. Towed behind the vessel the iron wedge loosens the oysters and they fall into the net.</skos:scopeNote>
		<cc:license rdf:resource="http://creativecommons.org/licenses/by/3.0" />
		<cc:attributionURL rdf:resource="http://www.english-heritage.org.uk" />
		<cc:attributionName xml:lang="en">English Heritage</cc:attributionName>
		<dcterms:publisher rdf:resource="http://www.english-heritage.org.uk" />
	</skos:Concept>
	<skos:Concept rdf:about="http://purl.org/heritagedata/schemes/eh_tmc/concepts/100418">
		<skos:inScheme rdf:resource="http://purl.org/heritagedata/schemes/eh_tmc" />
		<dcterms:identifier>http://purl.org/heritagedata/schemes/eh_tmc/concepts/100418</dcterms:identifier>
		<skos:prefLabel xml:lang="en">PADDLE STEAMER</skos:prefLabel>
		<dcterms:issued rdf:datatype="http://www.w3.org/2001/XMLSchema#dateTime">2013-07-17T09:01:43</dcterms:issued>
		<skos:broader rdf:resource="http://purl.org/heritagedata/schemes/eh_tmc/concepts/100394" />
		<skos:related rdf:resource="http://purl.org/heritagedata/schemes/eh_tmc/concepts/159232" />
		<skos:scopeNote xml:lang="en">A steam vessel propelled by a pair of paddle wheels amidships or a single wheel astern, driven by a reciprocating engine.</skos:scopeNote>
		<cc:license rdf:resource="http://creativecommons.org/licenses/by/3.0" />
		<cc:attributionURL rdf:resource="http://www.english-heritage.org.uk" />
		<cc:attributionName xml:lang="en">English Heritage</cc:attributionName>
		<dcterms:publisher rdf:resource="http://www.english-heritage.org.uk" />
	</skos:Concept>
	<skos:Concept rdf:about="http://purl.org/heritagedata/schemes/eh_tmc/concepts/100419">
		<skos:inScheme rdf:resource="http://purl.org/heritagedata/schemes/eh_tmc" />
		<dcterms:identifier>http://purl.org/heritagedata/schemes/eh_tmc/concepts/100419</dcterms:identifier>
		<skos:prefLabel xml:lang="en">PASSENGER VESSEL</skos:prefLabel>
		<dcterms:issued rdf:datatype="http://www.w3.org/2001/XMLSchema#dateTime">2013-07-17T09:01:43</dcterms:issued>
		<skos:narrower>
			<skos:Concept rdf:about="http://purl.org/heritagedata/schemes/eh_tmc/concepts/100309">
				<skos:inScheme rdf:resource="http://purl.org/heritagedata/schemes/eh_tmc" />
				<dcterms:identifier>http://purl.org/heritagedata/schemes/eh_tmc/concepts/100309</dcterms:identifier>
				<skos:prefLabel xml:lang="en">CRUISE BOAT</skos:prefLabel>
				<dcterms:issued rdf:datatype="http://www.w3.org/2001/XMLSchema#dateTime">2013-07-17T09:01:43</dcterms:issued>
				<skos:broader rdf:resource="http://purl.org/heritagedata/schemes/eh_tmc/concepts/100419" />
				<skos:scopeNote xml:lang="en">Open decked vessel used for sight seeing or pleasure voyages.</skos:scopeNote>
				<cc:license rdf:resource="http://creativecommons.org/licenses/by/3.0" />
				<cc:attributionURL rdf:resource="http://www.english-heritage.org.uk" />
				<cc:attributionName xml:lang="en">English Heritage</cc:attributionName>
				<dcterms:publisher rdf:resource="http://www.english-heritage.org.uk" />
			</skos:Concept>
		</skos:narrower>
		<skos:narrower>
			<skos:Concept rdf:about="http://purl.org/heritagedata/schemes/eh_tmc/concepts/100310">
				<skos:inScheme rdf:resource="http://purl.org/heritagedata/schemes/eh_tmc" />
				<dcterms:identifier>http://purl.org/heritagedata/schemes/eh_tmc/concepts/100310</dcterms:identifier>
				<skos:prefLabel xml:lang="en">CRUISE SHIP</skos:prefLabel>
				<dcterms:issued rdf:datatype="http://www.w3.org/2001/XMLSchema#dateTime">2013-07-17T09:01:43</dcterms:issued>
				<skos:broader rdf:resource="http://purl.org/heritagedata/schemes/eh_tmc/concepts/100419" />
				<skos:scopeNote xml:lang="en">A passenger vessel equipped with recreational facilities for long voyages for pleasure and sight seeing.</skos:scopeNote>
				<cc:license rdf:resource="http://creativecommons.org/licenses/by/3.0" />
				<cc:attributionURL rdf:resource="http://www.english-heritage.org.uk" />
				<cc:attributionName xml:lang="en">English Heritage</cc:attributionName>
				<dcterms:publisher rdf:resource="http://www.english-heritage.org.uk" />
			</skos:Concept>
		</skos:narrower>
		<skos:narrower>
			<skos:Concept rdf:about="http://purl.org/heritagedata/schemes/eh_tmc/concepts/100330">
				<skos:inScheme rdf:resource="http://purl.org/heritagedata/schemes/eh_tmc" />
				<dcterms:identifier>http://purl.org/heritagedata/schemes/eh_tmc/concepts/100330</dcterms:identifier>
				<skos:prefLabel xml:lang="en">EMIGRANT SHIP</skos:prefLabel>
				<dcterms:issued rdf:datatype="http://www.w3.org/2001/XMLSchema#dateTime">2013-07-17T09:01:43</dcterms:issued>
				<skos:broader rdf:resource="http://purl.org/heritagedata/schemes/eh_tmc/concepts/100419" />
				<skos:scopeNote xml:lang="en">A passenger vessel equipped to carry a large number of emigrants usually with large third class decks and plenty of cargo space.</skos:scopeNote>
				<cc:license rdf:resource="http://creativecommons.org/licenses/by/3.0" />
				<cc:attributionURL rdf:resource="http://www.english-heritage.org.uk" />
				<cc:attributionName xml:lang="en">English Heritage</cc:attributionName>
				<dcterms:publisher rdf:resource="http://www.english-heritage.org.uk" />
			</skos:Concept>
		</skos:narrower>
		<skos:narrower rdf:resource="http://purl.org/heritagedata/schemes/eh_tmc/concepts/100336" />
		<skos:narrower rdf:resource="http://purl.org/heritagedata/schemes/eh_tmc/concepts/100366" />
		<skos:narrower>
			<skos:Concept rdf:about="http://purl.org/heritagedata/schemes/eh_tmc/concepts/100389">
				<skos:inScheme rdf:resource="http://purl.org/heritagedata/schemes/eh_tmc" />
				<dcterms:identifier>http://purl.org/heritagedata/schemes/eh_tmc/concepts/100389</dcterms:identifier>
				<skos:prefLabel xml:lang="en">LINER</skos:prefLabel>
				<dcterms:issued rdf:datatype="http://www.w3.org/2001/XMLSchema#dateTime">2013-07-17T09:01:43</dcterms:issued>
				<skos:broader rdf:resource="http://purl.org/heritagedata/schemes/eh_tmc/concepts/100419" />
				<skos:scopeNote xml:lang="en">A ship belonging to a shipping company which carries passengers on a scheduled route usually applied to steam ships only.</skos:scopeNote>
				<cc:license rdf:resource="http://creativecommons.org/licenses/by/3.0" />
				<cc:attributionURL rdf:resource="http://www.english-heritage.org.uk" />
				<cc:attributionName xml:lang="en">English Heritage</cc:attributionName>
				<dcterms:publisher rdf:resource="http://www.english-heritage.org.uk" />
			</skos:Concept>
		</skos:narrower>
		<skos:broader rdf:resource="http://purl.org/heritagedata/schemes/eh_tmc/concepts/100295" />
		<skos:narrower rdf:resource="http://purl.org/heritagedata/schemes/eh_tmc/concepts/100483" />
		<skos:narrower>
			<skos:Concept rdf:about="http://purl.org/heritagedata/schemes/eh_tmc/concepts/100492">
				<skos:inScheme rdf:resource="http://purl.org/heritagedata/schemes/eh_tmc" />
				<dcterms:identifier>http://purl.org/heritagedata/schemes/eh_tmc/concepts/100492</dcterms:identifier>
				<skos:prefLabel xml:lang="en">WATER TAXI</skos:prefLabel>
				<dcterms:issued rdf:datatype="http://www.w3.org/2001/XMLSchema#dateTime">2013-07-17T09:01:43</dcterms:issued>
				<skos:broader rdf:resource="http://purl.org/heritagedata/schemes/eh_tmc/concepts/100419" />
				<skos:scopeNote xml:lang="en">A craft available for public hire for short journeys.</skos:scopeNote>
				<cc:license rdf:resource="http://creativecommons.org/licenses/by/3.0" />
				<cc:attributionURL rdf:resource="http://www.english-heritage.org.uk" />
				<cc:attributionName xml:lang="en">English Heritage</cc:attributionName>
				<dcterms:publisher rdf:resource="http://www.english-heritage.org.uk" />
			</skos:Concept>
		</skos:narrower>
		<skos:scopeNote xml:lang="en">A vessel designed principally for the carriage of fare paying passengers.</skos:scopeNote>
		<cc:license rdf:resource="http://creativecommons.org/licenses/by/3.0" />
		<cc:attributionURL rdf:resource="http://www.english-heritage.org.uk" />
		<cc:attributionName xml:lang="en">English Heritage</cc:attributionName>
		<dcterms:publisher rdf:resource="http://www.english-heritage.org.uk" />
	</skos:Concept>
	<skos:Concept rdf:about="http://purl.org/heritagedata/schemes/eh_tmc/concepts/100421">
		<skos:inScheme rdf:resource="http://purl.org/heritagedata/schemes/eh_tmc" />
		<dcterms:identifier>http://purl.org/heritagedata/schemes/eh_tmc/concepts/100421</dcterms:identifier>
		<skos:prefLabel xml:lang="en">PATROL SUBMARINE</skos:prefLabel>
		<dcterms:issued rdf:datatype="http://www.w3.org/2001/XMLSchema#dateTime">2013-07-17T09:01:43</dcterms:issued>
		<skos:altLabel xml:lang="en">E Class Submarine</skos:altLabel>
		<skos:altLabel xml:lang="en">H21 Class Submarine</skos:altLabel>
		<skos:altLabel xml:lang="en">L Class Submarine</skos:altLabel>
		<skos:altLabel xml:lang="en">Swordfish Class Submarine</skos:altLabel>
		<skos:altLabel xml:lang="en">U Class Submarine</skos:altLabel>
		<skos:broader rdf:resource="http://purl.org/heritagedata/schemes/eh_tmc/concepts/139837" />
		<skos:broader rdf:resource="http://purl.org/heritagedata/schemes/eh_tmc/concepts/100465" />
		<skos:scopeNote xml:lang="en">Diesel engined submarine designed for long ocean voyages in search of enemy shipping.</skos:scopeNote>
		<cc:license rdf:resource="http://creativecommons.org/licenses/by/3.0" />
		<cc:attributionURL rdf:resource="http://www.english-heritage.org.uk" />
		<cc:attributionName xml:lang="en">English Heritage</cc:attributionName>
		<dcterms:publisher rdf:resource="http://www.english-heritage.org.uk" />
	</skos:Concept>
	<skos:Concept rdf:about="http://purl.org/heritagedata/schemes/eh_tmc/concepts/100432">
		<skos:inScheme rdf:resource="http://purl.org/heritagedata/schemes/eh_tmc" />
		<dcterms:identifier>http://purl.org/heritagedata/schemes/eh_tmc/concepts/100432</dcterms:identifier>
		<skos:prefLabel xml:lang="en">PRIVATEER</skos:prefLabel>
		<dcterms:issued rdf:datatype="http://www.w3.org/2001/XMLSchema#dateTime">2013-07-17T09:01:43</dcterms:issued>
		<skos:narrower>
			<skos:Concept rdf:about="http://purl.org/heritagedata/schemes/eh_tmc/concepts/159159">
				<skos:inScheme rdf:resource="http://purl.org/heritagedata/schemes/eh_tmc" />
				<dcterms:identifier>http://purl.org/heritagedata/schemes/eh_tmc/concepts/159159</dcterms:identifier>
				<skos:prefLabel xml:lang="en">CAPER</skos:prefLabel>
				<dcterms:issued rdf:datatype="http://www.w3.org/2001/XMLSchema#dateTime">2013-07-17T09:01:43</dcterms:issued>
				<skos:broader rdf:resource="http://purl.org/heritagedata/schemes/eh_tmc/concepts/100432" />
				<skos:scopeNote xml:lang="en">17th/18th century lightly armed privateer, usually either a 'Dunkirker' or Dutch.</skos:scopeNote>
				<cc:license rdf:resource="http://creativecommons.org/licenses/by/3.0" />
				<cc:attributionURL rdf:resource="http://www.english-heritage.org.uk" />
				<cc:attributionName xml:lang="en">English Heritage</cc:attributionName>
				<dcterms:publisher rdf:resource="http://www.english-heritage.org.uk" />
			</skos:Concept>
		</skos:narrower>
		<skos:narrower>
			<skos:Concept rdf:about="http://purl.org/heritagedata/schemes/eh_tmc/concepts/139550">
				<skos:inScheme rdf:resource="http://purl.org/heritagedata/schemes/eh_tmc" />
				<dcterms:identifier>http://purl.org/heritagedata/schemes/eh_tmc/concepts/139550</dcterms:identifier>
				<skos:prefLabel xml:lang="en">CORSAIR</skos:prefLabel>
				<dcterms:issued rdf:datatype="http://www.w3.org/2001/XMLSchema#dateTime">2013-07-17T09:01:43</dcterms:issued>
				<skos:broader rdf:resource="http://purl.org/heritagedata/schemes/eh_tmc/concepts/100432" />
				<skos:scopeNote xml:lang="en">Privateer operating under government licence to act against enemy merchant shipping. The term is closely associated with North African privateers which operated off the Barbary coast prior to the mid-1800's.</skos:scopeNote>
				<cc:license rdf:resource="http://creativecommons.org/licenses/by/3.0" />
				<cc:attributionURL rdf:resource="http://www.english-heritage.org.uk" />
				<cc:attributionName xml:lang="en">English Heritage</cc:attributionName>
				<dcterms:publisher rdf:resource="http://www.english-heritage.org.uk" />
			</skos:Concept>
		</skos:narrower>
		<skos:broader rdf:resource="http://purl.org/heritagedata/schemes/eh_tmc/concepts/100394" />
		<skos:scopeNote xml:lang="en">A private fighting ship under a letter of marque or financed by subscribers, shareholders or individuals.</skos:scopeNote>
		<cc:license rdf:resource="http://creativecommons.org/licenses/by/3.0" />
		<cc:attributionURL rdf:resource="http://www.english-heritage.org.uk" />
		<cc:attributionName xml:lang="en">English Heritage</cc:attributionName>
		<dcterms:publisher rdf:resource="http://www.english-heritage.org.uk" />
	</skos:Concept>
	<skos:Concept rdf:about="http://purl.org/heritagedata/schemes/eh_tmc/concepts/100438">
		<skos:inScheme rdf:resource="http://purl.org/heritagedata/schemes/eh_tmc" />
		<dcterms:identifier>http://purl.org/heritagedata/schemes/eh_tmc/concepts/100438</dcterms:identifier>
		<skos:prefLabel xml:lang="en">RESCUE TUG</skos:prefLabel>
		<dcterms:issued rdf:datatype="http://www.w3.org/2001/XMLSchema#dateTime">2013-07-17T09:01:43</dcterms:issued>
		<skos:broader rdf:resource="http://purl.org/heritagedata/schemes/eh_tmc/concepts/100485" />
		<skos:broader rdf:resource="http://purl.org/heritagedata/schemes/eh_tmc/concepts/100439" />
		<skos:scopeNote xml:lang="en">A rescue tug equipped to care for survivors from torpedoed vessels and also available for towing to port ships damaged by enemy action.</skos:scopeNote>
		<cc:license rdf:resource="http://creativecommons.org/licenses/by/3.0" />
		<cc:attributionURL rdf:resource="http://www.english-heritage.org.uk" />
		<cc:attributionName xml:lang="en">English Heritage</cc:attributionName>
		<dcterms:publisher rdf:resource="http://www.english-heritage.org.uk" />
	</skos:Concept>
	<skos:Concept rdf:about="http://purl.org/heritagedata/schemes/eh_tmc/concepts/100439">
		<skos:inScheme rdf:resource="http://purl.org/heritagedata/schemes/eh_tmc" />
		<dcterms:identifier>http://purl.org/heritagedata/schemes/eh_tmc/concepts/100439</dcterms:identifier>
		<skos:prefLabel xml:lang="en">RESCUE VESSEL</skos:prefLabel>
		<dcterms:issued rdf:datatype="http://www.w3.org/2001/XMLSchema#dateTime">2013-07-17T09:01:43</dcterms:issued>
		<skos:altLabel xml:lang="en">Standby Safety Vessel</skos:altLabel>
		<skos:narrower>
			<skos:Concept rdf:about="http://purl.org/heritagedata/schemes/eh_tmc/concepts/100384">
				<skos:inScheme rdf:resource="http://purl.org/heritagedata/schemes/eh_tmc" />
				<dcterms:identifier>http://purl.org/heritagedata/schemes/eh_tmc/concepts/100384</dcterms:identifier>
				<skos:prefLabel xml:lang="en">LIFEBOAT</skos:prefLabel>
				<dcterms:issued rdf:datatype="http://www.w3.org/2001/XMLSchema#dateTime">2013-07-17T09:01:43</dcterms:issued>
				<skos:broader rdf:resource="http://purl.org/heritagedata/schemes/eh_tmc/concepts/100439" />
				<skos:scopeNote xml:lang="en">A boat specifically designed for saving lives at sea, they can be either: a boat carried on a larger vessel for use in emergency evacuation of crew and passengers in the event of shipwreck or a boat built for the purpose of shore-to-sea rescue missions.</skos:scopeNote>
				<cc:license rdf:resource="http://creativecommons.org/licenses/by/3.0" />
				<cc:attributionURL rdf:resource="http://www.english-heritage.org.uk" />
				<cc:attributionName xml:lang="en">English Heritage</cc:attributionName>
				<dcterms:publisher rdf:resource="http://www.english-heritage.org.uk" />
			</skos:Concept>
		</skos:narrower>
		<skos:narrower rdf:resource="http://purl.org/heritagedata/schemes/eh_tmc/concepts/100438" />
		<skos:broader rdf:resource="http://purl.org/heritagedata/schemes/eh_tmc/concepts/100450" />
		<skos:scopeNote xml:lang="en">A specially equipped ship designed to care for survivors of stricken vessels and offshore drilling platforms. These ships were often converted naval trawlers or minesweepers.</skos:scopeNote>
		<cc:license rdf:resource="http://creativecommons.org/licenses/by/3.0" />
		<cc:attributionURL rdf:resource="http://www.english-heritage.org.uk" />
		<cc:attributionName xml:lang="en">English Heritage</cc:attributionName>
		<dcterms:publisher rdf:resource="http://www.english-heritage.org.uk" />
	</skos:Concept>
	<skos:Concept rdf:about="http://purl.org/heritagedata/schemes/eh_tmc/concepts/100440">
		<skos:inScheme rdf:resource="http://purl.org/heritagedata/schemes/eh_tmc" />
		<dcterms:identifier>http://purl.org/heritagedata/schemes/eh_tmc/concepts/100440</dcterms:identifier>
		<skos:prefLabel xml:lang="en">REVENUE CUTTER</skos:prefLabel>
		<dcterms:issued rdf:datatype="http://www.w3.org/2001/XMLSchema#dateTime">2013-07-17T09:01:43</dcterms:issued>
		<skos:broader rdf:resource="http://purl.org/heritagedata/schemes/eh_tmc/concepts/145104" />
		<skos:broader rdf:resource="http://purl.org/heritagedata/schemes/eh_tmc/concepts/138609" />
		<skos:scopeNote xml:lang="en">A single masted cutter built specifically for the prevention of smuggling and the enforcement of customs regulations.</skos:scopeNote>
		<cc:license rdf:resource="http://creativecommons.org/licenses/by/3.0" />
		<cc:attributionURL rdf:resource="http://www.english-heritage.org.uk" />
		<cc:attributionName xml:lang="en">English Heritage</cc:attributionName>
		<dcterms:publisher rdf:resource="http://www.english-heritage.org.uk" />
	</skos:Concept>
	<skos:Concept rdf:about="http://purl.org/heritagedata/schemes/eh_tmc/concepts/100443">
		<skos:inScheme rdf:resource="http://purl.org/heritagedata/schemes/eh_tmc" />
		<dcterms:identifier>http://purl.org/heritagedata/schemes/eh_tmc/concepts/100443</dcterms:identifier>
		<skos:prefLabel xml:lang="en">SAILING VESSEL &lt;BY FORM/TYPE&gt;</skos:prefLabel>
		<dcterms:issued rdf:datatype="http://www.w3.org/2001/XMLSchema#dateTime">2013-07-17T09:01:43</dcterms:issued>
		<skos:narrower>
			<skos:Concept rdf:about="http://purl.org/heritagedata/schemes/eh_tmc/concepts/100279">
				<skos:inScheme rdf:resource="http://purl.org/heritagedata/schemes/eh_tmc" />
				<dcterms:identifier>http://purl.org/heritagedata/schemes/eh_tmc/concepts/100279</dcterms:identifier>
				<skos:prefLabel xml:lang="en">BAWLEY</skos:prefLabel>
				<dcterms:issued rdf:datatype="http://www.w3.org/2001/XMLSchema#dateTime">2013-07-17T09:01:43</dcterms:issued>
				<skos:broader rdf:resource="http://purl.org/heritagedata/schemes/eh_tmc/concepts/100443" />
				<skos:scopeNote xml:lang="en">A small coastal fishing vessel peculiar to Kent, cutter rigged.</skos:scopeNote>
				<cc:license rdf:resource="http://creativecommons.org/licenses/by/3.0" />
				<cc:attributionURL rdf:resource="http://www.english-heritage.org.uk" />
				<cc:attributionName xml:lang="en">English Heritage</cc:attributionName>
				<dcterms:publisher rdf:resource="http://www.english-heritage.org.uk" />
			</skos:Concept>
		</skos:narrower>
		<skos:narrower>
			<skos:Concept rdf:about="http://purl.org/heritagedata/schemes/eh_tmc/concepts/100280">
				<skos:inScheme rdf:resource="http://purl.org/heritagedata/schemes/eh_tmc" />
				<dcterms:identifier>http://purl.org/heritagedata/schemes/eh_tmc/concepts/100280</dcterms:identifier>
				<skos:prefLabel xml:lang="en">BILLYBOY</skos:prefLabel>
				<dcterms:issued rdf:datatype="http://www.w3.org/2001/XMLSchema#dateTime">2013-07-17T09:01:43</dcterms:issued>
				<skos:broader rdf:resource="http://purl.org/heritagedata/schemes/eh_tmc/concepts/100443" />
				<skos:scopeNote xml:lang="en">Single masted east coast trading vessel, ketch rigged or single masted.</skos:scopeNote>
				<cc:license rdf:resource="http://creativecommons.org/licenses/by/3.0" />
				<cc:attributionURL rdf:resource="http://www.english-heritage.org.uk" />
				<cc:attributionName xml:lang="en">English Heritage</cc:attributionName>
				<dcterms:publisher rdf:resource="http://www.english-heritage.org.uk" />
			</skos:Concept>
		</skos:narrower>
		<skos:narrower>
			<skos:Concept rdf:about="http://purl.org/heritagedata/schemes/eh_tmc/concepts/152510">
				<skos:inScheme rdf:resource="http://purl.org/heritagedata/schemes/eh_tmc" />
				<dcterms:identifier>http://purl.org/heritagedata/schemes/eh_tmc/concepts/152510</dcterms:identifier>
				<skos:prefLabel xml:lang="en">BOEIER</skos:prefLabel>
				<dcterms:issued rdf:datatype="http://www.w3.org/2001/XMLSchema#dateTime">2013-07-17T09:01:43</dcterms:issued>
				<skos:altLabel xml:lang="en">Boier</skos:altLabel>
				<skos:broader rdf:resource="http://purl.org/heritagedata/schemes/eh_tmc/concepts/100443" />
				<skos:scopeNote xml:lang="en">A Dutch barge-like sailing vessel whose shallow draught enables it to navigate in shallow water not accessible by other vessels. Used for fishing or carriage of cargo in the 19th century this type of vessel was adapted for use as a type of leisure craft.</skos:scopeNote>
				<cc:license rdf:resource="http://creativecommons.org/licenses/by/3.0" />
				<cc:attributionURL rdf:resource="http://www.english-heritage.org.uk" />
				<cc:attributionName xml:lang="en">English Heritage</cc:attributionName>
				<dcterms:publisher rdf:resource="http://www.english-heritage.org.uk" />
			</skos:Concept>
		</skos:narrower>
		<skos:narrower>
			<skos:Concept rdf:about="http://purl.org/heritagedata/schemes/eh_tmc/concepts/100294">
				<skos:inScheme rdf:resource="http://purl.org/heritagedata/schemes/eh_tmc" />
				<dcterms:identifier>http://purl.org/heritagedata/schemes/eh_tmc/concepts/100294</dcterms:identifier>
				<skos:prefLabel xml:lang="en">CARAVEL</skos:prefLabel>
				<dcterms:issued rdf:datatype="http://www.w3.org/2001/XMLSchema#dateTime">2013-07-17T09:01:43</dcterms:issued>
				<skos:broader rdf:resource="http://purl.org/heritagedata/schemes/eh_tmc/concepts/100443" />
				<skos:scopeNote xml:lang="en">Small two or three masted ship used as trading vessels in the medieval mediterranean.</skos:scopeNote>
				<cc:license rdf:resource="http://creativecommons.org/licenses/by/3.0" />
				<cc:attributionURL rdf:resource="http://www.english-heritage.org.uk" />
				<cc:attributionName xml:lang="en">English Heritage</cc:attributionName>
				<dcterms:publisher rdf:resource="http://www.english-heritage.org.uk" />
			</skos:Concept>
		</skos:narrower>
		<skos:narrower>
			<skos:Concept rdf:about="http://purl.org/heritagedata/schemes/eh_tmc/concepts/100296">
				<skos:inScheme rdf:resource="http://purl.org/heritagedata/schemes/eh_tmc" />
				<dcterms:identifier>http://purl.org/heritagedata/schemes/eh_tmc/concepts/100296</dcterms:identifier>
				<skos:prefLabel xml:lang="en">CARRACK</skos:prefLabel>
				<dcterms:issued rdf:datatype="http://www.w3.org/2001/XMLSchema#dateTime">2013-07-17T09:01:43</dcterms:issued>
				<skos:broader rdf:resource="http://purl.org/heritagedata/schemes/eh_tmc/concepts/100443" />
				<skos:scopeNote xml:lang="en">A three masted vessel with a square rig on the fore and main masts and lateen rig on the mizzen mast.</skos:scopeNote>
				<cc:license rdf:resource="http://creativecommons.org/licenses/by/3.0" />
				<cc:attributionURL rdf:resource="http://www.english-heritage.org.uk" />
				<cc:attributionName xml:lang="en">English Heritage</cc:attributionName>
				<dcterms:publisher rdf:resource="http://www.english-heritage.org.uk" />
			</skos:Concept>
		</skos:narrower>
		<skos:narrower>
			<skos:Concept rdf:about="http://purl.org/heritagedata/schemes/eh_tmc/concepts/100522">
				<skos:inScheme rdf:resource="http://purl.org/heritagedata/schemes/eh_tmc" />
				<dcterms:identifier>http://purl.org/heritagedata/schemes/eh_tmc/concepts/100522</dcterms:identifier>
				<skos:prefLabel xml:lang="en">CARVEL</skos:prefLabel>
				<dcterms:issued rdf:datatype="http://www.w3.org/2001/XMLSchema#dateTime">2013-07-17T09:01:43</dcterms:issued>
				<skos:broader rdf:resource="http://purl.org/heritagedata/schemes/eh_tmc/concepts/100443" />
				<skos:scopeNote xml:lang="en">A small cargo craft, usually with two masts and a lateen rig.</skos:scopeNote>
				<cc:license rdf:resource="http://creativecommons.org/licenses/by/3.0" />
				<cc:attributionURL rdf:resource="http://www.english-heritage.org.uk" />
				<cc:attributionName xml:lang="en">English Heritage</cc:attributionName>
				<dcterms:publisher rdf:resource="http://www.english-heritage.org.uk" />
			</skos:Concept>
		</skos:narrower>
		<skos:narrower>
			<skos:Concept rdf:about="http://purl.org/heritagedata/schemes/eh_tmc/concepts/111714">
				<skos:inScheme rdf:resource="http://purl.org/heritagedata/schemes/eh_tmc" />
				<dcterms:identifier>http://purl.org/heritagedata/schemes/eh_tmc/concepts/111714</dcterms:identifier>
				<skos:prefLabel xml:lang="en">CHASSE MAREE</skos:prefLabel>
				<dcterms:issued rdf:datatype="http://www.w3.org/2001/XMLSchema#dateTime">2013-07-17T09:01:43</dcterms:issued>
				<skos:altLabel xml:lang="en">Chasse Marie</skos:altLabel>
				<skos:broader rdf:resource="http://purl.org/heritagedata/schemes/eh_tmc/concepts/100443" />
				<skos:scopeNote xml:lang="en">French coasting vessel</skos:scopeNote>
				<cc:license rdf:resource="http://creativecommons.org/licenses/by/3.0" />
				<cc:attributionURL rdf:resource="http://www.english-heritage.org.uk" />
				<cc:attributionName xml:lang="en">English Heritage</cc:attributionName>
				<dcterms:publisher rdf:resource="http://www.english-heritage.org.uk" />
			</skos:Concept>
		</skos:narrower>
		<skos:narrower>
			<skos:Concept rdf:about="http://purl.org/heritagedata/schemes/eh_tmc/concepts/100299">
				<skos:inScheme rdf:resource="http://purl.org/heritagedata/schemes/eh_tmc" />
				<dcterms:identifier>http://purl.org/heritagedata/schemes/eh_tmc/concepts/100299</dcterms:identifier>
				<skos:prefLabel xml:lang="en">CLIPPER</skos:prefLabel>
				<dcterms:issued rdf:datatype="http://www.w3.org/2001/XMLSchema#dateTime">2013-07-17T09:01:43</dcterms:issued>
				<skos:broader rdf:resource="http://purl.org/heritagedata/schemes/eh_tmc/concepts/100443" />
				<skos:scopeNote xml:lang="en">Generic term for fast sailing ships with schooner rig and fine hull lines.</skos:scopeNote>
				<cc:license rdf:resource="http://creativecommons.org/licenses/by/3.0" />
				<cc:attributionURL rdf:resource="http://www.english-heritage.org.uk" />
				<cc:attributionName xml:lang="en">English Heritage</cc:attributionName>
				<dcterms:publisher rdf:resource="http://www.english-heritage.org.uk" />
			</skos:Concept>
		</skos:narrower>
		<skos:narrower>
			<skos:Concept rdf:about="http://purl.org/heritagedata/schemes/eh_tmc/concepts/100302">
				<skos:inScheme rdf:resource="http://purl.org/heritagedata/schemes/eh_tmc" />
				<dcterms:identifier>http://purl.org/heritagedata/schemes/eh_tmc/concepts/100302</dcterms:identifier>
				<skos:prefLabel xml:lang="en">COG</skos:prefLabel>
				<dcterms:issued rdf:datatype="http://www.w3.org/2001/XMLSchema#dateTime">2013-07-17T09:01:43</dcterms:issued>
				<skos:broader rdf:resource="http://purl.org/heritagedata/schemes/eh_tmc/concepts/100443" />
				<skos:scopeNote xml:lang="en">North European medieval merchant vessel.</skos:scopeNote>
				<cc:license rdf:resource="http://creativecommons.org/licenses/by/3.0" />
				<cc:attributionURL rdf:resource="http://www.english-heritage.org.uk" />
				<cc:attributionName xml:lang="en">English Heritage</cc:attributionName>
				<dcterms:publisher rdf:resource="http://www.english-heritage.org.uk" />
			</skos:Concept>
		</skos:narrower>
		<skos:narrower>
			<skos:Concept rdf:about="http://purl.org/heritagedata/schemes/eh_tmc/concepts/100523">
				<skos:inScheme rdf:resource="http://purl.org/heritagedata/schemes/eh_tmc" />
				<dcterms:identifier>http://purl.org/heritagedata/schemes/eh_tmc/concepts/100523</dcterms:identifier>
				<skos:prefLabel xml:lang="en">CRAYER</skos:prefLabel>
				<dcterms:issued rdf:datatype="http://www.w3.org/2001/XMLSchema#dateTime">2013-07-17T09:01:43</dcterms:issued>
				<skos:broader rdf:resource="http://purl.org/heritagedata/schemes/eh_tmc/concepts/100443" />
				<skos:scopeNote xml:lang="en">A small, single-masted merchant vessel, designed for maximum hold capacity and not for sailing ability.</skos:scopeNote>
				<cc:license rdf:resource="http://creativecommons.org/licenses/by/3.0" />
				<cc:attributionURL rdf:resource="http://www.english-heritage.org.uk" />
				<cc:attributionName xml:lang="en">English Heritage</cc:attributionName>
				<dcterms:publisher rdf:resource="http://www.english-heritage.org.uk" />
			</skos:Concept>
		</skos:narrower>
		<skos:narrower>
			<skos:Concept rdf:about="http://purl.org/heritagedata/schemes/eh_tmc/concepts/100519">
				<skos:inScheme rdf:resource="http://purl.org/heritagedata/schemes/eh_tmc" />
				<dcterms:identifier>http://purl.org/heritagedata/schemes/eh_tmc/concepts/100519</dcterms:identifier>
				<skos:prefLabel xml:lang="en">CUTTER</skos:prefLabel>
				<dcterms:issued rdf:datatype="http://www.w3.org/2001/XMLSchema#dateTime">2013-07-17T09:01:43</dcterms:issued>
				<skos:broader rdf:resource="http://purl.org/heritagedata/schemes/eh_tmc/concepts/100443" />
				<skos:scopeNote xml:lang="en">A small one masted craft, often using oars as well as sails.</skos:scopeNote>
				<cc:license rdf:resource="http://creativecommons.org/licenses/by/3.0" />
				<cc:attributionURL rdf:resource="http://www.english-heritage.org.uk" />
				<cc:attributionName xml:lang="en">English Heritage</cc:attributionName>
				<dcterms:publisher rdf:resource="http://www.english-heritage.org.uk" />
			</skos:Concept>
		</skos:narrower>
		<skos:narrower>
			<skos:Concept rdf:about="http://purl.org/heritagedata/schemes/eh_tmc/concepts/100315">
				<skos:inScheme rdf:resource="http://purl.org/heritagedata/schemes/eh_tmc" />
				<dcterms:identifier>http://purl.org/heritagedata/schemes/eh_tmc/concepts/100315</dcterms:identifier>
				<skos:prefLabel xml:lang="en">DANDY</skos:prefLabel>
				<dcterms:issued rdf:datatype="http://www.w3.org/2001/XMLSchema#dateTime">2013-07-17T09:01:43</dcterms:issued>
				<skos:broader rdf:resource="http://purl.org/heritagedata/schemes/eh_tmc/concepts/100443" />
				<skos:scopeNote xml:lang="en">Ketch or yawl rigged vessel with a large mizzen sail used in the west country.</skos:scopeNote>
				<cc:license rdf:resource="http://creativecommons.org/licenses/by/3.0" />
				<cc:attributionURL rdf:resource="http://www.english-heritage.org.uk" />
				<cc:attributionName xml:lang="en">English Heritage</cc:attributionName>
				<dcterms:publisher rdf:resource="http://www.english-heritage.org.uk" />
			</skos:Concept>
		</skos:narrower>
		<skos:narrower>
			<skos:Concept rdf:about="http://purl.org/heritagedata/schemes/eh_tmc/concepts/100329">
				<skos:inScheme rdf:resource="http://purl.org/heritagedata/schemes/eh_tmc" />
				<dcterms:identifier>http://purl.org/heritagedata/schemes/eh_tmc/concepts/100329</dcterms:identifier>
				<skos:prefLabel xml:lang="en">EAST INDIAMAN</skos:prefLabel>
				<dcterms:issued rdf:datatype="http://www.w3.org/2001/XMLSchema#dateTime">2013-07-17T09:01:43</dcterms:issued>
				<skos:altLabel xml:lang="en">East India Company Sloop</skos:altLabel>
				<skos:broader rdf:resource="http://purl.org/heritagedata/schemes/eh_tmc/concepts/100443" />
				<skos:scopeNote xml:lang="en">Name given to a vessel of the East India Company. Usually large, well built and magnificently decorated.</skos:scopeNote>
				<cc:license rdf:resource="http://creativecommons.org/licenses/by/3.0" />
				<cc:attributionURL rdf:resource="http://www.english-heritage.org.uk" />
				<cc:attributionName xml:lang="en">English Heritage</cc:attributionName>
				<dcterms:publisher rdf:resource="http://www.english-heritage.org.uk" />
			</skos:Concept>
		</skos:narrower>
		<skos:narrower>
			<skos:Concept rdf:about="http://purl.org/heritagedata/schemes/eh_tmc/concepts/100524">
				<skos:inScheme rdf:resource="http://purl.org/heritagedata/schemes/eh_tmc" />
				<dcterms:identifier>http://purl.org/heritagedata/schemes/eh_tmc/concepts/100524</dcterms:identifier>
				<skos:prefLabel xml:lang="en">FLAT</skos:prefLabel>
				<dcterms:issued rdf:datatype="http://www.w3.org/2001/XMLSchema#dateTime">2013-07-17T09:01:43</dcterms:issued>
				<skos:broader rdf:resource="http://purl.org/heritagedata/schemes/eh_tmc/concepts/100443" />
				<skos:scopeNote xml:lang="en">A broad, flat-bottomed boat.</skos:scopeNote>
				<cc:license rdf:resource="http://creativecommons.org/licenses/by/3.0" />
				<cc:attributionURL rdf:resource="http://www.english-heritage.org.uk" />
				<cc:attributionName xml:lang="en">English Heritage</cc:attributionName>
				<dcterms:publisher rdf:resource="http://www.english-heritage.org.uk" />
			</skos:Concept>
		</skos:narrower>
		<skos:narrower>
			<skos:Concept rdf:about="http://purl.org/heritagedata/schemes/eh_tmc/concepts/100347">
				<skos:inScheme rdf:resource="http://purl.org/heritagedata/schemes/eh_tmc" />
				<dcterms:identifier>http://purl.org/heritagedata/schemes/eh_tmc/concepts/100347</dcterms:identifier>
				<skos:prefLabel xml:lang="en">FLY BOAT</skos:prefLabel>
				<dcterms:issued rdf:datatype="http://www.w3.org/2001/XMLSchema#dateTime">2013-07-17T09:01:43</dcterms:issued>
				<skos:altLabel xml:lang="en">Vlieboot</skos:altLabel>
				<skos:broader rdf:resource="http://purl.org/heritagedata/schemes/eh_tmc/concepts/100443" />
				<skos:scopeNote xml:lang="en">Flat bottomed, two-masted Dutch coastal vessel of the sixteenth to nineteenth centuries. Sometimes used as an English term for fluit, also a flat-bottomed vessel.</skos:scopeNote>
				<cc:license rdf:resource="http://creativecommons.org/licenses/by/3.0" />
				<cc:attributionURL rdf:resource="http://www.english-heritage.org.uk" />
				<cc:attributionName xml:lang="en">English Heritage</cc:attributionName>
				<dcterms:publisher rdf:resource="http://www.english-heritage.org.uk" />
			</skos:Concept>
		</skos:narrower>
		<skos:narrower>
			<skos:Concept rdf:about="http://purl.org/heritagedata/schemes/eh_tmc/concepts/144488">
				<skos:inScheme rdf:resource="http://purl.org/heritagedata/schemes/eh_tmc" />
				<dcterms:identifier>http://purl.org/heritagedata/schemes/eh_tmc/concepts/144488</dcterms:identifier>
				<skos:prefLabel xml:lang="en">GALLEASS</skos:prefLabel>
				<dcterms:issued rdf:datatype="http://www.w3.org/2001/XMLSchema#dateTime">2013-07-17T09:01:43</dcterms:issued>
				<skos:altLabel xml:lang="en">Oared Galleass</skos:altLabel>
				<skos:broader rdf:resource="http://purl.org/heritagedata/schemes/eh_tmc/concepts/100443" />
				<skos:scopeNote xml:lang="en">Oared sailing vessel developed in the 15th century, the larger English version with secondary oars coming into use in the 16th century. Not to be confused with GALEAS.</skos:scopeNote>
				<cc:license rdf:resource="http://creativecommons.org/licenses/by/3.0" />
				<cc:attributionURL rdf:resource="http://www.english-heritage.org.uk" />
				<cc:attributionName xml:lang="en">English Heritage</cc:attributionName>
				<dcterms:publisher rdf:resource="http://www.english-heritage.org.uk" />
			</skos:Concept>
		</skos:narrower>
		<skos:narrower>
			<skos:Concept rdf:about="http://purl.org/heritagedata/schemes/eh_tmc/concepts/100354">
				<skos:inScheme rdf:resource="http://purl.org/heritagedata/schemes/eh_tmc" />
				<dcterms:identifier>http://purl.org/heritagedata/schemes/eh_tmc/concepts/100354</dcterms:identifier>
				<skos:prefLabel xml:lang="en">GALLEON</skos:prefLabel>
				<dcterms:issued rdf:datatype="http://www.w3.org/2001/XMLSchema#dateTime">2013-07-17T09:01:43</dcterms:issued>
				<skos:broader rdf:resource="http://purl.org/heritagedata/schemes/eh_tmc/concepts/100443" />
				<skos:scopeNote xml:lang="en">Warship or trading vessel, three masted with a low forecastle.</skos:scopeNote>
				<cc:license rdf:resource="http://creativecommons.org/licenses/by/3.0" />
				<cc:attributionURL rdf:resource="http://www.english-heritage.org.uk" />
				<cc:attributionName xml:lang="en">English Heritage</cc:attributionName>
				<dcterms:publisher rdf:resource="http://www.english-heritage.org.uk" />
			</skos:Concept>
		</skos:narrower>
		<skos:narrower>
			<skos:Concept rdf:about="http://purl.org/heritagedata/schemes/eh_tmc/concepts/100356">
				<skos:inScheme rdf:resource="http://purl.org/heritagedata/schemes/eh_tmc" />
				<dcterms:identifier>http://purl.org/heritagedata/schemes/eh_tmc/concepts/100356</dcterms:identifier>
				<skos:prefLabel xml:lang="en">GALLIOT</skos:prefLabel>
				<dcterms:issued rdf:datatype="http://www.w3.org/2001/XMLSchema#dateTime">2013-07-17T09:01:43</dcterms:issued>
				<skos:broader rdf:resource="http://purl.org/heritagedata/schemes/eh_tmc/concepts/100443" />
				<skos:scopeNote xml:lang="en">A small galley or Dutch trading vessel similar to a barge in construction.</skos:scopeNote>
				<cc:license rdf:resource="http://creativecommons.org/licenses/by/3.0" />
				<cc:attributionURL rdf:resource="http://www.english-heritage.org.uk" />
				<cc:attributionName xml:lang="en">English Heritage</cc:attributionName>
				<dcterms:publisher rdf:resource="http://www.english-heritage.org.uk" />
			</skos:Concept>
		</skos:narrower>
		<skos:narrower>
			<skos:Concept rdf:about="http://purl.org/heritagedata/schemes/eh_tmc/concepts/100368">
				<skos:inScheme rdf:resource="http://purl.org/heritagedata/schemes/eh_tmc" />
				<dcterms:identifier>http://purl.org/heritagedata/schemes/eh_tmc/concepts/100368</dcterms:identifier>
				<skos:prefLabel xml:lang="en">HOY</skos:prefLabel>
				<dcterms:issued rdf:datatype="http://www.w3.org/2001/XMLSchema#dateTime">2013-07-17T09:01:43</dcterms:issued>
				<skos:broader rdf:resource="http://purl.org/heritagedata/schemes/eh_tmc/concepts/100443" />
				<skos:scopeNote xml:lang="en">Small coastal vessel.</skos:scopeNote>
				<cc:license rdf:resource="http://creativecommons.org/licenses/by/3.0" />
				<cc:attributionURL rdf:resource="http://www.english-heritage.org.uk" />
				<cc:attributionName xml:lang="en">English Heritage</cc:attributionName>
				<dcterms:publisher rdf:resource="http://www.english-heritage.org.uk" />
			</skos:Concept>
		</skos:narrower>
		<skos:narrower rdf:resource="http://purl.org/heritagedata/schemes/eh_tmc/concepts/139373" />
		<skos:narrower>
			<skos:Concept rdf:about="http://purl.org/heritagedata/schemes/eh_tmc/concepts/100370">
				<skos:inScheme rdf:resource="http://purl.org/heritagedata/schemes/eh_tmc" />
				<dcterms:identifier>http://purl.org/heritagedata/schemes/eh_tmc/concepts/100370</dcterms:identifier>
				<skos:prefLabel xml:lang="en">HUMBER KEEL</skos:prefLabel>
				<dcterms:issued rdf:datatype="http://www.w3.org/2001/XMLSchema#dateTime">2013-07-17T09:01:43</dcterms:issued>
				<skos:broader rdf:resource="http://purl.org/heritagedata/schemes/eh_tmc/concepts/100443" />
				<skos:scopeNote xml:lang="en">Flat bottomed vessel used for coasting on the River Humber.</skos:scopeNote>
				<cc:license rdf:resource="http://creativecommons.org/licenses/by/3.0" />
				<cc:attributionURL rdf:resource="http://www.english-heritage.org.uk" />
				<cc:attributionName xml:lang="en">English Heritage</cc:attributionName>
				<dcterms:publisher rdf:resource="http://www.english-heritage.org.uk" />
			</skos:Concept>
		</skos:narrower>
		<skos:narrower>
			<skos:Concept rdf:about="http://purl.org/heritagedata/schemes/eh_tmc/concepts/100374">
				<skos:inScheme rdf:resource="http://purl.org/heritagedata/schemes/eh_tmc" />
				<dcterms:identifier>http://purl.org/heritagedata/schemes/eh_tmc/concepts/100374</dcterms:identifier>
				<skos:prefLabel xml:lang="en">KEEL</skos:prefLabel>
				<dcterms:issued rdf:datatype="http://www.w3.org/2001/XMLSchema#dateTime">2013-07-17T09:01:43</dcterms:issued>
				<skos:broader rdf:resource="http://purl.org/heritagedata/schemes/eh_tmc/concepts/100443" />
				<skos:scopeNote xml:lang="en">Flat bottomed vessel used for loading colliers in the north east, similar to a lighter.</skos:scopeNote>
				<cc:license rdf:resource="http://creativecommons.org/licenses/by/3.0" />
				<cc:attributionURL rdf:resource="http://www.english-heritage.org.uk" />
				<cc:attributionName xml:lang="en">English Heritage</cc:attributionName>
				<dcterms:publisher rdf:resource="http://www.english-heritage.org.uk" />
			</skos:Concept>
		</skos:narrower>
		<skos:narrower rdf:resource="http://purl.org/heritagedata/schemes/eh_tmc/concepts/100375" />
		<skos:narrower rdf:resource="http://purl.org/heritagedata/schemes/eh_tmc/concepts/100392" />
		<skos:narrower>
			<skos:Concept rdf:about="http://purl.org/heritagedata/schemes/eh_tmc/concepts/100417">
				<skos:inScheme rdf:resource="http://purl.org/heritagedata/schemes/eh_tmc" />
				<dcterms:identifier>http://purl.org/heritagedata/schemes/eh_tmc/concepts/100417</dcterms:identifier>
				<skos:prefLabel xml:lang="en">PACKET</skos:prefLabel>
				<dcterms:issued rdf:datatype="http://www.w3.org/2001/XMLSchema#dateTime">2013-07-17T09:01:43</dcterms:issued>
				<skos:broader rdf:resource="http://purl.org/heritagedata/schemes/eh_tmc/concepts/100443" />
				<skos:scopeNote xml:lang="en">A fast, armed vessel, small in size, often used for despatches and mail.</skos:scopeNote>
				<cc:license rdf:resource="http://creativecommons.org/licenses/by/3.0" />
				<cc:attributionURL rdf:resource="http://www.english-heritage.org.uk" />
				<cc:attributionName xml:lang="en">English Heritage</cc:attributionName>
				<dcterms:publisher rdf:resource="http://www.english-heritage.org.uk" />
			</skos:Concept>
		</skos:narrower>
		<skos:narrower>
			<skos:Concept rdf:about="http://purl.org/heritagedata/schemes/eh_tmc/concepts/111713">
				<skos:inScheme rdf:resource="http://purl.org/heritagedata/schemes/eh_tmc" />
				<dcterms:identifier>http://purl.org/heritagedata/schemes/eh_tmc/concepts/111713</dcterms:identifier>
				<skos:prefLabel xml:lang="en">POLACRE</skos:prefLabel>
				<dcterms:issued rdf:datatype="http://www.w3.org/2001/XMLSchema#dateTime">2013-07-17T09:01:43</dcterms:issued>
				<skos:altLabel xml:lang="en">Polacca</skos:altLabel>
				<skos:broader rdf:resource="http://purl.org/heritagedata/schemes/eh_tmc/concepts/100443" />
				<skos:scopeNote xml:lang="en">A ship or brig peculiar to the Mediterranean.</skos:scopeNote>
				<cc:license rdf:resource="http://creativecommons.org/licenses/by/3.0" />
				<cc:attributionURL rdf:resource="http://www.english-heritage.org.uk" />
				<cc:attributionName xml:lang="en">English Heritage</cc:attributionName>
				<dcterms:publisher rdf:resource="http://www.english-heritage.org.uk" />
			</skos:Concept>
		</skos:narrower>
		<skos:broader rdf:resource="http://purl.org/heritagedata/schemes/eh_tmc/concepts/100394" />
		<skos:narrower>
			<skos:Concept rdf:about="http://purl.org/heritagedata/schemes/eh_tmc/concepts/100452">
				<skos:inScheme rdf:resource="http://purl.org/heritagedata/schemes/eh_tmc" />
				<dcterms:identifier>http://purl.org/heritagedata/schemes/eh_tmc/concepts/100452</dcterms:identifier>
				<skos:prefLabel xml:lang="en">SHALLOP</skos:prefLabel>
				<dcterms:issued rdf:datatype="http://www.w3.org/2001/XMLSchema#dateTime">2013-07-17T09:01:43</dcterms:issued>
				<skos:broader rdf:resource="http://purl.org/heritagedata/schemes/eh_tmc/concepts/100443" />
				<skos:scopeNote xml:lang="en">A small light vessel with a schooner rig often used for fishing.</skos:scopeNote>
				<cc:license rdf:resource="http://creativecommons.org/licenses/by/3.0" />
				<cc:attributionURL rdf:resource="http://www.english-heritage.org.uk" />
				<cc:attributionName xml:lang="en">English Heritage</cc:attributionName>
				<dcterms:publisher rdf:resource="http://www.english-heritage.org.uk" />
			</skos:Concept>
		</skos:narrower>
		<skos:narrower>
			<skos:Concept rdf:about="http://purl.org/heritagedata/schemes/eh_tmc/concepts/100456">
				<skos:inScheme rdf:resource="http://purl.org/heritagedata/schemes/eh_tmc" />
				<dcterms:identifier>http://purl.org/heritagedata/schemes/eh_tmc/concepts/100456</dcterms:identifier>
				<skos:prefLabel xml:lang="en">SLOOP</skos:prefLabel>
				<dcterms:issued rdf:datatype="http://www.w3.org/2001/XMLSchema#dateTime">2013-07-17T09:01:43</dcterms:issued>
				<skos:broader rdf:resource="http://purl.org/heritagedata/schemes/eh_tmc/concepts/100443" />
				<skos:scopeNote xml:lang="en">A vessel with a single mast, fore and aft rigged.</skos:scopeNote>
				<cc:license rdf:resource="http://creativecommons.org/licenses/by/3.0" />
				<cc:attributionURL rdf:resource="http://www.english-heritage.org.uk" />
				<cc:attributionName xml:lang="en">English Heritage</cc:attributionName>
				<dcterms:publisher rdf:resource="http://www.english-heritage.org.uk" />
			</skos:Concept>
		</skos:narrower>
		<skos:narrower>
			<skos:Concept rdf:about="http://purl.org/heritagedata/schemes/eh_tmc/concepts/100458">
				<skos:inScheme rdf:resource="http://purl.org/heritagedata/schemes/eh_tmc" />
				<dcterms:identifier>http://purl.org/heritagedata/schemes/eh_tmc/concepts/100458</dcterms:identifier>
				<skos:prefLabel xml:lang="en">SMACK</skos:prefLabel>
				<dcterms:issued rdf:datatype="http://www.w3.org/2001/XMLSchema#dateTime">2013-07-17T09:01:43</dcterms:issued>
				<skos:broader rdf:resource="http://purl.org/heritagedata/schemes/eh_tmc/concepts/100443" />
				<skos:scopeNote xml:lang="en">Small fishing craft used mainly for fishing, cutter or ketch rigged.</skos:scopeNote>
				<cc:license rdf:resource="http://creativecommons.org/licenses/by/3.0" />
				<cc:attributionURL rdf:resource="http://www.english-heritage.org.uk" />
				<cc:attributionName xml:lang="en">English Heritage</cc:attributionName>
				<dcterms:publisher rdf:resource="http://www.english-heritage.org.uk" />
			</skos:Concept>
		</skos:narrower>
		<skos:narrower>
			<skos:Concept rdf:about="http://purl.org/heritagedata/schemes/eh_tmc/concepts/100484">
				<skos:inScheme rdf:resource="http://purl.org/heritagedata/schemes/eh_tmc" />
				<dcterms:identifier>http://purl.org/heritagedata/schemes/eh_tmc/concepts/100484</dcterms:identifier>
				<skos:prefLabel xml:lang="en">TROW</skos:prefLabel>
				<dcterms:issued rdf:datatype="http://www.w3.org/2001/XMLSchema#dateTime">2013-07-17T09:01:43</dcterms:issued>
				<skos:broader rdf:resource="http://purl.org/heritagedata/schemes/eh_tmc/concepts/100443" />
				<skos:scopeNote xml:lang="en">A small cargo boat found on the River Severn in England, with a mast which could be taken down to allow the boat to pass under low bridges.</skos:scopeNote>
				<cc:license rdf:resource="http://creativecommons.org/licenses/by/3.0" />
				<cc:attributionURL rdf:resource="http://www.english-heritage.org.uk" />
				<cc:attributionName xml:lang="en">English Heritage</cc:attributionName>
				<dcterms:publisher rdf:resource="http://www.english-heritage.org.uk" />
			</skos:Concept>
		</skos:narrower>
		<skos:narrower>
			<skos:Concept rdf:about="http://purl.org/heritagedata/schemes/eh_tmc/concepts/100493">
				<skos:inScheme rdf:resource="http://purl.org/heritagedata/schemes/eh_tmc" />
				<dcterms:identifier>http://purl.org/heritagedata/schemes/eh_tmc/concepts/100493</dcterms:identifier>
				<skos:prefLabel xml:lang="en">WEST INDIAMAN</skos:prefLabel>
				<dcterms:issued rdf:datatype="http://www.w3.org/2001/XMLSchema#dateTime">2013-07-17T09:01:43</dcterms:issued>
				<skos:broader rdf:resource="http://purl.org/heritagedata/schemes/eh_tmc/concepts/100443" />
				<skos:scopeNote xml:lang="en">Any vessel in use by the West India Company.</skos:scopeNote>
				<cc:license rdf:resource="http://creativecommons.org/licenses/by/3.0" />
				<cc:attributionURL rdf:resource="http://www.english-heritage.org.uk" />
				<cc:attributionName xml:lang="en">English Heritage</cc:attributionName>
				<dcterms:publisher rdf:resource="http://www.english-heritage.org.uk" />
			</skos:Concept>
		</skos:narrower>
		<skos:narrower>
			<skos:Concept rdf:about="http://purl.org/heritagedata/schemes/eh_tmc/concepts/100498">
				<skos:inScheme rdf:resource="http://purl.org/heritagedata/schemes/eh_tmc" />
				<dcterms:identifier>http://purl.org/heritagedata/schemes/eh_tmc/concepts/100498</dcterms:identifier>
				<skos:prefLabel xml:lang="en">WHERRY</skos:prefLabel>
				<dcterms:issued rdf:datatype="http://www.w3.org/2001/XMLSchema#dateTime">2013-07-17T09:01:43</dcterms:issued>
				<skos:broader rdf:resource="http://purl.org/heritagedata/schemes/eh_tmc/concepts/100443" />
				<skos:scopeNote xml:lang="en">A decked sailing vessel of shallow draft.</skos:scopeNote>
				<cc:license rdf:resource="http://creativecommons.org/licenses/by/3.0" />
				<cc:attributionURL rdf:resource="http://www.english-heritage.org.uk" />
				<cc:attributionName xml:lang="en">English Heritage</cc:attributionName>
				<dcterms:publisher rdf:resource="http://www.english-heritage.org.uk" />
			</skos:Concept>
		</skos:narrower>
		<skos:narrower>
			<skos:Concept rdf:about="http://purl.org/heritagedata/schemes/eh_tmc/concepts/139547">
				<skos:inScheme rdf:resource="http://purl.org/heritagedata/schemes/eh_tmc" />
				<dcterms:identifier>http://purl.org/heritagedata/schemes/eh_tmc/concepts/139547</dcterms:identifier>
				<skos:prefLabel xml:lang="en">XEBEC</skos:prefLabel>
				<dcterms:issued rdf:datatype="http://www.w3.org/2001/XMLSchema#dateTime">2013-07-17T09:01:43</dcterms:issued>
				<skos:broader rdf:resource="http://purl.org/heritagedata/schemes/eh_tmc/concepts/100443" />
				<skos:scopeNote xml:lang="en">A small three-masted lateen-rigged vessel used exclusively in the Mediterranean from the 16th to the 19th century. Its hull was similar in form to that of a polacre but with an extended bow and stern.</skos:scopeNote>
				<cc:license rdf:resource="http://creativecommons.org/licenses/by/3.0" />
				<cc:attributionURL rdf:resource="http://www.english-heritage.org.uk" />
				<cc:attributionName xml:lang="en">English Heritage</cc:attributionName>
				<dcterms:publisher rdf:resource="http://www.english-heritage.org.uk" />
			</skos:Concept>
		</skos:narrower>
		<skos:narrower rdf:resource="http://purl.org/heritagedata/schemes/eh_tmc/concepts/100499" />
		<skos:narrower>
			<skos:Concept rdf:about="http://purl.org/heritagedata/schemes/eh_tmc/concepts/100521">
				<skos:inScheme rdf:resource="http://purl.org/heritagedata/schemes/eh_tmc" />
				<dcterms:identifier>http://purl.org/heritagedata/schemes/eh_tmc/concepts/100521</dcterms:identifier>
				<skos:prefLabel xml:lang="en">YAWL</skos:prefLabel>
				<dcterms:issued rdf:datatype="http://www.w3.org/2001/XMLSchema#dateTime">2013-07-17T09:01:43</dcterms:issued>
				<skos:broader rdf:resource="http://purl.org/heritagedata/schemes/eh_tmc/concepts/100443" />
				<skos:scopeNote xml:lang="en">A craft with two masts.It is usually cutter rigged on the foremast and has a small mizzen mast.</skos:scopeNote>
				<cc:license rdf:resource="http://creativecommons.org/licenses/by/3.0" />
				<cc:attributionURL rdf:resource="http://www.english-heritage.org.uk" />
				<cc:attributionName xml:lang="en">English Heritage</cc:attributionName>
				<dcterms:publisher rdf:resource="http://www.english-heritage.org.uk" />
			</skos:Concept>
		</skos:narrower>
		<skos:scopeNote xml:lang="en">A sailing vessel defined by a combination of such factors as hull design, locality and rig.</skos:scopeNote>
		<cc:license rdf:resource="http://creativecommons.org/licenses/by/3.0" />
		<cc:attributionURL rdf:resource="http://www.english-heritage.org.uk" />
		<cc:attributionName xml:lang="en">English Heritage</cc:attributionName>
		<dcterms:publisher rdf:resource="http://www.english-heritage.org.uk" />
	</skos:Concept>
	<skos:Concept rdf:about="http://purl.org/heritagedata/schemes/eh_tmc/concepts/100444">
		<skos:inScheme rdf:resource="http://purl.org/heritagedata/schemes/eh_tmc" />
		<dcterms:identifier>http://purl.org/heritagedata/schemes/eh_tmc/concepts/100444</dcterms:identifier>
		<skos:prefLabel xml:lang="en">SAILING VESSEL &lt;BY RIG&gt;</skos:prefLabel>
		<dcterms:issued rdf:datatype="http://www.w3.org/2001/XMLSchema#dateTime">2013-07-17T09:01:43</dcterms:issued>
		<skos:narrower>
			<skos:Concept rdf:about="http://purl.org/heritagedata/schemes/eh_tmc/concepts/100274">
				<skos:inScheme rdf:resource="http://purl.org/heritagedata/schemes/eh_tmc" />
				<dcterms:identifier>http://purl.org/heritagedata/schemes/eh_tmc/concepts/100274</dcterms:identifier>
				<skos:prefLabel xml:lang="en">BARQUENTINE</skos:prefLabel>
				<dcterms:issued rdf:datatype="http://www.w3.org/2001/XMLSchema#dateTime">2013-07-17T09:01:43</dcterms:issued>
				<skos:broader rdf:resource="http://purl.org/heritagedata/schemes/eh_tmc/concepts/100444" />
				<skos:scopeNote xml:lang="en">Sailing vessel generally with three masts square rigged on the foremast only.</skos:scopeNote>
				<cc:license rdf:resource="http://creativecommons.org/licenses/by/3.0" />
				<cc:attributionURL rdf:resource="http://www.english-heritage.org.uk" />
				<cc:attributionName xml:lang="en">English Heritage</cc:attributionName>
				<dcterms:publisher rdf:resource="http://www.english-heritage.org.uk" />
			</skos:Concept>
		</skos:narrower>
		<skos:narrower>
			<skos:Concept rdf:about="http://purl.org/heritagedata/schemes/eh_tmc/concepts/100518">
				<skos:inScheme rdf:resource="http://purl.org/heritagedata/schemes/eh_tmc" />
				<dcterms:identifier>http://purl.org/heritagedata/schemes/eh_tmc/concepts/100518</dcterms:identifier>
				<skos:prefLabel xml:lang="en">BRIGANTINE</skos:prefLabel>
				<dcterms:issued rdf:datatype="http://www.w3.org/2001/XMLSchema#dateTime">2013-07-17T09:01:43</dcterms:issued>
				<skos:broader rdf:resource="http://purl.org/heritagedata/schemes/eh_tmc/concepts/100444" />
				<skos:scopeNote xml:lang="en">A two masted craft which is square rigged on the foremast and fore and aft rigged on the main mast.</skos:scopeNote>
				<cc:license rdf:resource="http://creativecommons.org/licenses/by/3.0" />
				<cc:attributionURL rdf:resource="http://www.english-heritage.org.uk" />
				<cc:attributionName xml:lang="en">English Heritage</cc:attributionName>
				<dcterms:publisher rdf:resource="http://www.english-heritage.org.uk" />
			</skos:Concept>
		</skos:narrower>
		<skos:narrower>
			<skos:Concept rdf:about="http://purl.org/heritagedata/schemes/eh_tmc/concepts/100352">
				<skos:inScheme rdf:resource="http://purl.org/heritagedata/schemes/eh_tmc" />
				<dcterms:identifier>http://purl.org/heritagedata/schemes/eh_tmc/concepts/100352</dcterms:identifier>
				<skos:prefLabel xml:lang="en">FULL RIGGED SHIP</skos:prefLabel>
				<dcterms:issued rdf:datatype="http://www.w3.org/2001/XMLSchema#dateTime">2013-07-17T09:01:43</dcterms:issued>
				<skos:altLabel xml:lang="en">4 Masted Ship</skos:altLabel>
				<skos:altLabel xml:lang="en">5 Masted Ship</skos:altLabel>
				<skos:broader rdf:resource="http://purl.org/heritagedata/schemes/eh_tmc/concepts/100444" />
				<skos:scopeNote xml:lang="en">A vessel carrying square sails on all masts and having three or more masts.</skos:scopeNote>
				<cc:license rdf:resource="http://creativecommons.org/licenses/by/3.0" />
				<cc:attributionURL rdf:resource="http://www.english-heritage.org.uk" />
				<cc:attributionName xml:lang="en">English Heritage</cc:attributionName>
				<dcterms:publisher rdf:resource="http://www.english-heritage.org.uk" />
			</skos:Concept>
		</skos:narrower>
		<skos:broader rdf:resource="http://purl.org/heritagedata/schemes/eh_tmc/concepts/100394" />
		<skos:narrower>
			<skos:Concept rdf:about="http://purl.org/heritagedata/schemes/eh_tmc/concepts/100447">
				<skos:inScheme rdf:resource="http://purl.org/heritagedata/schemes/eh_tmc" />
				<dcterms:identifier>http://purl.org/heritagedata/schemes/eh_tmc/concepts/100447</dcterms:identifier>
				<skos:prefLabel xml:lang="en">SCHOONER</skos:prefLabel>
				<dcterms:issued rdf:datatype="http://www.w3.org/2001/XMLSchema#dateTime">2013-07-17T09:01:43</dcterms:issued>
				<skos:altLabel xml:lang="en">5 Masted Schooner</skos:altLabel>
				<skos:broader rdf:resource="http://purl.org/heritagedata/schemes/eh_tmc/concepts/100444" />
				<skos:scopeNote xml:lang="en">Two masted ship with fore and aft sails and two or more masts.</skos:scopeNote>
				<cc:license rdf:resource="http://creativecommons.org/licenses/by/3.0" />
				<cc:attributionURL rdf:resource="http://www.english-heritage.org.uk" />
				<cc:attributionName xml:lang="en">English Heritage</cc:attributionName>
				<dcterms:publisher rdf:resource="http://www.english-heritage.org.uk" />
			</skos:Concept>
		</skos:narrower>
		<skos:narrower rdf:resource="http://purl.org/heritagedata/schemes/eh_tmc/concepts/100461" />
		<skos:scopeNote xml:lang="en">The characteristics of a sailing vessel where her type is determined by her masts and sails.</skos:scopeNote>
		<cc:license rdf:resource="http://creativecommons.org/licenses/by/3.0" />
		<cc:attributionURL rdf:resource="http://www.english-heritage.org.uk" />
		<cc:attributionName xml:lang="en">English Heritage</cc:attributionName>
		<dcterms:publisher rdf:resource="http://www.english-heritage.org.uk" />
	</skos:Concept>
	<skos:Concept rdf:about="http://purl.org/heritagedata/schemes/eh_tmc/concepts/100445">
		<skos:inScheme rdf:resource="http://purl.org/heritagedata/schemes/eh_tmc" />
		<dcterms:identifier>http://purl.org/heritagedata/schemes/eh_tmc/concepts/100445</dcterms:identifier>
		<skos:prefLabel xml:lang="en">SALVAGE TUG</skos:prefLabel>
		<dcterms:issued rdf:datatype="http://www.w3.org/2001/XMLSchema#dateTime">2013-07-17T09:01:43</dcterms:issued>
		<skos:broader rdf:resource="http://purl.org/heritagedata/schemes/eh_tmc/concepts/100485" />
		<skos:broader rdf:resource="http://purl.org/heritagedata/schemes/eh_tmc/concepts/100446" />
		<skos:scopeNote xml:lang="en">A small and powerful vessel used to assist vessels that are sinking or disabled at sea.</skos:scopeNote>
		<cc:license rdf:resource="http://creativecommons.org/licenses/by/3.0" />
		<cc:attributionURL rdf:resource="http://www.english-heritage.org.uk" />
		<cc:attributionName xml:lang="en">English Heritage</cc:attributionName>
		<dcterms:publisher rdf:resource="http://www.english-heritage.org.uk" />
	</skos:Concept>
	<skos:Concept rdf:about="http://purl.org/heritagedata/schemes/eh_tmc/concepts/100446">
		<skos:inScheme rdf:resource="http://purl.org/heritagedata/schemes/eh_tmc" />
		<dcterms:identifier>http://purl.org/heritagedata/schemes/eh_tmc/concepts/100446</dcterms:identifier>
		<skos:prefLabel xml:lang="en">SALVAGE VESSEL</skos:prefLabel>
		<dcterms:issued rdf:datatype="http://www.w3.org/2001/XMLSchema#dateTime">2013-07-17T09:01:43</dcterms:issued>
		<skos:narrower rdf:resource="http://purl.org/heritagedata/schemes/eh_tmc/concepts/100445" />
		<skos:broader rdf:resource="http://purl.org/heritagedata/schemes/eh_tmc/concepts/100450" />
		<skos:scopeNote xml:lang="en">A vessel used for the underwater recovery of a ship and/or her contents or to assist vessels that are sinking.</skos:scopeNote>
		<cc:license rdf:resource="http://creativecommons.org/licenses/by/3.0" />
		<cc:attributionURL rdf:resource="http://www.english-heritage.org.uk" />
		<cc:attributionName xml:lang="en">English Heritage</cc:attributionName>
		<dcterms:publisher rdf:resource="http://www.english-heritage.org.uk" />
	</skos:Concept>
	<skos:Concept rdf:about="http://purl.org/heritagedata/schemes/eh_tmc/concepts/100450">
		<skos:inScheme rdf:resource="http://purl.org/heritagedata/schemes/eh_tmc" />
		<dcterms:identifier>http://purl.org/heritagedata/schemes/eh_tmc/concepts/100450</dcterms:identifier>
		<skos:prefLabel xml:lang="en">SERVICE VESSEL</skos:prefLabel>
		<dcterms:issued rdf:datatype="http://www.w3.org/2001/XMLSchema#dateTime">2013-07-17T09:01:43</dcterms:issued>
		<skos:narrower rdf:resource="http://purl.org/heritagedata/schemes/eh_tmc/concepts/100338" />
		<skos:narrower rdf:resource="http://purl.org/heritagedata/schemes/eh_tmc/concepts/100361" />
		<skos:narrower>
			<skos:Concept rdf:about="http://purl.org/heritagedata/schemes/eh_tmc/concepts/100387">
				<skos:inScheme rdf:resource="http://purl.org/heritagedata/schemes/eh_tmc" />
				<dcterms:identifier>http://purl.org/heritagedata/schemes/eh_tmc/concepts/100387</dcterms:identifier>
				<skos:prefLabel xml:lang="en">LIGHTHOUSE TENDER</skos:prefLabel>
				<dcterms:issued rdf:datatype="http://www.w3.org/2001/XMLSchema#dateTime">2013-07-17T09:01:43</dcterms:issued>
				<skos:broader rdf:resource="http://purl.org/heritagedata/schemes/eh_tmc/concepts/100450" />
				<skos:scopeNote xml:lang="en">A small vessel used to carry supplies and personnel to lighthouses.</skos:scopeNote>
				<cc:license rdf:resource="http://creativecommons.org/licenses/by/3.0" />
				<cc:attributionURL rdf:resource="http://www.english-heritage.org.uk" />
				<cc:attributionName xml:lang="en">English Heritage</cc:attributionName>
				<dcterms:publisher rdf:resource="http://www.english-heritage.org.uk" />
			</skos:Concept>
		</skos:narrower>
		<skos:narrower>
			<skos:Concept rdf:about="http://purl.org/heritagedata/schemes/eh_tmc/concepts/100424">
				<skos:inScheme rdf:resource="http://purl.org/heritagedata/schemes/eh_tmc" />
				<dcterms:identifier>http://purl.org/heritagedata/schemes/eh_tmc/concepts/100424</dcterms:identifier>
				<skos:prefLabel xml:lang="en">PILOT VESSEL</skos:prefLabel>
				<dcterms:issued rdf:datatype="http://www.w3.org/2001/XMLSchema#dateTime">2013-07-17T09:01:43</dcterms:issued>
				<skos:broader rdf:resource="http://purl.org/heritagedata/schemes/eh_tmc/concepts/100450" />
				<skos:scopeNote xml:lang="en">A vessel used to carry a pilot to a ship.</skos:scopeNote>
				<cc:license rdf:resource="http://creativecommons.org/licenses/by/3.0" />
				<cc:attributionURL rdf:resource="http://www.english-heritage.org.uk" />
				<cc:attributionName xml:lang="en">English Heritage</cc:attributionName>
				<dcterms:publisher rdf:resource="http://www.english-heritage.org.uk" />
			</skos:Concept>
		</skos:narrower>
		<skos:narrower rdf:resource="http://purl.org/heritagedata/schemes/eh_tmc/concepts/100439" />
		<skos:narrower rdf:resource="http://purl.org/heritagedata/schemes/eh_tmc/concepts/100446" />
		<skos:broader rdf:resource="http://purl.org/heritagedata/schemes/eh_tmc/concepts/100394" />
		<skos:scopeNote xml:lang="en">A vessel used to maintain supply or assist larger vessels. Use more specific term.</skos:scopeNote>
		<cc:license rdf:resource="http://creativecommons.org/licenses/by/3.0" />
		<cc:attributionURL rdf:resource="http://www.english-heritage.org.uk" />
		<cc:attributionName xml:lang="en">English Heritage</cc:attributionName>
		<dcterms:publisher rdf:resource="http://www.english-heritage.org.uk" />
	</skos:Concept>
	<skos:Concept rdf:about="http://purl.org/heritagedata/schemes/eh_tmc/concepts/100455">
		<skos:inScheme rdf:resource="http://purl.org/heritagedata/schemes/eh_tmc" />
		<dcterms:identifier>http://purl.org/heritagedata/schemes/eh_tmc/concepts/100455</dcterms:identifier>
		<skos:prefLabel xml:lang="en">SHIP OF THE LINE</skos:prefLabel>
		<dcterms:issued rdf:datatype="http://www.w3.org/2001/XMLSchema#dateTime">2013-07-17T09:01:43</dcterms:issued>
		<skos:narrower>
			<skos:Concept rdf:about="http://purl.org/heritagedata/schemes/eh_tmc/concepts/100504">
				<skos:inScheme rdf:resource="http://purl.org/heritagedata/schemes/eh_tmc" />
				<dcterms:identifier>http://purl.org/heritagedata/schemes/eh_tmc/concepts/100504</dcterms:identifier>
				<skos:prefLabel xml:lang="en">FIFTH RATE SHIP OF THE LINE</skos:prefLabel>
				<dcterms:issued rdf:datatype="http://www.w3.org/2001/XMLSchema#dateTime">2013-07-17T09:01:43</dcterms:issued>
				<skos:altLabel xml:lang="en">32 Gun Ship</skos:altLabel>
				<skos:altLabel xml:lang="en">36 Gun Ship</skos:altLabel>
				<skos:altLabel xml:lang="en">44 Gun Ship</skos:altLabel>
				<skos:broader rdf:resource="http://purl.org/heritagedata/schemes/eh_tmc/concepts/100455" />
				<skos:scopeNote xml:lang="en">A sailing frigate mounting 32 to 44 guns with the main battery on a single deck.</skos:scopeNote>
				<cc:license rdf:resource="http://creativecommons.org/licenses/by/3.0" />
				<cc:attributionURL rdf:resource="http://www.english-heritage.org.uk" />
				<cc:attributionName xml:lang="en">English Heritage</cc:attributionName>
				<dcterms:publisher rdf:resource="http://www.english-heritage.org.uk" />
			</skos:Concept>
		</skos:narrower>
		<skos:narrower>
			<skos:Concept rdf:about="http://purl.org/heritagedata/schemes/eh_tmc/concepts/100500">
				<skos:inScheme rdf:resource="http://purl.org/heritagedata/schemes/eh_tmc" />
				<dcterms:identifier>http://purl.org/heritagedata/schemes/eh_tmc/concepts/100500</dcterms:identifier>
				<skos:prefLabel xml:lang="en">FIRST RATE SHIP OF THE LINE</skos:prefLabel>
				<dcterms:issued rdf:datatype="http://www.w3.org/2001/XMLSchema#dateTime">2013-07-17T09:01:43</dcterms:issued>
				<skos:altLabel xml:lang="en">100 Gun Ship</skos:altLabel>
				<skos:broader rdf:resource="http://purl.org/heritagedata/schemes/eh_tmc/concepts/100455" />
				<skos:scopeNote xml:lang="en">A ship of the line mounting 100 guns or more on three gundecks.</skos:scopeNote>
				<cc:license rdf:resource="http://creativecommons.org/licenses/by/3.0" />
				<cc:attributionURL rdf:resource="http://www.english-heritage.org.uk" />
				<cc:attributionName xml:lang="en">English Heritage</cc:attributionName>
				<dcterms:publisher rdf:resource="http://www.english-heritage.org.uk" />
			</skos:Concept>
		</skos:narrower>
		<skos:narrower>
			<skos:Concept rdf:about="http://purl.org/heritagedata/schemes/eh_tmc/concepts/100503">
				<skos:inScheme rdf:resource="http://purl.org/heritagedata/schemes/eh_tmc" />
				<dcterms:identifier>http://purl.org/heritagedata/schemes/eh_tmc/concepts/100503</dcterms:identifier>
				<skos:prefLabel xml:lang="en">FOURTH RATE SHIP OF THE LINE</skos:prefLabel>
				<dcterms:issued rdf:datatype="http://www.w3.org/2001/XMLSchema#dateTime">2013-07-17T09:01:43</dcterms:issued>
				<skos:altLabel xml:lang="en">64 Gun Ship</skos:altLabel>
				<skos:broader rdf:resource="http://purl.org/heritagedata/schemes/eh_tmc/concepts/100455" />
				<skos:scopeNote xml:lang="en">A ship of the line mounting between 46 and 64 guns</skos:scopeNote>
				<cc:license rdf:resource="http://creativecommons.org/licenses/by/3.0" />
				<cc:attributionURL rdf:resource="http://www.english-heritage.org.uk" />
				<cc:attributionName xml:lang="en">English Heritage</cc:attributionName>
				<dcterms:publisher rdf:resource="http://www.english-heritage.org.uk" />
			</skos:Concept>
		</skos:narrower>
		<skos:narrower>
			<skos:Concept rdf:about="http://purl.org/heritagedata/schemes/eh_tmc/concepts/100501">
				<skos:inScheme rdf:resource="http://purl.org/heritagedata/schemes/eh_tmc" />
				<dcterms:identifier>http://purl.org/heritagedata/schemes/eh_tmc/concepts/100501</dcterms:identifier>
				<skos:prefLabel xml:lang="en">SECOND RATE SHIP OF THE LINE</skos:prefLabel>
				<dcterms:issued rdf:datatype="http://www.w3.org/2001/XMLSchema#dateTime">2013-07-17T09:01:43</dcterms:issued>
				<skos:altLabel xml:lang="en">90 Gun Ship</skos:altLabel>
				<skos:broader rdf:resource="http://purl.org/heritagedata/schemes/eh_tmc/concepts/100455" />
				<skos:scopeNote xml:lang="en">A ship of the line mounting between 90 and 98 guns on three gun decks</skos:scopeNote>
				<cc:license rdf:resource="http://creativecommons.org/licenses/by/3.0" />
				<cc:attributionURL rdf:resource="http://www.english-heritage.org.uk" />
				<cc:attributionName xml:lang="en">English Heritage</cc:attributionName>
				<dcterms:publisher rdf:resource="http://www.english-heritage.org.uk" />
			</skos:Concept>
		</skos:narrower>
		<skos:broader rdf:resource="http://purl.org/heritagedata/schemes/eh_tmc/concepts/100490" />
		<skos:narrower>
			<skos:Concept rdf:about="http://purl.org/heritagedata/schemes/eh_tmc/concepts/100505">
				<skos:inScheme rdf:resource="http://purl.org/heritagedata/schemes/eh_tmc" />
				<dcterms:identifier>http://purl.org/heritagedata/schemes/eh_tmc/concepts/100505</dcterms:identifier>
				<skos:prefLabel xml:lang="en">SIXTH RATE SHIP OF THE LINE</skos:prefLabel>
				<dcterms:issued rdf:datatype="http://www.w3.org/2001/XMLSchema#dateTime">2013-07-17T09:01:43</dcterms:issued>
				<skos:altLabel xml:lang="en">24 Gun Ship</skos:altLabel>
				<skos:altLabel xml:lang="en">30 Gun Ship</skos:altLabel>
				<skos:broader rdf:resource="http://purl.org/heritagedata/schemes/eh_tmc/concepts/100455" />
				<skos:scopeNote xml:lang="en">A small warship mounting between 20 and 28 nine-pounder guns on a single deck.</skos:scopeNote>
				<cc:license rdf:resource="http://creativecommons.org/licenses/by/3.0" />
				<cc:attributionURL rdf:resource="http://www.english-heritage.org.uk" />
				<cc:attributionName xml:lang="en">English Heritage</cc:attributionName>
				<dcterms:publisher rdf:resource="http://www.english-heritage.org.uk" />
			</skos:Concept>
		</skos:narrower>
		<skos:narrower>
			<skos:Concept rdf:about="http://purl.org/heritagedata/schemes/eh_tmc/concepts/100502">
				<skos:inScheme rdf:resource="http://purl.org/heritagedata/schemes/eh_tmc" />
				<dcterms:identifier>http://purl.org/heritagedata/schemes/eh_tmc/concepts/100502</dcterms:identifier>
				<skos:prefLabel xml:lang="en">THIRD RATE SHIP OF THE LINE</skos:prefLabel>
				<dcterms:issued rdf:datatype="http://www.w3.org/2001/XMLSchema#dateTime">2013-07-17T09:01:43</dcterms:issued>
				<skos:altLabel xml:lang="en">70 Gun Ship</skos:altLabel>
				<skos:altLabel xml:lang="en">72 Gun Ship</skos:altLabel>
				<skos:altLabel xml:lang="en">74 Gun Ship</skos:altLabel>
				<skos:altLabel xml:lang="en">Dublin Class 74 Gun Ship</skos:altLabel>
				<skos:broader rdf:resource="http://purl.org/heritagedata/schemes/eh_tmc/concepts/100455" />
				<skos:scopeNote xml:lang="en">A ship of the line mounting between 64 and 80 guns typically built with two gun decks.</skos:scopeNote>
				<cc:license rdf:resource="http://creativecommons.org/licenses/by/3.0" />
				<cc:attributionURL rdf:resource="http://www.english-heritage.org.uk" />
				<cc:attributionName xml:lang="en">English Heritage</cc:attributionName>
				<dcterms:publisher rdf:resource="http://www.english-heritage.org.uk" />
			</skos:Concept>
		</skos:narrower>
		<skos:scopeNote xml:lang="en">A sailing ship with a sufficient numerically large gun armament to stand in the line of battle.</skos:scopeNote>
		<cc:license rdf:resource="http://creativecommons.org/licenses/by/3.0" />
		<cc:attributionURL rdf:resource="http://www.english-heritage.org.uk" />
		<cc:attributionName xml:lang="en">English Heritage</cc:attributionName>
		<dcterms:publisher rdf:resource="http://www.english-heritage.org.uk" />
	</skos:Concept>
	<skos:Concept rdf:about="http://purl.org/heritagedata/schemes/eh_tmc/concepts/100460">
		<skos:inScheme rdf:resource="http://purl.org/heritagedata/schemes/eh_tmc" />
		<dcterms:identifier>http://purl.org/heritagedata/schemes/eh_tmc/concepts/100460</dcterms:identifier>
		<skos:prefLabel xml:lang="en">SPRITSAIL BARGE</skos:prefLabel>
		<dcterms:issued rdf:datatype="http://www.w3.org/2001/XMLSchema#dateTime">2013-07-17T09:01:43</dcterms:issued>
		<skos:broader rdf:resource="http://purl.org/heritagedata/schemes/eh_tmc/concepts/100272" />
		<skos:narrower>
			<skos:Concept rdf:about="http://purl.org/heritagedata/schemes/eh_tmc/concepts/147517">
				<skos:inScheme rdf:resource="http://purl.org/heritagedata/schemes/eh_tmc" />
				<dcterms:identifier>http://purl.org/heritagedata/schemes/eh_tmc/concepts/147517</dcterms:identifier>
				<skos:prefLabel xml:lang="en">THAMES SAILING BARGE</skos:prefLabel>
				<dcterms:issued rdf:datatype="http://www.w3.org/2001/XMLSchema#dateTime">2013-07-17T09:01:43</dcterms:issued>
				<skos:altLabel xml:lang="en">Thames Barge</skos:altLabel>
				<skos:broader rdf:resource="http://purl.org/heritagedata/schemes/eh_tmc/concepts/100460" />
				<skos:scopeNote xml:lang="en">Flat-bottomed barge with shallow draft adapted for carrying bulk cargoes among the shoals of the Thames Estuary; usually spritsail-rigged, though other rigs were permissible.</skos:scopeNote>
				<cc:license rdf:resource="http://creativecommons.org/licenses/by/3.0" />
				<cc:attributionURL rdf:resource="http://www.english-heritage.org.uk" />
				<cc:attributionName xml:lang="en">English Heritage</cc:attributionName>
				<dcterms:publisher rdf:resource="http://www.english-heritage.org.uk" />
			</skos:Concept>
		</skos:narrower>
		<skos:scopeNote xml:lang="en">A barge with a spritsail rig commonly found on the River Thames.</skos:scopeNote>
		<cc:license rdf:resource="http://creativecommons.org/licenses/by/3.0" />
		<cc:attributionURL rdf:resource="http://www.english-heritage.org.uk" />
		<cc:attributionName xml:lang="en">English Heritage</cc:attributionName>
		<dcterms:publisher rdf:resource="http://www.english-heritage.org.uk" />
	</skos:Concept>
	<skos:Concept rdf:about="http://purl.org/heritagedata/schemes/eh_tmc/concepts/100461">
		<skos:inScheme rdf:resource="http://purl.org/heritagedata/schemes/eh_tmc" />
		<dcterms:identifier>http://purl.org/heritagedata/schemes/eh_tmc/concepts/100461</dcterms:identifier>
		<skos:prefLabel xml:lang="en">SQUARE RIGGED VESSEL</skos:prefLabel>
		<dcterms:issued rdf:datatype="http://www.w3.org/2001/XMLSchema#dateTime">2013-07-17T09:01:43</dcterms:issued>
		<skos:narrower>
			<skos:Concept rdf:about="http://purl.org/heritagedata/schemes/eh_tmc/concepts/100273">
				<skos:inScheme rdf:resource="http://purl.org/heritagedata/schemes/eh_tmc" />
				<dcterms:identifier>http://purl.org/heritagedata/schemes/eh_tmc/concepts/100273</dcterms:identifier>
				<skos:prefLabel xml:lang="en">BARQUE</skos:prefLabel>
				<dcterms:issued rdf:datatype="http://www.w3.org/2001/XMLSchema#dateTime">2013-07-17T09:01:43</dcterms:issued>
				<skos:broader rdf:resource="http://purl.org/heritagedata/schemes/eh_tmc/concepts/100461" />
				<skos:scopeNote xml:lang="en">A sailing vessel, generally with three masts, square rigged on the fore and main mast.</skos:scopeNote>
				<cc:license rdf:resource="http://creativecommons.org/licenses/by/3.0" />
				<cc:attributionURL rdf:resource="http://www.english-heritage.org.uk" />
				<cc:attributionName xml:lang="en">English Heritage</cc:attributionName>
				<dcterms:publisher rdf:resource="http://www.english-heritage.org.uk" />
			</skos:Concept>
		</skos:narrower>
		<skos:narrower>
			<skos:Concept rdf:about="http://purl.org/heritagedata/schemes/eh_tmc/concepts/100285">
				<skos:inScheme rdf:resource="http://purl.org/heritagedata/schemes/eh_tmc" />
				<dcterms:identifier>http://purl.org/heritagedata/schemes/eh_tmc/concepts/100285</dcterms:identifier>
				<skos:prefLabel xml:lang="en">BRIG</skos:prefLabel>
				<dcterms:issued rdf:datatype="http://www.w3.org/2001/XMLSchema#dateTime">2013-07-17T09:01:43</dcterms:issued>
				<skos:broader rdf:resource="http://purl.org/heritagedata/schemes/eh_tmc/concepts/100461" />
				<skos:scopeNote xml:lang="en">Two masted vessel with a square rig on both masts.</skos:scopeNote>
				<cc:license rdf:resource="http://creativecommons.org/licenses/by/3.0" />
				<cc:attributionURL rdf:resource="http://www.english-heritage.org.uk" />
				<cc:attributionName xml:lang="en">English Heritage</cc:attributionName>
				<dcterms:publisher rdf:resource="http://www.english-heritage.org.uk" />
			</skos:Concept>
		</skos:narrower>
		<skos:narrower>
			<skos:Concept rdf:about="http://purl.org/heritagedata/schemes/eh_tmc/concepts/100425">
				<skos:inScheme rdf:resource="http://purl.org/heritagedata/schemes/eh_tmc" />
				<dcterms:identifier>http://purl.org/heritagedata/schemes/eh_tmc/concepts/100425</dcterms:identifier>
				<skos:prefLabel xml:lang="en">PINK</skos:prefLabel>
				<dcterms:issued rdf:datatype="http://www.w3.org/2001/XMLSchema#dateTime">2013-07-17T09:01:43</dcterms:issued>
				<skos:broader rdf:resource="http://purl.org/heritagedata/schemes/eh_tmc/concepts/100461" />
				<skos:scopeNote xml:lang="en">Small square rigged ship with a narrow overhanging stern.</skos:scopeNote>
				<cc:license rdf:resource="http://creativecommons.org/licenses/by/3.0" />
				<cc:attributionURL rdf:resource="http://www.english-heritage.org.uk" />
				<cc:attributionName xml:lang="en">English Heritage</cc:attributionName>
				<dcterms:publisher rdf:resource="http://www.english-heritage.org.uk" />
			</skos:Concept>
		</skos:narrower>
		<skos:narrower>
			<skos:Concept rdf:about="http://purl.org/heritagedata/schemes/eh_tmc/concepts/100426">
				<skos:inScheme rdf:resource="http://purl.org/heritagedata/schemes/eh_tmc" />
				<dcterms:identifier>http://purl.org/heritagedata/schemes/eh_tmc/concepts/100426</dcterms:identifier>
				<skos:prefLabel xml:lang="en">PINNACE</skos:prefLabel>
				<dcterms:issued rdf:datatype="http://www.w3.org/2001/XMLSchema#dateTime">2013-07-17T09:01:43</dcterms:issued>
				<skos:broader rdf:resource="http://purl.org/heritagedata/schemes/eh_tmc/concepts/100461" />
				<skos:scopeNote xml:lang="en">A small two masted craft, with oars as well as sails.</skos:scopeNote>
				<cc:license rdf:resource="http://creativecommons.org/licenses/by/3.0" />
				<cc:attributionURL rdf:resource="http://www.english-heritage.org.uk" />
				<cc:attributionName xml:lang="en">English Heritage</cc:attributionName>
				<dcterms:publisher rdf:resource="http://www.english-heritage.org.uk" />
			</skos:Concept>
		</skos:narrower>
		<skos:narrower>
			<skos:Concept rdf:about="http://purl.org/heritagedata/schemes/eh_tmc/concepts/100459">
				<skos:inScheme rdf:resource="http://purl.org/heritagedata/schemes/eh_tmc" />
				<dcterms:identifier>http://purl.org/heritagedata/schemes/eh_tmc/concepts/100459</dcterms:identifier>
				<skos:prefLabel xml:lang="en">SNOW</skos:prefLabel>
				<dcterms:issued rdf:datatype="http://www.w3.org/2001/XMLSchema#dateTime">2013-07-17T09:01:43</dcterms:issued>
				<skos:broader rdf:resource="http://purl.org/heritagedata/schemes/eh_tmc/concepts/100461" />
				<skos:scopeNote xml:lang="en">Two masted merchant vessel, rigged as a brig.</skos:scopeNote>
				<cc:license rdf:resource="http://creativecommons.org/licenses/by/3.0" />
				<cc:attributionURL rdf:resource="http://www.english-heritage.org.uk" />
				<cc:attributionName xml:lang="en">English Heritage</cc:attributionName>
				<dcterms:publisher rdf:resource="http://www.english-heritage.org.uk" />
			</skos:Concept>
		</skos:narrower>
		<skos:broader rdf:resource="http://purl.org/heritagedata/schemes/eh_tmc/concepts/100444" />
		<skos:scopeNote xml:lang="en">A vessel with a type of rigging where the main driving sails are fixed to yards which lie square to the mast.</skos:scopeNote>
		<cc:license rdf:resource="http://creativecommons.org/licenses/by/3.0" />
		<cc:attributionURL rdf:resource="http://www.english-heritage.org.uk" />
		<cc:attributionName xml:lang="en">English Heritage</cc:attributionName>
		<dcterms:publisher rdf:resource="http://www.english-heritage.org.uk" />
	</skos:Concept>
	<skos:Concept rdf:about="http://purl.org/heritagedata/schemes/eh_tmc/concepts/100462">
		<skos:inScheme rdf:resource="http://purl.org/heritagedata/schemes/eh_tmc" />
		<dcterms:identifier>http://purl.org/heritagedata/schemes/eh_tmc/concepts/100462</dcterms:identifier>
		<skos:prefLabel xml:lang="en">STORAGE HULK</skos:prefLabel>
		<dcterms:issued rdf:datatype="http://www.w3.org/2001/XMLSchema#dateTime">2013-07-17T09:01:43</dcterms:issued>
		<skos:narrower>
			<skos:Concept rdf:about="http://purl.org/heritagedata/schemes/eh_tmc/concepts/139810">
				<skos:inScheme rdf:resource="http://purl.org/heritagedata/schemes/eh_tmc" />
				<dcterms:identifier>http://purl.org/heritagedata/schemes/eh_tmc/concepts/139810</dcterms:identifier>
				<skos:prefLabel xml:lang="en">GRAIN HULK</skos:prefLabel>
				<dcterms:issued rdf:datatype="http://www.w3.org/2001/XMLSchema#dateTime">2013-07-17T09:01:43</dcterms:issued>
				<skos:broader rdf:resource="http://purl.org/heritagedata/schemes/eh_tmc/concepts/100462" />
				<skos:scopeNote xml:lang="en">A demasted ship used exclusively for the storage of grain.</skos:scopeNote>
				<cc:license rdf:resource="http://creativecommons.org/licenses/by/3.0" />
				<cc:attributionURL rdf:resource="http://www.english-heritage.org.uk" />
				<cc:attributionName xml:lang="en">English Heritage</cc:attributionName>
				<dcterms:publisher rdf:resource="http://www.english-heritage.org.uk" />
			</skos:Concept>
		</skos:narrower>
		<skos:narrower>
			<skos:Concept rdf:about="http://purl.org/heritagedata/schemes/eh_tmc/concepts/100429">
				<skos:inScheme rdf:resource="http://purl.org/heritagedata/schemes/eh_tmc" />
				<dcterms:identifier>http://purl.org/heritagedata/schemes/eh_tmc/concepts/100429</dcterms:identifier>
				<skos:prefLabel xml:lang="en">POWDER HULK</skos:prefLabel>
				<dcterms:issued rdf:datatype="http://www.w3.org/2001/XMLSchema#dateTime">2013-07-17T09:01:43</dcterms:issued>
				<skos:broader rdf:resource="http://purl.org/heritagedata/schemes/eh_tmc/concepts/100462" />
				<skos:scopeNote xml:lang="en">A vessel used for storing and issuing gunpowder, usually moored well away from the dockyard.</skos:scopeNote>
				<cc:license rdf:resource="http://creativecommons.org/licenses/by/3.0" />
				<cc:attributionURL rdf:resource="http://www.english-heritage.org.uk" />
				<cc:attributionName xml:lang="en">English Heritage</cc:attributionName>
				<dcterms:publisher rdf:resource="http://www.english-heritage.org.uk" />
			</skos:Concept>
		</skos:narrower>
		<skos:broader rdf:resource="http://purl.org/heritagedata/schemes/eh_tmc/concepts/100369" />
		<skos:scopeNote xml:lang="en">A demasted old ship used for storing items.</skos:scopeNote>
		<cc:license rdf:resource="http://creativecommons.org/licenses/by/3.0" />
		<cc:attributionURL rdf:resource="http://www.english-heritage.org.uk" />
		<cc:attributionName xml:lang="en">English Heritage</cc:attributionName>
		<dcterms:publisher rdf:resource="http://www.english-heritage.org.uk" />
	</skos:Concept>
	<skos:Concept rdf:about="http://purl.org/heritagedata/schemes/eh_tmc/concepts/100465">
		<skos:inScheme rdf:resource="http://purl.org/heritagedata/schemes/eh_tmc" />
		<dcterms:identifier>http://purl.org/heritagedata/schemes/eh_tmc/concepts/100465</dcterms:identifier>
		<skos:prefLabel xml:lang="en">SUBMARINE</skos:prefLabel>
		<dcterms:issued rdf:datatype="http://www.w3.org/2001/XMLSchema#dateTime">2013-07-17T09:01:43</dcterms:issued>
		<skos:altLabel xml:lang="en">G Class Submarine</skos:altLabel>
		<skos:altLabel xml:lang="en">J Class Submarine</skos:altLabel>
		<skos:altLabel xml:lang="en">A Class Submarine</skos:altLabel>
		<skos:altLabel xml:lang="en">B Class Submarine</skos:altLabel>
		<skos:altLabel xml:lang="en">C Class Submarine</skos:altLabel>
		<skos:narrower>
			<skos:Concept rdf:about="http://purl.org/heritagedata/schemes/eh_tmc/concepts/100344">
				<skos:inScheme rdf:resource="http://purl.org/heritagedata/schemes/eh_tmc" />
				<dcterms:identifier>http://purl.org/heritagedata/schemes/eh_tmc/concepts/100344</dcterms:identifier>
				<skos:prefLabel xml:lang="en">FLEET SUBMARINE</skos:prefLabel>
				<dcterms:issued rdf:datatype="http://www.w3.org/2001/XMLSchema#dateTime">2013-07-17T09:01:43</dcterms:issued>
				<skos:broader rdf:resource="http://purl.org/heritagedata/schemes/eh_tmc/concepts/100465" />
				<skos:scopeNote xml:lang="en">Large submarine intended to operate with a surface fleet at sea.</skos:scopeNote>
				<cc:license rdf:resource="http://creativecommons.org/licenses/by/3.0" />
				<cc:attributionURL rdf:resource="http://www.english-heritage.org.uk" />
				<cc:attributionName xml:lang="en">English Heritage</cc:attributionName>
				<dcterms:publisher rdf:resource="http://www.english-heritage.org.uk" />
			</skos:Concept>
		</skos:narrower>
		<skos:narrower>
			<skos:Concept rdf:about="http://purl.org/heritagedata/schemes/eh_tmc/concepts/100362">
				<skos:inScheme rdf:resource="http://purl.org/heritagedata/schemes/eh_tmc" />
				<dcterms:identifier>http://purl.org/heritagedata/schemes/eh_tmc/concepts/100362</dcterms:identifier>
				<skos:prefLabel xml:lang="en">HOLLAND SUBMARINE</skos:prefLabel>
				<dcterms:issued rdf:datatype="http://www.w3.org/2001/XMLSchema#dateTime">2013-07-17T09:01:43</dcterms:issued>
				<skos:broader rdf:resource="http://purl.org/heritagedata/schemes/eh_tmc/concepts/100465" />
				<skos:scopeNote xml:lang="en">First practical submarine design. The first to use a combination of battery power and internal combustion engines.</skos:scopeNote>
				<cc:license rdf:resource="http://creativecommons.org/licenses/by/3.0" />
				<cc:attributionURL rdf:resource="http://www.english-heritage.org.uk" />
				<cc:attributionName xml:lang="en">English Heritage</cc:attributionName>
				<dcterms:publisher rdf:resource="http://www.english-heritage.org.uk" />
			</skos:Concept>
		</skos:narrower>
		<skos:narrower>
			<skos:Concept rdf:about="http://purl.org/heritagedata/schemes/eh_tmc/concepts/100396">
				<skos:inScheme rdf:resource="http://purl.org/heritagedata/schemes/eh_tmc" />
				<dcterms:identifier>http://purl.org/heritagedata/schemes/eh_tmc/concepts/100396</dcterms:identifier>
				<skos:prefLabel xml:lang="en">MIDGET SUBMARINE</skos:prefLabel>
				<dcterms:issued rdf:datatype="http://www.w3.org/2001/XMLSchema#dateTime">2013-07-17T09:01:43</dcterms:issued>
				<skos:altLabel xml:lang="en">X Craft</skos:altLabel>
				<skos:broader rdf:resource="http://purl.org/heritagedata/schemes/eh_tmc/concepts/100465" />
				<skos:scopeNote xml:lang="en">Small submarine with a two or three man crew. Used for special missions such as sinking warships in heavily defended harbours.</skos:scopeNote>
				<cc:license rdf:resource="http://creativecommons.org/licenses/by/3.0" />
				<cc:attributionURL rdf:resource="http://www.english-heritage.org.uk" />
				<cc:attributionName xml:lang="en">English Heritage</cc:attributionName>
				<dcterms:publisher rdf:resource="http://www.english-heritage.org.uk" />
			</skos:Concept>
		</skos:narrower>
		<skos:narrower>
			<skos:Concept rdf:about="http://purl.org/heritagedata/schemes/eh_tmc/concepts/100398">
				<skos:inScheme rdf:resource="http://purl.org/heritagedata/schemes/eh_tmc" />
				<dcterms:identifier>http://purl.org/heritagedata/schemes/eh_tmc/concepts/100398</dcterms:identifier>
				<skos:prefLabel xml:lang="en">MINE LAYING SUBMARINE</skos:prefLabel>
				<dcterms:issued rdf:datatype="http://www.w3.org/2001/XMLSchema#dateTime">2013-07-17T09:01:43</dcterms:issued>
				<skos:broader rdf:resource="http://purl.org/heritagedata/schemes/eh_tmc/concepts/100465" />
				<skos:scopeNote xml:lang="en">A submarine built or adapted to carry mines and lay minefields.</skos:scopeNote>
				<cc:license rdf:resource="http://creativecommons.org/licenses/by/3.0" />
				<cc:attributionURL rdf:resource="http://www.english-heritage.org.uk" />
				<cc:attributionName xml:lang="en">English Heritage</cc:attributionName>
				<dcterms:publisher rdf:resource="http://www.english-heritage.org.uk" />
			</skos:Concept>
		</skos:narrower>
		<skos:narrower rdf:resource="http://purl.org/heritagedata/schemes/eh_tmc/concepts/100421" />
		<skos:broader rdf:resource="http://purl.org/heritagedata/schemes/eh_tmc/concepts/100490" />
		<skos:narrower rdf:resource="http://purl.org/heritagedata/schemes/eh_tmc/concepts/100466" />
		<skos:narrower rdf:resource="http://purl.org/heritagedata/schemes/eh_tmc/concepts/100487" />
		<skos:scopeNote xml:lang="en">A vessel designed to operate below the surface of the sea.</skos:scopeNote>
		<cc:license rdf:resource="http://creativecommons.org/licenses/by/3.0" />
		<cc:attributionURL rdf:resource="http://www.english-heritage.org.uk" />
		<cc:attributionName xml:lang="en">English Heritage</cc:attributionName>
		<dcterms:publisher rdf:resource="http://www.english-heritage.org.uk" />
	</skos:Concept>
	<skos:Concept rdf:about="http://purl.org/heritagedata/schemes/eh_tmc/concepts/100466">
		<skos:inScheme rdf:resource="http://purl.org/heritagedata/schemes/eh_tmc" />
		<dcterms:identifier>http://purl.org/heritagedata/schemes/eh_tmc/concepts/100466</dcterms:identifier>
		<skos:prefLabel xml:lang="en">SUBMARINE SEAPLANE CARRIER</skos:prefLabel>
		<dcterms:issued rdf:datatype="http://www.w3.org/2001/XMLSchema#dateTime">2013-07-17T09:01:43</dcterms:issued>
		<skos:broader rdf:resource="http://purl.org/heritagedata/schemes/eh_tmc/concepts/100465" />
		<skos:related rdf:resource="http://purl.org/heritagedata/schemes/eh_tmc/concepts/100260" />
		<skos:scopeNote xml:lang="en">British 'M' class submarine modified to carry and launch a small sea plane.</skos:scopeNote>
		<cc:license rdf:resource="http://creativecommons.org/licenses/by/3.0" />
		<cc:attributionURL rdf:resource="http://www.english-heritage.org.uk" />
		<cc:attributionName xml:lang="en">English Heritage</cc:attributionName>
		<dcterms:publisher rdf:resource="http://www.english-heritage.org.uk" />
	</skos:Concept>
	<skos:Concept rdf:about="http://purl.org/heritagedata/schemes/eh_tmc/concepts/100474">
		<skos:inScheme rdf:resource="http://purl.org/heritagedata/schemes/eh_tmc" />
		<dcterms:identifier>http://purl.org/heritagedata/schemes/eh_tmc/concepts/100474</dcterms:identifier>
		<skos:prefLabel xml:lang="en">TENDER</skos:prefLabel>
		<dcterms:issued rdf:datatype="http://www.w3.org/2001/XMLSchema#dateTime">2013-07-17T09:01:43</dcterms:issued>
		<skos:narrower>
			<skos:Concept rdf:about="http://purl.org/heritagedata/schemes/eh_tmc/concepts/160143">
				<skos:inScheme rdf:resource="http://purl.org/heritagedata/schemes/eh_tmc" />
				<dcterms:identifier>http://purl.org/heritagedata/schemes/eh_tmc/concepts/160143</dcterms:identifier>
				<skos:prefLabel xml:lang="en">BOMB SCOW</skos:prefLabel>
				<dcterms:issued rdf:datatype="http://www.w3.org/2001/XMLSchema#dateTime">2013-07-17T09:01:43</dcterms:issued>
				<skos:broader rdf:resource="http://purl.org/heritagedata/schemes/eh_tmc/concepts/100474" />
				<skos:scopeNote xml:lang="en">A vessel used to transport bombs and depth charges from the shore to flying boats during the Second World War.</skos:scopeNote>
				<cc:license rdf:resource="http://creativecommons.org/licenses/by/3.0" />
				<cc:attributionURL rdf:resource="http://www.english-heritage.org.uk" />
				<cc:attributionName xml:lang="en">English Heritage</cc:attributionName>
				<dcterms:publisher rdf:resource="http://www.english-heritage.org.uk" />
			</skos:Concept>
		</skos:narrower>
		<skos:narrower rdf:resource="http://purl.org/heritagedata/schemes/eh_tmc/concepts/160144" />
		<skos:broader rdf:resource="http://purl.org/heritagedata/schemes/eh_tmc/concepts/100410" />
		<skos:scopeNote xml:lang="en">A small vessel attached to a larger vessel (usually a warship) for general harbour duties such as taking crewmen ashore or fetching supplies.</skos:scopeNote>
		<cc:license rdf:resource="http://creativecommons.org/licenses/by/3.0" />
		<cc:attributionURL rdf:resource="http://www.english-heritage.org.uk" />
		<cc:attributionName xml:lang="en">English Heritage</cc:attributionName>
		<dcterms:publisher rdf:resource="http://www.english-heritage.org.uk" />
	</skos:Concept>
	<skos:Concept rdf:about="http://purl.org/heritagedata/schemes/eh_tmc/concepts/100479">
		<skos:inScheme rdf:resource="http://purl.org/heritagedata/schemes/eh_tmc" />
		<dcterms:identifier>http://purl.org/heritagedata/schemes/eh_tmc/concepts/100479</dcterms:identifier>
		<skos:prefLabel xml:lang="en">TRAINING SHIP</skos:prefLabel>
		<dcterms:issued rdf:datatype="http://www.w3.org/2001/XMLSchema#dateTime">2013-07-17T09:01:43</dcterms:issued>
		<skos:narrower>
			<skos:Concept rdf:about="http://purl.org/heritagedata/schemes/eh_tmc/concepts/100437">
				<skos:inScheme rdf:resource="http://purl.org/heritagedata/schemes/eh_tmc" />
				<dcterms:identifier>http://purl.org/heritagedata/schemes/eh_tmc/concepts/100437</dcterms:identifier>
				<skos:prefLabel xml:lang="en">REFORMATORY SHIP</skos:prefLabel>
				<dcterms:issued rdf:datatype="http://www.w3.org/2001/XMLSchema#dateTime">2013-07-17T09:01:43</dcterms:issued>
				<skos:broader rdf:resource="http://purl.org/heritagedata/schemes/eh_tmc/concepts/100479" />
				<skos:scopeNote xml:lang="en">A training ship to which boys who had committed petty crimes were sentenced for 4 to 5 years to be reformed and trained as sailors.</skos:scopeNote>
				<cc:license rdf:resource="http://creativecommons.org/licenses/by/3.0" />
				<cc:attributionURL rdf:resource="http://www.english-heritage.org.uk" />
				<cc:attributionName xml:lang="en">English Heritage</cc:attributionName>
				<dcterms:publisher rdf:resource="http://www.english-heritage.org.uk" />
			</skos:Concept>
		</skos:narrower>
		<skos:broader rdf:resource="http://purl.org/heritagedata/schemes/eh_tmc/concepts/100394" />
		<skos:scopeNote xml:lang="en">Vessels of various types used specifically for providing an initial training in seamanship.</skos:scopeNote>
		<cc:license rdf:resource="http://creativecommons.org/licenses/by/3.0" />
		<cc:attributionURL rdf:resource="http://www.english-heritage.org.uk" />
		<cc:attributionName xml:lang="en">English Heritage</cc:attributionName>
		<dcterms:publisher rdf:resource="http://www.english-heritage.org.uk" />
	</skos:Concept>
	<skos:Concept rdf:about="http://purl.org/heritagedata/schemes/eh_tmc/concepts/100480">
		<skos:inScheme rdf:resource="http://purl.org/heritagedata/schemes/eh_tmc" />
		<dcterms:identifier>http://purl.org/heritagedata/schemes/eh_tmc/concepts/100480</dcterms:identifier>
		<skos:prefLabel xml:lang="en">TRANSPORT VESSEL</skos:prefLabel>
		<dcterms:issued rdf:datatype="http://www.w3.org/2001/XMLSchema#dateTime">2013-07-17T09:01:43</dcterms:issued>
		<skos:narrower rdf:resource="http://purl.org/heritagedata/schemes/eh_tmc/concepts/100295" />
		<skos:narrower>
			<skos:Concept rdf:about="http://purl.org/heritagedata/schemes/eh_tmc/concepts/147329">
				<skos:inScheme rdf:resource="http://purl.org/heritagedata/schemes/eh_tmc" />
				<dcterms:identifier>http://purl.org/heritagedata/schemes/eh_tmc/concepts/147329</dcterms:identifier>
				<skos:prefLabel xml:lang="en">CARTEL</skos:prefLabel>
				<dcterms:issued rdf:datatype="http://www.w3.org/2001/XMLSchema#dateTime">2013-07-17T09:01:43</dcterms:issued>
				<skos:broader rdf:resource="http://purl.org/heritagedata/schemes/eh_tmc/concepts/100480" />
				<skos:scopeNote xml:lang="en">Transport vessel, usually a hired vessel of mercantile origin, used for the exchange of prisoners-of-war; sometimes, specifically a hospital ship with such prisoners.</skos:scopeNote>
				<cc:license rdf:resource="http://creativecommons.org/licenses/by/3.0" />
				<cc:attributionURL rdf:resource="http://www.english-heritage.org.uk" />
				<cc:attributionName xml:lang="en">English Heritage</cc:attributionName>
				<dcterms:publisher rdf:resource="http://www.english-heritage.org.uk" />
			</skos:Concept>
		</skos:narrower>
		<skos:narrower rdf:resource="http://purl.org/heritagedata/schemes/eh_tmc/concepts/141858" />
		<skos:narrower>
			<skos:Concept rdf:about="http://purl.org/heritagedata/schemes/eh_tmc/concepts/147328">
				<skos:inScheme rdf:resource="http://purl.org/heritagedata/schemes/eh_tmc" />
				<dcterms:identifier>http://purl.org/heritagedata/schemes/eh_tmc/concepts/147328</dcterms:identifier>
				<skos:prefLabel xml:lang="en">CONVICT TRANSPORT</skos:prefLabel>
				<dcterms:issued rdf:datatype="http://www.w3.org/2001/XMLSchema#dateTime">2013-07-17T09:01:43</dcterms:issued>
				<skos:broader rdf:resource="http://purl.org/heritagedata/schemes/eh_tmc/concepts/100480" />
				<skos:scopeNote xml:lang="en">Transport vessel hired for the enforced removal of convicts to penal colonies abroad(e.g. Virginia, Australia), or for their return to Britain.</skos:scopeNote>
				<cc:license rdf:resource="http://creativecommons.org/licenses/by/3.0" />
				<cc:attributionURL rdf:resource="http://www.english-heritage.org.uk" />
				<cc:attributionName xml:lang="en">English Heritage</cc:attributionName>
				<dcterms:publisher rdf:resource="http://www.english-heritage.org.uk" />
			</skos:Concept>
		</skos:narrower>
		<skos:narrower>
			<skos:Concept rdf:about="http://purl.org/heritagedata/schemes/eh_tmc/concepts/152405">
				<skos:inScheme rdf:resource="http://purl.org/heritagedata/schemes/eh_tmc" />
				<dcterms:identifier>http://purl.org/heritagedata/schemes/eh_tmc/concepts/152405</dcterms:identifier>
				<skos:prefLabel xml:lang="en">PLATFORM SUPPLY VESSEL</skos:prefLabel>
				<dcterms:issued rdf:datatype="http://www.w3.org/2001/XMLSchema#dateTime">2013-07-17T09:01:43</dcterms:issued>
				<skos:altLabel xml:lang="en">Offshore Supply Vessel</skos:altLabel>
				<skos:broader rdf:resource="http://purl.org/heritagedata/schemes/eh_tmc/concepts/100480" />
				<skos:scopeNote xml:lang="en">Specially designed/fitted carriers of crew and/or supplies to offshore oil platforms.</skos:scopeNote>
				<cc:license rdf:resource="http://creativecommons.org/licenses/by/3.0" />
				<cc:attributionURL rdf:resource="http://www.english-heritage.org.uk" />
				<cc:attributionName xml:lang="en">English Heritage</cc:attributionName>
				<dcterms:publisher rdf:resource="http://www.english-heritage.org.uk" />
			</skos:Concept>
		</skos:narrower>
		<skos:broader rdf:resource="http://purl.org/heritagedata/schemes/eh_tmc/concepts/100394" />
		<skos:scopeNote xml:lang="en">A vessel used for transporting passengers or goods.</skos:scopeNote>
		<cc:license rdf:resource="http://creativecommons.org/licenses/by/3.0" />
		<cc:attributionURL rdf:resource="http://www.english-heritage.org.uk" />
		<cc:attributionName xml:lang="en">English Heritage</cc:attributionName>
		<dcterms:publisher rdf:resource="http://www.english-heritage.org.uk" />
	</skos:Concept>
	<skos:Concept rdf:about="http://purl.org/heritagedata/schemes/eh_tmc/concepts/100482">
		<skos:inScheme rdf:resource="http://purl.org/heritagedata/schemes/eh_tmc" />
		<dcterms:identifier>http://purl.org/heritagedata/schemes/eh_tmc/concepts/100482</dcterms:identifier>
		<skos:prefLabel xml:lang="en">TRINITY HOUSE VESSEL</skos:prefLabel>
		<dcterms:issued rdf:datatype="http://www.w3.org/2001/XMLSchema#dateTime">2013-07-17T09:01:43</dcterms:issued>
		<skos:narrower>
			<skos:Concept rdf:about="http://purl.org/heritagedata/schemes/eh_tmc/concepts/100388">
				<skos:inScheme rdf:resource="http://purl.org/heritagedata/schemes/eh_tmc" />
				<dcterms:identifier>http://purl.org/heritagedata/schemes/eh_tmc/concepts/100388</dcterms:identifier>
				<skos:prefLabel xml:lang="en">LIGHTSHIP</skos:prefLabel>
				<dcterms:issued rdf:datatype="http://www.w3.org/2001/XMLSchema#dateTime">2013-07-17T09:01:43</dcterms:issued>
				<skos:broader rdf:resource="http://purl.org/heritagedata/schemes/eh_tmc/concepts/100482" />
				<skos:scopeNote xml:lang="en">Normally an unpowered vessel, moored in places where the construction of a lighthouse is impractical.</skos:scopeNote>
				<cc:license rdf:resource="http://creativecommons.org/licenses/by/3.0" />
				<cc:attributionURL rdf:resource="http://www.english-heritage.org.uk" />
				<cc:attributionName xml:lang="en">English Heritage</cc:attributionName>
				<dcterms:publisher rdf:resource="http://www.english-heritage.org.uk" />
			</skos:Concept>
		</skos:narrower>
		<skos:broader rdf:resource="http://purl.org/heritagedata/schemes/eh_tmc/concepts/100394" />
		<skos:scopeNote xml:lang="en">Any vessel operated by Trinity house masters and brethren in the maintenance of lighthouses, lightships, buoys and other navigation aids.</skos:scopeNote>
		<cc:license rdf:resource="http://creativecommons.org/licenses/by/3.0" />
		<cc:attributionURL rdf:resource="http://www.english-heritage.org.uk" />
		<cc:attributionName xml:lang="en">English Heritage</cc:attributionName>
		<dcterms:publisher rdf:resource="http://www.english-heritage.org.uk" />
	</skos:Concept>
	<skos:Concept rdf:about="http://purl.org/heritagedata/schemes/eh_tmc/concepts/100483">
		<skos:inScheme rdf:resource="http://purl.org/heritagedata/schemes/eh_tmc" />
		<dcterms:identifier>http://purl.org/heritagedata/schemes/eh_tmc/concepts/100483</dcterms:identifier>
		<skos:prefLabel xml:lang="en">TROOP SHIP</skos:prefLabel>
		<dcterms:issued rdf:datatype="http://www.w3.org/2001/XMLSchema#dateTime">2013-07-17T09:01:43</dcterms:issued>
		<skos:broader rdf:resource="http://purl.org/heritagedata/schemes/eh_tmc/concepts/100419" />
		<skos:broader rdf:resource="http://purl.org/heritagedata/schemes/eh_tmc/concepts/100410" />
		<skos:scopeNote xml:lang="en">A vessel used for the transport of troops, either during wartime or for garrison duties in peacetime.</skos:scopeNote>
		<cc:license rdf:resource="http://creativecommons.org/licenses/by/3.0" />
		<cc:attributionURL rdf:resource="http://www.english-heritage.org.uk" />
		<cc:attributionName xml:lang="en">English Heritage</cc:attributionName>
		<dcterms:publisher rdf:resource="http://www.english-heritage.org.uk" />
	</skos:Concept>
	<skos:Concept rdf:about="http://purl.org/heritagedata/schemes/eh_tmc/concepts/100485">
		<skos:inScheme rdf:resource="http://purl.org/heritagedata/schemes/eh_tmc" />
		<dcterms:identifier>http://purl.org/heritagedata/schemes/eh_tmc/concepts/100485</dcterms:identifier>
		<skos:prefLabel xml:lang="en">TUG</skos:prefLabel>
		<dcterms:issued rdf:datatype="http://www.w3.org/2001/XMLSchema#dateTime">2013-07-17T09:01:43</dcterms:issued>
		<skos:altLabel xml:lang="en">Admiralty Tug</skos:altLabel>
		<skos:narrower rdf:resource="http://purl.org/heritagedata/schemes/eh_tmc/concepts/100337" />
		<skos:narrower rdf:resource="http://purl.org/heritagedata/schemes/eh_tmc/concepts/100438" />
		<skos:narrower rdf:resource="http://purl.org/heritagedata/schemes/eh_tmc/concepts/100445" />
		<skos:broader rdf:resource="http://purl.org/heritagedata/schemes/eh_tmc/concepts/100394" />
		<skos:broader rdf:resource="http://purl.org/heritagedata/schemes/eh_tmc/concepts/100361" />
		<skos:scopeNote xml:lang="en">A relatively small and heavily built vessel equipped with large engines. Used for towing ships at sea or manouevring them in tight spaces.</skos:scopeNote>
		<cc:license rdf:resource="http://creativecommons.org/licenses/by/3.0" />
		<cc:attributionURL rdf:resource="http://www.english-heritage.org.uk" />
		<cc:attributionName xml:lang="en">English Heritage</cc:attributionName>
		<dcterms:publisher rdf:resource="http://www.english-heritage.org.uk" />
	</skos:Concept>
	<skos:Concept rdf:about="http://purl.org/heritagedata/schemes/eh_tmc/concepts/100487">
		<skos:inScheme rdf:resource="http://purl.org/heritagedata/schemes/eh_tmc" />
		<dcterms:identifier>http://purl.org/heritagedata/schemes/eh_tmc/concepts/100487</dcterms:identifier>
		<skos:prefLabel xml:lang="en">U BOAT</skos:prefLabel>
		<dcterms:issued rdf:datatype="http://www.w3.org/2001/XMLSchema#dateTime">2013-07-17T09:01:43</dcterms:issued>
		<skos:altLabel xml:lang="en">U Boot</skos:altLabel>
		<skos:altLabel xml:lang="en">Unterseeboot</skos:altLabel>
		<skos:broader rdf:resource="http://purl.org/heritagedata/schemes/eh_tmc/concepts/100465" />
		<skos:narrower>
			<skos:Concept rdf:about="http://purl.org/heritagedata/schemes/eh_tmc/concepts/162696">
				<skos:inScheme rdf:resource="http://purl.org/heritagedata/schemes/eh_tmc" />
				<dcterms:identifier>http://purl.org/heritagedata/schemes/eh_tmc/concepts/162696</dcterms:identifier>
				<skos:prefLabel xml:lang="en">U BOAT (TYPE UBIII)</skos:prefLabel>
				<dcterms:issued rdf:datatype="http://www.w3.org/2001/XMLSchema#dateTime">2013-07-17T09:01:43</dcterms:issued>
				<skos:altLabel xml:lang="en">Type Ubiii Submarine</skos:altLabel>
				<skos:broader rdf:resource="http://purl.org/heritagedata/schemes/eh_tmc/concepts/100487" />
				<skos:scopeNote xml:lang="en">A German coastal attack submarine in use during the First World War. The U Boat had 5 torpedo tubes (4 bow/1 stern) and carried 10 torpedoes as well as an 88mm (or in some cases 105mm) deck gun.</skos:scopeNote>
				<cc:license rdf:resource="http://creativecommons.org/licenses/by/3.0" />
				<cc:attributionURL rdf:resource="http://www.english-heritage.org.uk" />
				<cc:attributionName xml:lang="en">English Heritage</cc:attributionName>
				<dcterms:publisher rdf:resource="http://www.english-heritage.org.uk" />
			</skos:Concept>
		</skos:narrower>
		<skos:narrower>
			<skos:Concept rdf:about="http://purl.org/heritagedata/schemes/eh_tmc/concepts/162694">
				<skos:inScheme rdf:resource="http://purl.org/heritagedata/schemes/eh_tmc" />
				<dcterms:identifier>http://purl.org/heritagedata/schemes/eh_tmc/concepts/162694</dcterms:identifier>
				<skos:prefLabel xml:lang="en">U BOAT (TYPE UCI)</skos:prefLabel>
				<dcterms:issued rdf:datatype="http://www.w3.org/2001/XMLSchema#dateTime">2013-07-17T09:01:43</dcterms:issued>
				<skos:altLabel xml:lang="en">Type Uci Submarine</skos:altLabel>
				<skos:broader rdf:resource="http://purl.org/heritagedata/schemes/eh_tmc/concepts/100487" />
				<skos:scopeNote xml:lang="en">A German coastal minelaying submarine in use during the First World War. The U Boat carried 12 mines but was otherwise unarmed with no deck gun or torpedo tubes.</skos:scopeNote>
				<cc:license rdf:resource="http://creativecommons.org/licenses/by/3.0" />
				<cc:attributionURL rdf:resource="http://www.english-heritage.org.uk" />
				<cc:attributionName xml:lang="en">English Heritage</cc:attributionName>
				<dcterms:publisher rdf:resource="http://www.english-heritage.org.uk" />
			</skos:Concept>
		</skos:narrower>
		<skos:narrower>
			<skos:Concept rdf:about="http://purl.org/heritagedata/schemes/eh_tmc/concepts/162698">
				<skos:inScheme rdf:resource="http://purl.org/heritagedata/schemes/eh_tmc" />
				<dcterms:identifier>http://purl.org/heritagedata/schemes/eh_tmc/concepts/162698</dcterms:identifier>
				<skos:prefLabel xml:lang="en">U BOAT (TYPE UCII)</skos:prefLabel>
				<dcterms:issued rdf:datatype="http://www.w3.org/2001/XMLSchema#dateTime">2013-07-17T09:01:43</dcterms:issued>
				<skos:altLabel xml:lang="en">Type Ucii Submarine</skos:altLabel>
				<skos:broader rdf:resource="http://purl.org/heritagedata/schemes/eh_tmc/concepts/100487" />
				<skos:scopeNote xml:lang="en">A German coastal minelaying submarine in use during the First World War. In addition to 18 mines, the U BOAT also carried 7 torpedoes in 3 tubes (2 bow/1 stern) and and 88mm or 105mm deck gun. A very successful design, UCIIs sank more than 1800 vessels.</skos:scopeNote>
				<cc:license rdf:resource="http://creativecommons.org/licenses/by/3.0" />
				<cc:attributionURL rdf:resource="http://www.english-heritage.org.uk" />
				<cc:attributionName xml:lang="en">English Heritage</cc:attributionName>
				<dcterms:publisher rdf:resource="http://www.english-heritage.org.uk" />
			</skos:Concept>
		</skos:narrower>
		<skos:scopeNote xml:lang="en">The British designation for any German submarine built for military purposes. U-Boat is an anglicization of the German U-Boot, an abbreviation for Unterseeboot (Undersea Boat). In German U-Boot refers to any submarine.</skos:scopeNote>
		<cc:license rdf:resource="http://creativecommons.org/licenses/by/3.0" />
		<cc:attributionURL rdf:resource="http://www.english-heritage.org.uk" />
		<cc:attributionName xml:lang="en">English Heritage</cc:attributionName>
		<dcterms:publisher rdf:resource="http://www.english-heritage.org.uk" />
	</skos:Concept>
	<skos:Concept rdf:about="http://purl.org/heritagedata/schemes/eh_tmc/concepts/100490">
		<skos:inScheme rdf:resource="http://purl.org/heritagedata/schemes/eh_tmc" />
		<dcterms:identifier>http://purl.org/heritagedata/schemes/eh_tmc/concepts/100490</dcterms:identifier>
		<skos:prefLabel xml:lang="en">WARSHIP</skos:prefLabel>
		<dcterms:issued rdf:datatype="http://www.w3.org/2001/XMLSchema#dateTime">2013-07-17T09:01:43</dcterms:issued>
		<skos:altLabel xml:lang="en">Man Of War</skos:altLabel>
		<skos:narrower rdf:resource="http://purl.org/heritagedata/schemes/eh_tmc/concepts/100259" />
		<skos:narrower>
			<skos:Concept rdf:about="http://purl.org/heritagedata/schemes/eh_tmc/concepts/100262">
				<skos:inScheme rdf:resource="http://purl.org/heritagedata/schemes/eh_tmc" />
				<dcterms:identifier>http://purl.org/heritagedata/schemes/eh_tmc/concepts/100262</dcterms:identifier>
				<skos:prefLabel xml:lang="en">ANTI AIRCRAFT VESSEL</skos:prefLabel>
				<dcterms:issued rdf:datatype="http://www.w3.org/2001/XMLSchema#dateTime">2013-07-17T09:01:43</dcterms:issued>
				<skos:broader rdf:resource="http://purl.org/heritagedata/schemes/eh_tmc/concepts/100490" />
				<skos:scopeNote xml:lang="en">A vessel (often small obsolete cruisers or pleasure steamers) equipped with batteries of anti aircraft guns as its main armament.</skos:scopeNote>
				<cc:license rdf:resource="http://creativecommons.org/licenses/by/3.0" />
				<cc:attributionURL rdf:resource="http://www.english-heritage.org.uk" />
				<cc:attributionName xml:lang="en">English Heritage</cc:attributionName>
				<dcterms:publisher rdf:resource="http://www.english-heritage.org.uk" />
			</skos:Concept>
		</skos:narrower>
		<skos:narrower>
			<skos:Concept rdf:about="http://purl.org/heritagedata/schemes/eh_tmc/concepts/100277">
				<skos:inScheme rdf:resource="http://purl.org/heritagedata/schemes/eh_tmc" />
				<dcterms:identifier>http://purl.org/heritagedata/schemes/eh_tmc/concepts/100277</dcterms:identifier>
				<skos:prefLabel xml:lang="en">BATTLECRUISER</skos:prefLabel>
				<dcterms:issued rdf:datatype="http://www.w3.org/2001/XMLSchema#dateTime">2013-07-17T09:01:43</dcterms:issued>
				<skos:broader rdf:resource="http://purl.org/heritagedata/schemes/eh_tmc/concepts/100490" />
				<skos:scopeNote xml:lang="en">A capital warship lightly armoured but with the same gun armament and stem turbine propulsion as a DREADNOUGHT BATTLESHIP.</skos:scopeNote>
				<cc:license rdf:resource="http://creativecommons.org/licenses/by/3.0" />
				<cc:attributionURL rdf:resource="http://www.english-heritage.org.uk" />
				<cc:attributionName xml:lang="en">English Heritage</cc:attributionName>
				<dcterms:publisher rdf:resource="http://www.english-heritage.org.uk" />
			</skos:Concept>
		</skos:narrower>
		<skos:narrower rdf:resource="http://purl.org/heritagedata/schemes/eh_tmc/concepts/100278" />
		<skos:narrower rdf:resource="http://purl.org/heritagedata/schemes/eh_tmc/concepts/100311" />
		<skos:narrower rdf:resource="http://purl.org/heritagedata/schemes/eh_tmc/concepts/100319" />
		<skos:narrower rdf:resource="http://purl.org/heritagedata/schemes/eh_tmc/concepts/100331" />
		<skos:narrower>
			<skos:Concept rdf:about="http://purl.org/heritagedata/schemes/eh_tmc/concepts/100339">
				<skos:inScheme rdf:resource="http://purl.org/heritagedata/schemes/eh_tmc" />
				<dcterms:identifier>http://purl.org/heritagedata/schemes/eh_tmc/concepts/100339</dcterms:identifier>
				<skos:prefLabel xml:lang="en">FIRESHIP</skos:prefLabel>
				<dcterms:issued rdf:datatype="http://www.w3.org/2001/XMLSchema#dateTime">2013-07-17T09:01:43</dcterms:issued>
				<skos:broader rdf:resource="http://purl.org/heritagedata/schemes/eh_tmc/concepts/100490" />
				<skos:scopeNote xml:lang="en">A small vessel used to attack other vessels and setting themselves and then the enemy alight.</skos:scopeNote>
				<cc:license rdf:resource="http://creativecommons.org/licenses/by/3.0" />
				<cc:attributionURL rdf:resource="http://www.english-heritage.org.uk" />
				<cc:attributionName xml:lang="en">English Heritage</cc:attributionName>
				<dcterms:publisher rdf:resource="http://www.english-heritage.org.uk" />
			</skos:Concept>
		</skos:narrower>
		<skos:narrower>
			<skos:Concept rdf:about="http://purl.org/heritagedata/schemes/eh_tmc/concepts/100345">
				<skos:inScheme rdf:resource="http://purl.org/heritagedata/schemes/eh_tmc" />
				<dcterms:identifier>http://purl.org/heritagedata/schemes/eh_tmc/concepts/100345</dcterms:identifier>
				<skos:prefLabel xml:lang="en">FLOATING BATTERY</skos:prefLabel>
				<dcterms:issued rdf:datatype="http://www.w3.org/2001/XMLSchema#dateTime">2013-07-17T09:01:43</dcterms:issued>
				<skos:broader rdf:resource="http://purl.org/heritagedata/schemes/eh_tmc/concepts/100490" />
				<skos:scopeNote xml:lang="en">A small stem powered warship with its hull protected by iron plates. Used to bombard targets onshore, especially in the Crimean War.</skos:scopeNote>
				<cc:license rdf:resource="http://creativecommons.org/licenses/by/3.0" />
				<cc:attributionURL rdf:resource="http://www.english-heritage.org.uk" />
				<cc:attributionName xml:lang="en">English Heritage</cc:attributionName>
				<dcterms:publisher rdf:resource="http://www.english-heritage.org.uk" />
			</skos:Concept>
		</skos:narrower>
		<skos:narrower>
			<skos:Concept rdf:about="http://purl.org/heritagedata/schemes/eh_tmc/concepts/141856">
				<skos:inScheme rdf:resource="http://purl.org/heritagedata/schemes/eh_tmc" />
				<dcterms:identifier>http://purl.org/heritagedata/schemes/eh_tmc/concepts/141856</dcterms:identifier>
				<skos:prefLabel xml:lang="en">FLUTE</skos:prefLabel>
				<dcterms:issued rdf:datatype="http://www.w3.org/2001/XMLSchema#dateTime">2013-07-17T09:01:43</dcterms:issued>
				<skos:broader rdf:resource="http://purl.org/heritagedata/schemes/eh_tmc/concepts/100490" />
				<skos:scopeNote xml:lang="en">French warship broadly equivalent to the English 4th to 6th Rates, with as few as 4 to as many as 50 guns.</skos:scopeNote>
				<cc:license rdf:resource="http://creativecommons.org/licenses/by/3.0" />
				<cc:attributionURL rdf:resource="http://www.english-heritage.org.uk" />
				<cc:attributionName xml:lang="en">English Heritage</cc:attributionName>
				<dcterms:publisher rdf:resource="http://www.english-heritage.org.uk" />
			</skos:Concept>
		</skos:narrower>
		<skos:narrower rdf:resource="http://purl.org/heritagedata/schemes/eh_tmc/concepts/100359" />
		<skos:narrower rdf:resource="http://purl.org/heritagedata/schemes/eh_tmc/concepts/100372" />
		<skos:narrower rdf:resource="http://purl.org/heritagedata/schemes/eh_tmc/concepts/100377" />
		<skos:narrower>
			<skos:Concept rdf:about="http://purl.org/heritagedata/schemes/eh_tmc/concepts/100380">
				<skos:inScheme rdf:resource="http://purl.org/heritagedata/schemes/eh_tmc" />
				<dcterms:identifier>http://purl.org/heritagedata/schemes/eh_tmc/concepts/100380</dcterms:identifier>
				<skos:prefLabel xml:lang="en">LANDING SHIP TANK</skos:prefLabel>
				<dcterms:issued rdf:datatype="http://www.w3.org/2001/XMLSchema#dateTime">2013-07-17T09:01:43</dcterms:issued>
				<skos:broader rdf:resource="http://purl.org/heritagedata/schemes/eh_tmc/concepts/100490" />
				<skos:scopeNote xml:lang="en">Small ocean going vessel fitted with loading doors in the bow. Used for ferrying tanks or other fighting vehicles to beach landings.</skos:scopeNote>
				<cc:license rdf:resource="http://creativecommons.org/licenses/by/3.0" />
				<cc:attributionURL rdf:resource="http://www.english-heritage.org.uk" />
				<cc:attributionName xml:lang="en">English Heritage</cc:attributionName>
				<dcterms:publisher rdf:resource="http://www.english-heritage.org.uk" />
			</skos:Concept>
		</skos:narrower>
		<skos:narrower rdf:resource="http://purl.org/heritagedata/schemes/eh_tmc/concepts/146425" />
		<skos:narrower rdf:resource="http://purl.org/heritagedata/schemes/eh_tmc/concepts/160147" />
		<skos:narrower>
			<skos:Concept rdf:about="http://purl.org/heritagedata/schemes/eh_tmc/concepts/100400">
				<skos:inScheme rdf:resource="http://purl.org/heritagedata/schemes/eh_tmc" />
				<dcterms:identifier>http://purl.org/heritagedata/schemes/eh_tmc/concepts/100400</dcterms:identifier>
				<skos:prefLabel xml:lang="en">MINELAYER</skos:prefLabel>
				<dcterms:issued rdf:datatype="http://www.w3.org/2001/XMLSchema#dateTime">2013-07-17T09:01:43</dcterms:issued>
				<skos:broader rdf:resource="http://purl.org/heritagedata/schemes/eh_tmc/concepts/100490" />
				<skos:scopeNote xml:lang="en">A ship designed or modified to carry large numbers of mines and be able to lay them as a minefield.</skos:scopeNote>
				<cc:license rdf:resource="http://creativecommons.org/licenses/by/3.0" />
				<cc:attributionURL rdf:resource="http://www.english-heritage.org.uk" />
				<cc:attributionName xml:lang="en">English Heritage</cc:attributionName>
				<dcterms:publisher rdf:resource="http://www.english-heritage.org.uk" />
			</skos:Concept>
		</skos:narrower>
		<skos:narrower rdf:resource="http://purl.org/heritagedata/schemes/eh_tmc/concepts/100406" />
		<skos:narrower>
			<skos:Concept rdf:about="http://purl.org/heritagedata/schemes/eh_tmc/concepts/100411">
				<skos:inScheme rdf:resource="http://purl.org/heritagedata/schemes/eh_tmc" />
				<dcterms:identifier>http://purl.org/heritagedata/schemes/eh_tmc/concepts/100411</dcterms:identifier>
				<skos:prefLabel xml:lang="en">NET LAYER</skos:prefLabel>
				<dcterms:issued rdf:datatype="http://www.w3.org/2001/XMLSchema#dateTime">2013-07-17T09:01:43</dcterms:issued>
				<skos:altLabel xml:lang="en">Admiralty Netlayer</skos:altLabel>
				<skos:broader rdf:resource="http://purl.org/heritagedata/schemes/eh_tmc/concepts/100490" />
				<skos:scopeNote xml:lang="en">Small vessel built or adapted to lay and recover anti submarine nets in harbours and anchorages.</skos:scopeNote>
				<cc:license rdf:resource="http://creativecommons.org/licenses/by/3.0" />
				<cc:attributionURL rdf:resource="http://www.english-heritage.org.uk" />
				<cc:attributionName xml:lang="en">English Heritage</cc:attributionName>
				<dcterms:publisher rdf:resource="http://www.english-heritage.org.uk" />
			</skos:Concept>
		</skos:narrower>
		<skos:narrower rdf:resource="http://purl.org/heritagedata/schemes/eh_tmc/concepts/100455" />
		<skos:narrower>
			<skos:Concept rdf:about="http://purl.org/heritagedata/schemes/eh_tmc/concepts/100457">
				<skos:inScheme rdf:resource="http://purl.org/heritagedata/schemes/eh_tmc" />
				<dcterms:identifier>http://purl.org/heritagedata/schemes/eh_tmc/concepts/100457</dcterms:identifier>
				<skos:prefLabel xml:lang="en">SLOOP OF WAR</skos:prefLabel>
				<dcterms:issued rdf:datatype="http://www.w3.org/2001/XMLSchema#dateTime">2013-07-17T09:01:43</dcterms:issued>
				<skos:altLabel xml:lang="en">Cherokee Class Sloop</skos:altLabel>
				<skos:broader rdf:resource="http://purl.org/heritagedata/schemes/eh_tmc/concepts/100490" />
				<skos:scopeNote xml:lang="en">Any small rigged warship below the sailing classification of frigate.</skos:scopeNote>
				<cc:license rdf:resource="http://creativecommons.org/licenses/by/3.0" />
				<cc:attributionURL rdf:resource="http://www.english-heritage.org.uk" />
				<cc:attributionName xml:lang="en">English Heritage</cc:attributionName>
				<dcterms:publisher rdf:resource="http://www.english-heritage.org.uk" />
			</skos:Concept>
		</skos:narrower>
		<skos:narrower rdf:resource="http://purl.org/heritagedata/schemes/eh_tmc/concepts/100465" />
		<skos:broader rdf:resource="http://purl.org/heritagedata/schemes/eh_tmc/concepts/100394" />
		<skos:scopeNote xml:lang="en">A ship that is built and primarily intended for war.</skos:scopeNote>
		<cc:license rdf:resource="http://creativecommons.org/licenses/by/3.0" />
		<cc:attributionURL rdf:resource="http://www.english-heritage.org.uk" />
		<cc:attributionName xml:lang="en">English Heritage</cc:attributionName>
		<dcterms:publisher rdf:resource="http://www.english-heritage.org.uk" />
	</skos:Concept>
	<skos:Concept rdf:about="http://purl.org/heritagedata/schemes/eh_tmc/concepts/100497">
		<skos:inScheme rdf:resource="http://purl.org/heritagedata/schemes/eh_tmc" />
		<dcterms:identifier>http://purl.org/heritagedata/schemes/eh_tmc/concepts/100497</dcterms:identifier>
		<skos:prefLabel xml:lang="en">WHALER</skos:prefLabel>
		<dcterms:issued rdf:datatype="http://www.w3.org/2001/XMLSchema#dateTime">2013-07-17T09:01:43</dcterms:issued>
		<skos:altLabel xml:lang="en">Admiralty Whaler</skos:altLabel>
		<skos:narrower>
			<skos:Concept rdf:about="http://purl.org/heritagedata/schemes/eh_tmc/concepts/100494">
				<skos:inScheme rdf:resource="http://purl.org/heritagedata/schemes/eh_tmc" />
				<dcterms:identifier>http://purl.org/heritagedata/schemes/eh_tmc/concepts/100494</dcterms:identifier>
				<skos:prefLabel xml:lang="en">WHALE CATCHER</skos:prefLabel>
				<dcterms:issued rdf:datatype="http://www.w3.org/2001/XMLSchema#dateTime">2013-07-17T09:01:43</dcterms:issued>
				<skos:broader rdf:resource="http://purl.org/heritagedata/schemes/eh_tmc/concepts/100497" />
				<skos:scopeNote xml:lang="en">A craft employed to harpoon whales and bring them in to be processed.</skos:scopeNote>
				<cc:license rdf:resource="http://creativecommons.org/licenses/by/3.0" />
				<cc:attributionURL rdf:resource="http://www.english-heritage.org.uk" />
				<cc:attributionName xml:lang="en">English Heritage</cc:attributionName>
				<dcterms:publisher rdf:resource="http://www.english-heritage.org.uk" />
			</skos:Concept>
		</skos:narrower>
		<skos:broader rdf:resource="http://purl.org/heritagedata/schemes/eh_tmc/concepts/100342" />
		<skos:scopeNote xml:lang="en">Any vessel involved in the catching or transportation of whales.</skos:scopeNote>
		<cc:license rdf:resource="http://creativecommons.org/licenses/by/3.0" />
		<cc:attributionURL rdf:resource="http://www.english-heritage.org.uk" />
		<cc:attributionName xml:lang="en">English Heritage</cc:attributionName>
		<dcterms:publisher rdf:resource="http://www.english-heritage.org.uk" />
	</skos:Concept>
	<skos:Concept rdf:about="http://purl.org/heritagedata/schemes/eh_tmc/concepts/100499">
		<skos:inScheme rdf:resource="http://purl.org/heritagedata/schemes/eh_tmc" />
		<dcterms:identifier>http://purl.org/heritagedata/schemes/eh_tmc/concepts/100499</dcterms:identifier>
		<skos:prefLabel xml:lang="en">YACHT</skos:prefLabel>
		<dcterms:issued rdf:datatype="http://www.w3.org/2001/XMLSchema#dateTime">2013-07-17T09:01:43</dcterms:issued>
		<skos:broader rdf:resource="http://purl.org/heritagedata/schemes/eh_tmc/concepts/100382" />
		<skos:broader rdf:resource="http://purl.org/heritagedata/schemes/eh_tmc/concepts/100443" />
		<skos:scopeNote xml:lang="en">Any vessel propelled by sail or power and used for pleasure and not plying for hire.</skos:scopeNote>
		<cc:license rdf:resource="http://creativecommons.org/licenses/by/3.0" />
		<cc:attributionURL rdf:resource="http://www.english-heritage.org.uk" />
		<cc:attributionName xml:lang="en">English Heritage</cc:attributionName>
		<dcterms:publisher rdf:resource="http://www.english-heritage.org.uk" />
	</skos:Concept>
	<skos:Concept rdf:about="http://purl.org/heritagedata/schemes/eh_tmc/concepts/100259">
		<skos:inScheme rdf:resource="http://purl.org/heritagedata/schemes/eh_tmc" />
		<dcterms:identifier>http://purl.org/heritagedata/schemes/eh_tmc/concepts/100259</dcterms:identifier>
		<skos:prefLabel xml:lang="en">AIRCRAFT CARRIER</skos:prefLabel>
		<dcterms:issued rdf:datatype="http://www.w3.org/2001/XMLSchema#dateTime">2013-07-17T09:01:43</dcterms:issued>
		<skos:broader rdf:resource="http://purl.org/heritagedata/schemes/eh_tmc/concepts/100490" />
		<skos:related rdf:resource="http://purl.org/heritagedata/schemes/eh_tmc/concepts/100260" />
		<skos:scopeNote xml:lang="en">A major warship equipped with a clear flat deck to provide a landing and taking off place for aircraft.</skos:scopeNote>
		<cc:license rdf:resource="http://creativecommons.org/licenses/by/3.0" />
		<cc:attributionURL rdf:resource="http://www.english-heritage.org.uk" />
		<cc:attributionName xml:lang="en">English Heritage</cc:attributionName>
		<dcterms:publisher rdf:resource="http://www.english-heritage.org.uk" />
	</skos:Concept>
	<skos:Concept rdf:about="http://purl.org/heritagedata/schemes/eh_tmc/concepts/100260">
		<skos:inScheme rdf:resource="http://purl.org/heritagedata/schemes/eh_tmc" />
		<dcterms:identifier>http://purl.org/heritagedata/schemes/eh_tmc/concepts/100260</dcterms:identifier>
		<skos:prefLabel xml:lang="en">AIRCRAFT CATAPULT VESSEL</skos:prefLabel>
		<dcterms:issued rdf:datatype="http://www.w3.org/2001/XMLSchema#dateTime">2013-07-17T09:01:43</dcterms:issued>
		<skos:broader rdf:resource="http://purl.org/heritagedata/schemes/eh_tmc/concepts/100394" />
		<skos:narrower>
			<skos:Concept rdf:about="http://purl.org/heritagedata/schemes/eh_tmc/concepts/159215">
				<skos:inScheme rdf:resource="http://purl.org/heritagedata/schemes/eh_tmc" />
				<dcterms:identifier>http://purl.org/heritagedata/schemes/eh_tmc/concepts/159215</dcterms:identifier>
				<skos:prefLabel xml:lang="en">CATAPULT ARMED MERCHANTMAN</skos:prefLabel>
				<dcterms:issued rdf:datatype="http://www.w3.org/2001/XMLSchema#dateTime">2013-07-17T09:01:43</dcterms:issued>
				<skos:altLabel xml:lang="en">Cam Ship</skos:altLabel>
				<skos:broader rdf:resource="http://purl.org/heritagedata/schemes/eh_tmc/concepts/100260" />
				<skos:scopeNote xml:lang="en">World War II-era British merchant ships used in convoys as an emergency stop-gap until sufficient escort carriers became available. They were equipped with a rocket-propelled catapult launching a single Hawker Sea Hurricane plane.</skos:scopeNote>
				<cc:license rdf:resource="http://creativecommons.org/licenses/by/3.0" />
				<cc:attributionURL rdf:resource="http://www.english-heritage.org.uk" />
				<cc:attributionName xml:lang="en">English Heritage</cc:attributionName>
				<dcterms:publisher rdf:resource="http://www.english-heritage.org.uk" />
			</skos:Concept>
		</skos:narrower>
		<skos:related rdf:resource="http://purl.org/heritagedata/schemes/eh_tmc/concepts/100259" />
		<skos:related rdf:resource="http://purl.org/heritagedata/schemes/eh_tmc/concepts/100466" />
		<skos:scopeNote xml:lang="en">A vessel fitted with a catapult for launching an aircraft.</skos:scopeNote>
		<cc:license rdf:resource="http://creativecommons.org/licenses/by/3.0" />
		<cc:attributionURL rdf:resource="http://www.english-heritage.org.uk" />
		<cc:attributionName xml:lang="en">English Heritage</cc:attributionName>
		<dcterms:publisher rdf:resource="http://www.english-heritage.org.uk" />
	</skos:Concept>
	<skos:Concept rdf:about="http://purl.org/heritagedata/schemes/eh_tmc/concepts/100272">
		<skos:inScheme rdf:resource="http://purl.org/heritagedata/schemes/eh_tmc" />
		<dcterms:identifier>http://purl.org/heritagedata/schemes/eh_tmc/concepts/100272</dcterms:identifier>
		<skos:prefLabel xml:lang="en">BARGE</skos:prefLabel>
		<dcterms:issued rdf:datatype="http://www.w3.org/2001/XMLSchema#dateTime">2013-07-17T09:01:43</dcterms:issued>
		<skos:altLabel xml:lang="en">Roads Barge</skos:altLabel>
		<skos:altLabel xml:lang="en">Stumpsail Barge</skos:altLabel>
		<skos:altLabel xml:lang="en">Swimhead Barge</skos:altLabel>
		<skos:altLabel xml:lang="en">Topsail Barge</skos:altLabel>
		<skos:narrower>
			<skos:Concept rdf:about="http://purl.org/heritagedata/schemes/eh_tmc/concepts/100261">
				<skos:inScheme rdf:resource="http://purl.org/heritagedata/schemes/eh_tmc" />
				<dcterms:identifier>http://purl.org/heritagedata/schemes/eh_tmc/concepts/100261</dcterms:identifier>
				<skos:prefLabel xml:lang="en">AMMUNITION BARGE</skos:prefLabel>
				<dcterms:issued rdf:datatype="http://www.w3.org/2001/XMLSchema#dateTime">2013-07-17T09:01:43</dcterms:issued>
				<skos:broader rdf:resource="http://purl.org/heritagedata/schemes/eh_tmc/concepts/100272" />
				<skos:scopeNote xml:lang="en">Shallow draft vessel used to carry ammunition.</skos:scopeNote>
				<cc:license rdf:resource="http://creativecommons.org/licenses/by/3.0" />
				<cc:attributionURL rdf:resource="http://www.english-heritage.org.uk" />
				<cc:attributionName xml:lang="en">English Heritage</cc:attributionName>
				<dcterms:publisher rdf:resource="http://www.english-heritage.org.uk" />
			</skos:Concept>
		</skos:narrower>
		<skos:broader rdf:resource="http://purl.org/heritagedata/schemes/eh_tmc/concepts/100295" />
		<skos:narrower>
			<skos:Concept rdf:about="http://purl.org/heritagedata/schemes/eh_tmc/concepts/100308">
				<skos:inScheme rdf:resource="http://purl.org/heritagedata/schemes/eh_tmc" />
				<dcterms:identifier>http://purl.org/heritagedata/schemes/eh_tmc/concepts/100308</dcterms:identifier>
				<skos:prefLabel xml:lang="en">CRANE BARGE</skos:prefLabel>
				<dcterms:issued rdf:datatype="http://www.w3.org/2001/XMLSchema#dateTime">2013-07-17T09:01:43</dcterms:issued>
				<skos:broader rdf:resource="http://purl.org/heritagedata/schemes/eh_tmc/concepts/100272" />
				<skos:scopeNote xml:lang="en">A shallow draft vessel used to carry a crane.</skos:scopeNote>
				<cc:license rdf:resource="http://creativecommons.org/licenses/by/3.0" />
				<cc:attributionURL rdf:resource="http://www.english-heritage.org.uk" />
				<cc:attributionName xml:lang="en">English Heritage</cc:attributionName>
				<dcterms:publisher rdf:resource="http://www.english-heritage.org.uk" />
			</skos:Concept>
		</skos:narrower>
		<skos:narrower>
			<skos:Concept rdf:about="http://purl.org/heritagedata/schemes/eh_tmc/concepts/100364">
				<skos:inScheme rdf:resource="http://purl.org/heritagedata/schemes/eh_tmc" />
				<dcterms:identifier>http://purl.org/heritagedata/schemes/eh_tmc/concepts/100364</dcterms:identifier>
				<skos:prefLabel xml:lang="en">HOPPER BARGE</skos:prefLabel>
				<dcterms:issued rdf:datatype="http://www.w3.org/2001/XMLSchema#dateTime">2013-07-17T09:01:43</dcterms:issued>
				<skos:altLabel xml:lang="en">Hopper</skos:altLabel>
				<skos:broader rdf:resource="http://purl.org/heritagedata/schemes/eh_tmc/concepts/100272" />
				<skos:scopeNote xml:lang="en">A vessel used to carry away mud etc from a dredging machine and discharging it elsewhere.</skos:scopeNote>
				<cc:license rdf:resource="http://creativecommons.org/licenses/by/3.0" />
				<cc:attributionURL rdf:resource="http://www.english-heritage.org.uk" />
				<cc:attributionName xml:lang="en">English Heritage</cc:attributionName>
				<dcterms:publisher rdf:resource="http://www.english-heritage.org.uk" />
			</skos:Concept>
		</skos:narrower>
		<skos:narrower>
			<skos:Concept rdf:about="http://purl.org/heritagedata/schemes/eh_tmc/concepts/100402">
				<skos:inScheme rdf:resource="http://purl.org/heritagedata/schemes/eh_tmc" />
				<dcterms:identifier>http://purl.org/heritagedata/schemes/eh_tmc/concepts/100402</dcterms:identifier>
				<skos:prefLabel xml:lang="en">MOORING BUOY LIFTER BARGE</skos:prefLabel>
				<dcterms:issued rdf:datatype="http://www.w3.org/2001/XMLSchema#dateTime">2013-07-17T09:01:43</dcterms:issued>
				<skos:broader rdf:resource="http://purl.org/heritagedata/schemes/eh_tmc/concepts/100272" />
				<skos:scopeNote xml:lang="en">A barge with a crane or sheer legs used for moving and maintaining mooring buoys.</skos:scopeNote>
				<cc:license rdf:resource="http://creativecommons.org/licenses/by/3.0" />
				<cc:attributionURL rdf:resource="http://www.english-heritage.org.uk" />
				<cc:attributionName xml:lang="en">English Heritage</cc:attributionName>
				<dcterms:publisher rdf:resource="http://www.english-heritage.org.uk" />
			</skos:Concept>
		</skos:narrower>
		<skos:narrower>
			<skos:Concept rdf:about="http://purl.org/heritagedata/schemes/eh_tmc/concepts/100408">
				<skos:inScheme rdf:resource="http://purl.org/heritagedata/schemes/eh_tmc" />
				<dcterms:identifier>http://purl.org/heritagedata/schemes/eh_tmc/concepts/100408</dcterms:identifier>
				<skos:prefLabel xml:lang="en">MUD BARGE</skos:prefLabel>
				<dcterms:issued rdf:datatype="http://www.w3.org/2001/XMLSchema#dateTime">2013-07-17T09:01:43</dcterms:issued>
				<skos:broader rdf:resource="http://purl.org/heritagedata/schemes/eh_tmc/concepts/100272" />
				<skos:scopeNote xml:lang="en">A flat bottomed vessel for receiving mud and other material from a dredger.</skos:scopeNote>
				<cc:license rdf:resource="http://creativecommons.org/licenses/by/3.0" />
				<cc:attributionURL rdf:resource="http://www.english-heritage.org.uk" />
				<cc:attributionName xml:lang="en">English Heritage</cc:attributionName>
				<dcterms:publisher rdf:resource="http://www.english-heritage.org.uk" />
			</skos:Concept>
		</skos:narrower>
		<skos:narrower>
			<skos:Concept rdf:about="http://purl.org/heritagedata/schemes/eh_tmc/concepts/100423">
				<skos:inScheme rdf:resource="http://purl.org/heritagedata/schemes/eh_tmc" />
				<dcterms:identifier>http://purl.org/heritagedata/schemes/eh_tmc/concepts/100423</dcterms:identifier>
				<skos:prefLabel xml:lang="en">PILE DRIVING BARGE</skos:prefLabel>
				<dcterms:issued rdf:datatype="http://www.w3.org/2001/XMLSchema#dateTime">2013-07-17T09:01:43</dcterms:issued>
				<skos:altLabel xml:lang="en">Pile Driver</skos:altLabel>
				<skos:broader rdf:resource="http://purl.org/heritagedata/schemes/eh_tmc/concepts/100272" />
				<skos:scopeNote xml:lang="en">Flat bottomed vessel used as a platform for a pile driver.</skos:scopeNote>
				<cc:license rdf:resource="http://creativecommons.org/licenses/by/3.0" />
				<cc:attributionURL rdf:resource="http://www.english-heritage.org.uk" />
				<cc:attributionName xml:lang="en">English Heritage</cc:attributionName>
				<dcterms:publisher rdf:resource="http://www.english-heritage.org.uk" />
			</skos:Concept>
		</skos:narrower>
		<skos:narrower>
			<skos:Concept rdf:about="http://purl.org/heritagedata/schemes/eh_tmc/concepts/163221">
				<skos:inScheme rdf:resource="http://purl.org/heritagedata/schemes/eh_tmc" />
				<dcterms:identifier>http://purl.org/heritagedata/schemes/eh_tmc/concepts/163221</dcterms:identifier>
				<skos:prefLabel xml:lang="en">REFUGE BARGE</skos:prefLabel>
				<dcterms:issued rdf:datatype="http://www.w3.org/2001/XMLSchema#dateTime">2013-07-17T09:01:43</dcterms:issued>
				<skos:broader rdf:resource="http://purl.org/heritagedata/schemes/eh_tmc/concepts/100272" />
				<skos:scopeNote xml:lang="en">Moored barge providing a refuge for shipwrecked sailors or downed airmen, for example the air-sea rescue Cuckoo barges of WWII.</skos:scopeNote>
				<cc:license rdf:resource="http://creativecommons.org/licenses/by/3.0" />
				<cc:attributionURL rdf:resource="http://www.english-heritage.org.uk" />
				<cc:attributionName xml:lang="en">English Heritage</cc:attributionName>
				<dcterms:publisher rdf:resource="http://www.english-heritage.org.uk" />
			</skos:Concept>
		</skos:narrower>
		<skos:narrower rdf:resource="http://purl.org/heritagedata/schemes/eh_tmc/concepts/100460" />
		<skos:narrower>
			<skos:Concept rdf:about="http://purl.org/heritagedata/schemes/eh_tmc/concepts/100471">
				<skos:inScheme rdf:resource="http://purl.org/heritagedata/schemes/eh_tmc" />
				<dcterms:identifier>http://purl.org/heritagedata/schemes/eh_tmc/concepts/100471</dcterms:identifier>
				<skos:prefLabel xml:lang="en">TANK BARGE</skos:prefLabel>
				<dcterms:issued rdf:datatype="http://www.w3.org/2001/XMLSchema#dateTime">2013-07-17T09:01:43</dcterms:issued>
				<skos:broader rdf:resource="http://purl.org/heritagedata/schemes/eh_tmc/concepts/100272" />
				<skos:scopeNote xml:lang="en">A barge fitted with a large tank in its hull for carried liquid cargoes.</skos:scopeNote>
				<cc:license rdf:resource="http://creativecommons.org/licenses/by/3.0" />
				<cc:attributionURL rdf:resource="http://www.english-heritage.org.uk" />
				<cc:attributionName xml:lang="en">English Heritage</cc:attributionName>
				<dcterms:publisher rdf:resource="http://www.english-heritage.org.uk" />
			</skos:Concept>
		</skos:narrower>
		<skos:scopeNote xml:lang="en">Shallow draft cargo vessel, often broad beamed and flat bottomed, powered by engine and or sail.</skos:scopeNote>
		<cc:license rdf:resource="http://creativecommons.org/licenses/by/3.0" />
		<cc:attributionURL rdf:resource="http://www.english-heritage.org.uk" />
		<cc:attributionName xml:lang="en">English Heritage</cc:attributionName>
		<dcterms:publisher rdf:resource="http://www.english-heritage.org.uk" />
	</skos:Concept>
	<skos:Concept rdf:about="http://purl.org/heritagedata/schemes/eh_tmc/concepts/100278">
		<skos:inScheme rdf:resource="http://purl.org/heritagedata/schemes/eh_tmc" />
		<dcterms:identifier>http://purl.org/heritagedata/schemes/eh_tmc/concepts/100278</dcterms:identifier>
		<skos:prefLabel xml:lang="en">BATTLESHIP</skos:prefLabel>
		<dcterms:issued rdf:datatype="http://www.w3.org/2001/XMLSchema#dateTime">2013-07-17T09:01:43</dcterms:issued>
		<skos:altLabel xml:lang="en">First Class Battleship</skos:altLabel>
		<skos:altLabel xml:lang="en">Orion Class Battleship</skos:altLabel>
		<skos:broader rdf:resource="http://purl.org/heritagedata/schemes/eh_tmc/concepts/100490" />
		<skos:narrower>
			<skos:Concept rdf:about="http://purl.org/heritagedata/schemes/eh_tmc/concepts/100321">
				<skos:inScheme rdf:resource="http://purl.org/heritagedata/schemes/eh_tmc" />
				<dcterms:identifier>http://purl.org/heritagedata/schemes/eh_tmc/concepts/100321</dcterms:identifier>
				<skos:prefLabel xml:lang="en">DREADNOUGHT BATTLESHIP</skos:prefLabel>
				<dcterms:issued rdf:datatype="http://www.w3.org/2001/XMLSchema#dateTime">2013-07-17T09:01:43</dcterms:issued>
				<skos:broader rdf:resource="http://purl.org/heritagedata/schemes/eh_tmc/concepts/100278" />
				<skos:scopeNote xml:lang="en">A heavily armoured capital ship with an armament composed entirely of large calibre guns and powered by stem turbines. In effect any battleship constructed after 1908.</skos:scopeNote>
				<cc:license rdf:resource="http://creativecommons.org/licenses/by/3.0" />
				<cc:attributionURL rdf:resource="http://www.english-heritage.org.uk" />
				<cc:attributionName xml:lang="en">English Heritage</cc:attributionName>
				<dcterms:publisher rdf:resource="http://www.english-heritage.org.uk" />
			</skos:Concept>
		</skos:narrower>
		<skos:scopeNote xml:lang="en">A capital warship, often steam driven, heavily armoured with armament of large calibre guns deployed in turrets.</skos:scopeNote>
		<cc:license rdf:resource="http://creativecommons.org/licenses/by/3.0" />
		<cc:attributionURL rdf:resource="http://www.english-heritage.org.uk" />
		<cc:attributionName xml:lang="en">English Heritage</cc:attributionName>
		<dcterms:publisher rdf:resource="http://www.english-heritage.org.uk" />
	</skos:Concept>
	<skos:Concept rdf:about="http://purl.org/heritagedata/schemes/eh_tmc/concepts/100290">
		<skos:inScheme rdf:resource="http://purl.org/heritagedata/schemes/eh_tmc" />
		<dcterms:identifier>http://purl.org/heritagedata/schemes/eh_tmc/concepts/100290</dcterms:identifier>
		<skos:prefLabel xml:lang="en">CABIN CRAFT</skos:prefLabel>
		<dcterms:issued rdf:datatype="http://www.w3.org/2001/XMLSchema#dateTime">2013-07-17T09:01:43</dcterms:issued>
		<skos:broader rdf:resource="http://purl.org/heritagedata/schemes/eh_tmc/concepts/100382" />
		<skos:narrower>
			<skos:Concept rdf:about="http://purl.org/heritagedata/schemes/eh_tmc/concepts/151871">
				<skos:inScheme rdf:resource="http://purl.org/heritagedata/schemes/eh_tmc" />
				<dcterms:identifier>http://purl.org/heritagedata/schemes/eh_tmc/concepts/151871</dcterms:identifier>
				<skos:prefLabel xml:lang="en">CABIN CRUISER</skos:prefLabel>
				<dcterms:issued rdf:datatype="http://www.w3.org/2001/XMLSchema#dateTime">2013-07-17T09:01:43</dcterms:issued>
				<skos:broader rdf:resource="http://purl.org/heritagedata/schemes/eh_tmc/concepts/100290" />
				<skos:scopeNote xml:lang="en">A type of motorboat that provides accommodation for crew and passengers within the crafts cabin. Cabin Cruisers are usually between 25 feet and 45 feet long in length and are not to be confused with cruise ships which are substantially larger.</skos:scopeNote>
				<cc:license rdf:resource="http://creativecommons.org/licenses/by/3.0" />
				<cc:attributionURL rdf:resource="http://www.english-heritage.org.uk" />
				<cc:attributionName xml:lang="en">English Heritage</cc:attributionName>
				<dcterms:publisher rdf:resource="http://www.english-heritage.org.uk" />
			</skos:Concept>
		</skos:narrower>
		<skos:scopeNote xml:lang="en">A small vessel with a cabin as an integral part of its construction.</skos:scopeNote>
		<cc:license rdf:resource="http://creativecommons.org/licenses/by/3.0" />
		<cc:attributionURL rdf:resource="http://www.english-heritage.org.uk" />
		<cc:attributionName xml:lang="en">English Heritage</cc:attributionName>
		<dcterms:publisher rdf:resource="http://www.english-heritage.org.uk" />
	</skos:Concept>
	<skos:Concept rdf:about="http://purl.org/heritagedata/schemes/eh_tmc/concepts/100295">
		<skos:inScheme rdf:resource="http://purl.org/heritagedata/schemes/eh_tmc" />
		<dcterms:identifier>http://purl.org/heritagedata/schemes/eh_tmc/concepts/100295</dcterms:identifier>
		<skos:prefLabel xml:lang="en">CARGO VESSEL</skos:prefLabel>
		<dcterms:issued rdf:datatype="http://www.w3.org/2001/XMLSchema#dateTime">2013-07-17T09:01:43</dcterms:issued>
		<skos:narrower>
			<skos:Concept rdf:about="http://purl.org/heritagedata/schemes/eh_tmc/concepts/100264">
				<skos:inScheme rdf:resource="http://purl.org/heritagedata/schemes/eh_tmc" />
				<dcterms:identifier>http://purl.org/heritagedata/schemes/eh_tmc/concepts/100264</dcterms:identifier>
				<skos:prefLabel xml:lang="en">ARMED CARGO VESSEL</skos:prefLabel>
				<dcterms:issued rdf:datatype="http://www.w3.org/2001/XMLSchema#dateTime">2013-07-17T09:01:43</dcterms:issued>
				<skos:broader rdf:resource="http://purl.org/heritagedata/schemes/eh_tmc/concepts/100295" />
				<skos:scopeNote xml:lang="en">A vessel used for carrying cargoes, fitted with defensive weapons. Use with specific type and form where known.</skos:scopeNote>
				<cc:license rdf:resource="http://creativecommons.org/licenses/by/3.0" />
				<cc:attributionURL rdf:resource="http://www.english-heritage.org.uk" />
				<cc:attributionName xml:lang="en">English Heritage</cc:attributionName>
				<dcterms:publisher rdf:resource="http://www.english-heritage.org.uk" />
			</skos:Concept>
		</skos:narrower>
		<skos:narrower rdf:resource="http://purl.org/heritagedata/schemes/eh_tmc/concepts/100272" />
		<skos:narrower>
			<skos:Concept rdf:about="http://purl.org/heritagedata/schemes/eh_tmc/concepts/100287">
				<skos:inScheme rdf:resource="http://purl.org/heritagedata/schemes/eh_tmc" />
				<dcterms:identifier>http://purl.org/heritagedata/schemes/eh_tmc/concepts/100287</dcterms:identifier>
				<skos:prefLabel xml:lang="en">BULK ORE CARRIER</skos:prefLabel>
				<dcterms:issued rdf:datatype="http://www.w3.org/2001/XMLSchema#dateTime">2013-07-17T09:01:43</dcterms:issued>
				<skos:broader rdf:resource="http://purl.org/heritagedata/schemes/eh_tmc/concepts/100295" />
				<skos:scopeNote xml:lang="en">Large cargo vessel specially built and equipped for handling large quantities of ore.</skos:scopeNote>
				<cc:license rdf:resource="http://creativecommons.org/licenses/by/3.0" />
				<cc:attributionURL rdf:resource="http://www.english-heritage.org.uk" />
				<cc:attributionName xml:lang="en">English Heritage</cc:attributionName>
				<dcterms:publisher rdf:resource="http://www.english-heritage.org.uk" />
			</skos:Concept>
		</skos:narrower>
		<skos:broader rdf:resource="http://purl.org/heritagedata/schemes/eh_tmc/concepts/100480" />
		<skos:narrower rdf:resource="http://purl.org/heritagedata/schemes/eh_tmc/concepts/100301" />
		<skos:narrower>
			<skos:Concept rdf:about="http://purl.org/heritagedata/schemes/eh_tmc/concepts/100303">
				<skos:inScheme rdf:resource="http://purl.org/heritagedata/schemes/eh_tmc" />
				<dcterms:identifier>http://purl.org/heritagedata/schemes/eh_tmc/concepts/100303</dcterms:identifier>
				<skos:prefLabel xml:lang="en">COLLIER</skos:prefLabel>
				<dcterms:issued rdf:datatype="http://www.w3.org/2001/XMLSchema#dateTime">2013-07-17T09:01:43</dcterms:issued>
				<skos:altLabel xml:lang="en">Admiralty Collier</skos:altLabel>
				<skos:broader rdf:resource="http://purl.org/heritagedata/schemes/eh_tmc/concepts/100295" />
				<skos:scopeNote xml:lang="en">A vessel for carrying a cargo of coal in bulk.</skos:scopeNote>
				<cc:license rdf:resource="http://creativecommons.org/licenses/by/3.0" />
				<cc:attributionURL rdf:resource="http://www.english-heritage.org.uk" />
				<cc:attributionName xml:lang="en">English Heritage</cc:attributionName>
				<dcterms:publisher rdf:resource="http://www.english-heritage.org.uk" />
			</skos:Concept>
		</skos:narrower>
		<skos:narrower>
			<skos:Concept rdf:about="http://purl.org/heritagedata/schemes/eh_tmc/concepts/143007">
				<skos:inScheme rdf:resource="http://purl.org/heritagedata/schemes/eh_tmc" />
				<dcterms:identifier>http://purl.org/heritagedata/schemes/eh_tmc/concepts/143007</dcterms:identifier>
				<skos:prefLabel xml:lang="en">CONTAINER SHIP</skos:prefLabel>
				<dcterms:issued rdf:datatype="http://www.w3.org/2001/XMLSchema#dateTime">2013-07-17T09:01:43</dcterms:issued>
				<skos:broader rdf:resource="http://purl.org/heritagedata/schemes/eh_tmc/concepts/100295" />
				<skos:scopeNote xml:lang="en">A cargo vessel designed to carry goods packed in large containers that can be loaded directly onto trains or lorries.</skos:scopeNote>
				<cc:license rdf:resource="http://creativecommons.org/licenses/by/3.0" />
				<cc:attributionURL rdf:resource="http://www.english-heritage.org.uk" />
				<cc:attributionName xml:lang="en">English Heritage</cc:attributionName>
				<dcterms:publisher rdf:resource="http://www.english-heritage.org.uk" />
			</skos:Concept>
		</skos:narrower>
		<skos:narrower>
			<skos:Concept rdf:about="http://purl.org/heritagedata/schemes/eh_tmc/concepts/142957">
				<skos:inScheme rdf:resource="http://purl.org/heritagedata/schemes/eh_tmc" />
				<dcterms:identifier>http://purl.org/heritagedata/schemes/eh_tmc/concepts/142957</dcterms:identifier>
				<skos:prefLabel xml:lang="en">DROMOND</skos:prefLabel>
				<dcterms:issued rdf:datatype="http://www.w3.org/2001/XMLSchema#dateTime">2013-07-17T09:01:43</dcterms:issued>
				<skos:broader rdf:resource="http://purl.org/heritagedata/schemes/eh_tmc/concepts/100295" />
				<skos:scopeNote xml:lang="en">Originally denoting a Byzantine vessel, powered by oars, from the 6th century onwards, this developed into a large Mediterranean ship with oars and a single mast, used for trade or for war transport, (e.g. during the Crusades) until the 15th century.</skos:scopeNote>
				<cc:license rdf:resource="http://creativecommons.org/licenses/by/3.0" />
				<cc:attributionURL rdf:resource="http://www.english-heritage.org.uk" />
				<cc:attributionName xml:lang="en">English Heritage</cc:attributionName>
				<dcterms:publisher rdf:resource="http://www.english-heritage.org.uk" />
			</skos:Concept>
		</skos:narrower>
		<skos:narrower>
			<skos:Concept rdf:about="http://purl.org/heritagedata/schemes/eh_tmc/concepts/100324">
				<skos:inScheme rdf:resource="http://purl.org/heritagedata/schemes/eh_tmc" />
				<dcterms:identifier>http://purl.org/heritagedata/schemes/eh_tmc/concepts/100324</dcterms:identifier>
				<skos:prefLabel xml:lang="en">DRY BULK CARGO CARRIER</skos:prefLabel>
				<dcterms:issued rdf:datatype="http://www.w3.org/2001/XMLSchema#dateTime">2013-07-17T09:01:43</dcterms:issued>
				<skos:broader rdf:resource="http://purl.org/heritagedata/schemes/eh_tmc/concepts/100295" />
				<skos:scopeNote xml:lang="en">Cargo vessel specially constructed to carry bulk items such as grain. Does not include liquid cargoes.</skos:scopeNote>
				<cc:license rdf:resource="http://creativecommons.org/licenses/by/3.0" />
				<cc:attributionURL rdf:resource="http://www.english-heritage.org.uk" />
				<cc:attributionName xml:lang="en">English Heritage</cc:attributionName>
				<dcterms:publisher rdf:resource="http://www.english-heritage.org.uk" />
			</skos:Concept>
		</skos:narrower>
		<skos:narrower>
			<skos:Concept rdf:about="http://purl.org/heritagedata/schemes/eh_tmc/concepts/139744">
				<skos:inScheme rdf:resource="http://purl.org/heritagedata/schemes/eh_tmc" />
				<dcterms:identifier>http://purl.org/heritagedata/schemes/eh_tmc/concepts/139744</dcterms:identifier>
				<skos:prefLabel xml:lang="en">FLUIT</skos:prefLabel>
				<dcterms:issued rdf:datatype="http://www.w3.org/2001/XMLSchema#dateTime">2013-07-17T09:01:43</dcterms:issued>
				<skos:altLabel xml:lang="en">Fluyt</skos:altLabel>
				<skos:broader rdf:resource="http://purl.org/heritagedata/schemes/eh_tmc/concepts/100295" />
				<skos:scopeNote xml:lang="en">17th century Dutch vessel built for naval or East India service, with a relatively flat bottom and narrow hull; sometimes rendered into English as `fly-boat'.</skos:scopeNote>
				<cc:license rdf:resource="http://creativecommons.org/licenses/by/3.0" />
				<cc:attributionURL rdf:resource="http://www.english-heritage.org.uk" />
				<cc:attributionName xml:lang="en">English Heritage</cc:attributionName>
				<dcterms:publisher rdf:resource="http://www.english-heritage.org.uk" />
			</skos:Concept>
		</skos:narrower>
		<skos:narrower>
			<skos:Concept rdf:about="http://purl.org/heritagedata/schemes/eh_tmc/concepts/100348">
				<skos:inScheme rdf:resource="http://purl.org/heritagedata/schemes/eh_tmc" />
				<dcterms:identifier>http://purl.org/heritagedata/schemes/eh_tmc/concepts/100348</dcterms:identifier>
				<skos:prefLabel xml:lang="en">FREIGHTER</skos:prefLabel>
				<dcterms:issued rdf:datatype="http://www.w3.org/2001/XMLSchema#dateTime">2013-07-17T09:01:43</dcterms:issued>
				<skos:broader rdf:resource="http://purl.org/heritagedata/schemes/eh_tmc/concepts/100295" />
				<skos:scopeNote xml:lang="en">A single decked cargo vessel carrying the majority of its cargo on deck.</skos:scopeNote>
				<cc:license rdf:resource="http://creativecommons.org/licenses/by/3.0" />
				<cc:attributionURL rdf:resource="http://www.english-heritage.org.uk" />
				<cc:attributionName xml:lang="en">English Heritage</cc:attributionName>
				<dcterms:publisher rdf:resource="http://www.english-heritage.org.uk" />
			</skos:Concept>
		</skos:narrower>
		<skos:narrower>
			<skos:Concept rdf:about="http://purl.org/heritagedata/schemes/eh_tmc/concepts/144486">
				<skos:inScheme rdf:resource="http://purl.org/heritagedata/schemes/eh_tmc" />
				<dcterms:identifier>http://purl.org/heritagedata/schemes/eh_tmc/concepts/144486</dcterms:identifier>
				<skos:prefLabel xml:lang="en">GALEAS</skos:prefLabel>
				<dcterms:issued rdf:datatype="http://www.w3.org/2001/XMLSchema#dateTime">2013-07-17T09:01:43</dcterms:issued>
				<skos:broader rdf:resource="http://purl.org/heritagedata/schemes/eh_tmc/concepts/100295" />
				<skos:scopeNote xml:lang="en">Any one of the cargo vessels of that name belonging to the different Baltic nations, in use from the mid 18th to the early 20th century. Usually ketch-rigged. Not to be confused with the oared GALEASS.</skos:scopeNote>
				<cc:license rdf:resource="http://creativecommons.org/licenses/by/3.0" />
				<cc:attributionURL rdf:resource="http://www.english-heritage.org.uk" />
				<cc:attributionName xml:lang="en">English Heritage</cc:attributionName>
				<dcterms:publisher rdf:resource="http://www.english-heritage.org.uk" />
			</skos:Concept>
		</skos:narrower>
		<skos:narrower rdf:resource="http://purl.org/heritagedata/schemes/eh_tmc/concepts/139373" />
		<skos:narrower rdf:resource="http://purl.org/heritagedata/schemes/eh_tmc/concepts/100383" />
		<skos:narrower>
			<skos:Concept rdf:about="http://purl.org/heritagedata/schemes/eh_tmc/concepts/100390">
				<skos:inScheme rdf:resource="http://purl.org/heritagedata/schemes/eh_tmc" />
				<dcterms:identifier>http://purl.org/heritagedata/schemes/eh_tmc/concepts/100390</dcterms:identifier>
				<skos:prefLabel xml:lang="en">LIVESTOCK SHIP</skos:prefLabel>
				<dcterms:issued rdf:datatype="http://www.w3.org/2001/XMLSchema#dateTime">2013-07-17T09:01:43</dcterms:issued>
				<skos:broader rdf:resource="http://purl.org/heritagedata/schemes/eh_tmc/concepts/100295" />
				<skos:scopeNote xml:lang="en">A designed for the carriage of livestock usually cattle or sheep.</skos:scopeNote>
				<cc:license rdf:resource="http://creativecommons.org/licenses/by/3.0" />
				<cc:attributionURL rdf:resource="http://www.english-heritage.org.uk" />
				<cc:attributionName xml:lang="en">English Heritage</cc:attributionName>
				<dcterms:publisher rdf:resource="http://www.english-heritage.org.uk" />
			</skos:Concept>
		</skos:narrower>
		<skos:narrower>
			<skos:Concept rdf:about="http://purl.org/heritagedata/schemes/eh_tmc/concepts/159219">
				<skos:inScheme rdf:resource="http://purl.org/heritagedata/schemes/eh_tmc" />
				<dcterms:identifier>http://purl.org/heritagedata/schemes/eh_tmc/concepts/159219</dcterms:identifier>
				<skos:prefLabel xml:lang="en">NARROW BOAT</skos:prefLabel>
				<dcterms:issued rdf:datatype="http://www.w3.org/2001/XMLSchema#dateTime">2013-07-17T09:01:43</dcterms:issued>
				<skos:altLabel xml:lang="en">Narrowboat</skos:altLabel>
				<skos:broader rdf:resource="http://purl.org/heritagedata/schemes/eh_tmc/concepts/100295" />
				<skos:scopeNote xml:lang="en">A craft designed for use on canals and inland waterways. Usually 70ft long x 7ft wide though can be longer and broader.</skos:scopeNote>
				<cc:license rdf:resource="http://creativecommons.org/licenses/by/3.0" />
				<cc:attributionURL rdf:resource="http://www.english-heritage.org.uk" />
				<cc:attributionName xml:lang="en">English Heritage</cc:attributionName>
				<dcterms:publisher rdf:resource="http://www.english-heritage.org.uk" />
			</skos:Concept>
		</skos:narrower>
		<skos:narrower rdf:resource="http://purl.org/heritagedata/schemes/eh_tmc/concepts/100419" />
		<skos:narrower>
			<skos:Concept rdf:about="http://purl.org/heritagedata/schemes/eh_tmc/concepts/143008">
				<skos:inScheme rdf:resource="http://purl.org/heritagedata/schemes/eh_tmc" />
				<dcterms:identifier>http://purl.org/heritagedata/schemes/eh_tmc/concepts/143008</dcterms:identifier>
				<skos:prefLabel xml:lang="en">PUFFER</skos:prefLabel>
				<dcterms:issued rdf:datatype="http://www.w3.org/2001/XMLSchema#dateTime">2013-07-17T09:01:43</dcterms:issued>
				<skos:broader rdf:resource="http://purl.org/heritagedata/schemes/eh_tmc/concepts/100295" />
				<skos:scopeNote xml:lang="en">A small cargo vessel used on the West coast of Scotland.</skos:scopeNote>
				<cc:license rdf:resource="http://creativecommons.org/licenses/by/3.0" />
				<cc:attributionURL rdf:resource="http://www.english-heritage.org.uk" />
				<cc:attributionName xml:lang="en">English Heritage</cc:attributionName>
				<dcterms:publisher rdf:resource="http://www.english-heritage.org.uk" />
			</skos:Concept>
		</skos:narrower>
		<skos:narrower>
			<skos:Concept rdf:about="http://purl.org/heritagedata/schemes/eh_tmc/concepts/138512">
				<skos:inScheme rdf:resource="http://purl.org/heritagedata/schemes/eh_tmc" />
				<dcterms:identifier>http://purl.org/heritagedata/schemes/eh_tmc/concepts/138512</dcterms:identifier>
				<skos:prefLabel xml:lang="en">SLAVE SHIP</skos:prefLabel>
				<dcterms:issued rdf:datatype="http://www.w3.org/2001/XMLSchema#dateTime">2013-07-17T09:01:43</dcterms:issued>
				<skos:broader rdf:resource="http://purl.org/heritagedata/schemes/eh_tmc/concepts/100295" />
				<skos:scopeNote xml:lang="en">A large cargo vessel, either purpose-fitted or converted, for the transportation of slaves.</skos:scopeNote>
				<cc:license rdf:resource="http://creativecommons.org/licenses/by/3.0" />
				<cc:attributionURL rdf:resource="http://www.english-heritage.org.uk" />
				<cc:attributionName xml:lang="en">English Heritage</cc:attributionName>
				<dcterms:publisher rdf:resource="http://www.english-heritage.org.uk" />
			</skos:Concept>
		</skos:narrower>
		<skos:narrower>
			<skos:Concept rdf:about="http://purl.org/heritagedata/schemes/eh_tmc/concepts/100472">
				<skos:inScheme rdf:resource="http://purl.org/heritagedata/schemes/eh_tmc" />
				<dcterms:identifier>http://purl.org/heritagedata/schemes/eh_tmc/concepts/100472</dcterms:identifier>
				<skos:prefLabel xml:lang="en">TANKER</skos:prefLabel>
				<dcterms:issued rdf:datatype="http://www.w3.org/2001/XMLSchema#dateTime">2013-07-17T09:01:43</dcterms:issued>
				<skos:broader rdf:resource="http://purl.org/heritagedata/schemes/eh_tmc/concepts/100295" />
				<skos:scopeNote xml:lang="en">A ship designed specifically for the carriage of liquid cargoes, particularly oil.</skos:scopeNote>
				<cc:license rdf:resource="http://creativecommons.org/licenses/by/3.0" />
				<cc:attributionURL rdf:resource="http://www.english-heritage.org.uk" />
				<cc:attributionName xml:lang="en">English Heritage</cc:attributionName>
				<dcterms:publisher rdf:resource="http://www.english-heritage.org.uk" />
			</skos:Concept>
		</skos:narrower>
		<skos:narrower rdf:resource="http://purl.org/heritagedata/schemes/eh_tmc/concepts/152307" />
		<skos:scopeNote xml:lang="en">A craft used for the transportation of cargoes. Use specific type where known.</skos:scopeNote>
		<cc:license rdf:resource="http://creativecommons.org/licenses/by/3.0" />
		<cc:attributionURL rdf:resource="http://www.english-heritage.org.uk" />
		<cc:attributionName xml:lang="en">English Heritage</cc:attributionName>
		<dcterms:publisher rdf:resource="http://www.english-heritage.org.uk" />
	</skos:Concept>
	<skos:Concept rdf:about="http://purl.org/heritagedata/schemes/eh_tmc/concepts/100301">
		<skos:inScheme rdf:resource="http://purl.org/heritagedata/schemes/eh_tmc" />
		<dcterms:identifier>http://purl.org/heritagedata/schemes/eh_tmc/concepts/100301</dcterms:identifier>
		<skos:prefLabel xml:lang="en">COASTER</skos:prefLabel>
		<dcterms:issued rdf:datatype="http://www.w3.org/2001/XMLSchema#dateTime">2013-07-17T09:01:43</dcterms:issued>
		<skos:broader rdf:resource="http://purl.org/heritagedata/schemes/eh_tmc/concepts/100295" />
		<skos:narrower>
			<skos:Concept rdf:about="http://purl.org/heritagedata/schemes/eh_tmc/concepts/162885">
				<skos:inScheme rdf:resource="http://purl.org/heritagedata/schemes/eh_tmc" />
				<dcterms:identifier>http://purl.org/heritagedata/schemes/eh_tmc/concepts/162885</dcterms:identifier>
				<skos:prefLabel xml:lang="en">KOF</skos:prefLabel>
				<dcterms:issued rdf:datatype="http://www.w3.org/2001/XMLSchema#dateTime">2013-07-17T09:01:43</dcterms:issued>
				<skos:broader rdf:resource="http://purl.org/heritagedata/schemes/eh_tmc/concepts/100301" />
				<skos:scopeNote xml:lang="en">Dutch coaster of the late 17th to late 19th centuries with a square hull and 2 masts, generally having a heavy keel and round stern and bilges, although later examples were built on more refined lines.</skos:scopeNote>
				<cc:license rdf:resource="http://creativecommons.org/licenses/by/3.0" />
				<cc:attributionURL rdf:resource="http://www.english-heritage.org.uk" />
				<cc:attributionName xml:lang="en">English Heritage</cc:attributionName>
				<dcterms:publisher rdf:resource="http://www.english-heritage.org.uk" />
			</skos:Concept>
		</skos:narrower>
		<skos:scopeNote xml:lang="en">Small cargo vessel used for short coastal voyages carrying a variety of cargoes.</skos:scopeNote>
		<cc:license rdf:resource="http://creativecommons.org/licenses/by/3.0" />
		<cc:attributionURL rdf:resource="http://www.english-heritage.org.uk" />
		<cc:attributionName xml:lang="en">English Heritage</cc:attributionName>
		<dcterms:publisher rdf:resource="http://www.english-heritage.org.uk" />
	</skos:Concept>
	<skos:Concept rdf:about="http://purl.org/heritagedata/schemes/eh_tmc/concepts/100307">
		<skos:inScheme rdf:resource="http://purl.org/heritagedata/schemes/eh_tmc" />
		<dcterms:identifier>http://purl.org/heritagedata/schemes/eh_tmc/concepts/100307</dcterms:identifier>
		<skos:prefLabel xml:lang="en">CRAFT</skos:prefLabel>
		<dcterms:issued rdf:datatype="http://www.w3.org/2001/XMLSchema#dateTime">2013-07-17T09:01:43</dcterms:issued>
		<skos:altLabel xml:lang="en">Ship</skos:altLabel>
		<skos:altLabel xml:lang="en">Boat</skos:altLabel>
		<skos:narrower>
			<skos:Concept rdf:about="http://purl.org/heritagedata/schemes/eh_tmc/concepts/100292">
				<skos:inScheme rdf:resource="http://purl.org/heritagedata/schemes/eh_tmc" />
				<dcterms:identifier>http://purl.org/heritagedata/schemes/eh_tmc/concepts/100292</dcterms:identifier>
				<skos:prefLabel xml:lang="en">CANOE</skos:prefLabel>
				<dcterms:issued rdf:datatype="http://www.w3.org/2001/XMLSchema#dateTime">2013-07-17T09:01:43</dcterms:issued>
				<skos:broader rdf:resource="http://purl.org/heritagedata/schemes/eh_tmc/concepts/100307" />
				<skos:scopeNote xml:lang="en">A small open boat, usually a very light craft propelled by a paddle.</skos:scopeNote>
				<cc:license rdf:resource="http://creativecommons.org/licenses/by/3.0" />
				<cc:attributionURL rdf:resource="http://www.english-heritage.org.uk" />
				<cc:attributionName xml:lang="en">English Heritage</cc:attributionName>
				<dcterms:publisher rdf:resource="http://www.english-heritage.org.uk" />
			</skos:Concept>
		</skos:narrower>
		<skos:narrower>
			<skos:Concept rdf:about="http://purl.org/heritagedata/schemes/eh_tmc/concepts/151866">
				<skos:inScheme rdf:resource="http://purl.org/heritagedata/schemes/eh_tmc" />
				<dcterms:identifier>http://purl.org/heritagedata/schemes/eh_tmc/concepts/151866</dcterms:identifier>
				<skos:prefLabel xml:lang="en">CATAMARAN</skos:prefLabel>
				<dcterms:issued rdf:datatype="http://www.w3.org/2001/XMLSchema#dateTime">2013-07-17T09:01:43</dcterms:issued>
				<skos:broader rdf:resource="http://purl.org/heritagedata/schemes/eh_tmc/concepts/100307" />
				<skos:scopeNote xml:lang="en">A multihulled craft consisting of two hulls, or vakas, which are usually joined together by a frame or other structure, formed of akas. Catamarans can be sail or engine powered.</skos:scopeNote>
				<cc:license rdf:resource="http://creativecommons.org/licenses/by/3.0" />
				<cc:attributionURL rdf:resource="http://www.english-heritage.org.uk" />
				<cc:attributionName xml:lang="en">English Heritage</cc:attributionName>
				<dcterms:publisher rdf:resource="http://www.english-heritage.org.uk" />
			</skos:Concept>
		</skos:narrower>
		<skos:narrower rdf:resource="http://purl.org/heritagedata/schemes/eh_tmc/concepts/139332" />
		<skos:narrower>
			<skos:Concept rdf:about="http://purl.org/heritagedata/schemes/eh_tmc/concepts/100304">
				<skos:inScheme rdf:resource="http://purl.org/heritagedata/schemes/eh_tmc" />
				<dcterms:identifier>http://purl.org/heritagedata/schemes/eh_tmc/concepts/100304</dcterms:identifier>
				<skos:prefLabel xml:lang="en">CORACLE</skos:prefLabel>
				<dcterms:issued rdf:datatype="http://www.w3.org/2001/XMLSchema#dateTime">2013-07-17T09:01:43</dcterms:issued>
				<skos:broader rdf:resource="http://purl.org/heritagedata/schemes/eh_tmc/concepts/100307" />
				<skos:scopeNote xml:lang="en">A small craft of wickerwork covered with waterproof material.</skos:scopeNote>
				<cc:license rdf:resource="http://creativecommons.org/licenses/by/3.0" />
				<cc:attributionURL rdf:resource="http://www.english-heritage.org.uk" />
				<cc:attributionName xml:lang="en">English Heritage</cc:attributionName>
				<dcterms:publisher rdf:resource="http://www.english-heritage.org.uk" />
			</skos:Concept>
		</skos:narrower>
		<skos:broader rdf:resource="http://purl.org/heritagedata/schemes/eh_tmc/concepts/100394" />
		<skos:narrower>
			<skos:Concept rdf:about="http://purl.org/heritagedata/schemes/eh_tmc/concepts/140248">
				<skos:inScheme rdf:resource="http://purl.org/heritagedata/schemes/eh_tmc" />
				<dcterms:identifier>http://purl.org/heritagedata/schemes/eh_tmc/concepts/140248</dcterms:identifier>
				<skos:prefLabel xml:lang="en">GIG</skos:prefLabel>
				<dcterms:issued rdf:datatype="http://www.w3.org/2001/XMLSchema#dateTime">2013-07-17T09:01:43</dcterms:issued>
				<skos:broader rdf:resource="http://purl.org/heritagedata/schemes/eh_tmc/concepts/100307" />
				<skos:scopeNote xml:lang="en">A six oared rowing boat which originated in Cornwall in the 18th century. Originally used as a pilot vessel, useage adapted to include cargo vessel and lifeboat. Today gigs are used in sporting events.</skos:scopeNote>
				<cc:license rdf:resource="http://creativecommons.org/licenses/by/3.0" />
				<cc:attributionURL rdf:resource="http://www.english-heritage.org.uk" />
				<cc:attributionName xml:lang="en">English Heritage</cc:attributionName>
				<dcterms:publisher rdf:resource="http://www.english-heritage.org.uk" />
			</skos:Concept>
		</skos:narrower>
		<skos:narrower>
			<skos:Concept rdf:about="http://purl.org/heritagedata/schemes/eh_tmc/concepts/164141">
				<skos:inScheme rdf:resource="http://purl.org/heritagedata/schemes/eh_tmc" />
				<dcterms:identifier>http://purl.org/heritagedata/schemes/eh_tmc/concepts/164141</dcterms:identifier>
				<skos:prefLabel xml:lang="en">HOVERCRAFT</skos:prefLabel>
				<dcterms:issued rdf:datatype="http://www.w3.org/2001/XMLSchema#dateTime">2013-07-17T09:01:43</dcterms:issued>
				<skos:broader rdf:resource="http://purl.org/heritagedata/schemes/eh_tmc/concepts/100307" />
				<skos:scopeNote xml:lang="en">An air-cushioned vehicle capable of travelling over land or water.</skos:scopeNote>
				<cc:license rdf:resource="http://creativecommons.org/licenses/by/3.0" />
				<cc:attributionURL rdf:resource="http://www.english-heritage.org.uk" />
				<cc:attributionName xml:lang="en">English Heritage</cc:attributionName>
				<dcterms:publisher rdf:resource="http://www.english-heritage.org.uk" />
			</skos:Concept>
		</skos:narrower>
		<skos:narrower>
			<skos:Concept rdf:about="http://purl.org/heritagedata/schemes/eh_tmc/concepts/151865">
				<skos:inScheme rdf:resource="http://purl.org/heritagedata/schemes/eh_tmc" />
				<dcterms:identifier>http://purl.org/heritagedata/schemes/eh_tmc/concepts/151865</dcterms:identifier>
				<skos:prefLabel xml:lang="en">HYDROFOIL</skos:prefLabel>
				<dcterms:issued rdf:datatype="http://www.w3.org/2001/XMLSchema#dateTime">2013-07-17T09:01:43</dcterms:issued>
				<skos:broader rdf:resource="http://purl.org/heritagedata/schemes/eh_tmc/concepts/100307" />
				<skos:scopeNote xml:lang="en">High speed craft developed in the 20th Century which employ a wing-like structure mounted on struts below the hull which lift the vessel above the water line during forward motion, reducing drag and increasing speed.</skos:scopeNote>
				<cc:license rdf:resource="http://creativecommons.org/licenses/by/3.0" />
				<cc:attributionURL rdf:resource="http://www.english-heritage.org.uk" />
				<cc:attributionName xml:lang="en">English Heritage</cc:attributionName>
				<dcterms:publisher rdf:resource="http://www.english-heritage.org.uk" />
			</skos:Concept>
		</skos:narrower>
		<skos:narrower>
			<skos:Concept rdf:about="http://purl.org/heritagedata/schemes/eh_tmc/concepts/100391">
				<skos:inScheme rdf:resource="http://purl.org/heritagedata/schemes/eh_tmc" />
				<dcterms:identifier>http://purl.org/heritagedata/schemes/eh_tmc/concepts/100391</dcterms:identifier>
				<skos:prefLabel xml:lang="en">LOGBOAT</skos:prefLabel>
				<dcterms:issued rdf:datatype="http://www.w3.org/2001/XMLSchema#dateTime">2013-07-17T09:01:43</dcterms:issued>
				<skos:broader rdf:resource="http://purl.org/heritagedata/schemes/eh_tmc/concepts/100307" />
				<skos:scopeNote xml:lang="en">A boat fashioned out of a section of tree trunk.</skos:scopeNote>
				<cc:license rdf:resource="http://creativecommons.org/licenses/by/3.0" />
				<cc:attributionURL rdf:resource="http://www.english-heritage.org.uk" />
				<cc:attributionName xml:lang="en">English Heritage</cc:attributionName>
				<dcterms:publisher rdf:resource="http://www.english-heritage.org.uk" />
			</skos:Concept>
		</skos:narrower>
		<skos:narrower>
			<skos:Concept rdf:about="http://purl.org/heritagedata/schemes/eh_tmc/concepts/140198">
				<skos:inScheme rdf:resource="http://purl.org/heritagedata/schemes/eh_tmc" />
				<dcterms:identifier>http://purl.org/heritagedata/schemes/eh_tmc/concepts/140198</dcterms:identifier>
				<skos:prefLabel xml:lang="en">SCHUIT</skos:prefLabel>
				<dcterms:issued rdf:datatype="http://www.w3.org/2001/XMLSchema#dateTime">2013-07-17T09:01:43</dcterms:issued>
				<skos:broader rdf:resource="http://purl.org/heritagedata/schemes/eh_tmc/concepts/100307" />
				<skos:scopeNote xml:lang="en">Dutch galliot-rigged vessel used mostly for river trade in Holland but sometimes also for coasting or short sea-going voyages</skos:scopeNote>
				<cc:license rdf:resource="http://creativecommons.org/licenses/by/3.0" />
				<cc:attributionURL rdf:resource="http://www.english-heritage.org.uk" />
				<cc:attributionName xml:lang="en">English Heritage</cc:attributionName>
				<dcterms:publisher rdf:resource="http://www.english-heritage.org.uk" />
			</skos:Concept>
		</skos:narrower>
		<skos:narrower>
			<skos:Concept rdf:about="http://purl.org/heritagedata/schemes/eh_tmc/concepts/145087">
				<skos:inScheme rdf:resource="http://purl.org/heritagedata/schemes/eh_tmc" />
				<dcterms:identifier>http://purl.org/heritagedata/schemes/eh_tmc/concepts/145087</dcterms:identifier>
				<skos:prefLabel xml:lang="en">SEWN BOAT</skos:prefLabel>
				<dcterms:issued rdf:datatype="http://www.w3.org/2001/XMLSchema#dateTime">2013-07-17T09:01:43</dcterms:issued>
				<skos:broader rdf:resource="http://purl.org/heritagedata/schemes/eh_tmc/concepts/100307" />
				<skos:scopeNote xml:lang="en">A type of clinker built wooden boat or ship held together with tendons of flexible wood such as roots and willow branches. Sewn boat construction techniques were used in many parts of the world prior to the development of metal fasteners.</skos:scopeNote>
				<cc:license rdf:resource="http://creativecommons.org/licenses/by/3.0" />
				<cc:attributionURL rdf:resource="http://www.english-heritage.org.uk" />
				<cc:attributionName xml:lang="en">English Heritage</cc:attributionName>
				<dcterms:publisher rdf:resource="http://www.english-heritage.org.uk" />
			</skos:Concept>
		</skos:narrower>
		<skos:narrower rdf:resource="http://purl.org/heritagedata/schemes/eh_tmc/concepts/141805" />
		<skos:scopeNote xml:lang="en">All vessels, use more specific type where known.</skos:scopeNote>
		<cc:license rdf:resource="http://creativecommons.org/licenses/by/3.0" />
		<cc:attributionURL rdf:resource="http://www.english-heritage.org.uk" />
		<cc:attributionName xml:lang="en">English Heritage</cc:attributionName>
		<dcterms:publisher rdf:resource="http://www.english-heritage.org.uk" />
	</skos:Concept>
	<skos:Concept rdf:about="http://purl.org/heritagedata/schemes/eh_tmc/concepts/100311">
		<skos:inScheme rdf:resource="http://purl.org/heritagedata/schemes/eh_tmc" />
		<dcterms:identifier>http://purl.org/heritagedata/schemes/eh_tmc/concepts/100311</dcterms:identifier>
		<skos:prefLabel xml:lang="en">CRUISER</skos:prefLabel>
		<dcterms:issued rdf:datatype="http://www.w3.org/2001/XMLSchema#dateTime">2013-07-17T09:01:43</dcterms:issued>
		<skos:altLabel xml:lang="en">Second Class Cruiser</skos:altLabel>
		<skos:broader rdf:resource="http://purl.org/heritagedata/schemes/eh_tmc/concepts/100490" />
		<skos:narrower>
			<skos:Concept rdf:about="http://purl.org/heritagedata/schemes/eh_tmc/concepts/100385">
				<skos:inScheme rdf:resource="http://purl.org/heritagedata/schemes/eh_tmc" />
				<dcterms:identifier>http://purl.org/heritagedata/schemes/eh_tmc/concepts/100385</dcterms:identifier>
				<skos:prefLabel xml:lang="en">LIGHT CRUISER</skos:prefLabel>
				<dcterms:issued rdf:datatype="http://www.w3.org/2001/XMLSchema#dateTime">2013-07-17T09:01:43</dcterms:issued>
				<skos:broader rdf:resource="http://purl.org/heritagedata/schemes/eh_tmc/concepts/100311" />
				<skos:scopeNote xml:lang="en">Large warship with no armour and a high speed. Used for reconnaisance and raids on enemy merchant shipping.</skos:scopeNote>
				<cc:license rdf:resource="http://creativecommons.org/licenses/by/3.0" />
				<cc:attributionURL rdf:resource="http://www.english-heritage.org.uk" />
				<cc:attributionName xml:lang="en">English Heritage</cc:attributionName>
				<dcterms:publisher rdf:resource="http://www.english-heritage.org.uk" />
			</skos:Concept>
		</skos:narrower>
		<skos:scopeNote xml:lang="en">Large warship equipped with turret mounted guns. Intended for independent action for trade protection, reconaissance and fire support for amphibious operations.</skos:scopeNote>
		<cc:license rdf:resource="http://creativecommons.org/licenses/by/3.0" />
		<cc:attributionURL rdf:resource="http://www.english-heritage.org.uk" />
		<cc:attributionName xml:lang="en">English Heritage</cc:attributionName>
		<dcterms:publisher rdf:resource="http://www.english-heritage.org.uk" />
	</skos:Concept>
	<skos:Concept rdf:about="http://purl.org/heritagedata/schemes/eh_tmc/concepts/100312">
		<skos:inScheme rdf:resource="http://purl.org/heritagedata/schemes/eh_tmc" />
		<dcterms:identifier>http://purl.org/heritagedata/schemes/eh_tmc/concepts/100312</dcterms:identifier>
		<skos:prefLabel xml:lang="en">CUSTOMS BOAT</skos:prefLabel>
		<dcterms:issued rdf:datatype="http://www.w3.org/2001/XMLSchema#dateTime">2013-07-17T09:01:43</dcterms:issued>
		<skos:broader rdf:resource="http://purl.org/heritagedata/schemes/eh_tmc/concepts/145105" />
		<skos:related rdf:resource="http://purl.org/heritagedata/schemes/eh_tmc/concepts/138609" />
		<skos:related rdf:resource="http://purl.org/heritagedata/schemes/eh_tmc/concepts/145104" />
		<skos:scopeNote xml:lang="en">A small vessel used as transport for customs officers.</skos:scopeNote>
		<cc:license rdf:resource="http://creativecommons.org/licenses/by/3.0" />
		<cc:attributionURL rdf:resource="http://www.english-heritage.org.uk" />
		<cc:attributionName xml:lang="en">English Heritage</cc:attributionName>
		<dcterms:publisher rdf:resource="http://www.english-heritage.org.uk" />
	</skos:Concept>
	<skos:Concept rdf:about="http://purl.org/heritagedata/schemes/eh_tmc/concepts/100316">
		<skos:inScheme rdf:resource="http://purl.org/heritagedata/schemes/eh_tmc" />
		<dcterms:identifier>http://purl.org/heritagedata/schemes/eh_tmc/concepts/100316</dcterms:identifier>
		<skos:prefLabel xml:lang="en">DECOY VESSEL</skos:prefLabel>
		<dcterms:issued rdf:datatype="http://www.w3.org/2001/XMLSchema#dateTime">2013-07-17T09:01:43</dcterms:issued>
		<skos:broader rdf:resource="http://purl.org/heritagedata/schemes/eh_tmc/concepts/100410" />
		<skos:narrower>
			<skos:Concept rdf:about="http://purl.org/heritagedata/schemes/eh_tmc/concepts/100326">
				<skos:inScheme rdf:resource="http://purl.org/heritagedata/schemes/eh_tmc" />
				<dcterms:identifier>http://purl.org/heritagedata/schemes/eh_tmc/concepts/100326</dcterms:identifier>
				<skos:prefLabel xml:lang="en">DUMMY WARSHIP</skos:prefLabel>
				<dcterms:issued rdf:datatype="http://www.w3.org/2001/XMLSchema#dateTime">2013-07-17T09:01:43</dcterms:issued>
				<skos:broader rdf:resource="http://purl.org/heritagedata/schemes/eh_tmc/concepts/100316" />
				<skos:scopeNote xml:lang="en">A civil vessel disguised as a warship.</skos:scopeNote>
				<cc:license rdf:resource="http://creativecommons.org/licenses/by/3.0" />
				<cc:attributionURL rdf:resource="http://www.english-heritage.org.uk" />
				<cc:attributionName xml:lang="en">English Heritage</cc:attributionName>
				<dcterms:publisher rdf:resource="http://www.english-heritage.org.uk" />
			</skos:Concept>
		</skos:narrower>
		<skos:narrower>
			<skos:Concept rdf:about="http://purl.org/heritagedata/schemes/eh_tmc/concepts/100433">
				<skos:inScheme rdf:resource="http://purl.org/heritagedata/schemes/eh_tmc" />
				<dcterms:identifier>http://purl.org/heritagedata/schemes/eh_tmc/concepts/100433</dcterms:identifier>
				<skos:prefLabel xml:lang="en">Q SHIP</skos:prefLabel>
				<dcterms:issued rdf:datatype="http://www.w3.org/2001/XMLSchema#dateTime">2013-07-17T09:01:43</dcterms:issued>
				<skos:broader rdf:resource="http://purl.org/heritagedata/schemes/eh_tmc/concepts/100316" />
				<skos:scopeNote xml:lang="en">A small merchant ship or warship with concealed weapons, intended as a trap for enemy submarines.</skos:scopeNote>
				<cc:license rdf:resource="http://creativecommons.org/licenses/by/3.0" />
				<cc:attributionURL rdf:resource="http://www.english-heritage.org.uk" />
				<cc:attributionName xml:lang="en">English Heritage</cc:attributionName>
				<dcterms:publisher rdf:resource="http://www.english-heritage.org.uk" />
			</skos:Concept>
		</skos:narrower>
		<skos:scopeNote xml:lang="en">A vessel, usually a merchant vessel, altered to resemble a warship or another vessel.</skos:scopeNote>
		<cc:license rdf:resource="http://creativecommons.org/licenses/by/3.0" />
		<cc:attributionURL rdf:resource="http://www.english-heritage.org.uk" />
		<cc:attributionName xml:lang="en">English Heritage</cc:attributionName>
		<dcterms:publisher rdf:resource="http://www.english-heritage.org.uk" />
	</skos:Concept>
	<skos:Concept rdf:about="http://purl.org/heritagedata/schemes/eh_tmc/concepts/138609">
		<skos:inScheme rdf:resource="http://purl.org/heritagedata/schemes/eh_tmc" />
		<dcterms:identifier>http://purl.org/heritagedata/schemes/eh_tmc/concepts/138609</dcterms:identifier>
		<skos:prefLabel xml:lang="en">PREVENTIVE SERVICE VESSEL</skos:prefLabel>
		<dcterms:issued rdf:datatype="http://www.w3.org/2001/XMLSchema#dateTime">2013-07-17T09:01:43</dcterms:issued>
		<skos:altLabel xml:lang="en">Preventative Service Vessel</skos:altLabel>
		<skos:broader rdf:resource="http://purl.org/heritagedata/schemes/eh_tmc/concepts/145105" />
		<skos:narrower rdf:resource="http://purl.org/heritagedata/schemes/eh_tmc/concepts/100440" />
		<skos:related rdf:resource="http://purl.org/heritagedata/schemes/eh_tmc/concepts/100312" />
		<skos:related rdf:resource="http://purl.org/heritagedata/schemes/eh_tmc/concepts/145104" />
		<skos:scopeNote xml:lang="en">Prior to 1822 a vessel used by the customs department involved with the prevention of smuggling.</skos:scopeNote>
		<cc:license rdf:resource="http://creativecommons.org/licenses/by/3.0" />
		<cc:attributionURL rdf:resource="http://www.english-heritage.org.uk" />
		<cc:attributionName xml:lang="en">English Heritage</cc:attributionName>
		<dcterms:publisher rdf:resource="http://www.english-heritage.org.uk" />
	</skos:Concept>
	<skos:Concept rdf:about="http://purl.org/heritagedata/schemes/eh_tmc/concepts/139837">
		<skos:inScheme rdf:resource="http://purl.org/heritagedata/schemes/eh_tmc" />
		<dcterms:identifier>http://purl.org/heritagedata/schemes/eh_tmc/concepts/139837</dcterms:identifier>
		<skos:prefLabel xml:lang="en">PATROL VESSEL</skos:prefLabel>
		<dcterms:issued rdf:datatype="http://www.w3.org/2001/XMLSchema#dateTime">2013-07-17T09:01:43</dcterms:issued>
		<skos:altLabel xml:lang="en">Patrol Ship</skos:altLabel>
		<skos:narrower>
			<skos:Concept rdf:about="http://purl.org/heritagedata/schemes/eh_tmc/concepts/100420">
				<skos:inScheme rdf:resource="http://purl.org/heritagedata/schemes/eh_tmc" />
				<dcterms:identifier>http://purl.org/heritagedata/schemes/eh_tmc/concepts/100420</dcterms:identifier>
				<skos:prefLabel xml:lang="en">PATROL BOAT</skos:prefLabel>
				<dcterms:issued rdf:datatype="http://www.w3.org/2001/XMLSchema#dateTime">2013-07-17T09:01:43</dcterms:issued>
				<skos:broader rdf:resource="http://purl.org/heritagedata/schemes/eh_tmc/concepts/139837" />
				<skos:scopeNote xml:lang="en">A small warship engaged in patrolling coastal waters.</skos:scopeNote>
				<cc:license rdf:resource="http://creativecommons.org/licenses/by/3.0" />
				<cc:attributionURL rdf:resource="http://www.english-heritage.org.uk" />
				<cc:attributionName xml:lang="en">English Heritage</cc:attributionName>
				<dcterms:publisher rdf:resource="http://www.english-heritage.org.uk" />
			</skos:Concept>
		</skos:narrower>
		<skos:narrower rdf:resource="http://purl.org/heritagedata/schemes/eh_tmc/concepts/100421" />
		<skos:broader rdf:resource="http://purl.org/heritagedata/schemes/eh_tmc/concepts/100394" />
		<skos:scopeNote xml:lang="en">A vessel, purpose-built or requisitioned, used for patrolling inland or coastal waters, e.g. Coastguard and Customs vessels.</skos:scopeNote>
		<cc:license rdf:resource="http://creativecommons.org/licenses/by/3.0" />
		<cc:attributionURL rdf:resource="http://www.english-heritage.org.uk" />
		<cc:attributionName xml:lang="en">English Heritage</cc:attributionName>
		<dcterms:publisher rdf:resource="http://www.english-heritage.org.uk" />
	</skos:Concept>
	<skos:Concept rdf:about="http://purl.org/heritagedata/schemes/eh_tmc/concepts/141805">
		<skos:inScheme rdf:resource="http://purl.org/heritagedata/schemes/eh_tmc" />
		<dcterms:identifier>http://purl.org/heritagedata/schemes/eh_tmc/concepts/141805</dcterms:identifier>
		<skos:prefLabel xml:lang="en">SHIPS BOAT</skos:prefLabel>
		<dcterms:issued rdf:datatype="http://www.w3.org/2001/XMLSchema#dateTime">2013-07-17T09:01:43</dcterms:issued>
		<skos:narrower rdf:resource="http://purl.org/heritagedata/schemes/eh_tmc/concepts/160144" />
		<skos:broader rdf:resource="http://purl.org/heritagedata/schemes/eh_tmc/concepts/100307" />
		<skos:scopeNote xml:lang="en">Satellite craft belonging to a larger vessel, usually a rowing vessel; used to pick up or set down passengers or crew when lying offshore, or stowed on board as the "long boat" or "jolly boat" for lifesaving purposes.</skos:scopeNote>
		<cc:license rdf:resource="http://creativecommons.org/licenses/by/3.0" />
		<cc:attributionURL rdf:resource="http://www.english-heritage.org.uk" />
		<cc:attributionName xml:lang="en">English Heritage</cc:attributionName>
		<dcterms:publisher rdf:resource="http://www.english-heritage.org.uk" />
	</skos:Concept>
	<skos:Concept rdf:about="http://purl.org/heritagedata/schemes/eh_tmc/concepts/141858">
		<skos:inScheme rdf:resource="http://purl.org/heritagedata/schemes/eh_tmc" />
		<dcterms:identifier>http://purl.org/heritagedata/schemes/eh_tmc/concepts/141858</dcterms:identifier>
		<skos:prefLabel xml:lang="en">CASUALTY CLEARING SHIP</skos:prefLabel>
		<dcterms:issued rdf:datatype="http://www.w3.org/2001/XMLSchema#dateTime">2013-07-17T09:01:43</dcterms:issued>
		<skos:broader rdf:resource="http://purl.org/heritagedata/schemes/eh_tmc/concepts/100480" />
		<skos:related rdf:resource="http://purl.org/heritagedata/schemes/eh_tmc/concepts/100366" />
		<skos:scopeNote xml:lang="en">Transport vessel used for the repatriation of wounded troops, particularly during the First World War. Loosely described as "hospital ships", these ships were distinct from hospital ships proper by being defensively armed.</skos:scopeNote>
		<cc:license rdf:resource="http://creativecommons.org/licenses/by/3.0" />
		<cc:attributionURL rdf:resource="http://www.english-heritage.org.uk" />
		<cc:attributionName xml:lang="en">English Heritage</cc:attributionName>
		<dcterms:publisher rdf:resource="http://www.english-heritage.org.uk" />
	</skos:Concept>
	<skos:Concept rdf:about="http://purl.org/heritagedata/schemes/eh_tmc/concepts/140478">
		<skos:inScheme rdf:resource="http://purl.org/heritagedata/schemes/eh_tmc" />
		<dcterms:identifier>http://purl.org/heritagedata/schemes/eh_tmc/concepts/140478</dcterms:identifier>
		<skos:prefLabel xml:lang="en">FIVE MAN BOAT</skos:prefLabel>
		<dcterms:issued rdf:datatype="http://www.w3.org/2001/XMLSchema#dateTime">2013-07-17T09:01:43</dcterms:issued>
		<skos:broader rdf:resource="http://purl.org/heritagedata/schemes/eh_tmc/concepts/100392" />
		<skos:broader rdf:resource="http://purl.org/heritagedata/schemes/eh_tmc/concepts/100342" />
		<skos:scopeNote xml:lang="en">Three-masted fishing lugger built in and operating out of Yorkshire on the North Sea fisheries; so named as it was crewed by five joint owners, plus two or three paid hands.</skos:scopeNote>
		<cc:license rdf:resource="http://creativecommons.org/licenses/by/3.0" />
		<cc:attributionURL rdf:resource="http://www.english-heritage.org.uk" />
		<cc:attributionName xml:lang="en">English Heritage</cc:attributionName>
		<dcterms:publisher rdf:resource="http://www.english-heritage.org.uk" />
	</skos:Concept>
	<skos:Concept rdf:about="http://purl.org/heritagedata/schemes/eh_tmc/concepts/139332">
		<skos:inScheme rdf:resource="http://purl.org/heritagedata/schemes/eh_tmc" />
		<dcterms:identifier>http://purl.org/heritagedata/schemes/eh_tmc/concepts/139332</dcterms:identifier>
		<skos:prefLabel xml:lang="en">COBLE</skos:prefLabel>
		<dcterms:issued rdf:datatype="http://www.w3.org/2001/XMLSchema#dateTime">2013-07-17T09:01:43</dcterms:issued>
		<skos:broader rdf:resource="http://purl.org/heritagedata/schemes/eh_tmc/concepts/100307" />
		<skos:narrower>
			<skos:Concept rdf:about="http://purl.org/heritagedata/schemes/eh_tmc/concepts/140562">
				<skos:inScheme rdf:resource="http://purl.org/heritagedata/schemes/eh_tmc" />
				<dcterms:identifier>http://purl.org/heritagedata/schemes/eh_tmc/concepts/140562</dcterms:identifier>
				<skos:prefLabel xml:lang="en">FOYBOAT</skos:prefLabel>
				<dcterms:issued rdf:datatype="http://www.w3.org/2001/XMLSchema#dateTime">2013-07-17T09:01:43</dcterms:issued>
				<skos:altLabel xml:lang="en">Foy</skos:altLabel>
				<skos:broader rdf:resource="http://purl.org/heritagedata/schemes/eh_tmc/concepts/139332" />
				<skos:scopeNote xml:lang="en">Small, heavily built coble, usually fitted with lugsail and oars, used on the north-east coast of England to assist, tow, pilot, provision or otherwise attend ships.</skos:scopeNote>
				<cc:license rdf:resource="http://creativecommons.org/licenses/by/3.0" />
				<cc:attributionURL rdf:resource="http://www.english-heritage.org.uk" />
				<cc:attributionName xml:lang="en">English Heritage</cc:attributionName>
				<dcterms:publisher rdf:resource="http://www.english-heritage.org.uk" />
			</skos:Concept>
		</skos:narrower>
		<skos:scopeNote xml:lang="en">A small clinker-built craft, dating primarily from the 19th and early 20th centuries, fitted with oars and often a sail, usually found on the north-east coast of England and used for fishing or pilotage.</skos:scopeNote>
		<cc:license rdf:resource="http://creativecommons.org/licenses/by/3.0" />
		<cc:attributionURL rdf:resource="http://www.english-heritage.org.uk" />
		<cc:attributionName xml:lang="en">English Heritage</cc:attributionName>
		<dcterms:publisher rdf:resource="http://www.english-heritage.org.uk" />
	</skos:Concept>
	<skos:Concept rdf:about="http://purl.org/heritagedata/schemes/eh_tmc/concepts/139373">
		<skos:inScheme rdf:resource="http://purl.org/heritagedata/schemes/eh_tmc" />
		<dcterms:identifier>http://purl.org/heritagedata/schemes/eh_tmc/concepts/139373</dcterms:identifier>
		<skos:prefLabel xml:lang="en">HULK (SAIL)</skos:prefLabel>
		<dcterms:issued rdf:datatype="http://www.w3.org/2001/XMLSchema#dateTime">2013-07-17T09:01:43</dcterms:issued>
		<skos:broader rdf:resource="http://purl.org/heritagedata/schemes/eh_tmc/concepts/100295" />
		<skos:broader rdf:resource="http://purl.org/heritagedata/schemes/eh_tmc/concepts/100443" />
		<skos:scopeNote xml:lang="en">A large Mediterranean cargo or transport vessel of the 15th to 17th century, usually less than 400 tons.</skos:scopeNote>
		<cc:license rdf:resource="http://creativecommons.org/licenses/by/3.0" />
		<cc:attributionURL rdf:resource="http://www.english-heritage.org.uk" />
		<cc:attributionName xml:lang="en">English Heritage</cc:attributionName>
		<dcterms:publisher rdf:resource="http://www.english-heritage.org.uk" />
	</skos:Concept>
	<skos:Concept rdf:about="http://purl.org/heritagedata/schemes/eh_tmc/concepts/145104">
		<skos:inScheme rdf:resource="http://purl.org/heritagedata/schemes/eh_tmc" />
		<dcterms:identifier>http://purl.org/heritagedata/schemes/eh_tmc/concepts/145104</dcterms:identifier>
		<skos:prefLabel xml:lang="en">COASTGUARD VESSEL</skos:prefLabel>
		<dcterms:issued rdf:datatype="http://www.w3.org/2001/XMLSchema#dateTime">2013-07-17T09:01:43</dcterms:issued>
		<skos:broader rdf:resource="http://purl.org/heritagedata/schemes/eh_tmc/concepts/145105" />
		<skos:narrower rdf:resource="http://purl.org/heritagedata/schemes/eh_tmc/concepts/100440" />
		<skos:related rdf:resource="http://purl.org/heritagedata/schemes/eh_tmc/concepts/100312" />
		<skos:related rdf:resource="http://purl.org/heritagedata/schemes/eh_tmc/concepts/138609" />
		<skos:scopeNote xml:lang="en">From 1822, any vessel in the service of HM Coastguard, principally deployed on Customs and Revenue duties, i.e. anti-smuggling operations. Superseded the Preventive Service Vessel.</skos:scopeNote>
		<cc:license rdf:resource="http://creativecommons.org/licenses/by/3.0" />
		<cc:attributionURL rdf:resource="http://www.english-heritage.org.uk" />
		<cc:attributionName xml:lang="en">English Heritage</cc:attributionName>
		<dcterms:publisher rdf:resource="http://www.english-heritage.org.uk" />
	</skos:Concept>
	<skos:Concept rdf:about="http://purl.org/heritagedata/schemes/eh_tmc/concepts/145105">
		<skos:inScheme rdf:resource="http://purl.org/heritagedata/schemes/eh_tmc" />
		<dcterms:identifier>http://purl.org/heritagedata/schemes/eh_tmc/concepts/145105</dcterms:identifier>
		<skos:prefLabel xml:lang="en">CUSTOMS AND EXCISE VESSEL</skos:prefLabel>
		<dcterms:issued rdf:datatype="http://www.w3.org/2001/XMLSchema#dateTime">2013-07-17T09:01:43</dcterms:issued>
		<skos:narrower rdf:resource="http://purl.org/heritagedata/schemes/eh_tmc/concepts/145104" />
		<skos:broader rdf:resource="http://purl.org/heritagedata/schemes/eh_tmc/concepts/100394" />
		<skos:narrower rdf:resource="http://purl.org/heritagedata/schemes/eh_tmc/concepts/100312" />
		<skos:narrower rdf:resource="http://purl.org/heritagedata/schemes/eh_tmc/concepts/138609" />
		<skos:scopeNote xml:lang="en">Any vessel in the service of one of the historical or modern agencies concerned with the prevention of inbound or outbound smuggling: namely the Preventive Service, the Coastguard, or the Customs and Excise. Use more specific term.</skos:scopeNote>
		<cc:license rdf:resource="http://creativecommons.org/licenses/by/3.0" />
		<cc:attributionURL rdf:resource="http://www.english-heritage.org.uk" />
		<cc:attributionName xml:lang="en">English Heritage</cc:attributionName>
		<dcterms:publisher rdf:resource="http://www.english-heritage.org.uk" />
	</skos:Concept>
	<skos:Concept rdf:about="http://purl.org/heritagedata/schemes/eh_tmc/concepts/146425">
		<skos:inScheme rdf:resource="http://purl.org/heritagedata/schemes/eh_tmc" />
		<dcterms:identifier>http://purl.org/heritagedata/schemes/eh_tmc/concepts/146425</dcterms:identifier>
		<skos:prefLabel xml:lang="en">LONGSHIP</skos:prefLabel>
		<dcterms:issued rdf:datatype="http://www.w3.org/2001/XMLSchema#dateTime">2013-07-17T09:01:43</dcterms:issued>
		<skos:broader rdf:resource="http://purl.org/heritagedata/schemes/eh_tmc/concepts/100490" />
		<skos:related rdf:resource="http://purl.org/heritagedata/schemes/eh_tmc/concepts/100355" />
		<skos:scopeNote xml:lang="en">A term for any vessel powered principally by sail and oars, or oars alone, used especially for war. As a broad term it may refer to Roman galleys, or more specifically to an Anglo-Saxon or Norse warship of the Viking Age.</skos:scopeNote>
		<cc:license rdf:resource="http://creativecommons.org/licenses/by/3.0" />
		<cc:attributionURL rdf:resource="http://www.english-heritage.org.uk" />
		<cc:attributionName xml:lang="en">English Heritage</cc:attributionName>
		<dcterms:publisher rdf:resource="http://www.english-heritage.org.uk" />
	</skos:Concept>
	<skos:Concept rdf:about="http://purl.org/heritagedata/schemes/eh_tmc/concepts/152307">
		<skos:inScheme rdf:resource="http://purl.org/heritagedata/schemes/eh_tmc" />
		<dcterms:identifier>http://purl.org/heritagedata/schemes/eh_tmc/concepts/152307</dcterms:identifier>
		<skos:prefLabel xml:lang="en">VICTORY SHIP</skos:prefLabel>
		<dcterms:issued rdf:datatype="http://www.w3.org/2001/XMLSchema#dateTime">2013-07-17T09:01:43</dcterms:issued>
		<skos:broader rdf:resource="http://purl.org/heritagedata/schemes/eh_tmc/concepts/100295" />
		<skos:related rdf:resource="http://purl.org/heritagedata/schemes/eh_tmc/concepts/100383" />
		<skos:scopeNote xml:lang="en">A prefabricated cargo vessel produced in large numbers by North American shipyards during World War II to replace shipping losses caused by German submarines and replacing the earlier 'LIBERTY' ships.</skos:scopeNote>
		<cc:license rdf:resource="http://creativecommons.org/licenses/by/3.0" />
		<cc:attributionURL rdf:resource="http://www.english-heritage.org.uk" />
		<cc:attributionName xml:lang="en">English Heritage</cc:attributionName>
		<dcterms:publisher rdf:resource="http://www.english-heritage.org.uk" />
	</skos:Concept>
	<skos:Concept rdf:about="http://purl.org/heritagedata/schemes/eh_tmc/concepts/160144">
		<skos:inScheme rdf:resource="http://purl.org/heritagedata/schemes/eh_tmc" />
		<dcterms:identifier>http://purl.org/heritagedata/schemes/eh_tmc/concepts/160144</dcterms:identifier>
		<skos:prefLabel xml:lang="en">DINGHY</skos:prefLabel>
		<dcterms:issued rdf:datatype="http://www.w3.org/2001/XMLSchema#dateTime">2013-07-17T09:01:43</dcterms:issued>
		<skos:broader rdf:resource="http://purl.org/heritagedata/schemes/eh_tmc/concepts/100474" />
		<skos:broader rdf:resource="http://purl.org/heritagedata/schemes/eh_tmc/concepts/141805" />
		<skos:broader rdf:resource="http://purl.org/heritagedata/schemes/eh_tmc/concepts/100382" />
		<skos:scopeNote xml:lang="en">A type of small boat that was often carried, or towed by a larger vessel and used as a ship's boat. Dinghies can also be used recreationally as independent sailing vessels.</skos:scopeNote>
		<cc:license rdf:resource="http://creativecommons.org/licenses/by/3.0" />
		<cc:attributionURL rdf:resource="http://www.english-heritage.org.uk" />
		<cc:attributionName xml:lang="en">English Heritage</cc:attributionName>
		<dcterms:publisher rdf:resource="http://www.english-heritage.org.uk" />
	</skos:Concept>
	<skos:Concept rdf:about="http://purl.org/heritagedata/schemes/eh_tmc/concepts/160147">
		<skos:inScheme rdf:resource="http://purl.org/heritagedata/schemes/eh_tmc" />
		<dcterms:identifier>http://purl.org/heritagedata/schemes/eh_tmc/concepts/160147</dcterms:identifier>
		<skos:prefLabel xml:lang="en">MINE COUNTERMEASURE VESSEL</skos:prefLabel>
		<dcterms:issued rdf:datatype="http://www.w3.org/2001/XMLSchema#dateTime">2013-07-17T09:01:43</dcterms:issued>
		<skos:broader rdf:resource="http://purl.org/heritagedata/schemes/eh_tmc/concepts/100490" />
		<skos:narrower>
			<skos:Concept rdf:about="http://purl.org/heritagedata/schemes/eh_tmc/concepts/160145">
				<skos:inScheme rdf:resource="http://purl.org/heritagedata/schemes/eh_tmc" />
				<dcterms:identifier>http://purl.org/heritagedata/schemes/eh_tmc/concepts/160145</dcterms:identifier>
				<skos:prefLabel xml:lang="en">MINEHUNTER</skos:prefLabel>
				<dcterms:issued rdf:datatype="http://www.w3.org/2001/XMLSchema#dateTime">2013-07-17T09:01:43</dcterms:issued>
				<skos:altLabel xml:lang="en">Mine Hunter</skos:altLabel>
				<skos:broader rdf:resource="http://purl.org/heritagedata/schemes/eh_tmc/concepts/160147" />
				<skos:scopeNote xml:lang="en">A mine countermeasure vessel built to detect and destroy individual naval mines. (See Minesweeper for vessels that sweep and explode mined areas at sea without prior detection).</skos:scopeNote>
				<cc:license rdf:resource="http://creativecommons.org/licenses/by/3.0" />
				<cc:attributionURL rdf:resource="http://www.english-heritage.org.uk" />
				<cc:attributionName xml:lang="en">English Heritage</cc:attributionName>
				<dcterms:publisher rdf:resource="http://www.english-heritage.org.uk" />
			</skos:Concept>
		</skos:narrower>
		<skos:narrower>
			<skos:Concept rdf:about="http://purl.org/heritagedata/schemes/eh_tmc/concepts/100401">
				<skos:inScheme rdf:resource="http://purl.org/heritagedata/schemes/eh_tmc" />
				<dcterms:identifier>http://purl.org/heritagedata/schemes/eh_tmc/concepts/100401</dcterms:identifier>
				<skos:prefLabel xml:lang="en">MINESWEEPER</skos:prefLabel>
				<dcterms:issued rdf:datatype="http://www.w3.org/2001/XMLSchema#dateTime">2013-07-17T09:01:43</dcterms:issued>
				<skos:altLabel xml:lang="en">Mine Sweeper</skos:altLabel>
				<skos:altLabel xml:lang="en">Ascot Class Minesweeper</skos:altLabel>
				<skos:altLabel xml:lang="en">Auxiliary Minesweeper</skos:altLabel>
				<skos:broader rdf:resource="http://purl.org/heritagedata/schemes/eh_tmc/concepts/160147" />
				<skos:scopeNote xml:lang="en">A vessel designed or adapted to sweep and explode mined areas at sea without prior detection. (See Minehunter for vessels that detect and destroy individual mines).</skos:scopeNote>
				<cc:license rdf:resource="http://creativecommons.org/licenses/by/3.0" />
				<cc:attributionURL rdf:resource="http://www.english-heritage.org.uk" />
				<cc:attributionName xml:lang="en">English Heritage</cc:attributionName>
				<dcterms:publisher rdf:resource="http://www.english-heritage.org.uk" />
			</skos:Concept>
		</skos:narrower>
		<skos:scopeNote xml:lang="en">A vessel designed or adapted for the task of keeping shipping lanes and ports free from the threat of naval mines. Use specific type where known. of</skos:scopeNote>
		<cc:license rdf:resource="http://creativecommons.org/licenses/by/3.0" />
		<cc:attributionURL rdf:resource="http://www.english-heritage.org.uk" />
		<cc:attributionName xml:lang="en">English Heritage</cc:attributionName>
		<dcterms:publisher rdf:resource="http://www.english-heritage.org.uk" />
	</skos:Concept>
	<skos:Concept rdf:about="http://purl.org/heritagedata/schemes/eh_tmc/concepts/159232">
		<skos:inScheme rdf:resource="http://purl.org/heritagedata/schemes/eh_tmc" />
		<dcterms:identifier>http://purl.org/heritagedata/schemes/eh_tmc/concepts/159232</dcterms:identifier>
		<skos:prefLabel xml:lang="en">SCREW STEAMER</skos:prefLabel>
		<dcterms:issued rdf:datatype="http://www.w3.org/2001/XMLSchema#dateTime">2013-07-17T09:01:43</dcterms:issued>
		<skos:broader rdf:resource="http://purl.org/heritagedata/schemes/eh_tmc/concepts/100394" />
		<skos:related rdf:resource="http://purl.org/heritagedata/schemes/eh_tmc/concepts/100418" />
		<skos:scopeNote xml:lang="en">A steam vessel propelled by rotating propellers called screws.</skos:scopeNote>
		<cc:license rdf:resource="http://creativecommons.org/licenses/by/3.0" />
		<cc:attributionURL rdf:resource="http://www.english-heritage.org.uk" />
		<cc:attributionName xml:lang="en">English Heritage</cc:attributionName>
		<dcterms:publisher rdf:resource="http://www.english-heritage.org.uk" />
	</skos:Concept>
</rdf:RDF>