<?xml version="1.0"?>
<rdf:RDF xmlns:dc="http://purl.org/dc/elements/1.1/" xmlns:owl="http://www.w3.org/2002/07/owl#" xmlns:skosxl="http://www.w3.org/2008/05/skos-xl#" xmlns:rdfs="http://www.w3.org/2000/01/rdf-schema#" xmlns:dcterms="http://purl.org/dc/terms/" xmlns:xsd="http://www.w3.org/2001/XMLSchema#" xmlns:rdf="http://www.w3.org/1999/02/22-rdf-syntax-ns#" xmlns:cc="http://creativecommons.org/ns#" xmlns:skos="http://www.w3.org/2004/02/skos/core#" xml:base="http://stellar/">
	<skos:ConceptScheme rdf:about="http://purl.org/heritagedata/schemes/eh_tbm">
		<dcterms:identifier>http://purl.org/heritagedata/schemes/eh_tbm</dcterms:identifier>
		<cc:license rdf:resource="http://creativecommons.org/licenses/by/3.0" />
		<cc:attributionURL rdf:resource="http://www.english-heritage.org.uk" />
		<cc:attributionName xml:lang="en">English Heritage</cc:attributionName>
		<dcterms:title xml:lang="en">BUILDING MATERIALS (EH)</dcterms:title>
		<rdfs:label xml:lang="en">BUILDING MATERIALS (EH)</rdfs:label>
		<dcterms:description xml:lang="en">Thesaurus of main constructional material types (eg. the walls) for indexing of monuments.</dcterms:description>
		<dcterms:coverage rdf:resource="http://data.ordnancesurvey.co.uk/id/country/england" />
		<dcterms:publisher rdf:resource="http://www.english-heritage.org.uk" />
		<dcterms:issued rdf:datatype="http://www.w3.org/2001/XMLSchema#dateTime">2013-07-17T09:02:16</dcterms:issued>
		<skos:hasTopConcept>
			<skos:Concept rdf:about="http://purl.org/heritagedata/schemes/eh_tbm/concepts/98041">
				<skos:topConceptOf rdf:resource="http://purl.org/heritagedata/schemes/eh_tbm" />
				<skos:inScheme rdf:resource="http://purl.org/heritagedata/schemes/eh_tbm" />
				<dcterms:identifier>http://purl.org/heritagedata/schemes/eh_tbm/concepts/98041</dcterms:identifier>
				<skos:prefLabel xml:lang="en">MAN MADE MATERIAL</skos:prefLabel>
				<dcterms:issued rdf:datatype="http://www.w3.org/2001/XMLSchema#dateTime">2013-07-17T09:02:16</dcterms:issued>
				<skos:narrower rdf:resource="http://purl.org/heritagedata/schemes/eh_tbm/concepts/97717" />
				<skos:narrower>
					<skos:Concept rdf:about="http://purl.org/heritagedata/schemes/eh_tbm/concepts/97718">
						<skos:inScheme rdf:resource="http://purl.org/heritagedata/schemes/eh_tbm" />
						<dcterms:identifier>http://purl.org/heritagedata/schemes/eh_tbm/concepts/97718</dcterms:identifier>
						<skos:prefLabel xml:lang="en">ARTIFICIAL TIMBER</skos:prefLabel>
						<dcterms:issued rdf:datatype="http://www.w3.org/2001/XMLSchema#dateTime">2013-07-17T09:02:16</dcterms:issued>
						<skos:broader rdf:resource="http://purl.org/heritagedata/schemes/eh_tbm/concepts/98041" />
						<skos:scopeNote xml:lang="en">Synthetic fibres and reconstituted materials imitating, or in the form of, timber created by a man-made process. Use carefully - do not confuse with mock and sham timber work.</skos:scopeNote>
						<cc:license rdf:resource="http://creativecommons.org/licenses/by/3.0" />
						<cc:attributionURL rdf:resource="http://www.english-heritage.org.uk" />
						<cc:attributionName xml:lang="en">English Heritage</cc:attributionName>
						<dcterms:publisher rdf:resource="http://www.english-heritage.org.uk" />
					</skos:Concept>
				</skos:narrower>
				<skos:narrower>
					<skos:Concept rdf:about="http://purl.org/heritagedata/schemes/eh_tbm/concepts/97719">
						<skos:inScheme rdf:resource="http://purl.org/heritagedata/schemes/eh_tbm" />
						<dcterms:identifier>http://purl.org/heritagedata/schemes/eh_tbm/concepts/97719</dcterms:identifier>
						<skos:prefLabel xml:lang="en">ASBESTOS</skos:prefLabel>
						<dcterms:issued rdf:datatype="http://www.w3.org/2001/XMLSchema#dateTime">2013-07-17T09:02:16</dcterms:issued>
						<skos:altLabel xml:lang="en">Asbestos Slate</skos:altLabel>
						<skos:altLabel xml:lang="en">Corrugated Asbestos</skos:altLabel>
						<skos:broader rdf:resource="http://purl.org/heritagedata/schemes/eh_tbm/concepts/98041" />
						<skos:scopeNote xml:lang="en">A mineral crystal of thin, tough fibres which can be woven. Used for high temperature insulation or as reinforcement in asbestos cement building board and corrugated roofing. If used to imitate slate, use artificial slate also.</skos:scopeNote>
						<cc:license rdf:resource="http://creativecommons.org/licenses/by/3.0" />
						<cc:attributionURL rdf:resource="http://www.english-heritage.org.uk" />
						<cc:attributionName xml:lang="en">English Heritage</cc:attributionName>
						<dcterms:publisher rdf:resource="http://www.english-heritage.org.uk" />
					</skos:Concept>
				</skos:narrower>
				<skos:narrower rdf:resource="http://purl.org/heritagedata/schemes/eh_tbm/concepts/97749" />
				<skos:narrower>
					<skos:Concept rdf:about="http://purl.org/heritagedata/schemes/eh_tbm/concepts/97750">
						<skos:inScheme rdf:resource="http://purl.org/heritagedata/schemes/eh_tbm" />
						<dcterms:identifier>http://purl.org/heritagedata/schemes/eh_tbm/concepts/97750</dcterms:identifier>
						<skos:prefLabel xml:lang="en">BITUMINOUS FELT</skos:prefLabel>
						<dcterms:issued rdf:datatype="http://www.w3.org/2001/XMLSchema#dateTime">2013-07-17T09:02:16</dcterms:issued>
						<skos:altLabel xml:lang="en">Roofing Felt</skos:altLabel>
						<skos:broader rdf:resource="http://purl.org/heritagedata/schemes/eh_tbm/concepts/98041" />
						<skos:scopeNote xml:lang="en">A material made of felted fibres bonded by bitumen. Often used as a roofing material.</skos:scopeNote>
						<cc:license rdf:resource="http://creativecommons.org/licenses/by/3.0" />
						<cc:attributionURL rdf:resource="http://www.english-heritage.org.uk" />
						<cc:attributionName xml:lang="en">English Heritage</cc:attributionName>
						<dcterms:publisher rdf:resource="http://www.english-heritage.org.uk" />
					</skos:Concept>
				</skos:narrower>
				<skos:narrower rdf:resource="http://purl.org/heritagedata/schemes/eh_tbm/concepts/97810" />
				<skos:narrower rdf:resource="http://purl.org/heritagedata/schemes/eh_tbm/concepts/97813" />
				<skos:narrower>
					<skos:Concept rdf:about="http://purl.org/heritagedata/schemes/eh_tbm/concepts/140459">
						<skos:inScheme rdf:resource="http://purl.org/heritagedata/schemes/eh_tbm" />
						<dcterms:identifier>http://purl.org/heritagedata/schemes/eh_tbm/concepts/140459</dcterms:identifier>
						<skos:prefLabel xml:lang="en">ETHYLTETRAFLUOROETHYLENE FOIL</skos:prefLabel>
						<dcterms:issued rdf:datatype="http://www.w3.org/2001/XMLSchema#dateTime">2013-07-17T09:02:16</dcterms:issued>
						<skos:altLabel xml:lang="en">Efte Foil</skos:altLabel>
						<skos:broader rdf:resource="http://purl.org/heritagedata/schemes/eh_tbm/concepts/98041" />
						<skos:scopeNote xml:lang="en">Extremely thin foil made out of ethyltetraflouroethylene, a modified copolymer which is extruded into a thin film and which is related to Teflon. It has a very high level of light transmission in visible and ultra violet range. Used instead of glass.</skos:scopeNote>
						<cc:license rdf:resource="http://creativecommons.org/licenses/by/3.0" />
						<cc:attributionURL rdf:resource="http://www.english-heritage.org.uk" />
						<cc:attributionName xml:lang="en">English Heritage</cc:attributionName>
						<dcterms:publisher rdf:resource="http://www.english-heritage.org.uk" />
					</skos:Concept>
				</skos:narrower>
				<skos:narrower>
					<skos:Concept rdf:about="http://purl.org/heritagedata/schemes/eh_tbm/concepts/97918">
						<skos:inScheme rdf:resource="http://purl.org/heritagedata/schemes/eh_tbm" />
						<dcterms:identifier>http://purl.org/heritagedata/schemes/eh_tbm/concepts/97918</dcterms:identifier>
						<skos:prefLabel xml:lang="en">FIBREGLASS</skos:prefLabel>
						<dcterms:issued rdf:datatype="http://www.w3.org/2001/XMLSchema#dateTime">2013-07-17T09:02:16</dcterms:issued>
						<skos:broader rdf:resource="http://purl.org/heritagedata/schemes/eh_tbm/concepts/98041" />
						<skos:scopeNote xml:lang="en">Any material consisting of glass filaments woven into textiles, paper or board.</skos:scopeNote>
						<cc:license rdf:resource="http://creativecommons.org/licenses/by/3.0" />
						<cc:attributionURL rdf:resource="http://www.english-heritage.org.uk" />
						<cc:attributionName xml:lang="en">English Heritage</cc:attributionName>
						<dcterms:publisher rdf:resource="http://www.english-heritage.org.uk" />
					</skos:Concept>
				</skos:narrower>
				<skos:narrower rdf:resource="http://purl.org/heritagedata/schemes/eh_tbm/concepts/97939" />
				<skos:narrower rdf:resource="http://purl.org/heritagedata/schemes/eh_tbm/concepts/98080" />
				<skos:narrower rdf:resource="http://purl.org/heritagedata/schemes/eh_tbm/concepts/98082" />
				<skos:narrower rdf:resource="http://purl.org/heritagedata/schemes/eh_tbm/concepts/98111" />
				<skos:narrower rdf:resource="http://purl.org/heritagedata/schemes/eh_tbm/concepts/98147" />
				<skos:narrower rdf:resource="http://purl.org/heritagedata/schemes/eh_tbm/concepts/98148" />
				<skos:narrower rdf:resource="http://purl.org/heritagedata/schemes/eh_tbm/concepts/98164" />
				<skos:scopeNote xml:lang="en">A material or combination of materials manufactured by human effort, or fashioned into shape by man or a man made industrial process (excluding metal). See MAN MADE MATERIAL Class List for narrow terms.</skos:scopeNote>
				<cc:license rdf:resource="http://creativecommons.org/licenses/by/3.0" />
				<cc:attributionURL rdf:resource="http://www.english-heritage.org.uk" />
				<cc:attributionName xml:lang="en">English Heritage</cc:attributionName>
				<dcterms:publisher rdf:resource="http://www.english-heritage.org.uk" />
			</skos:Concept>
		</skos:hasTopConcept>
		<skos:hasTopConcept>
			<skos:Concept rdf:about="http://purl.org/heritagedata/schemes/eh_tbm/concepts/98046">
				<skos:topConceptOf rdf:resource="http://purl.org/heritagedata/schemes/eh_tbm" />
				<skos:inScheme rdf:resource="http://purl.org/heritagedata/schemes/eh_tbm" />
				<dcterms:identifier>http://purl.org/heritagedata/schemes/eh_tbm/concepts/98046</dcterms:identifier>
				<skos:prefLabel xml:lang="en">MATERIAL &lt;BY FORM&gt;</skos:prefLabel>
				<dcterms:issued rdf:datatype="http://www.w3.org/2001/XMLSchema#dateTime">2013-07-17T09:02:16</dcterms:issued>
				<skos:narrower>
					<skos:Concept rdf:about="http://purl.org/heritagedata/schemes/eh_tbm/concepts/97716">
						<skos:inScheme rdf:resource="http://purl.org/heritagedata/schemes/eh_tbm" />
						<dcterms:identifier>http://purl.org/heritagedata/schemes/eh_tbm/concepts/97716</dcterms:identifier>
						<skos:prefLabel xml:lang="en">ARTIFICIAL SLATE</skos:prefLabel>
						<dcterms:issued rdf:datatype="http://www.w3.org/2001/XMLSchema#dateTime">2013-07-17T09:02:16</dcterms:issued>
						<skos:altLabel xml:lang="en">Asbestos Slate</skos:altLabel>
						<skos:broader rdf:resource="http://purl.org/heritagedata/schemes/eh_tbm/concepts/98046" />
						<skos:scopeNote xml:lang="en">A rectangular sheet of roofing material created by a man made process (eg. asbestos cement slate) and made to look like, and used in the same way as, natural slate.</skos:scopeNote>
						<cc:license rdf:resource="http://creativecommons.org/licenses/by/3.0" />
						<cc:attributionURL rdf:resource="http://www.english-heritage.org.uk" />
						<cc:attributionName xml:lang="en">English Heritage</cc:attributionName>
						<dcterms:publisher rdf:resource="http://www.english-heritage.org.uk" />
					</skos:Concept>
				</skos:narrower>
				<skos:narrower>
					<skos:Concept rdf:about="http://purl.org/heritagedata/schemes/eh_tbm/concepts/97722">
						<skos:inScheme rdf:resource="http://purl.org/heritagedata/schemes/eh_tbm" />
						<dcterms:identifier>http://purl.org/heritagedata/schemes/eh_tbm/concepts/97722</dcterms:identifier>
						<skos:prefLabel xml:lang="en">ASHLAR</skos:prefLabel>
						<dcterms:issued rdf:datatype="http://www.w3.org/2001/XMLSchema#dateTime">2013-07-17T09:02:16</dcterms:issued>
						<skos:broader rdf:resource="http://purl.org/heritagedata/schemes/eh_tbm/concepts/98046" />
						<skos:scopeNote xml:lang="en">A square, hewn or worked, high class freestone which can be 'freely' cut and is laid in horizontal courses with vertical joints.</skos:scopeNote>
						<cc:license rdf:resource="http://creativecommons.org/licenses/by/3.0" />
						<cc:attributionURL rdf:resource="http://www.english-heritage.org.uk" />
						<cc:attributionName xml:lang="en">English Heritage</cc:attributionName>
						<dcterms:publisher rdf:resource="http://www.english-heritage.org.uk" />
					</skos:Concept>
				</skos:narrower>
				<skos:narrower rdf:resource="http://purl.org/heritagedata/schemes/eh_tbm/concepts/97777" />
				<skos:narrower>
					<skos:Concept rdf:about="http://purl.org/heritagedata/schemes/eh_tbm/concepts/97798">
						<skos:inScheme rdf:resource="http://purl.org/heritagedata/schemes/eh_tbm" />
						<dcterms:identifier>http://purl.org/heritagedata/schemes/eh_tbm/concepts/97798</dcterms:identifier>
						<skos:prefLabel xml:lang="en">CANVAS</skos:prefLabel>
						<dcterms:issued rdf:datatype="http://www.w3.org/2001/XMLSchema#dateTime">2013-07-17T09:02:16</dcterms:issued>
						<skos:broader rdf:resource="http://purl.org/heritagedata/schemes/eh_tbm/concepts/98046" />
						<skos:scopeNote xml:lang="en">An unbleached cloth of hemp, flax or other coarse yarn.</skos:scopeNote>
						<cc:license rdf:resource="http://creativecommons.org/licenses/by/3.0" />
						<cc:attributionURL rdf:resource="http://www.english-heritage.org.uk" />
						<cc:attributionName xml:lang="en">English Heritage</cc:attributionName>
						<dcterms:publisher rdf:resource="http://www.english-heritage.org.uk" />
					</skos:Concept>
				</skos:narrower>
				<skos:narrower rdf:resource="http://purl.org/heritagedata/schemes/eh_tbm/concepts/97836" />
				<skos:narrower rdf:resource="http://purl.org/heritagedata/schemes/eh_tbm/concepts/97876" />
				<skos:narrower rdf:resource="http://purl.org/heritagedata/schemes/eh_tbm/concepts/97947" />
				<skos:narrower rdf:resource="http://purl.org/heritagedata/schemes/eh_tbm/concepts/98089" />
				<skos:narrower rdf:resource="http://purl.org/heritagedata/schemes/eh_tbm/concepts/98165" />
				<skos:narrower>
					<skos:Concept rdf:about="http://purl.org/heritagedata/schemes/eh_tbm/concepts/98237">
						<skos:inScheme rdf:resource="http://purl.org/heritagedata/schemes/eh_tbm" />
						<dcterms:identifier>http://purl.org/heritagedata/schemes/eh_tbm/concepts/98237</dcterms:identifier>
						<skos:prefLabel xml:lang="en">TESSERA</skos:prefLabel>
						<dcterms:issued rdf:datatype="http://www.w3.org/2001/XMLSchema#dateTime">2013-07-17T09:02:16</dcterms:issued>
						<skos:altLabel xml:lang="en">Mosaic</skos:altLabel>
						<skos:broader rdf:resource="http://purl.org/heritagedata/schemes/eh_tbm/concepts/98046" />
						<skos:scopeNote xml:lang="en">Squared block of glass, tile, stone or marble used in mosaic.</skos:scopeNote>
						<cc:license rdf:resource="http://creativecommons.org/licenses/by/3.0" />
						<cc:attributionURL rdf:resource="http://www.english-heritage.org.uk" />
						<cc:attributionName xml:lang="en">English Heritage</cc:attributionName>
						<dcterms:publisher rdf:resource="http://www.english-heritage.org.uk" />
					</skos:Concept>
				</skos:narrower>
				<skos:narrower rdf:resource="http://purl.org/heritagedata/schemes/eh_tbm/concepts/98239" />
				<skos:narrower rdf:resource="http://purl.org/heritagedata/schemes/eh_tbm/concepts/98241" />
				<skos:narrower rdf:resource="http://purl.org/heritagedata/schemes/eh_tbm/concepts/98242" />
				<skos:scopeNote xml:lang="en">A raw material determined by its form or a finished product material characterised by its end shape or form. See MATERIAL &lt;BY FORM&gt; Class List for narrow terms.</skos:scopeNote>
				<cc:license rdf:resource="http://creativecommons.org/licenses/by/3.0" />
				<cc:attributionURL rdf:resource="http://www.english-heritage.org.uk" />
				<cc:attributionName xml:lang="en">English Heritage</cc:attributionName>
				<dcterms:publisher rdf:resource="http://www.english-heritage.org.uk" />
			</skos:Concept>
		</skos:hasTopConcept>
		<skos:hasTopConcept>
			<skos:Concept rdf:about="http://purl.org/heritagedata/schemes/eh_tbm/concepts/98053">
				<skos:topConceptOf rdf:resource="http://purl.org/heritagedata/schemes/eh_tbm" />
				<skos:inScheme rdf:resource="http://purl.org/heritagedata/schemes/eh_tbm" />
				<dcterms:identifier>http://purl.org/heritagedata/schemes/eh_tbm/concepts/98053</dcterms:identifier>
				<skos:prefLabel xml:lang="en">METAL</skos:prefLabel>
				<dcterms:issued rdf:datatype="http://www.w3.org/2001/XMLSchema#dateTime">2013-07-17T09:02:16</dcterms:issued>
				<skos:narrower rdf:resource="http://purl.org/heritagedata/schemes/eh_tbm/concepts/97708" />
				<skos:narrower>
					<skos:Concept rdf:about="http://purl.org/heritagedata/schemes/eh_tbm/concepts/97772">
						<skos:inScheme rdf:resource="http://purl.org/heritagedata/schemes/eh_tbm" />
						<dcterms:identifier>http://purl.org/heritagedata/schemes/eh_tbm/concepts/97772</dcterms:identifier>
						<skos:prefLabel xml:lang="en">BRASS</skos:prefLabel>
						<dcterms:issued rdf:datatype="http://www.w3.org/2001/XMLSchema#dateTime">2013-07-17T09:02:16</dcterms:issued>
						<skos:broader rdf:resource="http://purl.org/heritagedata/schemes/eh_tbm/concepts/98053" />
						<skos:scopeNote xml:lang="en">Easily formed metal alloy composed of copper and zinc.</skos:scopeNote>
						<cc:license rdf:resource="http://creativecommons.org/licenses/by/3.0" />
						<cc:attributionURL rdf:resource="http://www.english-heritage.org.uk" />
						<cc:attributionName xml:lang="en">English Heritage</cc:attributionName>
						<dcterms:publisher rdf:resource="http://www.english-heritage.org.uk" />
					</skos:Concept>
				</skos:narrower>
				<skos:narrower rdf:resource="http://purl.org/heritagedata/schemes/eh_tbm/concepts/97779" />
				<skos:narrower rdf:resource="http://purl.org/heritagedata/schemes/eh_tbm/concepts/97845" />
				<skos:narrower>
					<skos:Concept rdf:about="http://purl.org/heritagedata/schemes/eh_tbm/concepts/97942">
						<skos:inScheme rdf:resource="http://purl.org/heritagedata/schemes/eh_tbm" />
						<dcterms:identifier>http://purl.org/heritagedata/schemes/eh_tbm/concepts/97942</dcterms:identifier>
						<skos:prefLabel xml:lang="en">GOLD</skos:prefLabel>
						<dcterms:issued rdf:datatype="http://www.w3.org/2001/XMLSchema#dateTime">2013-07-17T09:02:16</dcterms:issued>
						<skos:broader rdf:resource="http://purl.org/heritagedata/schemes/eh_tbm/concepts/98053" />
						<skos:scopeNote xml:lang="en">A precious metal characterised by its yellow colour and resistance to tarnishing.</skos:scopeNote>
						<cc:license rdf:resource="http://creativecommons.org/licenses/by/3.0" />
						<cc:attributionURL rdf:resource="http://www.english-heritage.org.uk" />
						<cc:attributionName xml:lang="en">English Heritage</cc:attributionName>
						<dcterms:publisher rdf:resource="http://www.english-heritage.org.uk" />
					</skos:Concept>
				</skos:narrower>
				<skos:narrower rdf:resource="http://purl.org/heritagedata/schemes/eh_tbm/concepts/97992" />
				<skos:narrower rdf:resource="http://purl.org/heritagedata/schemes/eh_tbm/concepts/98022" />
				<skos:narrower>
					<skos:Concept rdf:about="http://purl.org/heritagedata/schemes/eh_tbm/concepts/98189">
						<skos:inScheme rdf:resource="http://purl.org/heritagedata/schemes/eh_tbm" />
						<dcterms:identifier>http://purl.org/heritagedata/schemes/eh_tbm/concepts/98189</dcterms:identifier>
						<skos:prefLabel xml:lang="en">SILVER</skos:prefLabel>
						<dcterms:issued rdf:datatype="http://www.w3.org/2001/XMLSchema#dateTime">2013-07-17T09:02:16</dcterms:issued>
						<skos:broader rdf:resource="http://purl.org/heritagedata/schemes/eh_tbm/concepts/98053" />
						<skos:scopeNote xml:lang="en">A precious metal of lustrous white colour with great malleability and ductility.</skos:scopeNote>
						<cc:license rdf:resource="http://creativecommons.org/licenses/by/3.0" />
						<cc:attributionURL rdf:resource="http://www.english-heritage.org.uk" />
						<cc:attributionName xml:lang="en">English Heritage</cc:attributionName>
						<dcterms:publisher rdf:resource="http://www.english-heritage.org.uk" />
					</skos:Concept>
				</skos:narrower>
				<skos:narrower rdf:resource="http://purl.org/heritagedata/schemes/eh_tbm/concepts/98213" />
				<skos:narrower rdf:resource="http://purl.org/heritagedata/schemes/eh_tbm/concepts/98243" />
				<skos:narrower>
					<skos:Concept rdf:about="http://purl.org/heritagedata/schemes/eh_tbm/concepts/98312">
						<skos:inScheme rdf:resource="http://purl.org/heritagedata/schemes/eh_tbm" />
						<dcterms:identifier>http://purl.org/heritagedata/schemes/eh_tbm/concepts/98312</dcterms:identifier>
						<skos:prefLabel xml:lang="en">ZINC</skos:prefLabel>
						<dcterms:issued rdf:datatype="http://www.w3.org/2001/XMLSchema#dateTime">2013-07-17T09:02:16</dcterms:issued>
						<skos:broader rdf:resource="http://purl.org/heritagedata/schemes/eh_tbm/concepts/98053" />
						<skos:scopeNote xml:lang="en">A hard and lustrous metallic element, used for roofing, galvanising iron and a component of alloys such as brass.</skos:scopeNote>
						<cc:license rdf:resource="http://creativecommons.org/licenses/by/3.0" />
						<cc:attributionURL rdf:resource="http://www.english-heritage.org.uk" />
						<cc:attributionName xml:lang="en">English Heritage</cc:attributionName>
						<dcterms:publisher rdf:resource="http://www.english-heritage.org.uk" />
					</skos:Concept>
				</skos:narrower>
				<skos:related rdf:resource="http://purl.org/heritagedata/schemes/eh_tbm/concepts/98113" />
				<skos:scopeNote xml:lang="en">Class of elements and alloys that are characteristically lustrous,ductile, fusible and malleable. These are extracted from ore minerals originally existing in nature and processed before becoming a recognisable metal. See METAL Class List for narrow terms</skos:scopeNote>
				<cc:license rdf:resource="http://creativecommons.org/licenses/by/3.0" />
				<cc:attributionURL rdf:resource="http://www.english-heritage.org.uk" />
				<cc:attributionName xml:lang="en">English Heritage</cc:attributionName>
				<dcterms:publisher rdf:resource="http://www.english-heritage.org.uk" />
			</skos:Concept>
		</skos:hasTopConcept>
		<skos:hasTopConcept>
			<skos:Concept rdf:about="http://purl.org/heritagedata/schemes/eh_tbm/concepts/98058">
				<skos:topConceptOf rdf:resource="http://purl.org/heritagedata/schemes/eh_tbm" />
				<skos:inScheme rdf:resource="http://purl.org/heritagedata/schemes/eh_tbm" />
				<dcterms:identifier>http://purl.org/heritagedata/schemes/eh_tbm/concepts/98058</dcterms:identifier>
				<skos:prefLabel xml:lang="en">MINERAL</skos:prefLabel>
				<dcterms:issued rdf:datatype="http://www.w3.org/2001/XMLSchema#dateTime">2013-07-17T09:02:16</dcterms:issued>
				<skos:narrower rdf:resource="http://purl.org/heritagedata/schemes/eh_tbm/concepts/97892" />
				<skos:narrower>
					<skos:Concept rdf:about="http://purl.org/heritagedata/schemes/eh_tbm/concepts/97915">
						<skos:inScheme rdf:resource="http://purl.org/heritagedata/schemes/eh_tbm" />
						<dcterms:identifier>http://purl.org/heritagedata/schemes/eh_tbm/concepts/97915</dcterms:identifier>
						<skos:prefLabel xml:lang="en">FELDSPAR</skos:prefLabel>
						<dcterms:issued rdf:datatype="http://www.w3.org/2001/XMLSchema#dateTime">2013-07-17T09:02:16</dcterms:issued>
						<skos:broader rdf:resource="http://purl.org/heritagedata/schemes/eh_tbm/concepts/98058" />
						<skos:scopeNote xml:lang="en">Hard, often coloured, can be transparent. Found on its own as crystals and veins but also as a major constituent of all three geological rock types.</skos:scopeNote>
						<cc:license rdf:resource="http://creativecommons.org/licenses/by/3.0" />
						<cc:attributionURL rdf:resource="http://www.english-heritage.org.uk" />
						<cc:attributionName xml:lang="en">English Heritage</cc:attributionName>
						<dcterms:publisher rdf:resource="http://www.english-heritage.org.uk" />
					</skos:Concept>
				</skos:narrower>
				<skos:narrower>
					<skos:Concept rdf:about="http://purl.org/heritagedata/schemes/eh_tbm/concepts/97923">
						<skos:inScheme rdf:resource="http://purl.org/heritagedata/schemes/eh_tbm" />
						<dcterms:identifier>http://purl.org/heritagedata/schemes/eh_tbm/concepts/97923</dcterms:identifier>
						<skos:prefLabel xml:lang="en">FLUORITE</skos:prefLabel>
						<dcterms:issued rdf:datatype="http://www.w3.org/2001/XMLSchema#dateTime">2013-07-17T09:02:16</dcterms:issued>
						<skos:altLabel xml:lang="en">Fluorspar</skos:altLabel>
						<skos:broader rdf:resource="http://purl.org/heritagedata/schemes/eh_tbm/concepts/98058" />
						<skos:scopeNote xml:lang="en">Soft mineral, colour varying from black/purple to yellow/green. Commonly found as a mineral vein.</skos:scopeNote>
						<cc:license rdf:resource="http://creativecommons.org/licenses/by/3.0" />
						<cc:attributionURL rdf:resource="http://www.english-heritage.org.uk" />
						<cc:attributionName xml:lang="en">English Heritage</cc:attributionName>
						<dcterms:publisher rdf:resource="http://www.english-heritage.org.uk" />
					</skos:Concept>
				</skos:narrower>
				<skos:narrower>
					<skos:Concept rdf:about="http://purl.org/heritagedata/schemes/eh_tbm/concepts/97980">
						<skos:inScheme rdf:resource="http://purl.org/heritagedata/schemes/eh_tbm" />
						<dcterms:identifier>http://purl.org/heritagedata/schemes/eh_tbm/concepts/97980</dcterms:identifier>
						<skos:prefLabel xml:lang="en">HORNBLENDE</skos:prefLabel>
						<dcterms:issued rdf:datatype="http://www.w3.org/2001/XMLSchema#dateTime">2013-07-17T09:02:16</dcterms:issued>
						<skos:broader rdf:resource="http://purl.org/heritagedata/schemes/eh_tbm/concepts/98058" />
						<skos:scopeNote xml:lang="en">Medium hard, green/black coloured. Found in many igneous and metamorphic rocks.</skos:scopeNote>
						<cc:license rdf:resource="http://creativecommons.org/licenses/by/3.0" />
						<cc:attributionURL rdf:resource="http://www.english-heritage.org.uk" />
						<cc:attributionName xml:lang="en">English Heritage</cc:attributionName>
						<dcterms:publisher rdf:resource="http://www.english-heritage.org.uk" />
					</skos:Concept>
				</skos:narrower>
				<skos:narrower rdf:resource="http://purl.org/heritagedata/schemes/eh_tbm/concepts/98133" />
				<skos:related rdf:resource="http://purl.org/heritagedata/schemes/eh_tbm/concepts/97929" />
				<skos:scopeNote xml:lang="en">Natural inorganic substance possessing a definite chemical composition in a crystalline form. See MINERAL Class Listnfor narrow terms.</skos:scopeNote>
				<cc:license rdf:resource="http://creativecommons.org/licenses/by/3.0" />
				<cc:attributionURL rdf:resource="http://www.english-heritage.org.uk" />
				<cc:attributionName xml:lang="en">English Heritage</cc:attributionName>
				<dcterms:publisher rdf:resource="http://www.english-heritage.org.uk" />
			</skos:Concept>
		</skos:hasTopConcept>
		<skos:hasTopConcept>
			<skos:Concept rdf:about="http://purl.org/heritagedata/schemes/eh_tbm/concepts/98216">
				<skos:topConceptOf rdf:resource="http://purl.org/heritagedata/schemes/eh_tbm" />
				<skos:inScheme rdf:resource="http://purl.org/heritagedata/schemes/eh_tbm" />
				<dcterms:identifier>http://purl.org/heritagedata/schemes/eh_tbm/concepts/98216</dcterms:identifier>
				<skos:prefLabel xml:lang="en">STONE</skos:prefLabel>
				<dcterms:issued rdf:datatype="http://www.w3.org/2001/XMLSchema#dateTime">2013-07-17T09:02:16</dcterms:issued>
				<skos:altLabel xml:lang="en">Metamorphic Stone</skos:altLabel>
				<skos:altLabel xml:lang="en">Gaisby Stone</skos:altLabel>
				<skos:narrower rdf:resource="http://purl.org/heritagedata/schemes/eh_tbm/concepts/97704" />
				<skos:narrower rdf:resource="http://purl.org/heritagedata/schemes/eh_tbm/concepts/97734" />
				<skos:narrower rdf:resource="http://purl.org/heritagedata/schemes/eh_tbm/concepts/97774" />
				<skos:narrower rdf:resource="http://purl.org/heritagedata/schemes/eh_tbm/concepts/97821" />
				<skos:narrower rdf:resource="http://purl.org/heritagedata/schemes/eh_tbm/concepts/97843" />
				<skos:narrower>
					<skos:Concept rdf:about="http://purl.org/heritagedata/schemes/eh_tbm/concepts/97889">
						<skos:inScheme rdf:resource="http://purl.org/heritagedata/schemes/eh_tbm" />
						<dcterms:identifier>http://purl.org/heritagedata/schemes/eh_tbm/concepts/97889</dcterms:identifier>
						<skos:prefLabel xml:lang="en">DIORITE</skos:prefLabel>
						<dcterms:issued rdf:datatype="http://www.w3.org/2001/XMLSchema#dateTime">2013-07-17T09:02:16</dcterms:issued>
						<skos:altLabel xml:lang="en">Black Granite</skos:altLabel>
						<skos:broader rdf:resource="http://purl.org/heritagedata/schemes/eh_tbm/concepts/98216" />
						<skos:scopeNote xml:lang="en">Coarse grained, dark coloured, igneous rock.</skos:scopeNote>
						<cc:license rdf:resource="http://creativecommons.org/licenses/by/3.0" />
						<cc:attributionURL rdf:resource="http://www.english-heritage.org.uk" />
						<cc:attributionName xml:lang="en">English Heritage</cc:attributionName>
						<dcterms:publisher rdf:resource="http://www.english-heritage.org.uk" />
					</skos:Concept>
				</skos:narrower>
				<skos:narrower rdf:resource="http://purl.org/heritagedata/schemes/eh_tbm/concepts/97891" />
				<skos:narrower rdf:resource="http://purl.org/heritagedata/schemes/eh_tbm/concepts/97928" />
				<skos:narrower>
					<skos:Concept rdf:about="http://purl.org/heritagedata/schemes/eh_tbm/concepts/97932">
						<skos:inScheme rdf:resource="http://purl.org/heritagedata/schemes/eh_tbm" />
						<dcterms:identifier>http://purl.org/heritagedata/schemes/eh_tbm/concepts/97932</dcterms:identifier>
						<skos:prefLabel xml:lang="en">FREESTONE</skos:prefLabel>
						<dcterms:issued rdf:datatype="http://www.w3.org/2001/XMLSchema#dateTime">2013-07-17T09:02:16</dcterms:issued>
						<skos:altLabel xml:lang="en">Langton Freestone</skos:altLabel>
						<skos:altLabel xml:lang="en">Yorkshire Freestone</skos:altLabel>
						<skos:altLabel xml:lang="en">Hard York Freestone</skos:altLabel>
						<skos:broader rdf:resource="http://purl.org/heritagedata/schemes/eh_tbm/concepts/98216" />
						<skos:scopeNote xml:lang="en">Stonemason's term for any easily worked sedimentary rock. Index with specific stone type where given.</skos:scopeNote>
						<cc:license rdf:resource="http://creativecommons.org/licenses/by/3.0" />
						<cc:attributionURL rdf:resource="http://www.english-heritage.org.uk" />
						<cc:attributionName xml:lang="en">English Heritage</cc:attributionName>
						<dcterms:publisher rdf:resource="http://www.english-heritage.org.uk" />
					</skos:Concept>
				</skos:narrower>
				<skos:narrower rdf:resource="http://purl.org/heritagedata/schemes/eh_tbm/concepts/97940" />
				<skos:narrower rdf:resource="http://purl.org/heritagedata/schemes/eh_tbm/concepts/97944" />
				<skos:narrower rdf:resource="http://purl.org/heritagedata/schemes/eh_tbm/concepts/97952" />
				<skos:narrower rdf:resource="http://purl.org/heritagedata/schemes/eh_tbm/concepts/97993" />
				<skos:narrower rdf:resource="http://purl.org/heritagedata/schemes/eh_tbm/concepts/98028" />
				<skos:narrower rdf:resource="http://purl.org/heritagedata/schemes/eh_tbm/concepts/98044" />
				<skos:narrower rdf:resource="http://purl.org/heritagedata/schemes/eh_tbm/concepts/98118" />
				<skos:narrower rdf:resource="http://purl.org/heritagedata/schemes/eh_tbm/concepts/102688" />
				<skos:narrower rdf:resource="http://purl.org/heritagedata/schemes/eh_tbm/concepts/98134" />
				<skos:narrower>
					<skos:Concept rdf:about="http://purl.org/heritagedata/schemes/eh_tbm/concepts/98138">
						<skos:inScheme rdf:resource="http://purl.org/heritagedata/schemes/eh_tbm" />
						<dcterms:identifier>http://purl.org/heritagedata/schemes/eh_tbm/concepts/98138</dcterms:identifier>
						<skos:prefLabel xml:lang="en">RAGSTONE</skos:prefLabel>
						<dcterms:issued rdf:datatype="http://www.w3.org/2001/XMLSchema#dateTime">2013-07-17T09:02:16</dcterms:issued>
						<skos:altLabel xml:lang="en">Rag</skos:altLabel>
						<skos:broader rdf:resource="http://purl.org/heritagedata/schemes/eh_tbm/concepts/98216" />
						<skos:scopeNote xml:lang="en">Stonemason's term for any coarse/hard stone that is not easily worked. Index with specific stone type where given. Not to be confused with Kentish Ragstone.</skos:scopeNote>
						<cc:license rdf:resource="http://creativecommons.org/licenses/by/3.0" />
						<cc:attributionURL rdf:resource="http://www.english-heritage.org.uk" />
						<cc:attributionName xml:lang="en">English Heritage</cc:attributionName>
						<dcterms:publisher rdf:resource="http://www.english-heritage.org.uk" />
					</skos:Concept>
				</skos:narrower>
				<skos:narrower rdf:resource="http://purl.org/heritagedata/schemes/eh_tbm/concepts/98150" />
				<skos:narrower rdf:resource="http://purl.org/heritagedata/schemes/eh_tbm/concepts/98171" />
				<skos:narrower>
					<skos:Concept rdf:about="http://purl.org/heritagedata/schemes/eh_tbm/concepts/98175">
						<skos:inScheme rdf:resource="http://purl.org/heritagedata/schemes/eh_tbm" />
						<dcterms:identifier>http://purl.org/heritagedata/schemes/eh_tbm/concepts/98175</dcterms:identifier>
						<skos:prefLabel xml:lang="en">SCHIST</skos:prefLabel>
						<dcterms:issued rdf:datatype="http://www.w3.org/2001/XMLSchema#dateTime">2013-07-17T09:02:16</dcterms:issued>
						<skos:altLabel xml:lang="en">Pillaguri Slate</skos:altLabel>
						<skos:altLabel xml:lang="en">Otta Slate</skos:altLabel>
						<skos:altLabel xml:lang="en">Rembrandt Stone</skos:altLabel>
						<skos:altLabel xml:lang="en">Sanfront Stone</skos:altLabel>
						<skos:altLabel xml:lang="en">Alta Quartzite</skos:altLabel>
						<skos:altLabel xml:lang="en">Altazite</skos:altLabel>
						<skos:altLabel xml:lang="en">Barge Quartzite</skos:altLabel>
						<skos:altLabel xml:lang="en">Italian Quartzite</skos:altLabel>
						<skos:broader rdf:resource="http://purl.org/heritagedata/schemes/eh_tbm/concepts/98216" />
						<skos:scopeNote xml:lang="en">Medium to coarse grained metamorphic rock, colour being determined by its dominant mineral. Often used for floor and wall cladding.</skos:scopeNote>
						<cc:license rdf:resource="http://creativecommons.org/licenses/by/3.0" />
						<cc:attributionURL rdf:resource="http://www.english-heritage.org.uk" />
						<cc:attributionName xml:lang="en">English Heritage</cc:attributionName>
						<dcterms:publisher rdf:resource="http://www.english-heritage.org.uk" />
					</skos:Concept>
				</skos:narrower>
				<skos:narrower rdf:resource="http://purl.org/heritagedata/schemes/eh_tbm/concepts/98181" />
				<skos:narrower rdf:resource="http://purl.org/heritagedata/schemes/eh_tbm/concepts/98183" />
				<skos:narrower rdf:resource="http://purl.org/heritagedata/schemes/eh_tbm/concepts/98188" />
				<skos:narrower rdf:resource="http://purl.org/heritagedata/schemes/eh_tbm/concepts/98194" />
				<skos:narrower rdf:resource="http://purl.org/heritagedata/schemes/eh_tbm/concepts/98229" />
				<skos:narrower>
					<skos:Concept rdf:about="http://purl.org/heritagedata/schemes/eh_tbm/concepts/140228">
						<skos:inScheme rdf:resource="http://purl.org/heritagedata/schemes/eh_tbm" />
						<dcterms:identifier>http://purl.org/heritagedata/schemes/eh_tbm/concepts/140228</dcterms:identifier>
						<skos:prefLabel xml:lang="en">TUFF</skos:prefLabel>
						<dcterms:issued rdf:datatype="http://www.w3.org/2001/XMLSchema#dateTime">2013-07-17T09:02:16</dcterms:issued>
						<skos:broader rdf:resource="http://purl.org/heritagedata/schemes/eh_tbm/concepts/98216" />
						<skos:scopeNote xml:lang="en">A light porous cellular rock, consisting of consolidated volcanic ash ejected from vents during a volcanic eruption.</skos:scopeNote>
						<cc:license rdf:resource="http://creativecommons.org/licenses/by/3.0" />
						<cc:attributionURL rdf:resource="http://www.english-heritage.org.uk" />
						<cc:attributionName xml:lang="en">English Heritage</cc:attributionName>
						<dcterms:publisher rdf:resource="http://www.english-heritage.org.uk" />
					</skos:Concept>
				</skos:narrower>
				<skos:narrower rdf:resource="http://purl.org/heritagedata/schemes/eh_tbm/concepts/98293" />
				<skos:related rdf:resource="http://purl.org/heritagedata/schemes/eh_tbm/concepts/97717" />
				<skos:related rdf:resource="http://purl.org/heritagedata/schemes/eh_tbm/concepts/97836" />
				<skos:related rdf:resource="http://purl.org/heritagedata/schemes/eh_tbm/concepts/97929" />
				<skos:related rdf:resource="http://purl.org/heritagedata/schemes/eh_tbm/concepts/97947" />
				<skos:related rdf:resource="http://purl.org/heritagedata/schemes/eh_tbm/concepts/98089" />
				<skos:related rdf:resource="http://purl.org/heritagedata/schemes/eh_tbm/concepts/98165" />
				<skos:scopeNote xml:lang="en">Rock of definite form and size, usually artificially shaped. See STONE CLass List for narrow terms.</skos:scopeNote>
				<cc:license rdf:resource="http://creativecommons.org/licenses/by/3.0" />
				<cc:attributionURL rdf:resource="http://www.english-heritage.org.uk" />
				<cc:attributionName xml:lang="en">English Heritage</cc:attributionName>
				<dcterms:publisher rdf:resource="http://www.english-heritage.org.uk" />
			</skos:Concept>
		</skos:hasTopConcept>
		<skos:hasTopConcept>
			<skos:Concept rdf:about="http://purl.org/heritagedata/schemes/eh_tbm/concepts/98238">
				<skos:topConceptOf rdf:resource="http://purl.org/heritagedata/schemes/eh_tbm" />
				<skos:inScheme rdf:resource="http://purl.org/heritagedata/schemes/eh_tbm" />
				<dcterms:identifier>http://purl.org/heritagedata/schemes/eh_tbm/concepts/98238</dcterms:identifier>
				<skos:prefLabel xml:lang="en">TEXTILE</skos:prefLabel>
				<dcterms:issued rdf:datatype="http://www.w3.org/2001/XMLSchema#dateTime">2013-07-17T09:02:16</dcterms:issued>
				<skos:altLabel xml:lang="en">Fabric</skos:altLabel>
				<skos:narrower>
					<skos:Concept rdf:about="http://purl.org/heritagedata/schemes/eh_tbm/concepts/97916">
						<skos:inScheme rdf:resource="http://purl.org/heritagedata/schemes/eh_tbm" />
						<dcterms:identifier>http://purl.org/heritagedata/schemes/eh_tbm/concepts/97916</dcterms:identifier>
						<skos:prefLabel xml:lang="en">FELT</skos:prefLabel>
						<dcterms:issued rdf:datatype="http://www.w3.org/2001/XMLSchema#dateTime">2013-07-17T09:02:16</dcterms:issued>
						<skos:broader rdf:resource="http://purl.org/heritagedata/schemes/eh_tbm/concepts/98238" />
						<skos:scopeNote xml:lang="en">Fabric of fibrous materials consolidated by heat and mechanical action so that the fibres are matted together.</skos:scopeNote>
						<cc:license rdf:resource="http://creativecommons.org/licenses/by/3.0" />
						<cc:attributionURL rdf:resource="http://www.english-heritage.org.uk" />
						<cc:attributionName xml:lang="en">English Heritage</cc:attributionName>
						<dcterms:publisher rdf:resource="http://www.english-heritage.org.uk" />
					</skos:Concept>
				</skos:narrower>
				<skos:scopeNote xml:lang="en">A woven or bonded fabric or cloth. See TEXTILE Class List for narrow terms.</skos:scopeNote>
				<cc:license rdf:resource="http://creativecommons.org/licenses/by/3.0" />
				<cc:attributionURL rdf:resource="http://www.english-heritage.org.uk" />
				<cc:attributionName xml:lang="en">English Heritage</cc:attributionName>
				<dcterms:publisher rdf:resource="http://www.english-heritage.org.uk" />
			</skos:Concept>
		</skos:hasTopConcept>
		<skos:hasTopConcept>
			<skos:Concept rdf:about="http://purl.org/heritagedata/schemes/eh_tbm/concepts/98265">
				<skos:topConceptOf rdf:resource="http://purl.org/heritagedata/schemes/eh_tbm" />
				<skos:inScheme rdf:resource="http://purl.org/heritagedata/schemes/eh_tbm" />
				<dcterms:identifier>http://purl.org/heritagedata/schemes/eh_tbm/concepts/98265</dcterms:identifier>
				<skos:prefLabel xml:lang="en">VEGETAL</skos:prefLabel>
				<dcterms:issued rdf:datatype="http://www.w3.org/2001/XMLSchema#dateTime">2013-07-17T09:02:16</dcterms:issued>
				<skos:narrower rdf:resource="http://purl.org/heritagedata/schemes/eh_tbm/concepts/98087" />
				<skos:narrower rdf:resource="http://purl.org/heritagedata/schemes/eh_tbm/concepts/98109" />
				<skos:narrower rdf:resource="http://purl.org/heritagedata/schemes/eh_tbm/concepts/98262" />
				<skos:narrower rdf:resource="http://purl.org/heritagedata/schemes/eh_tbm/concepts/98301" />
				<skos:scopeNote xml:lang="en">Pertaining to or deriving from a botanical living organism. See VEGETAL Class List for narrow terms.</skos:scopeNote>
				<cc:license rdf:resource="http://creativecommons.org/licenses/by/3.0" />
				<cc:attributionURL rdf:resource="http://www.english-heritage.org.uk" />
				<cc:attributionName xml:lang="en">English Heritage</cc:attributionName>
				<dcterms:publisher rdf:resource="http://www.english-heritage.org.uk" />
			</skos:Concept>
		</skos:hasTopConcept>
		<skos:hasTopConcept>
			<skos:Concept rdf:about="http://purl.org/heritagedata/schemes/eh_tbm/concepts/97712">
				<skos:topConceptOf rdf:resource="http://purl.org/heritagedata/schemes/eh_tbm" />
				<skos:inScheme rdf:resource="http://purl.org/heritagedata/schemes/eh_tbm" />
				<dcterms:identifier>http://purl.org/heritagedata/schemes/eh_tbm/concepts/97712</dcterms:identifier>
				<skos:prefLabel xml:lang="en">ANIMAL</skos:prefLabel>
				<dcterms:issued rdf:datatype="http://www.w3.org/2001/XMLSchema#dateTime">2013-07-17T09:02:16</dcterms:issued>
				<skos:narrower>
					<skos:Concept rdf:about="http://purl.org/heritagedata/schemes/eh_tbm/concepts/97764">
						<skos:inScheme rdf:resource="http://purl.org/heritagedata/schemes/eh_tbm" />
						<dcterms:identifier>http://purl.org/heritagedata/schemes/eh_tbm/concepts/97764</dcterms:identifier>
						<skos:prefLabel xml:lang="en">BONE</skos:prefLabel>
						<dcterms:issued rdf:datatype="http://www.w3.org/2001/XMLSchema#dateTime">2013-07-17T09:02:16</dcterms:issued>
						<skos:broader rdf:resource="http://purl.org/heritagedata/schemes/eh_tbm/concepts/97712" />
						<skos:scopeNote xml:lang="en">Any of the pieces of hard tissue consisting largely of calcium phosphate that make up the skeleton of a vertebrate animal.</skos:scopeNote>
						<cc:license rdf:resource="http://creativecommons.org/licenses/by/3.0" />
						<cc:attributionURL rdf:resource="http://www.english-heritage.org.uk" />
						<cc:attributionName xml:lang="en">English Heritage</cc:attributionName>
						<dcterms:publisher rdf:resource="http://www.english-heritage.org.uk" />
					</skos:Concept>
				</skos:narrower>
				<skos:narrower rdf:resource="http://purl.org/heritagedata/schemes/eh_tbm/concepts/97929" />
				<skos:narrower>
					<skos:Concept rdf:about="http://purl.org/heritagedata/schemes/eh_tbm/concepts/98023">
						<skos:inScheme rdf:resource="http://purl.org/heritagedata/schemes/eh_tbm" />
						<dcterms:identifier>http://purl.org/heritagedata/schemes/eh_tbm/concepts/98023</dcterms:identifier>
						<skos:prefLabel xml:lang="en">LEATHER</skos:prefLabel>
						<dcterms:issued rdf:datatype="http://www.w3.org/2001/XMLSchema#dateTime">2013-07-17T09:02:16</dcterms:issued>
						<skos:broader rdf:resource="http://purl.org/heritagedata/schemes/eh_tbm/concepts/97712" />
						<skos:scopeNote xml:lang="en">Animal skin that has been hardened or treated by a tanning process.</skos:scopeNote>
						<cc:license rdf:resource="http://creativecommons.org/licenses/by/3.0" />
						<cc:attributionURL rdf:resource="http://www.english-heritage.org.uk" />
						<cc:attributionName xml:lang="en">English Heritage</cc:attributionName>
						<dcterms:publisher rdf:resource="http://www.english-heritage.org.uk" />
					</skos:Concept>
				</skos:narrower>
				<skos:narrower>
					<skos:Concept rdf:about="http://purl.org/heritagedata/schemes/eh_tbm/concepts/98185">
						<skos:inScheme rdf:resource="http://purl.org/heritagedata/schemes/eh_tbm" />
						<dcterms:identifier>http://purl.org/heritagedata/schemes/eh_tbm/concepts/98185</dcterms:identifier>
						<skos:prefLabel xml:lang="en">SHELL</skos:prefLabel>
						<dcterms:issued rdf:datatype="http://www.w3.org/2001/XMLSchema#dateTime">2013-07-17T09:02:16</dcterms:issued>
						<skos:broader rdf:resource="http://purl.org/heritagedata/schemes/eh_tbm/concepts/97712" />
						<skos:scopeNote xml:lang="en">Hard, protective covering made largely of calcium salts secreted by soft bodied invertebrate animals.</skos:scopeNote>
						<cc:license rdf:resource="http://creativecommons.org/licenses/by/3.0" />
						<cc:attributionURL rdf:resource="http://www.english-heritage.org.uk" />
						<cc:attributionName xml:lang="en">English Heritage</cc:attributionName>
						<dcterms:publisher rdf:resource="http://www.english-heritage.org.uk" />
					</skos:Concept>
				</skos:narrower>
				<skos:scopeNote xml:lang="en">Pertaining to or deriving from a living organism. See ANIMAL Class list for narrow terms.</skos:scopeNote>
				<cc:license rdf:resource="http://creativecommons.org/licenses/by/3.0" />
				<cc:attributionURL rdf:resource="http://www.english-heritage.org.uk" />
				<cc:attributionName xml:lang="en">English Heritage</cc:attributionName>
				<dcterms:publisher rdf:resource="http://www.english-heritage.org.uk" />
			</skos:Concept>
		</skos:hasTopConcept>
		<skos:hasTopConcept>
			<skos:Concept rdf:about="http://purl.org/heritagedata/schemes/eh_tbm/concepts/97903">
				<skos:topConceptOf rdf:resource="http://purl.org/heritagedata/schemes/eh_tbm" />
				<skos:inScheme rdf:resource="http://purl.org/heritagedata/schemes/eh_tbm" />
				<dcterms:identifier>http://purl.org/heritagedata/schemes/eh_tbm/concepts/97903</dcterms:identifier>
				<skos:prefLabel xml:lang="en">EARTH MIX</skos:prefLabel>
				<dcterms:issued rdf:datatype="http://www.w3.org/2001/XMLSchema#dateTime">2013-07-17T09:02:16</dcterms:issued>
				<skos:narrower>
					<skos:Concept rdf:about="http://purl.org/heritagedata/schemes/eh_tbm/concepts/142988">
						<skos:inScheme rdf:resource="http://purl.org/heritagedata/schemes/eh_tbm" />
						<dcterms:identifier>http://purl.org/heritagedata/schemes/eh_tbm/concepts/142988</dcterms:identifier>
						<skos:prefLabel xml:lang="en">BRICKEARTH</skos:prefLabel>
						<dcterms:issued rdf:datatype="http://www.w3.org/2001/XMLSchema#dateTime">2013-07-17T09:02:16</dcterms:issued>
						<skos:broader rdf:resource="http://purl.org/heritagedata/schemes/eh_tbm/concepts/97903" />
						<skos:scopeNote xml:lang="en">An unconsolidated geological deposit sometimes iused as a bonding material in stone walls.</skos:scopeNote>
						<cc:license rdf:resource="http://creativecommons.org/licenses/by/3.0" />
						<cc:attributionURL rdf:resource="http://www.english-heritage.org.uk" />
						<cc:attributionName xml:lang="en">English Heritage</cc:attributionName>
						<dcterms:publisher rdf:resource="http://www.english-heritage.org.uk" />
					</skos:Concept>
				</skos:narrower>
				<skos:narrower rdf:resource="http://purl.org/heritagedata/schemes/eh_tbm/concepts/97827" />
				<skos:narrower>
					<skos:Concept rdf:about="http://purl.org/heritagedata/schemes/eh_tbm/concepts/97828">
						<skos:inScheme rdf:resource="http://purl.org/heritagedata/schemes/eh_tbm" />
						<dcterms:identifier>http://purl.org/heritagedata/schemes/eh_tbm/concepts/97828</dcterms:identifier>
						<skos:prefLabel xml:lang="en">CLAY LUMP</skos:prefLabel>
						<dcterms:issued rdf:datatype="http://www.w3.org/2001/XMLSchema#dateTime">2013-07-17T09:02:16</dcterms:issued>
						<skos:broader rdf:resource="http://purl.org/heritagedata/schemes/eh_tbm/concepts/97903" />
						<skos:scopeNote xml:lang="en">Large, moulded, unburnt blocks of clay type soil laid in a similar way to brick, but bedded in lime and clay 'mortar'. The walls produced are characteristically thinner than those of cob and pise.</skos:scopeNote>
						<cc:license rdf:resource="http://creativecommons.org/licenses/by/3.0" />
						<cc:attributionURL rdf:resource="http://www.english-heritage.org.uk" />
						<cc:attributionName xml:lang="en">English Heritage</cc:attributionName>
						<dcterms:publisher rdf:resource="http://www.english-heritage.org.uk" />
					</skos:Concept>
				</skos:narrower>
				<skos:narrower rdf:resource="http://purl.org/heritagedata/schemes/eh_tbm/concepts/97835" />
				<skos:narrower rdf:resource="http://purl.org/heritagedata/schemes/eh_tbm/concepts/97873" />
				<skos:narrower rdf:resource="http://purl.org/heritagedata/schemes/eh_tbm/concepts/97902" />
				<skos:narrower>
					<skos:Concept rdf:about="http://purl.org/heritagedata/schemes/eh_tbm/concepts/140229">
						<skos:inScheme rdf:resource="http://purl.org/heritagedata/schemes/eh_tbm" />
						<dcterms:identifier>http://purl.org/heritagedata/schemes/eh_tbm/concepts/140229</dcterms:identifier>
						<skos:prefLabel xml:lang="en">MARL</skos:prefLabel>
						<dcterms:issued rdf:datatype="http://www.w3.org/2001/XMLSchema#dateTime">2013-07-17T09:02:16</dcterms:issued>
						<skos:broader rdf:resource="http://purl.org/heritagedata/schemes/eh_tbm/concepts/97903" />
						<skos:scopeNote xml:lang="en">A mixed earthy substance consisting principally of clay mixed with calcium carbonate and sand in very variable proportions.</skos:scopeNote>
						<cc:license rdf:resource="http://creativecommons.org/licenses/by/3.0" />
						<cc:attributionURL rdf:resource="http://www.english-heritage.org.uk" />
						<cc:attributionName xml:lang="en">English Heritage</cc:attributionName>
						<dcterms:publisher rdf:resource="http://www.english-heritage.org.uk" />
					</skos:Concept>
				</skos:narrower>
				<skos:narrower>
					<skos:Concept rdf:about="http://purl.org/heritagedata/schemes/eh_tbm/concepts/98069">
						<skos:inScheme rdf:resource="http://purl.org/heritagedata/schemes/eh_tbm" />
						<dcterms:identifier>http://purl.org/heritagedata/schemes/eh_tbm/concepts/98069</dcterms:identifier>
						<skos:prefLabel xml:lang="en">MUD</skos:prefLabel>
						<dcterms:issued rdf:datatype="http://www.w3.org/2001/XMLSchema#dateTime">2013-07-17T09:02:16</dcterms:issued>
						<skos:broader rdf:resource="http://purl.org/heritagedata/schemes/eh_tbm/concepts/97903" />
						<skos:scopeNote xml:lang="en">Wet soil, sand or other earthy matter combined with ballast and bonded with straw or other binding material. Walls are built in the absence of shuttering by the simple process of pitching in layers.</skos:scopeNote>
						<cc:license rdf:resource="http://creativecommons.org/licenses/by/3.0" />
						<cc:attributionURL rdf:resource="http://www.english-heritage.org.uk" />
						<cc:attributionName xml:lang="en">English Heritage</cc:attributionName>
						<dcterms:publisher rdf:resource="http://www.english-heritage.org.uk" />
					</skos:Concept>
				</skos:narrower>
				<skos:narrower>
					<skos:Concept rdf:about="http://purl.org/heritagedata/schemes/eh_tbm/concepts/98107">
						<skos:inScheme rdf:resource="http://purl.org/heritagedata/schemes/eh_tbm" />
						<dcterms:identifier>http://purl.org/heritagedata/schemes/eh_tbm/concepts/98107</dcterms:identifier>
						<skos:prefLabel xml:lang="en">PISE</skos:prefLabel>
						<dcterms:issued rdf:datatype="http://www.w3.org/2001/XMLSchema#dateTime">2013-07-17T09:02:16</dcterms:issued>
						<skos:altLabel xml:lang="en">Pise De Terre</skos:altLabel>
						<skos:broader rdf:resource="http://purl.org/heritagedata/schemes/eh_tbm/concepts/97903" />
						<skos:scopeNote xml:lang="en">Rammed earth or clay of a low moisture content used to make floors or walls, or found between shuttering.</skos:scopeNote>
						<cc:license rdf:resource="http://creativecommons.org/licenses/by/3.0" />
						<cc:attributionURL rdf:resource="http://www.english-heritage.org.uk" />
						<cc:attributionName xml:lang="en">English Heritage</cc:attributionName>
						<dcterms:publisher rdf:resource="http://www.english-heritage.org.uk" />
					</skos:Concept>
				</skos:narrower>
				<skos:narrower rdf:resource="http://purl.org/heritagedata/schemes/eh_tbm/concepts/98170" />
				<skos:scopeNote xml:lang="en">Unbaked clays and/or soil material often mixed with, or performing the function of an aggregate or binder. See EARTH MIX Class List for narrow terms.</skos:scopeNote>
				<cc:license rdf:resource="http://creativecommons.org/licenses/by/3.0" />
				<cc:attributionURL rdf:resource="http://www.english-heritage.org.uk" />
				<cc:attributionName xml:lang="en">English Heritage</cc:attributionName>
				<dcterms:publisher rdf:resource="http://www.english-heritage.org.uk" />
			</skos:Concept>
		</skos:hasTopConcept>
	</skos:ConceptScheme>
	<skos:Concept rdf:about="http://purl.org/heritagedata/schemes/eh_tbm/concepts/98082">
		<skos:inScheme rdf:resource="http://purl.org/heritagedata/schemes/eh_tbm" />
		<dcterms:identifier>http://purl.org/heritagedata/schemes/eh_tbm/concepts/98082</dcterms:identifier>
		<skos:prefLabel xml:lang="en">PAPER</skos:prefLabel>
		<dcterms:issued rdf:datatype="http://www.w3.org/2001/XMLSchema#dateTime">2013-07-17T09:02:16</dcterms:issued>
		<skos:broader rdf:resource="http://purl.org/heritagedata/schemes/eh_tbm/concepts/98041" />
		<skos:related rdf:resource="http://purl.org/heritagedata/schemes/eh_tbm/concepts/98301" />
		<skos:scopeNote xml:lang="en">Thin flexible sheets made from the pulp of wood or other fibrous matter.</skos:scopeNote>
		<cc:license rdf:resource="http://creativecommons.org/licenses/by/3.0" />
		<cc:attributionURL rdf:resource="http://www.english-heritage.org.uk" />
		<cc:attributionName xml:lang="en">English Heritage</cc:attributionName>
		<dcterms:publisher rdf:resource="http://www.english-heritage.org.uk" />
	</skos:Concept>
	<skos:Concept rdf:about="http://purl.org/heritagedata/schemes/eh_tbm/concepts/98087">
		<skos:inScheme rdf:resource="http://purl.org/heritagedata/schemes/eh_tbm" />
		<dcterms:identifier>http://purl.org/heritagedata/schemes/eh_tbm/concepts/98087</dcterms:identifier>
		<skos:prefLabel xml:lang="en">PEAT</skos:prefLabel>
		<dcterms:issued rdf:datatype="http://www.w3.org/2001/XMLSchema#dateTime">2013-07-17T09:02:16</dcterms:issued>
		<skos:altLabel xml:lang="en">Peat Brick</skos:altLabel>
		<skos:broader rdf:resource="http://purl.org/heritagedata/schemes/eh_tbm/concepts/98265" />
		<skos:related rdf:resource="http://purl.org/heritagedata/schemes/eh_tbm/concepts/97777" />
		<skos:related rdf:resource="http://purl.org/heritagedata/schemes/eh_tbm/concepts/97902" />
		<skos:scopeNote xml:lang="en">Part-decomposed vegetable matter formed under waterlogged conditions into a firm, brown deposit resembling soil. Used as a brick for infilling in timber framed walls.</skos:scopeNote>
		<cc:license rdf:resource="http://creativecommons.org/licenses/by/3.0" />
		<cc:attributionURL rdf:resource="http://www.english-heritage.org.uk" />
		<cc:attributionName xml:lang="en">English Heritage</cc:attributionName>
		<dcterms:publisher rdf:resource="http://www.english-heritage.org.uk" />
	</skos:Concept>
	<skos:Concept rdf:about="http://purl.org/heritagedata/schemes/eh_tbm/concepts/98089">
		<skos:inScheme rdf:resource="http://purl.org/heritagedata/schemes/eh_tbm" />
		<dcterms:identifier>http://purl.org/heritagedata/schemes/eh_tbm/concepts/98089</dcterms:identifier>
		<skos:prefLabel xml:lang="en">PEBBLE</skos:prefLabel>
		<dcterms:issued rdf:datatype="http://www.w3.org/2001/XMLSchema#dateTime">2013-07-17T09:02:16</dcterms:issued>
		<skos:broader rdf:resource="http://purl.org/heritagedata/schemes/eh_tbm/concepts/98046" />
		<skos:related rdf:resource="http://purl.org/heritagedata/schemes/eh_tbm/concepts/98090" />
		<skos:related rdf:resource="http://purl.org/heritagedata/schemes/eh_tbm/concepts/98216" />
		<skos:scopeNote xml:lang="en">Rock fragment (diameter 4-64mm) larger than gravel and smaller than cobble, combined with other material e.g. flint, for decorative effect.</skos:scopeNote>
		<cc:license rdf:resource="http://creativecommons.org/licenses/by/3.0" />
		<cc:attributionURL rdf:resource="http://www.english-heritage.org.uk" />
		<cc:attributionName xml:lang="en">English Heritage</cc:attributionName>
		<dcterms:publisher rdf:resource="http://www.english-heritage.org.uk" />
	</skos:Concept>
	<skos:Concept rdf:about="http://purl.org/heritagedata/schemes/eh_tbm/concepts/98090">
		<skos:inScheme rdf:resource="http://purl.org/heritagedata/schemes/eh_tbm" />
		<dcterms:identifier>http://purl.org/heritagedata/schemes/eh_tbm/concepts/98090</dcterms:identifier>
		<skos:prefLabel xml:lang="en">PEBBLEDASH</skos:prefLabel>
		<dcterms:issued rdf:datatype="http://www.w3.org/2001/XMLSchema#dateTime">2013-07-17T09:02:16</dcterms:issued>
		<skos:broader rdf:resource="http://purl.org/heritagedata/schemes/eh_tbm/concepts/98147" />
		<skos:related rdf:resource="http://purl.org/heritagedata/schemes/eh_tbm/concepts/98089" />
		<skos:scopeNote xml:lang="en">A render with small washed stones added as aggregate. Popular in the early 20th century.</skos:scopeNote>
		<cc:license rdf:resource="http://creativecommons.org/licenses/by/3.0" />
		<cc:attributionURL rdf:resource="http://www.english-heritage.org.uk" />
		<cc:attributionName xml:lang="en">English Heritage</cc:attributionName>
		<dcterms:publisher rdf:resource="http://www.english-heritage.org.uk" />
	</skos:Concept>
	<skos:Concept rdf:about="http://purl.org/heritagedata/schemes/eh_tbm/concepts/98109">
		<skos:inScheme rdf:resource="http://purl.org/heritagedata/schemes/eh_tbm" />
		<dcterms:identifier>http://purl.org/heritagedata/schemes/eh_tbm/concepts/98109</dcterms:identifier>
		<skos:prefLabel xml:lang="en">PLANT</skos:prefLabel>
		<dcterms:issued rdf:datatype="http://www.w3.org/2001/XMLSchema#dateTime">2013-07-17T09:02:16</dcterms:issued>
		<skos:narrower rdf:resource="http://purl.org/heritagedata/schemes/eh_tbm/concepts/97943" />
		<skos:narrower>
			<skos:Concept rdf:about="http://purl.org/heritagedata/schemes/eh_tbm/concepts/140464">
				<skos:inScheme rdf:resource="http://purl.org/heritagedata/schemes/eh_tbm" />
				<dcterms:identifier>http://purl.org/heritagedata/schemes/eh_tbm/concepts/140464</dcterms:identifier>
				<skos:prefLabel xml:lang="en">GRASS</skos:prefLabel>
				<dcterms:issued rdf:datatype="http://www.w3.org/2001/XMLSchema#dateTime">2013-07-17T09:02:16</dcterms:issued>
				<skos:broader rdf:resource="http://purl.org/heritagedata/schemes/eh_tbm/concepts/98109" />
				<skos:scopeNote xml:lang="en">Ground-covering herbage, some varieties of which can be used, especially when dried and in large quantities, as a construction material.</skos:scopeNote>
				<cc:license rdf:resource="http://creativecommons.org/licenses/by/3.0" />
				<cc:attributionURL rdf:resource="http://www.english-heritage.org.uk" />
				<cc:attributionName xml:lang="en">English Heritage</cc:attributionName>
				<dcterms:publisher rdf:resource="http://www.english-heritage.org.uk" />
			</skos:Concept>
		</skos:narrower>
		<skos:narrower rdf:resource="http://purl.org/heritagedata/schemes/eh_tbm/concepts/97974" />
		<skos:broader rdf:resource="http://purl.org/heritagedata/schemes/eh_tbm/concepts/98265" />
		<skos:narrower rdf:resource="http://purl.org/heritagedata/schemes/eh_tbm/concepts/98143" />
		<skos:narrower>
			<skos:Concept rdf:about="http://purl.org/heritagedata/schemes/eh_tbm/concepts/126913">
				<skos:inScheme rdf:resource="http://purl.org/heritagedata/schemes/eh_tbm" />
				<dcterms:identifier>http://purl.org/heritagedata/schemes/eh_tbm/concepts/126913</dcterms:identifier>
				<skos:prefLabel xml:lang="en">SEAWEED</skos:prefLabel>
				<dcterms:issued rdf:datatype="http://www.w3.org/2001/XMLSchema#dateTime">2013-07-17T09:02:16</dcterms:issued>
				<skos:broader rdf:resource="http://purl.org/heritagedata/schemes/eh_tbm/concepts/98109" />
				<skos:scopeNote xml:lang="en">Multicellular marine alga, which grows on the seashore, in salt marshes, in brackish water or submerged in the ocean.</skos:scopeNote>
				<cc:license rdf:resource="http://creativecommons.org/licenses/by/3.0" />
				<cc:attributionURL rdf:resource="http://www.english-heritage.org.uk" />
				<cc:attributionName xml:lang="en">English Heritage</cc:attributionName>
				<dcterms:publisher rdf:resource="http://www.english-heritage.org.uk" />
			</skos:Concept>
		</skos:narrower>
		<skos:narrower rdf:resource="http://purl.org/heritagedata/schemes/eh_tbm/concepts/98219" />
		<skos:scopeNote xml:lang="en">Any tree, shrub or herb of cellulose form, normally subsisting in soil and producing its food through photosynthesis.</skos:scopeNote>
		<cc:license rdf:resource="http://creativecommons.org/licenses/by/3.0" />
		<cc:attributionURL rdf:resource="http://www.english-heritage.org.uk" />
		<cc:attributionName xml:lang="en">English Heritage</cc:attributionName>
		<dcterms:publisher rdf:resource="http://www.english-heritage.org.uk" />
	</skos:Concept>
	<skos:Concept rdf:about="http://purl.org/heritagedata/schemes/eh_tbm/concepts/98110">
		<skos:inScheme rdf:resource="http://purl.org/heritagedata/schemes/eh_tbm" />
		<dcterms:identifier>http://purl.org/heritagedata/schemes/eh_tbm/concepts/98110</dcterms:identifier>
		<skos:prefLabel xml:lang="en">PLASTER</skos:prefLabel>
		<dcterms:issued rdf:datatype="http://www.w3.org/2001/XMLSchema#dateTime">2013-07-17T09:02:16</dcterms:issued>
		<skos:narrower rdf:resource="http://purl.org/heritagedata/schemes/eh_tbm/concepts/97876" />
		<skos:narrower>
			<skos:Concept rdf:about="http://purl.org/heritagedata/schemes/eh_tbm/concepts/143498">
				<skos:inScheme rdf:resource="http://purl.org/heritagedata/schemes/eh_tbm" />
				<dcterms:identifier>http://purl.org/heritagedata/schemes/eh_tbm/concepts/143498</dcterms:identifier>
				<skos:prefLabel xml:lang="en">PAINTED PLASTER</skos:prefLabel>
				<dcterms:issued rdf:datatype="http://www.w3.org/2001/XMLSchema#dateTime">2013-07-17T09:02:16</dcterms:issued>
				<skos:altLabel xml:lang="en">Painted Wall Plaster</skos:altLabel>
				<skos:broader rdf:resource="http://purl.org/heritagedata/schemes/eh_tbm/concepts/98110" />
				<skos:scopeNote xml:lang="en">Plaster which has been painted either for decorative purposes or to protect it.</skos:scopeNote>
				<cc:license rdf:resource="http://creativecommons.org/licenses/by/3.0" />
				<cc:attributionURL rdf:resource="http://www.english-heritage.org.uk" />
				<cc:attributionName xml:lang="en">English Heritage</cc:attributionName>
				<dcterms:publisher rdf:resource="http://www.english-heritage.org.uk" />
			</skos:Concept>
		</skos:narrower>
		<skos:broader rdf:resource="http://purl.org/heritagedata/schemes/eh_tbm/concepts/98147" />
		<skos:related rdf:resource="http://purl.org/heritagedata/schemes/eh_tbm/concepts/97873" />
		<skos:related rdf:resource="http://purl.org/heritagedata/schemes/eh_tbm/concepts/98018" />
		<skos:related rdf:resource="http://purl.org/heritagedata/schemes/eh_tbm/concepts/98026" />
		<skos:scopeNote xml:lang="en">Lime plaster, consisting of lime and sand, is the oldest type of render. Applied externally to walls or onto laths for infill panels and usually limewashed.</skos:scopeNote>
		<cc:license rdf:resource="http://creativecommons.org/licenses/by/3.0" />
		<cc:attributionURL rdf:resource="http://www.english-heritage.org.uk" />
		<cc:attributionName xml:lang="en">English Heritage</cc:attributionName>
		<dcterms:publisher rdf:resource="http://www.english-heritage.org.uk" />
	</skos:Concept>
	<skos:Concept rdf:about="http://purl.org/heritagedata/schemes/eh_tbm/concepts/98111">
		<skos:inScheme rdf:resource="http://purl.org/heritagedata/schemes/eh_tbm" />
		<dcterms:identifier>http://purl.org/heritagedata/schemes/eh_tbm/concepts/98111</dcterms:identifier>
		<skos:prefLabel xml:lang="en">PLASTIC</skos:prefLabel>
		<dcterms:issued rdf:datatype="http://www.w3.org/2001/XMLSchema#dateTime">2013-07-17T09:02:16</dcterms:issued>
		<skos:narrower>
			<skos:Concept rdf:about="http://purl.org/heritagedata/schemes/eh_tbm/concepts/97726">
				<skos:inScheme rdf:resource="http://purl.org/heritagedata/schemes/eh_tbm" />
				<dcterms:identifier>http://purl.org/heritagedata/schemes/eh_tbm/concepts/97726</dcterms:identifier>
				<skos:prefLabel xml:lang="en">BAKELITE</skos:prefLabel>
				<dcterms:issued rdf:datatype="http://www.w3.org/2001/XMLSchema#dateTime">2013-07-17T09:02:16</dcterms:issued>
				<skos:broader rdf:resource="http://purl.org/heritagedata/schemes/eh_tbm/concepts/98111" />
				<skos:scopeNote xml:lang="en">Thermosetting plastic commonly used for its properties of electrical insulation.</skos:scopeNote>
				<cc:license rdf:resource="http://creativecommons.org/licenses/by/3.0" />
				<cc:attributionURL rdf:resource="http://www.english-heritage.org.uk" />
				<cc:attributionName xml:lang="en">English Heritage</cc:attributionName>
				<dcterms:publisher rdf:resource="http://www.english-heritage.org.uk" />
			</skos:Concept>
		</skos:narrower>
		<skos:broader rdf:resource="http://purl.org/heritagedata/schemes/eh_tbm/concepts/98041" />
		<skos:narrower>
			<skos:Concept rdf:about="http://purl.org/heritagedata/schemes/eh_tbm/concepts/98117">
				<skos:inScheme rdf:resource="http://purl.org/heritagedata/schemes/eh_tbm" />
				<dcterms:identifier>http://purl.org/heritagedata/schemes/eh_tbm/concepts/98117</dcterms:identifier>
				<skos:prefLabel xml:lang="en">POLYCARBONATE</skos:prefLabel>
				<dcterms:issued rdf:datatype="http://www.w3.org/2001/XMLSchema#dateTime">2013-07-17T09:02:16</dcterms:issued>
				<skos:broader rdf:resource="http://purl.org/heritagedata/schemes/eh_tbm/concepts/98111" />
				<skos:scopeNote xml:lang="en">Very tough transparent sheeting often used for security glazing.</skos:scopeNote>
				<cc:license rdf:resource="http://creativecommons.org/licenses/by/3.0" />
				<cc:attributionURL rdf:resource="http://www.english-heritage.org.uk" />
				<cc:attributionName xml:lang="en">English Heritage</cc:attributionName>
				<dcterms:publisher rdf:resource="http://www.english-heritage.org.uk" />
			</skos:Concept>
		</skos:narrower>
		<skos:narrower>
			<skos:Concept rdf:about="http://purl.org/heritagedata/schemes/eh_tbm/concepts/98119">
				<skos:inScheme rdf:resource="http://purl.org/heritagedata/schemes/eh_tbm" />
				<dcterms:identifier>http://purl.org/heritagedata/schemes/eh_tbm/concepts/98119</dcterms:identifier>
				<skos:prefLabel xml:lang="en">POLYVINYL CHLORIDE</skos:prefLabel>
				<dcterms:issued rdf:datatype="http://www.w3.org/2001/XMLSchema#dateTime">2013-07-17T09:02:16</dcterms:issued>
				<skos:broader rdf:resource="http://purl.org/heritagedata/schemes/eh_tbm/concepts/98111" />
				<skos:scopeNote xml:lang="en">A type of thermoplastic polymer which is versatile and cheap, often referred to as PVC. This includes plasticized PVC and unplasticized PVC (uPVC).</skos:scopeNote>
				<cc:license rdf:resource="http://creativecommons.org/licenses/by/3.0" />
				<cc:attributionURL rdf:resource="http://www.english-heritage.org.uk" />
				<cc:attributionName xml:lang="en">English Heritage</cc:attributionName>
				<dcterms:publisher rdf:resource="http://www.english-heritage.org.uk" />
			</skos:Concept>
		</skos:narrower>
		<skos:related rdf:resource="http://purl.org/heritagedata/schemes/eh_tbm/concepts/98164" />
		<skos:scopeNote xml:lang="en">Any of large class of polymers based on synthetic resins or modified natural polymers which may be moulded, extruded or cast while soft or liquid, which then set rigidly or slightly elastic in form.</skos:scopeNote>
		<cc:license rdf:resource="http://creativecommons.org/licenses/by/3.0" />
		<cc:attributionURL rdf:resource="http://www.english-heritage.org.uk" />
		<cc:attributionName xml:lang="en">English Heritage</cc:attributionName>
		<dcterms:publisher rdf:resource="http://www.english-heritage.org.uk" />
	</skos:Concept>
	<skos:Concept rdf:about="http://purl.org/heritagedata/schemes/eh_tbm/concepts/98113">
		<skos:inScheme rdf:resource="http://purl.org/heritagedata/schemes/eh_tbm" />
		<dcterms:identifier>http://purl.org/heritagedata/schemes/eh_tbm/concepts/98113</dcterms:identifier>
		<skos:prefLabel xml:lang="en">PLYMETAL</skos:prefLabel>
		<dcterms:issued rdf:datatype="http://www.w3.org/2001/XMLSchema#dateTime">2013-07-17T09:02:16</dcterms:issued>
		<skos:altLabel xml:lang="en">Plymax</skos:altLabel>
		<skos:broader rdf:resource="http://purl.org/heritagedata/schemes/eh_tbm/concepts/98080" />
		<skos:related rdf:resource="http://purl.org/heritagedata/schemes/eh_tbm/concepts/98053" />
		<skos:related rdf:resource="http://purl.org/heritagedata/schemes/eh_tbm/concepts/98301" />
		<skos:scopeNote xml:lang="en">Structural board comprising a core of thin layers of wood bonded together, which is faced on one or both sides with a sheet of metal, usually galvanised steel or aluminium. Mainly used for external wall cladding.</skos:scopeNote>
		<cc:license rdf:resource="http://creativecommons.org/licenses/by/3.0" />
		<cc:attributionURL rdf:resource="http://www.english-heritage.org.uk" />
		<cc:attributionName xml:lang="en">English Heritage</cc:attributionName>
		<dcterms:publisher rdf:resource="http://www.english-heritage.org.uk" />
	</skos:Concept>
	<skos:Concept rdf:about="http://purl.org/heritagedata/schemes/eh_tbm/concepts/98116">
		<skos:inScheme rdf:resource="http://purl.org/heritagedata/schemes/eh_tbm" />
		<dcterms:identifier>http://purl.org/heritagedata/schemes/eh_tbm/concepts/98116</dcterms:identifier>
		<skos:prefLabel xml:lang="en">PLYWOOD</skos:prefLabel>
		<dcterms:issued rdf:datatype="http://www.w3.org/2001/XMLSchema#dateTime">2013-07-17T09:02:16</dcterms:issued>
		<skos:broader rdf:resource="http://purl.org/heritagedata/schemes/eh_tbm/concepts/98080" />
		<skos:related rdf:resource="http://purl.org/heritagedata/schemes/eh_tbm/concepts/98301" />
		<skos:scopeNote xml:lang="en">Thin layers of wood, bonded together to form a structural board. The grain of the adjacent layers lie across one another to give structural strength. Produced since mid 19th century for use in interior joinery, since 1930's for exterior use.</skos:scopeNote>
		<cc:license rdf:resource="http://creativecommons.org/licenses/by/3.0" />
		<cc:attributionURL rdf:resource="http://www.english-heritage.org.uk" />
		<cc:attributionName xml:lang="en">English Heritage</cc:attributionName>
		<dcterms:publisher rdf:resource="http://www.english-heritage.org.uk" />
	</skos:Concept>
	<skos:Concept rdf:about="http://purl.org/heritagedata/schemes/eh_tbm/concepts/98118">
		<skos:inScheme rdf:resource="http://purl.org/heritagedata/schemes/eh_tbm" />
		<dcterms:identifier>http://purl.org/heritagedata/schemes/eh_tbm/concepts/98118</dcterms:identifier>
		<skos:prefLabel xml:lang="en">POLYPHANT</skos:prefLabel>
		<dcterms:issued rdf:datatype="http://www.w3.org/2001/XMLSchema#dateTime">2013-07-17T09:02:16</dcterms:issued>
		<skos:broader rdf:resource="http://purl.org/heritagedata/schemes/eh_tbm/concepts/98216" />
		<skos:related rdf:resource="http://purl.org/heritagedata/schemes/eh_tbm/concepts/98044" />
		<skos:related rdf:resource="http://purl.org/heritagedata/schemes/eh_tbm/concepts/98181" />
		<skos:scopeNote xml:lang="en">Compact, grey/green/brown/white-speckled coloured igneous rock, peculiar to Cornwall. It is easy to carve and readily takes a polish, hence its similarity to British marbles.</skos:scopeNote>
		<cc:license rdf:resource="http://creativecommons.org/licenses/by/3.0" />
		<cc:attributionURL rdf:resource="http://www.english-heritage.org.uk" />
		<cc:attributionName xml:lang="en">English Heritage</cc:attributionName>
		<dcterms:publisher rdf:resource="http://www.english-heritage.org.uk" />
	</skos:Concept>
	<skos:Concept rdf:about="http://purl.org/heritagedata/schemes/eh_tbm/concepts/98123">
		<skos:inScheme rdf:resource="http://purl.org/heritagedata/schemes/eh_tbm" />
		<dcterms:identifier>http://purl.org/heritagedata/schemes/eh_tbm/concepts/98123</dcterms:identifier>
		<skos:prefLabel xml:lang="en">PORTLAND STONE</skos:prefLabel>
		<dcterms:issued rdf:datatype="http://www.w3.org/2001/XMLSchema#dateTime">2013-07-17T09:02:16</dcterms:issued>
		<skos:altLabel xml:lang="en">Portland Roach</skos:altLabel>
		<skos:altLabel xml:lang="en">Ridgeway Stone</skos:altLabel>
		<skos:altLabel xml:lang="en">Roach Stone</skos:altLabel>
		<skos:altLabel xml:lang="en">Tisbury Stone</skos:altLabel>
		<skos:altLabel xml:lang="en">Whit Bed</skos:altLabel>
		<skos:altLabel xml:lang="en">Whitbed</skos:altLabel>
		<skos:altLabel xml:lang="en">Chilmark Stone</skos:altLabel>
		<skos:altLabel xml:lang="en">Base Bed</skos:altLabel>
		<skos:altLabel xml:lang="en">Basebed</skos:altLabel>
		<skos:broader rdf:resource="http://purl.org/heritagedata/schemes/eh_tbm/concepts/98075" />
		<skos:narrower rdf:resource="http://purl.org/heritagedata/schemes/eh_tbm/concepts/98131" />
		<skos:scopeNote xml:lang="en">Fine to coarse grained, cream to green/grey coloured oolitic limestone. Quarried since Roman times, it is one of Britain's best building stones, hence its use throughout the country.</skos:scopeNote>
		<cc:license rdf:resource="http://creativecommons.org/licenses/by/3.0" />
		<cc:attributionURL rdf:resource="http://www.english-heritage.org.uk" />
		<cc:attributionName xml:lang="en">English Heritage</cc:attributionName>
		<dcterms:publisher rdf:resource="http://www.english-heritage.org.uk" />
	</skos:Concept>
	<skos:Concept rdf:about="http://purl.org/heritagedata/schemes/eh_tbm/concepts/98126">
		<skos:inScheme rdf:resource="http://purl.org/heritagedata/schemes/eh_tbm" />
		<dcterms:identifier>http://purl.org/heritagedata/schemes/eh_tbm/concepts/98126</dcterms:identifier>
		<skos:prefLabel xml:lang="en">PUDDINGSTONE</skos:prefLabel>
		<dcterms:issued rdf:datatype="http://www.w3.org/2001/XMLSchema#dateTime">2013-07-17T09:02:16</dcterms:issued>
		<skos:narrower rdf:resource="http://purl.org/heritagedata/schemes/eh_tbm/concepts/164108" />
		<skos:broader rdf:resource="http://purl.org/heritagedata/schemes/eh_tbm/concepts/97843" />
		<skos:related rdf:resource="http://purl.org/heritagedata/schemes/eh_tbm/concepts/97774" />
		<skos:scopeNote xml:lang="en">Conglomerate consisting of rounded flint pebbles held together in a natural silica and sand cement.</skos:scopeNote>
		<cc:license rdf:resource="http://creativecommons.org/licenses/by/3.0" />
		<cc:attributionURL rdf:resource="http://www.english-heritage.org.uk" />
		<cc:attributionName xml:lang="en">English Heritage</cc:attributionName>
		<dcterms:publisher rdf:resource="http://www.english-heritage.org.uk" />
	</skos:Concept>
	<skos:Concept rdf:about="http://purl.org/heritagedata/schemes/eh_tbm/concepts/98131">
		<skos:inScheme rdf:resource="http://purl.org/heritagedata/schemes/eh_tbm" />
		<dcterms:identifier>http://purl.org/heritagedata/schemes/eh_tbm/concepts/98131</dcterms:identifier>
		<skos:prefLabel xml:lang="en">PURBECK STONE</skos:prefLabel>
		<dcterms:issued rdf:datatype="http://www.w3.org/2001/XMLSchema#dateTime">2013-07-17T09:02:16</dcterms:issued>
		<skos:altLabel xml:lang="en">Purbeck Marble</skos:altLabel>
		<skos:altLabel xml:lang="en">Purbeck Portland</skos:altLabel>
		<skos:altLabel xml:lang="en">Langton Freestone</skos:altLabel>
		<skos:altLabel xml:lang="en">Swanage Stone</skos:altLabel>
		<skos:altLabel xml:lang="en">Corfe Stone</skos:altLabel>
		<skos:broader rdf:resource="http://purl.org/heritagedata/schemes/eh_tbm/concepts/98123" />
		<skos:related rdf:resource="http://purl.org/heritagedata/schemes/eh_tbm/concepts/98044" />
		<skos:scopeNote xml:lang="en">Collective name for the oolitic limestone quarried in the Isle of Purbeck region, geologically classified into two main groups. Firstly, a fine grained whitish variety, Purbeck Portland, secondly a fossil-rich cream/gold to grey variety, Swanage Stone etc</skos:scopeNote>
		<cc:license rdf:resource="http://creativecommons.org/licenses/by/3.0" />
		<cc:attributionURL rdf:resource="http://www.english-heritage.org.uk" />
		<cc:attributionName xml:lang="en">English Heritage</cc:attributionName>
		<dcterms:publisher rdf:resource="http://www.english-heritage.org.uk" />
	</skos:Concept>
	<skos:Concept rdf:about="http://purl.org/heritagedata/schemes/eh_tbm/concepts/98133">
		<skos:inScheme rdf:resource="http://purl.org/heritagedata/schemes/eh_tbm" />
		<dcterms:identifier>http://purl.org/heritagedata/schemes/eh_tbm/concepts/98133</dcterms:identifier>
		<skos:prefLabel xml:lang="en">QUARTZ</skos:prefLabel>
		<dcterms:issued rdf:datatype="http://www.w3.org/2001/XMLSchema#dateTime">2013-07-17T09:02:16</dcterms:issued>
		<skos:broader rdf:resource="http://purl.org/heritagedata/schemes/eh_tbm/concepts/98058" />
		<skos:related rdf:resource="http://purl.org/heritagedata/schemes/eh_tbm/concepts/98134" />
		<skos:scopeNote xml:lang="en">Hard, transparent, often coloured mineral. Can be found on its own as crystals and veins but also as a major constituent of rocks such as granite. Often used decoratively.</skos:scopeNote>
		<cc:license rdf:resource="http://creativecommons.org/licenses/by/3.0" />
		<cc:attributionURL rdf:resource="http://www.english-heritage.org.uk" />
		<cc:attributionName xml:lang="en">English Heritage</cc:attributionName>
		<dcterms:publisher rdf:resource="http://www.english-heritage.org.uk" />
	</skos:Concept>
	<skos:Concept rdf:about="http://purl.org/heritagedata/schemes/eh_tbm/concepts/98134">
		<skos:inScheme rdf:resource="http://purl.org/heritagedata/schemes/eh_tbm" />
		<dcterms:identifier>http://purl.org/heritagedata/schemes/eh_tbm/concepts/98134</dcterms:identifier>
		<skos:prefLabel xml:lang="en">QUARTZITE</skos:prefLabel>
		<dcterms:issued rdf:datatype="http://www.w3.org/2001/XMLSchema#dateTime">2013-07-17T09:02:16</dcterms:issued>
		<skos:altLabel xml:lang="en">Safari Quartzite</skos:altLabel>
		<skos:altLabel xml:lang="en">Diamanzite</skos:altLabel>
		<skos:broader rdf:resource="http://purl.org/heritagedata/schemes/eh_tbm/concepts/98216" />
		<skos:related rdf:resource="http://purl.org/heritagedata/schemes/eh_tbm/concepts/98133" />
		<skos:scopeNote xml:lang="en">Medium grained, hard, white/grey coloured stone consisting of quartz and often silica, produced by the metamorphosis of sandstone.</skos:scopeNote>
		<cc:license rdf:resource="http://creativecommons.org/licenses/by/3.0" />
		<cc:attributionURL rdf:resource="http://www.english-heritage.org.uk" />
		<cc:attributionName xml:lang="en">English Heritage</cc:attributionName>
		<dcterms:publisher rdf:resource="http://www.english-heritage.org.uk" />
	</skos:Concept>
	<skos:Concept rdf:about="http://purl.org/heritagedata/schemes/eh_tbm/concepts/98143">
		<skos:inScheme rdf:resource="http://purl.org/heritagedata/schemes/eh_tbm" />
		<dcterms:identifier>http://purl.org/heritagedata/schemes/eh_tbm/concepts/98143</dcterms:identifier>
		<skos:prefLabel xml:lang="en">REED</skos:prefLabel>
		<dcterms:issued rdf:datatype="http://www.w3.org/2001/XMLSchema#dateTime">2013-07-17T09:02:16</dcterms:issued>
		<skos:altLabel xml:lang="en">Water Reed</skos:altLabel>
		<skos:broader rdf:resource="http://purl.org/heritagedata/schemes/eh_tbm/concepts/98109" />
		<skos:related rdf:resource="http://purl.org/heritagedata/schemes/eh_tbm/concepts/98239" />
		<skos:scopeNote xml:lang="en">The tall, straight stalks or stems formed by plants found in the wetland areas, particularly The Fens. Used as a roofing material, the reed is laid with the ends forming the exposed covering surface.</skos:scopeNote>
		<cc:license rdf:resource="http://creativecommons.org/licenses/by/3.0" />
		<cc:attributionURL rdf:resource="http://www.english-heritage.org.uk" />
		<cc:attributionName xml:lang="en">English Heritage</cc:attributionName>
		<dcterms:publisher rdf:resource="http://www.english-heritage.org.uk" />
	</skos:Concept>
	<skos:Concept rdf:about="http://purl.org/heritagedata/schemes/eh_tbm/concepts/98144">
		<skos:inScheme rdf:resource="http://purl.org/heritagedata/schemes/eh_tbm" />
		<dcterms:identifier>http://purl.org/heritagedata/schemes/eh_tbm/concepts/98144</dcterms:identifier>
		<skos:prefLabel xml:lang="en">REIGATE STONE</skos:prefLabel>
		<dcterms:issued rdf:datatype="http://www.w3.org/2001/XMLSchema#dateTime">2013-07-17T09:02:16</dcterms:issued>
		<skos:altLabel xml:lang="en">Merstham Stone</skos:altLabel>
		<skos:altLabel xml:lang="en">Gatton Stone</skos:altLabel>
		<skos:altLabel xml:lang="en">Godstone Stone</skos:altLabel>
		<skos:broader rdf:resource="http://purl.org/heritagedata/schemes/eh_tbm/concepts/98171" />
		<skos:related rdf:resource="http://purl.org/heritagedata/schemes/eh_tbm/concepts/98028" />
		<skos:scopeNote xml:lang="en">Soft, medium grained, green/grey coloured, highly calcareous, cretaceous sandstone. Mined (more frequently than quarried) since pre-Norman times from the Reigate area of Surrey.</skos:scopeNote>
		<cc:license rdf:resource="http://creativecommons.org/licenses/by/3.0" />
		<cc:attributionURL rdf:resource="http://www.english-heritage.org.uk" />
		<cc:attributionName xml:lang="en">English Heritage</cc:attributionName>
		<dcterms:publisher rdf:resource="http://www.english-heritage.org.uk" />
	</skos:Concept>
	<skos:Concept rdf:about="http://purl.org/heritagedata/schemes/eh_tbm/concepts/98145">
		<skos:inScheme rdf:resource="http://purl.org/heritagedata/schemes/eh_tbm" />
		<dcterms:identifier>http://purl.org/heritagedata/schemes/eh_tbm/concepts/98145</dcterms:identifier>
		<skos:prefLabel xml:lang="en">REINFORCED CONCRETE</skos:prefLabel>
		<dcterms:issued rdf:datatype="http://www.w3.org/2001/XMLSchema#dateTime">2013-07-17T09:02:16</dcterms:issued>
		<skos:broader rdf:resource="http://purl.org/heritagedata/schemes/eh_tbm/concepts/97840" />
		<skos:related rdf:resource="http://purl.org/heritagedata/schemes/eh_tbm/concepts/98213" />
		<skos:scopeNote xml:lang="en">Aggregate, cement and mortar combined with structural elements of iron or steel mesh or rod reinforcement to form stonelike masses for load bearing, structural building work.</skos:scopeNote>
		<cc:license rdf:resource="http://creativecommons.org/licenses/by/3.0" />
		<cc:attributionURL rdf:resource="http://www.english-heritage.org.uk" />
		<cc:attributionName xml:lang="en">English Heritage</cc:attributionName>
		<dcterms:publisher rdf:resource="http://www.english-heritage.org.uk" />
	</skos:Concept>
	<skos:Concept rdf:about="http://purl.org/heritagedata/schemes/eh_tbm/concepts/98018">
		<skos:inScheme rdf:resource="http://purl.org/heritagedata/schemes/eh_tbm" />
		<dcterms:identifier>http://purl.org/heritagedata/schemes/eh_tbm/concepts/98018</dcterms:identifier>
		<skos:prefLabel xml:lang="en">LATH</skos:prefLabel>
		<dcterms:issued rdf:datatype="http://www.w3.org/2001/XMLSchema#dateTime">2013-07-17T09:02:16</dcterms:issued>
		<skos:broader rdf:resource="http://purl.org/heritagedata/schemes/eh_tbm/concepts/98242" />
		<skos:related rdf:resource="http://purl.org/heritagedata/schemes/eh_tbm/concepts/97873" />
		<skos:related rdf:resource="http://purl.org/heritagedata/schemes/eh_tbm/concepts/98110" />
		<skos:scopeNote xml:lang="en">Narrow strips of wood which can form the groundwork for slates, panels or plaster work.</skos:scopeNote>
		<cc:license rdf:resource="http://creativecommons.org/licenses/by/3.0" />
		<cc:attributionURL rdf:resource="http://www.english-heritage.org.uk" />
		<cc:attributionName xml:lang="en">English Heritage</cc:attributionName>
		<dcterms:publisher rdf:resource="http://www.english-heritage.org.uk" />
	</skos:Concept>
	<skos:Concept rdf:about="http://purl.org/heritagedata/schemes/eh_tbm/concepts/98022">
		<skos:inScheme rdf:resource="http://purl.org/heritagedata/schemes/eh_tbm" />
		<dcterms:identifier>http://purl.org/heritagedata/schemes/eh_tbm/concepts/98022</dcterms:identifier>
		<skos:prefLabel xml:lang="en">LEAD</skos:prefLabel>
		<dcterms:issued rdf:datatype="http://www.w3.org/2001/XMLSchema#dateTime">2013-07-17T09:02:16</dcterms:issued>
		<skos:broader rdf:resource="http://purl.org/heritagedata/schemes/eh_tbm/concepts/98053" />
		<skos:narrower>
			<skos:Concept rdf:about="http://purl.org/heritagedata/schemes/eh_tbm/concepts/143234">
				<skos:inScheme rdf:resource="http://purl.org/heritagedata/schemes/eh_tbm" />
				<dcterms:identifier>http://purl.org/heritagedata/schemes/eh_tbm/concepts/143234</dcterms:identifier>
				<skos:prefLabel xml:lang="en">SHEET LEAD</skos:prefLabel>
				<dcterms:issued rdf:datatype="http://www.w3.org/2001/XMLSchema#dateTime">2013-07-17T09:02:16</dcterms:issued>
				<skos:broader rdf:resource="http://purl.org/heritagedata/schemes/eh_tbm/concepts/98022" />
				<skos:scopeNote xml:lang="en">Lead which has been rolled into a sheet and often used as a roof covering.</skos:scopeNote>
				<cc:license rdf:resource="http://creativecommons.org/licenses/by/3.0" />
				<cc:attributionURL rdf:resource="http://www.english-heritage.org.uk" />
				<cc:attributionName xml:lang="en">English Heritage</cc:attributionName>
				<dcterms:publisher rdf:resource="http://www.english-heritage.org.uk" />
			</skos:Concept>
		</skos:narrower>
		<skos:scopeNote xml:lang="en">Metal used primarily for roof coverings and window fittings. It is easy to work, can be worked cold and does not rust which makes it suitable for holding or repelling water.</skos:scopeNote>
		<cc:license rdf:resource="http://creativecommons.org/licenses/by/3.0" />
		<cc:attributionURL rdf:resource="http://www.english-heritage.org.uk" />
		<cc:attributionName xml:lang="en">English Heritage</cc:attributionName>
		<dcterms:publisher rdf:resource="http://www.english-heritage.org.uk" />
	</skos:Concept>
	<skos:Concept rdf:about="http://purl.org/heritagedata/schemes/eh_tbm/concepts/98024">
		<skos:inScheme rdf:resource="http://purl.org/heritagedata/schemes/eh_tbm" />
		<dcterms:identifier>http://purl.org/heritagedata/schemes/eh_tbm/concepts/98024</dcterms:identifier>
		<skos:prefLabel xml:lang="en">LIAS</skos:prefLabel>
		<dcterms:issued rdf:datatype="http://www.w3.org/2001/XMLSchema#dateTime">2013-07-17T09:02:16</dcterms:issued>
		<skos:altLabel xml:lang="en">Stowey Stone</skos:altLabel>
		<skos:narrower rdf:resource="http://purl.org/heritagedata/schemes/eh_tbm/concepts/97756" />
		<skos:narrower>
			<skos:Concept rdf:about="http://purl.org/heritagedata/schemes/eh_tbm/concepts/97963">
				<skos:inScheme rdf:resource="http://purl.org/heritagedata/schemes/eh_tbm" />
				<dcterms:identifier>http://purl.org/heritagedata/schemes/eh_tbm/concepts/97963</dcterms:identifier>
				<skos:prefLabel xml:lang="en">HAM HILL STONE</skos:prefLabel>
				<dcterms:issued rdf:datatype="http://www.w3.org/2001/XMLSchema#dateTime">2013-07-17T09:02:16</dcterms:issued>
				<skos:altLabel xml:lang="en">Ham Stone</skos:altLabel>
				<skos:broader rdf:resource="http://purl.org/heritagedata/schemes/eh_tbm/concepts/98024" />
				<skos:scopeNote xml:lang="en">Shelly, gold/brown, coloured liassic limestone containing large quantities of crystalline calcite.</skos:scopeNote>
				<cc:license rdf:resource="http://creativecommons.org/licenses/by/3.0" />
				<cc:attributionURL rdf:resource="http://www.english-heritage.org.uk" />
				<cc:attributionName xml:lang="en">English Heritage</cc:attributionName>
				<dcterms:publisher rdf:resource="http://www.english-heritage.org.uk" />
			</skos:Concept>
		</skos:narrower>
		<skos:narrower>
			<skos:Concept rdf:about="http://purl.org/heritagedata/schemes/eh_tbm/concepts/97982">
				<skos:inScheme rdf:resource="http://purl.org/heritagedata/schemes/eh_tbm" />
				<dcterms:identifier>http://purl.org/heritagedata/schemes/eh_tbm/concepts/97982</dcterms:identifier>
				<skos:prefLabel xml:lang="en">HORNTON STONE</skos:prefLabel>
				<dcterms:issued rdf:datatype="http://www.w3.org/2001/XMLSchema#dateTime">2013-07-17T09:02:16</dcterms:issued>
				<skos:broader rdf:resource="http://purl.org/heritagedata/schemes/eh_tbm/concepts/98024" />
				<skos:scopeNote xml:lang="en">Compact grained, brown/yellow/green/grey blue, coloured liassic limestone.</skos:scopeNote>
				<cc:license rdf:resource="http://creativecommons.org/licenses/by/3.0" />
				<cc:attributionURL rdf:resource="http://www.english-heritage.org.uk" />
				<cc:attributionName xml:lang="en">English Heritage</cc:attributionName>
				<dcterms:publisher rdf:resource="http://www.english-heritage.org.uk" />
			</skos:Concept>
		</skos:narrower>
		<skos:broader rdf:resource="http://purl.org/heritagedata/schemes/eh_tbm/concepts/97999" />
		<skos:narrower rdf:resource="http://purl.org/heritagedata/schemes/eh_tbm/concepts/98045" />
		<skos:related rdf:resource="http://purl.org/heritagedata/schemes/eh_tbm/concepts/97827" />
		<skos:related rdf:resource="http://purl.org/heritagedata/schemes/eh_tbm/concepts/97993" />
		<skos:related rdf:resource="http://purl.org/heritagedata/schemes/eh_tbm/concepts/98171" />
		<skos:scopeNote xml:lang="en">Collective term for the building limestones formed during the Lower Jurassic period.</skos:scopeNote>
		<cc:license rdf:resource="http://creativecommons.org/licenses/by/3.0" />
		<cc:attributionURL rdf:resource="http://www.english-heritage.org.uk" />
		<cc:attributionName xml:lang="en">English Heritage</cc:attributionName>
		<dcterms:publisher rdf:resource="http://www.english-heritage.org.uk" />
	</skos:Concept>
	<skos:Concept rdf:about="http://purl.org/heritagedata/schemes/eh_tbm/concepts/98026">
		<skos:inScheme rdf:resource="http://purl.org/heritagedata/schemes/eh_tbm" />
		<dcterms:identifier>http://purl.org/heritagedata/schemes/eh_tbm/concepts/98026</dcterms:identifier>
		<skos:prefLabel xml:lang="en">LIME</skos:prefLabel>
		<dcterms:issued rdf:datatype="http://www.w3.org/2001/XMLSchema#dateTime">2013-07-17T09:02:16</dcterms:issued>
		<skos:altLabel xml:lang="en">Lime Mortar</skos:altLabel>
		<skos:broader rdf:resource="http://purl.org/heritagedata/schemes/eh_tbm/concepts/98148" />
		<skos:related rdf:resource="http://purl.org/heritagedata/schemes/eh_tbm/concepts/97809" />
		<skos:related rdf:resource="http://purl.org/heritagedata/schemes/eh_tbm/concepts/97873" />
		<skos:related rdf:resource="http://purl.org/heritagedata/schemes/eh_tbm/concepts/98062" />
		<skos:related rdf:resource="http://purl.org/heritagedata/schemes/eh_tbm/concepts/98110" />
		<skos:related rdf:resource="http://purl.org/heritagedata/schemes/eh_tbm/concepts/98156" />
		<skos:scopeNote xml:lang="en">Calcium Oxide obtained by heating limestone in a kiln. Used as a constituent of modern mortar, or as slaked (non-hydraulic) lime in lime putty, daub, limewash and traditional lime plaster, mortar and renders.</skos:scopeNote>
		<cc:license rdf:resource="http://creativecommons.org/licenses/by/3.0" />
		<cc:attributionURL rdf:resource="http://www.english-heritage.org.uk" />
		<cc:attributionName xml:lang="en">English Heritage</cc:attributionName>
		<dcterms:publisher rdf:resource="http://www.english-heritage.org.uk" />
	</skos:Concept>
	<skos:Concept rdf:about="http://purl.org/heritagedata/schemes/eh_tbm/concepts/98028">
		<skos:inScheme rdf:resource="http://purl.org/heritagedata/schemes/eh_tbm" />
		<dcterms:identifier>http://purl.org/heritagedata/schemes/eh_tbm/concepts/98028</dcterms:identifier>
		<skos:prefLabel xml:lang="en">LIMESTONE</skos:prefLabel>
		<dcterms:issued rdf:datatype="http://www.w3.org/2001/XMLSchema#dateTime">2013-07-17T09:02:16</dcterms:issued>
		<skos:altLabel xml:lang="en">Membury Stone</skos:altLabel>
		<skos:altLabel xml:lang="en">Moolham Stone</skos:altLabel>
		<skos:altLabel xml:lang="en">Todber Stone</skos:altLabel>
		<skos:altLabel xml:lang="en">Calcareous Spar</skos:altLabel>
		<skos:altLabel xml:lang="en">Devon Marble</skos:altLabel>
		<skos:narrower rdf:resource="http://purl.org/heritagedata/schemes/eh_tbm/concepts/97800" />
		<skos:narrower rdf:resource="http://purl.org/heritagedata/schemes/eh_tbm/concepts/97866" />
		<skos:narrower>
			<skos:Concept rdf:about="http://purl.org/heritagedata/schemes/eh_tbm/concepts/97887">
				<skos:inScheme rdf:resource="http://purl.org/heritagedata/schemes/eh_tbm" />
				<dcterms:identifier>http://purl.org/heritagedata/schemes/eh_tbm/concepts/97887</dcterms:identifier>
				<skos:prefLabel xml:lang="en">DEVONIAN LIMESTONE</skos:prefLabel>
				<dcterms:issued rdf:datatype="http://www.w3.org/2001/XMLSchema#dateTime">2013-07-17T09:02:16</dcterms:issued>
				<skos:altLabel xml:lang="en">Plymouth Limestone</skos:altLabel>
				<skos:altLabel xml:lang="en">Plymouth Stone</skos:altLabel>
				<skos:altLabel xml:lang="en">Torquay Limestone</skos:altLabel>
				<skos:altLabel xml:lang="en">Torquay Marble</skos:altLabel>
				<skos:altLabel xml:lang="en">Chudleigh Stone</skos:altLabel>
				<skos:altLabel xml:lang="en">Ashburton Marble</skos:altLabel>
				<skos:broader rdf:resource="http://purl.org/heritagedata/schemes/eh_tbm/concepts/98028" />
				<skos:scopeNote xml:lang="en">Limestone formed during the Devonian period, and found predominantly between the Exe and Tamar rivers in Devon. Varying in colour from black/grey to pink/white it was often polished to imitate, and be used as, marble.</skos:scopeNote>
				<cc:license rdf:resource="http://creativecommons.org/licenses/by/3.0" />
				<cc:attributionURL rdf:resource="http://www.english-heritage.org.uk" />
				<cc:attributionName xml:lang="en">English Heritage</cc:attributionName>
				<dcterms:publisher rdf:resource="http://www.english-heritage.org.uk" />
			</skos:Concept>
		</skos:narrower>
		<skos:narrower rdf:resource="http://purl.org/heritagedata/schemes/eh_tbm/concepts/97999" />
		<skos:broader rdf:resource="http://purl.org/heritagedata/schemes/eh_tbm/concepts/98216" />
		<skos:narrower rdf:resource="http://purl.org/heritagedata/schemes/eh_tbm/concepts/98036" />
		<skos:narrower rdf:resource="http://purl.org/heritagedata/schemes/eh_tbm/concepts/98236" />
		<skos:narrower>
			<skos:Concept rdf:about="http://purl.org/heritagedata/schemes/eh_tbm/concepts/98260">
				<skos:inScheme rdf:resource="http://purl.org/heritagedata/schemes/eh_tbm" />
				<dcterms:identifier>http://purl.org/heritagedata/schemes/eh_tbm/concepts/98260</dcterms:identifier>
				<skos:prefLabel xml:lang="en">TUFACEOUS LIMESTONE</skos:prefLabel>
				<dcterms:issued rdf:datatype="http://www.w3.org/2001/XMLSchema#dateTime">2013-07-17T09:02:16</dcterms:issued>
				<skos:altLabel xml:lang="en">Travertine</skos:altLabel>
				<skos:altLabel xml:lang="en">Tufa</skos:altLabel>
				<skos:broader rdf:resource="http://purl.org/heritagedata/schemes/eh_tbm/concepts/98028" />
				<skos:scopeNote xml:lang="en">Very light, depositional limestone formed by the precipitation of calcium carbonate rich water (Tufa). The more dense and compact form, Travertine, is formed in a similar way.</skos:scopeNote>
				<cc:license rdf:resource="http://creativecommons.org/licenses/by/3.0" />
				<cc:attributionURL rdf:resource="http://www.english-heritage.org.uk" />
				<cc:attributionName xml:lang="en">English Heritage</cc:attributionName>
				<dcterms:publisher rdf:resource="http://www.english-heritage.org.uk" />
			</skos:Concept>
		</skos:narrower>
		<skos:related rdf:resource="http://purl.org/heritagedata/schemes/eh_tbm/concepts/98040" />
		<skos:related rdf:resource="http://purl.org/heritagedata/schemes/eh_tbm/concepts/98044" />
		<skos:related rdf:resource="http://purl.org/heritagedata/schemes/eh_tbm/concepts/98144" />
		<skos:related rdf:resource="http://purl.org/heritagedata/schemes/eh_tbm/concepts/98183" />
		<skos:scopeNote xml:lang="en">Sedimentary rock consisting mainly of calcium carbonate. Varying in grain size, colour and hardness, quarried and used throughout the country.</skos:scopeNote>
		<cc:license rdf:resource="http://creativecommons.org/licenses/by/3.0" />
		<cc:attributionURL rdf:resource="http://www.english-heritage.org.uk" />
		<cc:attributionName xml:lang="en">English Heritage</cc:attributionName>
		<dcterms:publisher rdf:resource="http://www.english-heritage.org.uk" />
	</skos:Concept>
	<skos:Concept rdf:about="http://purl.org/heritagedata/schemes/eh_tbm/concepts/98031">
		<skos:inScheme rdf:resource="http://purl.org/heritagedata/schemes/eh_tbm" />
		<dcterms:identifier>http://purl.org/heritagedata/schemes/eh_tbm/concepts/98031</dcterms:identifier>
		<skos:prefLabel xml:lang="en">LONG STRAW</skos:prefLabel>
		<dcterms:issued rdf:datatype="http://www.w3.org/2001/XMLSchema#dateTime">2013-07-17T09:02:16</dcterms:issued>
		<skos:broader rdf:resource="http://purl.org/heritagedata/schemes/eh_tbm/concepts/98219" />
		<skos:related rdf:resource="http://purl.org/heritagedata/schemes/eh_tbm/concepts/98239" />
		<skos:scopeNote xml:lang="en">Composed of loose uncombed lengths of harvested wheat which are formed into bundles for laying. Distinctive appearance with both ears and butts visible on the surface traditionally using hazel spars which hold the straw in place.</skos:scopeNote>
		<cc:license rdf:resource="http://creativecommons.org/licenses/by/3.0" />
		<cc:attributionURL rdf:resource="http://www.english-heritage.org.uk" />
		<cc:attributionName xml:lang="en">English Heritage</cc:attributionName>
		<dcterms:publisher rdf:resource="http://www.english-heritage.org.uk" />
	</skos:Concept>
	<skos:Concept rdf:about="http://purl.org/heritagedata/schemes/eh_tbm/concepts/98036">
		<skos:inScheme rdf:resource="http://purl.org/heritagedata/schemes/eh_tbm" />
		<dcterms:identifier>http://purl.org/heritagedata/schemes/eh_tbm/concepts/98036</dcterms:identifier>
		<skos:prefLabel xml:lang="en">MAGNESIAN LIMESTONE</skos:prefLabel>
		<dcterms:issued rdf:datatype="http://www.w3.org/2001/XMLSchema#dateTime">2013-07-17T09:02:16</dcterms:issued>
		<skos:altLabel xml:lang="en">Mansfield Woodhouse Stone</skos:altLabel>
		<skos:altLabel xml:lang="en">Roche Abbey Stone</skos:altLabel>
		<skos:altLabel xml:lang="en">Steetly Stone</skos:altLabel>
		<skos:altLabel xml:lang="en">Tadcaster Stone</skos:altLabel>
		<skos:altLabel xml:lang="en">Bolsover Moor</skos:altLabel>
		<skos:altLabel xml:lang="en">Anston Stone</skos:altLabel>
		<skos:altLabel xml:lang="en">Huddlestone Stone</skos:altLabel>
		<skos:broader rdf:resource="http://purl.org/heritagedata/schemes/eh_tbm/concepts/98028" />
		<skos:related rdf:resource="http://purl.org/heritagedata/schemes/eh_tbm/concepts/97892" />
		<skos:scopeNote xml:lang="en">Permian limestones which have had their chemical composition naturally altered with the calcium content being replaced by magnesium. Fine grained and varying from yellow/brown to cream in colour, although they weather to a dark grey.</skos:scopeNote>
		<cc:license rdf:resource="http://creativecommons.org/licenses/by/3.0" />
		<cc:attributionURL rdf:resource="http://www.english-heritage.org.uk" />
		<cc:attributionName xml:lang="en">English Heritage</cc:attributionName>
		<dcterms:publisher rdf:resource="http://www.english-heritage.org.uk" />
	</skos:Concept>
	<skos:Concept rdf:about="http://purl.org/heritagedata/schemes/eh_tbm/concepts/98040">
		<skos:inScheme rdf:resource="http://purl.org/heritagedata/schemes/eh_tbm" />
		<dcterms:identifier>http://purl.org/heritagedata/schemes/eh_tbm/concepts/98040</dcterms:identifier>
		<skos:prefLabel xml:lang="en">MALMSTONE</skos:prefLabel>
		<dcterms:issued rdf:datatype="http://www.w3.org/2001/XMLSchema#dateTime">2013-07-17T09:02:16</dcterms:issued>
		<skos:altLabel xml:lang="en">Malm (Stone)</skos:altLabel>
		<skos:altLabel xml:lang="en">Green Ventnor Stone</skos:altLabel>
		<skos:broader rdf:resource="http://purl.org/heritagedata/schemes/eh_tbm/concepts/98171" />
		<skos:related rdf:resource="http://purl.org/heritagedata/schemes/eh_tbm/concepts/97993" />
		<skos:related rdf:resource="http://purl.org/heritagedata/schemes/eh_tbm/concepts/98028" />
		<skos:scopeNote xml:lang="en">A soft, grey to white coloured, sandstone formed during the Cretaceous period, whose sand grains are cemented together with lime.</skos:scopeNote>
		<cc:license rdf:resource="http://creativecommons.org/licenses/by/3.0" />
		<cc:attributionURL rdf:resource="http://www.english-heritage.org.uk" />
		<cc:attributionName xml:lang="en">English Heritage</cc:attributionName>
		<dcterms:publisher rdf:resource="http://www.english-heritage.org.uk" />
	</skos:Concept>
	<skos:Concept rdf:about="http://purl.org/heritagedata/schemes/eh_tbm/concepts/98044">
		<skos:inScheme rdf:resource="http://purl.org/heritagedata/schemes/eh_tbm" />
		<dcterms:identifier>http://purl.org/heritagedata/schemes/eh_tbm/concepts/98044</dcterms:identifier>
		<skos:prefLabel xml:lang="en">MARBLE</skos:prefLabel>
		<dcterms:issued rdf:datatype="http://www.w3.org/2001/XMLSchema#dateTime">2013-07-17T09:02:16</dcterms:issued>
		<skos:altLabel xml:lang="en">Parian Marble</skos:altLabel>
		<skos:altLabel xml:lang="en">Pennon Marble</skos:altLabel>
		<skos:altLabel xml:lang="en">Pentelic Marble</skos:altLabel>
		<skos:altLabel xml:lang="en">Petworth Marble</skos:altLabel>
		<skos:altLabel xml:lang="en">Pink Verona Marble</skos:altLabel>
		<skos:altLabel xml:lang="en">Purbeck Marble</skos:altLabel>
		<skos:altLabel xml:lang="en">Large Paludina Marble</skos:altLabel>
		<skos:altLabel xml:lang="en">Laughton Marble</skos:altLabel>
		<skos:altLabel xml:lang="en">Sicilian Marble</skos:altLabel>
		<skos:altLabel xml:lang="en">Skyros Marble</skos:altLabel>
		<skos:altLabel xml:lang="en">Small Paludina Marble</skos:altLabel>
		<skos:altLabel xml:lang="en">Sussex Marble</skos:altLabel>
		<skos:altLabel xml:lang="en">Teesdale Marble</skos:altLabel>
		<skos:altLabel xml:lang="en">Tinos</skos:altLabel>
		<skos:altLabel xml:lang="en">Torquay Marble</skos:altLabel>
		<skos:altLabel xml:lang="en">Travertine</skos:altLabel>
		<skos:altLabel xml:lang="en">Verde Antico</skos:altLabel>
		<skos:altLabel xml:lang="en">Verde Fraye</skos:altLabel>
		<skos:altLabel xml:lang="en">Verona Marble</skos:altLabel>
		<skos:altLabel xml:lang="en">Yeovil Marble</skos:altLabel>
		<skos:altLabel xml:lang="en">Bethersden Marble</skos:altLabel>
		<skos:altLabel xml:lang="en">Bletchingdon Marble</skos:altLabel>
		<skos:altLabel xml:lang="en">Breche Rose</skos:altLabel>
		<skos:altLabel xml:lang="en">Charlwood Stone</skos:altLabel>
		<skos:altLabel xml:lang="en">Ashburton Marble</skos:altLabel>
		<skos:altLabel xml:lang="en">Australian Marble</skos:altLabel>
		<skos:altLabel xml:lang="en">Devon Marble</skos:altLabel>
		<skos:altLabel xml:lang="en">Dundee Marble</skos:altLabel>
		<skos:altLabel xml:lang="en">Forest Marble</skos:altLabel>
		<skos:altLabel xml:lang="en">Frosterley Marble</skos:altLabel>
		<skos:altLabel xml:lang="en">Istrian Stone</skos:altLabel>
		<skos:altLabel xml:lang="en">Jaune Lamartine</skos:altLabel>
		<skos:narrower>
			<skos:Concept rdf:about="http://purl.org/heritagedata/schemes/eh_tbm/concepts/97793">
				<skos:inScheme rdf:resource="http://purl.org/heritagedata/schemes/eh_tbm" />
				<dcterms:identifier>http://purl.org/heritagedata/schemes/eh_tbm/concepts/97793</dcterms:identifier>
				<skos:prefLabel xml:lang="en">CAMPAN MARBLE</skos:prefLabel>
				<dcterms:issued rdf:datatype="http://www.w3.org/2001/XMLSchema#dateTime">2013-07-17T09:02:16</dcterms:issued>
				<skos:altLabel xml:lang="en">Campan Melange</skos:altLabel>
				<skos:altLabel xml:lang="en">Campan Rose</skos:altLabel>
				<skos:altLabel xml:lang="en">Campan Vert</skos:altLabel>
				<skos:broader rdf:resource="http://purl.org/heritagedata/schemes/eh_tbm/concepts/98044" />
				<skos:scopeNote xml:lang="en">White coloured marble. Imported from France.</skos:scopeNote>
				<cc:license rdf:resource="http://creativecommons.org/licenses/by/3.0" />
				<cc:attributionURL rdf:resource="http://www.english-heritage.org.uk" />
				<cc:attributionName xml:lang="en">English Heritage</cc:attributionName>
				<dcterms:publisher rdf:resource="http://www.english-heritage.org.uk" />
			</skos:Concept>
		</skos:narrower>
		<skos:narrower>
			<skos:Concept rdf:about="http://purl.org/heritagedata/schemes/eh_tbm/concepts/97802">
				<skos:inScheme rdf:resource="http://purl.org/heritagedata/schemes/eh_tbm" />
				<dcterms:identifier>http://purl.org/heritagedata/schemes/eh_tbm/concepts/97802</dcterms:identifier>
				<skos:prefLabel xml:lang="en">CARRARA MARBLE</skos:prefLabel>
				<dcterms:issued rdf:datatype="http://www.w3.org/2001/XMLSchema#dateTime">2013-07-17T09:02:16</dcterms:issued>
				<skos:altLabel xml:lang="en">Pavonazzo</skos:altLabel>
				<skos:altLabel xml:lang="en">Cipollino Marble</skos:altLabel>
				<skos:altLabel xml:lang="en">Arabescato Marble</skos:altLabel>
				<skos:altLabel xml:lang="en">Bardiglio Marble</skos:altLabel>
				<skos:broader rdf:resource="http://purl.org/heritagedata/schemes/eh_tbm/concepts/98044" />
				<skos:scopeNote xml:lang="en">Imported Italian marble varying in colour from green, blue, purple to white.</skos:scopeNote>
				<cc:license rdf:resource="http://creativecommons.org/licenses/by/3.0" />
				<cc:attributionURL rdf:resource="http://www.english-heritage.org.uk" />
				<cc:attributionName xml:lang="en">English Heritage</cc:attributionName>
				<dcterms:publisher rdf:resource="http://www.english-heritage.org.uk" />
			</skos:Concept>
		</skos:narrower>
		<skos:narrower rdf:resource="http://purl.org/heritagedata/schemes/eh_tbm/concepts/97844" />
		<skos:narrower>
			<skos:Concept rdf:about="http://purl.org/heritagedata/schemes/eh_tbm/concepts/97991">
				<skos:inScheme rdf:resource="http://purl.org/heritagedata/schemes/eh_tbm" />
				<dcterms:identifier>http://purl.org/heritagedata/schemes/eh_tbm/concepts/97991</dcterms:identifier>
				<skos:prefLabel xml:lang="en">IONA MARBLE</skos:prefLabel>
				<dcterms:issued rdf:datatype="http://www.w3.org/2001/XMLSchema#dateTime">2013-07-17T09:02:16</dcterms:issued>
				<skos:broader rdf:resource="http://purl.org/heritagedata/schemes/eh_tbm/concepts/98044" />
				<skos:scopeNote xml:lang="en">One of only three 'true' British marbles, pale green and white in colour.</skos:scopeNote>
				<cc:license rdf:resource="http://creativecommons.org/licenses/by/3.0" />
				<cc:attributionURL rdf:resource="http://www.english-heritage.org.uk" />
				<cc:attributionName xml:lang="en">English Heritage</cc:attributionName>
				<dcterms:publisher rdf:resource="http://www.english-heritage.org.uk" />
			</skos:Concept>
		</skos:narrower>
		<skos:broader rdf:resource="http://purl.org/heritagedata/schemes/eh_tbm/concepts/98216" />
		<skos:narrower>
			<skos:Concept rdf:about="http://purl.org/heritagedata/schemes/eh_tbm/concepts/98191">
				<skos:inScheme rdf:resource="http://purl.org/heritagedata/schemes/eh_tbm" />
				<dcterms:identifier>http://purl.org/heritagedata/schemes/eh_tbm/concepts/98191</dcterms:identifier>
				<skos:prefLabel xml:lang="en">SKYE MARBLE</skos:prefLabel>
				<dcterms:issued rdf:datatype="http://www.w3.org/2001/XMLSchema#dateTime">2013-07-17T09:02:16</dcterms:issued>
				<skos:broader rdf:resource="http://purl.org/heritagedata/schemes/eh_tbm/concepts/98044" />
				<skos:scopeNote xml:lang="en">One of only three 'true' British marbles, white in colour, predominantly used for sculptures and statues.</skos:scopeNote>
				<cc:license rdf:resource="http://creativecommons.org/licenses/by/3.0" />
				<cc:attributionURL rdf:resource="http://www.english-heritage.org.uk" />
				<cc:attributionName xml:lang="en">English Heritage</cc:attributionName>
				<dcterms:publisher rdf:resource="http://www.english-heritage.org.uk" />
			</skos:Concept>
		</skos:narrower>
		<skos:related rdf:resource="http://purl.org/heritagedata/schemes/eh_tbm/concepts/97704" />
		<skos:related rdf:resource="http://purl.org/heritagedata/schemes/eh_tbm/concepts/97800" />
		<skos:related rdf:resource="http://purl.org/heritagedata/schemes/eh_tbm/concepts/98028" />
		<skos:related rdf:resource="http://purl.org/heritagedata/schemes/eh_tbm/concepts/98118" />
		<skos:related rdf:resource="http://purl.org/heritagedata/schemes/eh_tbm/concepts/98131" />
		<skos:related rdf:resource="http://purl.org/heritagedata/schemes/eh_tbm/concepts/98174" />
		<skos:scopeNote xml:lang="en">Collective name for, in a true geological sense, a metamorphosed limestone, eg. Carrara marble, and, in the British sense any decorative stone that will take a polish, eg. Purbeck marble. In the latter's case index with specific stone type where given.</skos:scopeNote>
		<cc:license rdf:resource="http://creativecommons.org/licenses/by/3.0" />
		<cc:attributionURL rdf:resource="http://www.english-heritage.org.uk" />
		<cc:attributionName xml:lang="en">English Heritage</cc:attributionName>
		<dcterms:publisher rdf:resource="http://www.english-heritage.org.uk" />
	</skos:Concept>
	<skos:Concept rdf:about="http://purl.org/heritagedata/schemes/eh_tbm/concepts/98045">
		<skos:inScheme rdf:resource="http://purl.org/heritagedata/schemes/eh_tbm" />
		<dcterms:identifier>http://purl.org/heritagedata/schemes/eh_tbm/concepts/98045</dcterms:identifier>
		<skos:prefLabel xml:lang="en">MARLSTONE</skos:prefLabel>
		<dcterms:issued rdf:datatype="http://www.w3.org/2001/XMLSchema#dateTime">2013-07-17T09:02:16</dcterms:issued>
		<skos:altLabel xml:lang="en">Uppingham Stone</skos:altLabel>
		<skos:broader rdf:resource="http://purl.org/heritagedata/schemes/eh_tbm/concepts/98024" />
		<skos:related rdf:resource="http://purl.org/heritagedata/schemes/eh_tbm/concepts/97993" />
		<skos:related rdf:resource="http://purl.org/heritagedata/schemes/eh_tbm/concepts/98180" />
		<skos:scopeNote xml:lang="en">Fine grained, iron rich, liassic limestone, found in Dorset, Somerset, Oxfordshire, Northamptonshire, Leicestershire and Rutland.</skos:scopeNote>
		<cc:license rdf:resource="http://creativecommons.org/licenses/by/3.0" />
		<cc:attributionURL rdf:resource="http://www.english-heritage.org.uk" />
		<cc:attributionName xml:lang="en">English Heritage</cc:attributionName>
		<dcterms:publisher rdf:resource="http://www.english-heritage.org.uk" />
	</skos:Concept>
	<skos:Concept rdf:about="http://purl.org/heritagedata/schemes/eh_tbm/concepts/98047">
		<skos:inScheme rdf:resource="http://purl.org/heritagedata/schemes/eh_tbm" />
		<dcterms:identifier>http://purl.org/heritagedata/schemes/eh_tbm/concepts/98047</dcterms:identifier>
		<skos:prefLabel xml:lang="en">MATHEMATICAL TILE</skos:prefLabel>
		<dcterms:issued rdf:datatype="http://www.w3.org/2001/XMLSchema#dateTime">2013-07-17T09:02:16</dcterms:issued>
		<skos:broader rdf:resource="http://purl.org/heritagedata/schemes/eh_tbm/concepts/98241" />
		<skos:related rdf:resource="http://purl.org/heritagedata/schemes/eh_tbm/concepts/97777" />
		<skos:scopeNote xml:lang="en">Tile nailed externally to a wall and usually laid in mortar designed to present a brick-like appearance.</skos:scopeNote>
		<cc:license rdf:resource="http://creativecommons.org/licenses/by/3.0" />
		<cc:attributionURL rdf:resource="http://www.english-heritage.org.uk" />
		<cc:attributionName xml:lang="en">English Heritage</cc:attributionName>
		<dcterms:publisher rdf:resource="http://www.english-heritage.org.uk" />
	</skos:Concept>
	<skos:Concept rdf:about="http://purl.org/heritagedata/schemes/eh_tbm/concepts/98061">
		<skos:inScheme rdf:resource="http://purl.org/heritagedata/schemes/eh_tbm" />
		<dcterms:identifier>http://purl.org/heritagedata/schemes/eh_tbm/concepts/98061</dcterms:identifier>
		<skos:prefLabel xml:lang="en">MOORSTONE</skos:prefLabel>
		<dcterms:issued rdf:datatype="http://www.w3.org/2001/XMLSchema#dateTime">2013-07-17T09:02:16</dcterms:issued>
		<skos:broader rdf:resource="http://purl.org/heritagedata/schemes/eh_tbm/concepts/97944" />
		<skos:related rdf:resource="http://purl.org/heritagedata/schemes/eh_tbm/concepts/98173" />
		<skos:scopeNote xml:lang="en">Stonemason's name for granite found lying upon the moorland surface, as opposed to having been quarried, in the West Country and the Lake District. Used, as found, since prehistoric times, in later years was often dressed and shaped.</skos:scopeNote>
		<cc:license rdf:resource="http://creativecommons.org/licenses/by/3.0" />
		<cc:attributionURL rdf:resource="http://www.english-heritage.org.uk" />
		<cc:attributionName xml:lang="en">English Heritage</cc:attributionName>
		<dcterms:publisher rdf:resource="http://www.english-heritage.org.uk" />
	</skos:Concept>
	<skos:Concept rdf:about="http://purl.org/heritagedata/schemes/eh_tbm/concepts/98062">
		<skos:inScheme rdf:resource="http://purl.org/heritagedata/schemes/eh_tbm" />
		<dcterms:identifier>http://purl.org/heritagedata/schemes/eh_tbm/concepts/98062</dcterms:identifier>
		<skos:prefLabel xml:lang="en">MORTAR</skos:prefLabel>
		<dcterms:issued rdf:datatype="http://www.w3.org/2001/XMLSchema#dateTime">2013-07-17T09:02:16</dcterms:issued>
		<skos:altLabel xml:lang="en">Lime Mortar</skos:altLabel>
		<skos:broader rdf:resource="http://purl.org/heritagedata/schemes/eh_tbm/concepts/97810" />
		<skos:related rdf:resource="http://purl.org/heritagedata/schemes/eh_tbm/concepts/97809" />
		<skos:related rdf:resource="http://purl.org/heritagedata/schemes/eh_tbm/concepts/98026" />
		<skos:related rdf:resource="http://purl.org/heritagedata/schemes/eh_tbm/concepts/98170" />
		<skos:scopeNote xml:lang="en">A mixture of lime or more recently cement with sand and water used for bonding stones or bricks.</skos:scopeNote>
		<cc:license rdf:resource="http://creativecommons.org/licenses/by/3.0" />
		<cc:attributionURL rdf:resource="http://www.english-heritage.org.uk" />
		<cc:attributionName xml:lang="en">English Heritage</cc:attributionName>
		<dcterms:publisher rdf:resource="http://www.english-heritage.org.uk" />
	</skos:Concept>
	<skos:Concept rdf:about="http://purl.org/heritagedata/schemes/eh_tbm/concepts/98075">
		<skos:inScheme rdf:resource="http://purl.org/heritagedata/schemes/eh_tbm" />
		<dcterms:identifier>http://purl.org/heritagedata/schemes/eh_tbm/concepts/98075</dcterms:identifier>
		<skos:prefLabel xml:lang="en">OOLITIC LIMESTONE</skos:prefLabel>
		<dcterms:issued rdf:datatype="http://www.w3.org/2001/XMLSchema#dateTime">2013-07-17T09:02:16</dcterms:issued>
		<skos:altLabel xml:lang="en">Oxford Stone</skos:altLabel>
		<skos:altLabel xml:lang="en">Painswick Stone</skos:altLabel>
		<skos:altLabel xml:lang="en">Stonesfield Slate</skos:altLabel>
		<skos:altLabel xml:lang="en">Taynton Stone</skos:altLabel>
		<skos:altLabel xml:lang="en">Wheatley Stone</skos:altLabel>
		<skos:altLabel xml:lang="en">Campden Stone</skos:altLabel>
		<skos:altLabel xml:lang="en">Cary Stone</skos:altLabel>
		<skos:altLabel xml:lang="en">Charlbury Stone</skos:altLabel>
		<skos:altLabel xml:lang="en">Oolite</skos:altLabel>
		<skos:altLabel xml:lang="en">Coral Rag Limestone</skos:altLabel>
		<skos:altLabel xml:lang="en">Cornbrash Limestone</skos:altLabel>
		<skos:altLabel xml:lang="en">Doulting Stone</skos:altLabel>
		<skos:altLabel xml:lang="en">Dundry Stone</skos:altLabel>
		<skos:altLabel xml:lang="en">Headington Stone</skos:altLabel>
		<skos:narrower>
			<skos:Concept rdf:about="http://purl.org/heritagedata/schemes/eh_tbm/concepts/97737">
				<skos:inScheme rdf:resource="http://purl.org/heritagedata/schemes/eh_tbm" />
				<dcterms:identifier>http://purl.org/heritagedata/schemes/eh_tbm/concepts/97737</dcterms:identifier>
				<skos:prefLabel xml:lang="en">BATH STONE</skos:prefLabel>
				<dcterms:issued rdf:datatype="http://www.w3.org/2001/XMLSchema#dateTime">2013-07-17T09:02:16</dcterms:issued>
				<skos:altLabel xml:lang="en">Monks Park Stone</skos:altLabel>
				<skos:altLabel xml:lang="en">St Aldhelm Stone</skos:altLabel>
				<skos:altLabel xml:lang="en">Stoke Ground Stone</skos:altLabel>
				<skos:altLabel xml:lang="en">Westwood Stone</skos:altLabel>
				<skos:altLabel xml:lang="en">Winsley Ground</skos:altLabel>
				<skos:altLabel xml:lang="en">Box Ground</skos:altLabel>
				<skos:altLabel xml:lang="en">Box Rubblestone</skos:altLabel>
				<skos:altLabel xml:lang="en">Bradford Stone</skos:altLabel>
				<skos:altLabel xml:lang="en">Combe Down Stone</skos:altLabel>
				<skos:altLabel xml:lang="en">Corsham Stone</skos:altLabel>
				<skos:altLabel xml:lang="en">Hartham Park Stone</skos:altLabel>
				<skos:altLabel xml:lang="en">Hazlebury Stone</skos:altLabel>
				<skos:broader rdf:resource="http://purl.org/heritagedata/schemes/eh_tbm/concepts/98075" />
				<skos:scopeNote xml:lang="en">Even grained, poorly fossiliferous, light brown/cream coloured, oolitic limestone. Quarried in the Bath area.</skos:scopeNote>
				<cc:license rdf:resource="http://creativecommons.org/licenses/by/3.0" />
				<cc:attributionURL rdf:resource="http://www.english-heritage.org.uk" />
				<cc:attributionName xml:lang="en">English Heritage</cc:attributionName>
				<dcterms:publisher rdf:resource="http://www.english-heritage.org.uk" />
			</skos:Concept>
		</skos:narrower>
		<skos:narrower>
			<skos:Concept rdf:about="http://purl.org/heritagedata/schemes/eh_tbm/concepts/97863">
				<skos:inScheme rdf:resource="http://purl.org/heritagedata/schemes/eh_tbm" />
				<dcterms:identifier>http://purl.org/heritagedata/schemes/eh_tbm/concepts/97863</dcterms:identifier>
				<skos:prefLabel xml:lang="en">COTSWOLD STONE</skos:prefLabel>
				<dcterms:issued rdf:datatype="http://www.w3.org/2001/XMLSchema#dateTime">2013-07-17T09:02:16</dcterms:issued>
				<skos:altLabel xml:lang="en">Stanway Stone</skos:altLabel>
				<skos:altLabel xml:lang="en">Bladon Cotswold Stone</skos:altLabel>
				<skos:altLabel xml:lang="en">Cotswold Slate</skos:altLabel>
				<skos:altLabel xml:lang="en">Guiting Stone</skos:altLabel>
				<skos:broader rdf:resource="http://purl.org/heritagedata/schemes/eh_tbm/concepts/98075" />
				<skos:scopeNote xml:lang="en">Sandy, light brown (cream to golden) coloured limestone, easily worked and readily available.</skos:scopeNote>
				<cc:license rdf:resource="http://creativecommons.org/licenses/by/3.0" />
				<cc:attributionURL rdf:resource="http://www.english-heritage.org.uk" />
				<cc:attributionName xml:lang="en">English Heritage</cc:attributionName>
				<dcterms:publisher rdf:resource="http://www.english-heritage.org.uk" />
			</skos:Concept>
		</skos:narrower>
		<skos:narrower>
			<skos:Concept rdf:about="http://purl.org/heritagedata/schemes/eh_tbm/concepts/98029">
				<skos:inScheme rdf:resource="http://purl.org/heritagedata/schemes/eh_tbm" />
				<dcterms:identifier>http://purl.org/heritagedata/schemes/eh_tbm/concepts/98029</dcterms:identifier>
				<skos:prefLabel xml:lang="en">LINCOLNSHIRE LIMESTONE</skos:prefLabel>
				<dcterms:issued rdf:datatype="http://www.w3.org/2001/XMLSchema#dateTime">2013-07-17T09:02:16</dcterms:issued>
				<skos:altLabel xml:lang="en">Stamford Stone</skos:altLabel>
				<skos:altLabel xml:lang="en">Weatherbed</skos:altLabel>
				<skos:altLabel xml:lang="en">Weldon Stone</skos:altLabel>
				<skos:altLabel xml:lang="en">Casterton Stone</skos:altLabel>
				<skos:altLabel xml:lang="en">Clipsham Stone</skos:altLabel>
				<skos:altLabel xml:lang="en">Ancaster Stone</skos:altLabel>
				<skos:altLabel xml:lang="en">Barnack Stone</skos:altLabel>
				<skos:altLabel xml:lang="en">Collyweston Slate</skos:altLabel>
				<skos:altLabel xml:lang="en">Cosgrove Stone</skos:altLabel>
				<skos:altLabel xml:lang="en">Freebed</skos:altLabel>
				<skos:altLabel xml:lang="en">Hardwhite</skos:altLabel>
				<skos:altLabel xml:lang="en">Ketton Stone</skos:altLabel>
				<skos:broader rdf:resource="http://purl.org/heritagedata/schemes/eh_tbm/concepts/98075" />
				<skos:scopeNote xml:lang="en">Generic term for the oolitic limestones quarried in Northamptonshire, Lincolnshire and Rutland. Varying in grain size from medium to coarse, and colour from cream to pale brown.</skos:scopeNote>
				<cc:license rdf:resource="http://creativecommons.org/licenses/by/3.0" />
				<cc:attributionURL rdf:resource="http://www.english-heritage.org.uk" />
				<cc:attributionName xml:lang="en">English Heritage</cc:attributionName>
				<dcterms:publisher rdf:resource="http://www.english-heritage.org.uk" />
			</skos:Concept>
		</skos:narrower>
		<skos:broader rdf:resource="http://purl.org/heritagedata/schemes/eh_tbm/concepts/97999" />
		<skos:narrower rdf:resource="http://purl.org/heritagedata/schemes/eh_tbm/concepts/98123" />
		<skos:related rdf:resource="http://purl.org/heritagedata/schemes/eh_tbm/concepts/97993" />
		<skos:scopeNote xml:lang="en">Limestone formed during the Jurassic period. Composed of ooliths, literally small rock particles with the appearance of fish roe.</skos:scopeNote>
		<cc:license rdf:resource="http://creativecommons.org/licenses/by/3.0" />
		<cc:attributionURL rdf:resource="http://www.english-heritage.org.uk" />
		<cc:attributionName xml:lang="en">English Heritage</cc:attributionName>
		<dcterms:publisher rdf:resource="http://www.english-heritage.org.uk" />
	</skos:Concept>
	<skos:Concept rdf:about="http://purl.org/heritagedata/schemes/eh_tbm/concepts/98080">
		<skos:inScheme rdf:resource="http://purl.org/heritagedata/schemes/eh_tbm" />
		<dcterms:identifier>http://purl.org/heritagedata/schemes/eh_tbm/concepts/98080</dcterms:identifier>
		<skos:prefLabel xml:lang="en">PANEL BOARD</skos:prefLabel>
		<dcterms:issued rdf:datatype="http://www.w3.org/2001/XMLSchema#dateTime">2013-07-17T09:02:16</dcterms:issued>
		<skos:narrower rdf:resource="http://purl.org/heritagedata/schemes/eh_tbm/concepts/97917" />
		<skos:broader rdf:resource="http://purl.org/heritagedata/schemes/eh_tbm/concepts/98041" />
		<skos:narrower rdf:resource="http://purl.org/heritagedata/schemes/eh_tbm/concepts/98113" />
		<skos:narrower rdf:resource="http://purl.org/heritagedata/schemes/eh_tbm/concepts/98116" />
		<skos:narrower rdf:resource="http://purl.org/heritagedata/schemes/eh_tbm/concepts/98303" />
		<skos:scopeNote xml:lang="en">Large board used for covering the internal surfaces of a building, ie. floors, walls and ceilings. Some forms can be used as external cladding.</skos:scopeNote>
		<cc:license rdf:resource="http://creativecommons.org/licenses/by/3.0" />
		<cc:attributionURL rdf:resource="http://www.english-heritage.org.uk" />
		<cc:attributionName xml:lang="en">English Heritage</cc:attributionName>
		<dcterms:publisher rdf:resource="http://www.english-heritage.org.uk" />
	</skos:Concept>
	<skos:Concept rdf:about="http://purl.org/heritagedata/schemes/eh_tbm/concepts/98081">
		<skos:inScheme rdf:resource="http://purl.org/heritagedata/schemes/eh_tbm" />
		<dcterms:identifier>http://purl.org/heritagedata/schemes/eh_tbm/concepts/98081</dcterms:identifier>
		<skos:prefLabel xml:lang="en">PANTILE</skos:prefLabel>
		<dcterms:issued rdf:datatype="http://www.w3.org/2001/XMLSchema#dateTime">2013-07-17T09:02:16</dcterms:issued>
		<skos:broader rdf:resource="http://purl.org/heritagedata/schemes/eh_tbm/concepts/98241" />
		<skos:related rdf:resource="http://purl.org/heritagedata/schemes/eh_tbm/concepts/97827" />
		<skos:related rdf:resource="http://purl.org/heritagedata/schemes/eh_tbm/concepts/97840" />
		<skos:scopeNote xml:lang="en">Curved, interlocking roof tile of S-shaped section usually made of clay or concrete.</skos:scopeNote>
		<cc:license rdf:resource="http://creativecommons.org/licenses/by/3.0" />
		<cc:attributionURL rdf:resource="http://www.english-heritage.org.uk" />
		<cc:attributionName xml:lang="en">English Heritage</cc:attributionName>
		<dcterms:publisher rdf:resource="http://www.english-heritage.org.uk" />
	</skos:Concept>
	<skos:Concept rdf:about="http://purl.org/heritagedata/schemes/eh_tbm/concepts/98147">
		<skos:inScheme rdf:resource="http://purl.org/heritagedata/schemes/eh_tbm" />
		<dcterms:identifier>http://purl.org/heritagedata/schemes/eh_tbm/concepts/98147</dcterms:identifier>
		<skos:prefLabel xml:lang="en">RENDER</skos:prefLabel>
		<dcterms:issued rdf:datatype="http://www.w3.org/2001/XMLSchema#dateTime">2013-07-17T09:02:16</dcterms:issued>
		<skos:altLabel xml:lang="en">Tyrolean</skos:altLabel>
		<skos:altLabel xml:lang="en">Cement Render</skos:altLabel>
		<skos:narrower rdf:resource="http://purl.org/heritagedata/schemes/eh_tbm/concepts/98090" />
		<skos:narrower rdf:resource="http://purl.org/heritagedata/schemes/eh_tbm/concepts/98110" />
		<skos:broader rdf:resource="http://purl.org/heritagedata/schemes/eh_tbm/concepts/98041" />
		<skos:narrower>
			<skos:Concept rdf:about="http://purl.org/heritagedata/schemes/eh_tbm/concepts/98162">
				<skos:inScheme rdf:resource="http://purl.org/heritagedata/schemes/eh_tbm" />
				<dcterms:identifier>http://purl.org/heritagedata/schemes/eh_tbm/concepts/98162</dcterms:identifier>
				<skos:prefLabel xml:lang="en">ROUGHCAST</skos:prefLabel>
				<dcterms:issued rdf:datatype="http://www.w3.org/2001/XMLSchema#dateTime">2013-07-17T09:02:16</dcterms:issued>
				<skos:broader rdf:resource="http://purl.org/heritagedata/schemes/eh_tbm/concepts/98147" />
				<skos:scopeNote xml:lang="en">A render including an aggregate of gravel or stone chipping thrown rather than trowelled onto an external wall.</skos:scopeNote>
				<cc:license rdf:resource="http://creativecommons.org/licenses/by/3.0" />
				<cc:attributionURL rdf:resource="http://www.english-heritage.org.uk" />
				<cc:attributionName xml:lang="en">English Heritage</cc:attributionName>
				<dcterms:publisher rdf:resource="http://www.english-heritage.org.uk" />
			</skos:Concept>
		</skos:narrower>
		<skos:narrower>
			<skos:Concept rdf:about="http://purl.org/heritagedata/schemes/eh_tbm/concepts/98220">
				<skos:inScheme rdf:resource="http://purl.org/heritagedata/schemes/eh_tbm" />
				<dcterms:identifier>http://purl.org/heritagedata/schemes/eh_tbm/concepts/98220</dcterms:identifier>
				<skos:prefLabel xml:lang="en">STUCCO</skos:prefLabel>
				<dcterms:issued rdf:datatype="http://www.w3.org/2001/XMLSchema#dateTime">2013-07-17T09:02:16</dcterms:issued>
				<skos:broader rdf:resource="http://purl.org/heritagedata/schemes/eh_tbm/concepts/98147" />
				<skos:scopeNote xml:lang="en">Smooth rendering applied to the exterior of buildings which may be incised to suggest coursed masonry. Made of lime and sand or brick dust, and more recently, cement.</skos:scopeNote>
				<cc:license rdf:resource="http://creativecommons.org/licenses/by/3.0" />
				<cc:attributionURL rdf:resource="http://www.english-heritage.org.uk" />
				<cc:attributionName xml:lang="en">English Heritage</cc:attributionName>
				<dcterms:publisher rdf:resource="http://www.english-heritage.org.uk" />
			</skos:Concept>
		</skos:narrower>
		<skos:scopeNote xml:lang="en">A general term for the weatherproof coat on the external walls of a building.</skos:scopeNote>
		<cc:license rdf:resource="http://creativecommons.org/licenses/by/3.0" />
		<cc:attributionURL rdf:resource="http://www.english-heritage.org.uk" />
		<cc:attributionName xml:lang="en">English Heritage</cc:attributionName>
		<dcterms:publisher rdf:resource="http://www.english-heritage.org.uk" />
	</skos:Concept>
	<skos:Concept rdf:about="http://purl.org/heritagedata/schemes/eh_tbm/concepts/98148">
		<skos:inScheme rdf:resource="http://purl.org/heritagedata/schemes/eh_tbm" />
		<dcterms:identifier>http://purl.org/heritagedata/schemes/eh_tbm/concepts/98148</dcterms:identifier>
		<skos:prefLabel xml:lang="en">RESIDUE</skos:prefLabel>
		<dcterms:issued rdf:datatype="http://www.w3.org/2001/XMLSchema#dateTime">2013-07-17T09:02:16</dcterms:issued>
		<skos:altLabel xml:lang="en">Industrial Waste</skos:altLabel>
		<skos:narrower>
			<skos:Concept rdf:about="http://purl.org/heritagedata/schemes/eh_tbm/concepts/97830">
				<skos:inScheme rdf:resource="http://purl.org/heritagedata/schemes/eh_tbm" />
				<dcterms:identifier>http://purl.org/heritagedata/schemes/eh_tbm/concepts/97830</dcterms:identifier>
				<skos:prefLabel xml:lang="en">CLINKER</skos:prefLabel>
				<dcterms:issued rdf:datatype="http://www.w3.org/2001/XMLSchema#dateTime">2013-07-17T09:02:16</dcterms:issued>
				<skos:broader rdf:resource="http://purl.org/heritagedata/schemes/eh_tbm/concepts/98148" />
				<skos:scopeNote xml:lang="en">Fused ash from furnaces used as aggregate.</skos:scopeNote>
				<cc:license rdf:resource="http://creativecommons.org/licenses/by/3.0" />
				<cc:attributionURL rdf:resource="http://www.english-heritage.org.uk" />
				<cc:attributionName xml:lang="en">English Heritage</cc:attributionName>
				<dcterms:publisher rdf:resource="http://www.english-heritage.org.uk" />
			</skos:Concept>
		</skos:narrower>
		<skos:narrower rdf:resource="http://purl.org/heritagedata/schemes/eh_tbm/concepts/98026" />
		<skos:broader rdf:resource="http://purl.org/heritagedata/schemes/eh_tbm/concepts/98041" />
		<skos:narrower>
			<skos:Concept rdf:about="http://purl.org/heritagedata/schemes/eh_tbm/concepts/98193">
				<skos:inScheme rdf:resource="http://purl.org/heritagedata/schemes/eh_tbm" />
				<dcterms:identifier>http://purl.org/heritagedata/schemes/eh_tbm/concepts/98193</dcterms:identifier>
				<skos:prefLabel xml:lang="en">SLAG</skos:prefLabel>
				<dcterms:issued rdf:datatype="http://www.w3.org/2001/XMLSchema#dateTime">2013-07-17T09:02:16</dcterms:issued>
				<skos:broader rdf:resource="http://purl.org/heritagedata/schemes/eh_tbm/concepts/98148" />
				<skos:scopeNote xml:lang="en">Waste material or dross separated from metals during smelting or refining.</skos:scopeNote>
				<cc:license rdf:resource="http://creativecommons.org/licenses/by/3.0" />
				<cc:attributionURL rdf:resource="http://www.english-heritage.org.uk" />
				<cc:attributionName xml:lang="en">English Heritage</cc:attributionName>
				<dcterms:publisher rdf:resource="http://www.english-heritage.org.uk" />
			</skos:Concept>
		</skos:narrower>
		<skos:related rdf:resource="http://purl.org/heritagedata/schemes/eh_tbm/concepts/97776" />
		<skos:scopeNote xml:lang="en">By-product or waste, resulting from an industrial process.</skos:scopeNote>
		<cc:license rdf:resource="http://creativecommons.org/licenses/by/3.0" />
		<cc:attributionURL rdf:resource="http://www.english-heritage.org.uk" />
		<cc:attributionName xml:lang="en">English Heritage</cc:attributionName>
		<dcterms:publisher rdf:resource="http://www.english-heritage.org.uk" />
	</skos:Concept>
	<skos:Concept rdf:about="http://purl.org/heritagedata/schemes/eh_tbm/concepts/98150">
		<skos:inScheme rdf:resource="http://purl.org/heritagedata/schemes/eh_tbm" />
		<dcterms:identifier>http://purl.org/heritagedata/schemes/eh_tbm/concepts/98150</dcterms:identifier>
		<skos:prefLabel xml:lang="en">RHYOLITE</skos:prefLabel>
		<dcterms:issued rdf:datatype="http://www.w3.org/2001/XMLSchema#dateTime">2013-07-17T09:02:16</dcterms:issued>
		<skos:broader rdf:resource="http://purl.org/heritagedata/schemes/eh_tbm/concepts/98216" />
		<skos:related rdf:resource="http://purl.org/heritagedata/schemes/eh_tbm/concepts/97734" />
		<skos:related rdf:resource="http://purl.org/heritagedata/schemes/eh_tbm/concepts/97891" />
		<skos:related rdf:resource="http://purl.org/heritagedata/schemes/eh_tbm/concepts/98181" />
		<skos:related rdf:resource="http://purl.org/heritagedata/schemes/eh_tbm/concepts/98229" />
		<skos:scopeNote xml:lang="en">Fine grained, acidic, light-grey/white/ brown/red-coloured igneous rock.</skos:scopeNote>
		<cc:license rdf:resource="http://creativecommons.org/licenses/by/3.0" />
		<cc:attributionURL rdf:resource="http://www.english-heritage.org.uk" />
		<cc:attributionName xml:lang="en">English Heritage</cc:attributionName>
		<dcterms:publisher rdf:resource="http://www.english-heritage.org.uk" />
	</skos:Concept>
	<skos:Concept rdf:about="http://purl.org/heritagedata/schemes/eh_tbm/concepts/98156">
		<skos:inScheme rdf:resource="http://purl.org/heritagedata/schemes/eh_tbm" />
		<dcterms:identifier>http://purl.org/heritagedata/schemes/eh_tbm/concepts/98156</dcterms:identifier>
		<skos:prefLabel xml:lang="en">ROMAN CEMENT</skos:prefLabel>
		<dcterms:issued rdf:datatype="http://www.w3.org/2001/XMLSchema#dateTime">2013-07-17T09:02:16</dcterms:issued>
		<skos:broader rdf:resource="http://purl.org/heritagedata/schemes/eh_tbm/concepts/97810" />
		<skos:related rdf:resource="http://purl.org/heritagedata/schemes/eh_tbm/concepts/98026" />
		<skos:related rdf:resource="http://purl.org/heritagedata/schemes/eh_tbm/concepts/98180" />
		<skos:scopeNote xml:lang="en">Technically a quick setting hydraulic cement or lime,but term has been adapted to denote cement made from burning lumps of marl found in London clay,a technique adopted for C19th building work. Name not intended to denote a relationship with Roman period</skos:scopeNote>
		<cc:license rdf:resource="http://creativecommons.org/licenses/by/3.0" />
		<cc:attributionURL rdf:resource="http://www.english-heritage.org.uk" />
		<cc:attributionName xml:lang="en">English Heritage</cc:attributionName>
		<dcterms:publisher rdf:resource="http://www.english-heritage.org.uk" />
	</skos:Concept>
	<skos:Concept rdf:about="http://purl.org/heritagedata/schemes/eh_tbm/concepts/98164">
		<skos:inScheme rdf:resource="http://purl.org/heritagedata/schemes/eh_tbm" />
		<dcterms:identifier>http://purl.org/heritagedata/schemes/eh_tbm/concepts/98164</dcterms:identifier>
		<skos:prefLabel xml:lang="en">RUBBER</skos:prefLabel>
		<dcterms:issued rdf:datatype="http://www.w3.org/2001/XMLSchema#dateTime">2013-07-17T09:02:16</dcterms:issued>
		<skos:broader rdf:resource="http://purl.org/heritagedata/schemes/eh_tbm/concepts/98041" />
		<skos:related rdf:resource="http://purl.org/heritagedata/schemes/eh_tbm/concepts/98111" />
		<skos:scopeNote xml:lang="en">Flexible, synthetic, polymeric organic material formed by chemical synthesis usually in imitation of a natural substance. It can be moulded to shape, extruded or formed into a sheet from solid or foam material.</skos:scopeNote>
		<cc:license rdf:resource="http://creativecommons.org/licenses/by/3.0" />
		<cc:attributionURL rdf:resource="http://www.english-heritage.org.uk" />
		<cc:attributionName xml:lang="en">English Heritage</cc:attributionName>
		<dcterms:publisher rdf:resource="http://www.english-heritage.org.uk" />
	</skos:Concept>
	<skos:Concept rdf:about="http://purl.org/heritagedata/schemes/eh_tbm/concepts/98165">
		<skos:inScheme rdf:resource="http://purl.org/heritagedata/schemes/eh_tbm" />
		<dcterms:identifier>http://purl.org/heritagedata/schemes/eh_tbm/concepts/98165</dcterms:identifier>
		<skos:prefLabel xml:lang="en">RUBBLE</skos:prefLabel>
		<dcterms:issued rdf:datatype="http://www.w3.org/2001/XMLSchema#dateTime">2013-07-17T09:02:16</dcterms:issued>
		<skos:broader rdf:resource="http://purl.org/heritagedata/schemes/eh_tbm/concepts/98046" />
		<skos:related rdf:resource="http://purl.org/heritagedata/schemes/eh_tbm/concepts/98216" />
		<skos:scopeNote xml:lang="en">Rough, unhewn, undressed building stones with irregular faces, generally not laid in regular courses. Index with type of stone if specified.</skos:scopeNote>
		<cc:license rdf:resource="http://creativecommons.org/licenses/by/3.0" />
		<cc:attributionURL rdf:resource="http://www.english-heritage.org.uk" />
		<cc:attributionName xml:lang="en">English Heritage</cc:attributionName>
		<dcterms:publisher rdf:resource="http://www.english-heritage.org.uk" />
	</skos:Concept>
	<skos:Concept rdf:about="http://purl.org/heritagedata/schemes/eh_tbm/concepts/98170">
		<skos:inScheme rdf:resource="http://purl.org/heritagedata/schemes/eh_tbm" />
		<dcterms:identifier>http://purl.org/heritagedata/schemes/eh_tbm/concepts/98170</dcterms:identifier>
		<skos:prefLabel xml:lang="en">SAND</skos:prefLabel>
		<dcterms:issued rdf:datatype="http://www.w3.org/2001/XMLSchema#dateTime">2013-07-17T09:02:16</dcterms:issued>
		<skos:broader rdf:resource="http://purl.org/heritagedata/schemes/eh_tbm/concepts/97903" />
		<skos:related rdf:resource="http://purl.org/heritagedata/schemes/eh_tbm/concepts/97809" />
		<skos:related rdf:resource="http://purl.org/heritagedata/schemes/eh_tbm/concepts/97840" />
		<skos:related rdf:resource="http://purl.org/heritagedata/schemes/eh_tbm/concepts/97947" />
		<skos:related rdf:resource="http://purl.org/heritagedata/schemes/eh_tbm/concepts/98062" />
		<skos:scopeNote xml:lang="en">Granular material consisting of small eroded fragments of rock or mineral grains, finer than gravel used as an ingredient in mortar and other traditional building materials.</skos:scopeNote>
		<cc:license rdf:resource="http://creativecommons.org/licenses/by/3.0" />
		<cc:attributionURL rdf:resource="http://www.english-heritage.org.uk" />
		<cc:attributionName xml:lang="en">English Heritage</cc:attributionName>
		<dcterms:publisher rdf:resource="http://www.english-heritage.org.uk" />
	</skos:Concept>
	<skos:Concept rdf:about="http://purl.org/heritagedata/schemes/eh_tbm/concepts/98171">
		<skos:inScheme rdf:resource="http://purl.org/heritagedata/schemes/eh_tbm" />
		<dcterms:identifier>http://purl.org/heritagedata/schemes/eh_tbm/concepts/98171</dcterms:identifier>
		<skos:prefLabel xml:lang="en">SANDSTONE</skos:prefLabel>
		<dcterms:issued rdf:datatype="http://www.w3.org/2001/XMLSchema#dateTime">2013-07-17T09:02:16</dcterms:issued>
		<skos:altLabel xml:lang="en">Pencaemaur Stone</skos:altLabel>
		<skos:altLabel xml:lang="en">Penrith Red Sandstone</skos:altLabel>
		<skos:altLabel xml:lang="en">Penshaw Sandstone</skos:altLabel>
		<skos:altLabel xml:lang="en">Permian Sandstone</skos:altLabel>
		<skos:altLabel xml:lang="en">Prudham Stone</skos:altLabel>
		<skos:altLabel xml:lang="en">Rainhill Stone</skos:altLabel>
		<skos:altLabel xml:lang="en">Rainow Stone</skos:altLabel>
		<skos:altLabel xml:lang="en">Rassau Stone</skos:altLabel>
		<skos:altLabel xml:lang="en">Red Wilderness Stone</skos:altLabel>
		<skos:altLabel xml:lang="en">Lane Head Stone</skos:altLabel>
		<skos:altLabel xml:lang="en">Lazonby Red Sandstone</skos:altLabel>
		<skos:altLabel xml:lang="en">Locharbriggs Stone</skos:altLabel>
		<skos:altLabel xml:lang="en">Lower Greensand</skos:altLabel>
		<skos:altLabel xml:lang="en">Mansfield Stone</skos:altLabel>
		<skos:altLabel xml:lang="en">Moulton Stone</skos:altLabel>
		<skos:altLabel xml:lang="en">Ringby Stone</skos:altLabel>
		<skos:altLabel xml:lang="en">Rose Brae Stone</skos:altLabel>
		<skos:altLabel xml:lang="en">Salcombe Stone</skos:altLabel>
		<skos:altLabel xml:lang="en">Soudley Stone</skos:altLabel>
		<skos:altLabel xml:lang="en">Spinkwell Stone</skos:altLabel>
		<skos:altLabel xml:lang="en">Springwell Stone</skos:altLabel>
		<skos:altLabel xml:lang="en">Spynie Stone</skos:altLabel>
		<skos:altLabel xml:lang="en">St Bees Stone</skos:altLabel>
		<skos:altLabel xml:lang="en">St Boniface Stone</skos:altLabel>
		<skos:altLabel xml:lang="en">Stainton Stone</skos:altLabel>
		<skos:altLabel xml:lang="en">Swindon Stone</skos:altLabel>
		<skos:altLabel xml:lang="en">Thorverton Stone</skos:altLabel>
		<skos:altLabel xml:lang="en">Tixall Stone</skos:altLabel>
		<skos:altLabel xml:lang="en">Waterholes Sandstone</skos:altLabel>
		<skos:altLabel xml:lang="en">Wellfield Stone</skos:altLabel>
		<skos:altLabel xml:lang="en">Whitby Stone</skos:altLabel>
		<skos:altLabel xml:lang="en">Windy Hill Stone</skos:altLabel>
		<skos:altLabel xml:lang="en">Woolton Stone</skos:altLabel>
		<skos:altLabel xml:lang="en">Yorkshire Delph</skos:altLabel>
		<skos:altLabel xml:lang="en">Blaxter Stone</skos:altLabel>
		<skos:altLabel xml:lang="en">Bramley Fall Stone</skos:altLabel>
		<skos:altLabel xml:lang="en">Britannia Stone</skos:altLabel>
		<skos:altLabel xml:lang="en">Bunter Stone</skos:altLabel>
		<skos:altLabel xml:lang="en">Caerbwdy Stone</skos:altLabel>
		<skos:altLabel xml:lang="en">Caithness Flagstone</skos:altLabel>
		<skos:altLabel xml:lang="en">Cardeston Stone</skos:altLabel>
		<skos:altLabel xml:lang="en">Chatwell Stone</skos:altLabel>
		<skos:altLabel xml:lang="en">Clashach Stone</skos:altLabel>
		<skos:altLabel xml:lang="en">Auchinlea Stone</skos:altLabel>
		<skos:altLabel xml:lang="en">Corsehill Stone</skos:altLabel>
		<skos:altLabel xml:lang="en">Coxbench Sandstone</skos:altLabel>
		<skos:altLabel xml:lang="en">Craigleith Stone</skos:altLabel>
		<skos:altLabel xml:lang="en">Culm Measures Stone</skos:altLabel>
		<skos:altLabel xml:lang="en">Culm Stone</skos:altLabel>
		<skos:altLabel xml:lang="en">Cumberland Stone</skos:altLabel>
		<skos:altLabel xml:lang="en">Darney Stone</skos:altLabel>
		<skos:altLabel xml:lang="en">Davie Blocks Stone</skos:altLabel>
		<skos:altLabel xml:lang="en">Delph Stone</skos:altLabel>
		<skos:altLabel xml:lang="en">Derbyshire Stone</skos:altLabel>
		<skos:altLabel xml:lang="en">Doddington Stone</skos:altLabel>
		<skos:altLabel xml:lang="en">Dunhouse Stone</skos:altLabel>
		<skos:altLabel xml:lang="en">Dunston Stone</skos:altLabel>
		<skos:altLabel xml:lang="en">Forest Of Dean Stone</skos:altLabel>
		<skos:altLabel xml:lang="en">Forest Stone (Gloucestershire)</skos:altLabel>
		<skos:altLabel xml:lang="en">Foxs Wood Rubble</skos:altLabel>
		<skos:altLabel xml:lang="en">Green Brae Stone</skos:altLabel>
		<skos:altLabel xml:lang="en">Greensand Stone</skos:altLabel>
		<skos:altLabel xml:lang="en">Grinshill Stone</skos:altLabel>
		<skos:altLabel xml:lang="en">Hailes Stone</skos:altLabel>
		<skos:altLabel xml:lang="en">Hatherleigh Stone</skos:altLabel>
		<skos:altLabel xml:lang="en">Heavitree Stone</skos:altLabel>
		<skos:altLabel xml:lang="en">Hollington Stone</skos:altLabel>
		<skos:altLabel xml:lang="en">Kerridge Stone</skos:altLabel>
		<skos:altLabel xml:lang="en">Keuper Stone</skos:altLabel>
		<skos:altLabel xml:lang="en">Ladycross Stone</skos:altLabel>
		<skos:narrower>
			<skos:Concept rdf:about="http://purl.org/heritagedata/schemes/eh_tbm/concepts/97731">
				<skos:inScheme rdf:resource="http://purl.org/heritagedata/schemes/eh_tbm" />
				<dcterms:identifier>http://purl.org/heritagedata/schemes/eh_tbm/concepts/97731</dcterms:identifier>
				<skos:prefLabel xml:lang="en">BARGATE STONE</skos:prefLabel>
				<dcterms:issued rdf:datatype="http://www.w3.org/2001/XMLSchema#dateTime">2013-07-17T09:02:16</dcterms:issued>
				<skos:altLabel xml:lang="en">Burgate Stone</skos:altLabel>
				<skos:broader rdf:resource="http://purl.org/heritagedata/schemes/eh_tbm/concepts/98171" />
				<skos:scopeNote xml:lang="en">Hard, coarse grained, calcareous sandstone, coloured by iron oxide. Quarried in the Guildford and Godalming area of the South East.</skos:scopeNote>
				<cc:license rdf:resource="http://creativecommons.org/licenses/by/3.0" />
				<cc:attributionURL rdf:resource="http://www.english-heritage.org.uk" />
				<cc:attributionName xml:lang="en">English Heritage</cc:attributionName>
				<dcterms:publisher rdf:resource="http://www.english-heritage.org.uk" />
			</skos:Concept>
		</skos:narrower>
		<skos:narrower rdf:resource="http://purl.org/heritagedata/schemes/eh_tbm/concepts/97803" />
		<skos:narrower rdf:resource="http://purl.org/heritagedata/schemes/eh_tbm/concepts/97919" />
		<skos:narrower>
			<skos:Concept rdf:about="http://purl.org/heritagedata/schemes/eh_tbm/concepts/97957">
				<skos:inScheme rdf:resource="http://purl.org/heritagedata/schemes/eh_tbm" />
				<dcterms:identifier>http://purl.org/heritagedata/schemes/eh_tbm/concepts/97957</dcterms:identifier>
				<skos:prefLabel xml:lang="en">GRITSTONE (SANDSTONE)</skos:prefLabel>
				<dcterms:issued rdf:datatype="http://www.w3.org/2001/XMLSchema#dateTime">2013-07-17T09:02:16</dcterms:issued>
				<skos:altLabel xml:lang="en">Matlock Stone</skos:altLabel>
				<skos:altLabel xml:lang="en">Millstone Grit</skos:altLabel>
				<skos:altLabel xml:lang="en">Revidge Grit</skos:altLabel>
				<skos:altLabel xml:lang="en">Stancliffe Stone</skos:altLabel>
				<skos:altLabel xml:lang="en">Watts Cliff Stone</skos:altLabel>
				<skos:altLabel xml:lang="en">Wattscliffe Stone</skos:altLabel>
				<skos:altLabel xml:lang="en">Whatstandwell Stone</skos:altLabel>
				<skos:altLabel xml:lang="en">Birchover Stone</skos:altLabel>
				<skos:altLabel xml:lang="en">Birshover Gritstone</skos:altLabel>
				<skos:altLabel xml:lang="en">Chinley Moor Stone</skos:altLabel>
				<skos:altLabel xml:lang="en">Darley Dale Stone</skos:altLabel>
				<skos:altLabel xml:lang="en">Derbyshire Grit Stone</skos:altLabel>
				<skos:altLabel xml:lang="en">Hall Dale Stone</skos:altLabel>
				<skos:broader rdf:resource="http://purl.org/heritagedata/schemes/eh_tbm/concepts/98171" />
				<skos:scopeNote xml:lang="en">Carboniferous sandstone varying in grain size from coarse to fine and in colour from white, yellow, pink to brown. When only Gritstone is mentioned, unless otherwise specified, assume it to be Gritstone (Sandstone), as this is the more common usage.</skos:scopeNote>
				<cc:license rdf:resource="http://creativecommons.org/licenses/by/3.0" />
				<cc:attributionURL rdf:resource="http://www.english-heritage.org.uk" />
				<cc:attributionName xml:lang="en">English Heritage</cc:attributionName>
				<dcterms:publisher rdf:resource="http://www.english-heritage.org.uk" />
			</skos:Concept>
		</skos:narrower>
		<skos:narrower rdf:resource="http://purl.org/heritagedata/schemes/eh_tbm/concepts/98040" />
		<skos:narrower>
			<skos:Concept rdf:about="http://purl.org/heritagedata/schemes/eh_tbm/concepts/98093">
				<skos:inScheme rdf:resource="http://purl.org/heritagedata/schemes/eh_tbm" />
				<dcterms:identifier>http://purl.org/heritagedata/schemes/eh_tbm/concepts/98093</dcterms:identifier>
				<skos:prefLabel xml:lang="en">PENNANT STONE</skos:prefLabel>
				<dcterms:issued rdf:datatype="http://www.w3.org/2001/XMLSchema#dateTime">2013-07-17T09:02:16</dcterms:issued>
				<skos:broader rdf:resource="http://purl.org/heritagedata/schemes/eh_tbm/concepts/98171" />
				<skos:scopeNote xml:lang="en">Hard, fine grained, blue/grey coloured sandstone. Quarried in South Wales and the Bristol area and commonly used, throughout the country, as a stone roofing material (stone slate).</skos:scopeNote>
				<cc:license rdf:resource="http://creativecommons.org/licenses/by/3.0" />
				<cc:attributionURL rdf:resource="http://www.english-heritage.org.uk" />
				<cc:attributionName xml:lang="en">English Heritage</cc:attributionName>
				<dcterms:publisher rdf:resource="http://www.english-heritage.org.uk" />
			</skos:Concept>
		</skos:narrower>
		<skos:narrower rdf:resource="http://purl.org/heritagedata/schemes/eh_tbm/concepts/98144" />
		<skos:broader rdf:resource="http://purl.org/heritagedata/schemes/eh_tbm/concepts/98216" />
		<skos:narrower rdf:resource="http://purl.org/heritagedata/schemes/eh_tbm/concepts/98173" />
		<skos:narrower rdf:resource="http://purl.org/heritagedata/schemes/eh_tbm/concepts/98223" />
		<skos:narrower>
			<skos:Concept rdf:about="http://purl.org/heritagedata/schemes/eh_tbm/concepts/98307">
				<skos:inScheme rdf:resource="http://purl.org/heritagedata/schemes/eh_tbm" />
				<dcterms:identifier>http://purl.org/heritagedata/schemes/eh_tbm/concepts/98307</dcterms:identifier>
				<skos:prefLabel xml:lang="en">YORK STONE</skos:prefLabel>
				<dcterms:issued rdf:datatype="http://www.w3.org/2001/XMLSchema#dateTime">2013-07-17T09:02:16</dcterms:issued>
				<skos:altLabel xml:lang="en">Woodkirk Stone</skos:altLabel>
				<skos:altLabel xml:lang="en">Yorkshire Flagstone</skos:altLabel>
				<skos:altLabel xml:lang="en">Yorkshire Stone</skos:altLabel>
				<skos:altLabel xml:lang="en">Bolton Wood Stone</skos:altLabel>
				<skos:altLabel xml:lang="en">Crosland Hill Stone</skos:altLabel>
				<skos:altLabel xml:lang="en">Elland Edge Flagrock</skos:altLabel>
				<skos:altLabel xml:lang="en">Elland Edge Stone</skos:altLabel>
				<skos:altLabel xml:lang="en">Greenmoor Stone</skos:altLabel>
				<skos:altLabel xml:lang="en">Hard Rock</skos:altLabel>
				<skos:altLabel xml:lang="en">Hard York</skos:altLabel>
				<skos:altLabel xml:lang="en">Hard York Freestone</skos:altLabel>
				<skos:broader rdf:resource="http://purl.org/heritagedata/schemes/eh_tbm/concepts/98171" />
				<skos:scopeNote xml:lang="en">Generic name for the fine grained, brown coloured carboniferous sandstone, quarried in the Leeds, Bradford and Halifax area.</skos:scopeNote>
				<cc:license rdf:resource="http://creativecommons.org/licenses/by/3.0" />
				<cc:attributionURL rdf:resource="http://www.english-heritage.org.uk" />
				<cc:attributionName xml:lang="en">English Heritage</cc:attributionName>
				<dcterms:publisher rdf:resource="http://www.english-heritage.org.uk" />
			</skos:Concept>
		</skos:narrower>
		<skos:related rdf:resource="http://purl.org/heritagedata/schemes/eh_tbm/concepts/97800" />
		<skos:related rdf:resource="http://purl.org/heritagedata/schemes/eh_tbm/concepts/97993" />
		<skos:related rdf:resource="http://purl.org/heritagedata/schemes/eh_tbm/concepts/98024" />
		<skos:related rdf:resource="http://purl.org/heritagedata/schemes/eh_tbm/concepts/98183" />
		<skos:scopeNote xml:lang="en">Geologically sandstone consists of particles of quartz naturally cemented together by either silica, calcium or iron. It is this geological composition that accounts for the varying colours and grain sizes found in the many building sandstones.</skos:scopeNote>
		<cc:license rdf:resource="http://creativecommons.org/licenses/by/3.0" />
		<cc:attributionURL rdf:resource="http://www.english-heritage.org.uk" />
		<cc:attributionName xml:lang="en">English Heritage</cc:attributionName>
		<dcterms:publisher rdf:resource="http://www.english-heritage.org.uk" />
	</skos:Concept>
	<skos:Concept rdf:about="http://purl.org/heritagedata/schemes/eh_tbm/concepts/98173">
		<skos:inScheme rdf:resource="http://purl.org/heritagedata/schemes/eh_tbm" />
		<dcterms:identifier>http://purl.org/heritagedata/schemes/eh_tbm/concepts/98173</dcterms:identifier>
		<skos:prefLabel xml:lang="en">SARSEN STONE</skos:prefLabel>
		<dcterms:issued rdf:datatype="http://www.w3.org/2001/XMLSchema#dateTime">2013-07-17T09:02:16</dcterms:issued>
		<skos:altLabel xml:lang="en">Greyweathers</skos:altLabel>
		<skos:altLabel xml:lang="en">Heathstone</skos:altLabel>
		<skos:broader rdf:resource="http://purl.org/heritagedata/schemes/eh_tbm/concepts/98171" />
		<skos:related rdf:resource="http://purl.org/heritagedata/schemes/eh_tbm/concepts/98061" />
		<skos:scopeNote xml:lang="en">Extremely hard, fine grained, grey to brown silica rich sandstone. It is often found on the surface of the South Downs and has been used, as found, since prehistoric times.</skos:scopeNote>
		<cc:license rdf:resource="http://creativecommons.org/licenses/by/3.0" />
		<cc:attributionURL rdf:resource="http://www.english-heritage.org.uk" />
		<cc:attributionName xml:lang="en">English Heritage</cc:attributionName>
		<dcterms:publisher rdf:resource="http://www.english-heritage.org.uk" />
	</skos:Concept>
	<skos:Concept rdf:about="http://purl.org/heritagedata/schemes/eh_tbm/concepts/98174">
		<skos:inScheme rdf:resource="http://purl.org/heritagedata/schemes/eh_tbm" />
		<dcterms:identifier>http://purl.org/heritagedata/schemes/eh_tbm/concepts/98174</dcterms:identifier>
		<skos:prefLabel xml:lang="en">SCAGLIOLA</skos:prefLabel>
		<dcterms:issued rdf:datatype="http://www.w3.org/2001/XMLSchema#dateTime">2013-07-17T09:02:16</dcterms:issued>
		<skos:altLabel xml:lang="en">Stucco Lustro</skos:altLabel>
		<skos:broader rdf:resource="http://purl.org/heritagedata/schemes/eh_tbm/concepts/97876" />
		<skos:related rdf:resource="http://purl.org/heritagedata/schemes/eh_tbm/concepts/97717" />
		<skos:related rdf:resource="http://purl.org/heritagedata/schemes/eh_tbm/concepts/98044" />
		<skos:scopeNote xml:lang="en">Composite substance of plaster formed by gypsum, sand and lime and coloured with pigments, fixed under heat and highly polished. Used to imitate marble and popular in the 17th and 18th centuries for architectural features.</skos:scopeNote>
		<cc:license rdf:resource="http://creativecommons.org/licenses/by/3.0" />
		<cc:attributionURL rdf:resource="http://www.english-heritage.org.uk" />
		<cc:attributionName xml:lang="en">English Heritage</cc:attributionName>
		<dcterms:publisher rdf:resource="http://www.english-heritage.org.uk" />
	</skos:Concept>
	<skos:Concept rdf:about="http://purl.org/heritagedata/schemes/eh_tbm/concepts/98179">
		<skos:inScheme rdf:resource="http://purl.org/heritagedata/schemes/eh_tbm" />
		<dcterms:identifier>http://purl.org/heritagedata/schemes/eh_tbm/concepts/98179</dcterms:identifier>
		<skos:prefLabel xml:lang="en">SCOTTISH SLATE</skos:prefLabel>
		<dcterms:issued rdf:datatype="http://www.w3.org/2001/XMLSchema#dateTime">2013-07-17T09:02:16</dcterms:issued>
		<skos:altLabel xml:lang="en">Scotch Slate</skos:altLabel>
		<skos:altLabel xml:lang="en">Ballachulish Slate</skos:altLabel>
		<skos:broader rdf:resource="http://purl.org/heritagedata/schemes/eh_tbm/concepts/98194" />
		<skos:related rdf:resource="http://purl.org/heritagedata/schemes/eh_tbm/concepts/97928" />
		<skos:scopeNote xml:lang="en">Collective term for the Scottish Slates including the Aberdeen/Baniff and Ballachulish/Easdale groups. Fine grained, varying in colour from brown to dark grey/blue. Geologically different from Lake District, Welsh and West Country groups of slate.</skos:scopeNote>
		<cc:license rdf:resource="http://creativecommons.org/licenses/by/3.0" />
		<cc:attributionURL rdf:resource="http://www.english-heritage.org.uk" />
		<cc:attributionName xml:lang="en">English Heritage</cc:attributionName>
		<dcterms:publisher rdf:resource="http://www.english-heritage.org.uk" />
	</skos:Concept>
	<skos:Concept rdf:about="http://purl.org/heritagedata/schemes/eh_tbm/concepts/98180">
		<skos:inScheme rdf:resource="http://purl.org/heritagedata/schemes/eh_tbm" />
		<dcterms:identifier>http://purl.org/heritagedata/schemes/eh_tbm/concepts/98180</dcterms:identifier>
		<skos:prefLabel xml:lang="en">SEPTARIA</skos:prefLabel>
		<dcterms:issued rdf:datatype="http://www.w3.org/2001/XMLSchema#dateTime">2013-07-17T09:02:16</dcterms:issued>
		<skos:broader rdf:resource="http://purl.org/heritagedata/schemes/eh_tbm/concepts/97843" />
		<skos:related rdf:resource="http://purl.org/heritagedata/schemes/eh_tbm/concepts/98045" />
		<skos:related rdf:resource="http://purl.org/heritagedata/schemes/eh_tbm/concepts/98156" />
		<skos:scopeNote xml:lang="en">Conglomerate consisting of nodules of calcium rich clay (marl). Used as a building stone from Roman times and as a key ingredient in Parker's Roman Cement, between 1796 and circa 1850.</skos:scopeNote>
		<cc:license rdf:resource="http://creativecommons.org/licenses/by/3.0" />
		<cc:attributionURL rdf:resource="http://www.english-heritage.org.uk" />
		<cc:attributionName xml:lang="en">English Heritage</cc:attributionName>
		<dcterms:publisher rdf:resource="http://www.english-heritage.org.uk" />
	</skos:Concept>
	<skos:Concept rdf:about="http://purl.org/heritagedata/schemes/eh_tbm/concepts/98181">
		<skos:inScheme rdf:resource="http://purl.org/heritagedata/schemes/eh_tbm" />
		<dcterms:identifier>http://purl.org/heritagedata/schemes/eh_tbm/concepts/98181</dcterms:identifier>
		<skos:prefLabel xml:lang="en">SERPENTINE</skos:prefLabel>
		<dcterms:issued rdf:datatype="http://www.w3.org/2001/XMLSchema#dateTime">2013-07-17T09:02:16</dcterms:issued>
		<skos:altLabel xml:lang="en">Serpentinite</skos:altLabel>
		<skos:altLabel xml:lang="en">Tinos</skos:altLabel>
		<skos:altLabel xml:lang="en">Verde Antico</skos:altLabel>
		<skos:broader rdf:resource="http://purl.org/heritagedata/schemes/eh_tbm/concepts/98216" />
		<skos:related rdf:resource="http://purl.org/heritagedata/schemes/eh_tbm/concepts/97734" />
		<skos:related rdf:resource="http://purl.org/heritagedata/schemes/eh_tbm/concepts/97844" />
		<skos:related rdf:resource="http://purl.org/heritagedata/schemes/eh_tbm/concepts/98118" />
		<skos:related rdf:resource="http://purl.org/heritagedata/schemes/eh_tbm/concepts/98150" />
		<skos:related rdf:resource="http://purl.org/heritagedata/schemes/eh_tbm/concepts/98229" />
		<skos:scopeNote xml:lang="en">Medium to coarse grained, green to dark red/black coloured igneous rock, mainly found on The Lizard, South West Cornwall. Due to its fragmentary structure, Serpentine is mainly used for decorative and ornamental purposes.</skos:scopeNote>
		<cc:license rdf:resource="http://creativecommons.org/licenses/by/3.0" />
		<cc:attributionURL rdf:resource="http://www.english-heritage.org.uk" />
		<cc:attributionName xml:lang="en">English Heritage</cc:attributionName>
		<dcterms:publisher rdf:resource="http://www.english-heritage.org.uk" />
	</skos:Concept>
	<skos:Concept rdf:about="http://purl.org/heritagedata/schemes/eh_tbm/concepts/98183">
		<skos:inScheme rdf:resource="http://purl.org/heritagedata/schemes/eh_tbm" />
		<dcterms:identifier>http://purl.org/heritagedata/schemes/eh_tbm/concepts/98183</dcterms:identifier>
		<skos:prefLabel xml:lang="en">SHALE</skos:prefLabel>
		<dcterms:issued rdf:datatype="http://www.w3.org/2001/XMLSchema#dateTime">2013-07-17T09:02:16</dcterms:issued>
		<skos:altLabel xml:lang="en">Mudstone</skos:altLabel>
		<skos:broader rdf:resource="http://purl.org/heritagedata/schemes/eh_tbm/concepts/98216" />
		<skos:related rdf:resource="http://purl.org/heritagedata/schemes/eh_tbm/concepts/97800" />
		<skos:related rdf:resource="http://purl.org/heritagedata/schemes/eh_tbm/concepts/98013" />
		<skos:related rdf:resource="http://purl.org/heritagedata/schemes/eh_tbm/concepts/98028" />
		<skos:related rdf:resource="http://purl.org/heritagedata/schemes/eh_tbm/concepts/98171" />
		<skos:related rdf:resource="http://purl.org/heritagedata/schemes/eh_tbm/concepts/98188" />
		<skos:related rdf:resource="http://purl.org/heritagedata/schemes/eh_tbm/concepts/98194" />
		<skos:related rdf:resource="http://purl.org/heritagedata/schemes/eh_tbm/concepts/98286" />
		<skos:related rdf:resource="http://purl.org/heritagedata/schemes/eh_tbm/concepts/98287" />
		<skos:scopeNote xml:lang="en">Soft, very fine grained, dark coloured, sedimentary rock which splits easily.</skos:scopeNote>
		<cc:license rdf:resource="http://creativecommons.org/licenses/by/3.0" />
		<cc:attributionURL rdf:resource="http://www.english-heritage.org.uk" />
		<cc:attributionName xml:lang="en">English Heritage</cc:attributionName>
		<dcterms:publisher rdf:resource="http://www.english-heritage.org.uk" />
	</skos:Concept>
	<skos:Concept rdf:about="http://purl.org/heritagedata/schemes/eh_tbm/concepts/98186">
		<skos:inScheme rdf:resource="http://purl.org/heritagedata/schemes/eh_tbm" />
		<dcterms:identifier>http://purl.org/heritagedata/schemes/eh_tbm/concepts/98186</dcterms:identifier>
		<skos:prefLabel xml:lang="en">SHINGLE</skos:prefLabel>
		<dcterms:issued rdf:datatype="http://www.w3.org/2001/XMLSchema#dateTime">2013-07-17T09:02:16</dcterms:issued>
		<skos:broader rdf:resource="http://purl.org/heritagedata/schemes/eh_tbm/concepts/98242" />
		<skos:broader rdf:resource="http://purl.org/heritagedata/schemes/eh_tbm/concepts/98241" />
		<skos:scopeNote xml:lang="en">Wooden roof tile (traditionally oak) which is riven or sawn from good quality timber to a regular size and used as a roof and/or wall covering. Index with type of wood if known.</skos:scopeNote>
		<cc:license rdf:resource="http://creativecommons.org/licenses/by/3.0" />
		<cc:attributionURL rdf:resource="http://www.english-heritage.org.uk" />
		<cc:attributionName xml:lang="en">English Heritage</cc:attributionName>
		<dcterms:publisher rdf:resource="http://www.english-heritage.org.uk" />
	</skos:Concept>
	<skos:Concept rdf:about="http://purl.org/heritagedata/schemes/eh_tbm/concepts/98188">
		<skos:inScheme rdf:resource="http://purl.org/heritagedata/schemes/eh_tbm" />
		<dcterms:identifier>http://purl.org/heritagedata/schemes/eh_tbm/concepts/98188</dcterms:identifier>
		<skos:prefLabel xml:lang="en">SILTSTONE</skos:prefLabel>
		<dcterms:issued rdf:datatype="http://www.w3.org/2001/XMLSchema#dateTime">2013-07-17T09:02:16</dcterms:issued>
		<skos:broader rdf:resource="http://purl.org/heritagedata/schemes/eh_tbm/concepts/98216" />
		<skos:related rdf:resource="http://purl.org/heritagedata/schemes/eh_tbm/concepts/98183" />
		<skos:scopeNote xml:lang="en">Fine grained, yellow/buff to grey/black coloured sedimentary rock.</skos:scopeNote>
		<cc:license rdf:resource="http://creativecommons.org/licenses/by/3.0" />
		<cc:attributionURL rdf:resource="http://www.english-heritage.org.uk" />
		<cc:attributionName xml:lang="en">English Heritage</cc:attributionName>
		<dcterms:publisher rdf:resource="http://www.english-heritage.org.uk" />
	</skos:Concept>
	<skos:Concept rdf:about="http://purl.org/heritagedata/schemes/eh_tbm/concepts/98194">
		<skos:inScheme rdf:resource="http://purl.org/heritagedata/schemes/eh_tbm" />
		<dcterms:identifier>http://purl.org/heritagedata/schemes/eh_tbm/concepts/98194</dcterms:identifier>
		<skos:prefLabel xml:lang="en">SLATE</skos:prefLabel>
		<dcterms:issued rdf:datatype="http://www.w3.org/2001/XMLSchema#dateTime">2013-07-17T09:02:16</dcterms:issued>
		<skos:altLabel xml:lang="en">Rag Slate</skos:altLabel>
		<skos:altLabel xml:lang="en">Longford Rustic Slate</skos:altLabel>
		<skos:altLabel xml:lang="en">Riven Slate</skos:altLabel>
		<skos:altLabel xml:lang="en">Swithland Slate</skos:altLabel>
		<skos:narrower>
			<skos:Concept rdf:about="http://purl.org/heritagedata/schemes/eh_tbm/concepts/98007">
				<skos:inScheme rdf:resource="http://purl.org/heritagedata/schemes/eh_tbm" />
				<dcterms:identifier>http://purl.org/heritagedata/schemes/eh_tbm/concepts/98007</dcterms:identifier>
				<skos:prefLabel xml:lang="en">KILLAS</skos:prefLabel>
				<dcterms:issued rdf:datatype="http://www.w3.org/2001/XMLSchema#dateTime">2013-07-17T09:02:16</dcterms:issued>
				<skos:broader rdf:resource="http://purl.org/heritagedata/schemes/eh_tbm/concepts/98194" />
				<skos:scopeNote xml:lang="en">Cornish miner's term for slates formed during the Carboniferous and Devonian periods.</skos:scopeNote>
				<cc:license rdf:resource="http://creativecommons.org/licenses/by/3.0" />
				<cc:attributionURL rdf:resource="http://www.english-heritage.org.uk" />
				<cc:attributionName xml:lang="en">English Heritage</cc:attributionName>
				<dcterms:publisher rdf:resource="http://www.english-heritage.org.uk" />
			</skos:Concept>
		</skos:narrower>
		<skos:narrower rdf:resource="http://purl.org/heritagedata/schemes/eh_tbm/concepts/98013" />
		<skos:narrower rdf:resource="http://purl.org/heritagedata/schemes/eh_tbm/concepts/98179" />
		<skos:broader rdf:resource="http://purl.org/heritagedata/schemes/eh_tbm/concepts/98216" />
		<skos:narrower rdf:resource="http://purl.org/heritagedata/schemes/eh_tbm/concepts/98286" />
		<skos:narrower rdf:resource="http://purl.org/heritagedata/schemes/eh_tbm/concepts/98287" />
		<skos:related rdf:resource="http://purl.org/heritagedata/schemes/eh_tbm/concepts/97928" />
		<skos:related rdf:resource="http://purl.org/heritagedata/schemes/eh_tbm/concepts/98183" />
		<skos:scopeNote xml:lang="en">Collective term for a hard, fine grained, dark coloured metamorphic rock, which splits easily; hence its common use as a roofing and flooring material, and a functional description for any rectangular, sheet, roofing material.</skos:scopeNote>
		<cc:license rdf:resource="http://creativecommons.org/licenses/by/3.0" />
		<cc:attributionURL rdf:resource="http://www.english-heritage.org.uk" />
		<cc:attributionName xml:lang="en">English Heritage</cc:attributionName>
		<dcterms:publisher rdf:resource="http://www.english-heritage.org.uk" />
	</skos:Concept>
	<skos:Concept rdf:about="http://purl.org/heritagedata/schemes/eh_tbm/concepts/98195">
		<skos:inScheme rdf:resource="http://purl.org/heritagedata/schemes/eh_tbm" />
		<dcterms:identifier>http://purl.org/heritagedata/schemes/eh_tbm/concepts/98195</dcterms:identifier>
		<skos:prefLabel xml:lang="en">SLURRY</skos:prefLabel>
		<dcterms:issued rdf:datatype="http://www.w3.org/2001/XMLSchema#dateTime">2013-07-17T09:02:16</dcterms:issued>
		<skos:broader rdf:resource="http://purl.org/heritagedata/schemes/eh_tbm/concepts/97810" />
		<skos:related rdf:resource="http://purl.org/heritagedata/schemes/eh_tbm/concepts/97809" />
		<skos:scopeNote xml:lang="en">Cement/water mix often used as covering. Use this for entries including slurrying and slurried.</skos:scopeNote>
		<cc:license rdf:resource="http://creativecommons.org/licenses/by/3.0" />
		<cc:attributionURL rdf:resource="http://www.english-heritage.org.uk" />
		<cc:attributionName xml:lang="en">English Heritage</cc:attributionName>
		<dcterms:publisher rdf:resource="http://www.english-heritage.org.uk" />
	</skos:Concept>
	<skos:Concept rdf:about="http://purl.org/heritagedata/schemes/eh_tbm/concepts/98213">
		<skos:inScheme rdf:resource="http://purl.org/heritagedata/schemes/eh_tbm" />
		<dcterms:identifier>http://purl.org/heritagedata/schemes/eh_tbm/concepts/98213</dcterms:identifier>
		<skos:prefLabel xml:lang="en">STEEL</skos:prefLabel>
		<dcterms:issued rdf:datatype="http://www.w3.org/2001/XMLSchema#dateTime">2013-07-17T09:02:16</dcterms:issued>
		<skos:altLabel xml:lang="en">Stainless Steel</skos:altLabel>
		<skos:narrower>
			<skos:Concept rdf:about="http://purl.org/heritagedata/schemes/eh_tbm/concepts/102712">
				<skos:inScheme rdf:resource="http://purl.org/heritagedata/schemes/eh_tbm" />
				<dcterms:identifier>http://purl.org/heritagedata/schemes/eh_tbm/concepts/102712</dcterms:identifier>
				<skos:prefLabel xml:lang="en">GALVANIZED STEEL</skos:prefLabel>
				<dcterms:issued rdf:datatype="http://www.w3.org/2001/XMLSchema#dateTime">2013-07-17T09:02:16</dcterms:issued>
				<skos:altLabel xml:lang="en">Galvanised Steel</skos:altLabel>
				<skos:broader rdf:resource="http://purl.org/heritagedata/schemes/eh_tbm/concepts/98213" />
				<skos:scopeNote xml:lang="en">Steel coated in zinc, giving good protection against weathering.</skos:scopeNote>
				<cc:license rdf:resource="http://creativecommons.org/licenses/by/3.0" />
				<cc:attributionURL rdf:resource="http://www.english-heritage.org.uk" />
				<cc:attributionName xml:lang="en">English Heritage</cc:attributionName>
				<dcterms:publisher rdf:resource="http://www.english-heritage.org.uk" />
			</skos:Concept>
		</skos:narrower>
		<skos:narrower>
			<skos:Concept rdf:about="http://purl.org/heritagedata/schemes/eh_tbm/concepts/97977">
				<skos:inScheme rdf:resource="http://purl.org/heritagedata/schemes/eh_tbm" />
				<dcterms:identifier>http://purl.org/heritagedata/schemes/eh_tbm/concepts/97977</dcterms:identifier>
				<skos:prefLabel xml:lang="en">HIGH TENSILE STEEL</skos:prefLabel>
				<dcterms:issued rdf:datatype="http://www.w3.org/2001/XMLSchema#dateTime">2013-07-17T09:02:16</dcterms:issued>
				<skos:broader rdf:resource="http://purl.org/heritagedata/schemes/eh_tbm/concepts/98213" />
				<skos:scopeNote xml:lang="en">A strong alloy of steel.</skos:scopeNote>
				<cc:license rdf:resource="http://creativecommons.org/licenses/by/3.0" />
				<cc:attributionURL rdf:resource="http://www.english-heritage.org.uk" />
				<cc:attributionName xml:lang="en">English Heritage</cc:attributionName>
				<dcterms:publisher rdf:resource="http://www.english-heritage.org.uk" />
			</skos:Concept>
		</skos:narrower>
		<skos:broader rdf:resource="http://purl.org/heritagedata/schemes/eh_tbm/concepts/98053" />
		<skos:narrower>
			<skos:Concept rdf:about="http://purl.org/heritagedata/schemes/eh_tbm/concepts/98283">
				<skos:inScheme rdf:resource="http://purl.org/heritagedata/schemes/eh_tbm" />
				<dcterms:identifier>http://purl.org/heritagedata/schemes/eh_tbm/concepts/98283</dcterms:identifier>
				<skos:prefLabel xml:lang="en">WEATHERING STEEL</skos:prefLabel>
				<dcterms:issued rdf:datatype="http://www.w3.org/2001/XMLSchema#dateTime">2013-07-17T09:02:16</dcterms:issued>
				<skos:altLabel xml:lang="en">Cor Ten Steel</skos:altLabel>
				<skos:broader rdf:resource="http://purl.org/heritagedata/schemes/eh_tbm/concepts/98213" />
				<skos:scopeNote xml:lang="en">An alloy of steel.</skos:scopeNote>
				<cc:license rdf:resource="http://creativecommons.org/licenses/by/3.0" />
				<cc:attributionURL rdf:resource="http://www.english-heritage.org.uk" />
				<cc:attributionName xml:lang="en">English Heritage</cc:attributionName>
				<dcterms:publisher rdf:resource="http://www.english-heritage.org.uk" />
			</skos:Concept>
		</skos:narrower>
		<skos:related rdf:resource="http://purl.org/heritagedata/schemes/eh_tbm/concepts/98145" />
		<skos:scopeNote xml:lang="en">An alloy of iron and carbon, its strength makes it suitable for load bearing purposes. It is primarily used in structural steelwork and concrete reinforcement.</skos:scopeNote>
		<cc:license rdf:resource="http://creativecommons.org/licenses/by/3.0" />
		<cc:attributionURL rdf:resource="http://www.english-heritage.org.uk" />
		<cc:attributionName xml:lang="en">English Heritage</cc:attributionName>
		<dcterms:publisher rdf:resource="http://www.english-heritage.org.uk" />
	</skos:Concept>
	<skos:Concept rdf:about="http://purl.org/heritagedata/schemes/eh_tbm/concepts/98219">
		<skos:inScheme rdf:resource="http://purl.org/heritagedata/schemes/eh_tbm" />
		<dcterms:identifier>http://purl.org/heritagedata/schemes/eh_tbm/concepts/98219</dcterms:identifier>
		<skos:prefLabel xml:lang="en">STRAW</skos:prefLabel>
		<dcterms:issued rdf:datatype="http://www.w3.org/2001/XMLSchema#dateTime">2013-07-17T09:02:16</dcterms:issued>
		<skos:narrower>
			<skos:Concept rdf:about="http://purl.org/heritagedata/schemes/eh_tbm/concepts/139757">
				<skos:inScheme rdf:resource="http://purl.org/heritagedata/schemes/eh_tbm" />
				<dcterms:identifier>http://purl.org/heritagedata/schemes/eh_tbm/concepts/139757</dcterms:identifier>
				<skos:prefLabel xml:lang="en">COMBED WHEAT REED</skos:prefLabel>
				<dcterms:issued rdf:datatype="http://www.w3.org/2001/XMLSchema#dateTime">2013-07-17T09:02:16</dcterms:issued>
				<skos:broader rdf:resource="http://purl.org/heritagedata/schemes/eh_tbm/concepts/98219" />
				<skos:scopeNote xml:lang="en">A form of thatching straw composed of stems that have been combed mechanically to remove grain and extraneous waste material without crushing the stem.</skos:scopeNote>
				<cc:license rdf:resource="http://creativecommons.org/licenses/by/3.0" />
				<cc:attributionURL rdf:resource="http://www.english-heritage.org.uk" />
				<cc:attributionName xml:lang="en">English Heritage</cc:attributionName>
				<dcterms:publisher rdf:resource="http://www.english-heritage.org.uk" />
			</skos:Concept>
		</skos:narrower>
		<skos:narrower rdf:resource="http://purl.org/heritagedata/schemes/eh_tbm/concepts/98031" />
		<skos:broader rdf:resource="http://purl.org/heritagedata/schemes/eh_tbm/concepts/98109" />
		<skos:related rdf:resource="http://purl.org/heritagedata/schemes/eh_tbm/concepts/98239" />
		<skos:scopeNote xml:lang="en">Roofing material consisting of stems or stalks of wheat, rye, oats or barley separated from grain and laid flat in 'yealms' which form an overlapping surface which sheds water.</skos:scopeNote>
		<cc:license rdf:resource="http://creativecommons.org/licenses/by/3.0" />
		<cc:attributionURL rdf:resource="http://www.english-heritage.org.uk" />
		<cc:attributionName xml:lang="en">English Heritage</cc:attributionName>
		<dcterms:publisher rdf:resource="http://www.english-heritage.org.uk" />
	</skos:Concept>
	<skos:Concept rdf:about="http://purl.org/heritagedata/schemes/eh_tbm/concepts/98223">
		<skos:inScheme rdf:resource="http://purl.org/heritagedata/schemes/eh_tbm" />
		<dcterms:identifier>http://purl.org/heritagedata/schemes/eh_tbm/concepts/98223</dcterms:identifier>
		<skos:prefLabel xml:lang="en">SUSSEX STONE</skos:prefLabel>
		<dcterms:issued rdf:datatype="http://www.w3.org/2001/XMLSchema#dateTime">2013-07-17T09:02:16</dcterms:issued>
		<skos:altLabel xml:lang="en">Pulborough Stone</skos:altLabel>
		<skos:altLabel xml:lang="en">Midhurst Stone</skos:altLabel>
		<skos:altLabel xml:lang="en">Tunbridge Wells Stone</skos:altLabel>
		<skos:altLabel xml:lang="en">Bognor Rock</skos:altLabel>
		<skos:altLabel xml:lang="en">Calverley Stone</skos:altLabel>
		<skos:narrower>
			<skos:Concept rdf:about="http://purl.org/heritagedata/schemes/eh_tbm/concepts/97984">
				<skos:inScheme rdf:resource="http://purl.org/heritagedata/schemes/eh_tbm" />
				<dcterms:identifier>http://purl.org/heritagedata/schemes/eh_tbm/concepts/97984</dcterms:identifier>
				<skos:prefLabel xml:lang="en">HORSHAM STONE</skos:prefLabel>
				<dcterms:issued rdf:datatype="http://www.w3.org/2001/XMLSchema#dateTime">2013-07-17T09:02:16</dcterms:issued>
				<skos:altLabel xml:lang="en">Horsham Slab</skos:altLabel>
				<skos:broader rdf:resource="http://purl.org/heritagedata/schemes/eh_tbm/concepts/98223" />
				<skos:scopeNote xml:lang="en">Hard, fissile sandstone which weathers to a dark brown colour. Mainly used as a stone roofing material (stone slate) throughout Sussex and Surrey.</skos:scopeNote>
				<cc:license rdf:resource="http://creativecommons.org/licenses/by/3.0" />
				<cc:attributionURL rdf:resource="http://www.english-heritage.org.uk" />
				<cc:attributionName xml:lang="en">English Heritage</cc:attributionName>
				<dcterms:publisher rdf:resource="http://www.english-heritage.org.uk" />
			</skos:Concept>
		</skos:narrower>
		<skos:broader rdf:resource="http://purl.org/heritagedata/schemes/eh_tbm/concepts/98171" />
		<skos:narrower>
			<skos:Concept rdf:about="http://purl.org/heritagedata/schemes/eh_tbm/concepts/98280">
				<skos:inScheme rdf:resource="http://purl.org/heritagedata/schemes/eh_tbm" />
				<dcterms:identifier>http://purl.org/heritagedata/schemes/eh_tbm/concepts/98280</dcterms:identifier>
				<skos:prefLabel xml:lang="en">WEALDEN STONE</skos:prefLabel>
				<dcterms:issued rdf:datatype="http://www.w3.org/2001/XMLSchema#dateTime">2013-07-17T09:02:16</dcterms:issued>
				<skos:altLabel xml:lang="en">Weald Stone</skos:altLabel>
				<skos:broader rdf:resource="http://purl.org/heritagedata/schemes/eh_tbm/concepts/98223" />
				<skos:scopeNote xml:lang="en">Fine grained, brown/yellow to dark grey coloured cretaceous sandstone. It is a particularly good freestone and was often used for ashlar finishes.</skos:scopeNote>
				<cc:license rdf:resource="http://creativecommons.org/licenses/by/3.0" />
				<cc:attributionURL rdf:resource="http://www.english-heritage.org.uk" />
				<cc:attributionName xml:lang="en">English Heritage</cc:attributionName>
				<dcterms:publisher rdf:resource="http://www.english-heritage.org.uk" />
			</skos:Concept>
		</skos:narrower>
		<skos:related rdf:resource="http://purl.org/heritagedata/schemes/eh_tbm/concepts/97866" />
		<skos:scopeNote xml:lang="en">Fine grained, buff, brown to green coloured Cretaceous sandstone. Quarried at various locations in Sussex. Not to be confused with Sussex marble which is a cretaceous limestone.</skos:scopeNote>
		<cc:license rdf:resource="http://creativecommons.org/licenses/by/3.0" />
		<cc:attributionURL rdf:resource="http://www.english-heritage.org.uk" />
		<cc:attributionName xml:lang="en">English Heritage</cc:attributionName>
		<dcterms:publisher rdf:resource="http://www.english-heritage.org.uk" />
	</skos:Concept>
	<skos:Concept rdf:about="http://purl.org/heritagedata/schemes/eh_tbm/concepts/98229">
		<skos:inScheme rdf:resource="http://purl.org/heritagedata/schemes/eh_tbm" />
		<dcterms:identifier>http://purl.org/heritagedata/schemes/eh_tbm/concepts/98229</dcterms:identifier>
		<skos:prefLabel xml:lang="en">SYENITE</skos:prefLabel>
		<dcterms:issued rdf:datatype="http://www.w3.org/2001/XMLSchema#dateTime">2013-07-17T09:02:16</dcterms:issued>
		<skos:altLabel xml:lang="en">Swedish Green Granite</skos:altLabel>
		<skos:broader rdf:resource="http://purl.org/heritagedata/schemes/eh_tbm/concepts/98216" />
		<skos:related rdf:resource="http://purl.org/heritagedata/schemes/eh_tbm/concepts/97928" />
		<skos:related rdf:resource="http://purl.org/heritagedata/schemes/eh_tbm/concepts/98150" />
		<skos:related rdf:resource="http://purl.org/heritagedata/schemes/eh_tbm/concepts/98181" />
		<skos:scopeNote xml:lang="en">Hard, coarse grained, green to pink coloured igneous rock. Commonly used as a polished cladding.</skos:scopeNote>
		<cc:license rdf:resource="http://creativecommons.org/licenses/by/3.0" />
		<cc:attributionURL rdf:resource="http://www.english-heritage.org.uk" />
		<cc:attributionName xml:lang="en">English Heritage</cc:attributionName>
		<dcterms:publisher rdf:resource="http://www.english-heritage.org.uk" />
	</skos:Concept>
	<skos:Concept rdf:about="http://purl.org/heritagedata/schemes/eh_tbm/concepts/98235">
		<skos:inScheme rdf:resource="http://purl.org/heritagedata/schemes/eh_tbm" />
		<dcterms:identifier>http://purl.org/heritagedata/schemes/eh_tbm/concepts/98235</dcterms:identifier>
		<skos:prefLabel xml:lang="en">TERRACOTTA</skos:prefLabel>
		<dcterms:issued rdf:datatype="http://www.w3.org/2001/XMLSchema#dateTime">2013-07-17T09:02:16</dcterms:issued>
		<skos:altLabel xml:lang="en">Ruabon Brick</skos:altLabel>
		<skos:narrower rdf:resource="http://purl.org/heritagedata/schemes/eh_tbm/concepts/97914" />
		<skos:broader rdf:resource="http://purl.org/heritagedata/schemes/eh_tbm/concepts/97813" />
		<skos:related rdf:resource="http://purl.org/heritagedata/schemes/eh_tbm/concepts/98241" />
		<skos:scopeNote xml:lang="en">Hard, unglazed, brown, versatile earthenware which can be used as a tile or moulded into statuary. Used in a structural or semi-structural context as a moulded hollow block.</skos:scopeNote>
		<cc:license rdf:resource="http://creativecommons.org/licenses/by/3.0" />
		<cc:attributionURL rdf:resource="http://www.english-heritage.org.uk" />
		<cc:attributionName xml:lang="en">English Heritage</cc:attributionName>
		<dcterms:publisher rdf:resource="http://www.english-heritage.org.uk" />
	</skos:Concept>
	<skos:Concept rdf:about="http://purl.org/heritagedata/schemes/eh_tbm/concepts/98236">
		<skos:inScheme rdf:resource="http://purl.org/heritagedata/schemes/eh_tbm" />
		<dcterms:identifier>http://purl.org/heritagedata/schemes/eh_tbm/concepts/98236</dcterms:identifier>
		<skos:prefLabel xml:lang="en">TERTIARY LIMESTONE</skos:prefLabel>
		<dcterms:issued rdf:datatype="http://www.w3.org/2001/XMLSchema#dateTime">2013-07-17T09:02:16</dcterms:issued>
		<skos:altLabel xml:lang="en">Coralline Crag</skos:altLabel>
		<skos:altLabel xml:lang="en">Istrian Stone</skos:altLabel>
		<skos:narrower>
			<skos:Concept rdf:about="http://purl.org/heritagedata/schemes/eh_tbm/concepts/97741">
				<skos:inScheme rdf:resource="http://purl.org/heritagedata/schemes/eh_tbm" />
				<dcterms:identifier>http://purl.org/heritagedata/schemes/eh_tbm/concepts/97741</dcterms:identifier>
				<skos:prefLabel xml:lang="en">BEMBRIDGE LIMESTONE</skos:prefLabel>
				<dcterms:issued rdf:datatype="http://www.w3.org/2001/XMLSchema#dateTime">2013-07-17T09:02:16</dcterms:issued>
				<skos:altLabel xml:lang="en">Quarr Stone</skos:altLabel>
				<skos:altLabel xml:lang="en">Bembridge Stone</skos:altLabel>
				<skos:altLabel xml:lang="en">Binstead Stone</skos:altLabel>
				<skos:altLabel xml:lang="en">Isle Of Wight Stone</skos:altLabel>
				<skos:broader rdf:resource="http://purl.org/heritagedata/schemes/eh_tbm/concepts/98236" />
				<skos:scopeNote xml:lang="en">Generic name for the hard, white/cream coloured, freshwater limestone. Quarried on the Isle of Wight.</skos:scopeNote>
				<cc:license rdf:resource="http://creativecommons.org/licenses/by/3.0" />
				<cc:attributionURL rdf:resource="http://www.english-heritage.org.uk" />
				<cc:attributionName xml:lang="en">English Heritage</cc:attributionName>
				<dcterms:publisher rdf:resource="http://www.english-heritage.org.uk" />
			</skos:Concept>
		</skos:narrower>
		<skos:broader rdf:resource="http://purl.org/heritagedata/schemes/eh_tbm/concepts/98028" />
		<skos:scopeNote xml:lang="en">Hard, fossil rich, white to deep red coloured limestone, laid down during the Tertiary period. Used since Roman times because of its good durability and weathering properties.</skos:scopeNote>
		<cc:license rdf:resource="http://creativecommons.org/licenses/by/3.0" />
		<cc:attributionURL rdf:resource="http://www.english-heritage.org.uk" />
		<cc:attributionName xml:lang="en">English Heritage</cc:attributionName>
		<dcterms:publisher rdf:resource="http://www.english-heritage.org.uk" />
	</skos:Concept>
	<skos:Concept rdf:about="http://purl.org/heritagedata/schemes/eh_tbm/concepts/98239">
		<skos:inScheme rdf:resource="http://purl.org/heritagedata/schemes/eh_tbm" />
		<dcterms:identifier>http://purl.org/heritagedata/schemes/eh_tbm/concepts/98239</dcterms:identifier>
		<skos:prefLabel xml:lang="en">THATCH</skos:prefLabel>
		<dcterms:issued rdf:datatype="http://www.w3.org/2001/XMLSchema#dateTime">2013-07-17T09:02:16</dcterms:issued>
		<skos:broader rdf:resource="http://purl.org/heritagedata/schemes/eh_tbm/concepts/98046" />
		<skos:related rdf:resource="http://purl.org/heritagedata/schemes/eh_tbm/concepts/97943" />
		<skos:related rdf:resource="http://purl.org/heritagedata/schemes/eh_tbm/concepts/97974" />
		<skos:related rdf:resource="http://purl.org/heritagedata/schemes/eh_tbm/concepts/98031" />
		<skos:related rdf:resource="http://purl.org/heritagedata/schemes/eh_tbm/concepts/98143" />
		<skos:related rdf:resource="http://purl.org/heritagedata/schemes/eh_tbm/concepts/98219" />
		<skos:scopeNote xml:lang="en">Traditional roof covering consisting of materials such as reed, straw or heather layered and fastened together onto roof to form a run off to prevent water penetration.</skos:scopeNote>
		<cc:license rdf:resource="http://creativecommons.org/licenses/by/3.0" />
		<cc:attributionURL rdf:resource="http://www.english-heritage.org.uk" />
		<cc:attributionName xml:lang="en">English Heritage</cc:attributionName>
		<dcterms:publisher rdf:resource="http://www.english-heritage.org.uk" />
	</skos:Concept>
	<skos:Concept rdf:about="http://purl.org/heritagedata/schemes/eh_tbm/concepts/98241">
		<skos:inScheme rdf:resource="http://purl.org/heritagedata/schemes/eh_tbm" />
		<dcterms:identifier>http://purl.org/heritagedata/schemes/eh_tbm/concepts/98241</dcterms:identifier>
		<skos:prefLabel xml:lang="en">TILE</skos:prefLabel>
		<dcterms:issued rdf:datatype="http://www.w3.org/2001/XMLSchema#dateTime">2013-07-17T09:02:16</dcterms:issued>
		<skos:altLabel xml:lang="en">Cement Tile</skos:altLabel>
		<skos:altLabel xml:lang="en">Clay Tile</skos:altLabel>
		<skos:altLabel xml:lang="en">Concrete Tile</skos:altLabel>
		<skos:narrower>
			<skos:Concept rdf:about="http://purl.org/heritagedata/schemes/eh_tbm/concepts/140458">
				<skos:inScheme rdf:resource="http://purl.org/heritagedata/schemes/eh_tbm" />
				<dcterms:identifier>http://purl.org/heritagedata/schemes/eh_tbm/concepts/140458</dcterms:identifier>
				<skos:prefLabel xml:lang="en">DOUBLE ROMAN TILE</skos:prefLabel>
				<dcterms:issued rdf:datatype="http://www.w3.org/2001/XMLSchema#dateTime">2013-07-17T09:02:16</dcterms:issued>
				<skos:broader rdf:resource="http://purl.org/heritagedata/schemes/eh_tbm/concepts/98241" />
				<skos:scopeNote xml:lang="en">A large rectangle roof tile with an upstand on one side, a roll in the centre and another roll on the other side, which fits over the upstand of the adjacent tile. The name does not denote a relationship with the Roman period.</skos:scopeNote>
				<cc:license rdf:resource="http://creativecommons.org/licenses/by/3.0" />
				<cc:attributionURL rdf:resource="http://www.english-heritage.org.uk" />
				<cc:attributionName xml:lang="en">English Heritage</cc:attributionName>
				<dcterms:publisher rdf:resource="http://www.english-heritage.org.uk" />
			</skos:Concept>
		</skos:narrower>
		<skos:narrower>
			<skos:Concept rdf:about="http://purl.org/heritagedata/schemes/eh_tbm/concepts/97911">
				<skos:inScheme rdf:resource="http://purl.org/heritagedata/schemes/eh_tbm" />
				<dcterms:identifier>http://purl.org/heritagedata/schemes/eh_tbm/concepts/97911</dcterms:identifier>
				<skos:prefLabel xml:lang="en">ENCAUSTIC TILE</skos:prefLabel>
				<dcterms:issued rdf:datatype="http://www.w3.org/2001/XMLSchema#dateTime">2013-07-17T09:02:16</dcterms:issued>
				<skos:broader rdf:resource="http://purl.org/heritagedata/schemes/eh_tbm/concepts/98241" />
				<skos:scopeNote xml:lang="en">Glazed and decorated, patterned earthenware tile combining different coloured clays which are inlaid and burnt in. Mainly used for flooring and external decoration.</skos:scopeNote>
				<cc:license rdf:resource="http://creativecommons.org/licenses/by/3.0" />
				<cc:attributionURL rdf:resource="http://www.english-heritage.org.uk" />
				<cc:attributionName xml:lang="en">English Heritage</cc:attributionName>
				<dcterms:publisher rdf:resource="http://www.english-heritage.org.uk" />
			</skos:Concept>
		</skos:narrower>
		<skos:narrower rdf:resource="http://purl.org/heritagedata/schemes/eh_tbm/concepts/98047" />
		<skos:narrower rdf:resource="http://purl.org/heritagedata/schemes/eh_tbm/concepts/98081" />
		<skos:narrower>
			<skos:Concept rdf:about="http://purl.org/heritagedata/schemes/eh_tbm/concepts/98157">
				<skos:inScheme rdf:resource="http://purl.org/heritagedata/schemes/eh_tbm" />
				<dcterms:identifier>http://purl.org/heritagedata/schemes/eh_tbm/concepts/98157</dcterms:identifier>
				<skos:prefLabel xml:lang="en">ROMAN TILE</skos:prefLabel>
				<dcterms:issued rdf:datatype="http://www.w3.org/2001/XMLSchema#dateTime">2013-07-17T09:02:16</dcterms:issued>
				<skos:altLabel xml:lang="en">Single Roman Tile</skos:altLabel>
				<skos:broader rdf:resource="http://purl.org/heritagedata/schemes/eh_tbm/concepts/98241" />
				<skos:scopeNote xml:lang="en">Single lap regular shaped roof covering which can have one or more water channels. Typically made of clay or concrete. The name does not denote a relationship with the Roman period.</skos:scopeNote>
				<cc:license rdf:resource="http://creativecommons.org/licenses/by/3.0" />
				<cc:attributionURL rdf:resource="http://www.english-heritage.org.uk" />
				<cc:attributionName xml:lang="en">English Heritage</cc:attributionName>
				<dcterms:publisher rdf:resource="http://www.english-heritage.org.uk" />
			</skos:Concept>
		</skos:narrower>
		<skos:narrower rdf:resource="http://purl.org/heritagedata/schemes/eh_tbm/concepts/98186" />
		<skos:narrower>
			<skos:Concept rdf:about="http://purl.org/heritagedata/schemes/eh_tbm/concepts/98199">
				<skos:inScheme rdf:resource="http://purl.org/heritagedata/schemes/eh_tbm" />
				<dcterms:identifier>http://purl.org/heritagedata/schemes/eh_tbm/concepts/98199</dcterms:identifier>
				<skos:prefLabel xml:lang="en">SPANISH TILE</skos:prefLabel>
				<dcterms:issued rdf:datatype="http://www.w3.org/2001/XMLSchema#dateTime">2013-07-17T09:02:16</dcterms:issued>
				<skos:broader rdf:resource="http://purl.org/heritagedata/schemes/eh_tbm/concepts/98241" />
				<skos:scopeNote xml:lang="en">Single lap roof covering made of clay. Half cylinder in profile although one end is slightly wider than the other. A Spanish tile roof covering comprises under-tiles and over-tiles, the two have the same shape, but the under-tile is slightly larger.</skos:scopeNote>
				<cc:license rdf:resource="http://creativecommons.org/licenses/by/3.0" />
				<cc:attributionURL rdf:resource="http://www.english-heritage.org.uk" />
				<cc:attributionName xml:lang="en">English Heritage</cc:attributionName>
				<dcterms:publisher rdf:resource="http://www.english-heritage.org.uk" />
			</skos:Concept>
		</skos:narrower>
		<skos:broader rdf:resource="http://purl.org/heritagedata/schemes/eh_tbm/concepts/98046" />
		<skos:related rdf:resource="http://purl.org/heritagedata/schemes/eh_tbm/concepts/97813" />
		<skos:related rdf:resource="http://purl.org/heritagedata/schemes/eh_tbm/concepts/97827" />
		<skos:related rdf:resource="http://purl.org/heritagedata/schemes/eh_tbm/concepts/97840" />
		<skos:related rdf:resource="http://purl.org/heritagedata/schemes/eh_tbm/concepts/97914" />
		<skos:related rdf:resource="http://purl.org/heritagedata/schemes/eh_tbm/concepts/98235" />
		<skos:scopeNote xml:lang="en">Tablet of a uniform shape. Used as finishing or covering materials which fit together in a regular format.</skos:scopeNote>
		<cc:license rdf:resource="http://creativecommons.org/licenses/by/3.0" />
		<cc:attributionURL rdf:resource="http://www.english-heritage.org.uk" />
		<cc:attributionName xml:lang="en">English Heritage</cc:attributionName>
		<dcterms:publisher rdf:resource="http://www.english-heritage.org.uk" />
	</skos:Concept>
	<skos:Concept rdf:about="http://purl.org/heritagedata/schemes/eh_tbm/concepts/98242">
		<skos:inScheme rdf:resource="http://purl.org/heritagedata/schemes/eh_tbm" />
		<dcterms:identifier>http://purl.org/heritagedata/schemes/eh_tbm/concepts/98242</dcterms:identifier>
		<skos:prefLabel xml:lang="en">TIMBER</skos:prefLabel>
		<dcterms:issued rdf:datatype="http://www.w3.org/2001/XMLSchema#dateTime">2013-07-17T09:02:16</dcterms:issued>
		<skos:altLabel xml:lang="en">Deal</skos:altLabel>
		<skos:narrower rdf:resource="http://purl.org/heritagedata/schemes/eh_tbm/concepts/98018" />
		<skos:narrower rdf:resource="http://purl.org/heritagedata/schemes/eh_tbm/concepts/98186" />
		<skos:broader rdf:resource="http://purl.org/heritagedata/schemes/eh_tbm/concepts/98046" />
		<skos:narrower rdf:resource="http://purl.org/heritagedata/schemes/eh_tbm/concepts/98276" />
		<skos:narrower rdf:resource="http://purl.org/heritagedata/schemes/eh_tbm/concepts/98282" />
		<skos:related rdf:resource="http://purl.org/heritagedata/schemes/eh_tbm/concepts/98301" />
		<skos:scopeNote xml:lang="en">Wood, cut and seasoned so forming or capable of forming any part of a structure. May be treated with preservative before use.</skos:scopeNote>
		<cc:license rdf:resource="http://creativecommons.org/licenses/by/3.0" />
		<cc:attributionURL rdf:resource="http://www.english-heritage.org.uk" />
		<cc:attributionName xml:lang="en">English Heritage</cc:attributionName>
		<dcterms:publisher rdf:resource="http://www.english-heritage.org.uk" />
	</skos:Concept>
	<skos:Concept rdf:about="http://purl.org/heritagedata/schemes/eh_tbm/concepts/98243">
		<skos:inScheme rdf:resource="http://purl.org/heritagedata/schemes/eh_tbm" />
		<dcterms:identifier>http://purl.org/heritagedata/schemes/eh_tbm/concepts/98243</dcterms:identifier>
		<skos:prefLabel xml:lang="en">TIN</skos:prefLabel>
		<dcterms:issued rdf:datatype="http://www.w3.org/2001/XMLSchema#dateTime">2013-07-17T09:02:16</dcterms:issued>
		<skos:broader rdf:resource="http://purl.org/heritagedata/schemes/eh_tbm/concepts/98053" />
		<skos:related rdf:resource="http://purl.org/heritagedata/schemes/eh_tbm/concepts/97779" />
		<skos:scopeNote xml:lang="en">Malleable metal used for roofing and for alloys such as bronze.</skos:scopeNote>
		<cc:license rdf:resource="http://creativecommons.org/licenses/by/3.0" />
		<cc:attributionURL rdf:resource="http://www.english-heritage.org.uk" />
		<cc:attributionName xml:lang="en">English Heritage</cc:attributionName>
		<dcterms:publisher rdf:resource="http://www.english-heritage.org.uk" />
	</skos:Concept>
	<skos:Concept rdf:about="http://purl.org/heritagedata/schemes/eh_tbm/concepts/98262">
		<skos:inScheme rdf:resource="http://purl.org/heritagedata/schemes/eh_tbm" />
		<dcterms:identifier>http://purl.org/heritagedata/schemes/eh_tbm/concepts/98262</dcterms:identifier>
		<skos:prefLabel xml:lang="en">TURF</skos:prefLabel>
		<dcterms:issued rdf:datatype="http://www.w3.org/2001/XMLSchema#dateTime">2013-07-17T09:02:16</dcterms:issued>
		<skos:broader rdf:resource="http://purl.org/heritagedata/schemes/eh_tbm/concepts/98265" />
		<skos:related rdf:resource="http://purl.org/heritagedata/schemes/eh_tbm/concepts/97902" />
		<skos:scopeNote xml:lang="en">Layer of grass with earth and matted roots cut from the ground and used for earth buildings and as a covering material.</skos:scopeNote>
		<cc:license rdf:resource="http://creativecommons.org/licenses/by/3.0" />
		<cc:attributionURL rdf:resource="http://www.english-heritage.org.uk" />
		<cc:attributionName xml:lang="en">English Heritage</cc:attributionName>
		<dcterms:publisher rdf:resource="http://www.english-heritage.org.uk" />
	</skos:Concept>
	<skos:Concept rdf:about="http://purl.org/heritagedata/schemes/eh_tbm/concepts/98276">
		<skos:inScheme rdf:resource="http://purl.org/heritagedata/schemes/eh_tbm" />
		<dcterms:identifier>http://purl.org/heritagedata/schemes/eh_tbm/concepts/98276</dcterms:identifier>
		<skos:prefLabel xml:lang="en">WATTLE</skos:prefLabel>
		<dcterms:issued rdf:datatype="http://www.w3.org/2001/XMLSchema#dateTime">2013-07-17T09:02:16</dcterms:issued>
		<skos:broader rdf:resource="http://purl.org/heritagedata/schemes/eh_tbm/concepts/98242" />
		<skos:related rdf:resource="http://purl.org/heritagedata/schemes/eh_tbm/concepts/97873" />
		<skos:scopeNote xml:lang="en">Wooden rods or stakes which can be interlaced with twigs or branches to make walls or fences, or more commonly, to form the basis of panels in traditional timber framed buildings which are then covered with daub.</skos:scopeNote>
		<cc:license rdf:resource="http://creativecommons.org/licenses/by/3.0" />
		<cc:attributionURL rdf:resource="http://www.english-heritage.org.uk" />
		<cc:attributionName xml:lang="en">English Heritage</cc:attributionName>
		<dcterms:publisher rdf:resource="http://www.english-heritage.org.uk" />
	</skos:Concept>
	<skos:Concept rdf:about="http://purl.org/heritagedata/schemes/eh_tbm/concepts/98282">
		<skos:inScheme rdf:resource="http://purl.org/heritagedata/schemes/eh_tbm" />
		<dcterms:identifier>http://purl.org/heritagedata/schemes/eh_tbm/concepts/98282</dcterms:identifier>
		<skos:prefLabel xml:lang="en">WEATHERBOARD</skos:prefLabel>
		<dcterms:issued rdf:datatype="http://www.w3.org/2001/XMLSchema#dateTime">2013-07-17T09:02:16</dcterms:issued>
		<skos:broader rdf:resource="http://purl.org/heritagedata/schemes/eh_tbm/concepts/98242" />
		<skos:related rdf:resource="http://purl.org/heritagedata/schemes/eh_tbm/concepts/98301" />
		<skos:scopeNote xml:lang="en">Length of timber boarding (usually elm, now pine) fixed horizontally or vertically to the exterior of a structure which may be 'tongue and grooved' or 'feathered' to provide external protection.</skos:scopeNote>
		<cc:license rdf:resource="http://creativecommons.org/licenses/by/3.0" />
		<cc:attributionURL rdf:resource="http://www.english-heritage.org.uk" />
		<cc:attributionName xml:lang="en">English Heritage</cc:attributionName>
		<dcterms:publisher rdf:resource="http://www.english-heritage.org.uk" />
	</skos:Concept>
	<skos:Concept rdf:about="http://purl.org/heritagedata/schemes/eh_tbm/concepts/98286">
		<skos:inScheme rdf:resource="http://purl.org/heritagedata/schemes/eh_tbm" />
		<dcterms:identifier>http://purl.org/heritagedata/schemes/eh_tbm/concepts/98286</dcterms:identifier>
		<skos:prefLabel xml:lang="en">WELSH SLATE</skos:prefLabel>
		<dcterms:issued rdf:datatype="http://www.w3.org/2001/XMLSchema#dateTime">2013-07-17T09:02:16</dcterms:issued>
		<skos:altLabel xml:lang="en">Penrhyn Slate</skos:altLabel>
		<skos:altLabel xml:lang="en">Berwyn Slate</skos:altLabel>
		<skos:altLabel xml:lang="en">Blue Grey Slate</skos:altLabel>
		<skos:altLabel xml:lang="en">Blue Welsh Slate</skos:altLabel>
		<skos:broader rdf:resource="http://purl.org/heritagedata/schemes/eh_tbm/concepts/98194" />
		<skos:related rdf:resource="http://purl.org/heritagedata/schemes/eh_tbm/concepts/98183" />
		<skos:scopeNote xml:lang="en">Collective term for the North and South Wales groups of slate. Hard, fine grained, metamorphic rock, with varying dark shades.</skos:scopeNote>
		<cc:license rdf:resource="http://creativecommons.org/licenses/by/3.0" />
		<cc:attributionURL rdf:resource="http://www.english-heritage.org.uk" />
		<cc:attributionName xml:lang="en">English Heritage</cc:attributionName>
		<dcterms:publisher rdf:resource="http://www.english-heritage.org.uk" />
	</skos:Concept>
	<skos:Concept rdf:about="http://purl.org/heritagedata/schemes/eh_tbm/concepts/98287">
		<skos:inScheme rdf:resource="http://purl.org/heritagedata/schemes/eh_tbm" />
		<dcterms:identifier>http://purl.org/heritagedata/schemes/eh_tbm/concepts/98287</dcterms:identifier>
		<skos:prefLabel xml:lang="en">WEST COUNTRY SLATE</skos:prefLabel>
		<dcterms:issued rdf:datatype="http://www.w3.org/2001/XMLSchema#dateTime">2013-07-17T09:02:16</dcterms:issued>
		<skos:altLabel xml:lang="en">Mill Hill Slate</skos:altLabel>
		<skos:altLabel xml:lang="en">Tintagel Stone</skos:altLabel>
		<skos:altLabel xml:lang="en">Trebarwith Rustic Slate</skos:altLabel>
		<skos:altLabel xml:lang="en">Trecarne Rustic Slate</skos:altLabel>
		<skos:altLabel xml:lang="en">Tredinnick Rustic Slate</skos:altLabel>
		<skos:altLabel xml:lang="en">Bluestone</skos:altLabel>
		<skos:altLabel xml:lang="en">Cornish Rustic</skos:altLabel>
		<skos:altLabel xml:lang="en">Cornish Slate</skos:altLabel>
		<skos:altLabel xml:lang="en">Delabole Slate</skos:altLabel>
		<skos:altLabel xml:lang="en">Devon Slate</skos:altLabel>
		<skos:broader rdf:resource="http://purl.org/heritagedata/schemes/eh_tbm/concepts/98194" />
		<skos:related rdf:resource="http://purl.org/heritagedata/schemes/eh_tbm/concepts/98183" />
		<skos:scopeNote xml:lang="en">Collective term for the slates from Devon and Cornwall. Hard, fine grained metamorphic rock. Varying in colour from dark grey/green to blueish/grey. West Country Slate is geologically different from both Lake District and Welsh Slate.</skos:scopeNote>
		<cc:license rdf:resource="http://creativecommons.org/licenses/by/3.0" />
		<cc:attributionURL rdf:resource="http://www.english-heritage.org.uk" />
		<cc:attributionName xml:lang="en">English Heritage</cc:attributionName>
		<dcterms:publisher rdf:resource="http://www.english-heritage.org.uk" />
	</skos:Concept>
	<skos:Concept rdf:about="http://purl.org/heritagedata/schemes/eh_tbm/concepts/98293">
		<skos:inScheme rdf:resource="http://purl.org/heritagedata/schemes/eh_tbm" />
		<dcterms:identifier>http://purl.org/heritagedata/schemes/eh_tbm/concepts/98293</dcterms:identifier>
		<skos:prefLabel xml:lang="en">WHINSTONE</skos:prefLabel>
		<dcterms:issued rdf:datatype="http://www.w3.org/2001/XMLSchema#dateTime">2013-07-17T09:02:16</dcterms:issued>
		<skos:broader rdf:resource="http://purl.org/heritagedata/schemes/eh_tbm/concepts/98216" />
		<skos:related rdf:resource="http://purl.org/heritagedata/schemes/eh_tbm/concepts/97734" />
		<skos:related rdf:resource="http://purl.org/heritagedata/schemes/eh_tbm/concepts/97891" />
		<skos:scopeNote xml:lang="en">Northern quarryman's name for any fine grained, dark grey/black to green coloured igneous rock. Index with specific stone type where given.</skos:scopeNote>
		<cc:license rdf:resource="http://creativecommons.org/licenses/by/3.0" />
		<cc:attributionURL rdf:resource="http://www.english-heritage.org.uk" />
		<cc:attributionName xml:lang="en">English Heritage</cc:attributionName>
		<dcterms:publisher rdf:resource="http://www.english-heritage.org.uk" />
	</skos:Concept>
	<skos:Concept rdf:about="http://purl.org/heritagedata/schemes/eh_tbm/concepts/98301">
		<skos:inScheme rdf:resource="http://purl.org/heritagedata/schemes/eh_tbm" />
		<dcterms:identifier>http://purl.org/heritagedata/schemes/eh_tbm/concepts/98301</dcterms:identifier>
		<skos:prefLabel xml:lang="en">WOOD</skos:prefLabel>
		<dcterms:issued rdf:datatype="http://www.w3.org/2001/XMLSchema#dateTime">2013-07-17T09:02:16</dcterms:issued>
		<skos:narrower>
			<skos:Concept rdf:about="http://purl.org/heritagedata/schemes/eh_tbm/concepts/97729">
				<skos:inScheme rdf:resource="http://purl.org/heritagedata/schemes/eh_tbm" />
				<dcterms:identifier>http://purl.org/heritagedata/schemes/eh_tbm/concepts/97729</dcterms:identifier>
				<skos:prefLabel xml:lang="en">BAMBOO</skos:prefLabel>
				<dcterms:issued rdf:datatype="http://www.w3.org/2001/XMLSchema#dateTime">2013-07-17T09:02:16</dcterms:issued>
				<skos:broader rdf:resource="http://purl.org/heritagedata/schemes/eh_tbm/concepts/98301" />
				<skos:scopeNote xml:lang="en">Tropical giant grass with hollow stem used structurally or as a covering material.</skos:scopeNote>
				<cc:license rdf:resource="http://creativecommons.org/licenses/by/3.0" />
				<cc:attributionURL rdf:resource="http://www.english-heritage.org.uk" />
				<cc:attributionName xml:lang="en">English Heritage</cc:attributionName>
				<dcterms:publisher rdf:resource="http://www.english-heritage.org.uk" />
			</skos:Concept>
		</skos:narrower>
		<skos:narrower>
			<skos:Concept rdf:about="http://purl.org/heritagedata/schemes/eh_tbm/concepts/97808">
				<skos:inScheme rdf:resource="http://purl.org/heritagedata/schemes/eh_tbm" />
				<dcterms:identifier>http://purl.org/heritagedata/schemes/eh_tbm/concepts/97808</dcterms:identifier>
				<skos:prefLabel xml:lang="en">CEDAR</skos:prefLabel>
				<dcterms:issued rdf:datatype="http://www.w3.org/2001/XMLSchema#dateTime">2013-07-17T09:02:16</dcterms:issued>
				<skos:broader rdf:resource="http://purl.org/heritagedata/schemes/eh_tbm/concepts/98301" />
				<skos:scopeNote xml:lang="en">Durable wood from a non-native, evergreen conifer.</skos:scopeNote>
				<cc:license rdf:resource="http://creativecommons.org/licenses/by/3.0" />
				<cc:attributionURL rdf:resource="http://www.english-heritage.org.uk" />
				<cc:attributionName xml:lang="en">English Heritage</cc:attributionName>
				<dcterms:publisher rdf:resource="http://www.english-heritage.org.uk" />
			</skos:Concept>
		</skos:narrower>
		<skos:narrower>
			<skos:Concept rdf:about="http://purl.org/heritagedata/schemes/eh_tbm/concepts/97850">
				<skos:inScheme rdf:resource="http://purl.org/heritagedata/schemes/eh_tbm" />
				<dcterms:identifier>http://purl.org/heritagedata/schemes/eh_tbm/concepts/97850</dcterms:identifier>
				<skos:prefLabel xml:lang="en">CORK</skos:prefLabel>
				<dcterms:issued rdf:datatype="http://www.w3.org/2001/XMLSchema#dateTime">2013-07-17T09:02:16</dcterms:issued>
				<skos:broader rdf:resource="http://purl.org/heritagedata/schemes/eh_tbm/concepts/98301" />
				<skos:scopeNote xml:lang="en">Buoyant, light material obtained from the cork tree.</skos:scopeNote>
				<cc:license rdf:resource="http://creativecommons.org/licenses/by/3.0" />
				<cc:attributionURL rdf:resource="http://www.english-heritage.org.uk" />
				<cc:attributionName xml:lang="en">English Heritage</cc:attributionName>
				<dcterms:publisher rdf:resource="http://www.english-heritage.org.uk" />
			</skos:Concept>
		</skos:narrower>
		<skos:narrower>
			<skos:Concept rdf:about="http://purl.org/heritagedata/schemes/eh_tbm/concepts/97906">
				<skos:inScheme rdf:resource="http://purl.org/heritagedata/schemes/eh_tbm" />
				<dcterms:identifier>http://purl.org/heritagedata/schemes/eh_tbm/concepts/97906</dcterms:identifier>
				<skos:prefLabel xml:lang="en">ELM</skos:prefLabel>
				<dcterms:issued rdf:datatype="http://www.w3.org/2001/XMLSchema#dateTime">2013-07-17T09:02:16</dcterms:issued>
				<skos:broader rdf:resource="http://purl.org/heritagedata/schemes/eh_tbm/concepts/98301" />
				<skos:scopeNote xml:lang="en">Deciduous wood from the native elm tree, commonly used for framing or cladding of lesser timber framed structures due to its poorer weathering qualities as compared to oak.</skos:scopeNote>
				<cc:license rdf:resource="http://creativecommons.org/licenses/by/3.0" />
				<cc:attributionURL rdf:resource="http://www.english-heritage.org.uk" />
				<cc:attributionName xml:lang="en">English Heritage</cc:attributionName>
				<dcterms:publisher rdf:resource="http://www.english-heritage.org.uk" />
			</skos:Concept>
		</skos:narrower>
		<skos:narrower>
			<skos:Concept rdf:about="http://purl.org/heritagedata/schemes/eh_tbm/concepts/98074">
				<skos:inScheme rdf:resource="http://purl.org/heritagedata/schemes/eh_tbm" />
				<dcterms:identifier>http://purl.org/heritagedata/schemes/eh_tbm/concepts/98074</dcterms:identifier>
				<skos:prefLabel xml:lang="en">OAK</skos:prefLabel>
				<dcterms:issued rdf:datatype="http://www.w3.org/2001/XMLSchema#dateTime">2013-07-17T09:02:16</dcterms:issued>
				<skos:broader rdf:resource="http://purl.org/heritagedata/schemes/eh_tbm/concepts/98301" />
				<skos:scopeNote xml:lang="en">A native hardwood of the Beech family with hard and durable characteristics which traditionally made it appropriate for structural work.</skos:scopeNote>
				<cc:license rdf:resource="http://creativecommons.org/licenses/by/3.0" />
				<cc:attributionURL rdf:resource="http://www.english-heritage.org.uk" />
				<cc:attributionName xml:lang="en">English Heritage</cc:attributionName>
				<dcterms:publisher rdf:resource="http://www.english-heritage.org.uk" />
			</skos:Concept>
		</skos:narrower>
		<skos:narrower>
			<skos:Concept rdf:about="http://purl.org/heritagedata/schemes/eh_tbm/concepts/98104">
				<skos:inScheme rdf:resource="http://purl.org/heritagedata/schemes/eh_tbm" />
				<dcterms:identifier>http://purl.org/heritagedata/schemes/eh_tbm/concepts/98104</dcterms:identifier>
				<skos:prefLabel xml:lang="en">PINE</skos:prefLabel>
				<dcterms:issued rdf:datatype="http://www.w3.org/2001/XMLSchema#dateTime">2013-07-17T09:02:16</dcterms:issued>
				<skos:broader rdf:resource="http://purl.org/heritagedata/schemes/eh_tbm/concepts/98301" />
				<skos:scopeNote xml:lang="en">Wood of a coniferous tree native to Scotland and Scandinavia.</skos:scopeNote>
				<cc:license rdf:resource="http://creativecommons.org/licenses/by/3.0" />
				<cc:attributionURL rdf:resource="http://www.english-heritage.org.uk" />
				<cc:attributionName xml:lang="en">English Heritage</cc:attributionName>
				<dcterms:publisher rdf:resource="http://www.english-heritage.org.uk" />
			</skos:Concept>
		</skos:narrower>
		<skos:broader rdf:resource="http://purl.org/heritagedata/schemes/eh_tbm/concepts/98265" />
		<skos:related rdf:resource="http://purl.org/heritagedata/schemes/eh_tbm/concepts/97917" />
		<skos:related rdf:resource="http://purl.org/heritagedata/schemes/eh_tbm/concepts/98082" />
		<skos:related rdf:resource="http://purl.org/heritagedata/schemes/eh_tbm/concepts/98113" />
		<skos:related rdf:resource="http://purl.org/heritagedata/schemes/eh_tbm/concepts/98116" />
		<skos:related rdf:resource="http://purl.org/heritagedata/schemes/eh_tbm/concepts/98242" />
		<skos:related rdf:resource="http://purl.org/heritagedata/schemes/eh_tbm/concepts/98282" />
		<skos:related rdf:resource="http://purl.org/heritagedata/schemes/eh_tbm/concepts/98303" />
		<skos:scopeNote xml:lang="en">Hard, compact, unprocessed, fibrous cellulose substance. The roots, trunks and branches of trees and shrubs consist of this tissue.</skos:scopeNote>
		<cc:license rdf:resource="http://creativecommons.org/licenses/by/3.0" />
		<cc:attributionURL rdf:resource="http://www.english-heritage.org.uk" />
		<cc:attributionName xml:lang="en">English Heritage</cc:attributionName>
		<dcterms:publisher rdf:resource="http://www.english-heritage.org.uk" />
	</skos:Concept>
	<skos:Concept rdf:about="http://purl.org/heritagedata/schemes/eh_tbm/concepts/98303">
		<skos:inScheme rdf:resource="http://purl.org/heritagedata/schemes/eh_tbm" />
		<dcterms:identifier>http://purl.org/heritagedata/schemes/eh_tbm/concepts/98303</dcterms:identifier>
		<skos:prefLabel xml:lang="en">WOODWOOL SLAB</skos:prefLabel>
		<dcterms:issued rdf:datatype="http://www.w3.org/2001/XMLSchema#dateTime">2013-07-17T09:02:16</dcterms:issued>
		<skos:broader rdf:resource="http://purl.org/heritagedata/schemes/eh_tbm/concepts/98080" />
		<skos:related rdf:resource="http://purl.org/heritagedata/schemes/eh_tbm/concepts/97809" />
		<skos:related rdf:resource="http://purl.org/heritagedata/schemes/eh_tbm/concepts/98301" />
		<skos:scopeNote xml:lang="en">A sheet or board made from a mixture of thin strips of wood and cement which are bound together through compression within a mould. Woodwool slabs are used for roof or wall cladding, providing fire resistance, and heat and sound insulation.</skos:scopeNote>
		<cc:license rdf:resource="http://creativecommons.org/licenses/by/3.0" />
		<cc:attributionURL rdf:resource="http://www.english-heritage.org.uk" />
		<cc:attributionName xml:lang="en">English Heritage</cc:attributionName>
		<dcterms:publisher rdf:resource="http://www.english-heritage.org.uk" />
	</skos:Concept>
	<skos:Concept rdf:about="http://purl.org/heritagedata/schemes/eh_tbm/concepts/97749">
		<skos:inScheme rdf:resource="http://purl.org/heritagedata/schemes/eh_tbm" />
		<dcterms:identifier>http://purl.org/heritagedata/schemes/eh_tbm/concepts/97749</dcterms:identifier>
		<skos:prefLabel xml:lang="en">BITUMEN</skos:prefLabel>
		<dcterms:issued rdf:datatype="http://www.w3.org/2001/XMLSchema#dateTime">2013-07-17T09:02:16</dcterms:issued>
		<skos:narrower>
			<skos:Concept rdf:about="http://purl.org/heritagedata/schemes/eh_tbm/concepts/97723">
				<skos:inScheme rdf:resource="http://purl.org/heritagedata/schemes/eh_tbm" />
				<dcterms:identifier>http://purl.org/heritagedata/schemes/eh_tbm/concepts/97723</dcterms:identifier>
				<skos:prefLabel xml:lang="en">ASPHALT</skos:prefLabel>
				<dcterms:issued rdf:datatype="http://www.w3.org/2001/XMLSchema#dateTime">2013-07-17T09:02:16</dcterms:issued>
				<skos:broader rdf:resource="http://purl.org/heritagedata/schemes/eh_tbm/concepts/97749" />
				<skos:scopeNote xml:lang="en">Solid or viscous bituminous pitch of natural occurrence,or produced from petroleum mixed with sand or other aggregate filler, for use in roads or as a covering material</skos:scopeNote>
				<cc:license rdf:resource="http://creativecommons.org/licenses/by/3.0" />
				<cc:attributionURL rdf:resource="http://www.english-heritage.org.uk" />
				<cc:attributionName xml:lang="en">English Heritage</cc:attributionName>
				<dcterms:publisher rdf:resource="http://www.english-heritage.org.uk" />
			</skos:Concept>
		</skos:narrower>
		<skos:broader rdf:resource="http://purl.org/heritagedata/schemes/eh_tbm/concepts/98041" />
		<skos:narrower>
			<skos:Concept rdf:about="http://purl.org/heritagedata/schemes/eh_tbm/concepts/98231">
				<skos:inScheme rdf:resource="http://purl.org/heritagedata/schemes/eh_tbm" />
				<dcterms:identifier>http://purl.org/heritagedata/schemes/eh_tbm/concepts/98231</dcterms:identifier>
				<skos:prefLabel xml:lang="en">TAR</skos:prefLabel>
				<dcterms:issued rdf:datatype="http://www.w3.org/2001/XMLSchema#dateTime">2013-07-17T09:02:16</dcterms:issued>
				<skos:broader rdf:resource="http://purl.org/heritagedata/schemes/eh_tbm/concepts/97749" />
				<skos:scopeNote xml:lang="en">Thick, viscid liquid, obtained by the distillation of wood, coal or other organic substances, chemically a mixture of hydrocarbons with resins.</skos:scopeNote>
				<cc:license rdf:resource="http://creativecommons.org/licenses/by/3.0" />
				<cc:attributionURL rdf:resource="http://www.english-heritage.org.uk" />
				<cc:attributionName xml:lang="en">English Heritage</cc:attributionName>
				<dcterms:publisher rdf:resource="http://www.english-heritage.org.uk" />
			</skos:Concept>
		</skos:narrower>
		<skos:narrower>
			<skos:Concept rdf:about="http://purl.org/heritagedata/schemes/eh_tbm/concepts/98232">
				<skos:inScheme rdf:resource="http://purl.org/heritagedata/schemes/eh_tbm" />
				<dcterms:identifier>http://purl.org/heritagedata/schemes/eh_tbm/concepts/98232</dcterms:identifier>
				<skos:prefLabel xml:lang="en">TARMACADAM</skos:prefLabel>
				<dcterms:issued rdf:datatype="http://www.w3.org/2001/XMLSchema#dateTime">2013-07-17T09:02:16</dcterms:issued>
				<skos:broader rdf:resource="http://purl.org/heritagedata/schemes/eh_tbm/concepts/97749" />
				<skos:scopeNote xml:lang="en">Road or paving material combining crushed stone, rolled and mixed with bitumen type mixer.</skos:scopeNote>
				<cc:license rdf:resource="http://creativecommons.org/licenses/by/3.0" />
				<cc:attributionURL rdf:resource="http://www.english-heritage.org.uk" />
				<cc:attributionName xml:lang="en">English Heritage</cc:attributionName>
				<dcterms:publisher rdf:resource="http://www.english-heritage.org.uk" />
			</skos:Concept>
		</skos:narrower>
		<skos:scopeNote xml:lang="en">A semi solid mixture of complex hydrocarbons derived from coal or petroleum. Used as a waterproof binder or protective coating.</skos:scopeNote>
		<cc:license rdf:resource="http://creativecommons.org/licenses/by/3.0" />
		<cc:attributionURL rdf:resource="http://www.english-heritage.org.uk" />
		<cc:attributionName xml:lang="en">English Heritage</cc:attributionName>
		<dcterms:publisher rdf:resource="http://www.english-heritage.org.uk" />
	</skos:Concept>
	<skos:Concept rdf:about="http://purl.org/heritagedata/schemes/eh_tbm/concepts/97756">
		<skos:inScheme rdf:resource="http://purl.org/heritagedata/schemes/eh_tbm" />
		<dcterms:identifier>http://purl.org/heritagedata/schemes/eh_tbm/concepts/97756</dcterms:identifier>
		<skos:prefLabel xml:lang="en">BLUE LIAS</skos:prefLabel>
		<dcterms:issued rdf:datatype="http://www.w3.org/2001/XMLSchema#dateTime">2013-07-17T09:02:16</dcterms:issued>
		<skos:broader rdf:resource="http://purl.org/heritagedata/schemes/eh_tbm/concepts/98024" />
		<skos:narrower>
			<skos:Concept rdf:about="http://purl.org/heritagedata/schemes/eh_tbm/concepts/98000">
				<skos:inScheme rdf:resource="http://purl.org/heritagedata/schemes/eh_tbm" />
				<dcterms:identifier>http://purl.org/heritagedata/schemes/eh_tbm/concepts/98000</dcterms:identifier>
				<skos:prefLabel xml:lang="en">KEINTON STONE</skos:prefLabel>
				<dcterms:issued rdf:datatype="http://www.w3.org/2001/XMLSchema#dateTime">2013-07-17T09:02:16</dcterms:issued>
				<skos:broader rdf:resource="http://purl.org/heritagedata/schemes/eh_tbm/concepts/97756" />
				<skos:scopeNote xml:lang="en">Hard, white/grey coloured liassic limestone. Quarried near Somerton in Somerset.</skos:scopeNote>
				<cc:license rdf:resource="http://creativecommons.org/licenses/by/3.0" />
				<cc:attributionURL rdf:resource="http://www.english-heritage.org.uk" />
				<cc:attributionName xml:lang="en">English Heritage</cc:attributionName>
				<dcterms:publisher rdf:resource="http://www.english-heritage.org.uk" />
			</skos:Concept>
		</skos:narrower>
		<skos:scopeNote xml:lang="en">Hard white/grey coloured liassic limestone. Quarried on the Devon-Dorset border.</skos:scopeNote>
		<cc:license rdf:resource="http://creativecommons.org/licenses/by/3.0" />
		<cc:attributionURL rdf:resource="http://www.english-heritage.org.uk" />
		<cc:attributionName xml:lang="en">English Heritage</cc:attributionName>
		<dcterms:publisher rdf:resource="http://www.english-heritage.org.uk" />
	</skos:Concept>
	<skos:Concept rdf:about="http://purl.org/heritagedata/schemes/eh_tbm/concepts/97774">
		<skos:inScheme rdf:resource="http://purl.org/heritagedata/schemes/eh_tbm" />
		<dcterms:identifier>http://purl.org/heritagedata/schemes/eh_tbm/concepts/97774</dcterms:identifier>
		<skos:prefLabel xml:lang="en">BRECCIA</skos:prefLabel>
		<dcterms:issued rdf:datatype="http://www.w3.org/2001/XMLSchema#dateTime">2013-07-17T09:02:16</dcterms:issued>
		<skos:broader rdf:resource="http://purl.org/heritagedata/schemes/eh_tbm/concepts/98216" />
		<skos:related rdf:resource="http://purl.org/heritagedata/schemes/eh_tbm/concepts/164108" />
		<skos:related rdf:resource="http://purl.org/heritagedata/schemes/eh_tbm/concepts/97843" />
		<skos:related rdf:resource="http://purl.org/heritagedata/schemes/eh_tbm/concepts/98126" />
		<skos:scopeNote xml:lang="en">Sedimentary rock consisting of angular fragments naturally cemented together.</skos:scopeNote>
		<cc:license rdf:resource="http://creativecommons.org/licenses/by/3.0" />
		<cc:attributionURL rdf:resource="http://www.english-heritage.org.uk" />
		<cc:attributionName xml:lang="en">English Heritage</cc:attributionName>
		<dcterms:publisher rdf:resource="http://www.english-heritage.org.uk" />
	</skos:Concept>
	<skos:Concept rdf:about="http://purl.org/heritagedata/schemes/eh_tbm/concepts/97776">
		<skos:inScheme rdf:resource="http://purl.org/heritagedata/schemes/eh_tbm" />
		<dcterms:identifier>http://purl.org/heritagedata/schemes/eh_tbm/concepts/97776</dcterms:identifier>
		<skos:prefLabel xml:lang="en">BREEZE BLOCK</skos:prefLabel>
		<dcterms:issued rdf:datatype="http://www.w3.org/2001/XMLSchema#dateTime">2013-07-17T09:02:16</dcterms:issued>
		<skos:altLabel xml:lang="en">Thermalite</skos:altLabel>
		<skos:broader rdf:resource="http://purl.org/heritagedata/schemes/eh_tbm/concepts/97840" />
		<skos:related rdf:resource="http://purl.org/heritagedata/schemes/eh_tbm/concepts/98148" />
		<skos:scopeNote xml:lang="en">Lightweight building block traditionally made with coke breeze from gas works combined with sand and cement. Use this term generally to denote a light, modern concrete building block with man made characteristics.</skos:scopeNote>
		<cc:license rdf:resource="http://creativecommons.org/licenses/by/3.0" />
		<cc:attributionURL rdf:resource="http://www.english-heritage.org.uk" />
		<cc:attributionName xml:lang="en">English Heritage</cc:attributionName>
		<dcterms:publisher rdf:resource="http://www.english-heritage.org.uk" />
	</skos:Concept>
	<skos:Concept rdf:about="http://purl.org/heritagedata/schemes/eh_tbm/concepts/97777">
		<skos:inScheme rdf:resource="http://purl.org/heritagedata/schemes/eh_tbm" />
		<dcterms:identifier>http://purl.org/heritagedata/schemes/eh_tbm/concepts/97777</dcterms:identifier>
		<skos:prefLabel xml:lang="en">BRICK</skos:prefLabel>
		<dcterms:issued rdf:datatype="http://www.w3.org/2001/XMLSchema#dateTime">2013-07-17T09:02:16</dcterms:issued>
		<skos:altLabel xml:lang="en">Malm (Brick)</skos:altLabel>
		<skos:altLabel xml:lang="en">Ruabon Brick</skos:altLabel>
		<skos:altLabel xml:lang="en">Staffordshire Blue Brick</skos:altLabel>
		<skos:altLabel xml:lang="en">Vitrified Brick</skos:altLabel>
		<skos:altLabel xml:lang="en">Fletton Brick</skos:altLabel>
		<skos:altLabel xml:lang="en">Flint Lime Brick</skos:altLabel>
		<skos:broader rdf:resource="http://purl.org/heritagedata/schemes/eh_tbm/concepts/98046" />
		<skos:narrower>
			<skos:Concept rdf:about="http://purl.org/heritagedata/schemes/eh_tbm/concepts/97912">
				<skos:inScheme rdf:resource="http://purl.org/heritagedata/schemes/eh_tbm" />
				<dcterms:identifier>http://purl.org/heritagedata/schemes/eh_tbm/concepts/97912</dcterms:identifier>
				<skos:prefLabel xml:lang="en">ENGINEERING BRICK</skos:prefLabel>
				<dcterms:issued rdf:datatype="http://www.w3.org/2001/XMLSchema#dateTime">2013-07-17T09:02:16</dcterms:issued>
				<skos:broader rdf:resource="http://purl.org/heritagedata/schemes/eh_tbm/concepts/97777" />
				<skos:scopeNote xml:lang="en">A dense, high strength, low absorption brick of uniform size, employed predominantly in industrial structures such as railway viaducts.</skos:scopeNote>
				<cc:license rdf:resource="http://creativecommons.org/licenses/by/3.0" />
				<cc:attributionURL rdf:resource="http://www.english-heritage.org.uk" />
				<cc:attributionName xml:lang="en">English Heritage</cc:attributionName>
				<dcterms:publisher rdf:resource="http://www.english-heritage.org.uk" />
			</skos:Concept>
		</skos:narrower>
		<skos:related rdf:resource="http://purl.org/heritagedata/schemes/eh_tbm/concepts/97827" />
		<skos:related rdf:resource="http://purl.org/heritagedata/schemes/eh_tbm/concepts/98047" />
		<skos:related rdf:resource="http://purl.org/heritagedata/schemes/eh_tbm/concepts/98087" />
		<skos:scopeNote xml:lang="en">Standard rectangular block or tablet bonded on mortar joints in a regular arrangement or pattern for strength or decoration. Made from clay or brick earth which may contain varying quantities of chalk, lime or iron oxide which effect colour or density.</skos:scopeNote>
		<cc:license rdf:resource="http://creativecommons.org/licenses/by/3.0" />
		<cc:attributionURL rdf:resource="http://www.english-heritage.org.uk" />
		<cc:attributionName xml:lang="en">English Heritage</cc:attributionName>
		<dcterms:publisher rdf:resource="http://www.english-heritage.org.uk" />
	</skos:Concept>
	<skos:Concept rdf:about="http://purl.org/heritagedata/schemes/eh_tbm/concepts/97779">
		<skos:inScheme rdf:resource="http://purl.org/heritagedata/schemes/eh_tbm" />
		<dcterms:identifier>http://purl.org/heritagedata/schemes/eh_tbm/concepts/97779</dcterms:identifier>
		<skos:prefLabel xml:lang="en">BRONZE</skos:prefLabel>
		<dcterms:issued rdf:datatype="http://www.w3.org/2001/XMLSchema#dateTime">2013-07-17T09:02:16</dcterms:issued>
		<skos:broader rdf:resource="http://purl.org/heritagedata/schemes/eh_tbm/concepts/98053" />
		<skos:related rdf:resource="http://purl.org/heritagedata/schemes/eh_tbm/concepts/97845" />
		<skos:related rdf:resource="http://purl.org/heritagedata/schemes/eh_tbm/concepts/98243" />
		<skos:scopeNote xml:lang="en">Hard, corrosive resistant alloy of copper and tin.</skos:scopeNote>
		<cc:license rdf:resource="http://creativecommons.org/licenses/by/3.0" />
		<cc:attributionURL rdf:resource="http://www.english-heritage.org.uk" />
		<cc:attributionName xml:lang="en">English Heritage</cc:attributionName>
		<dcterms:publisher rdf:resource="http://www.english-heritage.org.uk" />
	</skos:Concept>
	<skos:Concept rdf:about="http://purl.org/heritagedata/schemes/eh_tbm/concepts/97800">
		<skos:inScheme rdf:resource="http://purl.org/heritagedata/schemes/eh_tbm" />
		<dcterms:identifier>http://purl.org/heritagedata/schemes/eh_tbm/concepts/97800</dcterms:identifier>
		<skos:prefLabel xml:lang="en">CARBONIFEROUS LIMESTONE</skos:prefLabel>
		<dcterms:issued rdf:datatype="http://www.w3.org/2001/XMLSchema#dateTime">2013-07-17T09:02:16</dcterms:issued>
		<skos:altLabel xml:lang="en">Penmon Limestone</skos:altLabel>
		<skos:altLabel xml:lang="en">Pennon Marble</skos:altLabel>
		<skos:altLabel xml:lang="en">Orton Scar Limestone</skos:altLabel>
		<skos:altLabel xml:lang="en">Salterwath</skos:altLabel>
		<skos:altLabel xml:lang="en">Swaledale Fossil</skos:altLabel>
		<skos:altLabel xml:lang="en">Cheddar Stone</skos:altLabel>
		<skos:altLabel xml:lang="en">Battscombe Stone</skos:altLabel>
		<skos:altLabel xml:lang="en">Deepdale Fossil</skos:altLabel>
		<skos:altLabel xml:lang="en">Derbydene</skos:altLabel>
		<skos:altLabel xml:lang="en">Derbyshire Fossil</skos:altLabel>
		<skos:altLabel xml:lang="en">Dukes Red Limestone</skos:altLabel>
		<skos:altLabel xml:lang="en">Frosterley Marble</skos:altLabel>
		<skos:altLabel xml:lang="en">Hadene Stone</skos:altLabel>
		<skos:altLabel xml:lang="en">Hoptons Wood Stone</skos:altLabel>
		<skos:broader rdf:resource="http://purl.org/heritagedata/schemes/eh_tbm/concepts/98028" />
		<skos:related rdf:resource="http://purl.org/heritagedata/schemes/eh_tbm/concepts/98044" />
		<skos:related rdf:resource="http://purl.org/heritagedata/schemes/eh_tbm/concepts/98171" />
		<skos:related rdf:resource="http://purl.org/heritagedata/schemes/eh_tbm/concepts/98183" />
		<skos:scopeNote xml:lang="en">Limestones formed during the Carboniferous period. Many are cut, polished and used as marble.</skos:scopeNote>
		<cc:license rdf:resource="http://creativecommons.org/licenses/by/3.0" />
		<cc:attributionURL rdf:resource="http://www.english-heritage.org.uk" />
		<cc:attributionName xml:lang="en">English Heritage</cc:attributionName>
		<dcterms:publisher rdf:resource="http://www.english-heritage.org.uk" />
	</skos:Concept>
	<skos:Concept rdf:about="http://purl.org/heritagedata/schemes/eh_tbm/concepts/97803">
		<skos:inScheme rdf:resource="http://purl.org/heritagedata/schemes/eh_tbm" />
		<dcterms:identifier>http://purl.org/heritagedata/schemes/eh_tbm/concepts/97803</dcterms:identifier>
		<skos:prefLabel xml:lang="en">CARSTONE</skos:prefLabel>
		<dcterms:issued rdf:datatype="http://www.w3.org/2001/XMLSchema#dateTime">2013-07-17T09:02:16</dcterms:issued>
		<skos:altLabel xml:lang="en">Car Stone</skos:altLabel>
		<skos:altLabel xml:lang="en">Ginger Bread Stone</skos:altLabel>
		<skos:broader rdf:resource="http://purl.org/heritagedata/schemes/eh_tbm/concepts/98171" />
		<skos:related rdf:resource="http://purl.org/heritagedata/schemes/eh_tbm/concepts/97993" />
		<skos:scopeNote xml:lang="en">Coarse hard sandstone often coloured with iron oxide creating its characteristic brown shades.</skos:scopeNote>
		<cc:license rdf:resource="http://creativecommons.org/licenses/by/3.0" />
		<cc:attributionURL rdf:resource="http://www.english-heritage.org.uk" />
		<cc:attributionName xml:lang="en">English Heritage</cc:attributionName>
		<dcterms:publisher rdf:resource="http://www.english-heritage.org.uk" />
	</skos:Concept>
	<skos:Concept rdf:about="http://purl.org/heritagedata/schemes/eh_tbm/concepts/97809">
		<skos:inScheme rdf:resource="http://purl.org/heritagedata/schemes/eh_tbm" />
		<dcterms:identifier>http://purl.org/heritagedata/schemes/eh_tbm/concepts/97809</dcterms:identifier>
		<skos:prefLabel xml:lang="en">CEMENT</skos:prefLabel>
		<dcterms:issued rdf:datatype="http://www.w3.org/2001/XMLSchema#dateTime">2013-07-17T09:02:16</dcterms:issued>
		<skos:altLabel xml:lang="en">Whitby Cement</skos:altLabel>
		<skos:altLabel xml:lang="en">Cement Render</skos:altLabel>
		<skos:altLabel xml:lang="en">Cement Tile</skos:altLabel>
		<skos:broader rdf:resource="http://purl.org/heritagedata/schemes/eh_tbm/concepts/97810" />
		<skos:narrower>
			<skos:Concept rdf:about="http://purl.org/heritagedata/schemes/eh_tbm/concepts/98121">
				<skos:inScheme rdf:resource="http://purl.org/heritagedata/schemes/eh_tbm" />
				<dcterms:identifier>http://purl.org/heritagedata/schemes/eh_tbm/concepts/98121</dcterms:identifier>
				<skos:prefLabel xml:lang="en">PORTLAND CEMENT</skos:prefLabel>
				<dcterms:issued rdf:datatype="http://www.w3.org/2001/XMLSchema#dateTime">2013-07-17T09:02:16</dcterms:issued>
				<skos:broader rdf:resource="http://purl.org/heritagedata/schemes/eh_tbm/concepts/97809" />
				<skos:scopeNote xml:lang="en">A form of cement originally named since it was said to be like Portland Stone in appearance.</skos:scopeNote>
				<cc:license rdf:resource="http://creativecommons.org/licenses/by/3.0" />
				<cc:attributionURL rdf:resource="http://www.english-heritage.org.uk" />
				<cc:attributionName xml:lang="en">English Heritage</cc:attributionName>
				<dcterms:publisher rdf:resource="http://www.english-heritage.org.uk" />
			</skos:Concept>
		</skos:narrower>
		<skos:related rdf:resource="http://purl.org/heritagedata/schemes/eh_tbm/concepts/97840" />
		<skos:related rdf:resource="http://purl.org/heritagedata/schemes/eh_tbm/concepts/98026" />
		<skos:related rdf:resource="http://purl.org/heritagedata/schemes/eh_tbm/concepts/98062" />
		<skos:related rdf:resource="http://purl.org/heritagedata/schemes/eh_tbm/concepts/98170" />
		<skos:related rdf:resource="http://purl.org/heritagedata/schemes/eh_tbm/concepts/98195" />
		<skos:related rdf:resource="http://purl.org/heritagedata/schemes/eh_tbm/concepts/98303" />
		<skos:scopeNote xml:lang="en">Originally obtained by burning limestone to produce quicklime. Now a fine grey powder made from a mixture of limestone and clay used with water and sand to make mortar or with water, sand and aggregate to make concrete.</skos:scopeNote>
		<cc:license rdf:resource="http://creativecommons.org/licenses/by/3.0" />
		<cc:attributionURL rdf:resource="http://www.english-heritage.org.uk" />
		<cc:attributionName xml:lang="en">English Heritage</cc:attributionName>
		<dcterms:publisher rdf:resource="http://www.english-heritage.org.uk" />
	</skos:Concept>
	<skos:Concept rdf:about="http://purl.org/heritagedata/schemes/eh_tbm/concepts/97810">
		<skos:inScheme rdf:resource="http://purl.org/heritagedata/schemes/eh_tbm" />
		<dcterms:identifier>http://purl.org/heritagedata/schemes/eh_tbm/concepts/97810</dcterms:identifier>
		<skos:prefLabel xml:lang="en">CEMENT MIX</skos:prefLabel>
		<dcterms:issued rdf:datatype="http://www.w3.org/2001/XMLSchema#dateTime">2013-07-17T09:02:16</dcterms:issued>
		<skos:narrower>
			<skos:Concept rdf:about="http://purl.org/heritagedata/schemes/eh_tbm/concepts/163248">
				<skos:inScheme rdf:resource="http://purl.org/heritagedata/schemes/eh_tbm" />
				<dcterms:identifier>http://purl.org/heritagedata/schemes/eh_tbm/concepts/163248</dcterms:identifier>
				<skos:prefLabel xml:lang="en">BUNGAROOSH</skos:prefLabel>
				<dcterms:issued rdf:datatype="http://www.w3.org/2001/XMLSchema#dateTime">2013-07-17T09:02:16</dcterms:issued>
				<skos:altLabel xml:lang="en">Bungeroosh</skos:altLabel>
				<skos:broader rdf:resource="http://purl.org/heritagedata/schemes/eh_tbm/concepts/97810" />
				<skos:scopeNote xml:lang="en">Composed of a wide variety of substances and materials such as whole or broken bricks, cobblestones, flints, pebbles and sand which are set into hydraulic lime. Used most often to form external walls and is commonly found in the Brighton/Lewes region.</skos:scopeNote>
				<cc:license rdf:resource="http://creativecommons.org/licenses/by/3.0" />
				<cc:attributionURL rdf:resource="http://www.english-heritage.org.uk" />
				<cc:attributionName xml:lang="en">English Heritage</cc:attributionName>
				<dcterms:publisher rdf:resource="http://www.english-heritage.org.uk" />
			</skos:Concept>
		</skos:narrower>
		<skos:narrower rdf:resource="http://purl.org/heritagedata/schemes/eh_tbm/concepts/97809" />
		<skos:broader rdf:resource="http://purl.org/heritagedata/schemes/eh_tbm/concepts/98041" />
		<skos:narrower rdf:resource="http://purl.org/heritagedata/schemes/eh_tbm/concepts/97840" />
		<skos:narrower rdf:resource="http://purl.org/heritagedata/schemes/eh_tbm/concepts/98062" />
		<skos:narrower rdf:resource="http://purl.org/heritagedata/schemes/eh_tbm/concepts/98156" />
		<skos:narrower rdf:resource="http://purl.org/heritagedata/schemes/eh_tbm/concepts/98195" />
		<skos:scopeNote xml:lang="en">A binder combined with various aggregates which sets and holds together into a mass which then hardens and gains strength.</skos:scopeNote>
		<cc:license rdf:resource="http://creativecommons.org/licenses/by/3.0" />
		<cc:attributionURL rdf:resource="http://www.english-heritage.org.uk" />
		<cc:attributionName xml:lang="en">English Heritage</cc:attributionName>
		<dcterms:publisher rdf:resource="http://www.english-heritage.org.uk" />
	</skos:Concept>
	<skos:Concept rdf:about="http://purl.org/heritagedata/schemes/eh_tbm/concepts/97813">
		<skos:inScheme rdf:resource="http://purl.org/heritagedata/schemes/eh_tbm" />
		<dcterms:identifier>http://purl.org/heritagedata/schemes/eh_tbm/concepts/97813</dcterms:identifier>
		<skos:prefLabel xml:lang="en">CERAMIC</skos:prefLabel>
		<dcterms:issued rdf:datatype="http://www.w3.org/2001/XMLSchema#dateTime">2013-07-17T09:02:16</dcterms:issued>
		<skos:broader rdf:resource="http://purl.org/heritagedata/schemes/eh_tbm/concepts/98041" />
		<skos:narrower>
			<skos:Concept rdf:about="http://purl.org/heritagedata/schemes/eh_tbm/concepts/98037">
				<skos:inScheme rdf:resource="http://purl.org/heritagedata/schemes/eh_tbm" />
				<dcterms:identifier>http://purl.org/heritagedata/schemes/eh_tbm/concepts/98037</dcterms:identifier>
				<skos:prefLabel xml:lang="en">MAJOLICA</skos:prefLabel>
				<dcterms:issued rdf:datatype="http://www.w3.org/2001/XMLSchema#dateTime">2013-07-17T09:02:16</dcterms:issued>
				<skos:broader rdf:resource="http://purl.org/heritagedata/schemes/eh_tbm/concepts/97813" />
				<skos:scopeNote xml:lang="en">Fine earthenware with raised patterns of coloured decoration in the form of an enamel or coloured opaque glaze. Use for decorative wall facings.</skos:scopeNote>
				<cc:license rdf:resource="http://creativecommons.org/licenses/by/3.0" />
				<cc:attributionURL rdf:resource="http://www.english-heritage.org.uk" />
				<cc:attributionName xml:lang="en">English Heritage</cc:attributionName>
				<dcterms:publisher rdf:resource="http://www.english-heritage.org.uk" />
			</skos:Concept>
		</skos:narrower>
		<skos:narrower rdf:resource="http://purl.org/heritagedata/schemes/eh_tbm/concepts/98235" />
		<skos:related rdf:resource="http://purl.org/heritagedata/schemes/eh_tbm/concepts/97827" />
		<skos:related rdf:resource="http://purl.org/heritagedata/schemes/eh_tbm/concepts/98241" />
		<skos:scopeNote xml:lang="en">Designating or pertaining to hard, brittle substances produced by strong heating of clay.</skos:scopeNote>
		<cc:license rdf:resource="http://creativecommons.org/licenses/by/3.0" />
		<cc:attributionURL rdf:resource="http://www.english-heritage.org.uk" />
		<cc:attributionName xml:lang="en">English Heritage</cc:attributionName>
		<dcterms:publisher rdf:resource="http://www.english-heritage.org.uk" />
	</skos:Concept>
	<skos:Concept rdf:about="http://purl.org/heritagedata/schemes/eh_tbm/concepts/97814">
		<skos:inScheme rdf:resource="http://purl.org/heritagedata/schemes/eh_tbm" />
		<dcterms:identifier>http://purl.org/heritagedata/schemes/eh_tbm/concepts/97814</dcterms:identifier>
		<skos:prefLabel xml:lang="en">CHALK</skos:prefLabel>
		<dcterms:issued rdf:datatype="http://www.w3.org/2001/XMLSchema#dateTime">2013-07-17T09:02:16</dcterms:issued>
		<skos:altLabel xml:lang="en">Amberley Stone</skos:altLabel>
		<skos:narrower>
			<skos:Concept rdf:about="http://purl.org/heritagedata/schemes/eh_tbm/concepts/97740">
				<skos:inScheme rdf:resource="http://purl.org/heritagedata/schemes/eh_tbm" />
				<dcterms:identifier>http://purl.org/heritagedata/schemes/eh_tbm/concepts/97740</dcterms:identifier>
				<skos:prefLabel xml:lang="en">BEER STONE</skos:prefLabel>
				<dcterms:issued rdf:datatype="http://www.w3.org/2001/XMLSchema#dateTime">2013-07-17T09:02:16</dcterms:issued>
				<skos:broader rdf:resource="http://purl.org/heritagedata/schemes/eh_tbm/concepts/97814" />
				<skos:scopeNote xml:lang="en">Coarse, hard Chalkstone, light grey to white coloured, containing shell fragments.</skos:scopeNote>
				<cc:license rdf:resource="http://creativecommons.org/licenses/by/3.0" />
				<cc:attributionURL rdf:resource="http://www.english-heritage.org.uk" />
				<cc:attributionName xml:lang="en">English Heritage</cc:attributionName>
				<dcterms:publisher rdf:resource="http://www.english-heritage.org.uk" />
			</skos:Concept>
		</skos:narrower>
		<skos:broader rdf:resource="http://purl.org/heritagedata/schemes/eh_tbm/concepts/97866" />
		<skos:narrower>
			<skos:Concept rdf:about="http://purl.org/heritagedata/schemes/eh_tbm/concepts/97833">
				<skos:inScheme rdf:resource="http://purl.org/heritagedata/schemes/eh_tbm" />
				<dcterms:identifier>http://purl.org/heritagedata/schemes/eh_tbm/concepts/97833</dcterms:identifier>
				<skos:prefLabel xml:lang="en">CLUNCH</skos:prefLabel>
				<dcterms:issued rdf:datatype="http://www.w3.org/2001/XMLSchema#dateTime">2013-07-17T09:02:16</dcterms:issued>
				<skos:altLabel xml:lang="en">Totternhoe Stone</skos:altLabel>
				<skos:altLabel xml:lang="en">Burwell Stone</skos:altLabel>
				<skos:broader rdf:resource="http://purl.org/heritagedata/schemes/eh_tbm/concepts/97814" />
				<skos:scopeNote xml:lang="en">A hard, gritty, grey/green coloured form of chalk.</skos:scopeNote>
				<cc:license rdf:resource="http://creativecommons.org/licenses/by/3.0" />
				<cc:attributionURL rdf:resource="http://www.english-heritage.org.uk" />
				<cc:attributionName xml:lang="en">English Heritage</cc:attributionName>
				<dcterms:publisher rdf:resource="http://www.english-heritage.org.uk" />
			</skos:Concept>
		</skos:narrower>
		<skos:scopeNote xml:lang="en">A soft, porous, white to light grey coloured limestone.</skos:scopeNote>
		<cc:license rdf:resource="http://creativecommons.org/licenses/by/3.0" />
		<cc:attributionURL rdf:resource="http://www.english-heritage.org.uk" />
		<cc:attributionName xml:lang="en">English Heritage</cc:attributionName>
		<dcterms:publisher rdf:resource="http://www.english-heritage.org.uk" />
	</skos:Concept>
	<skos:Concept rdf:about="http://purl.org/heritagedata/schemes/eh_tbm/concepts/97821">
		<skos:inScheme rdf:resource="http://purl.org/heritagedata/schemes/eh_tbm" />
		<dcterms:identifier>http://purl.org/heritagedata/schemes/eh_tbm/concepts/97821</dcterms:identifier>
		<skos:prefLabel xml:lang="en">CHERT</skos:prefLabel>
		<dcterms:issued rdf:datatype="http://www.w3.org/2001/XMLSchema#dateTime">2013-07-17T09:02:16</dcterms:issued>
		<skos:altLabel xml:lang="en">Lyddite</skos:altLabel>
		<skos:altLabel xml:lang="en">Knapped Chert</skos:altLabel>
		<skos:broader rdf:resource="http://purl.org/heritagedata/schemes/eh_tbm/concepts/98216" />
		<skos:narrower>
			<skos:Concept rdf:about="http://purl.org/heritagedata/schemes/eh_tbm/concepts/97921">
				<skos:inScheme rdf:resource="http://purl.org/heritagedata/schemes/eh_tbm" />
				<dcterms:identifier>http://purl.org/heritagedata/schemes/eh_tbm/concepts/97921</dcterms:identifier>
				<skos:prefLabel xml:lang="en">FLINT</skos:prefLabel>
				<dcterms:issued rdf:datatype="http://www.w3.org/2001/XMLSchema#dateTime">2013-07-17T09:02:16</dcterms:issued>
				<skos:altLabel xml:lang="en">Knapped Flint</skos:altLabel>
				<skos:broader rdf:resource="http://purl.org/heritagedata/schemes/eh_tbm/concepts/97821" />
				<skos:scopeNote xml:lang="en">Hard, durable, dark grey stone, the purest native form of silica, which can either be used decoratively or as a main material. Predominantly found in East Anglia and the South East.</skos:scopeNote>
				<cc:license rdf:resource="http://creativecommons.org/licenses/by/3.0" />
				<cc:attributionURL rdf:resource="http://www.english-heritage.org.uk" />
				<cc:attributionName xml:lang="en">English Heritage</cc:attributionName>
				<dcterms:publisher rdf:resource="http://www.english-heritage.org.uk" />
			</skos:Concept>
		</skos:narrower>
		<skos:scopeNote xml:lang="en">A hard, silica rich rock, black or brown coloured, commonly found in nodular form.</skos:scopeNote>
		<cc:license rdf:resource="http://creativecommons.org/licenses/by/3.0" />
		<cc:attributionURL rdf:resource="http://www.english-heritage.org.uk" />
		<cc:attributionName xml:lang="en">English Heritage</cc:attributionName>
		<dcterms:publisher rdf:resource="http://www.english-heritage.org.uk" />
	</skos:Concept>
	<skos:Concept rdf:about="http://purl.org/heritagedata/schemes/eh_tbm/concepts/97827">
		<skos:inScheme rdf:resource="http://purl.org/heritagedata/schemes/eh_tbm" />
		<dcterms:identifier>http://purl.org/heritagedata/schemes/eh_tbm/concepts/97827</dcterms:identifier>
		<skos:prefLabel xml:lang="en">CLAY</skos:prefLabel>
		<dcterms:issued rdf:datatype="http://www.w3.org/2001/XMLSchema#dateTime">2013-07-17T09:02:16</dcterms:issued>
		<skos:altLabel xml:lang="en">Clay Tile</skos:altLabel>
		<skos:broader rdf:resource="http://purl.org/heritagedata/schemes/eh_tbm/concepts/97903" />
		<skos:related rdf:resource="http://purl.org/heritagedata/schemes/eh_tbm/concepts/97777" />
		<skos:related rdf:resource="http://purl.org/heritagedata/schemes/eh_tbm/concepts/97813" />
		<skos:related rdf:resource="http://purl.org/heritagedata/schemes/eh_tbm/concepts/98024" />
		<skos:related rdf:resource="http://purl.org/heritagedata/schemes/eh_tbm/concepts/98081" />
		<skos:related rdf:resource="http://purl.org/heritagedata/schemes/eh_tbm/concepts/98241" />
		<skos:scopeNote xml:lang="en">A fine grained earth which becomes more plastic when water is added and can be moulded and dried to make bricks, tile, pottery, etc.</skos:scopeNote>
		<cc:license rdf:resource="http://creativecommons.org/licenses/by/3.0" />
		<cc:attributionURL rdf:resource="http://www.english-heritage.org.uk" />
		<cc:attributionName xml:lang="en">English Heritage</cc:attributionName>
		<dcterms:publisher rdf:resource="http://www.english-heritage.org.uk" />
	</skos:Concept>
	<skos:Concept rdf:about="http://purl.org/heritagedata/schemes/eh_tbm/concepts/97835">
		<skos:inScheme rdf:resource="http://purl.org/heritagedata/schemes/eh_tbm" />
		<dcterms:identifier>http://purl.org/heritagedata/schemes/eh_tbm/concepts/97835</dcterms:identifier>
		<skos:prefLabel xml:lang="en">COB</skos:prefLabel>
		<dcterms:issued rdf:datatype="http://www.w3.org/2001/XMLSchema#dateTime">2013-07-17T09:02:16</dcterms:issued>
		<skos:altLabel xml:lang="en">Clob</skos:altLabel>
		<skos:broader rdf:resource="http://purl.org/heritagedata/schemes/eh_tbm/concepts/97903" />
		<skos:narrower>
			<skos:Concept rdf:about="http://purl.org/heritagedata/schemes/eh_tbm/concepts/98298">
				<skos:inScheme rdf:resource="http://purl.org/heritagedata/schemes/eh_tbm" />
				<dcterms:identifier>http://purl.org/heritagedata/schemes/eh_tbm/concepts/98298</dcterms:identifier>
				<skos:prefLabel xml:lang="en">WICHERT</skos:prefLabel>
				<dcterms:issued rdf:datatype="http://www.w3.org/2001/XMLSchema#dateTime">2013-07-17T09:02:16</dcterms:issued>
				<skos:broader rdf:resource="http://purl.org/heritagedata/schemes/eh_tbm/concepts/97835" />
				<skos:scopeNote xml:lang="en">Cob type construction typical to Buckinghamshire using a local clay with a high chalk content to produce walls of notable inherent stability.</skos:scopeNote>
				<cc:license rdf:resource="http://creativecommons.org/licenses/by/3.0" />
				<cc:attributionURL rdf:resource="http://www.english-heritage.org.uk" />
				<cc:attributionName xml:lang="en">English Heritage</cc:attributionName>
				<dcterms:publisher rdf:resource="http://www.english-heritage.org.uk" />
			</skos:Concept>
		</skos:narrower>
		<skos:scopeNote xml:lang="en">Walls composed of clay, earth, straw, lime and sand, mixed with water. Constructed without shutters in layers upon a stone or brick plinth and usually covered with protective limewash.</skos:scopeNote>
		<cc:license rdf:resource="http://creativecommons.org/licenses/by/3.0" />
		<cc:attributionURL rdf:resource="http://www.english-heritage.org.uk" />
		<cc:attributionName xml:lang="en">English Heritage</cc:attributionName>
		<dcterms:publisher rdf:resource="http://www.english-heritage.org.uk" />
	</skos:Concept>
	<skos:Concept rdf:about="http://purl.org/heritagedata/schemes/eh_tbm/concepts/97704">
		<skos:inScheme rdf:resource="http://purl.org/heritagedata/schemes/eh_tbm" />
		<dcterms:identifier>http://purl.org/heritagedata/schemes/eh_tbm/concepts/97704</dcterms:identifier>
		<skos:prefLabel xml:lang="en">ALABASTER</skos:prefLabel>
		<dcterms:issued rdf:datatype="http://www.w3.org/2001/XMLSchema#dateTime">2013-07-17T09:02:16</dcterms:issued>
		<skos:broader rdf:resource="http://purl.org/heritagedata/schemes/eh_tbm/concepts/98216" />
		<skos:related rdf:resource="http://purl.org/heritagedata/schemes/eh_tbm/concepts/98044" />
		<skos:scopeNote xml:lang="en">Fine grained, whitish, granular variety of Gypsum. Suitable for carving.</skos:scopeNote>
		<cc:license rdf:resource="http://creativecommons.org/licenses/by/3.0" />
		<cc:attributionURL rdf:resource="http://www.english-heritage.org.uk" />
		<cc:attributionName xml:lang="en">English Heritage</cc:attributionName>
		<dcterms:publisher rdf:resource="http://www.english-heritage.org.uk" />
	</skos:Concept>
	<skos:Concept rdf:about="http://purl.org/heritagedata/schemes/eh_tbm/concepts/97708">
		<skos:inScheme rdf:resource="http://purl.org/heritagedata/schemes/eh_tbm" />
		<dcterms:identifier>http://purl.org/heritagedata/schemes/eh_tbm/concepts/97708</dcterms:identifier>
		<skos:prefLabel xml:lang="en">ALUMINIUM</skos:prefLabel>
		<dcterms:issued rdf:datatype="http://www.w3.org/2001/XMLSchema#dateTime">2013-07-17T09:02:16</dcterms:issued>
		<skos:altLabel xml:lang="en">Corrugated Aluminium</skos:altLabel>
		<skos:broader rdf:resource="http://purl.org/heritagedata/schemes/eh_tbm/concepts/98053" />
		<skos:narrower>
			<skos:Concept rdf:about="http://purl.org/heritagedata/schemes/eh_tbm/concepts/97713">
				<skos:inScheme rdf:resource="http://purl.org/heritagedata/schemes/eh_tbm" />
				<dcterms:identifier>http://purl.org/heritagedata/schemes/eh_tbm/concepts/97713</dcterms:identifier>
				<skos:prefLabel xml:lang="en">ANODIZED ALUMINIUM</skos:prefLabel>
				<dcterms:issued rdf:datatype="http://www.w3.org/2001/XMLSchema#dateTime">2013-07-17T09:02:16</dcterms:issued>
				<skos:broader rdf:resource="http://purl.org/heritagedata/schemes/eh_tbm/concepts/97708" />
				<skos:scopeNote xml:lang="en">Aluminium coated by a protective film of oxides created by electrolysis.</skos:scopeNote>
				<cc:license rdf:resource="http://creativecommons.org/licenses/by/3.0" />
				<cc:attributionURL rdf:resource="http://www.english-heritage.org.uk" />
				<cc:attributionName xml:lang="en">English Heritage</cc:attributionName>
				<dcterms:publisher rdf:resource="http://www.english-heritage.org.uk" />
			</skos:Concept>
		</skos:narrower>
		<skos:scopeNote xml:lang="en">Lightweight, strong metal with good corrosive resistance, normally used as an alloy.</skos:scopeNote>
		<cc:license rdf:resource="http://creativecommons.org/licenses/by/3.0" />
		<cc:attributionURL rdf:resource="http://www.english-heritage.org.uk" />
		<cc:attributionName xml:lang="en">English Heritage</cc:attributionName>
		<dcterms:publisher rdf:resource="http://www.english-heritage.org.uk" />
	</skos:Concept>
	<skos:Concept rdf:about="http://purl.org/heritagedata/schemes/eh_tbm/concepts/97717">
		<skos:inScheme rdf:resource="http://purl.org/heritagedata/schemes/eh_tbm" />
		<dcterms:identifier>http://purl.org/heritagedata/schemes/eh_tbm/concepts/97717</dcterms:identifier>
		<skos:prefLabel xml:lang="en">ARTIFICIAL STONE</skos:prefLabel>
		<dcterms:issued rdf:datatype="http://www.w3.org/2001/XMLSchema#dateTime">2013-07-17T09:02:16</dcterms:issued>
		<skos:altLabel xml:lang="en">Bradstone</skos:altLabel>
		<skos:altLabel xml:lang="en">Empire Stone</skos:altLabel>
		<skos:altLabel xml:lang="en">Imitation Stone</skos:altLabel>
		<skos:broader rdf:resource="http://purl.org/heritagedata/schemes/eh_tbm/concepts/98041" />
		<skos:narrower>
			<skos:Concept rdf:about="http://purl.org/heritagedata/schemes/eh_tbm/concepts/97834">
				<skos:inScheme rdf:resource="http://purl.org/heritagedata/schemes/eh_tbm" />
				<dcterms:identifier>http://purl.org/heritagedata/schemes/eh_tbm/concepts/97834</dcterms:identifier>
				<skos:prefLabel xml:lang="en">COADE STONE</skos:prefLabel>
				<dcterms:issued rdf:datatype="http://www.w3.org/2001/XMLSchema#dateTime">2013-07-17T09:02:16</dcterms:issued>
				<skos:broader rdf:resource="http://purl.org/heritagedata/schemes/eh_tbm/concepts/97717" />
				<skos:scopeNote xml:lang="en">Durable artificial stone consisting of china clay, sand and finely ground stoneware cast from moulds and fired in a kiln. Commonly used for architectural ornament and facings.</skos:scopeNote>
				<cc:license rdf:resource="http://creativecommons.org/licenses/by/3.0" />
				<cc:attributionURL rdf:resource="http://www.english-heritage.org.uk" />
				<cc:attributionName xml:lang="en">English Heritage</cc:attributionName>
				<dcterms:publisher rdf:resource="http://www.english-heritage.org.uk" />
			</skos:Concept>
		</skos:narrower>
		<skos:narrower>
			<skos:Concept rdf:about="http://purl.org/heritagedata/schemes/eh_tbm/concepts/98128">
				<skos:inScheme rdf:resource="http://purl.org/heritagedata/schemes/eh_tbm" />
				<dcterms:identifier>http://purl.org/heritagedata/schemes/eh_tbm/concepts/98128</dcterms:identifier>
				<skos:prefLabel xml:lang="en">PULHAMITE STONE</skos:prefLabel>
				<dcterms:issued rdf:datatype="http://www.w3.org/2001/XMLSchema#dateTime">2013-07-17T09:02:16</dcterms:issued>
				<skos:broader rdf:resource="http://purl.org/heritagedata/schemes/eh_tbm/concepts/97717" />
				<skos:scopeNote xml:lang="en">A patented manmade rock invented by James Pulham and Son of Broxbourne. Pulhamite was used to join natural rocks together or crafted to simulate natural stone features. It is an artificial form of sandstone.</skos:scopeNote>
				<cc:license rdf:resource="http://creativecommons.org/licenses/by/3.0" />
				<cc:attributionURL rdf:resource="http://www.english-heritage.org.uk" />
				<cc:attributionName xml:lang="en">English Heritage</cc:attributionName>
				<dcterms:publisher rdf:resource="http://www.english-heritage.org.uk" />
			</skos:Concept>
		</skos:narrower>
		<skos:related rdf:resource="http://purl.org/heritagedata/schemes/eh_tbm/concepts/98174" />
		<skos:related rdf:resource="http://purl.org/heritagedata/schemes/eh_tbm/concepts/98216" />
		<skos:scopeNote xml:lang="en">Synthetically manufactured stone made from natural stone aggregate or reconstituted ceramics or clay, and made to appear natural. Used as solid stone for masonry or for sculptural and architectural ornament.</skos:scopeNote>
		<cc:license rdf:resource="http://creativecommons.org/licenses/by/3.0" />
		<cc:attributionURL rdf:resource="http://www.english-heritage.org.uk" />
		<cc:attributionName xml:lang="en">English Heritage</cc:attributionName>
		<dcterms:publisher rdf:resource="http://www.english-heritage.org.uk" />
	</skos:Concept>
	<skos:Concept rdf:about="http://purl.org/heritagedata/schemes/eh_tbm/concepts/97734">
		<skos:inScheme rdf:resource="http://purl.org/heritagedata/schemes/eh_tbm" />
		<dcterms:identifier>http://purl.org/heritagedata/schemes/eh_tbm/concepts/97734</dcterms:identifier>
		<skos:prefLabel xml:lang="en">BASALT</skos:prefLabel>
		<dcterms:issued rdf:datatype="http://www.w3.org/2001/XMLSchema#dateTime">2013-07-17T09:02:16</dcterms:issued>
		<skos:altLabel xml:lang="en">Volcanic Stone</skos:altLabel>
		<skos:altLabel xml:lang="en">Volcanic Trap</skos:altLabel>
		<skos:altLabel xml:lang="en">Hurdwick Stone</skos:altLabel>
		<skos:altLabel xml:lang="en">Killerton Stone</skos:altLabel>
		<skos:broader rdf:resource="http://purl.org/heritagedata/schemes/eh_tbm/concepts/98216" />
		<skos:related rdf:resource="http://purl.org/heritagedata/schemes/eh_tbm/concepts/97952" />
		<skos:related rdf:resource="http://purl.org/heritagedata/schemes/eh_tbm/concepts/98150" />
		<skos:related rdf:resource="http://purl.org/heritagedata/schemes/eh_tbm/concepts/98181" />
		<skos:related rdf:resource="http://purl.org/heritagedata/schemes/eh_tbm/concepts/98293" />
		<skos:scopeNote xml:lang="en">Basic, black coloured, fine grained, igneous rock.</skos:scopeNote>
		<cc:license rdf:resource="http://creativecommons.org/licenses/by/3.0" />
		<cc:attributionURL rdf:resource="http://www.english-heritage.org.uk" />
		<cc:attributionName xml:lang="en">English Heritage</cc:attributionName>
		<dcterms:publisher rdf:resource="http://www.english-heritage.org.uk" />
	</skos:Concept>
	<skos:Concept rdf:about="http://purl.org/heritagedata/schemes/eh_tbm/concepts/97836">
		<skos:inScheme rdf:resource="http://purl.org/heritagedata/schemes/eh_tbm" />
		<dcterms:identifier>http://purl.org/heritagedata/schemes/eh_tbm/concepts/97836</dcterms:identifier>
		<skos:prefLabel xml:lang="en">COBBLE</skos:prefLabel>
		<dcterms:issued rdf:datatype="http://www.w3.org/2001/XMLSchema#dateTime">2013-07-17T09:02:16</dcterms:issued>
		<skos:broader rdf:resource="http://purl.org/heritagedata/schemes/eh_tbm/concepts/98046" />
		<skos:related rdf:resource="http://purl.org/heritagedata/schemes/eh_tbm/concepts/98216" />
		<skos:scopeNote xml:lang="en">Naturally occurring glacial rock fragments (diameter 64-256mm) larger than pebble and smaller than boulder.</skos:scopeNote>
		<cc:license rdf:resource="http://creativecommons.org/licenses/by/3.0" />
		<cc:attributionURL rdf:resource="http://www.english-heritage.org.uk" />
		<cc:attributionName xml:lang="en">English Heritage</cc:attributionName>
		<dcterms:publisher rdf:resource="http://www.english-heritage.org.uk" />
	</skos:Concept>
	<skos:Concept rdf:about="http://purl.org/heritagedata/schemes/eh_tbm/concepts/97840">
		<skos:inScheme rdf:resource="http://purl.org/heritagedata/schemes/eh_tbm" />
		<dcterms:identifier>http://purl.org/heritagedata/schemes/eh_tbm/concepts/97840</dcterms:identifier>
		<skos:prefLabel xml:lang="en">CONCRETE</skos:prefLabel>
		<dcterms:issued rdf:datatype="http://www.w3.org/2001/XMLSchema#dateTime">2013-07-17T09:02:16</dcterms:issued>
		<skos:altLabel xml:lang="en">Concrete Block</skos:altLabel>
		<skos:altLabel xml:lang="en">Concrete Tile</skos:altLabel>
		<skos:altLabel xml:lang="en">Granolithic Concrete</skos:altLabel>
		<skos:narrower rdf:resource="http://purl.org/heritagedata/schemes/eh_tbm/concepts/97776" />
		<skos:broader rdf:resource="http://purl.org/heritagedata/schemes/eh_tbm/concepts/97810" />
		<skos:narrower>
			<skos:Concept rdf:about="http://purl.org/heritagedata/schemes/eh_tbm/concepts/98025">
				<skos:inScheme rdf:resource="http://purl.org/heritagedata/schemes/eh_tbm" />
				<dcterms:identifier>http://purl.org/heritagedata/schemes/eh_tbm/concepts/98025</dcterms:identifier>
				<skos:prefLabel xml:lang="en">LIGHTWEIGHT CONCRETE</skos:prefLabel>
				<dcterms:issued rdf:datatype="http://www.w3.org/2001/XMLSchema#dateTime">2013-07-17T09:02:16</dcterms:issued>
				<skos:broader rdf:resource="http://purl.org/heritagedata/schemes/eh_tbm/concepts/97840" />
				<skos:scopeNote xml:lang="en">A concrete which is either aerated or made from lightweight aggregate.</skos:scopeNote>
				<cc:license rdf:resource="http://creativecommons.org/licenses/by/3.0" />
				<cc:attributionURL rdf:resource="http://www.english-heritage.org.uk" />
				<cc:attributionName xml:lang="en">English Heritage</cc:attributionName>
				<dcterms:publisher rdf:resource="http://www.english-heritage.org.uk" />
			</skos:Concept>
		</skos:narrower>
		<skos:narrower>
			<skos:Concept rdf:about="http://purl.org/heritagedata/schemes/eh_tbm/concepts/98124">
				<skos:inScheme rdf:resource="http://purl.org/heritagedata/schemes/eh_tbm" />
				<dcterms:identifier>http://purl.org/heritagedata/schemes/eh_tbm/concepts/98124</dcterms:identifier>
				<skos:prefLabel xml:lang="en">PRESTRESSED CONCRETE</skos:prefLabel>
				<dcterms:issued rdf:datatype="http://www.w3.org/2001/XMLSchema#dateTime">2013-07-17T09:02:16</dcterms:issued>
				<skos:broader rdf:resource="http://purl.org/heritagedata/schemes/eh_tbm/concepts/97840" />
				<skos:scopeNote xml:lang="en">Concrete, containing bars or wires, which is compressed to greatly increase its strength.</skos:scopeNote>
				<cc:license rdf:resource="http://creativecommons.org/licenses/by/3.0" />
				<cc:attributionURL rdf:resource="http://www.english-heritage.org.uk" />
				<cc:attributionName xml:lang="en">English Heritage</cc:attributionName>
				<dcterms:publisher rdf:resource="http://www.english-heritage.org.uk" />
			</skos:Concept>
		</skos:narrower>
		<skos:narrower rdf:resource="http://purl.org/heritagedata/schemes/eh_tbm/concepts/98145" />
		<skos:related rdf:resource="http://purl.org/heritagedata/schemes/eh_tbm/concepts/97809" />
		<skos:related rdf:resource="http://purl.org/heritagedata/schemes/eh_tbm/concepts/98081" />
		<skos:related rdf:resource="http://purl.org/heritagedata/schemes/eh_tbm/concepts/98170" />
		<skos:related rdf:resource="http://purl.org/heritagedata/schemes/eh_tbm/concepts/98241" />
		<skos:scopeNote xml:lang="en">Composed of sand, stones or other aggregate and cement mixed with water which sets in a hard mass. The material is usually associated with modern building but was developed by Romans where cement was obtained from quicklime.</skos:scopeNote>
		<cc:license rdf:resource="http://creativecommons.org/licenses/by/3.0" />
		<cc:attributionURL rdf:resource="http://www.english-heritage.org.uk" />
		<cc:attributionName xml:lang="en">English Heritage</cc:attributionName>
		<dcterms:publisher rdf:resource="http://www.english-heritage.org.uk" />
	</skos:Concept>
	<skos:Concept rdf:about="http://purl.org/heritagedata/schemes/eh_tbm/concepts/97843">
		<skos:inScheme rdf:resource="http://purl.org/heritagedata/schemes/eh_tbm" />
		<dcterms:identifier>http://purl.org/heritagedata/schemes/eh_tbm/concepts/97843</dcterms:identifier>
		<skos:prefLabel xml:lang="en">CONGLOMERATE</skos:prefLabel>
		<dcterms:issued rdf:datatype="http://www.w3.org/2001/XMLSchema#dateTime">2013-07-17T09:02:16</dcterms:issued>
		<skos:altLabel xml:lang="en">Brandon Hill Grit Rubble</skos:altLabel>
		<skos:altLabel xml:lang="en">Dolomitic Conglomerate</skos:altLabel>
		<skos:broader rdf:resource="http://purl.org/heritagedata/schemes/eh_tbm/concepts/98216" />
		<skos:narrower rdf:resource="http://purl.org/heritagedata/schemes/eh_tbm/concepts/98126" />
		<skos:narrower rdf:resource="http://purl.org/heritagedata/schemes/eh_tbm/concepts/98180" />
		<skos:related rdf:resource="http://purl.org/heritagedata/schemes/eh_tbm/concepts/97774" />
		<skos:scopeNote xml:lang="en">Sedimentary rock consisting of rounded pebbles naturally cemented together.</skos:scopeNote>
		<cc:license rdf:resource="http://creativecommons.org/licenses/by/3.0" />
		<cc:attributionURL rdf:resource="http://www.english-heritage.org.uk" />
		<cc:attributionName xml:lang="en">English Heritage</cc:attributionName>
		<dcterms:publisher rdf:resource="http://www.english-heritage.org.uk" />
	</skos:Concept>
	<skos:Concept rdf:about="http://purl.org/heritagedata/schemes/eh_tbm/concepts/97844">
		<skos:inScheme rdf:resource="http://purl.org/heritagedata/schemes/eh_tbm" />
		<dcterms:identifier>http://purl.org/heritagedata/schemes/eh_tbm/concepts/97844</dcterms:identifier>
		<skos:prefLabel xml:lang="en">CONNEMARA MARBLE</skos:prefLabel>
		<dcterms:issued rdf:datatype="http://www.w3.org/2001/XMLSchema#dateTime">2013-07-17T09:02:16</dcterms:issued>
		<skos:broader rdf:resource="http://purl.org/heritagedata/schemes/eh_tbm/concepts/98044" />
		<skos:related rdf:resource="http://purl.org/heritagedata/schemes/eh_tbm/concepts/98181" />
		<skos:scopeNote xml:lang="en">One of only three 'true' British marbles, green and white in colour, predominantly used in large public buildings.</skos:scopeNote>
		<cc:license rdf:resource="http://creativecommons.org/licenses/by/3.0" />
		<cc:attributionURL rdf:resource="http://www.english-heritage.org.uk" />
		<cc:attributionName xml:lang="en">English Heritage</cc:attributionName>
		<dcterms:publisher rdf:resource="http://www.english-heritage.org.uk" />
	</skos:Concept>
	<skos:Concept rdf:about="http://purl.org/heritagedata/schemes/eh_tbm/concepts/97845">
		<skos:inScheme rdf:resource="http://purl.org/heritagedata/schemes/eh_tbm" />
		<dcterms:identifier>http://purl.org/heritagedata/schemes/eh_tbm/concepts/97845</dcterms:identifier>
		<skos:prefLabel xml:lang="en">COPPER</skos:prefLabel>
		<dcterms:issued rdf:datatype="http://www.w3.org/2001/XMLSchema#dateTime">2013-07-17T09:02:16</dcterms:issued>
		<skos:broader rdf:resource="http://purl.org/heritagedata/schemes/eh_tbm/concepts/98053" />
		<skos:related rdf:resource="http://purl.org/heritagedata/schemes/eh_tbm/concepts/97779" />
		<skos:scopeNote xml:lang="en">Metal used primarily for roofing and ornamental purposes, being lighter and stronger than lead.</skos:scopeNote>
		<cc:license rdf:resource="http://creativecommons.org/licenses/by/3.0" />
		<cc:attributionURL rdf:resource="http://www.english-heritage.org.uk" />
		<cc:attributionName xml:lang="en">English Heritage</cc:attributionName>
		<dcterms:publisher rdf:resource="http://www.english-heritage.org.uk" />
	</skos:Concept>
	<skos:Concept rdf:about="http://purl.org/heritagedata/schemes/eh_tbm/concepts/97866">
		<skos:inScheme rdf:resource="http://purl.org/heritagedata/schemes/eh_tbm" />
		<dcterms:identifier>http://purl.org/heritagedata/schemes/eh_tbm/concepts/97866</dcterms:identifier>
		<skos:prefLabel xml:lang="en">CRETACEOUS LIMESTONE</skos:prefLabel>
		<dcterms:issued rdf:datatype="http://www.w3.org/2001/XMLSchema#dateTime">2013-07-17T09:02:16</dcterms:issued>
		<skos:altLabel xml:lang="en">Petworth Marble</skos:altLabel>
		<skos:altLabel xml:lang="en">Large Paludina Marble</skos:altLabel>
		<skos:altLabel xml:lang="en">Laughton Marble</skos:altLabel>
		<skos:altLabel xml:lang="en">Laughton Stone</skos:altLabel>
		<skos:altLabel xml:lang="en">Small Paludina Marble</skos:altLabel>
		<skos:altLabel xml:lang="en">Sussex Marble</skos:altLabel>
		<skos:altLabel xml:lang="en">Bethersden Marble</skos:altLabel>
		<skos:altLabel xml:lang="en">Charlwood Stone</skos:altLabel>
		<skos:altLabel xml:lang="en">Istrian Stone</skos:altLabel>
		<skos:narrower>
			<skos:Concept rdf:about="http://purl.org/heritagedata/schemes/eh_tbm/concepts/97788">
				<skos:inScheme rdf:resource="http://purl.org/heritagedata/schemes/eh_tbm" />
				<dcterms:identifier>http://purl.org/heritagedata/schemes/eh_tbm/concepts/97788</dcterms:identifier>
				<skos:prefLabel xml:lang="en">CAEN STONE</skos:prefLabel>
				<dcterms:issued rdf:datatype="http://www.w3.org/2001/XMLSchema#dateTime">2013-07-17T09:02:16</dcterms:issued>
				<skos:broader rdf:resource="http://purl.org/heritagedata/schemes/eh_tbm/concepts/97866" />
				<skos:scopeNote xml:lang="en">Fine grained limestone, yellow or yellow/white in colour. Imported from France, mainly for ecclesiastical use.</skos:scopeNote>
				<cc:license rdf:resource="http://creativecommons.org/licenses/by/3.0" />
				<cc:attributionURL rdf:resource="http://www.english-heritage.org.uk" />
				<cc:attributionName xml:lang="en">English Heritage</cc:attributionName>
				<dcterms:publisher rdf:resource="http://www.english-heritage.org.uk" />
			</skos:Concept>
		</skos:narrower>
		<skos:narrower rdf:resource="http://purl.org/heritagedata/schemes/eh_tbm/concepts/97814" />
		<skos:broader rdf:resource="http://purl.org/heritagedata/schemes/eh_tbm/concepts/98028" />
		<skos:narrower>
			<skos:Concept rdf:about="http://purl.org/heritagedata/schemes/eh_tbm/concepts/98003">
				<skos:inScheme rdf:resource="http://purl.org/heritagedata/schemes/eh_tbm" />
				<dcterms:identifier>http://purl.org/heritagedata/schemes/eh_tbm/concepts/98003</dcterms:identifier>
				<skos:prefLabel xml:lang="en">KENTISH RAGSTONE</skos:prefLabel>
				<dcterms:issued rdf:datatype="http://www.w3.org/2001/XMLSchema#dateTime">2013-07-17T09:02:16</dcterms:issued>
				<skos:altLabel xml:lang="en">Tonbridge Stone</skos:altLabel>
				<skos:altLabel xml:lang="en">Kentish Rag</skos:altLabel>
				<skos:broader rdf:resource="http://purl.org/heritagedata/schemes/eh_tbm/concepts/97866" />
				<skos:scopeNote xml:lang="en">Sandy, rough blue to green/grey coloured limestone. Quarried in Kent and widely used throughout the South East.</skos:scopeNote>
				<cc:license rdf:resource="http://creativecommons.org/licenses/by/3.0" />
				<cc:attributionURL rdf:resource="http://www.english-heritage.org.uk" />
				<cc:attributionName xml:lang="en">English Heritage</cc:attributionName>
				<dcterms:publisher rdf:resource="http://www.english-heritage.org.uk" />
			</skos:Concept>
		</skos:narrower>
		<skos:related rdf:resource="http://purl.org/heritagedata/schemes/eh_tbm/concepts/98223" />
		<skos:scopeNote xml:lang="en">Limestone formed during the Cretaceous period.</skos:scopeNote>
		<cc:license rdf:resource="http://creativecommons.org/licenses/by/3.0" />
		<cc:attributionURL rdf:resource="http://www.english-heritage.org.uk" />
		<cc:attributionName xml:lang="en">English Heritage</cc:attributionName>
		<dcterms:publisher rdf:resource="http://www.english-heritage.org.uk" />
	</skos:Concept>
	<skos:Concept rdf:about="http://purl.org/heritagedata/schemes/eh_tbm/concepts/97873">
		<skos:inScheme rdf:resource="http://purl.org/heritagedata/schemes/eh_tbm" />
		<dcterms:identifier>http://purl.org/heritagedata/schemes/eh_tbm/concepts/97873</dcterms:identifier>
		<skos:prefLabel xml:lang="en">DAUB</skos:prefLabel>
		<dcterms:issued rdf:datatype="http://www.w3.org/2001/XMLSchema#dateTime">2013-07-17T09:02:16</dcterms:issued>
		<skos:broader rdf:resource="http://purl.org/heritagedata/schemes/eh_tbm/concepts/97903" />
		<skos:related rdf:resource="http://purl.org/heritagedata/schemes/eh_tbm/concepts/98018" />
		<skos:related rdf:resource="http://purl.org/heritagedata/schemes/eh_tbm/concepts/98026" />
		<skos:related rdf:resource="http://purl.org/heritagedata/schemes/eh_tbm/concepts/98110" />
		<skos:related rdf:resource="http://purl.org/heritagedata/schemes/eh_tbm/concepts/98276" />
		<skos:scopeNote xml:lang="en">Application of earth based plaster to a backing of lath or wattle used in internal or external walls. Composite mixture which may include clay soil, dung, straw, lime putty, sand or horsehair.</skos:scopeNote>
		<cc:license rdf:resource="http://creativecommons.org/licenses/by/3.0" />
		<cc:attributionURL rdf:resource="http://www.english-heritage.org.uk" />
		<cc:attributionName xml:lang="en">English Heritage</cc:attributionName>
		<dcterms:publisher rdf:resource="http://www.english-heritage.org.uk" />
	</skos:Concept>
	<skos:Concept rdf:about="http://purl.org/heritagedata/schemes/eh_tbm/concepts/97876">
		<skos:inScheme rdf:resource="http://purl.org/heritagedata/schemes/eh_tbm" />
		<dcterms:identifier>http://purl.org/heritagedata/schemes/eh_tbm/concepts/97876</dcterms:identifier>
		<skos:prefLabel xml:lang="en">DECORATIVE PLASTER</skos:prefLabel>
		<dcterms:issued rdf:datatype="http://www.w3.org/2001/XMLSchema#dateTime">2013-07-17T09:02:16</dcterms:issued>
		<skos:broader rdf:resource="http://purl.org/heritagedata/schemes/eh_tbm/concepts/98046" />
		<skos:broader rdf:resource="http://purl.org/heritagedata/schemes/eh_tbm/concepts/98110" />
		<skos:narrower>
			<skos:Concept rdf:about="http://purl.org/heritagedata/schemes/eh_tbm/concepts/98083">
				<skos:inScheme rdf:resource="http://purl.org/heritagedata/schemes/eh_tbm" />
				<dcterms:identifier>http://purl.org/heritagedata/schemes/eh_tbm/concepts/98083</dcterms:identifier>
				<skos:prefLabel xml:lang="en">PARGETING</skos:prefLabel>
				<dcterms:issued rdf:datatype="http://www.w3.org/2001/XMLSchema#dateTime">2013-07-17T09:02:16</dcterms:issued>
				<skos:altLabel xml:lang="en">Pargetting</skos:altLabel>
				<skos:broader rdf:resource="http://purl.org/heritagedata/schemes/eh_tbm/concepts/97876" />
				<skos:scopeNote xml:lang="en">External decorative plasterwork often incised or modelled with ornamental patterns. Usually applied to timber-framed houses, especially during 16th and 17th centuries.</skos:scopeNote>
				<cc:license rdf:resource="http://creativecommons.org/licenses/by/3.0" />
				<cc:attributionURL rdf:resource="http://www.english-heritage.org.uk" />
				<cc:attributionName xml:lang="en">English Heritage</cc:attributionName>
				<dcterms:publisher rdf:resource="http://www.english-heritage.org.uk" />
			</skos:Concept>
		</skos:narrower>
		<skos:narrower rdf:resource="http://purl.org/heritagedata/schemes/eh_tbm/concepts/98174" />
		<skos:scopeNote xml:lang="en">Ornate or patterned decoration, carved into or moulded from plaster.</skos:scopeNote>
		<cc:license rdf:resource="http://creativecommons.org/licenses/by/3.0" />
		<cc:attributionURL rdf:resource="http://www.english-heritage.org.uk" />
		<cc:attributionName xml:lang="en">English Heritage</cc:attributionName>
		<dcterms:publisher rdf:resource="http://www.english-heritage.org.uk" />
	</skos:Concept>
	<skos:Concept rdf:about="http://purl.org/heritagedata/schemes/eh_tbm/concepts/97891">
		<skos:inScheme rdf:resource="http://purl.org/heritagedata/schemes/eh_tbm" />
		<dcterms:identifier>http://purl.org/heritagedata/schemes/eh_tbm/concepts/97891</dcterms:identifier>
		<skos:prefLabel xml:lang="en">DOLERITE</skos:prefLabel>
		<dcterms:issued rdf:datatype="http://www.w3.org/2001/XMLSchema#dateTime">2013-07-17T09:02:16</dcterms:issued>
		<skos:broader rdf:resource="http://purl.org/heritagedata/schemes/eh_tbm/concepts/98216" />
		<skos:related rdf:resource="http://purl.org/heritagedata/schemes/eh_tbm/concepts/97952" />
		<skos:related rdf:resource="http://purl.org/heritagedata/schemes/eh_tbm/concepts/98150" />
		<skos:related rdf:resource="http://purl.org/heritagedata/schemes/eh_tbm/concepts/98293" />
		<skos:scopeNote xml:lang="en">Medium grained, intrusive, black or dark green coloured, igneous rock.</skos:scopeNote>
		<cc:license rdf:resource="http://creativecommons.org/licenses/by/3.0" />
		<cc:attributionURL rdf:resource="http://www.english-heritage.org.uk" />
		<cc:attributionName xml:lang="en">English Heritage</cc:attributionName>
		<dcterms:publisher rdf:resource="http://www.english-heritage.org.uk" />
	</skos:Concept>
	<skos:Concept rdf:about="http://purl.org/heritagedata/schemes/eh_tbm/concepts/97892">
		<skos:inScheme rdf:resource="http://purl.org/heritagedata/schemes/eh_tbm" />
		<dcterms:identifier>http://purl.org/heritagedata/schemes/eh_tbm/concepts/97892</dcterms:identifier>
		<skos:prefLabel xml:lang="en">DOLOMITE</skos:prefLabel>
		<dcterms:issued rdf:datatype="http://www.w3.org/2001/XMLSchema#dateTime">2013-07-17T09:02:16</dcterms:issued>
		<skos:altLabel xml:lang="en">Dolomitic Conglomerate</skos:altLabel>
		<skos:broader rdf:resource="http://purl.org/heritagedata/schemes/eh_tbm/concepts/98058" />
		<skos:related rdf:resource="http://purl.org/heritagedata/schemes/eh_tbm/concepts/98036" />
		<skos:scopeNote xml:lang="en">Soft, often white, but may be transparent. Dolomite can be found on its own, but may also occur as a replacement mineral found in some rocks, particularly limestone, formed after action by magnesium-rich fluids.</skos:scopeNote>
		<cc:license rdf:resource="http://creativecommons.org/licenses/by/3.0" />
		<cc:attributionURL rdf:resource="http://www.english-heritage.org.uk" />
		<cc:attributionName xml:lang="en">English Heritage</cc:attributionName>
		<dcterms:publisher rdf:resource="http://www.english-heritage.org.uk" />
	</skos:Concept>
	<skos:Concept rdf:about="http://purl.org/heritagedata/schemes/eh_tbm/concepts/97902">
		<skos:inScheme rdf:resource="http://purl.org/heritagedata/schemes/eh_tbm" />
		<dcterms:identifier>http://purl.org/heritagedata/schemes/eh_tbm/concepts/97902</dcterms:identifier>
		<skos:prefLabel xml:lang="en">EARTH</skos:prefLabel>
		<dcterms:issued rdf:datatype="http://www.w3.org/2001/XMLSchema#dateTime">2013-07-17T09:02:16</dcterms:issued>
		<skos:broader rdf:resource="http://purl.org/heritagedata/schemes/eh_tbm/concepts/97903" />
		<skos:related rdf:resource="http://purl.org/heritagedata/schemes/eh_tbm/concepts/98087" />
		<skos:related rdf:resource="http://purl.org/heritagedata/schemes/eh_tbm/concepts/98262" />
		<skos:scopeNote xml:lang="en">Combination of organic and inorganic material cohered to form a hard solid wall or covering. Use for structures created by the excavation and piling up of earth, such as ice houses. Earth may be used in combination with other materials.</skos:scopeNote>
		<cc:license rdf:resource="http://creativecommons.org/licenses/by/3.0" />
		<cc:attributionURL rdf:resource="http://www.english-heritage.org.uk" />
		<cc:attributionName xml:lang="en">English Heritage</cc:attributionName>
		<dcterms:publisher rdf:resource="http://www.english-heritage.org.uk" />
	</skos:Concept>
	<skos:Concept rdf:about="http://purl.org/heritagedata/schemes/eh_tbm/concepts/97908">
		<skos:inScheme rdf:resource="http://purl.org/heritagedata/schemes/eh_tbm" />
		<dcterms:identifier>http://purl.org/heritagedata/schemes/eh_tbm/concepts/97908</dcterms:identifier>
		<skos:prefLabel xml:lang="en">ELVAN</skos:prefLabel>
		<dcterms:issued rdf:datatype="http://www.w3.org/2001/XMLSchema#dateTime">2013-07-17T09:02:16</dcterms:issued>
		<skos:altLabel xml:lang="en">Pentewan Stone</skos:altLabel>
		<skos:altLabel xml:lang="en">Trerice Porphry</skos:altLabel>
		<skos:altLabel xml:lang="en">Trerice Stone</skos:altLabel>
		<skos:altLabel xml:lang="en">Catacleuse</skos:altLabel>
		<skos:altLabel xml:lang="en">Growan</skos:altLabel>
		<skos:broader rdf:resource="http://purl.org/heritagedata/schemes/eh_tbm/concepts/102688" />
		<skos:related rdf:resource="http://purl.org/heritagedata/schemes/eh_tbm/concepts/97944" />
		<skos:scopeNote xml:lang="en">Miner's term for fine grained, often light grey/fawn coloured porphyritic rocks. Commonly found in Devon and Cornwall.</skos:scopeNote>
		<cc:license rdf:resource="http://creativecommons.org/licenses/by/3.0" />
		<cc:attributionURL rdf:resource="http://www.english-heritage.org.uk" />
		<cc:attributionName xml:lang="en">English Heritage</cc:attributionName>
		<dcterms:publisher rdf:resource="http://www.english-heritage.org.uk" />
	</skos:Concept>
	<skos:Concept rdf:about="http://purl.org/heritagedata/schemes/eh_tbm/concepts/97914">
		<skos:inScheme rdf:resource="http://purl.org/heritagedata/schemes/eh_tbm" />
		<dcterms:identifier>http://purl.org/heritagedata/schemes/eh_tbm/concepts/97914</dcterms:identifier>
		<skos:prefLabel xml:lang="en">FAIENCE</skos:prefLabel>
		<dcterms:issued rdf:datatype="http://www.w3.org/2001/XMLSchema#dateTime">2013-07-17T09:02:16</dcterms:issued>
		<skos:altLabel xml:lang="en">Marmo</skos:altLabel>
		<skos:broader rdf:resource="http://purl.org/heritagedata/schemes/eh_tbm/concepts/98235" />
		<skos:related rdf:resource="http://purl.org/heritagedata/schemes/eh_tbm/concepts/98241" />
		<skos:scopeNote xml:lang="en">Solid masonry slabs (tiles) of terracotta which are usually used as a cladding by bedding in concrete. Faience also refers to decorative glazed units.</skos:scopeNote>
		<cc:license rdf:resource="http://creativecommons.org/licenses/by/3.0" />
		<cc:attributionURL rdf:resource="http://www.english-heritage.org.uk" />
		<cc:attributionName xml:lang="en">English Heritage</cc:attributionName>
		<dcterms:publisher rdf:resource="http://www.english-heritage.org.uk" />
	</skos:Concept>
	<skos:Concept rdf:about="http://purl.org/heritagedata/schemes/eh_tbm/concepts/97917">
		<skos:inScheme rdf:resource="http://purl.org/heritagedata/schemes/eh_tbm" />
		<dcterms:identifier>http://purl.org/heritagedata/schemes/eh_tbm/concepts/97917</dcterms:identifier>
		<skos:prefLabel xml:lang="en">FIBREBOARD</skos:prefLabel>
		<dcterms:issued rdf:datatype="http://www.w3.org/2001/XMLSchema#dateTime">2013-07-17T09:02:16</dcterms:issued>
		<skos:altLabel xml:lang="en">Medium Board</skos:altLabel>
		<skos:altLabel xml:lang="en">Medium Density Fibreboard</skos:altLabel>
		<skos:altLabel xml:lang="en">Hardboard</skos:altLabel>
		<skos:broader rdf:resource="http://purl.org/heritagedata/schemes/eh_tbm/concepts/98080" />
		<skos:related rdf:resource="http://purl.org/heritagedata/schemes/eh_tbm/concepts/98301" />
		<skos:scopeNote xml:lang="en">A sheet formed from wood which has been separated into its fibrous elements and reconstituted under pressure. The natural fibres produce resins which act as adhesive, but often additional adhesives are used.</skos:scopeNote>
		<cc:license rdf:resource="http://creativecommons.org/licenses/by/3.0" />
		<cc:attributionURL rdf:resource="http://www.english-heritage.org.uk" />
		<cc:attributionName xml:lang="en">English Heritage</cc:attributionName>
		<dcterms:publisher rdf:resource="http://www.english-heritage.org.uk" />
	</skos:Concept>
	<skos:Concept rdf:about="http://purl.org/heritagedata/schemes/eh_tbm/concepts/97919">
		<skos:inScheme rdf:resource="http://purl.org/heritagedata/schemes/eh_tbm" />
		<dcterms:identifier>http://purl.org/heritagedata/schemes/eh_tbm/concepts/97919</dcterms:identifier>
		<skos:prefLabel xml:lang="en">FIRESTONE</skos:prefLabel>
		<dcterms:issued rdf:datatype="http://www.w3.org/2001/XMLSchema#dateTime">2013-07-17T09:02:16</dcterms:issued>
		<skos:broader rdf:resource="http://purl.org/heritagedata/schemes/eh_tbm/concepts/98171" />
		<skos:related rdf:resource="http://purl.org/heritagedata/schemes/eh_tbm/concepts/97993" />
		<skos:scopeNote xml:lang="en">Soft sandstone stained by iron oxide often used in the Surrey area.</skos:scopeNote>
		<cc:license rdf:resource="http://creativecommons.org/licenses/by/3.0" />
		<cc:attributionURL rdf:resource="http://www.english-heritage.org.uk" />
		<cc:attributionName xml:lang="en">English Heritage</cc:attributionName>
		<dcterms:publisher rdf:resource="http://www.english-heritage.org.uk" />
	</skos:Concept>
	<skos:Concept rdf:about="http://purl.org/heritagedata/schemes/eh_tbm/concepts/97928">
		<skos:inScheme rdf:resource="http://purl.org/heritagedata/schemes/eh_tbm" />
		<dcterms:identifier>http://purl.org/heritagedata/schemes/eh_tbm/concepts/97928</dcterms:identifier>
		<skos:prefLabel xml:lang="en">FOREST STONE (LEICESTERSHIRE)</skos:prefLabel>
		<dcterms:issued rdf:datatype="http://www.w3.org/2001/XMLSchema#dateTime">2013-07-17T09:02:16</dcterms:issued>
		<skos:altLabel xml:lang="en">Swithland Slate</skos:altLabel>
		<skos:altLabel xml:lang="en">Charnwood Stone</skos:altLabel>
		<skos:broader rdf:resource="http://purl.org/heritagedata/schemes/eh_tbm/concepts/98216" />
		<skos:related rdf:resource="http://purl.org/heritagedata/schemes/eh_tbm/concepts/102688" />
		<skos:related rdf:resource="http://purl.org/heritagedata/schemes/eh_tbm/concepts/98179" />
		<skos:related rdf:resource="http://purl.org/heritagedata/schemes/eh_tbm/concepts/98194" />
		<skos:related rdf:resource="http://purl.org/heritagedata/schemes/eh_tbm/concepts/98229" />
		<skos:scopeNote xml:lang="en">Collective name for a series of rocks (granite, syenite, porphry and slate) found in the Charnwood Forest of Leicestershire. Index with specific stone type where given.</skos:scopeNote>
		<cc:license rdf:resource="http://creativecommons.org/licenses/by/3.0" />
		<cc:attributionURL rdf:resource="http://www.english-heritage.org.uk" />
		<cc:attributionName xml:lang="en">English Heritage</cc:attributionName>
		<dcterms:publisher rdf:resource="http://www.english-heritage.org.uk" />
	</skos:Concept>
	<skos:Concept rdf:about="http://purl.org/heritagedata/schemes/eh_tbm/concepts/97929">
		<skos:inScheme rdf:resource="http://purl.org/heritagedata/schemes/eh_tbm" />
		<dcterms:identifier>http://purl.org/heritagedata/schemes/eh_tbm/concepts/97929</dcterms:identifier>
		<skos:prefLabel xml:lang="en">FOSSIL</skos:prefLabel>
		<dcterms:issued rdf:datatype="http://www.w3.org/2001/XMLSchema#dateTime">2013-07-17T09:02:16</dcterms:issued>
		<skos:altLabel xml:lang="en">Ammonite</skos:altLabel>
		<skos:broader rdf:resource="http://purl.org/heritagedata/schemes/eh_tbm/concepts/97712" />
		<skos:related rdf:resource="http://purl.org/heritagedata/schemes/eh_tbm/concepts/98058" />
		<skos:related rdf:resource="http://purl.org/heritagedata/schemes/eh_tbm/concepts/98216" />
		<skos:scopeNote xml:lang="en">The remains of living organisms preserved in stone over a long time period. This may be the internal or external moulds of, usually, the hard parts of an organism (shells, bones, etc.).</skos:scopeNote>
		<cc:license rdf:resource="http://creativecommons.org/licenses/by/3.0" />
		<cc:attributionURL rdf:resource="http://www.english-heritage.org.uk" />
		<cc:attributionName xml:lang="en">English Heritage</cc:attributionName>
		<dcterms:publisher rdf:resource="http://www.english-heritage.org.uk" />
	</skos:Concept>
	<skos:Concept rdf:about="http://purl.org/heritagedata/schemes/eh_tbm/concepts/97939">
		<skos:inScheme rdf:resource="http://purl.org/heritagedata/schemes/eh_tbm" />
		<dcterms:identifier>http://purl.org/heritagedata/schemes/eh_tbm/concepts/97939</dcterms:identifier>
		<skos:prefLabel xml:lang="en">GLASS</skos:prefLabel>
		<dcterms:issued rdf:datatype="http://www.w3.org/2001/XMLSchema#dateTime">2013-07-17T09:02:16</dcterms:issued>
		<skos:broader rdf:resource="http://purl.org/heritagedata/schemes/eh_tbm/concepts/98041" />
		<skos:narrower>
			<skos:Concept rdf:about="http://purl.org/heritagedata/schemes/eh_tbm/concepts/98197">
				<skos:inScheme rdf:resource="http://purl.org/heritagedata/schemes/eh_tbm" />
				<dcterms:identifier>http://purl.org/heritagedata/schemes/eh_tbm/concepts/98197</dcterms:identifier>
				<skos:prefLabel xml:lang="en">SOLAR CONTROL GLASS</skos:prefLabel>
				<dcterms:issued rdf:datatype="http://www.w3.org/2001/XMLSchema#dateTime">2013-07-17T09:02:16</dcterms:issued>
				<skos:broader rdf:resource="http://purl.org/heritagedata/schemes/eh_tbm/concepts/97939" />
				<skos:scopeNote xml:lang="en">Glass to control or reduce the effects of the sun, includes both reflective and absorpative types of glass.</skos:scopeNote>
				<cc:license rdf:resource="http://creativecommons.org/licenses/by/3.0" />
				<cc:attributionURL rdf:resource="http://www.english-heritage.org.uk" />
				<cc:attributionName xml:lang="en">English Heritage</cc:attributionName>
				<dcterms:publisher rdf:resource="http://www.english-heritage.org.uk" />
			</skos:Concept>
		</skos:narrower>
		<skos:scopeNote xml:lang="en">Transparent, hard substance made by fusing soda-silica which solidifies from a molten state.</skos:scopeNote>
		<cc:license rdf:resource="http://creativecommons.org/licenses/by/3.0" />
		<cc:attributionURL rdf:resource="http://www.english-heritage.org.uk" />
		<cc:attributionName xml:lang="en">English Heritage</cc:attributionName>
		<dcterms:publisher rdf:resource="http://www.english-heritage.org.uk" />
	</skos:Concept>
	<skos:Concept rdf:about="http://purl.org/heritagedata/schemes/eh_tbm/concepts/97940">
		<skos:inScheme rdf:resource="http://purl.org/heritagedata/schemes/eh_tbm" />
		<dcterms:identifier>http://purl.org/heritagedata/schemes/eh_tbm/concepts/97940</dcterms:identifier>
		<skos:prefLabel xml:lang="en">GNEISS</skos:prefLabel>
		<dcterms:issued rdf:datatype="http://www.w3.org/2001/XMLSchema#dateTime">2013-07-17T09:02:16</dcterms:issued>
		<skos:altLabel xml:lang="en">Madreperla</skos:altLabel>
		<skos:altLabel xml:lang="en">Verde Ematita</skos:altLabel>
		<skos:altLabel xml:lang="en">Alps Grey Granite</skos:altLabel>
		<skos:altLabel xml:lang="en">Ematita Granite</skos:altLabel>
		<skos:broader rdf:resource="http://purl.org/heritagedata/schemes/eh_tbm/concepts/98216" />
		<skos:related rdf:resource="http://purl.org/heritagedata/schemes/eh_tbm/concepts/97944" />
		<skos:scopeNote xml:lang="en">Coarse grained, metamorphic rock in which the colour is dependent upon the predominant mineral.</skos:scopeNote>
		<cc:license rdf:resource="http://creativecommons.org/licenses/by/3.0" />
		<cc:attributionURL rdf:resource="http://www.english-heritage.org.uk" />
		<cc:attributionName xml:lang="en">English Heritage</cc:attributionName>
		<dcterms:publisher rdf:resource="http://www.english-heritage.org.uk" />
	</skos:Concept>
	<skos:Concept rdf:about="http://purl.org/heritagedata/schemes/eh_tbm/concepts/97943">
		<skos:inScheme rdf:resource="http://purl.org/heritagedata/schemes/eh_tbm" />
		<dcterms:identifier>http://purl.org/heritagedata/schemes/eh_tbm/concepts/97943</dcterms:identifier>
		<skos:prefLabel xml:lang="en">GORSE</skos:prefLabel>
		<dcterms:issued rdf:datatype="http://www.w3.org/2001/XMLSchema#dateTime">2013-07-17T09:02:16</dcterms:issued>
		<skos:broader rdf:resource="http://purl.org/heritagedata/schemes/eh_tbm/concepts/98109" />
		<skos:related rdf:resource="http://purl.org/heritagedata/schemes/eh_tbm/concepts/98239" />
		<skos:scopeNote xml:lang="en">A spiny evergreen shrub of the pea family which can be utilized as a roof covering in areas of its predominance, eg. heathland.</skos:scopeNote>
		<cc:license rdf:resource="http://creativecommons.org/licenses/by/3.0" />
		<cc:attributionURL rdf:resource="http://www.english-heritage.org.uk" />
		<cc:attributionName xml:lang="en">English Heritage</cc:attributionName>
		<dcterms:publisher rdf:resource="http://www.english-heritage.org.uk" />
	</skos:Concept>
	<skos:Concept rdf:about="http://purl.org/heritagedata/schemes/eh_tbm/concepts/97944">
		<skos:inScheme rdf:resource="http://purl.org/heritagedata/schemes/eh_tbm" />
		<dcterms:identifier>http://purl.org/heritagedata/schemes/eh_tbm/concepts/97944</dcterms:identifier>
		<skos:prefLabel xml:lang="en">GRANITE</skos:prefLabel>
		<dcterms:issued rdf:datatype="http://www.w3.org/2001/XMLSchema#dateTime">2013-07-17T09:02:16</dcterms:issued>
		<skos:altLabel xml:lang="en">Pink Granite</skos:altLabel>
		<skos:altLabel xml:lang="en">Raddon Stone</skos:altLabel>
		<skos:altLabel xml:lang="en">Muscovite Granite</skos:altLabel>
		<skos:altLabel xml:lang="en">Newham Stone</skos:altLabel>
		<skos:altLabel xml:lang="en">Rose Swede Granite</skos:altLabel>
		<skos:altLabel xml:lang="en">Ross Of Mull Granite</skos:altLabel>
		<skos:altLabel xml:lang="en">Scotch Granite</skos:altLabel>
		<skos:altLabel xml:lang="en">Scottish Granite</skos:altLabel>
		<skos:altLabel xml:lang="en">Virgo Granite</skos:altLabel>
		<skos:altLabel xml:lang="en">Biotite Granite</skos:altLabel>
		<skos:altLabel xml:lang="en">Bon Accord Red Granite</skos:altLabel>
		<skos:altLabel xml:lang="en">Channel Isle Granite</skos:altLabel>
		<skos:altLabel xml:lang="en">Baveno Granite</skos:altLabel>
		<skos:altLabel xml:lang="en">Cornish Granite</skos:altLabel>
		<skos:altLabel xml:lang="en">Correnie Granite</skos:altLabel>
		<skos:altLabel xml:lang="en">Devon Granite</skos:altLabel>
		<skos:altLabel xml:lang="en">Drewsteignston Stone</skos:altLabel>
		<skos:altLabel xml:lang="en">Dundee Marble</skos:altLabel>
		<skos:altLabel xml:lang="en">Dunleary Stone</skos:altLabel>
		<skos:altLabel xml:lang="en">Granolithic Concrete</skos:altLabel>
		<skos:altLabel xml:lang="en">Graphic Granite</skos:altLabel>
		<skos:altLabel xml:lang="en">Grey Royal Granite</skos:altLabel>
		<skos:altLabel xml:lang="en">Hornblende Granite</skos:altLabel>
		<skos:altLabel xml:lang="en">Imperial Mahogany</skos:altLabel>
		<skos:altLabel xml:lang="en">Isle Of Man Granite</skos:altLabel>
		<skos:altLabel xml:lang="en">Kemnay Granite</skos:altLabel>
		<skos:narrower>
			<skos:Concept rdf:about="http://purl.org/heritagedata/schemes/eh_tbm/concepts/97702">
				<skos:inScheme rdf:resource="http://purl.org/heritagedata/schemes/eh_tbm" />
				<dcterms:identifier>http://purl.org/heritagedata/schemes/eh_tbm/concepts/97702</dcterms:identifier>
				<skos:prefLabel xml:lang="en">ABERDEEN GRANITE</skos:prefLabel>
				<dcterms:issued rdf:datatype="http://www.w3.org/2001/XMLSchema#dateTime">2013-07-17T09:02:16</dcterms:issued>
				<skos:altLabel xml:lang="en">Rubislaw Granite</skos:altLabel>
				<skos:altLabel xml:lang="en">Balmoral Granite</skos:altLabel>
				<skos:broader rdf:resource="http://purl.org/heritagedata/schemes/eh_tbm/concepts/97944" />
				<skos:scopeNote xml:lang="en">Medium grained, dark bluish-grey stone. Quarried mainly from the Rubislaw Quarry.</skos:scopeNote>
				<cc:license rdf:resource="http://creativecommons.org/licenses/by/3.0" />
				<cc:attributionURL rdf:resource="http://www.english-heritage.org.uk" />
				<cc:attributionName xml:lang="en">English Heritage</cc:attributionName>
				<dcterms:publisher rdf:resource="http://www.english-heritage.org.uk" />
			</skos:Concept>
		</skos:narrower>
		<skos:broader rdf:resource="http://purl.org/heritagedata/schemes/eh_tbm/concepts/98216" />
		<skos:narrower rdf:resource="http://purl.org/heritagedata/schemes/eh_tbm/concepts/98061" />
		<skos:narrower>
			<skos:Concept rdf:about="http://purl.org/heritagedata/schemes/eh_tbm/concepts/98067">
				<skos:inScheme rdf:resource="http://purl.org/heritagedata/schemes/eh_tbm" />
				<dcterms:identifier>http://purl.org/heritagedata/schemes/eh_tbm/concepts/98067</dcterms:identifier>
				<skos:prefLabel xml:lang="en">MOUNTSORREL GRANITE</skos:prefLabel>
				<dcterms:issued rdf:datatype="http://www.w3.org/2001/XMLSchema#dateTime">2013-07-17T09:02:16</dcterms:issued>
				<skos:altLabel xml:lang="en">Mount Sorrel Granite</skos:altLabel>
				<skos:altLabel xml:lang="en">Mountsorrel Stone</skos:altLabel>
				<skos:broader rdf:resource="http://purl.org/heritagedata/schemes/eh_tbm/concepts/97944" />
				<skos:scopeNote xml:lang="en">Very hard, rough medium/coarse grained, pink to grey coloured granite. Usually found and quarried in Leicestershire.</skos:scopeNote>
				<cc:license rdf:resource="http://creativecommons.org/licenses/by/3.0" />
				<cc:attributionURL rdf:resource="http://www.english-heritage.org.uk" />
				<cc:attributionName xml:lang="en">English Heritage</cc:attributionName>
				<dcterms:publisher rdf:resource="http://www.english-heritage.org.uk" />
			</skos:Concept>
		</skos:narrower>
		<skos:narrower>
			<skos:Concept rdf:about="http://purl.org/heritagedata/schemes/eh_tbm/concepts/98101">
				<skos:inScheme rdf:resource="http://purl.org/heritagedata/schemes/eh_tbm" />
				<dcterms:identifier>http://purl.org/heritagedata/schemes/eh_tbm/concepts/98101</dcterms:identifier>
				<skos:prefLabel xml:lang="en">PETERHEAD GRANITE</skos:prefLabel>
				<dcterms:issued rdf:datatype="http://www.w3.org/2001/XMLSchema#dateTime">2013-07-17T09:02:16</dcterms:issued>
				<skos:altLabel xml:lang="en">Blue Peterhead Granite</skos:altLabel>
				<skos:broader rdf:resource="http://purl.org/heritagedata/schemes/eh_tbm/concepts/97944" />
				<skos:scopeNote xml:lang="en">Coarse grained, dark coloured granite, quarried in the Peterhead and Cairngall areas of Scotland, but used throughout the North.</skos:scopeNote>
				<cc:license rdf:resource="http://creativecommons.org/licenses/by/3.0" />
				<cc:attributionURL rdf:resource="http://www.english-heritage.org.uk" />
				<cc:attributionName xml:lang="en">English Heritage</cc:attributionName>
				<dcterms:publisher rdf:resource="http://www.english-heritage.org.uk" />
			</skos:Concept>
		</skos:narrower>
		<skos:narrower>
			<skos:Concept rdf:about="http://purl.org/heritagedata/schemes/eh_tbm/concepts/98184">
				<skos:inScheme rdf:resource="http://purl.org/heritagedata/schemes/eh_tbm" />
				<dcterms:identifier>http://purl.org/heritagedata/schemes/eh_tbm/concepts/98184</dcterms:identifier>
				<skos:prefLabel xml:lang="en">SHAP GRANITE</skos:prefLabel>
				<dcterms:issued rdf:datatype="http://www.w3.org/2001/XMLSchema#dateTime">2013-07-17T09:02:16</dcterms:issued>
				<skos:altLabel xml:lang="en">Adamelite</skos:altLabel>
				<skos:broader rdf:resource="http://purl.org/heritagedata/schemes/eh_tbm/concepts/97944" />
				<skos:scopeNote xml:lang="en">Hard, coarse grained, grey to red/brown coloured granite. Used predominantly for tombstones becasuse of its ability to take a polish, but it is also in demand for underwater construction.</skos:scopeNote>
				<cc:license rdf:resource="http://creativecommons.org/licenses/by/3.0" />
				<cc:attributionURL rdf:resource="http://www.english-heritage.org.uk" />
				<cc:attributionName xml:lang="en">English Heritage</cc:attributionName>
				<dcterms:publisher rdf:resource="http://www.english-heritage.org.uk" />
			</skos:Concept>
		</skos:narrower>
		<skos:related rdf:resource="http://purl.org/heritagedata/schemes/eh_tbm/concepts/102688" />
		<skos:related rdf:resource="http://purl.org/heritagedata/schemes/eh_tbm/concepts/97908" />
		<skos:related rdf:resource="http://purl.org/heritagedata/schemes/eh_tbm/concepts/97940" />
		<skos:related rdf:resource="http://purl.org/heritagedata/schemes/eh_tbm/concepts/97952" />
		<skos:scopeNote xml:lang="en">A hard, coarse grained, durable igneous rock. Can be used decoratively or as a main material. Found throughout the country.</skos:scopeNote>
		<cc:license rdf:resource="http://creativecommons.org/licenses/by/3.0" />
		<cc:attributionURL rdf:resource="http://www.english-heritage.org.uk" />
		<cc:attributionName xml:lang="en">English Heritage</cc:attributionName>
		<dcterms:publisher rdf:resource="http://www.english-heritage.org.uk" />
	</skos:Concept>
	<skos:Concept rdf:about="http://purl.org/heritagedata/schemes/eh_tbm/concepts/97947">
		<skos:inScheme rdf:resource="http://purl.org/heritagedata/schemes/eh_tbm" />
		<dcterms:identifier>http://purl.org/heritagedata/schemes/eh_tbm/concepts/97947</dcterms:identifier>
		<skos:prefLabel xml:lang="en">GRAVEL</skos:prefLabel>
		<dcterms:issued rdf:datatype="http://www.w3.org/2001/XMLSchema#dateTime">2013-07-17T09:02:16</dcterms:issued>
		<skos:broader rdf:resource="http://purl.org/heritagedata/schemes/eh_tbm/concepts/98046" />
		<skos:related rdf:resource="http://purl.org/heritagedata/schemes/eh_tbm/concepts/98170" />
		<skos:related rdf:resource="http://purl.org/heritagedata/schemes/eh_tbm/concepts/98216" />
		<skos:scopeNote xml:lang="en">Grains of rock fragment larger than coarse sand and finer than pebbles (diameter 2-4mm).</skos:scopeNote>
		<cc:license rdf:resource="http://creativecommons.org/licenses/by/3.0" />
		<cc:attributionURL rdf:resource="http://www.english-heritage.org.uk" />
		<cc:attributionName xml:lang="en">English Heritage</cc:attributionName>
		<dcterms:publisher rdf:resource="http://www.english-heritage.org.uk" />
	</skos:Concept>
	<skos:Concept rdf:about="http://purl.org/heritagedata/schemes/eh_tbm/concepts/97952">
		<skos:inScheme rdf:resource="http://purl.org/heritagedata/schemes/eh_tbm" />
		<dcterms:identifier>http://purl.org/heritagedata/schemes/eh_tbm/concepts/97952</dcterms:identifier>
		<skos:prefLabel xml:lang="en">GREENSTONE</skos:prefLabel>
		<dcterms:issued rdf:datatype="http://www.w3.org/2001/XMLSchema#dateTime">2013-07-17T09:02:16</dcterms:issued>
		<skos:broader rdf:resource="http://purl.org/heritagedata/schemes/eh_tbm/concepts/98216" />
		<skos:related rdf:resource="http://purl.org/heritagedata/schemes/eh_tbm/concepts/97734" />
		<skos:related rdf:resource="http://purl.org/heritagedata/schemes/eh_tbm/concepts/97891" />
		<skos:related rdf:resource="http://purl.org/heritagedata/schemes/eh_tbm/concepts/97944" />
		<skos:scopeNote xml:lang="en">Geologist's term for any dark coloured, slightly metamorphosed igneous rock. Index with specific stone type where given.</skos:scopeNote>
		<cc:license rdf:resource="http://creativecommons.org/licenses/by/3.0" />
		<cc:attributionURL rdf:resource="http://www.english-heritage.org.uk" />
		<cc:attributionName xml:lang="en">English Heritage</cc:attributionName>
		<dcterms:publisher rdf:resource="http://www.english-heritage.org.uk" />
	</skos:Concept>
	<skos:Concept rdf:about="http://purl.org/heritagedata/schemes/eh_tbm/concepts/97974">
		<skos:inScheme rdf:resource="http://purl.org/heritagedata/schemes/eh_tbm" />
		<dcterms:identifier>http://purl.org/heritagedata/schemes/eh_tbm/concepts/97974</dcterms:identifier>
		<skos:prefLabel xml:lang="en">HEATHER</skos:prefLabel>
		<dcterms:issued rdf:datatype="http://www.w3.org/2001/XMLSchema#dateTime">2013-07-17T09:02:16</dcterms:issued>
		<skos:broader rdf:resource="http://purl.org/heritagedata/schemes/eh_tbm/concepts/98109" />
		<skos:related rdf:resource="http://purl.org/heritagedata/schemes/eh_tbm/concepts/98239" />
		<skos:scopeNote xml:lang="en">A dwarf shrub of the heath family used as an alternative to straw as a roof covering in moorland regions. Cut while in bloom and laid with the roots carefully entwined. The covering turns a characteristic black colour with age.</skos:scopeNote>
		<cc:license rdf:resource="http://creativecommons.org/licenses/by/3.0" />
		<cc:attributionURL rdf:resource="http://www.english-heritage.org.uk" />
		<cc:attributionName xml:lang="en">English Heritage</cc:attributionName>
		<dcterms:publisher rdf:resource="http://www.english-heritage.org.uk" />
	</skos:Concept>
	<skos:Concept rdf:about="http://purl.org/heritagedata/schemes/eh_tbm/concepts/97992">
		<skos:inScheme rdf:resource="http://purl.org/heritagedata/schemes/eh_tbm" />
		<dcterms:identifier>http://purl.org/heritagedata/schemes/eh_tbm/concepts/97992</dcterms:identifier>
		<skos:prefLabel xml:lang="en">IRON</skos:prefLabel>
		<dcterms:issued rdf:datatype="http://www.w3.org/2001/XMLSchema#dateTime">2013-07-17T09:02:16</dcterms:issued>
		<skos:altLabel xml:lang="en">Corrugated Iron</skos:altLabel>
		<skos:narrower>
			<skos:Concept rdf:about="http://purl.org/heritagedata/schemes/eh_tbm/concepts/97805">
				<skos:inScheme rdf:resource="http://purl.org/heritagedata/schemes/eh_tbm" />
				<dcterms:identifier>http://purl.org/heritagedata/schemes/eh_tbm/concepts/97805</dcterms:identifier>
				<skos:prefLabel xml:lang="en">CAST IRON</skos:prefLabel>
				<dcterms:issued rdf:datatype="http://www.w3.org/2001/XMLSchema#dateTime">2013-07-17T09:02:16</dcterms:issued>
				<skos:broader rdf:resource="http://purl.org/heritagedata/schemes/eh_tbm/concepts/97992" />
				<skos:scopeNote xml:lang="en">Dating from the 15th century, it is a hard alloy of iron and carbon, melted and shaped into various moulded forms.</skos:scopeNote>
				<cc:license rdf:resource="http://creativecommons.org/licenses/by/3.0" />
				<cc:attributionURL rdf:resource="http://www.english-heritage.org.uk" />
				<cc:attributionName xml:lang="en">English Heritage</cc:attributionName>
				<dcterms:publisher rdf:resource="http://www.english-heritage.org.uk" />
			</skos:Concept>
		</skos:narrower>
		<skos:narrower>
			<skos:Concept rdf:about="http://purl.org/heritagedata/schemes/eh_tbm/concepts/102713">
				<skos:inScheme rdf:resource="http://purl.org/heritagedata/schemes/eh_tbm" />
				<dcterms:identifier>http://purl.org/heritagedata/schemes/eh_tbm/concepts/102713</dcterms:identifier>
				<skos:prefLabel xml:lang="en">GALVANIZED IRON</skos:prefLabel>
				<dcterms:issued rdf:datatype="http://www.w3.org/2001/XMLSchema#dateTime">2013-07-17T09:02:16</dcterms:issued>
				<skos:altLabel xml:lang="en">Galvanised Iron</skos:altLabel>
				<skos:broader rdf:resource="http://purl.org/heritagedata/schemes/eh_tbm/concepts/97992" />
				<skos:scopeNote xml:lang="en">Iron coated in zinc, giving good protection against weathering.</skos:scopeNote>
				<cc:license rdf:resource="http://creativecommons.org/licenses/by/3.0" />
				<cc:attributionURL rdf:resource="http://www.english-heritage.org.uk" />
				<cc:attributionName xml:lang="en">English Heritage</cc:attributionName>
				<dcterms:publisher rdf:resource="http://www.english-heritage.org.uk" />
			</skos:Concept>
		</skos:narrower>
		<skos:broader rdf:resource="http://purl.org/heritagedata/schemes/eh_tbm/concepts/98053" />
		<skos:narrower>
			<skos:Concept rdf:about="http://purl.org/heritagedata/schemes/eh_tbm/concepts/98305">
				<skos:inScheme rdf:resource="http://purl.org/heritagedata/schemes/eh_tbm" />
				<dcterms:identifier>http://purl.org/heritagedata/schemes/eh_tbm/concepts/98305</dcterms:identifier>
				<skos:prefLabel xml:lang="en">WROUGHT IRON</skos:prefLabel>
				<dcterms:issued rdf:datatype="http://www.w3.org/2001/XMLSchema#dateTime">2013-07-17T09:02:16</dcterms:issued>
				<skos:broader rdf:resource="http://purl.org/heritagedata/schemes/eh_tbm/concepts/97992" />
				<skos:scopeNote xml:lang="en">The oldest form of iron, it is a tough, pure form of iron that can be fashioned into decorative items or shapes by hammering, squeezing or rolling.</skos:scopeNote>
				<cc:license rdf:resource="http://creativecommons.org/licenses/by/3.0" />
				<cc:attributionURL rdf:resource="http://www.english-heritage.org.uk" />
				<cc:attributionName xml:lang="en">English Heritage</cc:attributionName>
				<dcterms:publisher rdf:resource="http://www.english-heritage.org.uk" />
			</skos:Concept>
		</skos:narrower>
		<skos:scopeNote xml:lang="en">A malleable, ductile ferromagnetic metal widely used for structural and decorative purposes.</skos:scopeNote>
		<cc:license rdf:resource="http://creativecommons.org/licenses/by/3.0" />
		<cc:attributionURL rdf:resource="http://www.english-heritage.org.uk" />
		<cc:attributionName xml:lang="en">English Heritage</cc:attributionName>
		<dcterms:publisher rdf:resource="http://www.english-heritage.org.uk" />
	</skos:Concept>
	<skos:Concept rdf:about="http://purl.org/heritagedata/schemes/eh_tbm/concepts/97993">
		<skos:inScheme rdf:resource="http://purl.org/heritagedata/schemes/eh_tbm" />
		<dcterms:identifier>http://purl.org/heritagedata/schemes/eh_tbm/concepts/97993</dcterms:identifier>
		<skos:prefLabel xml:lang="en">IRONSTONE</skos:prefLabel>
		<dcterms:issued rdf:datatype="http://www.w3.org/2001/XMLSchema#dateTime">2013-07-17T09:02:16</dcterms:issued>
		<skos:altLabel xml:lang="en">Northamptonshire Stone</skos:altLabel>
		<skos:broader rdf:resource="http://purl.org/heritagedata/schemes/eh_tbm/concepts/98216" />
		<skos:related rdf:resource="http://purl.org/heritagedata/schemes/eh_tbm/concepts/97803" />
		<skos:related rdf:resource="http://purl.org/heritagedata/schemes/eh_tbm/concepts/97919" />
		<skos:related rdf:resource="http://purl.org/heritagedata/schemes/eh_tbm/concepts/98024" />
		<skos:related rdf:resource="http://purl.org/heritagedata/schemes/eh_tbm/concepts/98040" />
		<skos:related rdf:resource="http://purl.org/heritagedata/schemes/eh_tbm/concepts/98045" />
		<skos:related rdf:resource="http://purl.org/heritagedata/schemes/eh_tbm/concepts/98075" />
		<skos:related rdf:resource="http://purl.org/heritagedata/schemes/eh_tbm/concepts/98171" />
		<skos:scopeNote xml:lang="en">Collective name for any stone that has become impregnated with iron oxide. Index with specific stone type where given.</skos:scopeNote>
		<cc:license rdf:resource="http://creativecommons.org/licenses/by/3.0" />
		<cc:attributionURL rdf:resource="http://www.english-heritage.org.uk" />
		<cc:attributionName xml:lang="en">English Heritage</cc:attributionName>
		<dcterms:publisher rdf:resource="http://www.english-heritage.org.uk" />
	</skos:Concept>
	<skos:Concept rdf:about="http://purl.org/heritagedata/schemes/eh_tbm/concepts/97999">
		<skos:inScheme rdf:resource="http://purl.org/heritagedata/schemes/eh_tbm" />
		<dcterms:identifier>http://purl.org/heritagedata/schemes/eh_tbm/concepts/97999</dcterms:identifier>
		<skos:prefLabel xml:lang="en">JURASSIC LIMESTONE</skos:prefLabel>
		<dcterms:issued rdf:datatype="http://www.w3.org/2001/XMLSchema#dateTime">2013-07-17T09:02:16</dcterms:issued>
		<skos:altLabel xml:lang="en">Pink Verona Marble</skos:altLabel>
		<skos:altLabel xml:lang="en">Verde Fraye</skos:altLabel>
		<skos:altLabel xml:lang="en">Verona Marble</skos:altLabel>
		<skos:altLabel xml:lang="en">Walling Stone</skos:altLabel>
		<skos:altLabel xml:lang="en">Yeovil Marble</skos:altLabel>
		<skos:altLabel xml:lang="en">Bletchingdon Marble</skos:altLabel>
		<skos:altLabel xml:lang="en">Forest Marble</skos:altLabel>
		<skos:altLabel xml:lang="en">Hovingham Stone</skos:altLabel>
		<skos:narrower>
			<skos:Concept rdf:about="http://purl.org/heritagedata/schemes/eh_tbm/concepts/97956">
				<skos:inScheme rdf:resource="http://purl.org/heritagedata/schemes/eh_tbm" />
				<dcterms:identifier>http://purl.org/heritagedata/schemes/eh_tbm/concepts/97956</dcterms:identifier>
				<skos:prefLabel xml:lang="en">GRITSTONE (LIMESTONE)</skos:prefLabel>
				<dcterms:issued rdf:datatype="http://www.w3.org/2001/XMLSchema#dateTime">2013-07-17T09:02:16</dcterms:issued>
				<skos:broader rdf:resource="http://purl.org/heritagedata/schemes/eh_tbm/concepts/97999" />
				<skos:scopeNote xml:lang="en">Specific English quarryman's term for any limestone abundant in shell fragments. Use this term with care. When only Gritstone is mentioned, unless otherwise specified, assume it to be Gritstone (Sandstone), since this is the most common usage.</skos:scopeNote>
				<cc:license rdf:resource="http://creativecommons.org/licenses/by/3.0" />
				<cc:attributionURL rdf:resource="http://www.english-heritage.org.uk" />
				<cc:attributionName xml:lang="en">English Heritage</cc:attributionName>
				<dcterms:publisher rdf:resource="http://www.english-heritage.org.uk" />
			</skos:Concept>
		</skos:narrower>
		<skos:broader rdf:resource="http://purl.org/heritagedata/schemes/eh_tbm/concepts/98028" />
		<skos:narrower rdf:resource="http://purl.org/heritagedata/schemes/eh_tbm/concepts/98024" />
		<skos:narrower rdf:resource="http://purl.org/heritagedata/schemes/eh_tbm/concepts/98075" />
		<skos:scopeNote xml:lang="en">Limestone formed during the Jurassic period. Provides many widely used building stones.</skos:scopeNote>
		<cc:license rdf:resource="http://creativecommons.org/licenses/by/3.0" />
		<cc:attributionURL rdf:resource="http://www.english-heritage.org.uk" />
		<cc:attributionName xml:lang="en">English Heritage</cc:attributionName>
		<dcterms:publisher rdf:resource="http://www.english-heritage.org.uk" />
	</skos:Concept>
	<skos:Concept rdf:about="http://purl.org/heritagedata/schemes/eh_tbm/concepts/98013">
		<skos:inScheme rdf:resource="http://purl.org/heritagedata/schemes/eh_tbm" />
		<dcterms:identifier>http://purl.org/heritagedata/schemes/eh_tbm/concepts/98013</dcterms:identifier>
		<skos:prefLabel xml:lang="en">LAKE DISTRICT SLATE</skos:prefLabel>
		<dcterms:issued rdf:datatype="http://www.w3.org/2001/XMLSchema#dateTime">2013-07-17T09:02:16</dcterms:issued>
		<skos:altLabel xml:lang="en">Moss Rigg Slate</skos:altLabel>
		<skos:altLabel xml:lang="en">Skiddaw Slate</skos:altLabel>
		<skos:altLabel xml:lang="en">Spoutcrag</skos:altLabel>
		<skos:altLabel xml:lang="en">Westmoorland Green</skos:altLabel>
		<skos:altLabel xml:lang="en">Westmoorland Slate</skos:altLabel>
		<skos:altLabel xml:lang="en">Borrowdale Slate</skos:altLabel>
		<skos:altLabel xml:lang="en">Brathay Slate</skos:altLabel>
		<skos:altLabel xml:lang="en">Broughton Moor Slate</skos:altLabel>
		<skos:altLabel xml:lang="en">Burlington Blue Grey</skos:altLabel>
		<skos:altLabel xml:lang="en">Burlington Slate</skos:altLabel>
		<skos:altLabel xml:lang="en">Bursting Stone</skos:altLabel>
		<skos:altLabel xml:lang="en">Buttermere Slate</skos:altLabel>
		<skos:altLabel xml:lang="en">Cobble Stone</skos:altLabel>
		<skos:altLabel xml:lang="en">Elterwater Slate</skos:altLabel>
		<skos:altLabel xml:lang="en">Kirkstone Green</skos:altLabel>
		<skos:altLabel xml:lang="en">Lakeland Green</skos:altLabel>
		<skos:altLabel xml:lang="en">Greenslate</skos:altLabel>
		<skos:broader rdf:resource="http://purl.org/heritagedata/schemes/eh_tbm/concepts/98194" />
		<skos:related rdf:resource="http://purl.org/heritagedata/schemes/eh_tbm/concepts/98183" />
		<skos:scopeNote xml:lang="en">Collective term for the Burlington (Silurian period) and Borrowdale (Ordovician period) groups of slates from the Lake District and parts of Cumbria, Lancashire. Hard, fine grained metamorphic rock, varying in colour from green/olive to black/blue black.</skos:scopeNote>
		<cc:license rdf:resource="http://creativecommons.org/licenses/by/3.0" />
		<cc:attributionURL rdf:resource="http://www.english-heritage.org.uk" />
		<cc:attributionName xml:lang="en">English Heritage</cc:attributionName>
		<dcterms:publisher rdf:resource="http://www.english-heritage.org.uk" />
	</skos:Concept>
	<skos:Concept rdf:about="http://purl.org/heritagedata/schemes/eh_tbm/concepts/102688">
		<skos:inScheme rdf:resource="http://purl.org/heritagedata/schemes/eh_tbm" />
		<dcterms:identifier>http://purl.org/heritagedata/schemes/eh_tbm/concepts/102688</dcterms:identifier>
		<skos:prefLabel xml:lang="en">PORPHYRY</skos:prefLabel>
		<dcterms:issued rdf:datatype="http://www.w3.org/2001/XMLSchema#dateTime">2013-07-17T09:02:16</dcterms:issued>
		<skos:narrower rdf:resource="http://purl.org/heritagedata/schemes/eh_tbm/concepts/97908" />
		<skos:broader rdf:resource="http://purl.org/heritagedata/schemes/eh_tbm/concepts/98216" />
		<skos:related rdf:resource="http://purl.org/heritagedata/schemes/eh_tbm/concepts/97928" />
		<skos:related rdf:resource="http://purl.org/heritagedata/schemes/eh_tbm/concepts/97944" />
		<skos:scopeNote xml:lang="en">Traditional term for any fine to medium grained igneous rock, containing large crystal fragments.</skos:scopeNote>
		<cc:license rdf:resource="http://creativecommons.org/licenses/by/3.0" />
		<cc:attributionURL rdf:resource="http://www.english-heritage.org.uk" />
		<cc:attributionName xml:lang="en">English Heritage</cc:attributionName>
		<dcterms:publisher rdf:resource="http://www.english-heritage.org.uk" />
	</skos:Concept>
	<skos:Concept rdf:about="http://purl.org/heritagedata/schemes/eh_tbm/concepts/164108">
		<skos:inScheme rdf:resource="http://purl.org/heritagedata/schemes/eh_tbm" />
		<dcterms:identifier>http://purl.org/heritagedata/schemes/eh_tbm/concepts/164108</dcterms:identifier>
		<skos:prefLabel xml:lang="en">HERTFORDSHIRE PUDDINGSTONE</skos:prefLabel>
		<dcterms:issued rdf:datatype="http://www.w3.org/2001/XMLSchema#dateTime">2013-07-17T09:02:16</dcterms:issued>
		<skos:broader rdf:resource="http://purl.org/heritagedata/schemes/eh_tbm/concepts/98126" />
		<skos:related rdf:resource="http://purl.org/heritagedata/schemes/eh_tbm/concepts/97774" />
		<skos:scopeNote xml:lang="en">A conglomerate rock comprising well rounded flint pebbles in a very hard matrix of fine pale coloured sand, bound together by hard natural silica cement. The pebbles are usually coloured ochre or red and have black rims.</skos:scopeNote>
		<cc:license rdf:resource="http://creativecommons.org/licenses/by/3.0" />
		<cc:attributionURL rdf:resource="http://www.english-heritage.org.uk" />
		<cc:attributionName xml:lang="en">English Heritage</cc:attributionName>
		<dcterms:publisher rdf:resource="http://www.english-heritage.org.uk" />
	</skos:Concept>
</rdf:RDF>