<?xml version="1.0"?>
<rdf:RDF xmlns:dc="http://purl.org/dc/elements/1.1/" xmlns:owl="http://www.w3.org/2002/07/owl#" xmlns:skosxl="http://www.w3.org/2008/05/skos-xl#" xmlns:rdfs="http://www.w3.org/2000/01/rdf-schema#" xmlns:dcterms="http://purl.org/dc/terms/" xmlns:xsd="http://www.w3.org/2001/XMLSchema#" xmlns:rdf="http://www.w3.org/1999/02/22-rdf-syntax-ns#" xmlns:cc="http://creativecommons.org/ns#" xmlns:skos="http://www.w3.org/2004/02/skos/core#" xml:base="http://stellar/">
	<skos:ConceptScheme rdf:about="http://purl.org/heritagedata/schemes/560">
		<dcterms:identifier>http://purl.org/heritagedata/schemes/560</dcterms:identifier>
		<cc:license rdf:resource="http://creativecommons.org/licenses/by/3.0" />
		<cc:attributionURL rdf:resource="http://www.english-heritage.org.uk" />
		<cc:attributionName xml:lang="en">English Heritage</cc:attributionName>
		<dcterms:title xml:lang="en">ARCHAEOLOGICAL SCIENCES (EH)</dcterms:title>
		<rdfs:label xml:lang="en">ARCHAEOLOGICAL SCIENCES (EH)</rdfs:label>
		<dcterms:description xml:lang="en">Used for recording the techniques, recovery methods and materials associated with archaeological sciences.</dcterms:description>
		<dcterms:coverage rdf:resource="http://data.ordnancesurvey.co.uk/id/country/england" />
		<dcterms:publisher rdf:resource="http://www.english-heritage.org.uk" />
		<dcterms:issued rdf:datatype="http://www.w3.org/2001/XMLSchema#dateTime">2013-07-17T09:02:44</dcterms:issued>
		<skos:hasTopConcept>
			<skos:Concept rdf:about="http://purl.org/heritagedata/schemes/560/concepts/142105">
				<skos:topConceptOf rdf:resource="http://purl.org/heritagedata/schemes/560" />
				<skos:inScheme rdf:resource="http://purl.org/heritagedata/schemes/560" />
				<dcterms:identifier>http://purl.org/heritagedata/schemes/560/concepts/142105</dcterms:identifier>
				<skos:prefLabel xml:lang="en">ASPECT</skos:prefLabel>
				<dcterms:issued rdf:datatype="http://www.w3.org/2001/XMLSchema#dateTime">2013-07-17T09:02:45</dcterms:issued>
				<skos:narrower rdf:resource="http://purl.org/heritagedata/schemes/560/concepts/142148" />
				<skos:narrower rdf:resource="http://purl.org/heritagedata/schemes/560/concepts/142173" />
				<cc:license rdf:resource="http://creativecommons.org/licenses/by/3.0" />
				<cc:attributionURL rdf:resource="http://www.english-heritage.org.uk" />
				<cc:attributionName xml:lang="en">English Heritage</cc:attributionName>
				<dcterms:publisher rdf:resource="http://www.english-heritage.org.uk" />
			</skos:Concept>
		</skos:hasTopConcept>
		<skos:hasTopConcept>
			<skos:Concept rdf:about="http://purl.org/heritagedata/schemes/560/concepts/142153">
				<skos:topConceptOf rdf:resource="http://purl.org/heritagedata/schemes/560" />
				<skos:inScheme rdf:resource="http://purl.org/heritagedata/schemes/560" />
				<dcterms:identifier>http://purl.org/heritagedata/schemes/560/concepts/142153</dcterms:identifier>
				<skos:prefLabel xml:lang="en">INVESTIGATIVE TECHNIQUES</skos:prefLabel>
				<dcterms:issued rdf:datatype="http://www.w3.org/2001/XMLSchema#dateTime">2013-07-17T09:02:45</dcterms:issued>
				<skos:narrower rdf:resource="http://purl.org/heritagedata/schemes/560/concepts/142119" />
				<skos:narrower rdf:resource="http://purl.org/heritagedata/schemes/560/concepts/142128" />
				<skos:narrower rdf:resource="http://purl.org/heritagedata/schemes/560/concepts/142182" />
				<cc:license rdf:resource="http://creativecommons.org/licenses/by/3.0" />
				<cc:attributionURL rdf:resource="http://www.english-heritage.org.uk" />
				<cc:attributionName xml:lang="en">English Heritage</cc:attributionName>
				<dcterms:publisher rdf:resource="http://www.english-heritage.org.uk" />
			</skos:Concept>
		</skos:hasTopConcept>
		<skos:hasTopConcept>
			<skos:Concept rdf:about="http://purl.org/heritagedata/schemes/560/concepts/142160">
				<skos:topConceptOf rdf:resource="http://purl.org/heritagedata/schemes/560" />
				<skos:inScheme rdf:resource="http://purl.org/heritagedata/schemes/560" />
				<dcterms:identifier>http://purl.org/heritagedata/schemes/560/concepts/142160</dcterms:identifier>
				<skos:prefLabel xml:lang="en">MATERIAL TYPE</skos:prefLabel>
				<dcterms:issued rdf:datatype="http://www.w3.org/2001/XMLSchema#dateTime">2013-07-17T09:02:45</dcterms:issued>
				<skos:narrower>
					<skos:Concept rdf:about="http://purl.org/heritagedata/schemes/560/concepts/142103">
						<skos:inScheme rdf:resource="http://purl.org/heritagedata/schemes/560" />
						<dcterms:identifier>http://purl.org/heritagedata/schemes/560/concepts/142103</dcterms:identifier>
						<skos:prefLabel xml:lang="en">ANTLER</skos:prefLabel>
						<dcterms:issued rdf:datatype="http://www.w3.org/2001/XMLSchema#dateTime">2013-07-17T09:02:45</dcterms:issued>
						<skos:broader rdf:resource="http://purl.org/heritagedata/schemes/560/concepts/142160" />
						<skos:scopeNote xml:lang="en">Outgrowths of bone borne by most members of the deer family (Cervidae). They are shed and re-grow each year.</skos:scopeNote>
						<cc:license rdf:resource="http://creativecommons.org/licenses/by/3.0" />
						<cc:attributionURL rdf:resource="http://www.english-heritage.org.uk" />
						<cc:attributionName xml:lang="en">English Heritage</cc:attributionName>
						<dcterms:publisher rdf:resource="http://www.english-heritage.org.uk" />
					</skos:Concept>
				</skos:narrower>
				<skos:narrower>
					<skos:Concept rdf:about="http://purl.org/heritagedata/schemes/560/concepts/142981">
						<skos:inScheme rdf:resource="http://purl.org/heritagedata/schemes/560" />
						<dcterms:identifier>http://purl.org/heritagedata/schemes/560/concepts/142981</dcterms:identifier>
						<skos:prefLabel xml:lang="en">BEACH DEPOSIT</skos:prefLabel>
						<dcterms:issued rdf:datatype="http://www.w3.org/2001/XMLSchema#dateTime">2013-07-17T09:02:45</dcterms:issued>
						<skos:broader rdf:resource="http://purl.org/heritagedata/schemes/560/concepts/142160" />
						<skos:scopeNote xml:lang="en">A deposit formed by wave and tidal action on an estuarine or marine beach.</skos:scopeNote>
						<cc:license rdf:resource="http://creativecommons.org/licenses/by/3.0" />
						<cc:attributionURL rdf:resource="http://www.english-heritage.org.uk" />
						<cc:attributionName xml:lang="en">English Heritage</cc:attributionName>
						<dcterms:publisher rdf:resource="http://www.english-heritage.org.uk" />
					</skos:Concept>
				</skos:narrower>
				<skos:narrower>
					<skos:Concept rdf:about="http://purl.org/heritagedata/schemes/560/concepts/144519">
						<skos:inScheme rdf:resource="http://purl.org/heritagedata/schemes/560" />
						<dcterms:identifier>http://purl.org/heritagedata/schemes/560/concepts/144519</dcterms:identifier>
						<skos:prefLabel xml:lang="en">BIOGENIC CARBONATE</skos:prefLabel>
						<dcterms:issued rdf:datatype="http://www.w3.org/2001/XMLSchema#dateTime">2013-07-17T09:02:45</dcterms:issued>
						<skos:broader rdf:resource="http://purl.org/heritagedata/schemes/560/concepts/142160" />
						<skos:scopeNote xml:lang="en">Any carbonate material produced by biological activity, for instance operculae of snails.</skos:scopeNote>
						<cc:license rdf:resource="http://creativecommons.org/licenses/by/3.0" />
						<cc:attributionURL rdf:resource="http://www.english-heritage.org.uk" />
						<cc:attributionName xml:lang="en">English Heritage</cc:attributionName>
						<dcterms:publisher rdf:resource="http://www.english-heritage.org.uk" />
					</skos:Concept>
				</skos:narrower>
				<skos:narrower>
					<skos:Concept rdf:about="http://purl.org/heritagedata/schemes/560/concepts/142109">
						<skos:inScheme rdf:resource="http://purl.org/heritagedata/schemes/560" />
						<dcterms:identifier>http://purl.org/heritagedata/schemes/560/concepts/142109</dcterms:identifier>
						<skos:prefLabel xml:lang="en">BONE</skos:prefLabel>
						<dcterms:issued rdf:datatype="http://www.w3.org/2001/XMLSchema#dateTime">2013-07-17T09:02:45</dcterms:issued>
						<skos:broader rdf:resource="http://purl.org/heritagedata/schemes/560/concepts/142160" />
						<skos:scopeNote xml:lang="en">Any of the pieces of hard tissue consisting largely of calcium phosphate that make up the skeleton of a vertebrate animal.</skos:scopeNote>
						<cc:license rdf:resource="http://creativecommons.org/licenses/by/3.0" />
						<cc:attributionURL rdf:resource="http://www.english-heritage.org.uk" />
						<cc:attributionName xml:lang="en">English Heritage</cc:attributionName>
						<dcterms:publisher rdf:resource="http://www.english-heritage.org.uk" />
					</skos:Concept>
				</skos:narrower>
				<skos:narrower>
					<skos:Concept rdf:about="http://purl.org/heritagedata/schemes/560/concepts/144515">
						<skos:inScheme rdf:resource="http://purl.org/heritagedata/schemes/560" />
						<dcterms:identifier>http://purl.org/heritagedata/schemes/560/concepts/144515</dcterms:identifier>
						<skos:prefLabel xml:lang="en">BRICK</skos:prefLabel>
						<dcterms:issued rdf:datatype="http://www.w3.org/2001/XMLSchema#dateTime">2013-07-17T09:02:45</dcterms:issued>
						<skos:broader rdf:resource="http://purl.org/heritagedata/schemes/560/concepts/142160" />
						<skos:scopeNote xml:lang="en">Material used for construction, commonly fired in its manufacture.</skos:scopeNote>
						<cc:license rdf:resource="http://creativecommons.org/licenses/by/3.0" />
						<cc:attributionURL rdf:resource="http://www.english-heritage.org.uk" />
						<cc:attributionName xml:lang="en">English Heritage</cc:attributionName>
						<dcterms:publisher rdf:resource="http://www.english-heritage.org.uk" />
					</skos:Concept>
				</skos:narrower>
				<skos:narrower>
					<skos:Concept rdf:about="http://purl.org/heritagedata/schemes/560/concepts/144517">
						<skos:inScheme rdf:resource="http://purl.org/heritagedata/schemes/560" />
						<dcterms:identifier>http://purl.org/heritagedata/schemes/560/concepts/144517</dcterms:identifier>
						<skos:prefLabel xml:lang="en">BURNT FLINT</skos:prefLabel>
						<dcterms:issued rdf:datatype="http://www.w3.org/2001/XMLSchema#dateTime">2013-07-17T09:02:45</dcterms:issued>
						<skos:broader rdf:resource="http://purl.org/heritagedata/schemes/560/concepts/142160" />
						<skos:scopeNote xml:lang="en">A form of silica, similar to quartz. Commonly black or white in colour and used for tool manufacture. Flints heated in antiquity may be dated using thermoluminescence.</skos:scopeNote>
						<cc:license rdf:resource="http://creativecommons.org/licenses/by/3.0" />
						<cc:attributionURL rdf:resource="http://www.english-heritage.org.uk" />
						<cc:attributionName xml:lang="en">English Heritage</cc:attributionName>
						<dcterms:publisher rdf:resource="http://www.english-heritage.org.uk" />
					</skos:Concept>
				</skos:narrower>
				<skos:narrower>
					<skos:Concept rdf:about="http://purl.org/heritagedata/schemes/560/concepts/142126">
						<skos:inScheme rdf:resource="http://purl.org/heritagedata/schemes/560" />
						<dcterms:identifier>http://purl.org/heritagedata/schemes/560/concepts/142126</dcterms:identifier>
						<skos:prefLabel xml:lang="en">COPROLITE</skos:prefLabel>
						<dcterms:issued rdf:datatype="http://www.w3.org/2001/XMLSchema#dateTime">2013-07-17T09:02:45</dcterms:issued>
						<skos:broader rdf:resource="http://purl.org/heritagedata/schemes/560/concepts/142160" />
						<skos:scopeNote xml:lang="en">Waste material from the digestive tract of animals. The term coprolite comes from the Greek 'kopros' meaning dung and 'lithos' meaning stone, and is used for faecal matter that has been preserved by mineral replacement or dessication.</skos:scopeNote>
						<cc:license rdf:resource="http://creativecommons.org/licenses/by/3.0" />
						<cc:attributionURL rdf:resource="http://www.english-heritage.org.uk" />
						<cc:attributionName xml:lang="en">English Heritage</cc:attributionName>
						<dcterms:publisher rdf:resource="http://www.english-heritage.org.uk" />
					</skos:Concept>
				</skos:narrower>
				<skos:narrower>
					<skos:Concept rdf:about="http://purl.org/heritagedata/schemes/560/concepts/142135">
						<skos:inScheme rdf:resource="http://purl.org/heritagedata/schemes/560" />
						<dcterms:identifier>http://purl.org/heritagedata/schemes/560/concepts/142135</dcterms:identifier>
						<skos:prefLabel xml:lang="en">EGG SHELL</skos:prefLabel>
						<dcterms:issued rdf:datatype="http://www.w3.org/2001/XMLSchema#dateTime">2013-07-17T09:02:45</dcterms:issued>
						<skos:broader rdf:resource="http://purl.org/heritagedata/schemes/560/concepts/142160" />
						<skos:scopeNote xml:lang="en">Use for the remains of an egg whether from a bird, reptile or amphibian.</skos:scopeNote>
						<cc:license rdf:resource="http://creativecommons.org/licenses/by/3.0" />
						<cc:attributionURL rdf:resource="http://www.english-heritage.org.uk" />
						<cc:attributionName xml:lang="en">English Heritage</cc:attributionName>
						<dcterms:publisher rdf:resource="http://www.english-heritage.org.uk" />
					</skos:Concept>
				</skos:narrower>
				<skos:narrower>
					<skos:Concept rdf:about="http://purl.org/heritagedata/schemes/560/concepts/142977">
						<skos:inScheme rdf:resource="http://purl.org/heritagedata/schemes/560" />
						<dcterms:identifier>http://purl.org/heritagedata/schemes/560/concepts/142977</dcterms:identifier>
						<skos:prefLabel xml:lang="en">ESTUARINE DEPOSIT</skos:prefLabel>
						<dcterms:issued rdf:datatype="http://www.w3.org/2001/XMLSchema#dateTime">2013-07-17T09:02:45</dcterms:issued>
						<skos:broader rdf:resource="http://purl.org/heritagedata/schemes/560/concepts/142160" />
						<skos:scopeNote xml:lang="en">An alluvial deposit laid down in an estuary.</skos:scopeNote>
						<cc:license rdf:resource="http://creativecommons.org/licenses/by/3.0" />
						<cc:attributionURL rdf:resource="http://www.english-heritage.org.uk" />
						<cc:attributionName xml:lang="en">English Heritage</cc:attributionName>
						<dcterms:publisher rdf:resource="http://www.english-heritage.org.uk" />
					</skos:Concept>
				</skos:narrower>
				<skos:narrower>
					<skos:Concept rdf:about="http://purl.org/heritagedata/schemes/560/concepts/142137">
						<skos:inScheme rdf:resource="http://purl.org/heritagedata/schemes/560" />
						<dcterms:identifier>http://purl.org/heritagedata/schemes/560/concepts/142137</dcterms:identifier>
						<skos:prefLabel xml:lang="en">FEATHER</skos:prefLabel>
						<dcterms:issued rdf:datatype="http://www.w3.org/2001/XMLSchema#dateTime">2013-07-17T09:02:45</dcterms:issued>
						<skos:broader rdf:resource="http://purl.org/heritagedata/schemes/560/concepts/142160" />
						<skos:scopeNote xml:lang="en">Use for feathers, an epidermal growth found in birds consisting of a quill, shaft and two vanes of barbs.</skos:scopeNote>
						<cc:license rdf:resource="http://creativecommons.org/licenses/by/3.0" />
						<cc:attributionURL rdf:resource="http://www.english-heritage.org.uk" />
						<cc:attributionName xml:lang="en">English Heritage</cc:attributionName>
						<dcterms:publisher rdf:resource="http://www.english-heritage.org.uk" />
					</skos:Concept>
				</skos:narrower>
				<skos:narrower>
					<skos:Concept rdf:about="http://purl.org/heritagedata/schemes/560/concepts/142139">
						<skos:inScheme rdf:resource="http://purl.org/heritagedata/schemes/560" />
						<dcterms:identifier>http://purl.org/heritagedata/schemes/560/concepts/142139</dcterms:identifier>
						<skos:prefLabel xml:lang="en">FIBRE</skos:prefLabel>
						<dcterms:issued rdf:datatype="http://www.w3.org/2001/XMLSchema#dateTime">2013-07-17T09:02:45</dcterms:issued>
						<skos:broader rdf:resource="http://purl.org/heritagedata/schemes/560/concepts/142160" />
						<skos:scopeNote xml:lang="en">Use for any thread-like material.</skos:scopeNote>
						<cc:license rdf:resource="http://creativecommons.org/licenses/by/3.0" />
						<cc:attributionURL rdf:resource="http://www.english-heritage.org.uk" />
						<cc:attributionName xml:lang="en">English Heritage</cc:attributionName>
						<dcterms:publisher rdf:resource="http://www.english-heritage.org.uk" />
					</skos:Concept>
				</skos:narrower>
				<skos:narrower>
					<skos:Concept rdf:about="http://purl.org/heritagedata/schemes/560/concepts/148433">
						<skos:inScheme rdf:resource="http://purl.org/heritagedata/schemes/560" />
						<dcterms:identifier>http://purl.org/heritagedata/schemes/560/concepts/148433</dcterms:identifier>
						<skos:prefLabel xml:lang="en">FLOT</skos:prefLabel>
						<dcterms:issued rdf:datatype="http://www.w3.org/2001/XMLSchema#dateTime">2013-07-17T09:02:45</dcterms:issued>
						<skos:broader rdf:resource="http://purl.org/heritagedata/schemes/560/concepts/142160" />
						<skos:scopeNote xml:lang="en">The material which floats during the floatation of samples as a means of recovering charred plant remains from an archaeological context.</skos:scopeNote>
						<cc:license rdf:resource="http://creativecommons.org/licenses/by/3.0" />
						<cc:attributionURL rdf:resource="http://www.english-heritage.org.uk" />
						<cc:attributionName xml:lang="en">English Heritage</cc:attributionName>
						<dcterms:publisher rdf:resource="http://www.english-heritage.org.uk" />
					</skos:Concept>
				</skos:narrower>
				<skos:narrower rdf:resource="http://purl.org/heritagedata/schemes/560/concepts/144518" />
				<skos:narrower>
					<skos:Concept rdf:about="http://purl.org/heritagedata/schemes/560/concepts/142146">
						<skos:inScheme rdf:resource="http://purl.org/heritagedata/schemes/560" />
						<dcterms:identifier>http://purl.org/heritagedata/schemes/560/concepts/142146</dcterms:identifier>
						<skos:prefLabel xml:lang="en">HAIR</skos:prefLabel>
						<dcterms:issued rdf:datatype="http://www.w3.org/2001/XMLSchema#dateTime">2013-07-17T09:02:45</dcterms:issued>
						<skos:broader rdf:resource="http://purl.org/heritagedata/schemes/560/concepts/142160" />
						<skos:scopeNote xml:lang="en">Use for hair, fur etc: filaments growing out of the outermost layer of mammalian skin.</skos:scopeNote>
						<cc:license rdf:resource="http://creativecommons.org/licenses/by/3.0" />
						<cc:attributionURL rdf:resource="http://www.english-heritage.org.uk" />
						<cc:attributionName xml:lang="en">English Heritage</cc:attributionName>
						<dcterms:publisher rdf:resource="http://www.english-heritage.org.uk" />
					</skos:Concept>
				</skos:narrower>
				<skos:narrower rdf:resource="http://purl.org/heritagedata/schemes/560/concepts/142156" />
				<skos:narrower rdf:resource="http://purl.org/heritagedata/schemes/560/concepts/142161" />
				<skos:narrower>
					<skos:Concept rdf:about="http://purl.org/heritagedata/schemes/560/concepts/142980">
						<skos:inScheme rdf:resource="http://purl.org/heritagedata/schemes/560" />
						<dcterms:identifier>http://purl.org/heritagedata/schemes/560/concepts/142980</dcterms:identifier>
						<skos:prefLabel xml:lang="en">PEAT DEPOSIT</skos:prefLabel>
						<dcterms:issued rdf:datatype="http://www.w3.org/2001/XMLSchema#dateTime">2013-07-17T09:02:45</dcterms:issued>
						<skos:broader rdf:resource="http://purl.org/heritagedata/schemes/560/concepts/142160" />
						<skos:scopeNote xml:lang="en">A naturally occurring deposit formed by the decomposition and partial carbonisation of vegetable matter in waterlogged conditions.</skos:scopeNote>
						<cc:license rdf:resource="http://creativecommons.org/licenses/by/3.0" />
						<cc:attributionURL rdf:resource="http://www.english-heritage.org.uk" />
						<cc:attributionName xml:lang="en">English Heritage</cc:attributionName>
						<dcterms:publisher rdf:resource="http://www.english-heritage.org.uk" />
					</skos:Concept>
				</skos:narrower>
				<skos:narrower>
					<skos:Concept rdf:about="http://purl.org/heritagedata/schemes/560/concepts/142183">
						<skos:inScheme rdf:resource="http://purl.org/heritagedata/schemes/560" />
						<dcterms:identifier>http://purl.org/heritagedata/schemes/560/concepts/142183</dcterms:identifier>
						<skos:prefLabel xml:lang="en">PHYTOLITH</skos:prefLabel>
						<dcterms:issued rdf:datatype="http://www.w3.org/2001/XMLSchema#dateTime">2013-07-17T09:02:45</dcterms:issued>
						<skos:altLabel xml:lang="en">Microfossils</skos:altLabel>
						<skos:broader rdf:resource="http://purl.org/heritagedata/schemes/560/concepts/142160" />
						<skos:scopeNote xml:lang="en">Microscopic mineral body (usually silica) found in many plants.</skos:scopeNote>
						<cc:license rdf:resource="http://creativecommons.org/licenses/by/3.0" />
						<cc:attributionURL rdf:resource="http://www.english-heritage.org.uk" />
						<cc:attributionName xml:lang="en">English Heritage</cc:attributionName>
						<dcterms:publisher rdf:resource="http://www.english-heritage.org.uk" />
					</skos:Concept>
				</skos:narrower>
				<skos:narrower>
					<skos:Concept rdf:about="http://purl.org/heritagedata/schemes/560/concepts/142186">
						<skos:inScheme rdf:resource="http://purl.org/heritagedata/schemes/560" />
						<dcterms:identifier>http://purl.org/heritagedata/schemes/560/concepts/142186</dcterms:identifier>
						<skos:prefLabel xml:lang="en">POLLEN</skos:prefLabel>
						<dcterms:issued rdf:datatype="http://www.w3.org/2001/XMLSchema#dateTime">2013-07-17T09:02:45</dcterms:issued>
						<skos:broader rdf:resource="http://purl.org/heritagedata/schemes/560/concepts/142160" />
						<skos:scopeNote xml:lang="en">Use for pollen and diaspores. Pollen consists of pollen grains which are the male gametes of flowering plants. Diaspores are the dispersive units of mosses, ferns, fern allies and some plants. To describe the actual object use PLANT REMAINS.</skos:scopeNote>
						<cc:license rdf:resource="http://creativecommons.org/licenses/by/3.0" />
						<cc:attributionURL rdf:resource="http://www.english-heritage.org.uk" />
						<cc:attributionName xml:lang="en">English Heritage</cc:attributionName>
						<dcterms:publisher rdf:resource="http://www.english-heritage.org.uk" />
					</skos:Concept>
				</skos:narrower>
				<skos:narrower>
					<skos:Concept rdf:about="http://purl.org/heritagedata/schemes/560/concepts/144516">
						<skos:inScheme rdf:resource="http://purl.org/heritagedata/schemes/560" />
						<dcterms:identifier>http://purl.org/heritagedata/schemes/560/concepts/144516</dcterms:identifier>
						<skos:prefLabel xml:lang="en">POTTERY</skos:prefLabel>
						<dcterms:issued rdf:datatype="http://www.w3.org/2001/XMLSchema#dateTime">2013-07-17T09:02:45</dcterms:issued>
						<skos:broader rdf:resource="http://purl.org/heritagedata/schemes/560/concepts/142160" />
						<skos:scopeNote xml:lang="en">Object produced commonly by firing clay, but can include coarser material to temper it.</skos:scopeNote>
						<cc:license rdf:resource="http://creativecommons.org/licenses/by/3.0" />
						<cc:attributionURL rdf:resource="http://www.english-heritage.org.uk" />
						<cc:attributionName xml:lang="en">English Heritage</cc:attributionName>
						<dcterms:publisher rdf:resource="http://www.english-heritage.org.uk" />
					</skos:Concept>
				</skos:narrower>
				<skos:narrower>
					<skos:Concept rdf:about="http://purl.org/heritagedata/schemes/560/concepts/148434">
						<skos:inScheme rdf:resource="http://purl.org/heritagedata/schemes/560" />
						<dcterms:identifier>http://purl.org/heritagedata/schemes/560/concepts/148434</dcterms:identifier>
						<skos:prefLabel xml:lang="en">RESIDUE</skos:prefLabel>
						<dcterms:issued rdf:datatype="http://www.w3.org/2001/XMLSchema#dateTime">2013-07-17T09:02:45</dcterms:issued>
						<skos:altLabel xml:lang="en">Heavy Residue</skos:altLabel>
						<skos:broader rdf:resource="http://purl.org/heritagedata/schemes/560/concepts/142160" />
						<skos:scopeNote xml:lang="en">The material that does not float during the floatation of samples as a means of recovering charred plant remains from an archaeological context. Also, the material remaining following wet or dry sieving of course sieved samples.</skos:scopeNote>
						<cc:license rdf:resource="http://creativecommons.org/licenses/by/3.0" />
						<cc:attributionURL rdf:resource="http://www.english-heritage.org.uk" />
						<cc:attributionName xml:lang="en">English Heritage</cc:attributionName>
						<dcterms:publisher rdf:resource="http://www.english-heritage.org.uk" />
					</skos:Concept>
				</skos:narrower>
				<skos:narrower>
					<skos:Concept rdf:about="http://purl.org/heritagedata/schemes/560/concepts/142193">
						<skos:inScheme rdf:resource="http://purl.org/heritagedata/schemes/560" />
						<dcterms:identifier>http://purl.org/heritagedata/schemes/560/concepts/142193</dcterms:identifier>
						<skos:prefLabel xml:lang="en">SHELL</skos:prefLabel>
						<dcterms:issued rdf:datatype="http://www.w3.org/2001/XMLSchema#dateTime">2013-07-17T09:02:45</dcterms:issued>
						<skos:broader rdf:resource="http://purl.org/heritagedata/schemes/560/concepts/142160" />
						<skos:scopeNote xml:lang="en">Use for any shell of an animal, principally, molluscs, crabs etc.</skos:scopeNote>
						<cc:license rdf:resource="http://creativecommons.org/licenses/by/3.0" />
						<cc:attributionURL rdf:resource="http://www.english-heritage.org.uk" />
						<cc:attributionName xml:lang="en">English Heritage</cc:attributionName>
						<dcterms:publisher rdf:resource="http://www.english-heritage.org.uk" />
					</skos:Concept>
				</skos:narrower>
				<skos:narrower rdf:resource="http://purl.org/heritagedata/schemes/560/concepts/142196" />
				<skos:narrower rdf:resource="http://purl.org/heritagedata/schemes/560/concepts/142207" />
				<skos:narrower>
					<skos:Concept rdf:about="http://purl.org/heritagedata/schemes/560/concepts/142979">
						<skos:inScheme rdf:resource="http://purl.org/heritagedata/schemes/560" />
						<dcterms:identifier>http://purl.org/heritagedata/schemes/560/concepts/142979</dcterms:identifier>
						<skos:prefLabel xml:lang="en">TUFACEOUS DEPOSIT</skos:prefLabel>
						<dcterms:issued rdf:datatype="http://www.w3.org/2001/XMLSchema#dateTime">2013-07-17T09:02:45</dcterms:issued>
						<skos:broader rdf:resource="http://purl.org/heritagedata/schemes/560/concepts/142160" />
						<skos:scopeNote xml:lang="en">A naturally occuring deposit of calcareous tufa ('shell marl') sometimes found in alluvial deposits.</skos:scopeNote>
						<cc:license rdf:resource="http://creativecommons.org/licenses/by/3.0" />
						<cc:attributionURL rdf:resource="http://www.english-heritage.org.uk" />
						<cc:attributionName xml:lang="en">English Heritage</cc:attributionName>
						<dcterms:publisher rdf:resource="http://www.english-heritage.org.uk" />
					</skos:Concept>
				</skos:narrower>
				<skos:narrower rdf:resource="http://purl.org/heritagedata/schemes/560/concepts/142214" />
				<cc:license rdf:resource="http://creativecommons.org/licenses/by/3.0" />
				<cc:attributionURL rdf:resource="http://www.english-heritage.org.uk" />
				<cc:attributionName xml:lang="en">English Heritage</cc:attributionName>
				<dcterms:publisher rdf:resource="http://www.english-heritage.org.uk" />
			</skos:Concept>
		</skos:hasTopConcept>
		<skos:hasTopConcept>
			<skos:Concept rdf:about="http://purl.org/heritagedata/schemes/560/concepts/142162">
				<skos:topConceptOf rdf:resource="http://purl.org/heritagedata/schemes/560" />
				<skos:inScheme rdf:resource="http://purl.org/heritagedata/schemes/560" />
				<dcterms:identifier>http://purl.org/heritagedata/schemes/560/concepts/142162</dcterms:identifier>
				<skos:prefLabel xml:lang="en">METHOD OF RECOVERY</skos:prefLabel>
				<dcterms:issued rdf:datatype="http://www.w3.org/2001/XMLSchema#dateTime">2013-07-17T09:02:45</dcterms:issued>
				<skos:narrower>
					<skos:Concept rdf:about="http://purl.org/heritagedata/schemes/560/concepts/142108">
						<skos:inScheme rdf:resource="http://purl.org/heritagedata/schemes/560" />
						<dcterms:identifier>http://purl.org/heritagedata/schemes/560/concepts/142108</dcterms:identifier>
						<skos:prefLabel xml:lang="en">BLOCK LIFTING</skos:prefLabel>
						<dcterms:issued rdf:datatype="http://www.w3.org/2001/XMLSchema#dateTime">2013-07-17T09:02:45</dcterms:issued>
						<skos:broader rdf:resource="http://purl.org/heritagedata/schemes/560/concepts/142162" />
						<skos:scopeNote xml:lang="en">The removal of fragile or complex remains from an investigation as a block of earth for excavation under laboratory conditions. Typical examples are grave goods and cremation burials.</skos:scopeNote>
						<cc:license rdf:resource="http://creativecommons.org/licenses/by/3.0" />
						<cc:attributionURL rdf:resource="http://www.english-heritage.org.uk" />
						<cc:attributionName xml:lang="en">English Heritage</cc:attributionName>
						<dcterms:publisher rdf:resource="http://www.english-heritage.org.uk" />
					</skos:Concept>
				</skos:narrower>
				<skos:narrower>
					<skos:Concept rdf:about="http://purl.org/heritagedata/schemes/560/concepts/142122">
						<skos:inScheme rdf:resource="http://purl.org/heritagedata/schemes/560" />
						<dcterms:identifier>http://purl.org/heritagedata/schemes/560/concepts/142122</dcterms:identifier>
						<skos:prefLabel xml:lang="en">COARSE SIEVING</skos:prefLabel>
						<dcterms:issued rdf:datatype="http://www.w3.org/2001/XMLSchema#dateTime">2013-07-17T09:02:45</dcterms:issued>
						<skos:altLabel xml:lang="en">Bulk Sampling</skos:altLabel>
						<skos:broader rdf:resource="http://purl.org/heritagedata/schemes/560/concepts/142162" />
						<skos:scopeNote xml:lang="en">The method of retrieving animal remains, artefacts and other remains by dry or wet-sieving whole earth samples, typically over 100 litres, sieved through a 2mm or larger mesh.</skos:scopeNote>
						<cc:license rdf:resource="http://creativecommons.org/licenses/by/3.0" />
						<cc:attributionURL rdf:resource="http://www.english-heritage.org.uk" />
						<cc:attributionName xml:lang="en">English Heritage</cc:attributionName>
						<dcterms:publisher rdf:resource="http://www.english-heritage.org.uk" />
					</skos:Concept>
				</skos:narrower>
				<skos:narrower>
					<skos:Concept rdf:about="http://purl.org/heritagedata/schemes/560/concepts/142141">
						<skos:inScheme rdf:resource="http://purl.org/heritagedata/schemes/560" />
						<dcterms:identifier>http://purl.org/heritagedata/schemes/560/concepts/142141</dcterms:identifier>
						<skos:prefLabel xml:lang="en">FLOTATION</skos:prefLabel>
						<dcterms:issued rdf:datatype="http://www.w3.org/2001/XMLSchema#dateTime">2013-07-17T09:02:45</dcterms:issued>
						<skos:broader rdf:resource="http://purl.org/heritagedata/schemes/560/concepts/142162" />
						<skos:scopeNote xml:lang="en">Method used for the recovering of material by floating large whole earth samples, usually between 40-60 litres per context (or 100% if context contains less than this).</skos:scopeNote>
						<cc:license rdf:resource="http://creativecommons.org/licenses/by/3.0" />
						<cc:attributionURL rdf:resource="http://www.english-heritage.org.uk" />
						<cc:attributionName xml:lang="en">English Heritage</cc:attributionName>
						<dcterms:publisher rdf:resource="http://www.english-heritage.org.uk" />
					</skos:Concept>
				</skos:narrower>
				<skos:narrower>
					<skos:Concept rdf:about="http://purl.org/heritagedata/schemes/560/concepts/142147">
						<skos:inScheme rdf:resource="http://purl.org/heritagedata/schemes/560" />
						<dcterms:identifier>http://purl.org/heritagedata/schemes/560/concepts/142147</dcterms:identifier>
						<skos:prefLabel xml:lang="en">HAND RETRIEVAL</skos:prefLabel>
						<dcterms:issued rdf:datatype="http://www.w3.org/2001/XMLSchema#dateTime">2013-07-17T09:02:45</dcterms:issued>
						<skos:broader rdf:resource="http://purl.org/heritagedata/schemes/560/concepts/142162" />
						<skos:scopeNote xml:lang="en">The retrieval of material from deposits by hand, normally large objects visible with the naked eye, eg. Mammal remains and marine molluscs.</skos:scopeNote>
						<cc:license rdf:resource="http://creativecommons.org/licenses/by/3.0" />
						<cc:attributionURL rdf:resource="http://www.english-heritage.org.uk" />
						<cc:attributionName xml:lang="en">English Heritage</cc:attributionName>
						<dcterms:publisher rdf:resource="http://www.english-heritage.org.uk" />
					</skos:Concept>
				</skos:narrower>
				<skos:narrower>
					<skos:Concept rdf:about="http://purl.org/heritagedata/schemes/560/concepts/142198">
						<skos:inScheme rdf:resource="http://purl.org/heritagedata/schemes/560" />
						<dcterms:identifier>http://purl.org/heritagedata/schemes/560/concepts/142198</dcterms:identifier>
						<skos:prefLabel xml:lang="en">SPECIALIST SAMPLING</skos:prefLabel>
						<dcterms:issued rdf:datatype="http://www.w3.org/2001/XMLSchema#dateTime">2013-07-17T09:02:45</dcterms:issued>
						<skos:broader rdf:resource="http://purl.org/heritagedata/schemes/560/concepts/142162" />
						<skos:scopeNote xml:lang="en">The recovery of material from samples collected during field investigations, usually taken by specialists with a particular area of expertise. Normally processed in the laboratory. Also use for the processing of samples subsequent to investigation.</skos:scopeNote>
						<cc:license rdf:resource="http://creativecommons.org/licenses/by/3.0" />
						<cc:attributionURL rdf:resource="http://www.english-heritage.org.uk" />
						<cc:attributionName xml:lang="en">English Heritage</cc:attributionName>
						<dcterms:publisher rdf:resource="http://www.english-heritage.org.uk" />
					</skos:Concept>
				</skos:narrower>
				<cc:license rdf:resource="http://creativecommons.org/licenses/by/3.0" />
				<cc:attributionURL rdf:resource="http://www.english-heritage.org.uk" />
				<cc:attributionName xml:lang="en">English Heritage</cc:attributionName>
				<dcterms:publisher rdf:resource="http://www.english-heritage.org.uk" />
			</skos:Concept>
		</skos:hasTopConcept>
		<skos:hasTopConcept>
			<skos:Concept rdf:about="http://purl.org/heritagedata/schemes/560/concepts/142171">
				<skos:topConceptOf rdf:resource="http://purl.org/heritagedata/schemes/560" />
				<skos:inScheme rdf:resource="http://purl.org/heritagedata/schemes/560" />
				<dcterms:identifier>http://purl.org/heritagedata/schemes/560/concepts/142171</dcterms:identifier>
				<skos:prefLabel xml:lang="en">MODIFICATION STATE</skos:prefLabel>
				<dcterms:issued rdf:datatype="http://www.w3.org/2001/XMLSchema#dateTime">2013-07-17T09:02:45</dcterms:issued>
				<skos:narrower>
					<skos:Concept rdf:about="http://purl.org/heritagedata/schemes/560/concepts/142099">
						<skos:inScheme rdf:resource="http://purl.org/heritagedata/schemes/560" />
						<dcterms:identifier>http://purl.org/heritagedata/schemes/560/concepts/142099</dcterms:identifier>
						<skos:prefLabel xml:lang="en">ALTERED BY ANIMALS</skos:prefLabel>
						<dcterms:issued rdf:datatype="http://www.w3.org/2001/XMLSchema#dateTime">2013-07-17T09:02:45</dcterms:issued>
						<skos:broader rdf:resource="http://purl.org/heritagedata/schemes/560/concepts/142171" />
						<skos:scopeNote xml:lang="en">Modified or damaged by an animal.</skos:scopeNote>
						<cc:license rdf:resource="http://creativecommons.org/licenses/by/3.0" />
						<cc:attributionURL rdf:resource="http://www.english-heritage.org.uk" />
						<cc:attributionName xml:lang="en">English Heritage</cc:attributionName>
						<dcterms:publisher rdf:resource="http://www.english-heritage.org.uk" />
					</skos:Concept>
				</skos:narrower>
				<skos:narrower>
					<skos:Concept rdf:about="http://purl.org/heritagedata/schemes/560/concepts/142102">
						<skos:inScheme rdf:resource="http://purl.org/heritagedata/schemes/560" />
						<dcterms:identifier>http://purl.org/heritagedata/schemes/560/concepts/142102</dcterms:identifier>
						<skos:prefLabel xml:lang="en">ANOXIC</skos:prefLabel>
						<dcterms:issued rdf:datatype="http://www.w3.org/2001/XMLSchema#dateTime">2013-07-17T09:02:45</dcterms:issued>
						<skos:altLabel xml:lang="en">Waterlogged</skos:altLabel>
						<skos:broader rdf:resource="http://purl.org/heritagedata/schemes/560/concepts/142171" />
						<skos:scopeNote xml:lang="en">Material preserved by the exclusion of oxygen usually due to saturation with water which inhibits decay by micro-organisms.</skos:scopeNote>
						<cc:license rdf:resource="http://creativecommons.org/licenses/by/3.0" />
						<cc:attributionURL rdf:resource="http://www.english-heritage.org.uk" />
						<cc:attributionName xml:lang="en">English Heritage</cc:attributionName>
						<dcterms:publisher rdf:resource="http://www.english-heritage.org.uk" />
					</skos:Concept>
				</skos:narrower>
				<skos:narrower rdf:resource="http://purl.org/heritagedata/schemes/560/concepts/142111" />
				<skos:narrower>
					<skos:Concept rdf:about="http://purl.org/heritagedata/schemes/560/concepts/142120">
						<skos:inScheme rdf:resource="http://purl.org/heritagedata/schemes/560" />
						<dcterms:identifier>http://purl.org/heritagedata/schemes/560/concepts/142120</dcterms:identifier>
						<skos:prefLabel xml:lang="en">CHEMICALLY ALTERED</skos:prefLabel>
						<dcterms:issued rdf:datatype="http://www.w3.org/2001/XMLSchema#dateTime">2013-07-17T09:02:45</dcterms:issued>
						<skos:broader rdf:resource="http://purl.org/heritagedata/schemes/560/concepts/142171" />
						<skos:scopeNote xml:lang="en">Material that has been altered as a result of chemical action.</skos:scopeNote>
						<cc:license rdf:resource="http://creativecommons.org/licenses/by/3.0" />
						<cc:attributionURL rdf:resource="http://www.english-heritage.org.uk" />
						<cc:attributionName xml:lang="en">English Heritage</cc:attributionName>
						<dcterms:publisher rdf:resource="http://www.english-heritage.org.uk" />
					</skos:Concept>
				</skos:narrower>
				<skos:narrower>
					<skos:Concept rdf:about="http://purl.org/heritagedata/schemes/560/concepts/142132">
						<skos:inScheme rdf:resource="http://purl.org/heritagedata/schemes/560" />
						<dcterms:identifier>http://purl.org/heritagedata/schemes/560/concepts/142132</dcterms:identifier>
						<skos:prefLabel xml:lang="en">DESICCATED</skos:prefLabel>
						<dcterms:issued rdf:datatype="http://www.w3.org/2001/XMLSchema#dateTime">2013-07-17T09:02:45</dcterms:issued>
						<skos:broader rdf:resource="http://purl.org/heritagedata/schemes/560/concepts/142171" />
						<skos:scopeNote xml:lang="en">Material preserved due to very low humidity which inhibits decay by micro-organisms.</skos:scopeNote>
						<cc:license rdf:resource="http://creativecommons.org/licenses/by/3.0" />
						<cc:attributionURL rdf:resource="http://www.english-heritage.org.uk" />
						<cc:attributionName xml:lang="en">English Heritage</cc:attributionName>
						<dcterms:publisher rdf:resource="http://www.english-heritage.org.uk" />
					</skos:Concept>
				</skos:narrower>
				<skos:narrower>
					<skos:Concept rdf:about="http://purl.org/heritagedata/schemes/560/concepts/142144">
						<skos:inScheme rdf:resource="http://purl.org/heritagedata/schemes/560" />
						<dcterms:identifier>http://purl.org/heritagedata/schemes/560/concepts/142144</dcterms:identifier>
						<skos:prefLabel xml:lang="en">FUNGAL DAMAGE</skos:prefLabel>
						<dcterms:issued rdf:datatype="http://www.w3.org/2001/XMLSchema#dateTime">2013-07-17T09:02:45</dcterms:issued>
						<skos:broader rdf:resource="http://purl.org/heritagedata/schemes/560/concepts/142171" />
						<skos:scopeNote xml:lang="en">Material that has been damaged by fungal growth or secretions.</skos:scopeNote>
						<cc:license rdf:resource="http://creativecommons.org/licenses/by/3.0" />
						<cc:attributionURL rdf:resource="http://www.english-heritage.org.uk" />
						<cc:attributionName xml:lang="en">English Heritage</cc:attributionName>
						<dcterms:publisher rdf:resource="http://www.english-heritage.org.uk" />
					</skos:Concept>
				</skos:narrower>
				<skos:narrower>
					<skos:Concept rdf:about="http://purl.org/heritagedata/schemes/560/concepts/142149">
						<skos:inScheme rdf:resource="http://purl.org/heritagedata/schemes/560" />
						<dcterms:identifier>http://purl.org/heritagedata/schemes/560/concepts/142149</dcterms:identifier>
						<skos:prefLabel xml:lang="en">HYDROLYSIS</skos:prefLabel>
						<dcterms:issued rdf:datatype="http://www.w3.org/2001/XMLSchema#dateTime">2013-07-17T09:02:45</dcterms:issued>
						<skos:broader rdf:resource="http://purl.org/heritagedata/schemes/560/concepts/142171" />
						<skos:scopeNote xml:lang="en">The chemical breakdown of a material by water.</skos:scopeNote>
						<cc:license rdf:resource="http://creativecommons.org/licenses/by/3.0" />
						<cc:attributionURL rdf:resource="http://www.english-heritage.org.uk" />
						<cc:attributionName xml:lang="en">English Heritage</cc:attributionName>
						<dcterms:publisher rdf:resource="http://www.english-heritage.org.uk" />
					</skos:Concept>
				</skos:narrower>
				<skos:narrower>
					<skos:Concept rdf:about="http://purl.org/heritagedata/schemes/560/concepts/142150">
						<skos:inScheme rdf:resource="http://purl.org/heritagedata/schemes/560" />
						<dcterms:identifier>http://purl.org/heritagedata/schemes/560/concepts/142150</dcterms:identifier>
						<skos:prefLabel xml:lang="en">IMPRESSION</skos:prefLabel>
						<dcterms:issued rdf:datatype="http://www.w3.org/2001/XMLSchema#dateTime">2013-07-17T09:02:45</dcterms:issued>
						<skos:broader rdf:resource="http://purl.org/heritagedata/schemes/560/concepts/142171" />
						<skos:scopeNote xml:lang="en">The negative trace left by an object type or material (eg. animal, plant or textile) on another object type or material, often on ceramics or metal corrosion products.</skos:scopeNote>
						<cc:license rdf:resource="http://creativecommons.org/licenses/by/3.0" />
						<cc:attributionURL rdf:resource="http://www.english-heritage.org.uk" />
						<cc:attributionName xml:lang="en">English Heritage</cc:attributionName>
						<dcterms:publisher rdf:resource="http://www.english-heritage.org.uk" />
					</skos:Concept>
				</skos:narrower>
				<skos:narrower>
					<skos:Concept rdf:about="http://purl.org/heritagedata/schemes/560/concepts/142166">
						<skos:inScheme rdf:resource="http://purl.org/heritagedata/schemes/560" />
						<dcterms:identifier>http://purl.org/heritagedata/schemes/560/concepts/142166</dcterms:identifier>
						<skos:prefLabel xml:lang="en">MINERAL PRESERVED</skos:prefLabel>
						<dcterms:issued rdf:datatype="http://www.w3.org/2001/XMLSchema#dateTime">2013-07-17T09:02:45</dcterms:issued>
						<skos:broader rdf:resource="http://purl.org/heritagedata/schemes/560/concepts/142171" />
						<skos:scopeNote xml:lang="en">Preservation of material by toxic effect of corrosion products in the immediate vicinity, or within, the material.</skos:scopeNote>
						<cc:license rdf:resource="http://creativecommons.org/licenses/by/3.0" />
						<cc:attributionURL rdf:resource="http://www.english-heritage.org.uk" />
						<cc:attributionName xml:lang="en">English Heritage</cc:attributionName>
						<dcterms:publisher rdf:resource="http://www.english-heritage.org.uk" />
					</skos:Concept>
				</skos:narrower>
				<skos:narrower>
					<skos:Concept rdf:about="http://purl.org/heritagedata/schemes/560/concepts/142167">
						<skos:inScheme rdf:resource="http://purl.org/heritagedata/schemes/560" />
						<dcterms:identifier>http://purl.org/heritagedata/schemes/560/concepts/142167</dcterms:identifier>
						<skos:prefLabel xml:lang="en">MINERAL REPLACED</skos:prefLabel>
						<dcterms:issued rdf:datatype="http://www.w3.org/2001/XMLSchema#dateTime">2013-07-17T09:02:45</dcterms:issued>
						<skos:altLabel xml:lang="en">Fossilised</skos:altLabel>
						<skos:altLabel xml:lang="en">Mineralised</skos:altLabel>
						<skos:broader rdf:resource="http://purl.org/heritagedata/schemes/560/concepts/142171" />
						<skos:scopeNote xml:lang="en">Replacement of organic material by minerals, including calcium carbonate and calcium phosphate.</skos:scopeNote>
						<cc:license rdf:resource="http://creativecommons.org/licenses/by/3.0" />
						<cc:attributionURL rdf:resource="http://www.english-heritage.org.uk" />
						<cc:attributionName xml:lang="en">English Heritage</cc:attributionName>
						<dcterms:publisher rdf:resource="http://www.english-heritage.org.uk" />
					</skos:Concept>
				</skos:narrower>
				<skos:narrower>
					<skos:Concept rdf:about="http://purl.org/heritagedata/schemes/560/concepts/142184">
						<skos:inScheme rdf:resource="http://purl.org/heritagedata/schemes/560" />
						<dcterms:identifier>http://purl.org/heritagedata/schemes/560/concepts/142184</dcterms:identifier>
						<skos:prefLabel xml:lang="en">PLANT DAMAGE</skos:prefLabel>
						<dcterms:issued rdf:datatype="http://www.w3.org/2001/XMLSchema#dateTime">2013-07-17T09:02:45</dcterms:issued>
						<skos:broader rdf:resource="http://purl.org/heritagedata/schemes/560/concepts/142171" />
						<skos:scopeNote xml:lang="en">Material that has been penetrated or disrupted by the roots or rhizomes of plants.</skos:scopeNote>
						<cc:license rdf:resource="http://creativecommons.org/licenses/by/3.0" />
						<cc:attributionURL rdf:resource="http://www.english-heritage.org.uk" />
						<cc:attributionName xml:lang="en">English Heritage</cc:attributionName>
						<dcterms:publisher rdf:resource="http://www.english-heritage.org.uk" />
					</skos:Concept>
				</skos:narrower>
				<skos:narrower>
					<skos:Concept rdf:about="http://purl.org/heritagedata/schemes/560/concepts/148328">
						<skos:inScheme rdf:resource="http://purl.org/heritagedata/schemes/560" />
						<dcterms:identifier>http://purl.org/heritagedata/schemes/560/concepts/148328</dcterms:identifier>
						<skos:prefLabel xml:lang="en">WATERWORN</skos:prefLabel>
						<dcterms:issued rdf:datatype="http://www.w3.org/2001/XMLSchema#dateTime">2013-07-17T09:02:45</dcterms:issued>
						<skos:broader rdf:resource="http://purl.org/heritagedata/schemes/560/concepts/142171" />
						<skos:scopeNote xml:lang="en">Material, especially rock, worn smooth by the passage of water.</skos:scopeNote>
						<cc:license rdf:resource="http://creativecommons.org/licenses/by/3.0" />
						<cc:attributionURL rdf:resource="http://www.english-heritage.org.uk" />
						<cc:attributionName xml:lang="en">English Heritage</cc:attributionName>
						<dcterms:publisher rdf:resource="http://www.english-heritage.org.uk" />
					</skos:Concept>
				</skos:narrower>
				<cc:license rdf:resource="http://creativecommons.org/licenses/by/3.0" />
				<cc:attributionURL rdf:resource="http://www.english-heritage.org.uk" />
				<cc:attributionName xml:lang="en">English Heritage</cc:attributionName>
				<dcterms:publisher rdf:resource="http://www.english-heritage.org.uk" />
			</skos:Concept>
		</skos:hasTopConcept>
	</skos:ConceptScheme>
	<skos:Concept rdf:about="http://purl.org/heritagedata/schemes/560/concepts/142111">
		<skos:inScheme rdf:resource="http://purl.org/heritagedata/schemes/560" />
		<dcterms:identifier>http://purl.org/heritagedata/schemes/560/concepts/142111</dcterms:identifier>
		<skos:prefLabel xml:lang="en">BURNT</skos:prefLabel>
		<dcterms:issued rdf:datatype="http://www.w3.org/2001/XMLSchema#dateTime">2013-07-17T09:02:45</dcterms:issued>
		<skos:altLabel xml:lang="en">Burnt Deposit</skos:altLabel>
		<skos:broader rdf:resource="http://purl.org/heritagedata/schemes/560/concepts/142171" />
		<skos:narrower>
			<skos:Concept rdf:about="http://purl.org/heritagedata/schemes/560/concepts/142113">
				<skos:inScheme rdf:resource="http://purl.org/heritagedata/schemes/560" />
				<dcterms:identifier>http://purl.org/heritagedata/schemes/560/concepts/142113</dcterms:identifier>
				<skos:prefLabel xml:lang="en">CALCINED</skos:prefLabel>
				<dcterms:issued rdf:datatype="http://www.w3.org/2001/XMLSchema#dateTime">2013-07-17T09:02:45</dcterms:issued>
				<skos:altLabel xml:lang="en">Cremated</skos:altLabel>
				<skos:broader rdf:resource="http://purl.org/heritagedata/schemes/560/concepts/142111" />
				<skos:scopeNote xml:lang="en">Material burnt at high temperature (above 700 degrees Celsius) leaving only the mineral component.</skos:scopeNote>
				<cc:license rdf:resource="http://creativecommons.org/licenses/by/3.0" />
				<cc:attributionURL rdf:resource="http://www.english-heritage.org.uk" />
				<cc:attributionName xml:lang="en">English Heritage</cc:attributionName>
				<dcterms:publisher rdf:resource="http://www.english-heritage.org.uk" />
			</skos:Concept>
		</skos:narrower>
		<skos:narrower rdf:resource="http://purl.org/heritagedata/schemes/560/concepts/142118" />
		<skos:narrower>
			<skos:Concept rdf:about="http://purl.org/heritagedata/schemes/560/concepts/142194">
				<skos:inScheme rdf:resource="http://purl.org/heritagedata/schemes/560" />
				<dcterms:identifier>http://purl.org/heritagedata/schemes/560/concepts/142194</dcterms:identifier>
				<skos:prefLabel xml:lang="en">SILICIFIED</skos:prefLabel>
				<dcterms:issued rdf:datatype="http://www.w3.org/2001/XMLSchema#dateTime">2013-07-17T09:02:45</dcterms:issued>
				<skos:broader rdf:resource="http://purl.org/heritagedata/schemes/560/concepts/142111" />
				<skos:scopeNote xml:lang="en">Use for material that has been burnt at high temperature in a good air supply such that only the silica component remains.</skos:scopeNote>
				<cc:license rdf:resource="http://creativecommons.org/licenses/by/3.0" />
				<cc:attributionURL rdf:resource="http://www.english-heritage.org.uk" />
				<cc:attributionName xml:lang="en">English Heritage</cc:attributionName>
				<dcterms:publisher rdf:resource="http://www.english-heritage.org.uk" />
			</skos:Concept>
		</skos:narrower>
		<skos:scopeNote xml:lang="en">Use for material that has been burnt.</skos:scopeNote>
		<cc:license rdf:resource="http://creativecommons.org/licenses/by/3.0" />
		<cc:attributionURL rdf:resource="http://www.english-heritage.org.uk" />
		<cc:attributionName xml:lang="en">English Heritage</cc:attributionName>
		<dcterms:publisher rdf:resource="http://www.english-heritage.org.uk" />
	</skos:Concept>
	<skos:Concept rdf:about="http://purl.org/heritagedata/schemes/560/concepts/142117">
		<skos:inScheme rdf:resource="http://purl.org/heritagedata/schemes/560" />
		<dcterms:identifier>http://purl.org/heritagedata/schemes/560/concepts/142117</dcterms:identifier>
		<skos:prefLabel xml:lang="en">CHARCOAL</skos:prefLabel>
		<dcterms:issued rdf:datatype="http://www.w3.org/2001/XMLSchema#dateTime">2013-07-17T09:02:45</dcterms:issued>
		<skos:broader rdf:resource="http://purl.org/heritagedata/schemes/560/concepts/142214" />
		<skos:narrower>
			<skos:Concept rdf:about="http://purl.org/heritagedata/schemes/560/concepts/147276">
				<skos:inScheme rdf:resource="http://purl.org/heritagedata/schemes/560" />
				<dcterms:identifier>http://purl.org/heritagedata/schemes/560/concepts/147276</dcterms:identifier>
				<skos:prefLabel xml:lang="en">MICRO-CHARCOAL</skos:prefLabel>
				<dcterms:issued rdf:datatype="http://www.w3.org/2001/XMLSchema#dateTime">2013-07-17T09:02:45</dcterms:issued>
				<skos:broader rdf:resource="http://purl.org/heritagedata/schemes/560/concepts/142117" />
				<skos:scopeNote xml:lang="en">Microscopic charcoal fragments that are concentrated and counted as part of standard pollen preparation techniques.</skos:scopeNote>
				<cc:license rdf:resource="http://creativecommons.org/licenses/by/3.0" />
				<cc:attributionURL rdf:resource="http://www.english-heritage.org.uk" />
				<cc:attributionName xml:lang="en">English Heritage</cc:attributionName>
				<dcterms:publisher rdf:resource="http://www.english-heritage.org.uk" />
			</skos:Concept>
		</skos:narrower>
		<skos:narrower rdf:resource="http://purl.org/heritagedata/schemes/560/concepts/142189" />
		<skos:narrower rdf:resource="http://purl.org/heritagedata/schemes/560/concepts/142211" />
		<skos:related rdf:resource="http://purl.org/heritagedata/schemes/560/concepts/142118" />
		<skos:scopeNote xml:lang="en">Wood that has been burnt and largely reduced to carbon as a result of burning in a reducing atmosphere below 500 degress C (Celsius).</skos:scopeNote>
		<cc:license rdf:resource="http://creativecommons.org/licenses/by/3.0" />
		<cc:attributionURL rdf:resource="http://www.english-heritage.org.uk" />
		<cc:attributionName xml:lang="en">English Heritage</cc:attributionName>
		<dcterms:publisher rdf:resource="http://www.english-heritage.org.uk" />
	</skos:Concept>
	<skos:Concept rdf:about="http://purl.org/heritagedata/schemes/560/concepts/142118">
		<skos:inScheme rdf:resource="http://purl.org/heritagedata/schemes/560" />
		<dcterms:identifier>http://purl.org/heritagedata/schemes/560/concepts/142118</dcterms:identifier>
		<skos:prefLabel xml:lang="en">CHARRED</skos:prefLabel>
		<dcterms:issued rdf:datatype="http://www.w3.org/2001/XMLSchema#dateTime">2013-07-17T09:02:45</dcterms:issued>
		<skos:altLabel xml:lang="en">Carbonised</skos:altLabel>
		<skos:broader rdf:resource="http://purl.org/heritagedata/schemes/560/concepts/142111" />
		<skos:related rdf:resource="http://purl.org/heritagedata/schemes/560/concepts/142117" />
		<skos:scopeNote xml:lang="en">Material that has been burnt and at least in part reduced to carbon as a result of burning in a reducing atmosphere below 500 degrees Celsius.</skos:scopeNote>
		<cc:license rdf:resource="http://creativecommons.org/licenses/by/3.0" />
		<cc:attributionURL rdf:resource="http://www.english-heritage.org.uk" />
		<cc:attributionName xml:lang="en">English Heritage</cc:attributionName>
		<dcterms:publisher rdf:resource="http://www.english-heritage.org.uk" />
	</skos:Concept>
	<skos:Concept rdf:about="http://purl.org/heritagedata/schemes/560/concepts/142119">
		<skos:inScheme rdf:resource="http://purl.org/heritagedata/schemes/560" />
		<dcterms:identifier>http://purl.org/heritagedata/schemes/560/concepts/142119</dcterms:identifier>
		<skos:prefLabel xml:lang="en">CHEMICAL TECHNIQUES</skos:prefLabel>
		<dcterms:issued rdf:datatype="http://www.w3.org/2001/XMLSchema#dateTime">2013-07-17T09:02:45</dcterms:issued>
		<skos:narrower>
			<skos:Concept rdf:about="http://purl.org/heritagedata/schemes/560/concepts/144514">
				<skos:inScheme rdf:resource="http://purl.org/heritagedata/schemes/560" />
				<dcterms:identifier>http://purl.org/heritagedata/schemes/560/concepts/144514</dcterms:identifier>
				<skos:prefLabel xml:lang="en">ALPHA SPECTROMETRY</skos:prefLabel>
				<dcterms:issued rdf:datatype="http://www.w3.org/2001/XMLSchema#dateTime">2013-07-17T09:02:45</dcterms:issued>
				<skos:broader rdf:resource="http://purl.org/heritagedata/schemes/560/concepts/142119" />
				<skos:scopeNote xml:lang="en">A technique that uses the emission of alpha particles of specific energies to identify the presence and concentration of certain radioactive isotopes in a sample</skos:scopeNote>
				<cc:license rdf:resource="http://creativecommons.org/licenses/by/3.0" />
				<cc:attributionURL rdf:resource="http://www.english-heritage.org.uk" />
				<cc:attributionName xml:lang="en">English Heritage</cc:attributionName>
				<dcterms:publisher rdf:resource="http://www.english-heritage.org.uk" />
			</skos:Concept>
		</skos:narrower>
		<skos:narrower>
			<skos:Concept rdf:about="http://purl.org/heritagedata/schemes/560/concepts/142101">
				<skos:inScheme rdf:resource="http://purl.org/heritagedata/schemes/560" />
				<dcterms:identifier>http://purl.org/heritagedata/schemes/560/concepts/142101</dcterms:identifier>
				<skos:prefLabel xml:lang="en">ANCIENT BIOMOLECULAR ANALYSIS</skos:prefLabel>
				<dcterms:issued rdf:datatype="http://www.w3.org/2001/XMLSchema#dateTime">2013-07-17T09:02:45</dcterms:issued>
				<skos:broader rdf:resource="http://purl.org/heritagedata/schemes/560/concepts/142119" />
				<skos:scopeNote xml:lang="en">Characterisation of organic molecules extracted from fossil or sub-fossil materials, including lipids, DNA etc.</skos:scopeNote>
				<cc:license rdf:resource="http://creativecommons.org/licenses/by/3.0" />
				<cc:attributionURL rdf:resource="http://www.english-heritage.org.uk" />
				<cc:attributionName xml:lang="en">English Heritage</cc:attributionName>
				<dcterms:publisher rdf:resource="http://www.english-heritage.org.uk" />
			</skos:Concept>
		</skos:narrower>
		<skos:broader rdf:resource="http://purl.org/heritagedata/schemes/560/concepts/142153" />
		<skos:narrower>
			<skos:Concept rdf:about="http://purl.org/heritagedata/schemes/560/concepts/144513">
				<skos:inScheme rdf:resource="http://purl.org/heritagedata/schemes/560" />
				<dcterms:identifier>http://purl.org/heritagedata/schemes/560/concepts/144513</dcterms:identifier>
				<skos:prefLabel xml:lang="en">GAMMA SPECTROMETRY</skos:prefLabel>
				<dcterms:issued rdf:datatype="http://www.w3.org/2001/XMLSchema#dateTime">2013-07-17T09:02:45</dcterms:issued>
				<skos:broader rdf:resource="http://purl.org/heritagedata/schemes/560/concepts/142119" />
				<skos:scopeNote xml:lang="en">A technique that uses the emission of gamma rays of specific energies to identify the presence and concentration of certain radioactive isotopes in a sample</skos:scopeNote>
				<cc:license rdf:resource="http://creativecommons.org/licenses/by/3.0" />
				<cc:attributionURL rdf:resource="http://www.english-heritage.org.uk" />
				<cc:attributionName xml:lang="en">English Heritage</cc:attributionName>
				<dcterms:publisher rdf:resource="http://www.english-heritage.org.uk" />
			</skos:Concept>
		</skos:narrower>
		<skos:narrower rdf:resource="http://purl.org/heritagedata/schemes/560/concepts/142172" />
		<skos:narrower>
			<skos:Concept rdf:about="http://purl.org/heritagedata/schemes/560/concepts/147278">
				<skos:inScheme rdf:resource="http://purl.org/heritagedata/schemes/560" />
				<dcterms:identifier>http://purl.org/heritagedata/schemes/560/concepts/147278</dcterms:identifier>
				<skos:prefLabel xml:lang="en">PEAT HUMIFICATION</skos:prefLabel>
				<dcterms:issued rdf:datatype="http://www.w3.org/2001/XMLSchema#dateTime">2013-07-17T09:02:45</dcterms:issued>
				<skos:broader rdf:resource="http://purl.org/heritagedata/schemes/560/concepts/142119" />
				<skos:scopeNote xml:lang="en">A method of determining peat degradation; quantified as the percentage light transmission value of the extracted humic acids, measured at a specific wavelength.</skos:scopeNote>
				<cc:license rdf:resource="http://creativecommons.org/licenses/by/3.0" />
				<cc:attributionURL rdf:resource="http://www.english-heritage.org.uk" />
				<cc:attributionName xml:lang="en">English Heritage</cc:attributionName>
				<dcterms:publisher rdf:resource="http://www.english-heritage.org.uk" />
			</skos:Concept>
		</skos:narrower>
		<skos:narrower>
			<skos:Concept rdf:about="http://purl.org/heritagedata/schemes/560/concepts/142181">
				<skos:inScheme rdf:resource="http://purl.org/heritagedata/schemes/560" />
				<dcterms:identifier>http://purl.org/heritagedata/schemes/560/concepts/142181</dcterms:identifier>
				<skos:prefLabel xml:lang="en">PH DETERMINATION</skos:prefLabel>
				<dcterms:issued rdf:datatype="http://www.w3.org/2001/XMLSchema#dateTime">2013-07-17T09:02:45</dcterms:issued>
				<skos:broader rdf:resource="http://purl.org/heritagedata/schemes/560/concepts/142119" />
				<skos:scopeNote xml:lang="en">The degree of acidity or alkalinity of a material.</skos:scopeNote>
				<cc:license rdf:resource="http://creativecommons.org/licenses/by/3.0" />
				<cc:attributionURL rdf:resource="http://www.english-heritage.org.uk" />
				<cc:attributionName xml:lang="en">English Heritage</cc:attributionName>
				<dcterms:publisher rdf:resource="http://www.english-heritage.org.uk" />
			</skos:Concept>
		</skos:narrower>
		<skos:narrower rdf:resource="http://purl.org/heritagedata/schemes/560/concepts/142197" />
		<skos:narrower>
			<skos:Concept rdf:about="http://purl.org/heritagedata/schemes/560/concepts/142199">
				<skos:inScheme rdf:resource="http://purl.org/heritagedata/schemes/560" />
				<dcterms:identifier>http://purl.org/heritagedata/schemes/560/concepts/142199</dcterms:identifier>
				<skos:prefLabel xml:lang="en">SPOT TEST</skos:prefLabel>
				<dcterms:issued rdf:datatype="http://www.w3.org/2001/XMLSchema#dateTime">2013-07-17T09:02:45</dcterms:issued>
				<skos:broader rdf:resource="http://purl.org/heritagedata/schemes/560/concepts/142119" />
				<skos:scopeNote xml:lang="en">The application of a chemical test to a material, usually as a rapid approximation.</skos:scopeNote>
				<cc:license rdf:resource="http://creativecommons.org/licenses/by/3.0" />
				<cc:attributionURL rdf:resource="http://www.english-heritage.org.uk" />
				<cc:attributionName xml:lang="en">English Heritage</cc:attributionName>
				<dcterms:publisher rdf:resource="http://www.english-heritage.org.uk" />
			</skos:Concept>
		</skos:narrower>
		<skos:narrower>
			<skos:Concept rdf:about="http://purl.org/heritagedata/schemes/560/concepts/142200">
				<skos:inScheme rdf:resource="http://purl.org/heritagedata/schemes/560" />
				<dcterms:identifier>http://purl.org/heritagedata/schemes/560/concepts/142200</dcterms:identifier>
				<skos:prefLabel xml:lang="en">STABLE ISOTOPE ANALYSIS</skos:prefLabel>
				<dcterms:issued rdf:datatype="http://www.w3.org/2001/XMLSchema#dateTime">2013-07-17T09:02:45</dcterms:issued>
				<skos:broader rdf:resource="http://purl.org/heritagedata/schemes/560/concepts/142119" />
				<skos:scopeNote xml:lang="en">Comparison of different proportions of natural occurring isotopes of lead (Pb), strontium (Sr), oxygen (O), carbon (C) and nitrogen (N).</skos:scopeNote>
				<cc:license rdf:resource="http://creativecommons.org/licenses/by/3.0" />
				<cc:attributionURL rdf:resource="http://www.english-heritage.org.uk" />
				<cc:attributionName xml:lang="en">English Heritage</cc:attributionName>
				<dcterms:publisher rdf:resource="http://www.english-heritage.org.uk" />
			</skos:Concept>
		</skos:narrower>
		<skos:scopeNote xml:lang="en">Examination of a material using chemical means.</skos:scopeNote>
		<cc:license rdf:resource="http://creativecommons.org/licenses/by/3.0" />
		<cc:attributionURL rdf:resource="http://www.english-heritage.org.uk" />
		<cc:attributionName xml:lang="en">English Heritage</cc:attributionName>
		<dcterms:publisher rdf:resource="http://www.english-heritage.org.uk" />
	</skos:Concept>
	<skos:Concept rdf:about="http://purl.org/heritagedata/schemes/560/concepts/142128">
		<skos:inScheme rdf:resource="http://purl.org/heritagedata/schemes/560" />
		<dcterms:identifier>http://purl.org/heritagedata/schemes/560/concepts/142128</dcterms:identifier>
		<skos:prefLabel xml:lang="en">DATING TECHNIQUES</skos:prefLabel>
		<dcterms:issued rdf:datatype="http://www.w3.org/2001/XMLSchema#dateTime">2013-07-17T09:02:45</dcterms:issued>
		<skos:narrower>
			<skos:Concept rdf:about="http://purl.org/heritagedata/schemes/560/concepts/142100">
				<skos:inScheme rdf:resource="http://purl.org/heritagedata/schemes/560" />
				<dcterms:identifier>http://purl.org/heritagedata/schemes/560/concepts/142100</dcterms:identifier>
				<skos:prefLabel xml:lang="en">AMINO ACID RACEMISATION</skos:prefLabel>
				<dcterms:issued rdf:datatype="http://www.w3.org/2001/XMLSchema#dateTime">2013-07-17T09:02:45</dcterms:issued>
				<skos:broader rdf:resource="http://purl.org/heritagedata/schemes/560/concepts/142128" />
				<skos:scopeNote xml:lang="en">The measurement of chemical alterations in the amino acids in protein molecules from bones, shells and teeth. Date range can be between 1,000 and several million years.</skos:scopeNote>
				<cc:license rdf:resource="http://creativecommons.org/licenses/by/3.0" />
				<cc:attributionURL rdf:resource="http://www.english-heritage.org.uk" />
				<cc:attributionName xml:lang="en">English Heritage</cc:attributionName>
				<dcterms:publisher rdf:resource="http://www.english-heritage.org.uk" />
			</skos:Concept>
		</skos:narrower>
		<skos:narrower>
			<skos:Concept rdf:about="http://purl.org/heritagedata/schemes/560/concepts/142104">
				<skos:inScheme rdf:resource="http://purl.org/heritagedata/schemes/560" />
				<dcterms:identifier>http://purl.org/heritagedata/schemes/560/concepts/142104</dcterms:identifier>
				<skos:prefLabel xml:lang="en">ARCHAEOMAGNETISM</skos:prefLabel>
				<dcterms:issued rdf:datatype="http://www.w3.org/2001/XMLSchema#dateTime">2013-07-17T09:02:45</dcterms:issued>
				<skos:broader rdf:resource="http://purl.org/heritagedata/schemes/560/concepts/142128" />
				<skos:scopeNote xml:lang="en">Measures the remanent magnetisation direction of magnetic minerals. Useful for dating fired structures, in-situ since their last firing, and for sediments settling from non turbulent water bodies. In the UK, calibration data extends back to 1000BC.</skos:scopeNote>
				<cc:license rdf:resource="http://creativecommons.org/licenses/by/3.0" />
				<cc:attributionURL rdf:resource="http://www.english-heritage.org.uk" />
				<cc:attributionName xml:lang="en">English Heritage</cc:attributionName>
				<dcterms:publisher rdf:resource="http://www.english-heritage.org.uk" />
			</skos:Concept>
		</skos:narrower>
		<skos:narrower>
			<skos:Concept rdf:about="http://purl.org/heritagedata/schemes/560/concepts/142107">
				<skos:inScheme rdf:resource="http://purl.org/heritagedata/schemes/560" />
				<dcterms:identifier>http://purl.org/heritagedata/schemes/560/concepts/142107</dcterms:identifier>
				<skos:prefLabel xml:lang="en">BIOSTRATIGRAPHY</skos:prefLabel>
				<dcterms:issued rdf:datatype="http://www.w3.org/2001/XMLSchema#dateTime">2013-07-17T09:02:45</dcterms:issued>
				<skos:broader rdf:resource="http://purl.org/heritagedata/schemes/560/concepts/142128" />
				<skos:scopeNote xml:lang="en">A technique in which the date is deduced from the presence of fauna and/or flora considered to be characteristic of a given peirod of time or that gives and indication of a probable date.</skos:scopeNote>
				<cc:license rdf:resource="http://creativecommons.org/licenses/by/3.0" />
				<cc:attributionURL rdf:resource="http://www.english-heritage.org.uk" />
				<cc:attributionName xml:lang="en">English Heritage</cc:attributionName>
				<dcterms:publisher rdf:resource="http://www.english-heritage.org.uk" />
			</skos:Concept>
		</skos:narrower>
		<skos:broader rdf:resource="http://purl.org/heritagedata/schemes/560/concepts/142153" />
		<skos:narrower rdf:resource="http://purl.org/heritagedata/schemes/560/concepts/142131" />
		<skos:narrower>
			<skos:Concept rdf:about="http://purl.org/heritagedata/schemes/560/concepts/142136">
				<skos:inScheme rdf:resource="http://purl.org/heritagedata/schemes/560" />
				<dcterms:identifier>http://purl.org/heritagedata/schemes/560/concepts/142136</dcterms:identifier>
				<skos:prefLabel xml:lang="en">ELECTRON SPIN RESONANCE</skos:prefLabel>
				<dcterms:issued rdf:datatype="http://www.w3.org/2001/XMLSchema#dateTime">2013-07-17T09:02:45</dcterms:issued>
				<skos:broader rdf:resource="http://purl.org/heritagedata/schemes/560/concepts/142128" />
				<skos:scopeNote xml:lang="en">The measurement of trapped electrons by exposure to high-frequency electromagnetic radiation. A useful technique for dating tooth enamel, shells, coral and calcite form 5,000-1,000,000 years old.</skos:scopeNote>
				<cc:license rdf:resource="http://creativecommons.org/licenses/by/3.0" />
				<cc:attributionURL rdf:resource="http://www.english-heritage.org.uk" />
				<cc:attributionName xml:lang="en">English Heritage</cc:attributionName>
				<dcterms:publisher rdf:resource="http://www.english-heritage.org.uk" />
			</skos:Concept>
		</skos:narrower>
		<skos:narrower>
			<skos:Concept rdf:about="http://purl.org/heritagedata/schemes/560/concepts/142140">
				<skos:inScheme rdf:resource="http://purl.org/heritagedata/schemes/560" />
				<dcterms:identifier>http://purl.org/heritagedata/schemes/560/concepts/142140</dcterms:identifier>
				<skos:prefLabel xml:lang="en">FISSION TRACK ANALYSIS</skos:prefLabel>
				<dcterms:issued rdf:datatype="http://www.w3.org/2001/XMLSchema#dateTime">2013-07-17T09:02:45</dcterms:issued>
				<skos:broader rdf:resource="http://purl.org/heritagedata/schemes/560/concepts/142128" />
				<skos:scopeNote xml:lang="en">A technique for the dating of damage tracks in volcanic materials caused by the fissioning of decaying radioactive uranium (U) isotopes. Useful in samples more than 50,000 years old.</skos:scopeNote>
				<cc:license rdf:resource="http://creativecommons.org/licenses/by/3.0" />
				<cc:attributionURL rdf:resource="http://www.english-heritage.org.uk" />
				<cc:attributionName xml:lang="en">English Heritage</cc:attributionName>
				<dcterms:publisher rdf:resource="http://www.english-heritage.org.uk" />
			</skos:Concept>
		</skos:narrower>
		<skos:narrower>
			<skos:Concept rdf:about="http://purl.org/heritagedata/schemes/560/concepts/142142">
				<skos:inScheme rdf:resource="http://purl.org/heritagedata/schemes/560" />
				<dcterms:identifier>http://purl.org/heritagedata/schemes/560/concepts/142142</dcterms:identifier>
				<skos:prefLabel xml:lang="en">FLUORINE, URANIUM AND NITROGEN TESTS</skos:prefLabel>
				<dcterms:issued rdf:datatype="http://www.w3.org/2001/XMLSchema#dateTime">2013-07-17T09:02:45</dcterms:issued>
				<skos:broader rdf:resource="http://purl.org/heritagedata/schemes/560/concepts/142128" />
				<skos:scopeNote xml:lang="en">A relative dating technique for assessing bones from the same deposit. Often used to check for contemporaneity of bones selected for radiocarbon dating or to check for hoaxes such as the Piltdown Man.</skos:scopeNote>
				<cc:license rdf:resource="http://creativecommons.org/licenses/by/3.0" />
				<cc:attributionURL rdf:resource="http://www.english-heritage.org.uk" />
				<cc:attributionName xml:lang="en">English Heritage</cc:attributionName>
				<dcterms:publisher rdf:resource="http://www.english-heritage.org.uk" />
			</skos:Concept>
		</skos:narrower>
		<skos:narrower>
			<skos:Concept rdf:about="http://purl.org/heritagedata/schemes/560/concepts/142155">
				<skos:inScheme rdf:resource="http://purl.org/heritagedata/schemes/560" />
				<dcterms:identifier>http://purl.org/heritagedata/schemes/560/concepts/142155</dcterms:identifier>
				<skos:prefLabel xml:lang="en">LEAD ISOTOPE DATING</skos:prefLabel>
				<dcterms:issued rdf:datatype="http://www.w3.org/2001/XMLSchema#dateTime">2013-07-17T09:02:45</dcterms:issued>
				<skos:broader rdf:resource="http://purl.org/heritagedata/schemes/560/concepts/142128" />
				<skos:scopeNote xml:lang="en">A technique which uses the measurement of decay in radioactive lead (Pb) isotopes to determine a date. Useful for sediments and lead-based paints between 1 and 400 years old.</skos:scopeNote>
				<cc:license rdf:resource="http://creativecommons.org/licenses/by/3.0" />
				<cc:attributionURL rdf:resource="http://www.english-heritage.org.uk" />
				<cc:attributionName xml:lang="en">English Heritage</cc:attributionName>
				<dcterms:publisher rdf:resource="http://www.english-heritage.org.uk" />
			</skos:Concept>
		</skos:narrower>
		<skos:narrower rdf:resource="http://purl.org/heritagedata/schemes/560/concepts/144511" />
		<skos:narrower>
			<skos:Concept rdf:about="http://purl.org/heritagedata/schemes/560/concepts/142170">
				<skos:inScheme rdf:resource="http://purl.org/heritagedata/schemes/560" />
				<dcterms:identifier>http://purl.org/heritagedata/schemes/560/concepts/142170</dcterms:identifier>
				<skos:prefLabel xml:lang="en">MITOCHONDRIAL DNA</skos:prefLabel>
				<dcterms:issued rdf:datatype="http://www.w3.org/2001/XMLSchema#dateTime">2013-07-17T09:02:45</dcterms:issued>
				<skos:broader rdf:resource="http://purl.org/heritagedata/schemes/560/concepts/142128" />
				<skos:scopeNote xml:lang="en">A dating technique for the founding of individual populations based on the assumption of steady rates of mutation in mitochondrial DNA. Sometimes used to produce dates for stratigraphic layers containing fossil specimens of populations.</skos:scopeNote>
				<cc:license rdf:resource="http://creativecommons.org/licenses/by/3.0" />
				<cc:attributionURL rdf:resource="http://www.english-heritage.org.uk" />
				<cc:attributionName xml:lang="en">English Heritage</cc:attributionName>
				<dcterms:publisher rdf:resource="http://www.english-heritage.org.uk" />
			</skos:Concept>
		</skos:narrower>
		<skos:narrower>
			<skos:Concept rdf:about="http://purl.org/heritagedata/schemes/560/concepts/142176">
				<skos:inScheme rdf:resource="http://purl.org/heritagedata/schemes/560" />
				<dcterms:identifier>http://purl.org/heritagedata/schemes/560/concepts/142176</dcterms:identifier>
				<skos:prefLabel xml:lang="en">OBSIDIAN HYDRATION</skos:prefLabel>
				<dcterms:issued rdf:datatype="http://www.w3.org/2001/XMLSchema#dateTime">2013-07-17T09:02:45</dcterms:issued>
				<skos:broader rdf:resource="http://purl.org/heritagedata/schemes/560/concepts/142128" />
				<skos:scopeNote xml:lang="en">A technique used to date obsidian (volcanic glass) of all ages and is thus not commonly used in the UK.</skos:scopeNote>
				<cc:license rdf:resource="http://creativecommons.org/licenses/by/3.0" />
				<cc:attributionURL rdf:resource="http://www.english-heritage.org.uk" />
				<cc:attributionName xml:lang="en">English Heritage</cc:attributionName>
				<dcterms:publisher rdf:resource="http://www.english-heritage.org.uk" />
			</skos:Concept>
		</skos:narrower>
		<skos:narrower>
			<skos:Concept rdf:about="http://purl.org/heritagedata/schemes/560/concepts/142178">
				<skos:inScheme rdf:resource="http://purl.org/heritagedata/schemes/560" />
				<dcterms:identifier>http://purl.org/heritagedata/schemes/560/concepts/142178</dcterms:identifier>
				<skos:prefLabel xml:lang="en">OXYGEN ISOTOPE ANALYSIS</skos:prefLabel>
				<dcterms:issued rdf:datatype="http://www.w3.org/2001/XMLSchema#dateTime">2013-07-17T09:02:45</dcterms:issued>
				<skos:broader rdf:resource="http://purl.org/heritagedata/schemes/560/concepts/142128" />
				<skos:scopeNote xml:lang="en">The use of oxygen (O) isotope ratios in ice or ocean sediment cores to date global environmental change.</skos:scopeNote>
				<cc:license rdf:resource="http://creativecommons.org/licenses/by/3.0" />
				<cc:attributionURL rdf:resource="http://www.english-heritage.org.uk" />
				<cc:attributionName xml:lang="en">English Heritage</cc:attributionName>
				<dcterms:publisher rdf:resource="http://www.english-heritage.org.uk" />
			</skos:Concept>
		</skos:narrower>
		<skos:narrower>
			<skos:Concept rdf:about="http://purl.org/heritagedata/schemes/560/concepts/142187">
				<skos:inScheme rdf:resource="http://purl.org/heritagedata/schemes/560" />
				<dcterms:identifier>http://purl.org/heritagedata/schemes/560/concepts/142187</dcterms:identifier>
				<skos:prefLabel xml:lang="en">POTASSIUM ARGON DATING</skos:prefLabel>
				<dcterms:issued rdf:datatype="http://www.w3.org/2001/XMLSchema#dateTime">2013-07-17T09:02:45</dcterms:issued>
				<skos:broader rdf:resource="http://purl.org/heritagedata/schemes/560/concepts/142128" />
				<skos:scopeNote xml:lang="en">The measurement of the ratio of a radioactive potassium (K) isotope and the argon (Ar) gas produced as a by-product of its decay. Useful for dating volcanic material older than 1,000 years.</skos:scopeNote>
				<cc:license rdf:resource="http://creativecommons.org/licenses/by/3.0" />
				<cc:attributionURL rdf:resource="http://www.english-heritage.org.uk" />
				<cc:attributionName xml:lang="en">English Heritage</cc:attributionName>
				<dcterms:publisher rdf:resource="http://www.english-heritage.org.uk" />
			</skos:Concept>
		</skos:narrower>
		<skos:narrower>
			<skos:Concept rdf:about="http://purl.org/heritagedata/schemes/560/concepts/142188">
				<skos:inScheme rdf:resource="http://purl.org/heritagedata/schemes/560" />
				<dcterms:identifier>http://purl.org/heritagedata/schemes/560/concepts/142188</dcterms:identifier>
				<skos:prefLabel xml:lang="en">RADIOCARBON DATING</skos:prefLabel>
				<dcterms:issued rdf:datatype="http://www.w3.org/2001/XMLSchema#dateTime">2013-07-17T09:02:45</dcterms:issued>
				<skos:altLabel xml:lang="en">C14 Dating</skos:altLabel>
				<skos:altLabel xml:lang="en">Carbon 14 Dating</skos:altLabel>
				<skos:altLabel xml:lang="en">Carbon Dating</skos:altLabel>
				<skos:broader rdf:resource="http://purl.org/heritagedata/schemes/560/concepts/142128" />
				<skos:scopeNote xml:lang="en">The measurement of the ratio of the radioactive Carbon 14 (C-14) isotope and non-radioactive carbon isotopes. Useful for dating organic materials such as wood and bone between 500 and 45,000 years old.</skos:scopeNote>
				<cc:license rdf:resource="http://creativecommons.org/licenses/by/3.0" />
				<cc:attributionURL rdf:resource="http://www.english-heritage.org.uk" />
				<cc:attributionName xml:lang="en">English Heritage</cc:attributionName>
				<dcterms:publisher rdf:resource="http://www.english-heritage.org.uk" />
			</skos:Concept>
		</skos:narrower>
		<skos:narrower>
			<skos:Concept rdf:about="http://purl.org/heritagedata/schemes/560/concepts/142202">
				<skos:inScheme rdf:resource="http://purl.org/heritagedata/schemes/560" />
				<dcterms:identifier>http://purl.org/heritagedata/schemes/560/concepts/142202</dcterms:identifier>
				<skos:prefLabel xml:lang="en">TEPHROCHRONOLOGY</skos:prefLabel>
				<dcterms:issued rdf:datatype="http://www.w3.org/2001/XMLSchema#dateTime">2013-07-17T09:02:45</dcterms:issued>
				<skos:broader rdf:resource="http://purl.org/heritagedata/schemes/560/concepts/142128" />
				<skos:scopeNote xml:lang="en">The use of ash and tephra deposits characteristic of single known-date volcanic eruptions to date stratigraphic sequences.</skos:scopeNote>
				<cc:license rdf:resource="http://creativecommons.org/licenses/by/3.0" />
				<cc:attributionURL rdf:resource="http://www.english-heritage.org.uk" />
				<cc:attributionName xml:lang="en">English Heritage</cc:attributionName>
				<dcterms:publisher rdf:resource="http://www.english-heritage.org.uk" />
			</skos:Concept>
		</skos:narrower>
		<skos:narrower>
			<skos:Concept rdf:about="http://purl.org/heritagedata/schemes/560/concepts/142212">
				<skos:inScheme rdf:resource="http://purl.org/heritagedata/schemes/560" />
				<dcterms:identifier>http://purl.org/heritagedata/schemes/560/concepts/142212</dcterms:identifier>
				<skos:prefLabel xml:lang="en">URANIUM SERIES DATING</skos:prefLabel>
				<dcterms:issued rdf:datatype="http://www.w3.org/2001/XMLSchema#dateTime">2013-07-17T09:02:45</dcterms:issued>
				<skos:broader rdf:resource="http://purl.org/heritagedata/schemes/560/concepts/142128" />
				<skos:scopeNote xml:lang="en">The measurement of the decay of radioactive uranium (U) isotopes. Particularly useful for dating calcite and sometimes bone, tooth and shell up to 70,000 years old.</skos:scopeNote>
				<cc:license rdf:resource="http://creativecommons.org/licenses/by/3.0" />
				<cc:attributionURL rdf:resource="http://www.english-heritage.org.uk" />
				<cc:attributionName xml:lang="en">English Heritage</cc:attributionName>
				<dcterms:publisher rdf:resource="http://www.english-heritage.org.uk" />
			</skos:Concept>
		</skos:narrower>
		<skos:scopeNote xml:lang="en">Techniques applied to a material in order to date it or material associated with it. Use more specific terms.</skos:scopeNote>
		<cc:license rdf:resource="http://creativecommons.org/licenses/by/3.0" />
		<cc:attributionURL rdf:resource="http://www.english-heritage.org.uk" />
		<cc:attributionName xml:lang="en">English Heritage</cc:attributionName>
		<dcterms:publisher rdf:resource="http://www.english-heritage.org.uk" />
	</skos:Concept>
	<skos:Concept rdf:about="http://purl.org/heritagedata/schemes/560/concepts/142131">
		<skos:inScheme rdf:resource="http://purl.org/heritagedata/schemes/560" />
		<dcterms:identifier>http://purl.org/heritagedata/schemes/560/concepts/142131</dcterms:identifier>
		<skos:prefLabel xml:lang="en">DENDROCHRONOLOGY</skos:prefLabel>
		<dcterms:issued rdf:datatype="http://www.w3.org/2001/XMLSchema#dateTime">2013-07-17T09:02:45</dcterms:issued>
		<skos:broader rdf:resource="http://purl.org/heritagedata/schemes/560/concepts/142128" />
		<skos:related rdf:resource="http://purl.org/heritagedata/schemes/560/concepts/142209" />
		<skos:scopeNote xml:lang="en">The measuring of annual tree-ring growth shown by most tree species in temperated regions. Regional chronoliges are required to date any particular piece of wood, the longest of which, for Germany, works for the present to approximately 14,000 yrs ago.</skos:scopeNote>
		<cc:license rdf:resource="http://creativecommons.org/licenses/by/3.0" />
		<cc:attributionURL rdf:resource="http://www.english-heritage.org.uk" />
		<cc:attributionName xml:lang="en">English Heritage</cc:attributionName>
		<dcterms:publisher rdf:resource="http://www.english-heritage.org.uk" />
	</skos:Concept>
	<skos:Concept rdf:about="http://purl.org/heritagedata/schemes/560/concepts/142148">
		<skos:inScheme rdf:resource="http://purl.org/heritagedata/schemes/560" />
		<dcterms:identifier>http://purl.org/heritagedata/schemes/560/concepts/142148</dcterms:identifier>
		<skos:prefLabel xml:lang="en">HUMAN ASPECTS</skos:prefLabel>
		<dcterms:issued rdf:datatype="http://www.w3.org/2001/XMLSchema#dateTime">2013-07-17T09:02:45</dcterms:issued>
		<skos:broader rdf:resource="http://purl.org/heritagedata/schemes/560/concepts/142105" />
		<skos:narrower>
			<skos:Concept rdf:about="http://purl.org/heritagedata/schemes/560/concepts/142159">
				<skos:inScheme rdf:resource="http://purl.org/heritagedata/schemes/560" />
				<dcterms:identifier>http://purl.org/heritagedata/schemes/560/concepts/142159</dcterms:identifier>
				<skos:prefLabel xml:lang="en">MANUFACTURING DEBRIS</skos:prefLabel>
				<dcterms:issued rdf:datatype="http://www.w3.org/2001/XMLSchema#dateTime">2013-07-17T09:02:45</dcterms:issued>
				<skos:broader rdf:resource="http://purl.org/heritagedata/schemes/560/concepts/142148" />
				<skos:scopeNote xml:lang="en">Use where the material presents debris or waste from manufacturing.</skos:scopeNote>
				<cc:license rdf:resource="http://creativecommons.org/licenses/by/3.0" />
				<cc:attributionURL rdf:resource="http://www.english-heritage.org.uk" />
				<cc:attributionName xml:lang="en">English Heritage</cc:attributionName>
				<dcterms:publisher rdf:resource="http://www.english-heritage.org.uk" />
			</skos:Concept>
		</skos:narrower>
		<skos:narrower rdf:resource="http://purl.org/heritagedata/schemes/560/concepts/142215" />
		<skos:scopeNote xml:lang="en">Aspects of a material which result from the modification or use of the material by humans.</skos:scopeNote>
		<cc:license rdf:resource="http://creativecommons.org/licenses/by/3.0" />
		<cc:attributionURL rdf:resource="http://www.english-heritage.org.uk" />
		<cc:attributionName xml:lang="en">English Heritage</cc:attributionName>
		<dcterms:publisher rdf:resource="http://www.english-heritage.org.uk" />
	</skos:Concept>
	<skos:Concept rdf:about="http://purl.org/heritagedata/schemes/560/concepts/142156">
		<skos:inScheme rdf:resource="http://purl.org/heritagedata/schemes/560" />
		<dcterms:identifier>http://purl.org/heritagedata/schemes/560/concepts/142156</dcterms:identifier>
		<skos:prefLabel xml:lang="en">LEATHER</skos:prefLabel>
		<dcterms:issued rdf:datatype="http://www.w3.org/2001/XMLSchema#dateTime">2013-07-17T09:02:45</dcterms:issued>
		<skos:broader rdf:resource="http://purl.org/heritagedata/schemes/560/concepts/142160" />
		<skos:related rdf:resource="http://purl.org/heritagedata/schemes/560/concepts/142196" />
		<skos:scopeNote xml:lang="en">Animal skin that has been tanned or tawed.</skos:scopeNote>
		<cc:license rdf:resource="http://creativecommons.org/licenses/by/3.0" />
		<cc:attributionURL rdf:resource="http://www.english-heritage.org.uk" />
		<cc:attributionName xml:lang="en">English Heritage</cc:attributionName>
		<dcterms:publisher rdf:resource="http://www.english-heritage.org.uk" />
	</skos:Concept>
	<skos:Concept rdf:about="http://purl.org/heritagedata/schemes/560/concepts/142161">
		<skos:inScheme rdf:resource="http://purl.org/heritagedata/schemes/560" />
		<dcterms:identifier>http://purl.org/heritagedata/schemes/560/concepts/142161</dcterms:identifier>
		<skos:prefLabel xml:lang="en">METAL</skos:prefLabel>
		<dcterms:issued rdf:datatype="http://www.w3.org/2001/XMLSchema#dateTime">2013-07-17T09:02:45</dcterms:issued>
		<skos:narrower>
			<skos:Concept rdf:about="http://purl.org/heritagedata/schemes/560/concepts/142138">
				<skos:inScheme rdf:resource="http://purl.org/heritagedata/schemes/560" />
				<dcterms:identifier>http://purl.org/heritagedata/schemes/560/concepts/142138</dcterms:identifier>
				<skos:prefLabel xml:lang="en">FERROUS METAL</skos:prefLabel>
				<dcterms:issued rdf:datatype="http://www.w3.org/2001/XMLSchema#dateTime">2013-07-17T09:02:45</dcterms:issued>
				<skos:broader rdf:resource="http://purl.org/heritagedata/schemes/560/concepts/142161" />
				<skos:scopeNote xml:lang="en">Any metal prinicipally composed of the chemical element Iron (Fe).</skos:scopeNote>
				<cc:license rdf:resource="http://creativecommons.org/licenses/by/3.0" />
				<cc:attributionURL rdf:resource="http://www.english-heritage.org.uk" />
				<cc:attributionName xml:lang="en">English Heritage</cc:attributionName>
				<dcterms:publisher rdf:resource="http://www.english-heritage.org.uk" />
			</skos:Concept>
		</skos:narrower>
		<skos:broader rdf:resource="http://purl.org/heritagedata/schemes/560/concepts/142160" />
		<skos:narrower rdf:resource="http://purl.org/heritagedata/schemes/560/concepts/142174" />
		<skos:scopeNote xml:lang="en">Class of elements and alloys that are characteristically lustrous, ductile, fusible and malleable. These are extracted from ore minerals originally existing in nature and processed before becoming a recognisable metal.</skos:scopeNote>
		<cc:license rdf:resource="http://creativecommons.org/licenses/by/3.0" />
		<cc:attributionURL rdf:resource="http://www.english-heritage.org.uk" />
		<cc:attributionName xml:lang="en">English Heritage</cc:attributionName>
		<dcterms:publisher rdf:resource="http://www.english-heritage.org.uk" />
	</skos:Concept>
	<skos:Concept rdf:about="http://purl.org/heritagedata/schemes/560/concepts/142165">
		<skos:inScheme rdf:resource="http://purl.org/heritagedata/schemes/560" />
		<dcterms:identifier>http://purl.org/heritagedata/schemes/560/concepts/142165</dcterms:identifier>
		<skos:prefLabel xml:lang="en">MICROSCOPY</skos:prefLabel>
		<dcterms:issued rdf:datatype="http://www.w3.org/2001/XMLSchema#dateTime">2013-07-17T09:02:45</dcterms:issued>
		<skos:broader rdf:resource="http://purl.org/heritagedata/schemes/560/concepts/142182" />
		<skos:narrower>
			<skos:Concept rdf:about="http://purl.org/heritagedata/schemes/560/concepts/142185">
				<skos:inScheme rdf:resource="http://purl.org/heritagedata/schemes/560" />
				<dcterms:identifier>http://purl.org/heritagedata/schemes/560/concepts/142185</dcterms:identifier>
				<skos:prefLabel xml:lang="en">POLARISED LIGHT MICROSCOPY</skos:prefLabel>
				<dcterms:issued rdf:datatype="http://www.w3.org/2001/XMLSchema#dateTime">2013-07-17T09:02:45</dcterms:issued>
				<skos:broader rdf:resource="http://purl.org/heritagedata/schemes/560/concepts/142165" />
				<skos:scopeNote xml:lang="en">Light microscopy in which vibration directions of the light are constrained into single planes.</skos:scopeNote>
				<cc:license rdf:resource="http://creativecommons.org/licenses/by/3.0" />
				<cc:attributionURL rdf:resource="http://www.english-heritage.org.uk" />
				<cc:attributionName xml:lang="en">English Heritage</cc:attributionName>
				<dcterms:publisher rdf:resource="http://www.english-heritage.org.uk" />
			</skos:Concept>
		</skos:narrower>
		<skos:narrower>
			<skos:Concept rdf:about="http://purl.org/heritagedata/schemes/560/concepts/142191">
				<skos:inScheme rdf:resource="http://purl.org/heritagedata/schemes/560" />
				<dcterms:identifier>http://purl.org/heritagedata/schemes/560/concepts/142191</dcterms:identifier>
				<skos:prefLabel xml:lang="en">SCANNING ELECTRON MICROSCOPY</skos:prefLabel>
				<dcterms:issued rdf:datatype="http://www.w3.org/2001/XMLSchema#dateTime">2013-07-17T09:02:45</dcterms:issued>
				<skos:altLabel xml:lang="en">S.E.M.</skos:altLabel>
				<skos:altLabel xml:lang="en">Sem</skos:altLabel>
				<skos:broader rdf:resource="http://purl.org/heritagedata/schemes/560/concepts/142165" />
				<skos:scopeNote xml:lang="en">A process using an electron microscope in which the surface of the specimen is scanned by a beam of electrons which are reflected to form an image. Very high magnification is possible.</skos:scopeNote>
				<cc:license rdf:resource="http://creativecommons.org/licenses/by/3.0" />
				<cc:attributionURL rdf:resource="http://www.english-heritage.org.uk" />
				<cc:attributionName xml:lang="en">English Heritage</cc:attributionName>
				<dcterms:publisher rdf:resource="http://www.english-heritage.org.uk" />
			</skos:Concept>
		</skos:narrower>
		<skos:scopeNote xml:lang="en">The use of magnifying equipment to examine materials not visible to the naked eye.</skos:scopeNote>
		<cc:license rdf:resource="http://creativecommons.org/licenses/by/3.0" />
		<cc:attributionURL rdf:resource="http://www.english-heritage.org.uk" />
		<cc:attributionName xml:lang="en">English Heritage</cc:attributionName>
		<dcterms:publisher rdf:resource="http://www.english-heritage.org.uk" />
	</skos:Concept>
	<skos:Concept rdf:about="http://purl.org/heritagedata/schemes/560/concepts/142172">
		<skos:inScheme rdf:resource="http://purl.org/heritagedata/schemes/560" />
		<dcterms:identifier>http://purl.org/heritagedata/schemes/560/concepts/142172</dcterms:identifier>
		<skos:prefLabel xml:lang="en">MULTI-ELEMENT ANALYSIS</skos:prefLabel>
		<dcterms:issued rdf:datatype="http://www.w3.org/2001/XMLSchema#dateTime">2013-07-17T09:02:45</dcterms:issued>
		<skos:broader rdf:resource="http://purl.org/heritagedata/schemes/560/concepts/142119" />
		<skos:narrower>
			<skos:Concept rdf:about="http://purl.org/heritagedata/schemes/560/concepts/142217">
				<skos:inScheme rdf:resource="http://purl.org/heritagedata/schemes/560" />
				<dcterms:identifier>http://purl.org/heritagedata/schemes/560/concepts/142217</dcterms:identifier>
				<skos:prefLabel xml:lang="en">X-RAY DIFFRACTION</skos:prefLabel>
				<dcterms:issued rdf:datatype="http://www.w3.org/2001/XMLSchema#dateTime">2013-07-17T09:02:45</dcterms:issued>
				<skos:altLabel xml:lang="en">Xrd</skos:altLabel>
				<skos:broader rdf:resource="http://purl.org/heritagedata/schemes/560/concepts/142172" />
				<skos:scopeNote xml:lang="en">A surface technique that uses the diffraction of X-rays to examine the mineral composition of a sample. Useful for identifying corrosion products, pigments etc. but of little use with organic compounds which consist largely of carbon, oxygen and hydrogen.</skos:scopeNote>
				<cc:license rdf:resource="http://creativecommons.org/licenses/by/3.0" />
				<cc:attributionURL rdf:resource="http://www.english-heritage.org.uk" />
				<cc:attributionName xml:lang="en">English Heritage</cc:attributionName>
				<dcterms:publisher rdf:resource="http://www.english-heritage.org.uk" />
			</skos:Concept>
		</skos:narrower>
		<skos:narrower>
			<skos:Concept rdf:about="http://purl.org/heritagedata/schemes/560/concepts/142218">
				<skos:inScheme rdf:resource="http://purl.org/heritagedata/schemes/560" />
				<dcterms:identifier>http://purl.org/heritagedata/schemes/560/concepts/142218</dcterms:identifier>
				<skos:prefLabel xml:lang="en">X-RAY FLUORESCENCE SPECTROMETRY</skos:prefLabel>
				<dcterms:issued rdf:datatype="http://www.w3.org/2001/XMLSchema#dateTime">2013-07-17T09:02:45</dcterms:issued>
				<skos:altLabel xml:lang="en">Xrf</skos:altLabel>
				<skos:broader rdf:resource="http://purl.org/heritagedata/schemes/560/concepts/142172" />
				<skos:scopeNote xml:lang="en">A surface technique of spectroscopic analysis which relies on the interaction of primary X-rays with the sample to generate a range of secondary X-rays. These have energies characteristic of the elements present in the sample.</skos:scopeNote>
				<cc:license rdf:resource="http://creativecommons.org/licenses/by/3.0" />
				<cc:attributionURL rdf:resource="http://www.english-heritage.org.uk" />
				<cc:attributionName xml:lang="en">English Heritage</cc:attributionName>
				<dcterms:publisher rdf:resource="http://www.english-heritage.org.uk" />
			</skos:Concept>
		</skos:narrower>
		<skos:scopeNote xml:lang="en">Techniques investigating more than one element at a time.</skos:scopeNote>
		<cc:license rdf:resource="http://creativecommons.org/licenses/by/3.0" />
		<cc:attributionURL rdf:resource="http://www.english-heritage.org.uk" />
		<cc:attributionName xml:lang="en">English Heritage</cc:attributionName>
		<dcterms:publisher rdf:resource="http://www.english-heritage.org.uk" />
	</skos:Concept>
	<skos:Concept rdf:about="http://purl.org/heritagedata/schemes/560/concepts/142173">
		<skos:inScheme rdf:resource="http://purl.org/heritagedata/schemes/560" />
		<dcterms:identifier>http://purl.org/heritagedata/schemes/560/concepts/142173</dcterms:identifier>
		<skos:prefLabel xml:lang="en">NATURAL ASPECTS</skos:prefLabel>
		<dcterms:issued rdf:datatype="http://www.w3.org/2001/XMLSchema#dateTime">2013-07-17T09:02:45</dcterms:issued>
		<skos:broader rdf:resource="http://purl.org/heritagedata/schemes/560/concepts/142105" />
		<skos:narrower>
			<skos:Concept rdf:about="http://purl.org/heritagedata/schemes/560/concepts/142175">
				<skos:inScheme rdf:resource="http://purl.org/heritagedata/schemes/560" />
				<dcterms:identifier>http://purl.org/heritagedata/schemes/560/concepts/142175</dcterms:identifier>
				<skos:prefLabel xml:lang="en">NON-METRIC TRAITS</skos:prefLabel>
				<dcterms:issued rdf:datatype="http://www.w3.org/2001/XMLSchema#dateTime">2013-07-17T09:02:45</dcterms:issued>
				<skos:broader rdf:resource="http://purl.org/heritagedata/schemes/560/concepts/142173" />
				<skos:scopeNote xml:lang="en">Use for congenital (present at birth) abnormalities (absent/extra or morphologically unusual features) present in an individual or population.</skos:scopeNote>
				<cc:license rdf:resource="http://creativecommons.org/licenses/by/3.0" />
				<cc:attributionURL rdf:resource="http://www.english-heritage.org.uk" />
				<cc:attributionName xml:lang="en">English Heritage</cc:attributionName>
				<dcterms:publisher rdf:resource="http://www.english-heritage.org.uk" />
			</skos:Concept>
		</skos:narrower>
		<skos:narrower>
			<skos:Concept rdf:about="http://purl.org/heritagedata/schemes/560/concepts/142180">
				<skos:inScheme rdf:resource="http://purl.org/heritagedata/schemes/560" />
				<dcterms:identifier>http://purl.org/heritagedata/schemes/560/concepts/142180</dcterms:identifier>
				<skos:prefLabel xml:lang="en">PATHOLOGY</skos:prefLabel>
				<dcterms:issued rdf:datatype="http://www.w3.org/2001/XMLSchema#dateTime">2013-07-17T09:02:45</dcterms:issued>
				<skos:altLabel xml:lang="en">Disease</skos:altLabel>
				<skos:altLabel xml:lang="en">Diseased</skos:altLabel>
				<skos:broader rdf:resource="http://purl.org/heritagedata/schemes/560/concepts/142173" />
				<skos:scopeNote xml:lang="en">Use for bone remodelling, new growth, loss or destruction caused by age, activity, disease or trauma during life.</skos:scopeNote>
				<cc:license rdf:resource="http://creativecommons.org/licenses/by/3.0" />
				<cc:attributionURL rdf:resource="http://www.english-heritage.org.uk" />
				<cc:attributionName xml:lang="en">English Heritage</cc:attributionName>
				<dcterms:publisher rdf:resource="http://www.english-heritage.org.uk" />
			</skos:Concept>
		</skos:narrower>
		<skos:scopeNote xml:lang="en">Aspects associated with the genetic make up and/or factors that affected the organism from which the material is derived during its life</skos:scopeNote>
		<cc:license rdf:resource="http://creativecommons.org/licenses/by/3.0" />
		<cc:attributionURL rdf:resource="http://www.english-heritage.org.uk" />
		<cc:attributionName xml:lang="en">English Heritage</cc:attributionName>
		<dcterms:publisher rdf:resource="http://www.english-heritage.org.uk" />
	</skos:Concept>
	<skos:Concept rdf:about="http://purl.org/heritagedata/schemes/560/concepts/142174">
		<skos:inScheme rdf:resource="http://purl.org/heritagedata/schemes/560" />
		<dcterms:identifier>http://purl.org/heritagedata/schemes/560/concepts/142174</dcterms:identifier>
		<skos:prefLabel xml:lang="en">NON-FERROUS METAL</skos:prefLabel>
		<dcterms:issued rdf:datatype="http://www.w3.org/2001/XMLSchema#dateTime">2013-07-17T09:02:45</dcterms:issued>
		<skos:narrower>
			<skos:Concept rdf:about="http://purl.org/heritagedata/schemes/560/concepts/142125">
				<skos:inScheme rdf:resource="http://purl.org/heritagedata/schemes/560" />
				<dcterms:identifier>http://purl.org/heritagedata/schemes/560/concepts/142125</dcterms:identifier>
				<skos:prefLabel xml:lang="en">COPPER ALLOY</skos:prefLabel>
				<dcterms:issued rdf:datatype="http://www.w3.org/2001/XMLSchema#dateTime">2013-07-17T09:02:45</dcterms:issued>
				<skos:broader rdf:resource="http://purl.org/heritagedata/schemes/560/concepts/142174" />
				<skos:scopeNote xml:lang="en">Use for a combination (alloy) of two or more different metals where copper (Cu) is the principal component.</skos:scopeNote>
				<cc:license rdf:resource="http://creativecommons.org/licenses/by/3.0" />
				<cc:attributionURL rdf:resource="http://www.english-heritage.org.uk" />
				<cc:attributionName xml:lang="en">English Heritage</cc:attributionName>
				<dcterms:publisher rdf:resource="http://www.english-heritage.org.uk" />
			</skos:Concept>
		</skos:narrower>
		<skos:narrower>
			<skos:Concept rdf:about="http://purl.org/heritagedata/schemes/560/concepts/142145">
				<skos:inScheme rdf:resource="http://purl.org/heritagedata/schemes/560" />
				<dcterms:identifier>http://purl.org/heritagedata/schemes/560/concepts/142145</dcterms:identifier>
				<skos:prefLabel xml:lang="en">GOLD</skos:prefLabel>
				<dcterms:issued rdf:datatype="http://www.w3.org/2001/XMLSchema#dateTime">2013-07-17T09:02:45</dcterms:issued>
				<skos:broader rdf:resource="http://purl.org/heritagedata/schemes/560/concepts/142174" />
				<skos:scopeNote xml:lang="en">A precious metal characterised by its yellow colour and resistance to tarnishing.</skos:scopeNote>
				<cc:license rdf:resource="http://creativecommons.org/licenses/by/3.0" />
				<cc:attributionURL rdf:resource="http://www.english-heritage.org.uk" />
				<cc:attributionName xml:lang="en">English Heritage</cc:attributionName>
				<dcterms:publisher rdf:resource="http://www.english-heritage.org.uk" />
			</skos:Concept>
		</skos:narrower>
		<skos:broader rdf:resource="http://purl.org/heritagedata/schemes/560/concepts/142161" />
		<skos:narrower>
			<skos:Concept rdf:about="http://purl.org/heritagedata/schemes/560/concepts/142195">
				<skos:inScheme rdf:resource="http://purl.org/heritagedata/schemes/560" />
				<dcterms:identifier>http://purl.org/heritagedata/schemes/560/concepts/142195</dcterms:identifier>
				<skos:prefLabel xml:lang="en">SILVER</skos:prefLabel>
				<dcterms:issued rdf:datatype="http://www.w3.org/2001/XMLSchema#dateTime">2013-07-17T09:02:45</dcterms:issued>
				<skos:broader rdf:resource="http://purl.org/heritagedata/schemes/560/concepts/142174" />
				<skos:scopeNote xml:lang="en">A precious metal of lustrous, white colour with great malleability and ductility.</skos:scopeNote>
				<cc:license rdf:resource="http://creativecommons.org/licenses/by/3.0" />
				<cc:attributionURL rdf:resource="http://www.english-heritage.org.uk" />
				<cc:attributionName xml:lang="en">English Heritage</cc:attributionName>
				<dcterms:publisher rdf:resource="http://www.english-heritage.org.uk" />
			</skos:Concept>
		</skos:narrower>
		<skos:scopeNote xml:lang="en">Any metal that does not contain the chemical element Iron (Fe) as a principal component.</skos:scopeNote>
		<cc:license rdf:resource="http://creativecommons.org/licenses/by/3.0" />
		<cc:attributionURL rdf:resource="http://www.english-heritage.org.uk" />
		<cc:attributionName xml:lang="en">English Heritage</cc:attributionName>
		<dcterms:publisher rdf:resource="http://www.english-heritage.org.uk" />
	</skos:Concept>
	<skos:Concept rdf:about="http://purl.org/heritagedata/schemes/560/concepts/142182">
		<skos:inScheme rdf:resource="http://purl.org/heritagedata/schemes/560" />
		<dcterms:identifier>http://purl.org/heritagedata/schemes/560/concepts/142182</dcterms:identifier>
		<skos:prefLabel xml:lang="en">PHYSICAL TECHNIQUES</skos:prefLabel>
		<dcterms:issued rdf:datatype="http://www.w3.org/2001/XMLSchema#dateTime">2013-07-17T09:02:45</dcterms:issued>
		<skos:narrower>
			<skos:Concept rdf:about="http://purl.org/heritagedata/schemes/560/concepts/142121">
				<skos:inScheme rdf:resource="http://purl.org/heritagedata/schemes/560" />
				<dcterms:identifier>http://purl.org/heritagedata/schemes/560/concepts/142121</dcterms:identifier>
				<skos:prefLabel xml:lang="en">CLAST LITHOLOGICAL ANALYSIS</skos:prefLabel>
				<dcterms:issued rdf:datatype="http://www.w3.org/2001/XMLSchema#dateTime">2013-07-17T09:02:45</dcterms:issued>
				<skos:broader rdf:resource="http://purl.org/heritagedata/schemes/560/concepts/142182" />
				<skos:scopeNote xml:lang="en">The identification and grouping of stone types in stratigraphy.</skos:scopeNote>
				<cc:license rdf:resource="http://creativecommons.org/licenses/by/3.0" />
				<cc:attributionURL rdf:resource="http://www.english-heritage.org.uk" />
				<cc:attributionName xml:lang="en">English Heritage</cc:attributionName>
				<dcterms:publisher rdf:resource="http://www.english-heritage.org.uk" />
			</skos:Concept>
		</skos:narrower>
		<skos:narrower>
			<skos:Concept rdf:about="http://purl.org/heritagedata/schemes/560/concepts/142157">
				<skos:inScheme rdf:resource="http://purl.org/heritagedata/schemes/560" />
				<dcterms:identifier>http://purl.org/heritagedata/schemes/560/concepts/142157</dcterms:identifier>
				<skos:prefLabel xml:lang="en">LOSS ON IGNITION DETERMINATION</skos:prefLabel>
				<dcterms:issued rdf:datatype="http://www.w3.org/2001/XMLSchema#dateTime">2013-07-17T09:02:45</dcterms:issued>
				<skos:broader rdf:resource="http://purl.org/heritagedata/schemes/560/concepts/142182" />
				<skos:scopeNote xml:lang="en">The weight loss from low-temperature burning of material. It correlates well with organic matter (material derived from living things) content.</skos:scopeNote>
				<cc:license rdf:resource="http://creativecommons.org/licenses/by/3.0" />
				<cc:attributionURL rdf:resource="http://www.english-heritage.org.uk" />
				<cc:attributionName xml:lang="en">English Heritage</cc:attributionName>
				<dcterms:publisher rdf:resource="http://www.english-heritage.org.uk" />
			</skos:Concept>
		</skos:narrower>
		<skos:narrower>
			<skos:Concept rdf:about="http://purl.org/heritagedata/schemes/560/concepts/142158">
				<skos:inScheme rdf:resource="http://purl.org/heritagedata/schemes/560" />
				<dcterms:identifier>http://purl.org/heritagedata/schemes/560/concepts/142158</dcterms:identifier>
				<skos:prefLabel xml:lang="en">MAGNETIC SUSCEPTIBILITY</skos:prefLabel>
				<dcterms:issued rdf:datatype="http://www.w3.org/2001/XMLSchema#dateTime">2013-07-17T09:02:45</dcterms:issued>
				<skos:broader rdf:resource="http://purl.org/heritagedata/schemes/560/concepts/142182" />
				<skos:scopeNote xml:lang="en">The degree to which a material will become magnetised when placed in a magnetic field.</skos:scopeNote>
				<cc:license rdf:resource="http://creativecommons.org/licenses/by/3.0" />
				<cc:attributionURL rdf:resource="http://www.english-heritage.org.uk" />
				<cc:attributionName xml:lang="en">English Heritage</cc:attributionName>
				<dcterms:publisher rdf:resource="http://www.english-heritage.org.uk" />
			</skos:Concept>
		</skos:narrower>
		<skos:narrower>
			<skos:Concept rdf:about="http://purl.org/heritagedata/schemes/560/concepts/142164">
				<skos:inScheme rdf:resource="http://purl.org/heritagedata/schemes/560" />
				<dcterms:identifier>http://purl.org/heritagedata/schemes/560/concepts/142164</dcterms:identifier>
				<skos:prefLabel xml:lang="en">MICROMORPHOLOGY</skos:prefLabel>
				<dcterms:issued rdf:datatype="http://www.w3.org/2001/XMLSchema#dateTime">2013-07-17T09:02:45</dcterms:issued>
				<skos:broader rdf:resource="http://purl.org/heritagedata/schemes/560/concepts/142182" />
				<skos:scopeNote xml:lang="en">The microscopic analysis of thin sections of resin impregnated stratigraphy.</skos:scopeNote>
				<cc:license rdf:resource="http://creativecommons.org/licenses/by/3.0" />
				<cc:attributionURL rdf:resource="http://www.english-heritage.org.uk" />
				<cc:attributionName xml:lang="en">English Heritage</cc:attributionName>
				<dcterms:publisher rdf:resource="http://www.english-heritage.org.uk" />
			</skos:Concept>
		</skos:narrower>
		<skos:narrower rdf:resource="http://purl.org/heritagedata/schemes/560/concepts/142165" />
		<skos:narrower>
			<skos:Concept rdf:about="http://purl.org/heritagedata/schemes/560/concepts/142169">
				<skos:inScheme rdf:resource="http://purl.org/heritagedata/schemes/560" />
				<dcterms:identifier>http://purl.org/heritagedata/schemes/560/concepts/142169</dcterms:identifier>
				<skos:prefLabel xml:lang="en">MINERALOGY</skos:prefLabel>
				<dcterms:issued rdf:datatype="http://www.w3.org/2001/XMLSchema#dateTime">2013-07-17T09:02:45</dcterms:issued>
				<skos:broader rdf:resource="http://purl.org/heritagedata/schemes/560/concepts/142182" />
				<skos:scopeNote xml:lang="en">The study of minerals.</skos:scopeNote>
				<cc:license rdf:resource="http://creativecommons.org/licenses/by/3.0" />
				<cc:attributionURL rdf:resource="http://www.english-heritage.org.uk" />
				<cc:attributionName xml:lang="en">English Heritage</cc:attributionName>
				<dcterms:publisher rdf:resource="http://www.english-heritage.org.uk" />
			</skos:Concept>
		</skos:narrower>
		<skos:narrower>
			<skos:Concept rdf:about="http://purl.org/heritagedata/schemes/560/concepts/147277">
				<skos:inScheme rdf:resource="http://purl.org/heritagedata/schemes/560" />
				<dcterms:identifier>http://purl.org/heritagedata/schemes/560/concepts/147277</dcterms:identifier>
				<skos:prefLabel xml:lang="en">MOISTURE CONTENT</skos:prefLabel>
				<dcterms:issued rdf:datatype="http://www.w3.org/2001/XMLSchema#dateTime">2013-07-17T09:02:45</dcterms:issued>
				<skos:broader rdf:resource="http://purl.org/heritagedata/schemes/560/concepts/142182" />
				<skos:scopeNote xml:lang="en">A measure of the proportion of water within a sample.</skos:scopeNote>
				<cc:license rdf:resource="http://creativecommons.org/licenses/by/3.0" />
				<cc:attributionURL rdf:resource="http://www.english-heritage.org.uk" />
				<cc:attributionName xml:lang="en">English Heritage</cc:attributionName>
				<dcterms:publisher rdf:resource="http://www.english-heritage.org.uk" />
			</skos:Concept>
		</skos:narrower>
		<skos:narrower>
			<skos:Concept rdf:about="http://purl.org/heritagedata/schemes/560/concepts/142179">
				<skos:inScheme rdf:resource="http://purl.org/heritagedata/schemes/560" />
				<dcterms:identifier>http://purl.org/heritagedata/schemes/560/concepts/142179</dcterms:identifier>
				<skos:prefLabel xml:lang="en">PARTICLE SIZE ANALYSIS</skos:prefLabel>
				<dcterms:issued rdf:datatype="http://www.w3.org/2001/XMLSchema#dateTime">2013-07-17T09:02:45</dcterms:issued>
				<skos:broader rdf:resource="http://purl.org/heritagedata/schemes/560/concepts/142182" />
				<skos:scopeNote xml:lang="en">The analysis of the distribution and proportion of sand, silt and clay in a deposit.</skos:scopeNote>
				<cc:license rdf:resource="http://creativecommons.org/licenses/by/3.0" />
				<cc:attributionURL rdf:resource="http://www.english-heritage.org.uk" />
				<cc:attributionName xml:lang="en">English Heritage</cc:attributionName>
				<dcterms:publisher rdf:resource="http://www.english-heritage.org.uk" />
			</skos:Concept>
		</skos:narrower>
		<skos:broader rdf:resource="http://purl.org/heritagedata/schemes/560/concepts/142153" />
		<skos:narrower>
			<skos:Concept rdf:about="http://purl.org/heritagedata/schemes/560/concepts/142201">
				<skos:inScheme rdf:resource="http://purl.org/heritagedata/schemes/560" />
				<dcterms:identifier>http://purl.org/heritagedata/schemes/560/concepts/142201</dcterms:identifier>
				<skos:prefLabel xml:lang="en">STRATIGRAPHIC DESCRIPTION</skos:prefLabel>
				<dcterms:issued rdf:datatype="http://www.w3.org/2001/XMLSchema#dateTime">2013-07-17T09:02:45</dcterms:issued>
				<skos:broader rdf:resource="http://purl.org/heritagedata/schemes/560/concepts/142182" />
				<skos:scopeNote xml:lang="en">The careful observation and written description of the physical characteristics of stratigraphy. It will normally include information on texture, colour and the nature of the different components.</skos:scopeNote>
				<cc:license rdf:resource="http://creativecommons.org/licenses/by/3.0" />
				<cc:attributionURL rdf:resource="http://www.english-heritage.org.uk" />
				<cc:attributionName xml:lang="en">English Heritage</cc:attributionName>
				<dcterms:publisher rdf:resource="http://www.english-heritage.org.uk" />
			</skos:Concept>
		</skos:narrower>
		<skos:narrower rdf:resource="http://purl.org/heritagedata/schemes/560/concepts/142209" />
		<skos:narrower>
			<skos:Concept rdf:about="http://purl.org/heritagedata/schemes/560/concepts/142216">
				<skos:inScheme rdf:resource="http://purl.org/heritagedata/schemes/560" />
				<dcterms:identifier>http://purl.org/heritagedata/schemes/560/concepts/142216</dcterms:identifier>
				<skos:prefLabel xml:lang="en">X-RADIOGRAPHY</skos:prefLabel>
				<dcterms:issued rdf:datatype="http://www.w3.org/2001/XMLSchema#dateTime">2013-07-17T09:02:45</dcterms:issued>
				<skos:broader rdf:resource="http://purl.org/heritagedata/schemes/560/concepts/142182" />
				<skos:scopeNote xml:lang="en">The production of an image on a photographic plate as a result of X-rays (very short wavelength electromagnetic radiation) being passed through an object.</skos:scopeNote>
				<cc:license rdf:resource="http://creativecommons.org/licenses/by/3.0" />
				<cc:attributionURL rdf:resource="http://www.english-heritage.org.uk" />
				<cc:attributionName xml:lang="en">English Heritage</cc:attributionName>
				<dcterms:publisher rdf:resource="http://www.english-heritage.org.uk" />
			</skos:Concept>
		</skos:narrower>
		<skos:scopeNote xml:lang="en">The examination of material by physical means, including detailed observation.</skos:scopeNote>
		<cc:license rdf:resource="http://creativecommons.org/licenses/by/3.0" />
		<cc:attributionURL rdf:resource="http://www.english-heritage.org.uk" />
		<cc:attributionName xml:lang="en">English Heritage</cc:attributionName>
		<dcterms:publisher rdf:resource="http://www.english-heritage.org.uk" />
	</skos:Concept>
	<skos:Concept rdf:about="http://purl.org/heritagedata/schemes/560/concepts/142189">
		<skos:inScheme rdf:resource="http://purl.org/heritagedata/schemes/560" />
		<dcterms:identifier>http://purl.org/heritagedata/schemes/560/concepts/142189</dcterms:identifier>
		<skos:prefLabel xml:lang="en">ROUNDWOOD</skos:prefLabel>
		<dcterms:issued rdf:datatype="http://www.w3.org/2001/XMLSchema#dateTime">2013-07-17T09:02:45</dcterms:issued>
		<skos:broader rdf:resource="http://purl.org/heritagedata/schemes/560/concepts/142117" />
		<skos:broader rdf:resource="http://purl.org/heritagedata/schemes/560/concepts/142214" />
		<skos:scopeNote xml:lang="en">Material comprising entrie or partial transverse sections of stems. Bark may be present or not. Can include complete sections of tree trunk but generally comprises smaller (&lt;20cm diameter) material.</skos:scopeNote>
		<cc:license rdf:resource="http://creativecommons.org/licenses/by/3.0" />
		<cc:attributionURL rdf:resource="http://www.english-heritage.org.uk" />
		<cc:attributionName xml:lang="en">English Heritage</cc:attributionName>
		<dcterms:publisher rdf:resource="http://www.english-heritage.org.uk" />
	</skos:Concept>
	<skos:Concept rdf:about="http://purl.org/heritagedata/schemes/560/concepts/142196">
		<skos:inScheme rdf:resource="http://purl.org/heritagedata/schemes/560" />
		<dcterms:identifier>http://purl.org/heritagedata/schemes/560/concepts/142196</dcterms:identifier>
		<skos:prefLabel xml:lang="en">SKIN</skos:prefLabel>
		<dcterms:issued rdf:datatype="http://www.w3.org/2001/XMLSchema#dateTime">2013-07-17T09:02:45</dcterms:issued>
		<skos:broader rdf:resource="http://purl.org/heritagedata/schemes/560/concepts/142160" />
		<skos:related rdf:resource="http://purl.org/heritagedata/schemes/560/concepts/142156" />
		<skos:scopeNote xml:lang="en">Use for the remains of epidermis or outermost layer. Relates to both animals and plants. If describing the actual object use PLANT REMAINS, ANIMAL REMAINS or HUMAN REMAINS.</skos:scopeNote>
		<cc:license rdf:resource="http://creativecommons.org/licenses/by/3.0" />
		<cc:attributionURL rdf:resource="http://www.english-heritage.org.uk" />
		<cc:attributionName xml:lang="en">English Heritage</cc:attributionName>
		<dcterms:publisher rdf:resource="http://www.english-heritage.org.uk" />
	</skos:Concept>
	<skos:Concept rdf:about="http://purl.org/heritagedata/schemes/560/concepts/142197">
		<skos:inScheme rdf:resource="http://purl.org/heritagedata/schemes/560" />
		<dcterms:identifier>http://purl.org/heritagedata/schemes/560/concepts/142197</dcterms:identifier>
		<skos:prefLabel xml:lang="en">SOIL PHOSPHORUS ANALYSIS</skos:prefLabel>
		<dcterms:issued rdf:datatype="http://www.w3.org/2001/XMLSchema#dateTime">2013-07-17T09:02:45</dcterms:issued>
		<skos:narrower>
			<skos:Concept rdf:about="http://purl.org/heritagedata/schemes/560/concepts/142106">
				<skos:inScheme rdf:resource="http://purl.org/heritagedata/schemes/560" />
				<dcterms:identifier>http://purl.org/heritagedata/schemes/560/concepts/142106</dcterms:identifier>
				<skos:prefLabel xml:lang="en">AVAILABLE PHOSPHORUS ANALYSIS</skos:prefLabel>
				<dcterms:issued rdf:datatype="http://www.w3.org/2001/XMLSchema#dateTime">2013-07-17T09:02:45</dcterms:issued>
				<skos:broader rdf:resource="http://purl.org/heritagedata/schemes/560/concepts/142197" />
				<skos:scopeNote xml:lang="en">The analysis of the amount of phosphorus (P) (liable fraction) available to plants.</skos:scopeNote>
				<cc:license rdf:resource="http://creativecommons.org/licenses/by/3.0" />
				<cc:attributionURL rdf:resource="http://www.english-heritage.org.uk" />
				<cc:attributionName xml:lang="en">English Heritage</cc:attributionName>
				<dcterms:publisher rdf:resource="http://www.english-heritage.org.uk" />
			</skos:Concept>
		</skos:narrower>
		<skos:narrower>
			<skos:Concept rdf:about="http://purl.org/heritagedata/schemes/560/concepts/142152">
				<skos:inScheme rdf:resource="http://purl.org/heritagedata/schemes/560" />
				<dcterms:identifier>http://purl.org/heritagedata/schemes/560/concepts/142152</dcterms:identifier>
				<skos:prefLabel xml:lang="en">INORGANIC PHOSPHORUS ANALYSIS</skos:prefLabel>
				<dcterms:issued rdf:datatype="http://www.w3.org/2001/XMLSchema#dateTime">2013-07-17T09:02:45</dcterms:issued>
				<skos:broader rdf:resource="http://purl.org/heritagedata/schemes/560/concepts/142197" />
				<skos:scopeNote xml:lang="en">The analysis of inorganic phosphorus (P).</skos:scopeNote>
				<cc:license rdf:resource="http://creativecommons.org/licenses/by/3.0" />
				<cc:attributionURL rdf:resource="http://www.english-heritage.org.uk" />
				<cc:attributionName xml:lang="en">English Heritage</cc:attributionName>
				<dcterms:publisher rdf:resource="http://www.english-heritage.org.uk" />
			</skos:Concept>
		</skos:narrower>
		<skos:broader rdf:resource="http://purl.org/heritagedata/schemes/560/concepts/142119" />
		<skos:narrower>
			<skos:Concept rdf:about="http://purl.org/heritagedata/schemes/560/concepts/142208">
				<skos:inScheme rdf:resource="http://purl.org/heritagedata/schemes/560" />
				<dcterms:identifier>http://purl.org/heritagedata/schemes/560/concepts/142208</dcterms:identifier>
				<skos:prefLabel xml:lang="en">TOTAL PHOSPHORUS ANALYSIS</skos:prefLabel>
				<dcterms:issued rdf:datatype="http://www.w3.org/2001/XMLSchema#dateTime">2013-07-17T09:02:45</dcterms:issued>
				<skos:broader rdf:resource="http://purl.org/heritagedata/schemes/560/concepts/142197" />
				<skos:scopeNote xml:lang="en">The analysis of organic plus inorganic phosphorus (P).</skos:scopeNote>
				<cc:license rdf:resource="http://creativecommons.org/licenses/by/3.0" />
				<cc:attributionURL rdf:resource="http://www.english-heritage.org.uk" />
				<cc:attributionName xml:lang="en">English Heritage</cc:attributionName>
				<dcterms:publisher rdf:resource="http://www.english-heritage.org.uk" />
			</skos:Concept>
		</skos:narrower>
		<skos:scopeNote xml:lang="en">The analysis of the amount of phosphorus (P) present in a soil.</skos:scopeNote>
		<cc:license rdf:resource="http://creativecommons.org/licenses/by/3.0" />
		<cc:attributionURL rdf:resource="http://www.english-heritage.org.uk" />
		<cc:attributionName xml:lang="en">English Heritage</cc:attributionName>
		<dcterms:publisher rdf:resource="http://www.english-heritage.org.uk" />
	</skos:Concept>
	<skos:Concept rdf:about="http://purl.org/heritagedata/schemes/560/concepts/142207">
		<skos:inScheme rdf:resource="http://purl.org/heritagedata/schemes/560" />
		<dcterms:identifier>http://purl.org/heritagedata/schemes/560/concepts/142207</dcterms:identifier>
		<skos:prefLabel xml:lang="en">TOOTH</skos:prefLabel>
		<dcterms:issued rdf:datatype="http://www.w3.org/2001/XMLSchema#dateTime">2013-07-17T09:02:45</dcterms:issued>
		<skos:narrower>
			<skos:Concept rdf:about="http://purl.org/heritagedata/schemes/560/concepts/142154">
				<skos:inScheme rdf:resource="http://purl.org/heritagedata/schemes/560" />
				<dcterms:identifier>http://purl.org/heritagedata/schemes/560/concepts/142154</dcterms:identifier>
				<skos:prefLabel xml:lang="en">IVORY</skos:prefLabel>
				<dcterms:issued rdf:datatype="http://www.w3.org/2001/XMLSchema#dateTime">2013-07-17T09:02:45</dcterms:issued>
				<skos:broader rdf:resource="http://purl.org/heritagedata/schemes/560/concepts/142207" />
				<skos:scopeNote xml:lang="en">Use for a tusk or tooth of a mammal large enough to be carved or used to make objects such as those of mammoths, elephants, walruses and whales.</skos:scopeNote>
				<cc:license rdf:resource="http://creativecommons.org/licenses/by/3.0" />
				<cc:attributionURL rdf:resource="http://www.english-heritage.org.uk" />
				<cc:attributionName xml:lang="en">English Heritage</cc:attributionName>
				<dcterms:publisher rdf:resource="http://www.english-heritage.org.uk" />
			</skos:Concept>
		</skos:narrower>
		<skos:broader rdf:resource="http://purl.org/heritagedata/schemes/560/concepts/142160" />
		<skos:scopeNote xml:lang="en">Use for teeth, hard structures found in the jaws of vertebrates used principally for chewing and eating.</skos:scopeNote>
		<cc:license rdf:resource="http://creativecommons.org/licenses/by/3.0" />
		<cc:attributionURL rdf:resource="http://www.english-heritage.org.uk" />
		<cc:attributionName xml:lang="en">English Heritage</cc:attributionName>
		<dcterms:publisher rdf:resource="http://www.english-heritage.org.uk" />
	</skos:Concept>
	<skos:Concept rdf:about="http://purl.org/heritagedata/schemes/560/concepts/142209">
		<skos:inScheme rdf:resource="http://purl.org/heritagedata/schemes/560" />
		<dcterms:identifier>http://purl.org/heritagedata/schemes/560/concepts/142209</dcterms:identifier>
		<skos:prefLabel xml:lang="en">TREE-RING ANALYSIS</skos:prefLabel>
		<dcterms:issued rdf:datatype="http://www.w3.org/2001/XMLSchema#dateTime">2013-07-17T09:02:45</dcterms:issued>
		<skos:altLabel xml:lang="en">Tree-Ring Studies</skos:altLabel>
		<skos:broader rdf:resource="http://purl.org/heritagedata/schemes/560/concepts/142182" />
		<skos:related rdf:resource="http://purl.org/heritagedata/schemes/560/concepts/142131" />
		<skos:scopeNote xml:lang="en">The use of annual incremental growth in temperate trees to investigate environmental, especially local, parameters and the history of individual trees.</skos:scopeNote>
		<cc:license rdf:resource="http://creativecommons.org/licenses/by/3.0" />
		<cc:attributionURL rdf:resource="http://www.english-heritage.org.uk" />
		<cc:attributionName xml:lang="en">English Heritage</cc:attributionName>
		<dcterms:publisher rdf:resource="http://www.english-heritage.org.uk" />
	</skos:Concept>
	<skos:Concept rdf:about="http://purl.org/heritagedata/schemes/560/concepts/142211">
		<skos:inScheme rdf:resource="http://purl.org/heritagedata/schemes/560" />
		<dcterms:identifier>http://purl.org/heritagedata/schemes/560/concepts/142211</dcterms:identifier>
		<skos:prefLabel xml:lang="en">TWIG</skos:prefLabel>
		<dcterms:issued rdf:datatype="http://www.w3.org/2001/XMLSchema#dateTime">2013-07-17T09:02:45</dcterms:issued>
		<skos:broader rdf:resource="http://purl.org/heritagedata/schemes/560/concepts/142214" />
		<skos:broader rdf:resource="http://purl.org/heritagedata/schemes/560/concepts/142117" />
		<skos:scopeNote xml:lang="en">Small (&lt;2cm diameter) roundwood often complete with buds or leaf scars.</skos:scopeNote>
		<cc:license rdf:resource="http://creativecommons.org/licenses/by/3.0" />
		<cc:attributionURL rdf:resource="http://www.english-heritage.org.uk" />
		<cc:attributionName xml:lang="en">English Heritage</cc:attributionName>
		<dcterms:publisher rdf:resource="http://www.english-heritage.org.uk" />
	</skos:Concept>
	<skos:Concept rdf:about="http://purl.org/heritagedata/schemes/560/concepts/142214">
		<skos:inScheme rdf:resource="http://purl.org/heritagedata/schemes/560" />
		<dcterms:identifier>http://purl.org/heritagedata/schemes/560/concepts/142214</dcterms:identifier>
		<skos:prefLabel xml:lang="en">WOOD</skos:prefLabel>
		<dcterms:issued rdf:datatype="http://www.w3.org/2001/XMLSchema#dateTime">2013-07-17T09:02:45</dcterms:issued>
		<skos:narrower rdf:resource="http://purl.org/heritagedata/schemes/560/concepts/142117" />
		<skos:narrower rdf:resource="http://purl.org/heritagedata/schemes/560/concepts/142189" />
		<skos:narrower rdf:resource="http://purl.org/heritagedata/schemes/560/concepts/142211" />
		<skos:broader rdf:resource="http://purl.org/heritagedata/schemes/560/concepts/142160" />
		<skos:scopeNote xml:lang="en">Hard, compact, unprocessed, fibrous cellulose substance. The roots, trunks and branches of trees and shrubs consist of this tissue.</skos:scopeNote>
		<cc:license rdf:resource="http://creativecommons.org/licenses/by/3.0" />
		<cc:attributionURL rdf:resource="http://www.english-heritage.org.uk" />
		<cc:attributionName xml:lang="en">English Heritage</cc:attributionName>
		<dcterms:publisher rdf:resource="http://www.english-heritage.org.uk" />
	</skos:Concept>
	<skos:Concept rdf:about="http://purl.org/heritagedata/schemes/560/concepts/142215">
		<skos:inScheme rdf:resource="http://purl.org/heritagedata/schemes/560" />
		<dcterms:identifier>http://purl.org/heritagedata/schemes/560/concepts/142215</dcterms:identifier>
		<skos:prefLabel xml:lang="en">WORKED</skos:prefLabel>
		<dcterms:issued rdf:datatype="http://www.w3.org/2001/XMLSchema#dateTime">2013-07-17T09:02:45</dcterms:issued>
		<skos:narrower>
			<skos:Concept rdf:about="http://purl.org/heritagedata/schemes/560/concepts/148327">
				<skos:inScheme rdf:resource="http://purl.org/heritagedata/schemes/560" />
				<dcterms:identifier>http://purl.org/heritagedata/schemes/560/concepts/148327</dcterms:identifier>
				<skos:prefLabel xml:lang="en">CARVED</skos:prefLabel>
				<dcterms:issued rdf:datatype="http://www.w3.org/2001/XMLSchema#dateTime">2013-07-17T09:02:45</dcterms:issued>
				<skos:broader rdf:resource="http://purl.org/heritagedata/schemes/560/concepts/142215" />
				<cc:license rdf:resource="http://creativecommons.org/licenses/by/3.0" />
				<cc:attributionURL rdf:resource="http://www.english-heritage.org.uk" />
				<cc:attributionName xml:lang="en">English Heritage</cc:attributionName>
				<dcterms:publisher rdf:resource="http://www.english-heritage.org.uk" />
			</skos:Concept>
		</skos:narrower>
		<skos:narrower>
			<skos:Concept rdf:about="http://purl.org/heritagedata/schemes/560/concepts/142124">
				<skos:inScheme rdf:resource="http://purl.org/heritagedata/schemes/560" />
				<dcterms:identifier>http://purl.org/heritagedata/schemes/560/concepts/142124</dcterms:identifier>
				<skos:prefLabel xml:lang="en">COLOURED</skos:prefLabel>
				<dcterms:issued rdf:datatype="http://www.w3.org/2001/XMLSchema#dateTime">2013-07-17T09:02:45</dcterms:issued>
				<skos:altLabel xml:lang="en">Colored</skos:altLabel>
				<skos:broader rdf:resource="http://purl.org/heritagedata/schemes/560/concepts/142215" />
				<skos:scopeNote xml:lang="en">Material with evidence of the application of a pigment or dye.</skos:scopeNote>
				<cc:license rdf:resource="http://creativecommons.org/licenses/by/3.0" />
				<cc:attributionURL rdf:resource="http://www.english-heritage.org.uk" />
				<cc:attributionName xml:lang="en">English Heritage</cc:attributionName>
				<dcterms:publisher rdf:resource="http://www.english-heritage.org.uk" />
			</skos:Concept>
		</skos:narrower>
		<skos:narrower>
			<skos:Concept rdf:about="http://purl.org/heritagedata/schemes/560/concepts/142129">
				<skos:inScheme rdf:resource="http://purl.org/heritagedata/schemes/560" />
				<dcterms:identifier>http://purl.org/heritagedata/schemes/560/concepts/142129</dcterms:identifier>
				<skos:prefLabel xml:lang="en">DECORATED</skos:prefLabel>
				<dcterms:issued rdf:datatype="http://www.w3.org/2001/XMLSchema#dateTime">2013-07-17T09:02:45</dcterms:issued>
				<skos:altLabel xml:lang="en">Decoration</skos:altLabel>
				<skos:broader rdf:resource="http://purl.org/heritagedata/schemes/560/concepts/142215" />
				<skos:scopeNote xml:lang="en">Use where decoration is present.</skos:scopeNote>
				<cc:license rdf:resource="http://creativecommons.org/licenses/by/3.0" />
				<cc:attributionURL rdf:resource="http://www.english-heritage.org.uk" />
				<cc:attributionName xml:lang="en">English Heritage</cc:attributionName>
				<dcterms:publisher rdf:resource="http://www.english-heritage.org.uk" />
			</skos:Concept>
		</skos:narrower>
		<skos:narrower>
			<skos:Concept rdf:about="http://purl.org/heritagedata/schemes/560/concepts/142205">
				<skos:inScheme rdf:resource="http://purl.org/heritagedata/schemes/560" />
				<dcterms:identifier>http://purl.org/heritagedata/schemes/560/concepts/142205</dcterms:identifier>
				<skos:prefLabel xml:lang="en">TOOL MARKED</skos:prefLabel>
				<dcterms:issued rdf:datatype="http://www.w3.org/2001/XMLSchema#dateTime">2013-07-17T09:02:45</dcterms:issued>
				<skos:altLabel xml:lang="en">Tool Marks</skos:altLabel>
				<skos:broader rdf:resource="http://purl.org/heritagedata/schemes/560/concepts/142215" />
				<skos:scopeNote xml:lang="en">Use where evidence of tool marks is present</skos:scopeNote>
				<cc:license rdf:resource="http://creativecommons.org/licenses/by/3.0" />
				<cc:attributionURL rdf:resource="http://www.english-heritage.org.uk" />
				<cc:attributionName xml:lang="en">English Heritage</cc:attributionName>
				<dcterms:publisher rdf:resource="http://www.english-heritage.org.uk" />
			</skos:Concept>
		</skos:narrower>
		<skos:broader rdf:resource="http://purl.org/heritagedata/schemes/560/concepts/142148" />
		<skos:scopeNote xml:lang="en">Use for any material that shows evidence of modification by humans.</skos:scopeNote>
		<cc:license rdf:resource="http://creativecommons.org/licenses/by/3.0" />
		<cc:attributionURL rdf:resource="http://www.english-heritage.org.uk" />
		<cc:attributionName xml:lang="en">English Heritage</cc:attributionName>
		<dcterms:publisher rdf:resource="http://www.english-heritage.org.uk" />
	</skos:Concept>
	<skos:Concept rdf:about="http://purl.org/heritagedata/schemes/560/concepts/144511">
		<skos:inScheme rdf:resource="http://purl.org/heritagedata/schemes/560" />
		<dcterms:identifier>http://purl.org/heritagedata/schemes/560/concepts/144511</dcterms:identifier>
		<skos:prefLabel xml:lang="en">LUMINESCENCE DATING</skos:prefLabel>
		<dcterms:issued rdf:datatype="http://www.w3.org/2001/XMLSchema#dateTime">2013-07-17T09:02:45</dcterms:issued>
		<skos:narrower>
			<skos:Concept rdf:about="http://purl.org/heritagedata/schemes/560/concepts/142151">
				<skos:inScheme rdf:resource="http://purl.org/heritagedata/schemes/560" />
				<dcterms:identifier>http://purl.org/heritagedata/schemes/560/concepts/142151</dcterms:identifier>
				<skos:prefLabel xml:lang="en">INFRA-RED STIMULATED LUMINESCENCE</skos:prefLabel>
				<dcterms:issued rdf:datatype="http://www.w3.org/2001/XMLSchema#dateTime">2013-07-17T09:02:45</dcterms:issued>
				<skos:altLabel xml:lang="en">Irsl</skos:altLabel>
				<skos:altLabel xml:lang="en">Irsl Dating</skos:altLabel>
				<skos:broader rdf:resource="http://purl.org/heritagedata/schemes/560/concepts/144511" />
				<skos:scopeNote xml:lang="en">The light emitted from sedimentary minerals or mineral inclusions in bricks when stimulated in the laboratory by infrared light. Used to date samples up to 250,000 years old; especially appropriate for geological sediments containing feldspars</skos:scopeNote>
				<cc:license rdf:resource="http://creativecommons.org/licenses/by/3.0" />
				<cc:attributionURL rdf:resource="http://www.english-heritage.org.uk" />
				<cc:attributionName xml:lang="en">English Heritage</cc:attributionName>
				<dcterms:publisher rdf:resource="http://www.english-heritage.org.uk" />
			</skos:Concept>
		</skos:narrower>
		<skos:broader rdf:resource="http://purl.org/heritagedata/schemes/560/concepts/142128" />
		<skos:narrower>
			<skos:Concept rdf:about="http://purl.org/heritagedata/schemes/560/concepts/142177">
				<skos:inScheme rdf:resource="http://purl.org/heritagedata/schemes/560" />
				<dcterms:identifier>http://purl.org/heritagedata/schemes/560/concepts/142177</dcterms:identifier>
				<skos:prefLabel xml:lang="en">OPTICALLY STIMULATED LUMINESCENCE</skos:prefLabel>
				<dcterms:issued rdf:datatype="http://www.w3.org/2001/XMLSchema#dateTime">2013-07-17T09:02:45</dcterms:issued>
				<skos:altLabel xml:lang="en">Osl</skos:altLabel>
				<skos:altLabel xml:lang="en">Osl Dating</skos:altLabel>
				<skos:broader rdf:resource="http://purl.org/heritagedata/schemes/560/concepts/144511" />
				<skos:scopeNote xml:lang="en">The light emitted from sedimentary minerals or mineral inclusions in bricks when stimulated in the laboratory by light of a different wavelength. Used to date samples up to 250,000 years old; especially appropriate for geological sediments.</skos:scopeNote>
				<cc:license rdf:resource="http://creativecommons.org/licenses/by/3.0" />
				<cc:attributionURL rdf:resource="http://www.english-heritage.org.uk" />
				<cc:attributionName xml:lang="en">English Heritage</cc:attributionName>
				<dcterms:publisher rdf:resource="http://www.english-heritage.org.uk" />
			</skos:Concept>
		</skos:narrower>
		<skos:narrower>
			<skos:Concept rdf:about="http://purl.org/heritagedata/schemes/560/concepts/142203">
				<skos:inScheme rdf:resource="http://purl.org/heritagedata/schemes/560" />
				<dcterms:identifier>http://purl.org/heritagedata/schemes/560/concepts/142203</dcterms:identifier>
				<skos:prefLabel xml:lang="en">THERMOLUMINESCENCE</skos:prefLabel>
				<dcterms:issued rdf:datatype="http://www.w3.org/2001/XMLSchema#dateTime">2013-07-17T09:02:45</dcterms:issued>
				<skos:altLabel xml:lang="en">Tl Dating</skos:altLabel>
				<skos:altLabel xml:lang="en">Tl</skos:altLabel>
				<skos:broader rdf:resource="http://purl.org/heritagedata/schemes/560/concepts/144511" />
				<skos:scopeNote xml:lang="en">The measurement of the light emitted from sedimentary minerals, mineral inclusions in bricks, burnt flint or unburnt calcite when they are heated. The signal relates to their prior exposure to radioactivity. Used to date samples up to 500,000 years old.</skos:scopeNote>
				<cc:license rdf:resource="http://creativecommons.org/licenses/by/3.0" />
				<cc:attributionURL rdf:resource="http://www.english-heritage.org.uk" />
				<cc:attributionName xml:lang="en">English Heritage</cc:attributionName>
				<dcterms:publisher rdf:resource="http://www.english-heritage.org.uk" />
			</skos:Concept>
		</skos:narrower>
		<skos:scopeNote xml:lang="en">A range of techniques that use the build up of charge stored within a crystalline material to estimate its age</skos:scopeNote>
		<cc:license rdf:resource="http://creativecommons.org/licenses/by/3.0" />
		<cc:attributionURL rdf:resource="http://www.english-heritage.org.uk" />
		<cc:attributionName xml:lang="en">English Heritage</cc:attributionName>
		<dcterms:publisher rdf:resource="http://www.english-heritage.org.uk" />
	</skos:Concept>
	<skos:Concept rdf:about="http://purl.org/heritagedata/schemes/560/concepts/144518">
		<skos:inScheme rdf:resource="http://purl.org/heritagedata/schemes/560" />
		<dcterms:identifier>http://purl.org/heritagedata/schemes/560/concepts/144518</dcterms:identifier>
		<skos:prefLabel xml:lang="en">GEOLOGICAL SEDIMENT</skos:prefLabel>
		<dcterms:issued rdf:datatype="http://www.w3.org/2001/XMLSchema#dateTime">2013-07-17T09:02:45</dcterms:issued>
		<skos:narrower>
			<skos:Concept rdf:about="http://purl.org/heritagedata/schemes/560/concepts/144521">
				<skos:inScheme rdf:resource="http://purl.org/heritagedata/schemes/560" />
				<dcterms:identifier>http://purl.org/heritagedata/schemes/560/concepts/144521</dcterms:identifier>
				<skos:prefLabel xml:lang="en">FELDSPAR</skos:prefLabel>
				<dcterms:issued rdf:datatype="http://www.w3.org/2001/XMLSchema#dateTime">2013-07-17T09:02:45</dcterms:issued>
				<skos:broader rdf:resource="http://purl.org/heritagedata/schemes/560/concepts/144518" />
				<skos:scopeNote xml:lang="en">A group of aluminosilicate minerals with varying compositions. The most common mineral in igneous rocks, and common in other rocks and sediments.</skos:scopeNote>
				<cc:license rdf:resource="http://creativecommons.org/licenses/by/3.0" />
				<cc:attributionURL rdf:resource="http://www.english-heritage.org.uk" />
				<cc:attributionName xml:lang="en">English Heritage</cc:attributionName>
				<dcterms:publisher rdf:resource="http://www.english-heritage.org.uk" />
			</skos:Concept>
		</skos:narrower>
		<skos:broader rdf:resource="http://purl.org/heritagedata/schemes/560/concepts/142160" />
		<skos:narrower>
			<skos:Concept rdf:about="http://purl.org/heritagedata/schemes/560/concepts/144523">
				<skos:inScheme rdf:resource="http://purl.org/heritagedata/schemes/560" />
				<dcterms:identifier>http://purl.org/heritagedata/schemes/560/concepts/144523</dcterms:identifier>
				<skos:prefLabel xml:lang="en">POLYMINERAL</skos:prefLabel>
				<dcterms:issued rdf:datatype="http://www.w3.org/2001/XMLSchema#dateTime">2013-07-17T09:02:45</dcterms:issued>
				<skos:broader rdf:resource="http://purl.org/heritagedata/schemes/560/concepts/144518" />
				<skos:scopeNote xml:lang="en">A general term to describe a sediment or sample that contains a variety of different minerals.</skos:scopeNote>
				<cc:license rdf:resource="http://creativecommons.org/licenses/by/3.0" />
				<cc:attributionURL rdf:resource="http://www.english-heritage.org.uk" />
				<cc:attributionName xml:lang="en">English Heritage</cc:attributionName>
				<dcterms:publisher rdf:resource="http://www.english-heritage.org.uk" />
			</skos:Concept>
		</skos:narrower>
		<skos:narrower>
			<skos:Concept rdf:about="http://purl.org/heritagedata/schemes/560/concepts/144520">
				<skos:inScheme rdf:resource="http://purl.org/heritagedata/schemes/560" />
				<dcterms:identifier>http://purl.org/heritagedata/schemes/560/concepts/144520</dcterms:identifier>
				<skos:prefLabel xml:lang="en">QUARTZ</skos:prefLabel>
				<dcterms:issued rdf:datatype="http://www.w3.org/2001/XMLSchema#dateTime">2013-07-17T09:02:45</dcterms:issued>
				<skos:broader rdf:resource="http://purl.org/heritagedata/schemes/560/concepts/144518" />
				<skos:scopeNote xml:lang="en">A mineral composed of SiO2. Commonly clear or milky in appearance. A common constituent of rocks and sediments.</skos:scopeNote>
				<cc:license rdf:resource="http://creativecommons.org/licenses/by/3.0" />
				<cc:attributionURL rdf:resource="http://www.english-heritage.org.uk" />
				<cc:attributionName xml:lang="en">English Heritage</cc:attributionName>
				<dcterms:publisher rdf:resource="http://www.english-heritage.org.uk" />
			</skos:Concept>
		</skos:narrower>
		<skos:narrower>
			<skos:Concept rdf:about="http://purl.org/heritagedata/schemes/560/concepts/144522">
				<skos:inScheme rdf:resource="http://purl.org/heritagedata/schemes/560" />
				<dcterms:identifier>http://purl.org/heritagedata/schemes/560/concepts/144522</dcterms:identifier>
				<skos:prefLabel xml:lang="en">ZIRCON</skos:prefLabel>
				<dcterms:issued rdf:datatype="http://www.w3.org/2001/XMLSchema#dateTime">2013-07-17T09:02:45</dcterms:issued>
				<skos:broader rdf:resource="http://purl.org/heritagedata/schemes/560/concepts/144518" />
				<skos:scopeNote xml:lang="en">A mineral of the composition Zr[SiO4]. Commonly brown or yellow in colour. May contain high levels of uranium and thorium. Can be used for dating using luminescence or fission track methods.</skos:scopeNote>
				<cc:license rdf:resource="http://creativecommons.org/licenses/by/3.0" />
				<cc:attributionURL rdf:resource="http://www.english-heritage.org.uk" />
				<cc:attributionName xml:lang="en">English Heritage</cc:attributionName>
				<dcterms:publisher rdf:resource="http://www.english-heritage.org.uk" />
			</skos:Concept>
		</skos:narrower>
		<skos:scopeNote xml:lang="en">A material composed of mineral grains derived from the breakdown of rocks by environmental processes.</skos:scopeNote>
		<cc:license rdf:resource="http://creativecommons.org/licenses/by/3.0" />
		<cc:attributionURL rdf:resource="http://www.english-heritage.org.uk" />
		<cc:attributionName xml:lang="en">English Heritage</cc:attributionName>
		<dcterms:publisher rdf:resource="http://www.english-heritage.org.uk" />
	</skos:Concept>
</rdf:RDF>