<?xml version="1.0"?>
<rdf:RDF xmlns:dc="http://purl.org/dc/elements/1.1/" xmlns:owl="http://www.w3.org/2002/07/owl#" xmlns:skosxl="http://www.w3.org/2008/05/skos-xl#" xmlns:rdfs="http://www.w3.org/2000/01/rdf-schema#" xmlns:dcterms="http://purl.org/dc/terms/" xmlns:xsd="http://www.w3.org/2001/XMLSchema#" xmlns:rdf="http://www.w3.org/1999/02/22-rdf-syntax-ns#" xmlns:cc="http://creativecommons.org/ns#" xmlns:skos="http://www.w3.org/2004/02/skos/core#" xml:base="http://stellar/">
	<skos:Concept rdf:about="http://purl.org/heritagedata/schemes/3/concepts/501846">
		<skos:inScheme rdf:resource="http://purl.org/heritagedata/schemes/3" />
		<dcterms:identifier>http://purl.org/heritagedata/schemes/3/concepts/501846</dcterms:identifier>
		<cc:license rdf:resource="http://reference.data.gov.uk/id/open-government-licence" />
		<cc:attributionURL rdf:resource="http://www.rcahms.gov.uk" />
		<cc:attributionName xml:lang="en">RCAHMS</cc:attributionName>
		<dcterms:publisher rdf:resource="http://www.rcahms.gov.uk" />
		<skos:prefLabel xml:lang="en">BILLYBOY</skos:prefLabel>
		<dcterms:issued rdf:datatype="http://www.w3.org/2001/XMLSchema#dateTime">2013-07-17T10:08:39</dcterms:issued>
		<skos:broader rdf:resource="http://purl.org/heritagedata/schemes/3/concepts/501968" />
		<skos:broader rdf:resource="http://purl.org/heritagedata/schemes/3/concepts/501841" />
		<skos:scopeNote xml:lang="en">Single masted east coast trading vessel, ketch rigged or single masted.</skos:scopeNote>
	</skos:Concept>
	<skos:Concept rdf:about="http://purl.org/heritagedata/schemes/3/concepts/501848">
		<skos:inScheme rdf:resource="http://purl.org/heritagedata/schemes/3" />
		<dcterms:identifier>http://purl.org/heritagedata/schemes/3/concepts/501848</dcterms:identifier>
		<cc:license rdf:resource="http://reference.data.gov.uk/id/open-government-licence" />
		<cc:attributionURL rdf:resource="http://www.rcahms.gov.uk" />
		<cc:attributionName xml:lang="en">RCAHMS</cc:attributionName>
		<dcterms:publisher rdf:resource="http://www.rcahms.gov.uk" />
		<skos:prefLabel xml:lang="en">BOAT</skos:prefLabel>
		<dcterms:modified rdf:datatype="http://www.w3.org/2001/XMLSchema#dateTime">2007-04-24T11:54:05</dcterms:modified>
		<dcterms:issued rdf:datatype="http://www.w3.org/2001/XMLSchema#dateTime">2013-07-17T10:08:39</dcterms:issued>
		<skos:broader rdf:resource="http://purl.org/heritagedata/schemes/3/concepts/501925" />
		<skos:broader rdf:resource="http://purl.org/heritagedata/schemes/3/concepts/501968" />
		<skos:scopeNote xml:lang="en">A vague term loosely applied to a vessel of any type, form or construction considered too small to be a ship.Such vessels vary considerably in construction and form, and are used for a variety of purposes.
The term is generally applied to undecked vessels, and has connotations of unseaworthiness, unsuitability for independent operation, portability and/or unsophisticated construction.</skos:scopeNote>
	</skos:Concept>
	<skos:Concept rdf:about="http://purl.org/heritagedata/schemes/3/concepts/501850">
		<skos:inScheme rdf:resource="http://purl.org/heritagedata/schemes/3" />
		<dcterms:identifier>http://purl.org/heritagedata/schemes/3/concepts/501850</dcterms:identifier>
		<cc:license rdf:resource="http://reference.data.gov.uk/id/open-government-licence" />
		<cc:attributionURL rdf:resource="http://www.rcahms.gov.uk" />
		<cc:attributionName xml:lang="en">RCAHMS</cc:attributionName>
		<dcterms:publisher rdf:resource="http://www.rcahms.gov.uk" />
		<skos:prefLabel xml:lang="en">BRIG</skos:prefLabel>
		<dcterms:modified rdf:datatype="http://www.w3.org/2001/XMLSchema#dateTime">2007-04-24T12:15:56</dcterms:modified>
		<dcterms:issued rdf:datatype="http://www.w3.org/2001/XMLSchema#dateTime">2013-07-17T10:08:39</dcterms:issued>
		<skos:narrower>
			<skos:Concept rdf:about="http://purl.org/heritagedata/schemes/3/concepts/501831">
				<skos:inScheme rdf:resource="http://purl.org/heritagedata/schemes/3" />
				<dcterms:identifier>http://purl.org/heritagedata/schemes/3/concepts/501831</dcterms:identifier>
				<cc:license rdf:resource="http://reference.data.gov.uk/id/open-government-licence" />
				<cc:attributionURL rdf:resource="http://www.rcahms.gov.uk" />
				<cc:attributionName xml:lang="en">RCAHMS</cc:attributionName>
				<dcterms:publisher rdf:resource="http://www.rcahms.gov.uk" />
				<skos:prefLabel xml:lang="en">AUXILIARY BRIG</skos:prefLabel>
				<dcterms:issued rdf:datatype="http://www.w3.org/2001/XMLSchema#dateTime">2013-07-17T10:08:39</dcterms:issued>
				<skos:broader rdf:resource="http://purl.org/heritagedata/schemes/3/concepts/501850" />
				<skos:scopeNote xml:lang="en">Variant of the Brig having auxiliary steam or diesel propulsion for use in light airs or contrary winds.</skos:scopeNote>
			</skos:Concept>
		</skos:narrower>
		<skos:broader rdf:resource="http://purl.org/heritagedata/schemes/3/concepts/501987" />
		<skos:narrower>
			<skos:Concept rdf:about="http://purl.org/heritagedata/schemes/3/concepts/501899">
				<skos:inScheme rdf:resource="http://purl.org/heritagedata/schemes/3" />
				<dcterms:identifier>http://purl.org/heritagedata/schemes/3/concepts/501899</dcterms:identifier>
				<cc:license rdf:resource="http://reference.data.gov.uk/id/open-government-licence" />
				<cc:attributionURL rdf:resource="http://www.rcahms.gov.uk" />
				<cc:attributionName xml:lang="en">RCAHMS</cc:attributionName>
				<dcterms:publisher rdf:resource="http://www.rcahms.gov.uk" />
				<skos:prefLabel xml:lang="en">HERMAPHRODITE BRIG</skos:prefLabel>
				<dcterms:issued rdf:datatype="http://www.w3.org/2001/XMLSchema#dateTime">2013-07-17T10:08:39</dcterms:issued>
				<skos:broader rdf:resource="http://purl.org/heritagedata/schemes/3/concepts/501850" />
				<skos:scopeNote xml:lang="en">Variant of the Brig having square sails on the foremast and a square topsail above a gaff main on the main. The term brig-schooner has also been applied.</skos:scopeNote>
			</skos:Concept>
		</skos:narrower>
		<skos:scopeNote xml:lang="en">Medium-sized decked sailing vessel having two masts, with square sails on both and normally of timber construction. Vessels of this type were significant in the 18th century for the carriage of coal (collier brigs); several cadet or school ships have this rig.</skos:scopeNote>
	</skos:Concept>
	<skos:Concept rdf:about="http://purl.org/heritagedata/schemes/3/concepts/501857">
		<skos:inScheme rdf:resource="http://purl.org/heritagedata/schemes/3" />
		<dcterms:identifier>http://purl.org/heritagedata/schemes/3/concepts/501857</dcterms:identifier>
		<cc:license rdf:resource="http://reference.data.gov.uk/id/open-government-licence" />
		<cc:attributionURL rdf:resource="http://www.rcahms.gov.uk" />
		<cc:attributionName xml:lang="en">RCAHMS</cc:attributionName>
		<dcterms:publisher rdf:resource="http://www.rcahms.gov.uk" />
		<skos:prefLabel xml:lang="en">CARGO VESSEL</skos:prefLabel>
		<dcterms:issued rdf:datatype="http://www.w3.org/2001/XMLSchema#dateTime">2013-07-17T10:08:39</dcterms:issued>
		<skos:narrower rdf:resource="http://purl.org/heritagedata/schemes/3/concepts/501841" />
		<skos:broader rdf:resource="http://purl.org/heritagedata/schemes/3/concepts/502011" />
		<skos:narrower>
			<skos:Concept rdf:about="http://purl.org/heritagedata/schemes/3/concepts/501860">
				<skos:inScheme rdf:resource="http://purl.org/heritagedata/schemes/3" />
				<dcterms:identifier>http://purl.org/heritagedata/schemes/3/concepts/501860</dcterms:identifier>
				<cc:license rdf:resource="http://reference.data.gov.uk/id/open-government-licence" />
				<cc:attributionURL rdf:resource="http://www.rcahms.gov.uk" />
				<cc:attributionName xml:lang="en">RCAHMS</cc:attributionName>
				<dcterms:publisher rdf:resource="http://www.rcahms.gov.uk" />
				<skos:prefLabel xml:lang="en">COLLIER</skos:prefLabel>
				<dcterms:issued rdf:datatype="http://www.w3.org/2001/XMLSchema#dateTime">2013-07-17T10:08:39</dcterms:issued>
				<skos:broader rdf:resource="http://purl.org/heritagedata/schemes/3/concepts/501857" />
				<skos:scopeNote xml:lang="en">A vessel for carrying a cargo of coal in bulk.</skos:scopeNote>
			</skos:Concept>
		</skos:narrower>
		<skos:narrower>
			<skos:Concept rdf:about="http://purl.org/heritagedata/schemes/3/concepts/501917">
				<skos:inScheme rdf:resource="http://purl.org/heritagedata/schemes/3" />
				<dcterms:identifier>http://purl.org/heritagedata/schemes/3/concepts/501917</dcterms:identifier>
				<cc:license rdf:resource="http://reference.data.gov.uk/id/open-government-licence" />
				<cc:attributionURL rdf:resource="http://www.rcahms.gov.uk" />
				<cc:attributionName xml:lang="en">RCAHMS</cc:attributionName>
				<dcterms:publisher rdf:resource="http://www.rcahms.gov.uk" />
				<skos:prefLabel xml:lang="en">LIBERTY SHIP</skos:prefLabel>
				<dcterms:issued rdf:datatype="http://www.w3.org/2001/XMLSchema#dateTime">2013-07-17T10:08:39</dcterms:issued>
				<skos:broader rdf:resource="http://purl.org/heritagedata/schemes/3/concepts/501857" />
				<skos:scopeNote xml:lang="en">A specialised form of Steamship built during the Second World War for to carry large volumes of war materials. They were optimised for rapid construction by unskilled labour and with the minimum use of scarce industrial capacity; riveted construction and reciprocating engines being used. Comparable ships were built during the First World War, but not given the name.</skos:scopeNote>
			</skos:Concept>
		</skos:narrower>
		<skos:narrower rdf:resource="http://purl.org/heritagedata/schemes/3/concepts/501948" />
		<skos:narrower rdf:resource="http://purl.org/heritagedata/schemes/3/concepts/502007" />
		<skos:narrower>
			<skos:Concept rdf:about="http://purl.org/heritagedata/schemes/3/concepts/503980">
				<skos:inScheme rdf:resource="http://purl.org/heritagedata/schemes/3" />
				<dcterms:identifier>http://purl.org/heritagedata/schemes/3/concepts/503980</dcterms:identifier>
				<cc:license rdf:resource="http://reference.data.gov.uk/id/open-government-licence" />
				<cc:attributionURL rdf:resource="http://www.rcahms.gov.uk" />
				<cc:attributionName xml:lang="en">RCAHMS</cc:attributionName>
				<dcterms:publisher rdf:resource="http://www.rcahms.gov.uk" />
				<skos:prefLabel xml:lang="en">CONTAINER SHIP</skos:prefLabel>
				<dcterms:created rdf:datatype="http://www.w3.org/2001/XMLSchema#dateTime">2009-02-26T14:38:37</dcterms:created>
				<dcterms:modified rdf:datatype="http://www.w3.org/2001/XMLSchema#dateTime">2009-02-26T14:40:21</dcterms:modified>
				<dcterms:issued rdf:datatype="http://www.w3.org/2001/XMLSchema#dateTime">2013-07-17T10:08:39</dcterms:issued>
				<skos:broader rdf:resource="http://purl.org/heritagedata/schemes/3/concepts/501857" />
				<skos:scopeNote xml:lang="en">A merchant cargo vessel specifically designed and used for the carriage of containers, and typically non-self discharging.</skos:scopeNote>
			</skos:Concept>
		</skos:narrower>
		<skos:scopeNote xml:lang="en">A craft used for the transportation of cargoes. Use specific type where known.</skos:scopeNote>
	</skos:Concept>
	<skos:Concept rdf:about="http://purl.org/heritagedata/schemes/3/concepts/501943">
		<skos:inScheme rdf:resource="http://purl.org/heritagedata/schemes/3" />
		<dcterms:identifier>http://purl.org/heritagedata/schemes/3/concepts/501943</dcterms:identifier>
		<cc:license rdf:resource="http://reference.data.gov.uk/id/open-government-licence" />
		<cc:attributionURL rdf:resource="http://www.rcahms.gov.uk" />
		<cc:attributionName xml:lang="en">RCAHMS</cc:attributionName>
		<dcterms:publisher rdf:resource="http://www.rcahms.gov.uk" />
		<skos:prefLabel xml:lang="en">NAVAL SUPPORT VESSEL</skos:prefLabel>
		<dcterms:modified rdf:datatype="http://www.w3.org/2001/XMLSchema#dateTime">2011-08-19T09:36:54</dcterms:modified>
		<dcterms:issued rdf:datatype="http://www.w3.org/2001/XMLSchema#dateTime">2013-07-17T10:08:39</dcterms:issued>
		<skos:narrower>
			<skos:Concept rdf:about="http://purl.org/heritagedata/schemes/3/concepts/501829">
				<skos:inScheme rdf:resource="http://purl.org/heritagedata/schemes/3" />
				<dcterms:identifier>http://purl.org/heritagedata/schemes/3/concepts/501829</dcterms:identifier>
				<cc:license rdf:resource="http://reference.data.gov.uk/id/open-government-licence" />
				<cc:attributionURL rdf:resource="http://www.rcahms.gov.uk" />
				<cc:attributionName xml:lang="en">RCAHMS</cc:attributionName>
				<dcterms:publisher rdf:resource="http://www.rcahms.gov.uk" />
				<skos:prefLabel xml:lang="en">ARMED MERCHANT CRUISER</skos:prefLabel>
				<dcterms:issued rdf:datatype="http://www.w3.org/2001/XMLSchema#dateTime">2013-07-17T10:08:39</dcterms:issued>
				<skos:broader rdf:resource="http://purl.org/heritagedata/schemes/3/concepts/501943" />
				<skos:scopeNote xml:lang="en">A requisitioned merchant vessel (generally of considerable speed and size) given an extempore armament fit to allow her limited use in convoy protection or to enforce a naval blockade, pending the construction of adequate specialised warships.</skos:scopeNote>
			</skos:Concept>
		</skos:narrower>
		<skos:narrower>
			<skos:Concept rdf:about="http://purl.org/heritagedata/schemes/3/concepts/501849">
				<skos:inScheme rdf:resource="http://purl.org/heritagedata/schemes/3" />
				<dcterms:identifier>http://purl.org/heritagedata/schemes/3/concepts/501849</dcterms:identifier>
				<cc:license rdf:resource="http://reference.data.gov.uk/id/open-government-licence" />
				<cc:attributionURL rdf:resource="http://www.rcahms.gov.uk" />
				<cc:attributionName xml:lang="en">RCAHMS</cc:attributionName>
				<dcterms:publisher rdf:resource="http://www.rcahms.gov.uk" />
				<skos:prefLabel xml:lang="en">BOOM DEFENCE VESSEL</skos:prefLabel>
				<dcterms:issued rdf:datatype="http://www.w3.org/2001/XMLSchema#dateTime">2013-07-17T10:08:39</dcterms:issued>
				<skos:broader rdf:resource="http://purl.org/heritagedata/schemes/3/concepts/501943" />
				<skos:scopeNote xml:lang="en">A specialised form of yard or service craft typically operated as a naval auxiliary for the laying of maintenance of moorings and boom defences, and for light general salvage. The type is characterised by the fitting of prominent projecting lifting-horns at the bow.</skos:scopeNote>
			</skos:Concept>
		</skos:narrower>
		<skos:narrower>
			<skos:Concept rdf:about="http://purl.org/heritagedata/schemes/3/concepts/501869">
				<skos:inScheme rdf:resource="http://purl.org/heritagedata/schemes/3" />
				<dcterms:identifier>http://purl.org/heritagedata/schemes/3/concepts/501869</dcterms:identifier>
				<cc:license rdf:resource="http://reference.data.gov.uk/id/open-government-licence" />
				<cc:attributionURL rdf:resource="http://www.rcahms.gov.uk" />
				<cc:attributionName xml:lang="en">RCAHMS</cc:attributionName>
				<dcterms:publisher rdf:resource="http://www.rcahms.gov.uk" />
				<skos:prefLabel xml:lang="en">DEGAUSSING BARGE</skos:prefLabel>
				<dcterms:modified rdf:datatype="http://www.w3.org/2001/XMLSchema#dateTime">2007-04-24T12:09:21</dcterms:modified>
				<dcterms:issued rdf:datatype="http://www.w3.org/2001/XMLSchema#dateTime">2013-07-17T10:08:39</dcterms:issued>
				<skos:altLabel xml:lang="en">DEGUASSING VESSEL</skos:altLabel>
				<skos:broader rdf:resource="http://purl.org/heritagedata/schemes/3/concepts/501943" />
				<skos:scopeNote xml:lang="en">A non self-propelled vessel used within a dockyard to facilitate 'wiping', the passage of a heavy electrical current across a ferrous hull to negate the magnetism induced into the hull during building, and so provide short-term protection against magnetic mines. Such a vessel is essentially a floating electrical battery, and may also to be used to provide an external (shore) power supply to vessels in refit.</skos:scopeNote>
			</skos:Concept>
		</skos:narrower>
		<skos:narrower rdf:resource="http://purl.org/heritagedata/schemes/3/concepts/501905" />
		<skos:narrower>
			<skos:Concept rdf:about="http://purl.org/heritagedata/schemes/3/concepts/501942">
				<skos:inScheme rdf:resource="http://purl.org/heritagedata/schemes/3" />
				<dcterms:identifier>http://purl.org/heritagedata/schemes/3/concepts/501942</dcterms:identifier>
				<cc:license rdf:resource="http://reference.data.gov.uk/id/open-government-licence" />
				<cc:attributionURL rdf:resource="http://www.rcahms.gov.uk" />
				<cc:attributionName xml:lang="en">RCAHMS</cc:attributionName>
				<dcterms:publisher rdf:resource="http://www.rcahms.gov.uk" />
				<skos:prefLabel xml:lang="en">NAVAL AUXILLIARY</skos:prefLabel>
				<dcterms:modified rdf:datatype="http://www.w3.org/2001/XMLSchema#dateTime">2007-04-24T12:10:07</dcterms:modified>
				<dcterms:issued rdf:datatype="http://www.w3.org/2001/XMLSchema#dateTime">2013-07-17T10:08:39</dcterms:issued>
				<skos:broader rdf:resource="http://purl.org/heritagedata/schemes/3/concepts/501943" />
				<skos:scopeNote xml:lang="en">A vessel (generally of considerable size and sophistication) specifically constructed for the afloat support of combatant warships. Such vessels typically incorporate features of warship construction (including damage control and action information systems, and facilities for helicopter operations), and may be armed. They should be distinguished from Requisitioned craft which may be used for similar purposes.
Such vessels have become more numerous since the Second World War and may be divided between Replenishment Vessels and Depot Ships. The former are the more numerous, are intended for the rapid supply of fuel and dry stores at sea, and carry prominent fuelling rigs for the purpose. The latter are intended to make a fleet self-sufficient by providing comprehensive repair and maintenance facilities away from major naval bases.</skos:scopeNote>
			</skos:Concept>
		</skos:narrower>
		<skos:broader rdf:resource="http://purl.org/heritagedata/schemes/3/concepts/501925" />
		<skos:narrower>
			<skos:Concept rdf:about="http://purl.org/heritagedata/schemes/3/concepts/502008">
				<skos:inScheme rdf:resource="http://purl.org/heritagedata/schemes/3" />
				<dcterms:identifier>http://purl.org/heritagedata/schemes/3/concepts/502008</dcterms:identifier>
				<cc:license rdf:resource="http://reference.data.gov.uk/id/open-government-licence" />
				<cc:attributionURL rdf:resource="http://www.rcahms.gov.uk" />
				<cc:attributionName xml:lang="en">RCAHMS</cc:attributionName>
				<dcterms:publisher rdf:resource="http://www.rcahms.gov.uk" />
				<skos:prefLabel xml:lang="en">TARGET CRAFT</skos:prefLabel>
				<dcterms:modified rdf:datatype="http://www.w3.org/2001/XMLSchema#dateTime">2011-04-12T15:40:55</dcterms:modified>
				<dcterms:issued rdf:datatype="http://www.w3.org/2001/XMLSchema#dateTime">2013-07-17T10:08:39</dcterms:issued>
				<skos:broader rdf:resource="http://purl.org/heritagedata/schemes/3/concepts/501943" />
				<skos:scopeNote xml:lang="en">A simple, unpowered, and commonly improvised vessel used for surface gunnery practice by warships. Most such vessels were small and towed, being essentially simple barges and expendable. A few were larger, armoured, self-propelled and radio-controlled.</skos:scopeNote>
			</skos:Concept>
		</skos:narrower>
		<skos:scopeNote xml:lang="en">A vessel used to carry essential supplies, such as food and armaments, to naval ships in order to keep them replenished whilst on patrol. Use more specific term.</skos:scopeNote>
	</skos:Concept>
	<skos:Concept rdf:about="http://purl.org/heritagedata/schemes/3/concepts/501948">
		<skos:inScheme rdf:resource="http://purl.org/heritagedata/schemes/3" />
		<dcterms:identifier>http://purl.org/heritagedata/schemes/3/concepts/501948</dcterms:identifier>
		<cc:license rdf:resource="http://reference.data.gov.uk/id/open-government-licence" />
		<cc:attributionURL rdf:resource="http://www.rcahms.gov.uk" />
		<cc:attributionName xml:lang="en">RCAHMS</cc:attributionName>
		<dcterms:publisher rdf:resource="http://www.rcahms.gov.uk" />
		<skos:prefLabel xml:lang="en">PASSENGER VESSEL</skos:prefLabel>
		<dcterms:issued rdf:datatype="http://www.w3.org/2001/XMLSchema#dateTime">2013-07-17T10:08:39</dcterms:issued>
		<skos:narrower>
			<skos:Concept rdf:about="http://purl.org/heritagedata/schemes/3/concepts/501884">
				<skos:inScheme rdf:resource="http://purl.org/heritagedata/schemes/3" />
				<dcterms:identifier>http://purl.org/heritagedata/schemes/3/concepts/501884</dcterms:identifier>
				<cc:license rdf:resource="http://reference.data.gov.uk/id/open-government-licence" />
				<cc:attributionURL rdf:resource="http://www.rcahms.gov.uk" />
				<cc:attributionName xml:lang="en">RCAHMS</cc:attributionName>
				<dcterms:publisher rdf:resource="http://www.rcahms.gov.uk" />
				<skos:prefLabel xml:lang="en">FERRY</skos:prefLabel>
				<dcterms:issued rdf:datatype="http://www.w3.org/2001/XMLSchema#dateTime">2013-07-17T10:08:39</dcterms:issued>
				<skos:broader rdf:resource="http://purl.org/heritagedata/schemes/3/concepts/501948" />
				<skos:scopeNote xml:lang="en">This term denotes a regular service carrying passengers and/or freight across a specific body of water. No specific type need be implied, those used may vary between simple rowing boats and sophisticated Roll-on/Roll-off (Ro-Ro) vessels. Such specialised types as hydrofoils and planing craft, chain ferries and double-decked ferries may be used in specific circumstances.</skos:scopeNote>
			</skos:Concept>
		</skos:narrower>
		<skos:narrower rdf:resource="http://purl.org/heritagedata/schemes/3/concepts/501905" />
		<skos:narrower>
			<skos:Concept rdf:about="http://purl.org/heritagedata/schemes/3/concepts/501922">
				<skos:inScheme rdf:resource="http://purl.org/heritagedata/schemes/3" />
				<dcterms:identifier>http://purl.org/heritagedata/schemes/3/concepts/501922</dcterms:identifier>
				<cc:license rdf:resource="http://reference.data.gov.uk/id/open-government-licence" />
				<cc:attributionURL rdf:resource="http://www.rcahms.gov.uk" />
				<cc:attributionName xml:lang="en">RCAHMS</cc:attributionName>
				<dcterms:publisher rdf:resource="http://www.rcahms.gov.uk" />
				<skos:prefLabel xml:lang="en">LINER</skos:prefLabel>
				<dcterms:issued rdf:datatype="http://www.w3.org/2001/XMLSchema#dateTime">2013-07-17T10:08:39</dcterms:issued>
				<skos:broader rdf:resource="http://purl.org/heritagedata/schemes/3/concepts/501948" />
				<skos:scopeNote xml:lang="en">A ship belonging to a shipping company which carries passengers on a scheduled route usually applied to steam ships only.</skos:scopeNote>
			</skos:Concept>
		</skos:narrower>
		<skos:broader rdf:resource="http://purl.org/heritagedata/schemes/3/concepts/501857" />
		<skos:scopeNote xml:lang="en">A vessel designed principally for the carriage of fare paying passengers.</skos:scopeNote>
	</skos:Concept>
	<skos:Concept rdf:about="http://purl.org/heritagedata/schemes/3/concepts/501950">
		<skos:inScheme rdf:resource="http://purl.org/heritagedata/schemes/3" />
		<dcterms:identifier>http://purl.org/heritagedata/schemes/3/concepts/501950</dcterms:identifier>
		<cc:license rdf:resource="http://reference.data.gov.uk/id/open-government-licence" />
		<cc:attributionURL rdf:resource="http://www.rcahms.gov.uk" />
		<cc:attributionName xml:lang="en">RCAHMS</cc:attributionName>
		<dcterms:publisher rdf:resource="http://www.rcahms.gov.uk" />
		<skos:prefLabel xml:lang="en">PATROL VESSEL</skos:prefLabel>
		<dcterms:issued rdf:datatype="http://www.w3.org/2001/XMLSchema#dateTime">2013-07-17T10:08:39</dcterms:issued>
		<skos:narrower>
			<skos:Concept rdf:about="http://purl.org/heritagedata/schemes/3/concepts/501949">
				<skos:inScheme rdf:resource="http://purl.org/heritagedata/schemes/3" />
				<dcterms:identifier>http://purl.org/heritagedata/schemes/3/concepts/501949</dcterms:identifier>
				<cc:license rdf:resource="http://reference.data.gov.uk/id/open-government-licence" />
				<cc:attributionURL rdf:resource="http://www.rcahms.gov.uk" />
				<cc:attributionName xml:lang="en">RCAHMS</cc:attributionName>
				<dcterms:publisher rdf:resource="http://www.rcahms.gov.uk" />
				<skos:prefLabel xml:lang="en">PATROL BOAT</skos:prefLabel>
				<dcterms:issued rdf:datatype="http://www.w3.org/2001/XMLSchema#dateTime">2013-07-17T10:08:39</dcterms:issued>
				<skos:broader rdf:resource="http://purl.org/heritagedata/schemes/3/concepts/501950" />
				<skos:scopeNote xml:lang="en">A small warship engaged in patrolling coastal waters.</skos:scopeNote>
			</skos:Concept>
		</skos:narrower>
		<skos:broader rdf:resource="http://purl.org/heritagedata/schemes/3/concepts/501925" />
		<skos:scopeNote xml:lang="en">A vessel, purpose-built or requisitioned, used for patrolling inland or coastal waters, e.g. Coastguard and Customs vessels.</skos:scopeNote>
	</skos:Concept>
	<skos:Concept rdf:about="http://purl.org/heritagedata/schemes/3/concepts/501952">
		<skos:inScheme rdf:resource="http://purl.org/heritagedata/schemes/3" />
		<dcterms:identifier>http://purl.org/heritagedata/schemes/3/concepts/501952</dcterms:identifier>
		<cc:license rdf:resource="http://reference.data.gov.uk/id/open-government-licence" />
		<cc:attributionURL rdf:resource="http://www.rcahms.gov.uk" />
		<cc:attributionName xml:lang="en">RCAHMS</cc:attributionName>
		<dcterms:publisher rdf:resource="http://www.rcahms.gov.uk" />
		<skos:prefLabel xml:lang="en">PINNACE</skos:prefLabel>
		<dcterms:issued rdf:datatype="http://www.w3.org/2001/XMLSchema#dateTime">2013-07-17T10:08:39</dcterms:issued>
		<skos:broader rdf:resource="http://purl.org/heritagedata/schemes/3/concepts/501987" />
		<skos:narrower>
			<skos:Concept rdf:about="http://purl.org/heritagedata/schemes/3/concepts/501995">
				<skos:inScheme rdf:resource="http://purl.org/heritagedata/schemes/3" />
				<dcterms:identifier>http://purl.org/heritagedata/schemes/3/concepts/501995</dcterms:identifier>
				<cc:license rdf:resource="http://reference.data.gov.uk/id/open-government-licence" />
				<cc:attributionURL rdf:resource="http://www.rcahms.gov.uk" />
				<cc:attributionName xml:lang="en">RCAHMS</cc:attributionName>
				<dcterms:publisher rdf:resource="http://www.rcahms.gov.uk" />
				<skos:prefLabel xml:lang="en">STEAM PINNACE</skos:prefLabel>
				<dcterms:issued rdf:datatype="http://www.w3.org/2001/XMLSchema#dateTime">2013-07-17T10:08:39</dcterms:issued>
				<skos:broader rdf:resource="http://purl.org/heritagedata/schemes/3/concepts/501952" />
				<skos:scopeNote xml:lang="en">A steam-powered Pinnace. Vessels of this type were frequently used as fleet tenders and ferries within naval anchorages.</skos:scopeNote>
			</skos:Concept>
		</skos:narrower>
		<skos:scopeNote xml:lang="en">The meaning of this term has varied considerably over time, being applied to both small seagoing vessels and to some larger forms of ship¿s boat. The precise meaning of the term in Scottish contexts remains unclear, but it may be presumed to apply to a large (and probably decked) transport craft of unknown rig, intended for use in sheltered waters.</skos:scopeNote>
	</skos:Concept>
	<skos:Concept rdf:about="http://purl.org/heritagedata/schemes/3/concepts/503372">
		<skos:inScheme rdf:resource="http://purl.org/heritagedata/schemes/3" />
		<dcterms:identifier>http://purl.org/heritagedata/schemes/3/concepts/503372</dcterms:identifier>
		<cc:license rdf:resource="http://reference.data.gov.uk/id/open-government-licence" />
		<cc:attributionURL rdf:resource="http://www.rcahms.gov.uk" />
		<cc:attributionName xml:lang="en">RCAHMS</cc:attributionName>
		<dcterms:publisher rdf:resource="http://www.rcahms.gov.uk" />
		<skos:prefLabel xml:lang="en">HUMAN TORPEDO</skos:prefLabel>
		<dcterms:created rdf:datatype="http://www.w3.org/2001/XMLSchema#dateTime">2008-04-16T14:07:38</dcterms:created>
		<dcterms:modified rdf:datatype="http://www.w3.org/2001/XMLSchema#dateTime">2008-04-16T16:24:11</dcterms:modified>
		<dcterms:issued rdf:datatype="http://www.w3.org/2001/XMLSchema#dateTime">2013-07-17T10:08:39</dcterms:issued>
		<skos:broader rdf:resource="http://purl.org/heritagedata/schemes/3/concepts/502015" />
		<skos:related rdf:resource="http://purl.org/heritagedata/schemes/3/concepts/501926" />
		<skos:scopeNote xml:lang="en">A specialised weapon system comprising a heavyweight torpedo and used in the Second World War to attack enemy vessels in harbour. It comprised a heavyweight torpedo controlled by two divers seated astride it; the bow was formed by a detachable explosive charge. This class of vessel is distinguished from the MIDGET SUBMARINE by not having an integral pressure hull.</skos:scopeNote>
	</skos:Concept>
	<skos:Concept rdf:about="http://purl.org/heritagedata/schemes/3/concepts/505281">
		<skos:inScheme rdf:resource="http://purl.org/heritagedata/schemes/3" />
		<dcterms:identifier>http://purl.org/heritagedata/schemes/3/concepts/505281</dcterms:identifier>
		<cc:license rdf:resource="http://reference.data.gov.uk/id/open-government-licence" />
		<cc:attributionURL rdf:resource="http://www.rcahms.gov.uk" />
		<cc:attributionName xml:lang="en">RCAHMS</cc:attributionName>
		<dcterms:publisher rdf:resource="http://www.rcahms.gov.uk" />
		<skos:prefLabel xml:lang="en">WHALE FACTORY SHIP</skos:prefLabel>
		<dcterms:created rdf:datatype="http://www.w3.org/2001/XMLSchema#dateTime">2010-08-09T10:24:34</dcterms:created>
		<dcterms:modified rdf:datatype="http://www.w3.org/2001/XMLSchema#dateTime">2010-08-09T10:29:35</dcterms:modified>
		<dcterms:issued rdf:datatype="http://www.w3.org/2001/XMLSchema#dateTime">2013-07-17T10:08:39</dcterms:issued>
		<skos:altLabel xml:lang="en">WHALE PROCESSING SHIP</skos:altLabel>
		<skos:broader rdf:resource="http://purl.org/heritagedata/schemes/3/concepts/501882" />
		<skos:related rdf:resource="http://purl.org/heritagedata/schemes/3/concepts/502016" />
		<skos:scopeNote xml:lang="en">A specialised large merchant ship built or converted for service in the Southern Ocean, cutting up (‘flensing’) whales caught by smaller catchers or whalers, boiling down the blubber, and storing the bone, flesh and oil products for the return voyage.</skos:scopeNote>
	</skos:Concept>
	<skos:Concept rdf:about="http://purl.org/heritagedata/schemes/3/concepts/501889">
		<skos:inScheme rdf:resource="http://purl.org/heritagedata/schemes/3" />
		<dcterms:identifier>http://purl.org/heritagedata/schemes/3/concepts/501889</dcterms:identifier>
		<cc:license rdf:resource="http://reference.data.gov.uk/id/open-government-licence" />
		<cc:attributionURL rdf:resource="http://www.rcahms.gov.uk" />
		<cc:attributionName xml:lang="en">RCAHMS</cc:attributionName>
		<dcterms:publisher rdf:resource="http://www.rcahms.gov.uk" />
		<skos:prefLabel xml:lang="en">FISHING VESSEL</skos:prefLabel>
		<dcterms:issued rdf:datatype="http://www.w3.org/2001/XMLSchema#dateTime">2013-07-17T10:08:39</dcterms:issued>
		<skos:narrower>
			<skos:Concept rdf:about="http://purl.org/heritagedata/schemes/3/concepts/501833">
				<skos:inScheme rdf:resource="http://purl.org/heritagedata/schemes/3" />
				<dcterms:identifier>http://purl.org/heritagedata/schemes/3/concepts/501833</dcterms:identifier>
				<cc:license rdf:resource="http://reference.data.gov.uk/id/open-government-licence" />
				<cc:attributionURL rdf:resource="http://www.rcahms.gov.uk" />
				<cc:attributionName xml:lang="en">RCAHMS</cc:attributionName>
				<dcterms:publisher rdf:resource="http://www.rcahms.gov.uk" />
				<skos:prefLabel xml:lang="en">AUXILIARY FISHING VESSEL</skos:prefLabel>
				<dcterms:modified rdf:datatype="http://www.w3.org/2001/XMLSchema#dateTime">2007-04-24T11:48:22</dcterms:modified>
				<dcterms:issued rdf:datatype="http://www.w3.org/2001/XMLSchema#dateTime">2013-07-17T10:08:39</dcterms:issued>
				<skos:broader rdf:resource="http://purl.org/heritagedata/schemes/3/concepts/501889" />
				<skos:scopeNote xml:lang="en">A fishing vessel having auxiliary steam or diesel propulsion for use in harbour areas, light airs or contrary winds.</skos:scopeNote>
			</skos:Concept>
		</skos:narrower>
		<skos:narrower>
			<skos:Concept rdf:about="http://purl.org/heritagedata/schemes/3/concepts/501854">
				<skos:inScheme rdf:resource="http://purl.org/heritagedata/schemes/3" />
				<dcterms:identifier>http://purl.org/heritagedata/schemes/3/concepts/501854</dcterms:identifier>
				<cc:license rdf:resource="http://reference.data.gov.uk/id/open-government-licence" />
				<cc:attributionURL rdf:resource="http://www.rcahms.gov.uk" />
				<cc:attributionName xml:lang="en">RCAHMS</cc:attributionName>
				<dcterms:publisher rdf:resource="http://www.rcahms.gov.uk" />
				<skos:prefLabel xml:lang="en">BUSS</skos:prefLabel>
				<dcterms:issued rdf:datatype="http://www.w3.org/2001/XMLSchema#dateTime">2013-07-17T10:08:39</dcterms:issued>
				<skos:broader rdf:resource="http://purl.org/heritagedata/schemes/3/concepts/501889" />
				<skos:scopeNote xml:lang="en">A fishing vessel of Dutch origin, commonly used (notably in the North Sea and around Northern Scotland) in the 17th and 18th centuries. Characteristically broad in the beam, and having two or three masts, each carrying a separate square sail.</skos:scopeNote>
			</skos:Concept>
		</skos:narrower>
		<skos:narrower rdf:resource="http://purl.org/heritagedata/schemes/3/concepts/501873" />
		<skos:broader rdf:resource="http://purl.org/heritagedata/schemes/3/concepts/501925" />
		<skos:narrower>
			<skos:Concept rdf:about="http://purl.org/heritagedata/schemes/3/concepts/501902">
				<skos:inScheme rdf:resource="http://purl.org/heritagedata/schemes/3" />
				<dcterms:identifier>http://purl.org/heritagedata/schemes/3/concepts/501902</dcterms:identifier>
				<cc:license rdf:resource="http://reference.data.gov.uk/id/open-government-licence" />
				<cc:attributionURL rdf:resource="http://www.rcahms.gov.uk" />
				<cc:attributionName xml:lang="en">RCAHMS</cc:attributionName>
				<dcterms:publisher rdf:resource="http://www.rcahms.gov.uk" />
				<skos:prefLabel xml:lang="en">HOOKER</skos:prefLabel>
				<dcterms:issued rdf:datatype="http://www.w3.org/2001/XMLSchema#dateTime">2013-07-17T10:08:39</dcterms:issued>
				<skos:broader rdf:resource="http://purl.org/heritagedata/schemes/3/concepts/501889" />
				<skos:scopeNote xml:lang="en">A ketch-rigged vessel of Dutch origin, characterised by a tubby form and commonly used for line fishing.</skos:scopeNote>
			</skos:Concept>
		</skos:narrower>
		<skos:narrower>
			<skos:Concept rdf:about="http://purl.org/heritagedata/schemes/3/concepts/501932">
				<skos:inScheme rdf:resource="http://purl.org/heritagedata/schemes/3" />
				<dcterms:identifier>http://purl.org/heritagedata/schemes/3/concepts/501932</dcterms:identifier>
				<cc:license rdf:resource="http://reference.data.gov.uk/id/open-government-licence" />
				<cc:attributionURL rdf:resource="http://www.rcahms.gov.uk" />
				<cc:attributionName xml:lang="en">RCAHMS</cc:attributionName>
				<dcterms:publisher rdf:resource="http://www.rcahms.gov.uk" />
				<skos:prefLabel xml:lang="en">MOTOR FISHING VESSEL</skos:prefLabel>
				<dcterms:modified rdf:datatype="http://www.w3.org/2001/XMLSchema#dateTime">2007-04-24T12:06:23</dcterms:modified>
				<dcterms:issued rdf:datatype="http://www.w3.org/2001/XMLSchema#dateTime">2013-07-17T10:08:39</dcterms:issued>
				<skos:broader rdf:resource="http://purl.org/heritagedata/schemes/3/concepts/501889" />
				<skos:scopeNote xml:lang="en">This term is loosely applied to any Fishing Vessel with integral motor propulsion, whether intended for use as a Drifter, as a Trawler or in line-fishing. Such vessels vary considerably in size, form and construction.
The term is also applied more specifically to a type of vessel (known colloquially as an 'MFV') built for naval service as light support craft, fleet tenders, diving vessels and patrol duties, but suitable for sale and civilian use when no longer required.</skos:scopeNote>
			</skos:Concept>
		</skos:narrower>
		<skos:narrower>
			<skos:Concept rdf:about="http://purl.org/heritagedata/schemes/3/concepts/501933">
				<skos:inScheme rdf:resource="http://purl.org/heritagedata/schemes/3" />
				<dcterms:identifier>http://purl.org/heritagedata/schemes/3/concepts/501933</dcterms:identifier>
				<cc:license rdf:resource="http://reference.data.gov.uk/id/open-government-licence" />
				<cc:attributionURL rdf:resource="http://www.rcahms.gov.uk" />
				<cc:attributionName xml:lang="en">RCAHMS</cc:attributionName>
				<dcterms:publisher rdf:resource="http://www.rcahms.gov.uk" />
				<skos:prefLabel xml:lang="en">MOTOR FREEZER TRAWLER</skos:prefLabel>
				<dcterms:modified rdf:datatype="http://www.w3.org/2001/XMLSchema#dateTime">2007-04-24T12:06:55</dcterms:modified>
				<dcterms:issued rdf:datatype="http://www.w3.org/2001/XMLSchema#dateTime">2013-07-17T10:08:39</dcterms:issued>
				<skos:broader rdf:resource="http://purl.org/heritagedata/schemes/3/concepts/501889" />
				<skos:scopeNote xml:lang="en">A form of Motor Fishing Vessel with integral motor propulsion and onboard refrigeration, typically of considerable size and fitted for stern trawling. Such vessels were the norm among the Soviet 'Klondykers' in the 1970s and 1980s.</skos:scopeNote>
			</skos:Concept>
		</skos:narrower>
		<skos:narrower>
			<skos:Concept rdf:about="http://purl.org/heritagedata/schemes/3/concepts/501958">
				<skos:inScheme rdf:resource="http://purl.org/heritagedata/schemes/3" />
				<dcterms:identifier>http://purl.org/heritagedata/schemes/3/concepts/501958</dcterms:identifier>
				<cc:license rdf:resource="http://reference.data.gov.uk/id/open-government-licence" />
				<cc:attributionURL rdf:resource="http://www.rcahms.gov.uk" />
				<cc:attributionName xml:lang="en">RCAHMS</cc:attributionName>
				<dcterms:publisher rdf:resource="http://www.rcahms.gov.uk" />
				<skos:prefLabel xml:lang="en">REQUISITIONED FISHING VESSEL</skos:prefLabel>
				<dcterms:issued rdf:datatype="http://www.w3.org/2001/XMLSchema#dateTime">2013-07-17T10:08:39</dcterms:issued>
				<skos:broader rdf:resource="http://purl.org/heritagedata/schemes/3/concepts/501889" />
				<skos:scopeNote xml:lang="en">A Fishing Vessel which has been requisitioned for war service, generally within its local area, with an unchanged crew and with the fitting of only basic armament (if any Such vessels were used for transport and light towage as well as patrol purposes.</skos:scopeNote>
			</skos:Concept>
		</skos:narrower>
		<skos:narrower>
			<skos:Concept rdf:about="http://purl.org/heritagedata/schemes/3/concepts/501960">
				<skos:inScheme rdf:resource="http://purl.org/heritagedata/schemes/3" />
				<dcterms:identifier>http://purl.org/heritagedata/schemes/3/concepts/501960</dcterms:identifier>
				<cc:license rdf:resource="http://reference.data.gov.uk/id/open-government-licence" />
				<cc:attributionURL rdf:resource="http://www.rcahms.gov.uk" />
				<cc:attributionName xml:lang="en">RCAHMS</cc:attributionName>
				<dcterms:publisher rdf:resource="http://www.rcahms.gov.uk" />
				<skos:prefLabel xml:lang="en">REQUISITIONED MOTOR FISHING VESSEL</skos:prefLabel>
				<dcterms:issued rdf:datatype="http://www.w3.org/2001/XMLSchema#dateTime">2013-07-17T10:08:39</dcterms:issued>
				<skos:broader rdf:resource="http://purl.org/heritagedata/schemes/3/concepts/501889" />
				<skos:scopeNote xml:lang="en">A Motor Fishing Vessel which has been requisitioned for war service, generally within its local area, with an unchanged crew and with the fitting of only basic armament (if any). Such vessels were used for transport and light towage as well as patrol purposes.</skos:scopeNote>
			</skos:Concept>
		</skos:narrower>
		<skos:narrower>
			<skos:Concept rdf:about="http://purl.org/heritagedata/schemes/3/concepts/501976">
				<skos:inScheme rdf:resource="http://purl.org/heritagedata/schemes/3" />
				<dcterms:identifier>http://purl.org/heritagedata/schemes/3/concepts/501976</dcterms:identifier>
				<cc:license rdf:resource="http://reference.data.gov.uk/id/open-government-licence" />
				<cc:attributionURL rdf:resource="http://www.rcahms.gov.uk" />
				<cc:attributionName xml:lang="en">RCAHMS</cc:attributionName>
				<dcterms:publisher rdf:resource="http://www.rcahms.gov.uk" />
				<skos:prefLabel xml:lang="en">SEINE NET FISHING VESSEL</skos:prefLabel>
				<dcterms:issued rdf:datatype="http://www.w3.org/2001/XMLSchema#dateTime">2013-07-17T10:08:39</dcterms:issued>
				<skos:altLabel xml:lang="en">PURSE SEINER</skos:altLabel>
				<skos:altLabel xml:lang="en">SEINER</skos:altLabel>
				<skos:broader rdf:resource="http://purl.org/heritagedata/schemes/3/concepts/501889" />
				<skos:scopeNote xml:lang="en">A Fishing Vessel typically of medium size, constructed and used specifically for Seine Net fishing.</skos:scopeNote>
			</skos:Concept>
		</skos:narrower>
		<skos:narrower rdf:resource="http://purl.org/heritagedata/schemes/3/concepts/502012" />
		<skos:narrower rdf:resource="http://purl.org/heritagedata/schemes/3/concepts/502016" />
		<skos:scopeNote xml:lang="en">A vessel or craft used for catching or harvesting marine life by a variety of methods, use specific method where known.</skos:scopeNote>
	</skos:Concept>
	<skos:Concept rdf:about="http://purl.org/heritagedata/schemes/3/concepts/501898">
		<skos:inScheme rdf:resource="http://purl.org/heritagedata/schemes/3" />
		<dcterms:identifier>http://purl.org/heritagedata/schemes/3/concepts/501898</dcterms:identifier>
		<cc:license rdf:resource="http://reference.data.gov.uk/id/open-government-licence" />
		<cc:attributionURL rdf:resource="http://www.rcahms.gov.uk" />
		<cc:attributionName xml:lang="en">RCAHMS</cc:attributionName>
		<dcterms:publisher rdf:resource="http://www.rcahms.gov.uk" />
		<skos:prefLabel xml:lang="en">HARBOUR SERVICE CRAFT</skos:prefLabel>
		<dcterms:issued rdf:datatype="http://www.w3.org/2001/XMLSchema#dateTime">2013-07-17T10:08:39</dcterms:issued>
		<skos:broader rdf:resource="http://purl.org/heritagedata/schemes/3/concepts/501977" />
		<skos:narrower rdf:resource="http://purl.org/heritagedata/schemes/3/concepts/501919" />
		<skos:narrower rdf:resource="http://purl.org/heritagedata/schemes/3/concepts/502014" />
		<skos:scopeNote xml:lang="en">Craft used to maintain, supply or assist larger vessels whilst in harbour.</skos:scopeNote>
	</skos:Concept>
	<skos:Concept rdf:about="http://purl.org/heritagedata/schemes/3/concepts/501901">
		<skos:inScheme rdf:resource="http://purl.org/heritagedata/schemes/3" />
		<dcterms:identifier>http://purl.org/heritagedata/schemes/3/concepts/501901</dcterms:identifier>
		<cc:license rdf:resource="http://reference.data.gov.uk/id/open-government-licence" />
		<cc:attributionURL rdf:resource="http://www.rcahms.gov.uk" />
		<cc:attributionName xml:lang="en">RCAHMS</cc:attributionName>
		<dcterms:publisher rdf:resource="http://www.rcahms.gov.uk" />
		<skos:prefLabel xml:lang="en">HIGH SPEED LAUNCH</skos:prefLabel>
		<dcterms:issued rdf:datatype="http://www.w3.org/2001/XMLSchema#dateTime">2013-07-17T10:08:39</dcterms:issued>
		<skos:broader rdf:resource="http://purl.org/heritagedata/schemes/3/concepts/501925" />
		<skos:narrower>
			<skos:Concept rdf:about="http://purl.org/heritagedata/schemes/3/concepts/501974">
				<skos:inScheme rdf:resource="http://purl.org/heritagedata/schemes/3" />
				<dcterms:identifier>http://purl.org/heritagedata/schemes/3/concepts/501974</dcterms:identifier>
				<cc:license rdf:resource="http://reference.data.gov.uk/id/open-government-licence" />
				<cc:attributionURL rdf:resource="http://www.rcahms.gov.uk" />
				<cc:attributionName xml:lang="en">RCAHMS</cc:attributionName>
				<dcterms:publisher rdf:resource="http://www.rcahms.gov.uk" />
				<skos:prefLabel xml:lang="en">SEAPLANE TENDER</skos:prefLabel>
				<dcterms:issued rdf:datatype="http://www.w3.org/2001/XMLSchema#dateTime">2013-07-17T10:08:39</dcterms:issued>
				<skos:broader rdf:resource="http://purl.org/heritagedata/schemes/3/concepts/501901" />
				<skos:scopeNote xml:lang="en">A small (but frequently fast and speliciased) vessel used for a variety of tasks concerned with the operation of seaplanes and flying boats. These would typically include towing aircraft, the supply of fuel and weapons, the carriage of crew and passengers, the laying-out of flarepaths, and the provision of rescue cover. There are a number of specialised sub-types within this type, for which the term scow was also used.</skos:scopeNote>
			</skos:Concept>
		</skos:narrower>
		<skos:scopeNote xml:lang="en">Small, fast and powerful craft, typically having planing hulls, limited armament and sparse accommodation, used in military service for aviation-related purposes but not intended for offensive operations. Larger craft of this type were used offshore for air-sea rescue duties, while smaller examples were used in estuaries to support the operation of seaplanes and flying-boats. The former function has been taken over by helicopters while the latter is obsolete.</skos:scopeNote>
	</skos:Concept>
	<skos:Concept rdf:about="http://purl.org/heritagedata/schemes/3/concepts/501905">
		<skos:inScheme rdf:resource="http://purl.org/heritagedata/schemes/3" />
		<dcterms:identifier>http://purl.org/heritagedata/schemes/3/concepts/501905</dcterms:identifier>
		<cc:license rdf:resource="http://reference.data.gov.uk/id/open-government-licence" />
		<cc:attributionURL rdf:resource="http://www.rcahms.gov.uk" />
		<cc:attributionName xml:lang="en">RCAHMS</cc:attributionName>
		<dcterms:publisher rdf:resource="http://www.rcahms.gov.uk" />
		<skos:prefLabel xml:lang="en">HOSPITAL SHIP</skos:prefLabel>
		<dcterms:issued rdf:datatype="http://www.w3.org/2001/XMLSchema#dateTime">2013-07-17T10:08:39</dcterms:issued>
		<skos:broader rdf:resource="http://purl.org/heritagedata/schemes/3/concepts/501943" />
		<skos:broader rdf:resource="http://purl.org/heritagedata/schemes/3/concepts/501948" />
		<skos:scopeNote xml:lang="en">A ship constructed and/or used to accommodate and treat casualties of military operations, usually under specific conditions of the Geneva Convention. Such vessels are normally of considerable size and carry distinctive markings; requisitioned passenger ships are frequently used.</skos:scopeNote>
	</skos:Concept>
	<skos:Concept rdf:about="http://purl.org/heritagedata/schemes/3/concepts/501909">
		<skos:inScheme rdf:resource="http://purl.org/heritagedata/schemes/3" />
		<dcterms:identifier>http://purl.org/heritagedata/schemes/3/concepts/501909</dcterms:identifier>
		<cc:license rdf:resource="http://reference.data.gov.uk/id/open-government-licence" />
		<cc:attributionURL rdf:resource="http://www.rcahms.gov.uk" />
		<cc:attributionName xml:lang="en">RCAHMS</cc:attributionName>
		<dcterms:publisher rdf:resource="http://www.rcahms.gov.uk" />
		<skos:prefLabel xml:lang="en">KETCH</skos:prefLabel>
		<dcterms:issued rdf:datatype="http://www.w3.org/2001/XMLSchema#dateTime">2013-07-17T10:08:39</dcterms:issued>
		<skos:narrower>
			<skos:Concept rdf:about="http://purl.org/heritagedata/schemes/3/concepts/501834">
				<skos:inScheme rdf:resource="http://purl.org/heritagedata/schemes/3" />
				<dcterms:identifier>http://purl.org/heritagedata/schemes/3/concepts/501834</dcterms:identifier>
				<cc:license rdf:resource="http://reference.data.gov.uk/id/open-government-licence" />
				<cc:attributionURL rdf:resource="http://www.rcahms.gov.uk" />
				<cc:attributionName xml:lang="en">RCAHMS</cc:attributionName>
				<dcterms:publisher rdf:resource="http://www.rcahms.gov.uk" />
				<skos:prefLabel xml:lang="en">AUXILIARY KETCH</skos:prefLabel>
				<dcterms:modified rdf:datatype="http://www.w3.org/2001/XMLSchema#dateTime">2007-04-24T11:38:06</dcterms:modified>
				<dcterms:issued rdf:datatype="http://www.w3.org/2001/XMLSchema#dateTime">2013-07-17T10:08:39</dcterms:issued>
				<skos:broader rdf:resource="http://purl.org/heritagedata/schemes/3/concepts/501909" />
				<skos:scopeNote xml:lang="en">A ketch having auxiliary steam or deisel propulsion for use in harbour areas, light airs or contrary winds.</skos:scopeNote>
			</skos:Concept>
		</skos:narrower>
		<skos:narrower>
			<skos:Concept rdf:about="http://purl.org/heritagedata/schemes/3/concepts/501871">
				<skos:inScheme rdf:resource="http://purl.org/heritagedata/schemes/3" />
				<dcterms:identifier>http://purl.org/heritagedata/schemes/3/concepts/501871</dcterms:identifier>
				<cc:license rdf:resource="http://reference.data.gov.uk/id/open-government-licence" />
				<cc:attributionURL rdf:resource="http://www.rcahms.gov.uk" />
				<cc:attributionName xml:lang="en">RCAHMS</cc:attributionName>
				<dcterms:publisher rdf:resource="http://www.rcahms.gov.uk" />
				<skos:prefLabel xml:lang="en">DOGGER</skos:prefLabel>
				<dcterms:issued rdf:datatype="http://www.w3.org/2001/XMLSchema#dateTime">2013-07-17T10:08:39</dcterms:issued>
				<skos:broader rdf:resource="http://purl.org/heritagedata/schemes/3/concepts/501909" />
				<skos:scopeNote xml:lang="en">a small and wide-beamed fishing vessel used in the 17th century and later in the North Sea, traditionally for trawling and line-fishing on the Dogger Bank. This type was rigged as a ketch, having square sails on the mainmast, a lugsail aft, and two jibs on a long bowsprit.</skos:scopeNote>
			</skos:Concept>
		</skos:narrower>
		<skos:broader rdf:resource="http://purl.org/heritagedata/schemes/3/concepts/501968" />
		<skos:scopeNote xml:lang="en">A vessel with two masts, rigged as a ketch, used for coastal trading.</skos:scopeNote>
	</skos:Concept>
	<skos:Concept rdf:about="http://purl.org/heritagedata/schemes/3/concepts/501913">
		<skos:inScheme rdf:resource="http://purl.org/heritagedata/schemes/3" />
		<dcterms:identifier>http://purl.org/heritagedata/schemes/3/concepts/501913</dcterms:identifier>
		<cc:license rdf:resource="http://reference.data.gov.uk/id/open-government-licence" />
		<cc:attributionURL rdf:resource="http://www.rcahms.gov.uk" />
		<cc:attributionName xml:lang="en">RCAHMS</cc:attributionName>
		<dcterms:publisher rdf:resource="http://www.rcahms.gov.uk" />
		<skos:prefLabel xml:lang="en">LANDING CRAFT</skos:prefLabel>
		<dcterms:issued rdf:datatype="http://www.w3.org/2001/XMLSchema#dateTime">2013-07-17T10:08:39</dcterms:issued>
		<skos:broader rdf:resource="http://purl.org/heritagedata/schemes/3/concepts/502015" />
		<skos:narrower>
			<skos:Concept rdf:about="http://purl.org/heritagedata/schemes/3/concepts/501914">
				<skos:inScheme rdf:resource="http://purl.org/heritagedata/schemes/3" />
				<dcterms:identifier>http://purl.org/heritagedata/schemes/3/concepts/501914</dcterms:identifier>
				<cc:license rdf:resource="http://reference.data.gov.uk/id/open-government-licence" />
				<cc:attributionURL rdf:resource="http://www.rcahms.gov.uk" />
				<cc:attributionName xml:lang="en">RCAHMS</cc:attributionName>
				<dcterms:publisher rdf:resource="http://www.rcahms.gov.uk" />
				<skos:prefLabel xml:lang="en">LANDING SHIP INFANTRY</skos:prefLabel>
				<dcterms:modified rdf:datatype="http://www.w3.org/2001/XMLSchema#dateTime">2008-12-08T12:26:03</dcterms:modified>
				<dcterms:issued rdf:datatype="http://www.w3.org/2001/XMLSchema#dateTime">2013-07-17T10:08:39</dcterms:issued>
				<skos:broader rdf:resource="http://purl.org/heritagedata/schemes/3/concepts/501913" />
				<skos:scopeNote xml:lang="en">Landing Ship Infantry (LSI): vessels of this type were constructed or converted from merchant ships to troops over considerable distances prior to landing them on hostile shore from (smaller) Landing Craft (qv) which were carried on outboard davits. Vessels of this type were used in considerable numbers in the Second World War, being fundamental to operations in the Pacific, but have since been superseded by vessels of the Landing Platform Dock (LPD) and Landing Platform Helicopter (LPH) types.</skos:scopeNote>
			</skos:Concept>
		</skos:narrower>
		<skos:narrower>
			<skos:Concept rdf:about="http://purl.org/heritagedata/schemes/3/concepts/501915">
				<skos:inScheme rdf:resource="http://purl.org/heritagedata/schemes/3" />
				<dcterms:identifier>http://purl.org/heritagedata/schemes/3/concepts/501915</dcterms:identifier>
				<cc:license rdf:resource="http://reference.data.gov.uk/id/open-government-licence" />
				<cc:attributionURL rdf:resource="http://www.rcahms.gov.uk" />
				<cc:attributionName xml:lang="en">RCAHMS</cc:attributionName>
				<dcterms:publisher rdf:resource="http://www.rcahms.gov.uk" />
				<skos:prefLabel xml:lang="en">LANDING CRAFT TANK</skos:prefLabel>
				<dcterms:modified rdf:datatype="http://www.w3.org/2001/XMLSchema#dateTime">2007-04-24T14:38:07</dcterms:modified>
				<dcterms:issued rdf:datatype="http://www.w3.org/2001/XMLSchema#dateTime">2013-07-17T10:08:39</dcterms:issued>
				<skos:broader rdf:resource="http://purl.org/heritagedata/schemes/3/concepts/501913" />
				<skos:scopeNote xml:lang="en">A large Landing Craft specialised to land vehicles (including armoured fighting vehicles) and heavy equipment on beaches from larger vessels moored offshore. Vessels of this type are frequently launched from floodable docks within the parent vessel.</skos:scopeNote>
			</skos:Concept>
		</skos:narrower>
		<skos:scopeNote xml:lang="en">A vessel specialised to land troops and/or military equipment (including artillery and vehicles) on beaches from larger vessels moored offshore. They vary considerably in size, are only used in sheltered waters, and are characterised by having a box-like form and prominent bow-doors.</skos:scopeNote>
	</skos:Concept>
	<skos:Concept rdf:about="http://purl.org/heritagedata/schemes/3/concepts/501916">
		<skos:inScheme rdf:resource="http://purl.org/heritagedata/schemes/3" />
		<dcterms:identifier>http://purl.org/heritagedata/schemes/3/concepts/501916</dcterms:identifier>
		<cc:license rdf:resource="http://reference.data.gov.uk/id/open-government-licence" />
		<cc:attributionURL rdf:resource="http://www.rcahms.gov.uk" />
		<cc:attributionName xml:lang="en">RCAHMS</cc:attributionName>
		<dcterms:publisher rdf:resource="http://www.rcahms.gov.uk" />
		<skos:prefLabel xml:lang="en">LAUNCH</skos:prefLabel>
		<dcterms:issued rdf:datatype="http://www.w3.org/2001/XMLSchema#dateTime">2013-07-17T10:08:39</dcterms:issued>
		<skos:broader rdf:resource="http://purl.org/heritagedata/schemes/3/concepts/501925" />
		<skos:narrower>
			<skos:Concept rdf:about="http://purl.org/heritagedata/schemes/3/concepts/501934">
				<skos:inScheme rdf:resource="http://purl.org/heritagedata/schemes/3" />
				<dcterms:identifier>http://purl.org/heritagedata/schemes/3/concepts/501934</dcterms:identifier>
				<cc:license rdf:resource="http://reference.data.gov.uk/id/open-government-licence" />
				<cc:attributionURL rdf:resource="http://www.rcahms.gov.uk" />
				<cc:attributionName xml:lang="en">RCAHMS</cc:attributionName>
				<dcterms:publisher rdf:resource="http://www.rcahms.gov.uk" />
				<skos:prefLabel xml:lang="en">MOTOR LAUNCH</skos:prefLabel>
				<dcterms:issued rdf:datatype="http://www.w3.org/2001/XMLSchema#dateTime">2013-07-17T10:08:39</dcterms:issued>
				<skos:broader rdf:resource="http://purl.org/heritagedata/schemes/3/concepts/501916" />
				<skos:scopeNote xml:lang="en">Generic name for a small steam or power boat often carried on board a larger vessel.</skos:scopeNote>
			</skos:Concept>
		</skos:narrower>
		<skos:narrower>
			<skos:Concept rdf:about="http://purl.org/heritagedata/schemes/3/concepts/501990">
				<skos:inScheme rdf:resource="http://purl.org/heritagedata/schemes/3" />
				<dcterms:identifier>http://purl.org/heritagedata/schemes/3/concepts/501990</dcterms:identifier>
				<cc:license rdf:resource="http://reference.data.gov.uk/id/open-government-licence" />
				<cc:attributionURL rdf:resource="http://www.rcahms.gov.uk" />
				<cc:attributionName xml:lang="en">RCAHMS</cc:attributionName>
				<dcterms:publisher rdf:resource="http://www.rcahms.gov.uk" />
				<skos:prefLabel xml:lang="en">STEAM LAUNCH</skos:prefLabel>
				<dcterms:issued rdf:datatype="http://www.w3.org/2001/XMLSchema#dateTime">2013-07-17T10:08:39</dcterms:issued>
				<skos:broader rdf:resource="http://purl.org/heritagedata/schemes/3/concepts/501916" />
				<skos:scopeNote xml:lang="en">A Launch powered by an integral diesel engine.</skos:scopeNote>
			</skos:Concept>
		</skos:narrower>
		<skos:scopeNote xml:lang="en">The meaning of this term has varied considerably over time, being applied to both large and heavy ship¿s boats and small open or half-decked vessels intended for general use in sheltered waters. Vessels within the latter category generally have mechanical propulsion, and are of flat-bottomed form. The term is characterised by a degree of status, which may be reflected in ostentatious ornament.</skos:scopeNote>
	</skos:Concept>
	<skos:Concept rdf:about="http://purl.org/heritagedata/schemes/3/concepts/501919">
		<skos:inScheme rdf:resource="http://purl.org/heritagedata/schemes/3" />
		<dcterms:identifier>http://purl.org/heritagedata/schemes/3/concepts/501919</dcterms:identifier>
		<cc:license rdf:resource="http://reference.data.gov.uk/id/open-government-licence" />
		<cc:attributionURL rdf:resource="http://www.rcahms.gov.uk" />
		<cc:attributionName xml:lang="en">RCAHMS</cc:attributionName>
		<dcterms:publisher rdf:resource="http://www.rcahms.gov.uk" />
		<skos:prefLabel xml:lang="en">LIGHTER</skos:prefLabel>
		<dcterms:issued rdf:datatype="http://www.w3.org/2001/XMLSchema#dateTime">2013-07-17T10:08:39</dcterms:issued>
		<skos:broader rdf:resource="http://purl.org/heritagedata/schemes/3/concepts/501898" />
		<skos:narrower>
			<skos:Concept rdf:about="http://purl.org/heritagedata/schemes/3/concepts/501991">
				<skos:inScheme rdf:resource="http://purl.org/heritagedata/schemes/3" />
				<dcterms:identifier>http://purl.org/heritagedata/schemes/3/concepts/501991</dcterms:identifier>
				<cc:license rdf:resource="http://reference.data.gov.uk/id/open-government-licence" />
				<cc:attributionURL rdf:resource="http://www.rcahms.gov.uk" />
				<cc:attributionName xml:lang="en">RCAHMS</cc:attributionName>
				<dcterms:publisher rdf:resource="http://www.rcahms.gov.uk" />
				<skos:prefLabel xml:lang="en">STEAM LIGHTER</skos:prefLabel>
				<dcterms:issued rdf:datatype="http://www.w3.org/2001/XMLSchema#dateTime">2013-07-17T10:08:39</dcterms:issued>
				<skos:broader rdf:resource="http://purl.org/heritagedata/schemes/3/concepts/501919" />
				<skos:scopeNote xml:lang="en">A simple vessel used for cargo-carrying in sheltered waters. Many of the losses recorded as steam lighters were probably puffers.</skos:scopeNote>
			</skos:Concept>
		</skos:narrower>
		<skos:scopeNote xml:lang="en">a simple vessel used for cargo-carrying in sheltered waters, and generally unpowered except by sweeps on occasion.</skos:scopeNote>
	</skos:Concept>
	<skos:Concept rdf:about="http://purl.org/heritagedata/schemes/3/concepts/501924">
		<skos:inScheme rdf:resource="http://purl.org/heritagedata/schemes/3" />
		<dcterms:identifier>http://purl.org/heritagedata/schemes/3/concepts/501924</dcterms:identifier>
		<cc:license rdf:resource="http://reference.data.gov.uk/id/open-government-licence" />
		<cc:attributionURL rdf:resource="http://www.rcahms.gov.uk" />
		<cc:attributionName xml:lang="en">RCAHMS</cc:attributionName>
		<dcterms:publisher rdf:resource="http://www.rcahms.gov.uk" />
		<skos:prefLabel xml:lang="en">LUGGER</skos:prefLabel>
		<dcterms:issued rdf:datatype="http://www.w3.org/2001/XMLSchema#dateTime">2013-07-17T10:08:39</dcterms:issued>
		<skos:narrower>
			<skos:Concept rdf:about="http://purl.org/heritagedata/schemes/3/concepts/501835">
				<skos:inScheme rdf:resource="http://purl.org/heritagedata/schemes/3" />
				<dcterms:identifier>http://purl.org/heritagedata/schemes/3/concepts/501835</dcterms:identifier>
				<cc:license rdf:resource="http://reference.data.gov.uk/id/open-government-licence" />
				<cc:attributionURL rdf:resource="http://www.rcahms.gov.uk" />
				<cc:attributionName xml:lang="en">RCAHMS</cc:attributionName>
				<dcterms:publisher rdf:resource="http://www.rcahms.gov.uk" />
				<skos:prefLabel xml:lang="en">AUXILIARY LUGGER</skos:prefLabel>
				<dcterms:modified rdf:datatype="http://www.w3.org/2001/XMLSchema#dateTime">2007-04-24T11:49:00</dcterms:modified>
				<dcterms:issued rdf:datatype="http://www.w3.org/2001/XMLSchema#dateTime">2013-07-17T10:08:39</dcterms:issued>
				<skos:broader rdf:resource="http://purl.org/heritagedata/schemes/3/concepts/501924" />
				<skos:scopeNote xml:lang="en">A lugger having auxiliary steam or deisel propulsion for use in harbour areas, light airs or contrary winds.</skos:scopeNote>
			</skos:Concept>
		</skos:narrower>
		<skos:broader rdf:resource="http://purl.org/heritagedata/schemes/3/concepts/501968" />
		<skos:scopeNote xml:lang="en">In general terms, vessel powered by a quadrilateral sail which projects forward of the mast. Specifically, a vessel (generally decked and of considerable size) used typically as a drifter and having a single mast which was lowered during fishing; a small steam engine was sometimes fitted for sail- and net-handling. The terms Fifie, Zulu and Scaffie refer to variations within this type, which were unspecified in reports of loss.
The puffer has become a Scottish icon; several examples are preserved, notably at the Scottish Fisheries Museum, Anstruther.</skos:scopeNote>
	</skos:Concept>
	<skos:Concept rdf:about="http://purl.org/heritagedata/schemes/3/concepts/501925">
		<skos:inScheme rdf:resource="http://purl.org/heritagedata/schemes/3" />
		<dcterms:identifier>http://purl.org/heritagedata/schemes/3/concepts/501925</dcterms:identifier>
		<cc:license rdf:resource="http://reference.data.gov.uk/id/open-government-licence" />
		<cc:attributionURL rdf:resource="http://www.rcahms.gov.uk" />
		<cc:attributionName xml:lang="en">RCAHMS</cc:attributionName>
		<dcterms:publisher rdf:resource="http://www.rcahms.gov.uk" />
		<skos:topConceptOf rdf:resource="http://purl.org/heritagedata/schemes/3" />
		<skos:prefLabel xml:lang="en">MARITIME CRAFT</skos:prefLabel>
		<dcterms:modified rdf:datatype="http://www.w3.org/2001/XMLSchema#dateTime">2007-07-19T08:51:34</dcterms:modified>
		<dcterms:issued rdf:datatype="http://www.w3.org/2001/XMLSchema#dateTime">2013-07-17T10:08:39</dcterms:issued>
		<skos:narrower>
			<skos:Concept rdf:about="http://purl.org/heritagedata/schemes/3/concepts/501828">
				<skos:inScheme rdf:resource="http://purl.org/heritagedata/schemes/3" />
				<dcterms:identifier>http://purl.org/heritagedata/schemes/3/concepts/501828</dcterms:identifier>
				<cc:license rdf:resource="http://reference.data.gov.uk/id/open-government-licence" />
				<cc:attributionURL rdf:resource="http://www.rcahms.gov.uk" />
				<cc:attributionName xml:lang="en">RCAHMS</cc:attributionName>
				<dcterms:publisher rdf:resource="http://www.rcahms.gov.uk" />
				<skos:prefLabel xml:lang="en">ARMED BOARDING VESSEL</skos:prefLabel>
				<dcterms:issued rdf:datatype="http://www.w3.org/2001/XMLSchema#dateTime">2013-07-17T10:08:39</dcterms:issued>
				<skos:broader rdf:resource="http://purl.org/heritagedata/schemes/3/concepts/501925" />
				<skos:scopeNote xml:lang="en">A requisitioned, adapted and (generally) armed merchant vessel used to enforce a naval blockade by boarding suspect vessels and inspecting them for contraband. In practice, this category covers a wide variety of vessel, and merges into the various categories of requisitioned craft that are noted as such.</skos:scopeNote>
			</skos:Concept>
		</skos:narrower>
		<skos:narrower rdf:resource="http://purl.org/heritagedata/schemes/3/concepts/501848" />
		<skos:narrower rdf:resource="http://purl.org/heritagedata/schemes/3/concepts/501863" />
		<skos:narrower rdf:resource="http://purl.org/heritagedata/schemes/3/concepts/501865" />
		<skos:narrower rdf:resource="http://purl.org/heritagedata/schemes/3/concepts/501872" />
		<skos:narrower rdf:resource="http://purl.org/heritagedata/schemes/3/concepts/501882" />
		<skos:narrower>
			<skos:Concept rdf:about="http://purl.org/heritagedata/schemes/3/concepts/501883">
				<skos:inScheme rdf:resource="http://purl.org/heritagedata/schemes/3" />
				<dcterms:identifier>http://purl.org/heritagedata/schemes/3/concepts/501883</dcterms:identifier>
				<cc:license rdf:resource="http://reference.data.gov.uk/id/open-government-licence" />
				<cc:attributionURL rdf:resource="http://www.rcahms.gov.uk" />
				<cc:attributionName xml:lang="en">RCAHMS</cc:attributionName>
				<dcterms:publisher rdf:resource="http://www.rcahms.gov.uk" />
				<skos:prefLabel xml:lang="en">FACTORY TRAWLER</skos:prefLabel>
				<dcterms:modified rdf:datatype="http://www.w3.org/2001/XMLSchema#dateTime">2007-04-24T12:03:52</dcterms:modified>
				<dcterms:issued rdf:datatype="http://www.w3.org/2001/XMLSchema#dateTime">2013-07-17T10:08:39</dcterms:issued>
				<skos:broader rdf:resource="http://purl.org/heritagedata/schemes/3/concepts/501925" />
				<skos:scopeNote xml:lang="en">A large and powerful trawler comprehensively equipped for the gutting, preparation and freezing of fish on board. Like other trawlers of recent years, such vessels typically shoot nets astern, and have large stern ramps for the purpose. Some fish by suction, rather than trawling.Together with Fish Carriers and Fish Factory Ships vessels of this type are associated with the Russian 'Klondykers' which operated off Scotland during the Soviet period.</skos:scopeNote>
			</skos:Concept>
		</skos:narrower>
		<skos:narrower>
			<skos:Concept rdf:about="http://purl.org/heritagedata/schemes/3/concepts/501887">
				<skos:inScheme rdf:resource="http://purl.org/heritagedata/schemes/3" />
				<dcterms:identifier>http://purl.org/heritagedata/schemes/3/concepts/501887</dcterms:identifier>
				<cc:license rdf:resource="http://reference.data.gov.uk/id/open-government-licence" />
				<cc:attributionURL rdf:resource="http://www.rcahms.gov.uk" />
				<cc:attributionName xml:lang="en">RCAHMS</cc:attributionName>
				<dcterms:publisher rdf:resource="http://www.rcahms.gov.uk" />
				<skos:prefLabel xml:lang="en">FISH CARRIER</skos:prefLabel>
				<dcterms:modified rdf:datatype="http://www.w3.org/2001/XMLSchema#dateTime">2007-04-24T12:04:31</dcterms:modified>
				<dcterms:issued rdf:datatype="http://www.w3.org/2001/XMLSchema#dateTime">2013-07-17T10:08:39</dcterms:issued>
				<skos:broader rdf:resource="http://purl.org/heritagedata/schemes/3/concepts/501925" />
				<skos:scopeNote xml:lang="en">A refrigerated ship used to take the processed catch back to the home port after receipt from Factory Trawlers and Fish Factory Ships.
Together with Factory Trawlers and Fish Factory Ships vessels of this type are associated with the Russian 'Klondykers' which operated off Scotland during the Soviet period.</skos:scopeNote>
			</skos:Concept>
		</skos:narrower>
		<skos:narrower>
			<skos:Concept rdf:about="http://purl.org/heritagedata/schemes/3/concepts/501888">
				<skos:inScheme rdf:resource="http://purl.org/heritagedata/schemes/3" />
				<dcterms:identifier>http://purl.org/heritagedata/schemes/3/concepts/501888</dcterms:identifier>
				<cc:license rdf:resource="http://reference.data.gov.uk/id/open-government-licence" />
				<cc:attributionURL rdf:resource="http://www.rcahms.gov.uk" />
				<cc:attributionName xml:lang="en">RCAHMS</cc:attributionName>
				<dcterms:publisher rdf:resource="http://www.rcahms.gov.uk" />
				<skos:prefLabel xml:lang="en">FISH FACTORY SHIP</skos:prefLabel>
				<dcterms:modified rdf:datatype="http://www.w3.org/2001/XMLSchema#dateTime">2007-04-24T12:05:24</dcterms:modified>
				<dcterms:issued rdf:datatype="http://www.w3.org/2001/XMLSchema#dateTime">2013-07-17T10:08:39</dcterms:issued>
				<skos:broader rdf:resource="http://purl.org/heritagedata/schemes/3/concepts/501925" />
				<skos:scopeNote xml:lang="en">A specialised vessel equipped for the gutting, preparation and freezing of fish received from associated trawlers of recent years.
Together with Fish Carriers and Fish Factory Ships vessels of this type are associated with the Russian 'Klondykers' which operated off Scotland during the Soviet period.</skos:scopeNote>
			</skos:Concept>
		</skos:narrower>
		<skos:narrower rdf:resource="http://purl.org/heritagedata/schemes/3/concepts/501889" />
		<skos:narrower>
			<skos:Concept rdf:about="http://purl.org/heritagedata/schemes/3/concepts/501890">
				<skos:inScheme rdf:resource="http://purl.org/heritagedata/schemes/3" />
				<dcterms:identifier>http://purl.org/heritagedata/schemes/3/concepts/501890</dcterms:identifier>
				<cc:license rdf:resource="http://reference.data.gov.uk/id/open-government-licence" />
				<cc:attributionURL rdf:resource="http://www.rcahms.gov.uk" />
				<cc:attributionName xml:lang="en">RCAHMS</cc:attributionName>
				<dcterms:publisher rdf:resource="http://www.rcahms.gov.uk" />
				<skos:prefLabel xml:lang="en">FLYING BOAT</skos:prefLabel>
				<dcterms:modified rdf:datatype="http://www.w3.org/2001/XMLSchema#dateTime">2011-08-19T08:45:30</dcterms:modified>
				<dcterms:issued rdf:datatype="http://www.w3.org/2001/XMLSchema#dateTime">2013-07-17T10:08:39</dcterms:issued>
				<skos:broader rdf:resource="http://purl.org/heritagedata/schemes/3/concepts/501925" />
				<skos:scopeNote xml:lang="en">An aircraft intended for operation from water and built around a watertight hull of planing form. Such aircraft may be fitted with wheels for beaching and/or amphibious operation, and should be differentiated from Seaplanes.</skos:scopeNote>
			</skos:Concept>
		</skos:narrower>
		<skos:narrower>
			<skos:Concept rdf:about="http://purl.org/heritagedata/schemes/3/concepts/501894">
				<skos:inScheme rdf:resource="http://purl.org/heritagedata/schemes/3" />
				<dcterms:identifier>http://purl.org/heritagedata/schemes/3/concepts/501894</dcterms:identifier>
				<cc:license rdf:resource="http://reference.data.gov.uk/id/open-government-licence" />
				<cc:attributionURL rdf:resource="http://www.rcahms.gov.uk" />
				<cc:attributionName xml:lang="en">RCAHMS</cc:attributionName>
				<dcterms:publisher rdf:resource="http://www.rcahms.gov.uk" />
				<skos:prefLabel xml:lang="en">GABBART</skos:prefLabel>
				<dcterms:modified rdf:datatype="http://www.w3.org/2001/XMLSchema#dateTime">2011-08-19T08:45:42</dcterms:modified>
				<dcterms:issued rdf:datatype="http://www.w3.org/2001/XMLSchema#dateTime">2013-07-17T10:08:39</dcterms:issued>
				<skos:broader rdf:resource="http://purl.org/heritagedata/schemes/3/concepts/501925" />
				<skos:scopeNote xml:lang="en">Double-ended and full-bodied sailing vessel common around Scotland and sized to pass through the central Scottish canals; typically gaff-rigged.</skos:scopeNote>
			</skos:Concept>
		</skos:narrower>
		<skos:narrower rdf:resource="http://purl.org/heritagedata/schemes/3/concepts/501901" />
		<skos:narrower rdf:resource="http://purl.org/heritagedata/schemes/3/concepts/501916" />
		<skos:narrower>
			<skos:Concept rdf:about="http://purl.org/heritagedata/schemes/3/concepts/501936">
				<skos:inScheme rdf:resource="http://purl.org/heritagedata/schemes/3" />
				<dcterms:identifier>http://purl.org/heritagedata/schemes/3/concepts/501936</dcterms:identifier>
				<cc:license rdf:resource="http://reference.data.gov.uk/id/open-government-licence" />
				<cc:attributionURL rdf:resource="http://www.rcahms.gov.uk" />
				<cc:attributionName xml:lang="en">RCAHMS</cc:attributionName>
				<dcterms:publisher rdf:resource="http://www.rcahms.gov.uk" />
				<skos:prefLabel xml:lang="en">MOTOR TANKER</skos:prefLabel>
				<dcterms:issued rdf:datatype="http://www.w3.org/2001/XMLSchema#dateTime">2013-07-17T10:08:39</dcterms:issued>
				<skos:broader rdf:resource="http://purl.org/heritagedata/schemes/3/concepts/501925" />
				<skos:scopeNote xml:lang="en">A Tanker with  integral motor propulsion.</skos:scopeNote>
			</skos:Concept>
		</skos:narrower>
		<skos:narrower rdf:resource="http://purl.org/heritagedata/schemes/3/concepts/501939" />
		<skos:narrower rdf:resource="http://purl.org/heritagedata/schemes/3/concepts/501943" />
		<skos:narrower>
			<skos:Concept rdf:about="http://purl.org/heritagedata/schemes/3/concepts/501944">
				<skos:inScheme rdf:resource="http://purl.org/heritagedata/schemes/3" />
				<dcterms:identifier>http://purl.org/heritagedata/schemes/3/concepts/501944</dcterms:identifier>
				<cc:license rdf:resource="http://reference.data.gov.uk/id/open-government-licence" />
				<cc:attributionURL rdf:resource="http://www.rcahms.gov.uk" />
				<cc:attributionName xml:lang="en">RCAHMS</cc:attributionName>
				<dcterms:publisher rdf:resource="http://www.rcahms.gov.uk" />
				<skos:prefLabel xml:lang="en">OFFSHORE SUPPORT VESSEL</skos:prefLabel>
				<dcterms:modified rdf:datatype="http://www.w3.org/2001/XMLSchema#dateTime">2007-04-24T12:10:33</dcterms:modified>
				<dcterms:issued rdf:datatype="http://www.w3.org/2001/XMLSchema#dateTime">2013-07-17T10:08:39</dcterms:issued>
				<skos:broader rdf:resource="http://purl.org/heritagedata/schemes/3/concepts/501925" />
				<skos:scopeNote xml:lang="en">Developed in the 1970s as the workhorse of offshore industry, this type of vessel is characterised by a long after deck which is placed beneath the oil or gas platform to allow cargo and personnel to be hoisted vertically from it. Other storage facilities include tanks for drinking water, drilling mud, and various types of fuel. Towing bitts, a helicopter pad and firefighting equipment are also commonly fitted while some have been converted for diving support and as rescue vessels. The term Rig Support Vessel has also been applied to this versatile type.</skos:scopeNote>
			</skos:Concept>
		</skos:narrower>
		<skos:narrower>
			<skos:Concept rdf:about="http://purl.org/heritagedata/schemes/3/concepts/501945">
				<skos:inScheme rdf:resource="http://purl.org/heritagedata/schemes/3" />
				<dcterms:identifier>http://purl.org/heritagedata/schemes/3/concepts/501945</dcterms:identifier>
				<cc:license rdf:resource="http://reference.data.gov.uk/id/open-government-licence" />
				<cc:attributionURL rdf:resource="http://www.rcahms.gov.uk" />
				<cc:attributionName xml:lang="en">RCAHMS</cc:attributionName>
				<dcterms:publisher rdf:resource="http://www.rcahms.gov.uk" />
				<skos:prefLabel xml:lang="en">OILER</skos:prefLabel>
				<dcterms:issued rdf:datatype="http://www.w3.org/2001/XMLSchema#dateTime">2013-07-17T10:08:39</dcterms:issued>
				<skos:broader rdf:resource="http://purl.org/heritagedata/schemes/3/concepts/501925" />
				<skos:scopeNote xml:lang="en">Generic term for all vessels used to supply warships with any type of fuel.</skos:scopeNote>
			</skos:Concept>
		</skos:narrower>
		<skos:narrower>
			<skos:Concept rdf:about="http://purl.org/heritagedata/schemes/3/concepts/501947">
				<skos:inScheme rdf:resource="http://purl.org/heritagedata/schemes/3" />
				<dcterms:identifier>http://purl.org/heritagedata/schemes/3/concepts/501947</dcterms:identifier>
				<cc:license rdf:resource="http://reference.data.gov.uk/id/open-government-licence" />
				<cc:attributionURL rdf:resource="http://www.rcahms.gov.uk" />
				<cc:attributionName xml:lang="en">RCAHMS</cc:attributionName>
				<dcterms:publisher rdf:resource="http://www.rcahms.gov.uk" />
				<skos:prefLabel xml:lang="en">PADDLE STEAMER</skos:prefLabel>
				<dcterms:issued rdf:datatype="http://www.w3.org/2001/XMLSchema#dateTime">2013-07-17T10:08:39</dcterms:issued>
				<skos:broader rdf:resource="http://purl.org/heritagedata/schemes/3/concepts/501925" />
				<skos:scopeNote xml:lang="en">A steam vessel propelled by a pair of paddle wheels amidships or a single wheel astern, driven by a reciprocating engine.</skos:scopeNote>
			</skos:Concept>
		</skos:narrower>
		<skos:narrower rdf:resource="http://purl.org/heritagedata/schemes/3/concepts/501950" />
		<skos:narrower rdf:resource="http://purl.org/heritagedata/schemes/3/concepts/501956" />
		<skos:narrower rdf:resource="http://purl.org/heritagedata/schemes/3/concepts/501968" />
		<skos:narrower rdf:resource="http://purl.org/heritagedata/schemes/3/concepts/501969" />
		<skos:narrower>
			<skos:Concept rdf:about="http://purl.org/heritagedata/schemes/3/concepts/501972">
				<skos:inScheme rdf:resource="http://purl.org/heritagedata/schemes/3" />
				<dcterms:identifier>http://purl.org/heritagedata/schemes/3/concepts/501972</dcterms:identifier>
				<cc:license rdf:resource="http://reference.data.gov.uk/id/open-government-licence" />
				<cc:attributionURL rdf:resource="http://www.rcahms.gov.uk" />
				<cc:attributionName xml:lang="en">RCAHMS</cc:attributionName>
				<dcterms:publisher rdf:resource="http://www.rcahms.gov.uk" />
				<skos:prefLabel xml:lang="en">SCOW</skos:prefLabel>
				<dcterms:issued rdf:datatype="http://www.w3.org/2001/XMLSchema#dateTime">2013-07-17T10:08:39</dcterms:issued>
				<skos:broader rdf:resource="http://purl.org/heritagedata/schemes/3/concepts/501925" />
				<skos:scopeNote xml:lang="en">A large flat-bottomed boat, towed or propelled by oars (sweeps), and commonly used as a ferry or lighter.</skos:scopeNote>
			</skos:Concept>
		</skos:narrower>
		<skos:narrower>
			<skos:Concept rdf:about="http://purl.org/heritagedata/schemes/3/concepts/501973">
				<skos:inScheme rdf:resource="http://purl.org/heritagedata/schemes/3" />
				<dcterms:identifier>http://purl.org/heritagedata/schemes/3/concepts/501973</dcterms:identifier>
				<cc:license rdf:resource="http://reference.data.gov.uk/id/open-government-licence" />
				<cc:attributionURL rdf:resource="http://www.rcahms.gov.uk" />
				<cc:attributionName xml:lang="en">RCAHMS</cc:attributionName>
				<dcterms:publisher rdf:resource="http://www.rcahms.gov.uk" />
				<skos:prefLabel xml:lang="en">SEAPLANE</skos:prefLabel>
				<dcterms:issued rdf:datatype="http://www.w3.org/2001/XMLSchema#dateTime">2013-07-17T10:08:39</dcterms:issued>
				<skos:broader rdf:resource="http://purl.org/heritagedata/schemes/3/concepts/501925" />
				<skos:scopeNote xml:lang="en">An aircraft intended for operation from water but built without  a watertight hull, having instead a float undercarriage. Such aircraft may be fitted with wheels for beaching and/or amphibious operation, and should be differentiated from Flying Boats.</skos:scopeNote>
			</skos:Concept>
		</skos:narrower>
		<skos:narrower rdf:resource="http://purl.org/heritagedata/schemes/3/concepts/501977" />
		<skos:narrower>
			<skos:Concept rdf:about="http://purl.org/heritagedata/schemes/3/concepts/501978">
				<skos:inScheme rdf:resource="http://purl.org/heritagedata/schemes/3" />
				<dcterms:identifier>http://purl.org/heritagedata/schemes/3/concepts/501978</dcterms:identifier>
				<cc:license rdf:resource="http://reference.data.gov.uk/id/open-government-licence" />
				<cc:attributionURL rdf:resource="http://www.rcahms.gov.uk" />
				<cc:attributionName xml:lang="en">RCAHMS</cc:attributionName>
				<dcterms:publisher rdf:resource="http://www.rcahms.gov.uk" />
				<skos:prefLabel xml:lang="en">SHIP</skos:prefLabel>
				<dcterms:modified rdf:datatype="http://www.w3.org/2001/XMLSchema#dateTime">2007-04-24T12:17:55</dcterms:modified>
				<dcterms:issued rdf:datatype="http://www.w3.org/2001/XMLSchema#dateTime">2013-07-17T10:08:39</dcterms:issued>
				<skos:broader rdf:resource="http://purl.org/heritagedata/schemes/3/concepts/501925" />
				<skos:scopeNote xml:lang="en">A sailing vessel (by contrast to Steamship) of considerable size and full-rigged, having square sails on all of three or more masts, by contrast with a Barque, which only has fore-and-aft sails on the mizzen. Most large warships of the classic (Nelsonian) period fall within this category.</skos:scopeNote>
			</skos:Concept>
		</skos:narrower>
		<skos:narrower>
			<skos:Concept rdf:about="http://purl.org/heritagedata/schemes/3/concepts/501986">
				<skos:inScheme rdf:resource="http://purl.org/heritagedata/schemes/3" />
				<dcterms:identifier>http://purl.org/heritagedata/schemes/3/concepts/501986</dcterms:identifier>
				<cc:license rdf:resource="http://reference.data.gov.uk/id/open-government-licence" />
				<cc:attributionURL rdf:resource="http://www.rcahms.gov.uk" />
				<cc:attributionName xml:lang="en">RCAHMS</cc:attributionName>
				<dcterms:publisher rdf:resource="http://www.rcahms.gov.uk" />
				<skos:prefLabel xml:lang="en">SPEEDBOAT</skos:prefLabel>
				<dcterms:issued rdf:datatype="http://www.w3.org/2001/XMLSchema#dateTime">2013-07-17T10:08:39</dcterms:issued>
				<skos:broader rdf:resource="http://purl.org/heritagedata/schemes/3/concepts/501925" />
				<skos:scopeNote xml:lang="en">A specialised type of vessel, built around an inboard engine (of either internal combustion or gas turbine type) optimised specifically for performance, often within defined specifications or formulae. Such craft may be used for competition (in racing or by record-breaking) or experimental purposes, and are commonly kept ashore, being used only in sheltered waters under favourable conditions. The hulls may be of displacement, planing or hydrofoil form, the second being the most common.</skos:scopeNote>
			</skos:Concept>
		</skos:narrower>
		<skos:narrower>
			<skos:Concept rdf:about="http://purl.org/heritagedata/schemes/3/concepts/501992">
				<skos:inScheme rdf:resource="http://purl.org/heritagedata/schemes/3" />
				<dcterms:identifier>http://purl.org/heritagedata/schemes/3/concepts/501992</dcterms:identifier>
				<cc:license rdf:resource="http://reference.data.gov.uk/id/open-government-licence" />
				<cc:attributionURL rdf:resource="http://www.rcahms.gov.uk" />
				<cc:attributionName xml:lang="en">RCAHMS</cc:attributionName>
				<dcterms:publisher rdf:resource="http://www.rcahms.gov.uk" />
				<skos:prefLabel xml:lang="en">STEAM PACKET</skos:prefLabel>
				<dcterms:issued rdf:datatype="http://www.w3.org/2001/XMLSchema#dateTime">2013-07-17T10:08:39</dcterms:issued>
				<skos:broader rdf:resource="http://purl.org/heritagedata/schemes/3/concepts/501925" />
				<skos:scopeNote xml:lang="en">A vessel powered by an integral steam engine and used for the carriage of mail (and commonly also passengers), typically along set routes and in accordance with a published timetable. Vessels of this type were commonly built for speed (with fine lines) and were on occasion operated by the Admiralty, being naval-manned and/or lightly armed. The term remained in anachronistic use after the type was superseded, the concept being revived as Royal Mail Ship (RMS).</skos:scopeNote>
			</skos:Concept>
		</skos:narrower>
		<skos:narrower>
			<skos:Concept rdf:about="http://purl.org/heritagedata/schemes/3/concepts/502004">
				<skos:inScheme rdf:resource="http://purl.org/heritagedata/schemes/3" />
				<dcterms:identifier>http://purl.org/heritagedata/schemes/3/concepts/502004</dcterms:identifier>
				<cc:license rdf:resource="http://reference.data.gov.uk/id/open-government-licence" />
				<cc:attributionURL rdf:resource="http://www.rcahms.gov.uk" />
				<cc:attributionName xml:lang="en">RCAHMS</cc:attributionName>
				<dcterms:publisher rdf:resource="http://www.rcahms.gov.uk" />
				<skos:prefLabel xml:lang="en">SURVEY VESSEL</skos:prefLabel>
				<dcterms:issued rdf:datatype="http://www.w3.org/2001/XMLSchema#dateTime">2013-07-17T10:08:39</dcterms:issued>
				<skos:broader rdf:resource="http://purl.org/heritagedata/schemes/3/concepts/501925" />
				<skos:scopeNote xml:lang="en">A craft which is equipped for and performs hydrographic surveys.</skos:scopeNote>
			</skos:Concept>
		</skos:narrower>
		<skos:narrower rdf:resource="http://purl.org/heritagedata/schemes/3/concepts/502011" />
		<skos:narrower rdf:resource="http://purl.org/heritagedata/schemes/3/concepts/502013" />
		<skos:narrower rdf:resource="http://purl.org/heritagedata/schemes/3/concepts/502015" />
		<skos:narrower>
			<skos:Concept rdf:about="http://purl.org/heritagedata/schemes/3/concepts/506041">
				<skos:inScheme rdf:resource="http://purl.org/heritagedata/schemes/3" />
				<dcterms:identifier>http://purl.org/heritagedata/schemes/3/concepts/506041</dcterms:identifier>
				<cc:license rdf:resource="http://reference.data.gov.uk/id/open-government-licence" />
				<cc:attributionURL rdf:resource="http://www.rcahms.gov.uk" />
				<cc:attributionName xml:lang="en">RCAHMS</cc:attributionName>
				<dcterms:publisher rdf:resource="http://www.rcahms.gov.uk" />
				<skos:prefLabel xml:lang="en">GALLEY</skos:prefLabel>
				<dcterms:created rdf:datatype="http://www.w3.org/2001/XMLSchema#dateTime">2011-08-25T14:12:36</dcterms:created>
				<dcterms:modified rdf:datatype="http://www.w3.org/2001/XMLSchema#dateTime">2011-08-25T14:13:22</dcterms:modified>
				<dcterms:issued rdf:datatype="http://www.w3.org/2001/XMLSchema#dateTime">2013-07-17T10:08:39</dcterms:issued>
				<skos:broader rdf:resource="http://purl.org/heritagedata/schemes/3/concepts/501925" />
				<skos:scopeNote xml:lang="en">A specialised class of light oared warship, most commonly used in the Mediterranean, but sometimes used in Northern waters with fore-and-aft rigged sails and a bow-mounted cannon.</skos:scopeNote>
			</skos:Concept>
		</skos:narrower>
		<skos:narrower>
			<skos:Concept rdf:about="http://purl.org/heritagedata/schemes/3/concepts/506161">
				<skos:inScheme rdf:resource="http://purl.org/heritagedata/schemes/3" />
				<dcterms:identifier>http://purl.org/heritagedata/schemes/3/concepts/506161</dcterms:identifier>
				<cc:license rdf:resource="http://reference.data.gov.uk/id/open-government-licence" />
				<cc:attributionURL rdf:resource="http://www.rcahms.gov.uk" />
				<cc:attributionName xml:lang="en">RCAHMS</cc:attributionName>
				<dcterms:publisher rdf:resource="http://www.rcahms.gov.uk" />
				<skos:prefLabel xml:lang="en">PRIVATEER</skos:prefLabel>
				<dcterms:created rdf:datatype="http://www.w3.org/2001/XMLSchema#dateTime">2011-10-18T15:50:06</dcterms:created>
				<dcterms:modified rdf:datatype="http://www.w3.org/2001/XMLSchema#dateTime">2011-10-18T15:51:44</dcterms:modified>
				<dcterms:issued rdf:datatype="http://www.w3.org/2001/XMLSchema#dateTime">2013-07-17T10:08:39</dcterms:issued>
				<skos:broader rdf:resource="http://purl.org/heritagedata/schemes/3/concepts/501925" />
				<skos:scopeNote xml:lang="en">A seagoing vessel designed or operated as a light sailing warship, and deployed semi-officially, with sovereign state sanction ('letters of marque') rather than as a part of of formally-constituted navy. Such vessels were regularly deployed in the Early Modern period, for independent commerce raiding rather than to fight in fleet actions.</skos:scopeNote>
			</skos:Concept>
		</skos:narrower>
		<skos:narrower>
			<skos:Concept rdf:about="http://purl.org/heritagedata/schemes/3/concepts/506081">
				<skos:inScheme rdf:resource="http://purl.org/heritagedata/schemes/3" />
				<dcterms:identifier>http://purl.org/heritagedata/schemes/3/concepts/506081</dcterms:identifier>
				<cc:license rdf:resource="http://reference.data.gov.uk/id/open-government-licence" />
				<cc:attributionURL rdf:resource="http://www.rcahms.gov.uk" />
				<cc:attributionName xml:lang="en">RCAHMS</cc:attributionName>
				<dcterms:publisher rdf:resource="http://www.rcahms.gov.uk" />
				<skos:prefLabel xml:lang="en">HOY</skos:prefLabel>
				<dcterms:created rdf:datatype="http://www.w3.org/2001/XMLSchema#dateTime">2011-09-23T14:56:52</dcterms:created>
				<dcterms:modified rdf:datatype="http://www.w3.org/2001/XMLSchema#dateTime">2011-09-23T14:57:23</dcterms:modified>
				<dcterms:issued rdf:datatype="http://www.w3.org/2001/XMLSchema#dateTime">2013-07-17T10:08:39</dcterms:issued>
				<skos:broader rdf:resource="http://purl.org/heritagedata/schemes/3/concepts/501925" />
				<skos:scopeNote xml:lang="en">General term for a small coasting sailing vessel. No specific sailplan or rig is implied, but the type is of 17th-century Dutch derivation.</skos:scopeNote>
			</skos:Concept>
		</skos:narrower>
		<skos:narrower>
			<skos:Concept rdf:about="http://purl.org/heritagedata/schemes/3/concepts/502891">
				<skos:inScheme rdf:resource="http://purl.org/heritagedata/schemes/3" />
				<dcterms:identifier>http://purl.org/heritagedata/schemes/3/concepts/502891</dcterms:identifier>
				<cc:license rdf:resource="http://reference.data.gov.uk/id/open-government-licence" />
				<cc:attributionURL rdf:resource="http://www.rcahms.gov.uk" />
				<cc:attributionName xml:lang="en">RCAHMS</cc:attributionName>
				<dcterms:publisher rdf:resource="http://www.rcahms.gov.uk" />
				<skos:prefLabel xml:lang="en">OBSTRUCTION</skos:prefLabel>
				<dcterms:created rdf:datatype="http://www.w3.org/2001/XMLSchema#dateTime">2007-09-11T10:04:30</dcterms:created>
				<dcterms:modified rdf:datatype="http://www.w3.org/2001/XMLSchema#dateTime">2007-09-11T10:04:38</dcterms:modified>
				<dcterms:issued rdf:datatype="http://www.w3.org/2001/XMLSchema#dateTime">2013-07-17T10:08:39</dcterms:issued>
				<skos:broader rdf:resource="http://purl.org/heritagedata/schemes/3/concepts/501925" />
				<skos:scopeNote xml:lang="en">Submerged feature of unknown type usually discovered by sailors snagging nets or scraping the keel of a water vessel.</skos:scopeNote>
			</skos:Concept>
		</skos:narrower>
		<skos:narrower>
			<skos:Concept rdf:about="http://purl.org/heritagedata/schemes/3/concepts/503761">
				<skos:inScheme rdf:resource="http://purl.org/heritagedata/schemes/3" />
				<dcterms:identifier>http://purl.org/heritagedata/schemes/3/concepts/503761</dcterms:identifier>
				<cc:license rdf:resource="http://reference.data.gov.uk/id/open-government-licence" />
				<cc:attributionURL rdf:resource="http://www.rcahms.gov.uk" />
				<cc:attributionName xml:lang="en">RCAHMS</cc:attributionName>
				<dcterms:publisher rdf:resource="http://www.rcahms.gov.uk" />
				<skos:prefLabel xml:lang="en">HOUSEBOAT</skos:prefLabel>
				<dcterms:created rdf:datatype="http://www.w3.org/2001/XMLSchema#dateTime">2008-11-24T11:34:30</dcterms:created>
				<dcterms:modified rdf:datatype="http://www.w3.org/2001/XMLSchema#dateTime">2008-11-24T11:43:58</dcterms:modified>
				<dcterms:issued rdf:datatype="http://www.w3.org/2001/XMLSchema#dateTime">2013-07-17T10:08:39</dcterms:issued>
				<skos:altLabel xml:lang="en">HOUSE BOAT</skos:altLabel>
				<skos:broader rdf:resource="http://purl.org/heritagedata/schemes/3/concepts/501925" />
				<skos:scopeNote xml:lang="en">A vessel constructed or adapted for permament or semi-permanent residential occupation, and typically found on inland waterways. Such vessels are unpowered and unseaworthy, and may have fitted mains services. They should be differentiated from accommodation hulks (converted warships) in military service.</skos:scopeNote>
			</skos:Concept>
		</skos:narrower>
		<skos:narrower>
			<skos:Concept rdf:about="http://purl.org/heritagedata/schemes/3/concepts/504420">
				<skos:inScheme rdf:resource="http://purl.org/heritagedata/schemes/3" />
				<dcterms:identifier>http://purl.org/heritagedata/schemes/3/concepts/504420</dcterms:identifier>
				<cc:license rdf:resource="http://reference.data.gov.uk/id/open-government-licence" />
				<cc:attributionURL rdf:resource="http://www.rcahms.gov.uk" />
				<cc:attributionName xml:lang="en">RCAHMS</cc:attributionName>
				<dcterms:publisher rdf:resource="http://www.rcahms.gov.uk" />
				<skos:prefLabel xml:lang="en">AIR SEA RESCUE CRAFT</skos:prefLabel>
				<dcterms:created rdf:datatype="http://www.w3.org/2001/XMLSchema#dateTime">2009-06-23T14:03:39</dcterms:created>
				<dcterms:modified rdf:datatype="http://www.w3.org/2001/XMLSchema#dateTime">2009-06-23T14:04:21</dcterms:modified>
				<dcterms:issued rdf:datatype="http://www.w3.org/2001/XMLSchema#dateTime">2013-07-17T10:08:39</dcterms:issued>
				<skos:broader rdf:resource="http://purl.org/heritagedata/schemes/3/concepts/501925" />
				<skos:scopeNote xml:lang="en">A small but seaworthy vessel designed for the rescue of downed aircrew, often under wartime conditions. Such vessels were typically manned by uniformed (Royal Air Force) personnel, and varied considerably in size and form. The smaller types were high-speed planing craft, and normally termed Rescue Launches; the larger types were slower and had secondary functions as range control and target towing vessels.</skos:scopeNote>
			</skos:Concept>
		</skos:narrower>
		<skos:narrower>
			<skos:Concept rdf:about="http://purl.org/heritagedata/schemes/3/concepts/505962">
				<skos:inScheme rdf:resource="http://purl.org/heritagedata/schemes/3" />
				<dcterms:identifier>http://purl.org/heritagedata/schemes/3/concepts/505962</dcterms:identifier>
				<cc:license rdf:resource="http://reference.data.gov.uk/id/open-government-licence" />
				<cc:attributionURL rdf:resource="http://www.rcahms.gov.uk" />
				<cc:attributionName xml:lang="en">RCAHMS</cc:attributionName>
				<dcterms:publisher rdf:resource="http://www.rcahms.gov.uk" />
				<skos:prefLabel xml:lang="en">RAFT</skos:prefLabel>
				<dcterms:created rdf:datatype="http://www.w3.org/2001/XMLSchema#dateTime">2011-08-01T16:27:29</dcterms:created>
				<dcterms:modified rdf:datatype="http://www.w3.org/2001/XMLSchema#dateTime">2011-08-01T16:28:43</dcterms:modified>
				<dcterms:issued rdf:datatype="http://www.w3.org/2001/XMLSchema#dateTime">2013-07-17T10:08:39</dcterms:issued>
				<skos:broader rdf:resource="http://purl.org/heritagedata/schemes/3/concepts/501925" />
				<skos:scopeNote xml:lang="en">A flat floating framework of planks or other materials used for supporting or carrying persons or goods.</skos:scopeNote>
			</skos:Concept>
		</skos:narrower>
		<skos:scopeNote xml:lang="en">This is the top term for the thesaurus. See the Class List for narrow terms.</skos:scopeNote>
	</skos:Concept>
	<skos:Concept rdf:about="http://purl.org/heritagedata/schemes/3/concepts/501926">
		<skos:inScheme rdf:resource="http://purl.org/heritagedata/schemes/3" />
		<dcterms:identifier>http://purl.org/heritagedata/schemes/3/concepts/501926</dcterms:identifier>
		<cc:license rdf:resource="http://reference.data.gov.uk/id/open-government-licence" />
		<cc:attributionURL rdf:resource="http://www.rcahms.gov.uk" />
		<cc:attributionName xml:lang="en">RCAHMS</cc:attributionName>
		<dcterms:publisher rdf:resource="http://www.rcahms.gov.uk" />
		<skos:prefLabel xml:lang="en">MIDGET SUBMARINE</skos:prefLabel>
		<dcterms:issued rdf:datatype="http://www.w3.org/2001/XMLSchema#dateTime">2013-07-17T10:08:39</dcterms:issued>
		<skos:broader rdf:resource="http://purl.org/heritagedata/schemes/3/concepts/502002" />
		<skos:related rdf:resource="http://purl.org/heritagedata/schemes/3/concepts/503372" />
		<skos:scopeNote xml:lang="en">Small submarine with a two or three man crew. Used for special missions such as sinking warships in heavily defended harbours.</skos:scopeNote>
	</skos:Concept>
	<skos:Concept rdf:about="http://purl.org/heritagedata/schemes/3/concepts/501931">
		<skos:inScheme rdf:resource="http://purl.org/heritagedata/schemes/3" />
		<dcterms:identifier>http://purl.org/heritagedata/schemes/3/concepts/501931</dcterms:identifier>
		<cc:license rdf:resource="http://reference.data.gov.uk/id/open-government-licence" />
		<cc:attributionURL rdf:resource="http://www.rcahms.gov.uk" />
		<cc:attributionName xml:lang="en">RCAHMS</cc:attributionName>
		<dcterms:publisher rdf:resource="http://www.rcahms.gov.uk" />
		<skos:prefLabel xml:lang="en">MOTOR DRIFTER</skos:prefLabel>
		<dcterms:issued rdf:datatype="http://www.w3.org/2001/XMLSchema#dateTime">2013-07-17T10:08:39</dcterms:issued>
		<skos:broader rdf:resource="http://purl.org/heritagedata/schemes/3/concepts/501873" />
		<skos:narrower>
			<skos:Concept rdf:about="http://purl.org/heritagedata/schemes/3/concepts/501959">
				<skos:inScheme rdf:resource="http://purl.org/heritagedata/schemes/3" />
				<dcterms:identifier>http://purl.org/heritagedata/schemes/3/concepts/501959</dcterms:identifier>
				<cc:license rdf:resource="http://reference.data.gov.uk/id/open-government-licence" />
				<cc:attributionURL rdf:resource="http://www.rcahms.gov.uk" />
				<cc:attributionName xml:lang="en">RCAHMS</cc:attributionName>
				<dcterms:publisher rdf:resource="http://www.rcahms.gov.uk" />
				<skos:prefLabel xml:lang="en">REQUISITIONED MOTOR DRIFTER</skos:prefLabel>
				<dcterms:issued rdf:datatype="http://www.w3.org/2001/XMLSchema#dateTime">2013-07-17T10:08:39</dcterms:issued>
				<skos:broader rdf:resource="http://purl.org/heritagedata/schemes/3/concepts/501931" />
				<skos:scopeNote xml:lang="en">A Motor Drifter which has been requisitioned for war service, generally within its local area, with an unchanged crew and with the fitting of only basic armament (if any). Such vessels were used for transport and target-towing as well as patrol duties.</skos:scopeNote>
			</skos:Concept>
		</skos:narrower>
		<skos:scopeNote xml:lang="en">A Drifter with integral motor propulsion.</skos:scopeNote>
	</skos:Concept>
	<skos:Concept rdf:about="http://purl.org/heritagedata/schemes/3/concepts/501938">
		<skos:inScheme rdf:resource="http://purl.org/heritagedata/schemes/3" />
		<dcterms:identifier>http://purl.org/heritagedata/schemes/3/concepts/501938</dcterms:identifier>
		<cc:license rdf:resource="http://reference.data.gov.uk/id/open-government-licence" />
		<cc:attributionURL rdf:resource="http://www.rcahms.gov.uk" />
		<cc:attributionName xml:lang="en">RCAHMS</cc:attributionName>
		<dcterms:publisher rdf:resource="http://www.rcahms.gov.uk" />
		<skos:prefLabel xml:lang="en">MOTOR TRAWLER</skos:prefLabel>
		<dcterms:issued rdf:datatype="http://www.w3.org/2001/XMLSchema#dateTime">2013-07-17T10:08:39</dcterms:issued>
		<skos:broader rdf:resource="http://purl.org/heritagedata/schemes/3/concepts/502012" />
		<skos:narrower>
			<skos:Concept rdf:about="http://purl.org/heritagedata/schemes/3/concepts/502240">
				<skos:inScheme rdf:resource="http://purl.org/heritagedata/schemes/3" />
				<dcterms:identifier>http://purl.org/heritagedata/schemes/3/concepts/502240</dcterms:identifier>
				<cc:license rdf:resource="http://reference.data.gov.uk/id/open-government-licence" />
				<cc:attributionURL rdf:resource="http://www.rcahms.gov.uk" />
				<cc:attributionName xml:lang="en">RCAHMS</cc:attributionName>
				<dcterms:publisher rdf:resource="http://www.rcahms.gov.uk" />
				<skos:prefLabel xml:lang="en">MOTOR STERN TRAWLER</skos:prefLabel>
				<dcterms:created rdf:datatype="http://www.w3.org/2001/XMLSchema#dateTime">2007-05-18T09:06:34</dcterms:created>
				<dcterms:modified rdf:datatype="http://www.w3.org/2001/XMLSchema#dateTime">2007-05-18T09:06:55</dcterms:modified>
				<dcterms:issued rdf:datatype="http://www.w3.org/2001/XMLSchema#dateTime">2013-07-17T10:08:39</dcterms:issued>
				<skos:broader rdf:resource="http://purl.org/heritagedata/schemes/3/concepts/501938" />
				<skos:scopeNote xml:lang="en">A Motor Trawler with integral motor propulsion and built for stern-trawling, now the normal practice. Such vessels vary considerably in size, form and construction; larger examples may carry onboard refrigeration. The class thus grades into Motor Freezer Trawler.</skos:scopeNote>
			</skos:Concept>
		</skos:narrower>
		<skos:scopeNote xml:lang="en">A Fishing Vessel with integral motor propulsion and built for side- or stern-trawling, the latter practice now being prevalent. Such vessels vary considerably in size, form and construction; larger examples may carry onboard refrigeration.</skos:scopeNote>
	</skos:Concept>
	<skos:Concept rdf:about="http://purl.org/heritagedata/schemes/3/concepts/501939">
		<skos:inScheme rdf:resource="http://purl.org/heritagedata/schemes/3" />
		<dcterms:identifier>http://purl.org/heritagedata/schemes/3/concepts/501939</dcterms:identifier>
		<cc:license rdf:resource="http://reference.data.gov.uk/id/open-government-licence" />
		<cc:attributionURL rdf:resource="http://www.rcahms.gov.uk" />
		<cc:attributionName xml:lang="en">RCAHMS</cc:attributionName>
		<dcterms:publisher rdf:resource="http://www.rcahms.gov.uk" />
		<skos:prefLabel xml:lang="en">MOTOR VESSEL</skos:prefLabel>
		<dcterms:issued rdf:datatype="http://www.w3.org/2001/XMLSchema#dateTime">2013-07-17T10:08:39</dcterms:issued>
		<skos:narrower>
			<skos:Concept rdf:about="http://purl.org/heritagedata/schemes/3/concepts/501935">
				<skos:inScheme rdf:resource="http://purl.org/heritagedata/schemes/3" />
				<dcterms:identifier>http://purl.org/heritagedata/schemes/3/concepts/501935</dcterms:identifier>
				<cc:license rdf:resource="http://reference.data.gov.uk/id/open-government-licence" />
				<cc:attributionURL rdf:resource="http://www.rcahms.gov.uk" />
				<cc:attributionName xml:lang="en">RCAHMS</cc:attributionName>
				<dcterms:publisher rdf:resource="http://www.rcahms.gov.uk" />
				<skos:prefLabel xml:lang="en">MOTOR SHIP</skos:prefLabel>
				<dcterms:issued rdf:datatype="http://www.w3.org/2001/XMLSchema#dateTime">2013-07-17T10:08:39</dcterms:issued>
				<skos:broader rdf:resource="http://purl.org/heritagedata/schemes/3/concepts/501939" />
				<skos:scopeNote xml:lang="en">A medium-sized or large sea- or ocean-going vessel, with integral motor propulsion and used for a variety of purposes.</skos:scopeNote>
			</skos:Concept>
		</skos:narrower>
		<skos:broader rdf:resource="http://purl.org/heritagedata/schemes/3/concepts/501925" />
		<skos:scopeNote xml:lang="en">A medium-sized or large sea- or ocean-going vessel, with integral motor propulsion and used for a variety of purposes.</skos:scopeNote>
	</skos:Concept>
	<skos:Concept rdf:about="http://purl.org/heritagedata/schemes/3/concepts/501956">
		<skos:inScheme rdf:resource="http://purl.org/heritagedata/schemes/3" />
		<dcterms:identifier>http://purl.org/heritagedata/schemes/3/concepts/501956</dcterms:identifier>
		<cc:license rdf:resource="http://reference.data.gov.uk/id/open-government-licence" />
		<cc:attributionURL rdf:resource="http://www.rcahms.gov.uk" />
		<cc:attributionName xml:lang="en">RCAHMS</cc:attributionName>
		<dcterms:publisher rdf:resource="http://www.rcahms.gov.uk" />
		<skos:prefLabel xml:lang="en">RECREATIONAL VESSEL</skos:prefLabel>
		<dcterms:modified rdf:datatype="http://www.w3.org/2001/XMLSchema#dateTime">2007-04-24T12:11:36</dcterms:modified>
		<dcterms:issued rdf:datatype="http://www.w3.org/2001/XMLSchema#dateTime">2013-07-17T10:08:39</dcterms:issued>
		<skos:broader rdf:resource="http://purl.org/heritagedata/schemes/3/concepts/501925" />
		<skos:narrower rdf:resource="http://purl.org/heritagedata/schemes/3/concepts/502018" />
		<skos:scopeNote xml:lang="en">Any vessel constructed or used for recreational, leisure, pleasure or avocational purposes. Such vessels may be of considerable size and status, and may be of specialised form and construction. Motor Yachts, Steam Yachts and Yachts fall within this category.</skos:scopeNote>
	</skos:Concept>
	<skos:Concept rdf:about="http://purl.org/heritagedata/schemes/3/concepts/501841">
		<skos:inScheme rdf:resource="http://purl.org/heritagedata/schemes/3" />
		<dcterms:identifier>http://purl.org/heritagedata/schemes/3/concepts/501841</dcterms:identifier>
		<cc:license rdf:resource="http://reference.data.gov.uk/id/open-government-licence" />
		<cc:attributionURL rdf:resource="http://www.rcahms.gov.uk" />
		<cc:attributionName xml:lang="en">RCAHMS</cc:attributionName>
		<dcterms:publisher rdf:resource="http://www.rcahms.gov.uk" />
		<skos:prefLabel xml:lang="en">BARGE</skos:prefLabel>
		<dcterms:issued rdf:datatype="http://www.w3.org/2001/XMLSchema#dateTime">2013-07-17T10:08:39</dcterms:issued>
		<skos:broader rdf:resource="http://purl.org/heritagedata/schemes/3/concepts/501857" />
		<skos:narrower rdf:resource="http://purl.org/heritagedata/schemes/3/concepts/501846" />
		<skos:narrower>
			<skos:Concept rdf:about="http://purl.org/heritagedata/schemes/3/concepts/501861">
				<skos:inScheme rdf:resource="http://purl.org/heritagedata/schemes/3" />
				<dcterms:identifier>http://purl.org/heritagedata/schemes/3/concepts/501861</dcterms:identifier>
				<cc:license rdf:resource="http://reference.data.gov.uk/id/open-government-licence" />
				<cc:attributionURL rdf:resource="http://www.rcahms.gov.uk" />
				<cc:attributionName xml:lang="en">RCAHMS</cc:attributionName>
				<dcterms:publisher rdf:resource="http://www.rcahms.gov.uk" />
				<skos:prefLabel xml:lang="en">CONCRETE BARGE</skos:prefLabel>
				<dcterms:issued rdf:datatype="http://www.w3.org/2001/XMLSchema#dateTime">2013-07-17T10:08:39</dcterms:issued>
				<skos:broader rdf:resource="http://purl.org/heritagedata/schemes/3/concepts/501841" />
				<skos:scopeNote xml:lang="en">A Barge of concrete construction. This variant of the type was probably uncommon.</skos:scopeNote>
			</skos:Concept>
		</skos:narrower>
		<skos:narrower>
			<skos:Concept rdf:about="http://purl.org/heritagedata/schemes/3/concepts/501874">
				<skos:inScheme rdf:resource="http://purl.org/heritagedata/schemes/3" />
				<dcterms:identifier>http://purl.org/heritagedata/schemes/3/concepts/501874</dcterms:identifier>
				<cc:license rdf:resource="http://reference.data.gov.uk/id/open-government-licence" />
				<cc:attributionURL rdf:resource="http://www.rcahms.gov.uk" />
				<cc:attributionName xml:lang="en">RCAHMS</cc:attributionName>
				<dcterms:publisher rdf:resource="http://www.rcahms.gov.uk" />
				<skos:prefLabel xml:lang="en">DUMB BARGE</skos:prefLabel>
				<dcterms:issued rdf:datatype="http://www.w3.org/2001/XMLSchema#dateTime">2013-07-17T10:08:39</dcterms:issued>
				<skos:broader rdf:resource="http://purl.org/heritagedata/schemes/3/concepts/501841" />
				<skos:scopeNote xml:lang="en">A Barge without integral means of propulsion other than sweeps or oars. This variant of the type was probably the norm, being towed as required.</skos:scopeNote>
			</skos:Concept>
		</skos:narrower>
		<skos:narrower>
			<skos:Concept rdf:about="http://purl.org/heritagedata/schemes/3/concepts/501875">
				<skos:inScheme rdf:resource="http://purl.org/heritagedata/schemes/3" />
				<dcterms:identifier>http://purl.org/heritagedata/schemes/3/concepts/501875</dcterms:identifier>
				<cc:license rdf:resource="http://reference.data.gov.uk/id/open-government-licence" />
				<cc:attributionURL rdf:resource="http://www.rcahms.gov.uk" />
				<cc:attributionName xml:lang="en">RCAHMS</cc:attributionName>
				<dcterms:publisher rdf:resource="http://www.rcahms.gov.uk" />
				<skos:prefLabel xml:lang="en">DUMB CONCRETE BARGE</skos:prefLabel>
				<dcterms:issued rdf:datatype="http://www.w3.org/2001/XMLSchema#dateTime">2013-07-17T10:08:39</dcterms:issued>
				<skos:broader rdf:resource="http://purl.org/heritagedata/schemes/3/concepts/501841" />
				<skos:scopeNote xml:lang="en">A Barge of concrete construction and without integral means of propulsion other than sweeps or oars. This variant of the type was probably uncommon.</skos:scopeNote>
			</skos:Concept>
		</skos:narrower>
		<skos:narrower>
			<skos:Concept rdf:about="http://purl.org/heritagedata/schemes/3/concepts/501877">
				<skos:inScheme rdf:resource="http://purl.org/heritagedata/schemes/3" />
				<dcterms:identifier>http://purl.org/heritagedata/schemes/3/concepts/501877</dcterms:identifier>
				<cc:license rdf:resource="http://reference.data.gov.uk/id/open-government-licence" />
				<cc:attributionURL rdf:resource="http://www.rcahms.gov.uk" />
				<cc:attributionName xml:lang="en">RCAHMS</cc:attributionName>
				<dcterms:publisher rdf:resource="http://www.rcahms.gov.uk" />
				<skos:prefLabel xml:lang="en">DUMB HOPPER BARGE</skos:prefLabel>
				<dcterms:issued rdf:datatype="http://www.w3.org/2001/XMLSchema#dateTime">2013-07-17T10:08:39</dcterms:issued>
				<skos:broader rdf:resource="http://purl.org/heritagedata/schemes/3/concepts/501841" />
				<skos:scopeNote xml:lang="en">A Barge without integral means of propulsion other than sweeps or oars, and fitted to self-discharge through large doors in the bottom. This variant of the type was probably uncommon, and typically used to carry dredging spoil to the dumping ground.</skos:scopeNote>
			</skos:Concept>
		</skos:narrower>
		<skos:narrower>
			<skos:Concept rdf:about="http://purl.org/heritagedata/schemes/3/concepts/501903">
				<skos:inScheme rdf:resource="http://purl.org/heritagedata/schemes/3" />
				<dcterms:identifier>http://purl.org/heritagedata/schemes/3/concepts/501903</dcterms:identifier>
				<cc:license rdf:resource="http://reference.data.gov.uk/id/open-government-licence" />
				<cc:attributionURL rdf:resource="http://www.rcahms.gov.uk" />
				<cc:attributionName xml:lang="en">RCAHMS</cc:attributionName>
				<dcterms:publisher rdf:resource="http://www.rcahms.gov.uk" />
				<skos:prefLabel xml:lang="en">HOPPER BARGE</skos:prefLabel>
				<dcterms:issued rdf:datatype="http://www.w3.org/2001/XMLSchema#dateTime">2013-07-17T10:08:39</dcterms:issued>
				<skos:altLabel xml:lang="en">HOPPER</skos:altLabel>
				<skos:broader rdf:resource="http://purl.org/heritagedata/schemes/3/concepts/501841" />
				<skos:scopeNote xml:lang="en">A Barge fitted to self-discharge through large doors in the bottom. This variant of the type was probably uncommon, and typically used to carry dredging spoil to the dumping ground. Such vessels may be either powered or dumb.</skos:scopeNote>
			</skos:Concept>
		</skos:narrower>
		<skos:narrower>
			<skos:Concept rdf:about="http://purl.org/heritagedata/schemes/3/concepts/501929">
				<skos:inScheme rdf:resource="http://purl.org/heritagedata/schemes/3" />
				<dcterms:identifier>http://purl.org/heritagedata/schemes/3/concepts/501929</dcterms:identifier>
				<cc:license rdf:resource="http://reference.data.gov.uk/id/open-government-licence" />
				<cc:attributionURL rdf:resource="http://www.rcahms.gov.uk" />
				<cc:attributionName xml:lang="en">RCAHMS</cc:attributionName>
				<dcterms:publisher rdf:resource="http://www.rcahms.gov.uk" />
				<skos:prefLabel xml:lang="en">MOTOR BARGE</skos:prefLabel>
				<dcterms:issued rdf:datatype="http://www.w3.org/2001/XMLSchema#dateTime">2013-07-17T10:08:39</dcterms:issued>
				<skos:broader rdf:resource="http://purl.org/heritagedata/schemes/3/concepts/501841" />
				<skos:scopeNote xml:lang="en">A Barge with integral motor propulsion. This variant of the type was probably uncommon.</skos:scopeNote>
			</skos:Concept>
		</skos:narrower>
		<skos:narrower>
			<skos:Concept rdf:about="http://purl.org/heritagedata/schemes/3/concepts/502198">
				<skos:inScheme rdf:resource="http://purl.org/heritagedata/schemes/3" />
				<dcterms:identifier>http://purl.org/heritagedata/schemes/3/concepts/502198</dcterms:identifier>
				<cc:license rdf:resource="http://reference.data.gov.uk/id/open-government-licence" />
				<cc:attributionURL rdf:resource="http://www.rcahms.gov.uk" />
				<cc:attributionName xml:lang="en">RCAHMS</cc:attributionName>
				<dcterms:publisher rdf:resource="http://www.rcahms.gov.uk" />
				<skos:prefLabel xml:lang="en">TANK BARGE</skos:prefLabel>
				<dcterms:created rdf:datatype="http://www.w3.org/2001/XMLSchema#dateTime">2007-05-16T14:13:59</dcterms:created>
				<dcterms:modified rdf:datatype="http://www.w3.org/2001/XMLSchema#dateTime">2007-05-16T14:14:02</dcterms:modified>
				<dcterms:issued rdf:datatype="http://www.w3.org/2001/XMLSchema#dateTime">2013-07-17T10:08:39</dcterms:issued>
				<skos:broader rdf:resource="http://purl.org/heritagedata/schemes/3/concepts/501841" />
				<skos:scopeNote xml:lang="en">a dumb vessel, of iron or steel construction and box-like form, specialised for the bulk carriage of liquids (most commonly hydrocarbon fuels) in sheltered waters (including canals).</skos:scopeNote>
			</skos:Concept>
		</skos:narrower>
		<skos:narrower>
			<skos:Concept rdf:about="http://purl.org/heritagedata/schemes/3/concepts/502262">
				<skos:inScheme rdf:resource="http://purl.org/heritagedata/schemes/3" />
				<dcterms:identifier>http://purl.org/heritagedata/schemes/3/concepts/502262</dcterms:identifier>
				<cc:license rdf:resource="http://reference.data.gov.uk/id/open-government-licence" />
				<cc:attributionURL rdf:resource="http://www.rcahms.gov.uk" />
				<cc:attributionName xml:lang="en">RCAHMS</cc:attributionName>
				<dcterms:publisher rdf:resource="http://www.rcahms.gov.uk" />
				<skos:prefLabel xml:lang="en">CRANE BARGE</skos:prefLabel>
				<dcterms:created rdf:datatype="http://www.w3.org/2001/XMLSchema#dateTime">2007-05-18T15:27:41</dcterms:created>
				<dcterms:modified rdf:datatype="http://www.w3.org/2001/XMLSchema#dateTime">2007-05-18T15:27:46</dcterms:modified>
				<dcterms:issued rdf:datatype="http://www.w3.org/2001/XMLSchema#dateTime">2013-07-17T10:08:39</dcterms:issued>
				<skos:broader rdf:resource="http://purl.org/heritagedata/schemes/3/concepts/501841" />
				<skos:scopeNote xml:lang="en">A shallow draft vessel used to carry a crane.</skos:scopeNote>
			</skos:Concept>
		</skos:narrower>
		<skos:scopeNote xml:lang="en">Shallow draft cargo vessel, often broad beamed and flat bottomed, powered by engine and or sail.</skos:scopeNote>
	</skos:Concept>
	<skos:Concept rdf:about="http://purl.org/heritagedata/schemes/3/concepts/501842">
		<skos:inScheme rdf:resource="http://purl.org/heritagedata/schemes/3" />
		<dcterms:identifier>http://purl.org/heritagedata/schemes/3/concepts/501842</dcterms:identifier>
		<cc:license rdf:resource="http://reference.data.gov.uk/id/open-government-licence" />
		<cc:attributionURL rdf:resource="http://www.rcahms.gov.uk" />
		<cc:attributionName xml:lang="en">RCAHMS</cc:attributionName>
		<dcterms:publisher rdf:resource="http://www.rcahms.gov.uk" />
		<skos:prefLabel xml:lang="en">BARQUE</skos:prefLabel>
		<dcterms:modified rdf:datatype="http://www.w3.org/2001/XMLSchema#dateTime">2007-04-24T12:14:59</dcterms:modified>
		<dcterms:issued rdf:datatype="http://www.w3.org/2001/XMLSchema#dateTime">2013-07-17T10:08:39</dcterms:issued>
		<skos:altLabel xml:lang="en">BARK</skos:altLabel>
		<skos:narrower>
			<skos:Concept rdf:about="http://purl.org/heritagedata/schemes/3/concepts/501830">
				<skos:inScheme rdf:resource="http://purl.org/heritagedata/schemes/3" />
				<dcterms:identifier>http://purl.org/heritagedata/schemes/3/concepts/501830</dcterms:identifier>
				<cc:license rdf:resource="http://reference.data.gov.uk/id/open-government-licence" />
				<cc:attributionURL rdf:resource="http://www.rcahms.gov.uk" />
				<cc:attributionName xml:lang="en">RCAHMS</cc:attributionName>
				<dcterms:publisher rdf:resource="http://www.rcahms.gov.uk" />
				<skos:prefLabel xml:lang="en">AUXILIARY BARQUE</skos:prefLabel>
				<dcterms:issued rdf:datatype="http://www.w3.org/2001/XMLSchema#dateTime">2013-07-17T10:08:39</dcterms:issued>
				<skos:broader rdf:resource="http://purl.org/heritagedata/schemes/3/concepts/501842" />
				<skos:scopeNote xml:lang="en">Variant of the Barque having auxiliary steam or diesel propulsion for use in light airs or contrary winds.</skos:scopeNote>
			</skos:Concept>
		</skos:narrower>
		<skos:broader rdf:resource="http://purl.org/heritagedata/schemes/3/concepts/501987" />
		<skos:scopeNote xml:lang="en">A large decked sailing vessel having three or more masts, with square sails on all but the mizzen, which was fore-and-aft rigged. Vessels of this type and of steel construction were the norm in ocean trading in the latter days of sail. Most of the Cape Horners, windjammers and clipper ships fall within this category.</skos:scopeNote>
	</skos:Concept>
	<skos:Concept rdf:about="http://purl.org/heritagedata/schemes/3/concepts/501863">
		<skos:inScheme rdf:resource="http://purl.org/heritagedata/schemes/3" />
		<dcterms:identifier>http://purl.org/heritagedata/schemes/3/concepts/501863</dcterms:identifier>
		<cc:license rdf:resource="http://reference.data.gov.uk/id/open-government-licence" />
		<cc:attributionURL rdf:resource="http://www.rcahms.gov.uk" />
		<cc:attributionName xml:lang="en">RCAHMS</cc:attributionName>
		<dcterms:publisher rdf:resource="http://www.rcahms.gov.uk" />
		<skos:prefLabel xml:lang="en">CRAFT</skos:prefLabel>
		<dcterms:issued rdf:datatype="http://www.w3.org/2001/XMLSchema#dateTime">2013-07-17T10:08:39</dcterms:issued>
		<skos:narrower>
			<skos:Concept rdf:about="http://purl.org/heritagedata/schemes/3/concepts/501859">
				<skos:inScheme rdf:resource="http://purl.org/heritagedata/schemes/3" />
				<dcterms:identifier>http://purl.org/heritagedata/schemes/3/concepts/501859</dcterms:identifier>
				<cc:license rdf:resource="http://reference.data.gov.uk/id/open-government-licence" />
				<cc:attributionURL rdf:resource="http://www.rcahms.gov.uk" />
				<cc:attributionName xml:lang="en">RCAHMS</cc:attributionName>
				<dcterms:publisher rdf:resource="http://www.rcahms.gov.uk" />
				<skos:prefLabel xml:lang="en">COBLE</skos:prefLabel>
				<dcterms:issued rdf:datatype="http://www.w3.org/2001/XMLSchema#dateTime">2013-07-17T10:08:39</dcterms:issued>
				<skos:broader rdf:resource="http://purl.org/heritagedata/schemes/3/concepts/501863" />
				<skos:scopeNote xml:lang="en">This term applies to two types of coastal or estuarine craft used (notably for salmon netting) in coastal and estuarine contexts in Eastern Scotland. The heavier-built is of North-East English origin, and is distinguished by an undercut transom intended for beaching in surf. The type found further North is of lighter construction and has a vertical transom stern. Both types may be rowed or sailed, and are traditionally clinker-built, but are nowadays formed in fibreglass.</skos:scopeNote>
			</skos:Concept>
		</skos:narrower>
		<skos:broader rdf:resource="http://purl.org/heritagedata/schemes/3/concepts/501925" />
		<skos:narrower>
			<skos:Concept rdf:about="http://purl.org/heritagedata/schemes/3/concepts/501923">
				<skos:inScheme rdf:resource="http://purl.org/heritagedata/schemes/3" />
				<dcterms:identifier>http://purl.org/heritagedata/schemes/3/concepts/501923</dcterms:identifier>
				<cc:license rdf:resource="http://reference.data.gov.uk/id/open-government-licence" />
				<cc:attributionURL rdf:resource="http://www.rcahms.gov.uk" />
				<cc:attributionName xml:lang="en">RCAHMS</cc:attributionName>
				<dcterms:publisher rdf:resource="http://www.rcahms.gov.uk" />
				<skos:prefLabel xml:lang="en">LOGBOAT</skos:prefLabel>
				<dcterms:issued rdf:datatype="http://www.w3.org/2001/XMLSchema#dateTime">2013-07-17T10:08:39</dcterms:issued>
				<skos:broader rdf:resource="http://purl.org/heritagedata/schemes/3/concepts/501863" />
				<skos:scopeNote xml:lang="en">A boat fashioned out of a section of tree trunk.</skos:scopeNote>
			</skos:Concept>
		</skos:narrower>
		<skos:scopeNote xml:lang="en">This term (which may be either singular or plural) applies within RCAHMS terminology to any vessel (demonstrable or suggested) which cannot be classified more  accurately.</skos:scopeNote>
	</skos:Concept>
	<skos:Concept rdf:about="http://purl.org/heritagedata/schemes/3/concepts/501865">
		<skos:inScheme rdf:resource="http://purl.org/heritagedata/schemes/3" />
		<dcterms:identifier>http://purl.org/heritagedata/schemes/3/concepts/501865</dcterms:identifier>
		<cc:license rdf:resource="http://reference.data.gov.uk/id/open-government-licence" />
		<cc:attributionURL rdf:resource="http://www.rcahms.gov.uk" />
		<cc:attributionName xml:lang="en">RCAHMS</cc:attributionName>
		<dcterms:publisher rdf:resource="http://www.rcahms.gov.uk" />
		<skos:prefLabel xml:lang="en">CUSTOMS BOAT</skos:prefLabel>
		<dcterms:issued rdf:datatype="http://www.w3.org/2001/XMLSchema#dateTime">2013-07-17T10:08:39</dcterms:issued>
		<skos:broader rdf:resource="http://purl.org/heritagedata/schemes/3/concepts/501925" />
		<skos:narrower>
			<skos:Concept rdf:about="http://purl.org/heritagedata/schemes/3/concepts/501967">
				<skos:inScheme rdf:resource="http://purl.org/heritagedata/schemes/3" />
				<dcterms:identifier>http://purl.org/heritagedata/schemes/3/concepts/501967</dcterms:identifier>
				<cc:license rdf:resource="http://reference.data.gov.uk/id/open-government-licence" />
				<cc:attributionURL rdf:resource="http://www.rcahms.gov.uk" />
				<cc:attributionName xml:lang="en">RCAHMS</cc:attributionName>
				<dcterms:publisher rdf:resource="http://www.rcahms.gov.uk" />
				<skos:prefLabel xml:lang="en">REVENUE CUTTER</skos:prefLabel>
				<dcterms:modified rdf:datatype="http://www.w3.org/2001/XMLSchema#dateTime">2011-08-19T09:40:19</dcterms:modified>
				<dcterms:issued rdf:datatype="http://www.w3.org/2001/XMLSchema#dateTime">2013-07-17T10:08:39</dcterms:issued>
				<skos:broader rdf:resource="http://purl.org/heritagedata/schemes/3/concepts/501865" />
				<skos:scopeNote xml:lang="en">A single masted cutter built specifically for the prevention of smuggling and the enforcement of customs regulations. In practice, the term was also applied to vessels in revenue service not rigged as cutters.</skos:scopeNote>
			</skos:Concept>
		</skos:narrower>
		<skos:scopeNote xml:lang="en">A small vessel used as transport for customs officers.</skos:scopeNote>
	</skos:Concept>
	<skos:Concept rdf:about="http://purl.org/heritagedata/schemes/3/concepts/501872">
		<skos:inScheme rdf:resource="http://purl.org/heritagedata/schemes/3" />
		<dcterms:identifier>http://purl.org/heritagedata/schemes/3/concepts/501872</dcterms:identifier>
		<cc:license rdf:resource="http://reference.data.gov.uk/id/open-government-licence" />
		<cc:attributionURL rdf:resource="http://www.rcahms.gov.uk" />
		<cc:attributionName xml:lang="en">RCAHMS</cc:attributionName>
		<dcterms:publisher rdf:resource="http://www.rcahms.gov.uk" />
		<skos:prefLabel xml:lang="en">DREDGER</skos:prefLabel>
		<dcterms:issued rdf:datatype="http://www.w3.org/2001/XMLSchema#dateTime">2013-07-17T10:08:39</dcterms:issued>
		<skos:narrower>
			<skos:Concept rdf:about="http://purl.org/heritagedata/schemes/3/concepts/501852">
				<skos:inScheme rdf:resource="http://purl.org/heritagedata/schemes/3" />
				<dcterms:identifier>http://purl.org/heritagedata/schemes/3/concepts/501852</dcterms:identifier>
				<cc:license rdf:resource="http://reference.data.gov.uk/id/open-government-licence" />
				<cc:attributionURL rdf:resource="http://www.rcahms.gov.uk" />
				<cc:attributionName xml:lang="en">RCAHMS</cc:attributionName>
				<dcterms:publisher rdf:resource="http://www.rcahms.gov.uk" />
				<skos:prefLabel xml:lang="en">BUCKET DREDGER</skos:prefLabel>
				<dcterms:issued rdf:datatype="http://www.w3.org/2001/XMLSchema#dateTime">2013-07-17T10:08:39</dcterms:issued>
				<skos:broader rdf:resource="http://purl.org/heritagedata/schemes/3/concepts/501872" />
				<skos:scopeNote xml:lang="en">This refers to a variant of the Dredger intended to excavate sediment by the use of an endless chain of buckets. Such vessels are generally of considerable size.</skos:scopeNote>
			</skos:Concept>
		</skos:narrower>
		<skos:broader rdf:resource="http://purl.org/heritagedata/schemes/3/concepts/501925" />
		<skos:narrower>
			<skos:Concept rdf:about="http://purl.org/heritagedata/schemes/3/concepts/501876">
				<skos:inScheme rdf:resource="http://purl.org/heritagedata/schemes/3" />
				<dcterms:identifier>http://purl.org/heritagedata/schemes/3/concepts/501876</dcterms:identifier>
				<cc:license rdf:resource="http://reference.data.gov.uk/id/open-government-licence" />
				<cc:attributionURL rdf:resource="http://www.rcahms.gov.uk" />
				<cc:attributionName xml:lang="en">RCAHMS</cc:attributionName>
				<dcterms:publisher rdf:resource="http://www.rcahms.gov.uk" />
				<skos:prefLabel xml:lang="en">DUMB DREDGER</skos:prefLabel>
				<dcterms:issued rdf:datatype="http://www.w3.org/2001/XMLSchema#dateTime">2013-07-17T10:08:39</dcterms:issued>
				<skos:broader rdf:resource="http://purl.org/heritagedata/schemes/3/concepts/501872" />
				<skos:scopeNote xml:lang="en">This refers to a variant of the Dredger without integral propulsion. Any of a number of methods of excavation may be employed, and some vessels of this type are known to have been driven by manpower and moved from traction engines on shore.</skos:scopeNote>
			</skos:Concept>
		</skos:narrower>
		<skos:narrower>
			<skos:Concept rdf:about="http://purl.org/heritagedata/schemes/3/concepts/501897">
				<skos:inScheme rdf:resource="http://purl.org/heritagedata/schemes/3" />
				<dcterms:identifier>http://purl.org/heritagedata/schemes/3/concepts/501897</dcterms:identifier>
				<cc:license rdf:resource="http://reference.data.gov.uk/id/open-government-licence" />
				<cc:attributionURL rdf:resource="http://www.rcahms.gov.uk" />
				<cc:attributionName xml:lang="en">RCAHMS</cc:attributionName>
				<dcterms:publisher rdf:resource="http://www.rcahms.gov.uk" />
				<skos:prefLabel xml:lang="en">GRAB DREDGER</skos:prefLabel>
				<dcterms:modified rdf:datatype="http://www.w3.org/2001/XMLSchema#dateTime">2007-04-24T11:54:53</dcterms:modified>
				<dcterms:issued rdf:datatype="http://www.w3.org/2001/XMLSchema#dateTime">2013-07-17T10:08:39</dcterms:issued>
				<skos:broader rdf:resource="http://purl.org/heritagedata/schemes/3/concepts/501872" />
				<skos:scopeNote xml:lang="en">this refers to a variant of the Dredger intended to excavate sediment by the use of a grab mounted on board. Such vessels are generally of smaller size that Bucket Dredgers or Suction Dredgers. Most Steam Dredgers probably fall within this category.</skos:scopeNote>
			</skos:Concept>
		</skos:narrower>
		<skos:narrower>
			<skos:Concept rdf:about="http://purl.org/heritagedata/schemes/3/concepts/501904">
				<skos:inScheme rdf:resource="http://purl.org/heritagedata/schemes/3" />
				<dcterms:identifier>http://purl.org/heritagedata/schemes/3/concepts/501904</dcterms:identifier>
				<cc:license rdf:resource="http://reference.data.gov.uk/id/open-government-licence" />
				<cc:attributionURL rdf:resource="http://www.rcahms.gov.uk" />
				<cc:attributionName xml:lang="en">RCAHMS</cc:attributionName>
				<dcterms:publisher rdf:resource="http://www.rcahms.gov.uk" />
				<skos:prefLabel xml:lang="en">HOPPER DREDGER</skos:prefLabel>
				<dcterms:issued rdf:datatype="http://www.w3.org/2001/XMLSchema#dateTime">2013-07-17T10:08:39</dcterms:issued>
				<skos:broader rdf:resource="http://purl.org/heritagedata/schemes/3/concepts/501872" />
				<skos:scopeNote xml:lang="en">This refers to a specialised form of service or yard craft constructed for the underwater excavation of soft sediment to maintain a specified channel depth for the passage of shipping, and built around an integral hopper or hoppers to contain material being taken for dumping.</skos:scopeNote>
			</skos:Concept>
		</skos:narrower>
		<skos:narrower>
			<skos:Concept rdf:about="http://purl.org/heritagedata/schemes/3/concepts/501988">
				<skos:inScheme rdf:resource="http://purl.org/heritagedata/schemes/3" />
				<dcterms:identifier>http://purl.org/heritagedata/schemes/3/concepts/501988</dcterms:identifier>
				<cc:license rdf:resource="http://reference.data.gov.uk/id/open-government-licence" />
				<cc:attributionURL rdf:resource="http://www.rcahms.gov.uk" />
				<cc:attributionName xml:lang="en">RCAHMS</cc:attributionName>
				<dcterms:publisher rdf:resource="http://www.rcahms.gov.uk" />
				<skos:prefLabel xml:lang="en">STEAM DREDGER</skos:prefLabel>
				<dcterms:issued rdf:datatype="http://www.w3.org/2001/XMLSchema#dateTime">2013-07-17T10:08:39</dcterms:issued>
				<skos:broader rdf:resource="http://purl.org/heritagedata/schemes/3/concepts/501872" />
				<skos:scopeNote xml:lang="en">Dredger powered by an integral steam engine. Although not specifically stated, vessels within this category were probably Grab Dredgers.</skos:scopeNote>
			</skos:Concept>
		</skos:narrower>
		<skos:narrower>
			<skos:Concept rdf:about="http://purl.org/heritagedata/schemes/3/concepts/502003">
				<skos:inScheme rdf:resource="http://purl.org/heritagedata/schemes/3" />
				<dcterms:identifier>http://purl.org/heritagedata/schemes/3/concepts/502003</dcterms:identifier>
				<cc:license rdf:resource="http://reference.data.gov.uk/id/open-government-licence" />
				<cc:attributionURL rdf:resource="http://www.rcahms.gov.uk" />
				<cc:attributionName xml:lang="en">RCAHMS</cc:attributionName>
				<dcterms:publisher rdf:resource="http://www.rcahms.gov.uk" />
				<skos:prefLabel xml:lang="en">SUCTION DREDGER</skos:prefLabel>
				<dcterms:issued rdf:datatype="http://www.w3.org/2001/XMLSchema#dateTime">2013-07-17T10:08:39</dcterms:issued>
				<skos:broader rdf:resource="http://purl.org/heritagedata/schemes/3/concepts/501872" />
				<skos:scopeNote xml:lang="en">This refers to a variant of the Dredger intended to excavate sediment by the use of suction pipes mounted down the sides. Such vessels are generally of considerable size.</skos:scopeNote>
			</skos:Concept>
		</skos:narrower>
		<skos:scopeNote xml:lang="en">This refers to a specialised form of service or yard craft constructed for the underwater excavation of soft sediment to maintain a specified channel depth for the passage of shipping. Various methods of excavation are employed, and some dredgers have integral hoppers to contain material being taken for dumping, while others require the associated use of a Hopper Barge.</skos:scopeNote>
	</skos:Concept>
	<skos:Concept rdf:about="http://purl.org/heritagedata/schemes/3/concepts/501873">
		<skos:inScheme rdf:resource="http://purl.org/heritagedata/schemes/3" />
		<dcterms:identifier>http://purl.org/heritagedata/schemes/3/concepts/501873</dcterms:identifier>
		<cc:license rdf:resource="http://reference.data.gov.uk/id/open-government-licence" />
		<cc:attributionURL rdf:resource="http://www.rcahms.gov.uk" />
		<cc:attributionName xml:lang="en">RCAHMS</cc:attributionName>
		<dcterms:publisher rdf:resource="http://www.rcahms.gov.uk" />
		<skos:prefLabel xml:lang="en">DRIFTER</skos:prefLabel>
		<dcterms:issued rdf:datatype="http://www.w3.org/2001/XMLSchema#dateTime">2013-07-17T10:08:39</dcterms:issued>
		<skos:broader rdf:resource="http://purl.org/heritagedata/schemes/3/concepts/501889" />
		<skos:narrower rdf:resource="http://purl.org/heritagedata/schemes/3/concepts/501931" />
		<skos:narrower>
			<skos:Concept rdf:about="http://purl.org/heritagedata/schemes/3/concepts/501957">
				<skos:inScheme rdf:resource="http://purl.org/heritagedata/schemes/3" />
				<dcterms:identifier>http://purl.org/heritagedata/schemes/3/concepts/501957</dcterms:identifier>
				<cc:license rdf:resource="http://reference.data.gov.uk/id/open-government-licence" />
				<cc:attributionURL rdf:resource="http://www.rcahms.gov.uk" />
				<cc:attributionName xml:lang="en">RCAHMS</cc:attributionName>
				<dcterms:publisher rdf:resource="http://www.rcahms.gov.uk" />
				<skos:prefLabel xml:lang="en">REQUISITIONED DRIFTER</skos:prefLabel>
				<dcterms:issued rdf:datatype="http://www.w3.org/2001/XMLSchema#dateTime">2013-07-17T10:08:39</dcterms:issued>
				<skos:broader rdf:resource="http://purl.org/heritagedata/schemes/3/concepts/501873" />
				<skos:scopeNote xml:lang="en">A Drifter which has been requisitioned for war service, generally within its local area, with an unchanged crew and with the fitting of only basic armament (if any). Such vessels were used for transport and target-towing as well as patrol purposes.</skos:scopeNote>
			</skos:Concept>
		</skos:narrower>
		<skos:narrower rdf:resource="http://purl.org/heritagedata/schemes/3/concepts/501989" />
		<skos:scopeNote xml:lang="en">A fishing boat using nets which are free to move with the tides and currents.</skos:scopeNote>
	</skos:Concept>
	<skos:Concept rdf:about="http://purl.org/heritagedata/schemes/3/concepts/501880">
		<skos:inScheme rdf:resource="http://purl.org/heritagedata/schemes/3" />
		<dcterms:identifier>http://purl.org/heritagedata/schemes/3/concepts/501880</dcterms:identifier>
		<cc:license rdf:resource="http://reference.data.gov.uk/id/open-government-licence" />
		<cc:attributionURL rdf:resource="http://www.rcahms.gov.uk" />
		<cc:attributionName xml:lang="en">RCAHMS</cc:attributionName>
		<dcterms:publisher rdf:resource="http://www.rcahms.gov.uk" />
		<skos:prefLabel xml:lang="en">EAST INDIAMAN</skos:prefLabel>
		<dcterms:issued rdf:datatype="http://www.w3.org/2001/XMLSchema#dateTime">2013-07-17T10:08:39</dcterms:issued>
		<skos:narrower>
			<skos:Concept rdf:about="http://purl.org/heritagedata/schemes/3/concepts/501868">
				<skos:inScheme rdf:resource="http://purl.org/heritagedata/schemes/3" />
				<dcterms:identifier>http://purl.org/heritagedata/schemes/3/concepts/501868</dcterms:identifier>
				<cc:license rdf:resource="http://reference.data.gov.uk/id/open-government-licence" />
				<cc:attributionURL rdf:resource="http://www.rcahms.gov.uk" />
				<cc:attributionName xml:lang="en">RCAHMS</cc:attributionName>
				<dcterms:publisher rdf:resource="http://www.rcahms.gov.uk" />
				<skos:prefLabel xml:lang="en">DANISH EAST INDIAMAN</skos:prefLabel>
				<dcterms:issued rdf:datatype="http://www.w3.org/2001/XMLSchema#dateTime">2013-07-17T10:08:39</dcterms:issued>
				<skos:broader rdf:resource="http://purl.org/heritagedata/schemes/3/concepts/501880" />
				<skos:scopeNote xml:lang="en">an armed merchant vessel of Danish origin, equipped and used for the specialised Eastern trade, notably in spices, by the Danish East Indies Company between the 17th and 19th centuries. Vessels of this type were unusually large for the period and considered of extremely high status, this being reflected in their rich ornament.</skos:scopeNote>
			</skos:Concept>
		</skos:narrower>
		<skos:narrower>
			<skos:Concept rdf:about="http://purl.org/heritagedata/schemes/3/concepts/501878">
				<skos:inScheme rdf:resource="http://purl.org/heritagedata/schemes/3" />
				<dcterms:identifier>http://purl.org/heritagedata/schemes/3/concepts/501878</dcterms:identifier>
				<cc:license rdf:resource="http://reference.data.gov.uk/id/open-government-licence" />
				<cc:attributionURL rdf:resource="http://www.rcahms.gov.uk" />
				<cc:attributionName xml:lang="en">RCAHMS</cc:attributionName>
				<dcterms:publisher rdf:resource="http://www.rcahms.gov.uk" />
				<skos:prefLabel xml:lang="en">DUTCH EAST INDIAMAN</skos:prefLabel>
				<dcterms:issued rdf:datatype="http://www.w3.org/2001/XMLSchema#dateTime">2013-07-17T10:08:39</dcterms:issued>
				<skos:broader rdf:resource="http://purl.org/heritagedata/schemes/3/concepts/501880" />
				<skos:scopeNote xml:lang="en">An armed merchant vessel of Dutch origin, equipped and used for the specialised Eastern trade, notably in spices, by the Dutch East Indies Company (VOC) between the 17th and 19th centuries. Vessels of this type were unusually large for the period and considered of extremely high status, this being reflected in their rich ornament.</skos:scopeNote>
			</skos:Concept>
		</skos:narrower>
		<skos:broader rdf:resource="http://purl.org/heritagedata/schemes/3/concepts/501968" />
		<skos:narrower>
			<skos:Concept rdf:about="http://purl.org/heritagedata/schemes/3/concepts/502005">
				<skos:inScheme rdf:resource="http://purl.org/heritagedata/schemes/3" />
				<dcterms:identifier>http://purl.org/heritagedata/schemes/3/concepts/502005</dcterms:identifier>
				<cc:license rdf:resource="http://reference.data.gov.uk/id/open-government-licence" />
				<cc:attributionURL rdf:resource="http://www.rcahms.gov.uk" />
				<cc:attributionName xml:lang="en">RCAHMS</cc:attributionName>
				<dcterms:publisher rdf:resource="http://www.rcahms.gov.uk" />
				<skos:prefLabel xml:lang="en">SWEDISH EAST INDIAMAN</skos:prefLabel>
				<dcterms:issued rdf:datatype="http://www.w3.org/2001/XMLSchema#dateTime">2013-07-17T10:08:39</dcterms:issued>
				<skos:broader rdf:resource="http://purl.org/heritagedata/schemes/3/concepts/501880" />
				<skos:scopeNote xml:lang="en">An armed merchant vessel of Swedish origin, equipped and used for the specialised Eastern trade, notably in spices, by the Swedish East Indies Company between the 17th and 19th centuries. Vessels of this type were unusually large for the period and considered of extremely status, this being reflected in their rich ornament.</skos:scopeNote>
			</skos:Concept>
		</skos:narrower>
		<skos:scopeNote xml:lang="en">Name given to a vessel of the East India Company. Usually large, well built and magnificently decorated.</skos:scopeNote>
	</skos:Concept>
	<skos:Concept rdf:about="http://purl.org/heritagedata/schemes/3/concepts/501881">
		<skos:inScheme rdf:resource="http://purl.org/heritagedata/schemes/3" />
		<dcterms:identifier>http://purl.org/heritagedata/schemes/3/concepts/501881</dcterms:identifier>
		<cc:license rdf:resource="http://reference.data.gov.uk/id/open-government-licence" />
		<cc:attributionURL rdf:resource="http://www.rcahms.gov.uk" />
		<cc:attributionName xml:lang="en">RCAHMS</cc:attributionName>
		<dcterms:publisher rdf:resource="http://www.rcahms.gov.uk" />
		<skos:prefLabel xml:lang="en">ESCORT VESSEL</skos:prefLabel>
		<dcterms:issued rdf:datatype="http://www.w3.org/2001/XMLSchema#dateTime">2013-07-17T10:08:39</dcterms:issued>
		<skos:broader rdf:resource="http://purl.org/heritagedata/schemes/3/concepts/502015" />
		<skos:narrower>
			<skos:Concept rdf:about="http://purl.org/heritagedata/schemes/3/concepts/501893">
				<skos:inScheme rdf:resource="http://purl.org/heritagedata/schemes/3" />
				<dcterms:identifier>http://purl.org/heritagedata/schemes/3/concepts/501893</dcterms:identifier>
				<cc:license rdf:resource="http://reference.data.gov.uk/id/open-government-licence" />
				<cc:attributionURL rdf:resource="http://www.rcahms.gov.uk" />
				<cc:attributionName xml:lang="en">RCAHMS</cc:attributionName>
				<dcterms:publisher rdf:resource="http://www.rcahms.gov.uk" />
				<skos:prefLabel xml:lang="en">FRIGATE</skos:prefLabel>
				<dcterms:modified rdf:datatype="http://www.w3.org/2001/XMLSchema#dateTime">2007-04-24T14:37:41</dcterms:modified>
				<dcterms:issued rdf:datatype="http://www.w3.org/2001/XMLSchema#dateTime">2013-07-17T10:08:39</dcterms:issued>
				<skos:broader rdf:resource="http://purl.org/heritagedata/schemes/3/concepts/501881" />
				<skos:scopeNote xml:lang="en">A small- to medium-sized warship built around steam or gas turbine propulsion and carrying a range of weaponry, and carrying a helicopter for anti-submarine operations. Vessels of this type are now distinguished from Destroyers by not having a long-range (area defence) anti-aircraft missile system, Warships of this type have traditionally tended to operate as part of larger formations rather than independently, being similar to Destroyers in this respect.</skos:scopeNote>
			</skos:Concept>
		</skos:narrower>
		<skos:scopeNote xml:lang="en">A warship used to provide an escort to other warships or merchant ships against attack.</skos:scopeNote>
	</skos:Concept>
	<skos:Concept rdf:about="http://purl.org/heritagedata/schemes/3/concepts/501882">
		<skos:inScheme rdf:resource="http://purl.org/heritagedata/schemes/3" />
		<dcterms:identifier>http://purl.org/heritagedata/schemes/3/concepts/501882</dcterms:identifier>
		<cc:license rdf:resource="http://reference.data.gov.uk/id/open-government-licence" />
		<cc:attributionURL rdf:resource="http://www.rcahms.gov.uk" />
		<cc:attributionName xml:lang="en">RCAHMS</cc:attributionName>
		<dcterms:publisher rdf:resource="http://www.rcahms.gov.uk" />
		<skos:prefLabel xml:lang="en">FACTORY SHIP</skos:prefLabel>
		<dcterms:issued rdf:datatype="http://www.w3.org/2001/XMLSchema#dateTime">2013-07-17T10:08:39</dcterms:issued>
		<skos:broader rdf:resource="http://purl.org/heritagedata/schemes/3/concepts/501925" />
		<skos:narrower rdf:resource="http://purl.org/heritagedata/schemes/3/concepts/505281" />
		<skos:scopeNote xml:lang="en">A vessel with equipment for processing dead marine life whilst still at sea.</skos:scopeNote>
	</skos:Concept>
	<skos:Concept rdf:about="http://purl.org/heritagedata/schemes/3/concepts/501966">
		<skos:inScheme rdf:resource="http://purl.org/heritagedata/schemes/3" />
		<dcterms:identifier>http://purl.org/heritagedata/schemes/3/concepts/501966</dcterms:identifier>
		<cc:license rdf:resource="http://reference.data.gov.uk/id/open-government-licence" />
		<cc:attributionURL rdf:resource="http://www.rcahms.gov.uk" />
		<cc:attributionName xml:lang="en">RCAHMS</cc:attributionName>
		<dcterms:publisher rdf:resource="http://www.rcahms.gov.uk" />
		<skos:prefLabel xml:lang="en">RESCUE VESSEL</skos:prefLabel>
		<dcterms:issued rdf:datatype="http://www.w3.org/2001/XMLSchema#dateTime">2013-07-17T10:08:39</dcterms:issued>
		<skos:narrower>
			<skos:Concept rdf:about="http://purl.org/heritagedata/schemes/3/concepts/501826">
				<skos:inScheme rdf:resource="http://purl.org/heritagedata/schemes/3" />
				<dcterms:identifier>http://purl.org/heritagedata/schemes/3/concepts/501826</dcterms:identifier>
				<cc:license rdf:resource="http://reference.data.gov.uk/id/open-government-licence" />
				<cc:attributionURL rdf:resource="http://www.rcahms.gov.uk" />
				<cc:attributionName xml:lang="en">RCAHMS</cc:attributionName>
				<dcterms:publisher rdf:resource="http://www.rcahms.gov.uk" />
				<skos:prefLabel xml:lang="en">AIR SEA RESCUE BUOY</skos:prefLabel>
				<dcterms:issued rdf:datatype="http://www.w3.org/2001/XMLSchema#dateTime">2013-07-17T10:08:39</dcterms:issued>
				<skos:broader rdf:resource="http://purl.org/heritagedata/schemes/3/concepts/501966" />
				<skos:scopeNote xml:lang="en">An unpowered and unmanned vessel containing basic survival and communications facilities, and intended to be moored in a known position to provide a refuge for aircrew in distress after they ditched alongside it.</skos:scopeNote>
			</skos:Concept>
		</skos:narrower>
		<skos:narrower>
			<skos:Concept rdf:about="http://purl.org/heritagedata/schemes/3/concepts/501918">
				<skos:inScheme rdf:resource="http://purl.org/heritagedata/schemes/3" />
				<dcterms:identifier>http://purl.org/heritagedata/schemes/3/concepts/501918</dcterms:identifier>
				<cc:license rdf:resource="http://reference.data.gov.uk/id/open-government-licence" />
				<cc:attributionURL rdf:resource="http://www.rcahms.gov.uk" />
				<cc:attributionName xml:lang="en">RCAHMS</cc:attributionName>
				<dcterms:publisher rdf:resource="http://www.rcahms.gov.uk" />
				<skos:prefLabel xml:lang="en">LIFEBOAT</skos:prefLabel>
				<dcterms:issued rdf:datatype="http://www.w3.org/2001/XMLSchema#dateTime">2013-07-17T10:08:39</dcterms:issued>
				<skos:broader rdf:resource="http://purl.org/heritagedata/schemes/3/concepts/501966" />
				<skos:scopeNote xml:lang="en">A specialised form of vessel, typically of small size, intended for the saving of life at sea. The term covers both vessels mounted on a parent vessel to save the lives of those on boar in the event of sinking, and also vessels maintained in readiness (either in harbour or on shore) to save lives in emergency. 
Vessels of both sub-types are specialised for seaworthiness, being fitted on occasion with self-righting gear, and low in silhouette. Although originally rowed, powerful diesel engines have long been universal.
Most of the RCAHMS entries fall within the latter category. The smaller boats of the former category frequently remain in service long after improvised conversion for other purposes.</skos:scopeNote>
			</skos:Concept>
		</skos:narrower>
		<skos:broader rdf:resource="http://purl.org/heritagedata/schemes/3/concepts/501977" />
		<skos:scopeNote xml:lang="en">A specially equipped small merchant ship used during World War II to care for survivors of torpedoed ships in convoys.</skos:scopeNote>
	</skos:Concept>
	<skos:Concept rdf:about="http://purl.org/heritagedata/schemes/3/concepts/501968">
		<skos:inScheme rdf:resource="http://purl.org/heritagedata/schemes/3" />
		<dcterms:identifier>http://purl.org/heritagedata/schemes/3/concepts/501968</dcterms:identifier>
		<cc:license rdf:resource="http://reference.data.gov.uk/id/open-government-licence" />
		<cc:attributionURL rdf:resource="http://www.rcahms.gov.uk" />
		<cc:attributionName xml:lang="en">RCAHMS</cc:attributionName>
		<dcterms:publisher rdf:resource="http://www.rcahms.gov.uk" />
		<skos:prefLabel xml:lang="en">SAILING VESSEL (BY FORM/TYPE)</skos:prefLabel>
		<dcterms:modified rdf:datatype="http://www.w3.org/2001/XMLSchema#dateTime">2007-04-23T18:02:06</dcterms:modified>
		<dcterms:issued rdf:datatype="http://www.w3.org/2001/XMLSchema#dateTime">2013-07-17T10:08:39</dcterms:issued>
		<skos:narrower rdf:resource="http://purl.org/heritagedata/schemes/3/concepts/501846" />
		<skos:narrower>
			<skos:Concept rdf:about="http://purl.org/heritagedata/schemes/3/concepts/501847">
				<skos:inScheme rdf:resource="http://purl.org/heritagedata/schemes/3" />
				<dcterms:identifier>http://purl.org/heritagedata/schemes/3/concepts/501847</dcterms:identifier>
				<cc:license rdf:resource="http://reference.data.gov.uk/id/open-government-licence" />
				<cc:attributionURL rdf:resource="http://www.rcahms.gov.uk" />
				<cc:attributionName xml:lang="en">RCAHMS</cc:attributionName>
				<dcterms:publisher rdf:resource="http://www.rcahms.gov.uk" />
				<skos:prefLabel xml:lang="en">BIRLINN</skos:prefLabel>
				<dcterms:modified rdf:datatype="http://www.w3.org/2001/XMLSchema#dateTime">2011-08-19T09:29:21</dcterms:modified>
				<dcterms:issued rdf:datatype="http://www.w3.org/2001/XMLSchema#dateTime">2013-07-17T10:08:39</dcterms:issued>
				<skos:broader rdf:resource="http://purl.org/heritagedata/schemes/3/concepts/501968" />
				<skos:scopeNote xml:lang="en">An imprecise term, loosely used to vessels built by clinker or 'clenched lap' construction but having a transom stern. Essentially a late development of the Norse or Viking tradition.</skos:scopeNote>
			</skos:Concept>
		</skos:narrower>
		<skos:narrower rdf:resource="http://purl.org/heritagedata/schemes/3/concepts/501848" />
		<skos:narrower>
			<skos:Concept rdf:about="http://purl.org/heritagedata/schemes/3/concepts/501858">
				<skos:inScheme rdf:resource="http://purl.org/heritagedata/schemes/3" />
				<dcterms:identifier>http://purl.org/heritagedata/schemes/3/concepts/501858</dcterms:identifier>
				<cc:license rdf:resource="http://reference.data.gov.uk/id/open-government-licence" />
				<cc:attributionURL rdf:resource="http://www.rcahms.gov.uk" />
				<cc:attributionName xml:lang="en">RCAHMS</cc:attributionName>
				<dcterms:publisher rdf:resource="http://www.rcahms.gov.uk" />
				<skos:prefLabel xml:lang="en">CARRACK</skos:prefLabel>
				<dcterms:modified rdf:datatype="http://www.w3.org/2001/XMLSchema#dateTime">2007-04-24T12:12:05</dcterms:modified>
				<dcterms:issued rdf:datatype="http://www.w3.org/2001/XMLSchema#dateTime">2013-07-17T10:08:39</dcterms:issued>
				<skos:broader rdf:resource="http://purl.org/heritagedata/schemes/3/concepts/501968" />
				<skos:scopeNote xml:lang="en">A large and robust trading vessel of North European origin, developed from the Mediterranean Caravel and characterised by having three masts, large castles fore and aft and a mixture of square and lateen sails.</skos:scopeNote>
			</skos:Concept>
		</skos:narrower>
		<skos:narrower>
			<skos:Concept rdf:about="http://purl.org/heritagedata/schemes/3/concepts/501866">
				<skos:inScheme rdf:resource="http://purl.org/heritagedata/schemes/3" />
				<dcterms:identifier>http://purl.org/heritagedata/schemes/3/concepts/501866</dcterms:identifier>
				<cc:license rdf:resource="http://reference.data.gov.uk/id/open-government-licence" />
				<cc:attributionURL rdf:resource="http://www.rcahms.gov.uk" />
				<cc:attributionName xml:lang="en">RCAHMS</cc:attributionName>
				<dcterms:publisher rdf:resource="http://www.rcahms.gov.uk" />
				<skos:prefLabel xml:lang="en">CUTTER</skos:prefLabel>
				<dcterms:issued rdf:datatype="http://www.w3.org/2001/XMLSchema#dateTime">2013-07-17T10:08:39</dcterms:issued>
				<skos:broader rdf:resource="http://purl.org/heritagedata/schemes/3/concepts/501968" />
				<skos:scopeNote xml:lang="en">This term has had a variety of meanings, the most significant being the original use to describe a small decked vessel with a fore-and-aft rig comprising a gaff mainsail and two headsails on a boom. Such a rig was inherently fast, leading to their use as light armed craft, notably against smugglers, and to carry pilots. The use of the term to describe a double-banked pulling craft in naval service is inapplicable.</skos:scopeNote>
			</skos:Concept>
		</skos:narrower>
		<skos:narrower>
			<skos:Concept rdf:about="http://purl.org/heritagedata/schemes/3/concepts/501867">
				<skos:inScheme rdf:resource="http://purl.org/heritagedata/schemes/3" />
				<dcterms:identifier>http://purl.org/heritagedata/schemes/3/concepts/501867</dcterms:identifier>
				<cc:license rdf:resource="http://reference.data.gov.uk/id/open-government-licence" />
				<cc:attributionURL rdf:resource="http://www.rcahms.gov.uk" />
				<cc:attributionName xml:lang="en">RCAHMS</cc:attributionName>
				<dcterms:publisher rdf:resource="http://www.rcahms.gov.uk" />
				<skos:prefLabel xml:lang="en">DANDY</skos:prefLabel>
				<dcterms:issued rdf:datatype="http://www.w3.org/2001/XMLSchema#dateTime">2013-07-17T10:08:39</dcterms:issued>
				<skos:broader rdf:resource="http://purl.org/heritagedata/schemes/3/concepts/501968" />
				<skos:scopeNote xml:lang="en">An imprecise term, loosely used to cover a variety of small fore-and-aft rigged sailed vessels having a mizzen mast and some or all of the characteristics of smacks and luggers.</skos:scopeNote>
			</skos:Concept>
		</skos:narrower>
		<skos:narrower rdf:resource="http://purl.org/heritagedata/schemes/3/concepts/501880" />
		<skos:narrower>
			<skos:Concept rdf:about="http://purl.org/heritagedata/schemes/3/concepts/501891">
				<skos:inScheme rdf:resource="http://purl.org/heritagedata/schemes/3" />
				<dcterms:identifier>http://purl.org/heritagedata/schemes/3/concepts/501891</dcterms:identifier>
				<cc:license rdf:resource="http://reference.data.gov.uk/id/open-government-licence" />
				<cc:attributionURL rdf:resource="http://www.rcahms.gov.uk" />
				<cc:attributionName xml:lang="en">RCAHMS</cc:attributionName>
				<dcterms:publisher rdf:resource="http://www.rcahms.gov.uk" />
				<skos:prefLabel xml:lang="en">FOURERN</skos:prefLabel>
				<dcterms:issued rdf:datatype="http://www.w3.org/2001/XMLSchema#dateTime">2013-07-17T10:08:39</dcterms:issued>
				<skos:broader rdf:resource="http://purl.org/heritagedata/schemes/3/concepts/501968" />
				<skos:scopeNote xml:lang="en">A small open boat typically used around Shetland, and propelled by rowing with four oars or (occasionally) a single square sail. Essentially a late development of the Norse or Viking tradition in series with the yoal and sixern; commonly developed for racing and recreational use.</skos:scopeNote>
			</skos:Concept>
		</skos:narrower>
		<skos:narrower>
			<skos:Concept rdf:about="http://purl.org/heritagedata/schemes/3/concepts/501895">
				<skos:inScheme rdf:resource="http://purl.org/heritagedata/schemes/3" />
				<dcterms:identifier>http://purl.org/heritagedata/schemes/3/concepts/501895</dcterms:identifier>
				<cc:license rdf:resource="http://reference.data.gov.uk/id/open-government-licence" />
				<cc:attributionURL rdf:resource="http://www.rcahms.gov.uk" />
				<cc:attributionName xml:lang="en">RCAHMS</cc:attributionName>
				<dcterms:publisher rdf:resource="http://www.rcahms.gov.uk" />
				<skos:prefLabel xml:lang="en">GALLEON</skos:prefLabel>
				<dcterms:modified rdf:datatype="http://www.w3.org/2001/XMLSchema#dateTime">2007-04-24T12:12:48</dcterms:modified>
				<dcterms:issued rdf:datatype="http://www.w3.org/2001/XMLSchema#dateTime">2013-07-17T10:08:39</dcterms:issued>
				<skos:broader rdf:resource="http://purl.org/heritagedata/schemes/3/concepts/501968" />
				<skos:scopeNote xml:lang="en">A large sailing vessel of the late 16th and early 17th centuries, used both for cargo transport and as a warship. Essentially a development of the Carrack with the high forecastle removed to improve the vessel's ability to turn and point into wind.</skos:scopeNote>
			</skos:Concept>
		</skos:narrower>
		<skos:narrower>
			<skos:Concept rdf:about="http://purl.org/heritagedata/schemes/3/concepts/501896">
				<skos:inScheme rdf:resource="http://purl.org/heritagedata/schemes/3" />
				<dcterms:identifier>http://purl.org/heritagedata/schemes/3/concepts/501896</dcterms:identifier>
				<cc:license rdf:resource="http://reference.data.gov.uk/id/open-government-licence" />
				<cc:attributionURL rdf:resource="http://www.rcahms.gov.uk" />
				<cc:attributionName xml:lang="en">RCAHMS</cc:attributionName>
				<dcterms:publisher rdf:resource="http://www.rcahms.gov.uk" />
				<skos:prefLabel xml:lang="en">GALLIOT</skos:prefLabel>
				<dcterms:issued rdf:datatype="http://www.w3.org/2001/XMLSchema#dateTime">2013-07-17T10:08:39</dcterms:issued>
				<skos:broader rdf:resource="http://purl.org/heritagedata/schemes/3/concepts/501968" />
				<skos:scopeNote xml:lang="en">A small transport vessel of Dutch type, having a bluff, rounded bow and fitted with leeboards. The type was usually fore-and-aft rigged on a single mast, often with a sprit.</skos:scopeNote>
			</skos:Concept>
		</skos:narrower>
		<skos:narrower>
			<skos:Concept rdf:about="http://purl.org/heritagedata/schemes/3/concepts/501908">
				<skos:inScheme rdf:resource="http://purl.org/heritagedata/schemes/3" />
				<dcterms:identifier>http://purl.org/heritagedata/schemes/3/concepts/501908</dcterms:identifier>
				<cc:license rdf:resource="http://reference.data.gov.uk/id/open-government-licence" />
				<cc:attributionURL rdf:resource="http://www.rcahms.gov.uk" />
				<cc:attributionName xml:lang="en">RCAHMS</cc:attributionName>
				<dcterms:publisher rdf:resource="http://www.rcahms.gov.uk" />
				<skos:prefLabel xml:lang="en">JIGGER</skos:prefLabel>
				<dcterms:issued rdf:datatype="http://www.w3.org/2001/XMLSchema#dateTime">2013-07-17T10:08:39</dcterms:issued>
				<skos:broader rdf:resource="http://purl.org/heritagedata/schemes/3/concepts/501968" />
				<skos:scopeNote xml:lang="en">An imprecise term apparently used to describe a small decked sailing vessel having a mizzen mast set after the fashion of a yawl.</skos:scopeNote>
			</skos:Concept>
		</skos:narrower>
		<skos:narrower rdf:resource="http://purl.org/heritagedata/schemes/3/concepts/501909" />
		<skos:narrower>
			<skos:Concept rdf:about="http://purl.org/heritagedata/schemes/3/concepts/501910">
				<skos:inScheme rdf:resource="http://purl.org/heritagedata/schemes/3" />
				<dcterms:identifier>http://purl.org/heritagedata/schemes/3/concepts/501910</dcterms:identifier>
				<cc:license rdf:resource="http://reference.data.gov.uk/id/open-government-licence" />
				<cc:attributionURL rdf:resource="http://www.rcahms.gov.uk" />
				<cc:attributionName xml:lang="en">RCAHMS</cc:attributionName>
				<dcterms:publisher rdf:resource="http://www.rcahms.gov.uk" />
				<skos:prefLabel xml:lang="en">KUFF</skos:prefLabel>
				<dcterms:issued rdf:datatype="http://www.w3.org/2001/XMLSchema#dateTime">2013-07-17T10:08:39</dcterms:issued>
				<skos:altLabel xml:lang="en">KOFF</skos:altLabel>
				<skos:altLabel xml:lang="en">KOFSCHIP</skos:altLabel>
				<skos:broader rdf:resource="http://purl.org/heritagedata/schemes/3/concepts/501968" />
				<skos:scopeNote xml:lang="en">A ketch-, schooner- or barque-rigged coastal cargo vessel of Dutch origin, characterised by very full and stern stem and stern.</skos:scopeNote>
			</skos:Concept>
		</skos:narrower>
		<skos:narrower rdf:resource="http://purl.org/heritagedata/schemes/3/concepts/501924" />
		<skos:narrower>
			<skos:Concept rdf:about="http://purl.org/heritagedata/schemes/3/concepts/501930">
				<skos:inScheme rdf:resource="http://purl.org/heritagedata/schemes/3" />
				<dcterms:identifier>http://purl.org/heritagedata/schemes/3/concepts/501930</dcterms:identifier>
				<cc:license rdf:resource="http://reference.data.gov.uk/id/open-government-licence" />
				<cc:attributionURL rdf:resource="http://www.rcahms.gov.uk" />
				<cc:attributionName xml:lang="en">RCAHMS</cc:attributionName>
				<dcterms:publisher rdf:resource="http://www.rcahms.gov.uk" />
				<skos:prefLabel xml:lang="en">MOTOR BOAT</skos:prefLabel>
				<dcterms:issued rdf:datatype="http://www.w3.org/2001/XMLSchema#dateTime">2013-07-17T10:08:39</dcterms:issued>
				<skos:broader rdf:resource="http://purl.org/heritagedata/schemes/3/concepts/501968" />
				<skos:scopeNote xml:lang="en">A Boat propelled by in inboard diesel engine.</skos:scopeNote>
			</skos:Concept>
		</skos:narrower>
		<skos:narrower>
			<skos:Concept rdf:about="http://purl.org/heritagedata/schemes/3/concepts/501946">
				<skos:inScheme rdf:resource="http://purl.org/heritagedata/schemes/3" />
				<dcterms:identifier>http://purl.org/heritagedata/schemes/3/concepts/501946</dcterms:identifier>
				<cc:license rdf:resource="http://reference.data.gov.uk/id/open-government-licence" />
				<cc:attributionURL rdf:resource="http://www.rcahms.gov.uk" />
				<cc:attributionName xml:lang="en">RCAHMS</cc:attributionName>
				<dcterms:publisher rdf:resource="http://www.rcahms.gov.uk" />
				<skos:prefLabel xml:lang="en">PACKET</skos:prefLabel>
				<dcterms:issued rdf:datatype="http://www.w3.org/2001/XMLSchema#dateTime">2013-07-17T10:08:39</dcterms:issued>
				<skos:broader rdf:resource="http://purl.org/heritagedata/schemes/3/concepts/501968" />
				<skos:scopeNote xml:lang="en">A fast, armed vessel, small in size, often used for despatches and mail.</skos:scopeNote>
			</skos:Concept>
		</skos:narrower>
		<skos:narrower>
			<skos:Concept rdf:about="http://purl.org/heritagedata/schemes/3/concepts/501954">
				<skos:inScheme rdf:resource="http://purl.org/heritagedata/schemes/3" />
				<dcterms:identifier>http://purl.org/heritagedata/schemes/3/concepts/501954</dcterms:identifier>
				<cc:license rdf:resource="http://reference.data.gov.uk/id/open-government-licence" />
				<cc:attributionURL rdf:resource="http://www.rcahms.gov.uk" />
				<cc:attributionName xml:lang="en">RCAHMS</cc:attributionName>
				<dcterms:publisher rdf:resource="http://www.rcahms.gov.uk" />
				<skos:prefLabel xml:lang="en">PUFFER</skos:prefLabel>
				<dcterms:issued rdf:datatype="http://www.w3.org/2001/XMLSchema#dateTime">2013-07-17T10:08:39</dcterms:issued>
				<skos:broader rdf:resource="http://purl.org/heritagedata/schemes/3/concepts/501968" />
				<skos:scopeNote xml:lang="en">Small steel-built trading vessel with a capacious hold, able to take the ground for loading, and sized to pass through the central Scottish canals. In their original form, they were powered by non-condensing steam engines. Later examples were built as military service craft under the designation Victualling Inshore Craft or VIC, and powered by diesel engines: the term puffer is applied to both types. Many of the losses recorded as steam lighters were probably vessels of this type.
The puffer has become a Scottish icon through the Para Handy books and television series; several examples are preserved.</skos:scopeNote>
			</skos:Concept>
		</skos:narrower>
		<skos:broader rdf:resource="http://purl.org/heritagedata/schemes/3/concepts/501925" />
		<skos:narrower>
			<skos:Concept rdf:about="http://purl.org/heritagedata/schemes/3/concepts/501980">
				<skos:inScheme rdf:resource="http://purl.org/heritagedata/schemes/3" />
				<dcterms:identifier>http://purl.org/heritagedata/schemes/3/concepts/501980</dcterms:identifier>
				<cc:license rdf:resource="http://reference.data.gov.uk/id/open-government-licence" />
				<cc:attributionURL rdf:resource="http://www.rcahms.gov.uk" />
				<cc:attributionName xml:lang="en">RCAHMS</cc:attributionName>
				<dcterms:publisher rdf:resource="http://www.rcahms.gov.uk" />
				<skos:prefLabel xml:lang="en">SIXERN</skos:prefLabel>
				<dcterms:issued rdf:datatype="http://www.w3.org/2001/XMLSchema#dateTime">2013-07-17T10:08:39</dcterms:issued>
				<skos:broader rdf:resource="http://purl.org/heritagedata/schemes/3/concepts/501968" />
				<skos:scopeNote xml:lang="en">A small open boat typically used for long-line fishing around Shetland, and propped by rowing with six oars or a single square sail. Essentially a late development of the Norse or Viking tradition; commonly developed for racing and recreational use.</skos:scopeNote>
			</skos:Concept>
		</skos:narrower>
		<skos:narrower>
			<skos:Concept rdf:about="http://purl.org/heritagedata/schemes/3/concepts/501982">
				<skos:inScheme rdf:resource="http://purl.org/heritagedata/schemes/3" />
				<dcterms:identifier>http://purl.org/heritagedata/schemes/3/concepts/501982</dcterms:identifier>
				<cc:license rdf:resource="http://reference.data.gov.uk/id/open-government-licence" />
				<cc:attributionURL rdf:resource="http://www.rcahms.gov.uk" />
				<cc:attributionName xml:lang="en">RCAHMS</cc:attributionName>
				<dcterms:publisher rdf:resource="http://www.rcahms.gov.uk" />
				<skos:prefLabel xml:lang="en">SKIFF</skos:prefLabel>
				<dcterms:modified rdf:datatype="http://www.w3.org/2001/XMLSchema#dateTime">2007-04-24T12:13:47</dcterms:modified>
				<dcterms:issued rdf:datatype="http://www.w3.org/2001/XMLSchema#dateTime">2013-07-17T10:08:39</dcterms:issued>
				<skos:broader rdf:resource="http://purl.org/heritagedata/schemes/3/concepts/501968" />
				<skos:scopeNote xml:lang="en">In general terms, this term is applied either to a small and generalised ship's boat of undecked form, or to one of a variety of specialised craft used on inland waterways, typically for recreational purposes. Specifically, the term indicates any of a variety of sailing vessels  used for ring-net fishing along the West coast, notably in Argyll. The term Nabbie refers to a variation within this type, which was unspecified in reports of loss.</skos:scopeNote>
			</skos:Concept>
		</skos:narrower>
		<skos:narrower rdf:resource="http://purl.org/heritagedata/schemes/3/concepts/501983" />
		<skos:narrower rdf:resource="http://purl.org/heritagedata/schemes/3/concepts/501984" />
		<skos:narrower>
			<skos:Concept rdf:about="http://purl.org/heritagedata/schemes/3/concepts/502001">
				<skos:inScheme rdf:resource="http://purl.org/heritagedata/schemes/3" />
				<dcterms:identifier>http://purl.org/heritagedata/schemes/3/concepts/502001</dcterms:identifier>
				<cc:license rdf:resource="http://reference.data.gov.uk/id/open-government-licence" />
				<cc:attributionURL rdf:resource="http://www.rcahms.gov.uk" />
				<cc:attributionName xml:lang="en">RCAHMS</cc:attributionName>
				<dcterms:publisher rdf:resource="http://www.rcahms.gov.uk" />
				<skos:prefLabel xml:lang="en">STEAMSHIP</skos:prefLabel>
				<dcterms:issued rdf:datatype="http://www.w3.org/2001/XMLSchema#dateTime">2013-07-17T10:08:39</dcterms:issued>
				<skos:broader rdf:resource="http://purl.org/heritagedata/schemes/3/concepts/501968" />
				<skos:scopeNote xml:lang="en">A medium-sized or large sea- or ocean-going vessel, with integral steam propulsion and used for a variety of purposes.</skos:scopeNote>
			</skos:Concept>
		</skos:narrower>
		<skos:narrower rdf:resource="http://purl.org/heritagedata/schemes/3/concepts/502017" />
		<skos:narrower rdf:resource="http://purl.org/heritagedata/schemes/3/concepts/502018" />
		<skos:narrower rdf:resource="http://purl.org/heritagedata/schemes/3/concepts/502019" />
		<skos:narrower>
			<skos:Concept rdf:about="http://purl.org/heritagedata/schemes/3/concepts/502020">
				<skos:inScheme rdf:resource="http://purl.org/heritagedata/schemes/3" />
				<dcterms:identifier>http://purl.org/heritagedata/schemes/3/concepts/502020</dcterms:identifier>
				<cc:license rdf:resource="http://reference.data.gov.uk/id/open-government-licence" />
				<cc:attributionURL rdf:resource="http://www.rcahms.gov.uk" />
				<cc:attributionName xml:lang="en">RCAHMS</cc:attributionName>
				<dcterms:publisher rdf:resource="http://www.rcahms.gov.uk" />
				<skos:prefLabel xml:lang="en">YOLE</skos:prefLabel>
				<dcterms:issued rdf:datatype="http://www.w3.org/2001/XMLSchema#dateTime">2013-07-17T10:08:39</dcterms:issued>
				<skos:altLabel xml:lang="en">YOAL</skos:altLabel>
				<skos:broader rdf:resource="http://purl.org/heritagedata/schemes/3/concepts/501968" />
				<skos:scopeNote xml:lang="en">A small open boat typically used around Shetland, and propelled by rowing, sails or an auxiliary engine. Essentially a late development of the Norse or Viking tradition in series with the fouern and sixern; commonly developed for racing and recreational use.
The term is cognate with yawl, but denotes a class of totally different and construction.</skos:scopeNote>
			</skos:Concept>
		</skos:narrower>
		<skos:scopeNote xml:lang="en">A sailing vessel defined by a combination of such factors as hull design, locality and rig.</skos:scopeNote>
	</skos:Concept>
	<skos:Concept rdf:about="http://purl.org/heritagedata/schemes/3/concepts/501969">
		<skos:inScheme rdf:resource="http://purl.org/heritagedata/schemes/3" />
		<dcterms:identifier>http://purl.org/heritagedata/schemes/3/concepts/501969</dcterms:identifier>
		<cc:license rdf:resource="http://reference.data.gov.uk/id/open-government-licence" />
		<cc:attributionURL rdf:resource="http://www.rcahms.gov.uk" />
		<cc:attributionName xml:lang="en">RCAHMS</cc:attributionName>
		<dcterms:publisher rdf:resource="http://www.rcahms.gov.uk" />
		<skos:prefLabel xml:lang="en">SAILING VESSEL (BY RIG)</skos:prefLabel>
		<dcterms:modified rdf:datatype="http://www.w3.org/2001/XMLSchema#dateTime">2007-04-23T18:02:06</dcterms:modified>
		<dcterms:issued rdf:datatype="http://www.w3.org/2001/XMLSchema#dateTime">2013-07-17T10:08:39</dcterms:issued>
		<skos:narrower>
			<skos:Concept rdf:about="http://purl.org/heritagedata/schemes/3/concepts/501843">
				<skos:inScheme rdf:resource="http://purl.org/heritagedata/schemes/3" />
				<dcterms:identifier>http://purl.org/heritagedata/schemes/3/concepts/501843</dcterms:identifier>
				<cc:license rdf:resource="http://reference.data.gov.uk/id/open-government-licence" />
				<cc:attributionURL rdf:resource="http://www.rcahms.gov.uk" />
				<cc:attributionName xml:lang="en">RCAHMS</cc:attributionName>
				<dcterms:publisher rdf:resource="http://www.rcahms.gov.uk" />
				<skos:prefLabel xml:lang="en">BARQUENTINE</skos:prefLabel>
				<dcterms:issued rdf:datatype="http://www.w3.org/2001/XMLSchema#dateTime">2013-07-17T10:08:39</dcterms:issued>
				<skos:altLabel xml:lang="en">BARKENTEEN</skos:altLabel>
				<skos:broader rdf:resource="http://purl.org/heritagedata/schemes/3/concepts/501969" />
				<skos:scopeNote xml:lang="en">A medium-sized decked sailing vessel (normally of timber construction) having three masts, with square sails on the foremast, while the main and mizzen masts were fore-and-aft rigged.</skos:scopeNote>
			</skos:Concept>
		</skos:narrower>
		<skos:narrower>
			<skos:Concept rdf:about="http://purl.org/heritagedata/schemes/3/concepts/501851">
				<skos:inScheme rdf:resource="http://purl.org/heritagedata/schemes/3" />
				<dcterms:identifier>http://purl.org/heritagedata/schemes/3/concepts/501851</dcterms:identifier>
				<cc:license rdf:resource="http://reference.data.gov.uk/id/open-government-licence" />
				<cc:attributionURL rdf:resource="http://www.rcahms.gov.uk" />
				<cc:attributionName xml:lang="en">RCAHMS</cc:attributionName>
				<dcterms:publisher rdf:resource="http://www.rcahms.gov.uk" />
				<skos:prefLabel xml:lang="en">BRIGANTINE</skos:prefLabel>
				<dcterms:issued rdf:datatype="http://www.w3.org/2001/XMLSchema#dateTime">2013-07-17T10:08:39</dcterms:issued>
				<skos:broader rdf:resource="http://purl.org/heritagedata/schemes/3/concepts/501969" />
				<skos:scopeNote xml:lang="en">Medium-sized decked sailing vessel (normally of timber construction) having two masts, with square sails on the foremast and fore-and-aft sails on the mainmast.</skos:scopeNote>
			</skos:Concept>
		</skos:narrower>
		<skos:broader rdf:resource="http://purl.org/heritagedata/schemes/3/concepts/501925" />
		<skos:narrower rdf:resource="http://purl.org/heritagedata/schemes/3/concepts/501971" />
		<skos:narrower rdf:resource="http://purl.org/heritagedata/schemes/3/concepts/501987" />
		<skos:scopeNote xml:lang="en">The characteristics of a sailing vessel where her type is determined by her masts and sails.</skos:scopeNote>
	</skos:Concept>
	<skos:Concept rdf:about="http://purl.org/heritagedata/schemes/3/concepts/501971">
		<skos:inScheme rdf:resource="http://purl.org/heritagedata/schemes/3" />
		<dcterms:identifier>http://purl.org/heritagedata/schemes/3/concepts/501971</dcterms:identifier>
		<cc:license rdf:resource="http://reference.data.gov.uk/id/open-government-licence" />
		<cc:attributionURL rdf:resource="http://www.rcahms.gov.uk" />
		<cc:attributionName xml:lang="en">RCAHMS</cc:attributionName>
		<dcterms:publisher rdf:resource="http://www.rcahms.gov.uk" />
		<skos:prefLabel xml:lang="en">SCHOONER</skos:prefLabel>
		<dcterms:issued rdf:datatype="http://www.w3.org/2001/XMLSchema#dateTime">2013-07-17T10:08:39</dcterms:issued>
		<skos:altLabel xml:lang="en">5 MASTED SCHOONER</skos:altLabel>
		<skos:narrower>
			<skos:Concept rdf:about="http://purl.org/heritagedata/schemes/3/concepts/501837">
				<skos:inScheme rdf:resource="http://purl.org/heritagedata/schemes/3" />
				<dcterms:identifier>http://purl.org/heritagedata/schemes/3/concepts/501837</dcterms:identifier>
				<cc:license rdf:resource="http://reference.data.gov.uk/id/open-government-licence" />
				<cc:attributionURL rdf:resource="http://www.rcahms.gov.uk" />
				<cc:attributionName xml:lang="en">RCAHMS</cc:attributionName>
				<dcterms:publisher rdf:resource="http://www.rcahms.gov.uk" />
				<skos:prefLabel xml:lang="en">AUXILIARY SCHOONER</skos:prefLabel>
				<dcterms:modified rdf:datatype="http://www.w3.org/2001/XMLSchema#dateTime">2007-04-24T11:43:47</dcterms:modified>
				<dcterms:issued rdf:datatype="http://www.w3.org/2001/XMLSchema#dateTime">2013-07-17T10:08:39</dcterms:issued>
				<skos:broader rdf:resource="http://purl.org/heritagedata/schemes/3/concepts/501971" />
				<skos:scopeNote xml:lang="en">A schooner having auxiliary steam or diesel propulsion for use in harbour areas, light airs or contrary winds.</skos:scopeNote>
			</skos:Concept>
		</skos:narrower>
		<skos:narrower>
			<skos:Concept rdf:about="http://purl.org/heritagedata/schemes/3/concepts/501900">
				<skos:inScheme rdf:resource="http://purl.org/heritagedata/schemes/3" />
				<dcterms:identifier>http://purl.org/heritagedata/schemes/3/concepts/501900</dcterms:identifier>
				<cc:license rdf:resource="http://reference.data.gov.uk/id/open-government-licence" />
				<cc:attributionURL rdf:resource="http://www.rcahms.gov.uk" />
				<cc:attributionName xml:lang="en">RCAHMS</cc:attributionName>
				<dcterms:publisher rdf:resource="http://www.rcahms.gov.uk" />
				<skos:prefLabel xml:lang="en">HERMAPHRODITE SCHOONER</skos:prefLabel>
				<dcterms:issued rdf:datatype="http://www.w3.org/2001/XMLSchema#dateTime">2013-07-17T10:08:39</dcterms:issued>
				<skos:broader rdf:resource="http://purl.org/heritagedata/schemes/3/concepts/501971" />
				<skos:scopeNote xml:lang="en">Variant of the Schooner having fore-and-aft sails on the foremast and a square topsail above a gaff main on the main.</skos:scopeNote>
			</skos:Concept>
		</skos:narrower>
		<skos:broader rdf:resource="http://purl.org/heritagedata/schemes/3/concepts/501969" />
		<skos:narrower>
			<skos:Concept rdf:about="http://purl.org/heritagedata/schemes/3/concepts/502010">
				<skos:inScheme rdf:resource="http://purl.org/heritagedata/schemes/3" />
				<dcterms:identifier>http://purl.org/heritagedata/schemes/3/concepts/502010</dcterms:identifier>
				<cc:license rdf:resource="http://reference.data.gov.uk/id/open-government-licence" />
				<cc:attributionURL rdf:resource="http://www.rcahms.gov.uk" />
				<cc:attributionName xml:lang="en">RCAHMS</cc:attributionName>
				<dcterms:publisher rdf:resource="http://www.rcahms.gov.uk" />
				<skos:prefLabel xml:lang="en">TOPSAIL SCHOONER</skos:prefLabel>
				<dcterms:issued rdf:datatype="http://www.w3.org/2001/XMLSchema#dateTime">2013-07-17T10:08:39</dcterms:issued>
				<skos:broader rdf:resource="http://purl.org/heritagedata/schemes/3/concepts/501971" />
				<skos:scopeNote xml:lang="en">A common variant of the Schooner type, having a square topsail or topsails on the foremast.</skos:scopeNote>
			</skos:Concept>
		</skos:narrower>
		<skos:scopeNote xml:lang="en">A decked sailing vessel, having fore-and-aft sails on two or more masts. Several variants have been recognised within this generalised type of vessel, which was used for a variety of purposes.</skos:scopeNote>
	</skos:Concept>
	<skos:Concept rdf:about="http://purl.org/heritagedata/schemes/3/concepts/501977">
		<skos:inScheme rdf:resource="http://purl.org/heritagedata/schemes/3" />
		<dcterms:identifier>http://purl.org/heritagedata/schemes/3/concepts/501977</dcterms:identifier>
		<cc:license rdf:resource="http://reference.data.gov.uk/id/open-government-licence" />
		<cc:attributionURL rdf:resource="http://www.rcahms.gov.uk" />
		<cc:attributionName xml:lang="en">RCAHMS</cc:attributionName>
		<dcterms:publisher rdf:resource="http://www.rcahms.gov.uk" />
		<skos:prefLabel xml:lang="en">SERVICE VESSEL</skos:prefLabel>
		<dcterms:modified rdf:datatype="http://www.w3.org/2001/XMLSchema#dateTime">2012-12-04T11:39:28</dcterms:modified>
		<dcterms:issued rdf:datatype="http://www.w3.org/2001/XMLSchema#dateTime">2013-07-17T10:08:39</dcterms:issued>
		<skos:narrower>
			<skos:Concept rdf:about="http://purl.org/heritagedata/schemes/3/concepts/502027">
				<skos:inScheme rdf:resource="http://purl.org/heritagedata/schemes/3" />
				<dcterms:identifier>http://purl.org/heritagedata/schemes/3/concepts/502027</dcterms:identifier>
				<cc:license rdf:resource="http://reference.data.gov.uk/id/open-government-licence" />
				<cc:attributionURL rdf:resource="http://www.rcahms.gov.uk" />
				<cc:attributionName xml:lang="en">RCAHMS</cc:attributionName>
				<dcterms:publisher rdf:resource="http://www.rcahms.gov.uk" />
				<skos:prefLabel xml:lang="en">PILOT VESSEL</skos:prefLabel>
				<dcterms:created rdf:datatype="http://www.w3.org/2001/XMLSchema#dateTime">2007-05-10T08:39:45</dcterms:created>
				<dcterms:modified rdf:datatype="http://www.w3.org/2001/XMLSchema#dateTime">2007-05-10T08:41:29</dcterms:modified>
				<dcterms:issued rdf:datatype="http://www.w3.org/2001/XMLSchema#dateTime">2013-07-17T10:08:39</dcterms:issued>
				<skos:broader rdf:resource="http://purl.org/heritagedata/schemes/3/concepts/501977" />
				<skos:scopeNote xml:lang="en">A boat or (more commonly) small ship used (and generally built) to transport and transfer pilots to and from incoming and outgoing vessels at the limit of pilotage waters in outer estuaries. Traditionally, these have built for speed as pilotage services have often been sold commercially, and the first pilot to reach the vessel secured the traffic. Such sailing vessels were typically rigged as cutters, giving rise to the alternative name Pilot Cutter, and were also used for racing, More recent practice has been to station pilot vessels semi-permanently in harbour approaches, the pilots waiting on board for traffic. The previous practice remains in use, however, at those ports where pilots wait onshore, being transferred by fast Pilot Launches.</skos:scopeNote>
			</skos:Concept>
		</skos:narrower>
		<skos:narrower>
			<skos:Concept rdf:about="http://purl.org/heritagedata/schemes/3/concepts/501853">
				<skos:inScheme rdf:resource="http://purl.org/heritagedata/schemes/3" />
				<dcterms:identifier>http://purl.org/heritagedata/schemes/3/concepts/501853</dcterms:identifier>
				<cc:license rdf:resource="http://reference.data.gov.uk/id/open-government-licence" />
				<cc:attributionURL rdf:resource="http://www.rcahms.gov.uk" />
				<cc:attributionName xml:lang="en">RCAHMS</cc:attributionName>
				<dcterms:publisher rdf:resource="http://www.rcahms.gov.uk" />
				<skos:prefLabel xml:lang="en">BUOY TENDER</skos:prefLabel>
				<dcterms:issued rdf:datatype="http://www.w3.org/2001/XMLSchema#dateTime">2013-07-17T10:08:39</dcterms:issued>
				<skos:broader rdf:resource="http://purl.org/heritagedata/schemes/3/concepts/501977" />
				<skos:scopeNote xml:lang="en">a service craft (typically of small to medium size) intended to lay, lift and resupply navigation buoys. They usually have a well deck and heavy derrick or crane forward for handling heavy equipment; most have a helicopter deck aft.</skos:scopeNote>
			</skos:Concept>
		</skos:narrower>
		<skos:narrower rdf:resource="http://purl.org/heritagedata/schemes/3/concepts/501898" />
		<skos:narrower>
			<skos:Concept rdf:about="http://purl.org/heritagedata/schemes/3/concepts/501906">
				<skos:inScheme rdf:resource="http://purl.org/heritagedata/schemes/3" />
				<dcterms:identifier>http://purl.org/heritagedata/schemes/3/concepts/501906</dcterms:identifier>
				<cc:license rdf:resource="http://reference.data.gov.uk/id/open-government-licence" />
				<cc:attributionURL rdf:resource="http://www.rcahms.gov.uk" />
				<cc:attributionName xml:lang="en">RCAHMS</cc:attributionName>
				<dcterms:publisher rdf:resource="http://www.rcahms.gov.uk" />
				<skos:prefLabel xml:lang="en">HULK</skos:prefLabel>
				<dcterms:issued rdf:datatype="http://www.w3.org/2001/XMLSchema#dateTime">2013-07-17T10:08:39</dcterms:issued>
				<skos:broader rdf:resource="http://purl.org/heritagedata/schemes/3/concepts/501977" />
				<skos:scopeNote xml:lang="en">General term of a superseded ship (of any type or construction) converted for static but floating use in harbours, dockyards or engineering works. Typical examples include sheer hulks (for fitting masts), stores and accommodation hulks, and prison hulks.</skos:scopeNote>
			</skos:Concept>
		</skos:narrower>
		<skos:narrower>
			<skos:Concept rdf:about="http://purl.org/heritagedata/schemes/3/concepts/501920">
				<skos:inScheme rdf:resource="http://purl.org/heritagedata/schemes/3" />
				<dcterms:identifier>http://purl.org/heritagedata/schemes/3/concepts/501920</dcterms:identifier>
				<cc:license rdf:resource="http://reference.data.gov.uk/id/open-government-licence" />
				<cc:attributionURL rdf:resource="http://www.rcahms.gov.uk" />
				<cc:attributionName xml:lang="en">RCAHMS</cc:attributionName>
				<dcterms:publisher rdf:resource="http://www.rcahms.gov.uk" />
				<skos:prefLabel xml:lang="en">LIGHTHOUSE TENDER</skos:prefLabel>
				<dcterms:modified rdf:datatype="http://www.w3.org/2001/XMLSchema#dateTime">2007-04-24T12:17:07</dcterms:modified>
				<dcterms:issued rdf:datatype="http://www.w3.org/2001/XMLSchema#dateTime">2013-07-17T10:08:39</dcterms:issued>
				<skos:broader rdf:resource="http://purl.org/heritagedata/schemes/3/concepts/501977" />
				<skos:scopeNote xml:lang="en">A service craft (typically of small to medium size) intended to support and resupply lighthouses and light vessels. They usually also serve as Buoy Tenders and may have a well deck and heavy derrick or crane forward for handling heavy equipment; most have a helicopter deck aft. They also serve as inspection vessels for Lighthouse Board members, and are outfitted accordingly, being known popularly as `Lighthouse Yachts'.</skos:scopeNote>
			</skos:Concept>
		</skos:narrower>
		<skos:narrower rdf:resource="http://purl.org/heritagedata/schemes/3/concepts/501966" />
		<skos:narrower>
			<skos:Concept rdf:about="http://purl.org/heritagedata/schemes/3/concepts/501970">
				<skos:inScheme rdf:resource="http://purl.org/heritagedata/schemes/3" />
				<dcterms:identifier>http://purl.org/heritagedata/schemes/3/concepts/501970</dcterms:identifier>
				<cc:license rdf:resource="http://reference.data.gov.uk/id/open-government-licence" />
				<cc:attributionURL rdf:resource="http://www.rcahms.gov.uk" />
				<cc:attributionName xml:lang="en">RCAHMS</cc:attributionName>
				<dcterms:publisher rdf:resource="http://www.rcahms.gov.uk" />
				<skos:prefLabel xml:lang="en">SALVAGE VESSEL</skos:prefLabel>
				<dcterms:issued rdf:datatype="http://www.w3.org/2001/XMLSchema#dateTime">2013-07-17T10:08:39</dcterms:issued>
				<skos:broader rdf:resource="http://purl.org/heritagedata/schemes/3/concepts/501977" />
				<skos:scopeNote xml:lang="en">A vessel used for the underwater recovery of a ship and/or her contents or to assist vessels that are sinking.</skos:scopeNote>
			</skos:Concept>
		</skos:narrower>
		<skos:broader rdf:resource="http://purl.org/heritagedata/schemes/3/concepts/501925" />
		<skos:scopeNote xml:lang="en">A vessel used to maintain supply or assist larger vessels. Use more specific term.</skos:scopeNote>
	</skos:Concept>
	<skos:Concept rdf:about="http://purl.org/heritagedata/schemes/3/concepts/501979">
		<skos:inScheme rdf:resource="http://purl.org/heritagedata/schemes/3" />
		<dcterms:identifier>http://purl.org/heritagedata/schemes/3/concepts/501979</dcterms:identifier>
		<cc:license rdf:resource="http://reference.data.gov.uk/id/open-government-licence" />
		<cc:attributionURL rdf:resource="http://www.rcahms.gov.uk" />
		<cc:attributionName xml:lang="en">RCAHMS</cc:attributionName>
		<dcterms:publisher rdf:resource="http://www.rcahms.gov.uk" />
		<skos:prefLabel xml:lang="en">SHIP OF THE LINE</skos:prefLabel>
		<dcterms:issued rdf:datatype="http://www.w3.org/2001/XMLSchema#dateTime">2013-07-17T10:08:39</dcterms:issued>
		<skos:narrower>
			<skos:Concept rdf:about="http://purl.org/heritagedata/schemes/3/concepts/501885">
				<skos:inScheme rdf:resource="http://purl.org/heritagedata/schemes/3" />
				<dcterms:identifier>http://purl.org/heritagedata/schemes/3/concepts/501885</dcterms:identifier>
				<cc:license rdf:resource="http://reference.data.gov.uk/id/open-government-licence" />
				<cc:attributionURL rdf:resource="http://www.rcahms.gov.uk" />
				<cc:attributionName xml:lang="en">RCAHMS</cc:attributionName>
				<dcterms:publisher rdf:resource="http://www.rcahms.gov.uk" />
				<skos:prefLabel xml:lang="en">FIFTH RATE WARSHIP</skos:prefLabel>
				<dcterms:modified rdf:datatype="http://www.w3.org/2001/XMLSchema#dateTime">2007-04-24T14:44:15</dcterms:modified>
				<dcterms:issued rdf:datatype="http://www.w3.org/2001/XMLSchema#dateTime">2013-07-17T10:08:39</dcterms:issued>
				<skos:broader rdf:resource="http://purl.org/heritagedata/schemes/3/concepts/501979" />
				<skos:scopeNote xml:lang="en">Under the rating system introduced into the Royal Navy by Admiral Lord Anson in 1751-6, fifth rate warships were those carrying between 32 and 50 guns (increased to between 32 and 60 from 1810). Such vessels were the larger Frigates (otherwise termed Cruisers), and were built with a sufficient speed to make them suitable for scouting and detached duties. HMS Unicorn and HMS Tricomalee (in preservation at Dundee and Hartlepool respectively) exemplify the type.</skos:scopeNote>
			</skos:Concept>
		</skos:narrower>
		<skos:narrower>
			<skos:Concept rdf:about="http://purl.org/heritagedata/schemes/3/concepts/501886">
				<skos:inScheme rdf:resource="http://purl.org/heritagedata/schemes/3" />
				<dcterms:identifier>http://purl.org/heritagedata/schemes/3/concepts/501886</dcterms:identifier>
				<cc:license rdf:resource="http://reference.data.gov.uk/id/open-government-licence" />
				<cc:attributionURL rdf:resource="http://www.rcahms.gov.uk" />
				<cc:attributionName xml:lang="en">RCAHMS</cc:attributionName>
				<dcterms:publisher rdf:resource="http://www.rcahms.gov.uk" />
				<skos:prefLabel xml:lang="en">FIRST RATE WARSHIP</skos:prefLabel>
				<dcterms:modified rdf:datatype="http://www.w3.org/2001/XMLSchema#dateTime">2007-04-24T14:42:42</dcterms:modified>
				<dcterms:issued rdf:datatype="http://www.w3.org/2001/XMLSchema#dateTime">2013-07-17T10:08:39</dcterms:issued>
				<skos:broader rdf:resource="http://purl.org/heritagedata/schemes/3/concepts/501979" />
				<skos:scopeNote xml:lang="en">Under the rating system introduced into the Royal Navy by Admiral Lord Anson in 1751-6, first rate warships were those carrying over 100 guns (increased to 110 from 1810) on three decks. Such vessels were the heaviest 'Ships of the Line [of Battle]', being optimised for armament above all else.</skos:scopeNote>
			</skos:Concept>
		</skos:narrower>
		<skos:narrower>
			<skos:Concept rdf:about="http://purl.org/heritagedata/schemes/3/concepts/501892">
				<skos:inScheme rdf:resource="http://purl.org/heritagedata/schemes/3" />
				<dcterms:identifier>http://purl.org/heritagedata/schemes/3/concepts/501892</dcterms:identifier>
				<cc:license rdf:resource="http://reference.data.gov.uk/id/open-government-licence" />
				<cc:attributionURL rdf:resource="http://www.rcahms.gov.uk" />
				<cc:attributionName xml:lang="en">RCAHMS</cc:attributionName>
				<dcterms:publisher rdf:resource="http://www.rcahms.gov.uk" />
				<skos:prefLabel xml:lang="en">FOURTH RATE WARSHIP</skos:prefLabel>
				<dcterms:modified rdf:datatype="http://www.w3.org/2001/XMLSchema#dateTime">2007-04-24T14:44:59</dcterms:modified>
				<dcterms:issued rdf:datatype="http://www.w3.org/2001/XMLSchema#dateTime">2013-07-17T10:08:39</dcterms:issued>
				<skos:broader rdf:resource="http://purl.org/heritagedata/schemes/3/concepts/501979" />
				<skos:scopeNote xml:lang="en">Under the rating system introduced into the Royal Navy by Admiral Lord Anson in 1751-6, 'fourth rate' warships were those carrying between 50 and 70 guns (increased to between 60 and 80 from 1810). Such vessels rarely built, and occupied an equivocal status between the larger Ships of the Line and the smaller Frigates.</skos:scopeNote>
			</skos:Concept>
		</skos:narrower>
		<skos:narrower>
			<skos:Concept rdf:about="http://purl.org/heritagedata/schemes/3/concepts/501975">
				<skos:inScheme rdf:resource="http://purl.org/heritagedata/schemes/3" />
				<dcterms:identifier>http://purl.org/heritagedata/schemes/3/concepts/501975</dcterms:identifier>
				<cc:license rdf:resource="http://reference.data.gov.uk/id/open-government-licence" />
				<cc:attributionURL rdf:resource="http://www.rcahms.gov.uk" />
				<cc:attributionName xml:lang="en">RCAHMS</cc:attributionName>
				<dcterms:publisher rdf:resource="http://www.rcahms.gov.uk" />
				<skos:prefLabel xml:lang="en">SECOND RATE WARSHIP</skos:prefLabel>
				<dcterms:modified rdf:datatype="http://www.w3.org/2001/XMLSchema#dateTime">2007-04-24T14:50:31</dcterms:modified>
				<dcterms:issued rdf:datatype="http://www.w3.org/2001/XMLSchema#dateTime">2013-07-17T10:08:39</dcterms:issued>
				<skos:broader rdf:resource="http://purl.org/heritagedata/schemes/3/concepts/501979" />
				<skos:scopeNote xml:lang="en">Under the rating system introduced into the Royal Navy by Admiral Lord Anson in 1751-6, second rate warships were those carrying between 84 and 100 guns (increased to between 90 and 110 from 1810) on three decks. Such vessels were the heavier Ships of the Line [of Battle], being optimised for armament above all else.</skos:scopeNote>
			</skos:Concept>
		</skos:narrower>
		<skos:broader rdf:resource="http://purl.org/heritagedata/schemes/3/concepts/502015" />
		<skos:narrower>
			<skos:Concept rdf:about="http://purl.org/heritagedata/schemes/3/concepts/501981">
				<skos:inScheme rdf:resource="http://purl.org/heritagedata/schemes/3" />
				<dcterms:identifier>http://purl.org/heritagedata/schemes/3/concepts/501981</dcterms:identifier>
				<cc:license rdf:resource="http://reference.data.gov.uk/id/open-government-licence" />
				<cc:attributionURL rdf:resource="http://www.rcahms.gov.uk" />
				<cc:attributionName xml:lang="en">RCAHMS</cc:attributionName>
				<dcterms:publisher rdf:resource="http://www.rcahms.gov.uk" />
				<skos:prefLabel xml:lang="en">SIXTH RATE WARSHIP</skos:prefLabel>
				<dcterms:modified rdf:datatype="http://www.w3.org/2001/XMLSchema#dateTime">2007-04-24T14:51:01</dcterms:modified>
				<dcterms:issued rdf:datatype="http://www.w3.org/2001/XMLSchema#dateTime">2013-07-17T10:08:39</dcterms:issued>
				<skos:broader rdf:resource="http://purl.org/heritagedata/schemes/3/concepts/501979" />
				<skos:scopeNote xml:lang="en">Under the rating system introduced into the Royal Navy by Admiral Lord Anson in 1751-6, sixth rate warships were those carrying fewer than 32 guns. Such vessels were termed Frigates if commanded by a post-captain, but sloops if commanded by a commander. They were built with a sufficient speed to make them suitable for scouting and detached duties.</skos:scopeNote>
			</skos:Concept>
		</skos:narrower>
		<skos:narrower>
			<skos:Concept rdf:about="http://purl.org/heritagedata/schemes/3/concepts/502009">
				<skos:inScheme rdf:resource="http://purl.org/heritagedata/schemes/3" />
				<dcterms:identifier>http://purl.org/heritagedata/schemes/3/concepts/502009</dcterms:identifier>
				<cc:license rdf:resource="http://reference.data.gov.uk/id/open-government-licence" />
				<cc:attributionURL rdf:resource="http://www.rcahms.gov.uk" />
				<cc:attributionName xml:lang="en">RCAHMS</cc:attributionName>
				<dcterms:publisher rdf:resource="http://www.rcahms.gov.uk" />
				<skos:prefLabel xml:lang="en">THIRD RATE WARSHIP</skos:prefLabel>
				<dcterms:modified rdf:datatype="http://www.w3.org/2001/XMLSchema#dateTime">2007-04-24T14:45:34</dcterms:modified>
				<dcterms:issued rdf:datatype="http://www.w3.org/2001/XMLSchema#dateTime">2013-07-17T10:08:39</dcterms:issued>
				<skos:broader rdf:resource="http://purl.org/heritagedata/schemes/3/concepts/501979" />
				<skos:scopeNote xml:lang="en">Under the rating system introduced into the Royal Navy by Admiral Lord Anson in 1751-6, third rate warships were those carrying between 70 and 84 guns (increased to between 80 and 90 from 1810) on two decks. Such vessels were the norm among the 'Ships of the Line [of Battle]'.</skos:scopeNote>
			</skos:Concept>
		</skos:narrower>
		<skos:scopeNote xml:lang="en">A sailing ship with a sufficient numerically large gun armament to stand in the line of battle.</skos:scopeNote>
	</skos:Concept>
	<skos:Concept rdf:about="http://purl.org/heritagedata/schemes/3/concepts/501983">
		<skos:inScheme rdf:resource="http://purl.org/heritagedata/schemes/3" />
		<dcterms:identifier>http://purl.org/heritagedata/schemes/3/concepts/501983</dcterms:identifier>
		<cc:license rdf:resource="http://reference.data.gov.uk/id/open-government-licence" />
		<cc:attributionURL rdf:resource="http://www.rcahms.gov.uk" />
		<cc:attributionName xml:lang="en">RCAHMS</cc:attributionName>
		<dcterms:publisher rdf:resource="http://www.rcahms.gov.uk" />
		<skos:prefLabel xml:lang="en">SLOOP</skos:prefLabel>
		<dcterms:issued rdf:datatype="http://www.w3.org/2001/XMLSchema#dateTime">2013-07-17T10:08:39</dcterms:issued>
		<skos:broader rdf:resource="http://purl.org/heritagedata/schemes/3/concepts/501968" />
		<skos:narrower>
			<skos:Concept rdf:about="http://purl.org/heritagedata/schemes/3/concepts/502263">
				<skos:inScheme rdf:resource="http://purl.org/heritagedata/schemes/3" />
				<dcterms:identifier>http://purl.org/heritagedata/schemes/3/concepts/502263</dcterms:identifier>
				<cc:license rdf:resource="http://reference.data.gov.uk/id/open-government-licence" />
				<cc:attributionURL rdf:resource="http://www.rcahms.gov.uk" />
				<cc:attributionName xml:lang="en">RCAHMS</cc:attributionName>
				<dcterms:publisher rdf:resource="http://www.rcahms.gov.uk" />
				<skos:prefLabel xml:lang="en">AUXILIARY SLOOP</skos:prefLabel>
				<dcterms:created rdf:datatype="http://www.w3.org/2001/XMLSchema#dateTime">2007-05-18T15:48:11</dcterms:created>
				<dcterms:modified rdf:datatype="http://www.w3.org/2001/XMLSchema#dateTime">2007-05-18T15:48:35</dcterms:modified>
				<dcterms:issued rdf:datatype="http://www.w3.org/2001/XMLSchema#dateTime">2013-07-17T10:08:39</dcterms:issued>
				<skos:broader rdf:resource="http://purl.org/heritagedata/schemes/3/concepts/501983" />
				<skos:scopeNote xml:lang="en">A decked sailing vessel, having fore-and-aft sails (including a single headsail and often a gaff main) on a single mast. Several variants have been recognised within this generalised type of vessel, which was used for a variety of purposes. In naval service, the term was commonly applied to a vessel deemed too small to be given a formal rating; these vessels carried between 18 and 36 guns, and were rigged as Ships or Brigs, being termed Ship-sloops or Brig-sloops respectively.</skos:scopeNote>
			</skos:Concept>
		</skos:narrower>
		<skos:scopeNote xml:lang="en">A decked sailing vessel, having fore-and-aft sails (including a single headsail and often a gaff main) on a single mast. Several variants have been recognised within this generalised type of vessel, which was used for a variety of purposes.</skos:scopeNote>
	</skos:Concept>
	<skos:Concept rdf:about="http://purl.org/heritagedata/schemes/3/concepts/501984">
		<skos:inScheme rdf:resource="http://purl.org/heritagedata/schemes/3" />
		<dcterms:identifier>http://purl.org/heritagedata/schemes/3/concepts/501984</dcterms:identifier>
		<cc:license rdf:resource="http://reference.data.gov.uk/id/open-government-licence" />
		<cc:attributionURL rdf:resource="http://www.rcahms.gov.uk" />
		<cc:attributionName xml:lang="en">RCAHMS</cc:attributionName>
		<dcterms:publisher rdf:resource="http://www.rcahms.gov.uk" />
		<skos:prefLabel xml:lang="en">SMACK</skos:prefLabel>
		<dcterms:issued rdf:datatype="http://www.w3.org/2001/XMLSchema#dateTime">2013-07-17T10:08:39</dcterms:issued>
		<skos:narrower>
			<skos:Concept rdf:about="http://purl.org/heritagedata/schemes/3/concepts/501838">
				<skos:inScheme rdf:resource="http://purl.org/heritagedata/schemes/3" />
				<dcterms:identifier>http://purl.org/heritagedata/schemes/3/concepts/501838</dcterms:identifier>
				<cc:license rdf:resource="http://reference.data.gov.uk/id/open-government-licence" />
				<cc:attributionURL rdf:resource="http://www.rcahms.gov.uk" />
				<cc:attributionName xml:lang="en">RCAHMS</cc:attributionName>
				<dcterms:publisher rdf:resource="http://www.rcahms.gov.uk" />
				<skos:prefLabel xml:lang="en">AUXILIARY SMACK</skos:prefLabel>
				<dcterms:modified rdf:datatype="http://www.w3.org/2001/XMLSchema#dateTime">2007-04-24T11:45:44</dcterms:modified>
				<dcterms:issued rdf:datatype="http://www.w3.org/2001/XMLSchema#dateTime">2013-07-17T10:08:39</dcterms:issued>
				<skos:broader rdf:resource="http://purl.org/heritagedata/schemes/3/concepts/501984" />
				<skos:scopeNote xml:lang="en">A smack having auxiliary steam or diesel propulsion for use in harbour areas, light airs or contrary winds.</skos:scopeNote>
			</skos:Concept>
		</skos:narrower>
		<skos:broader rdf:resource="http://purl.org/heritagedata/schemes/3/concepts/501968" />
		<skos:scopeNote xml:lang="en">A transom-sterned and decked vessel, commonly used for cargo-carrying around the Firth of Clyde. Such vessels were commonly cutter- or ketch-rigged, often with a gaff main.</skos:scopeNote>
	</skos:Concept>
	<skos:Concept rdf:about="http://purl.org/heritagedata/schemes/3/concepts/501987">
		<skos:inScheme rdf:resource="http://purl.org/heritagedata/schemes/3" />
		<dcterms:identifier>http://purl.org/heritagedata/schemes/3/concepts/501987</dcterms:identifier>
		<cc:license rdf:resource="http://reference.data.gov.uk/id/open-government-licence" />
		<cc:attributionURL rdf:resource="http://www.rcahms.gov.uk" />
		<cc:attributionName xml:lang="en">RCAHMS</cc:attributionName>
		<dcterms:publisher rdf:resource="http://www.rcahms.gov.uk" />
		<skos:prefLabel xml:lang="en">SQUARE RIGGED VESSEL</skos:prefLabel>
		<dcterms:issued rdf:datatype="http://www.w3.org/2001/XMLSchema#dateTime">2013-07-17T10:08:39</dcterms:issued>
		<skos:narrower rdf:resource="http://purl.org/heritagedata/schemes/3/concepts/501842" />
		<skos:narrower rdf:resource="http://purl.org/heritagedata/schemes/3/concepts/501850" />
		<skos:narrower>
			<skos:Concept rdf:about="http://purl.org/heritagedata/schemes/3/concepts/501951">
				<skos:inScheme rdf:resource="http://purl.org/heritagedata/schemes/3" />
				<dcterms:identifier>http://purl.org/heritagedata/schemes/3/concepts/501951</dcterms:identifier>
				<cc:license rdf:resource="http://reference.data.gov.uk/id/open-government-licence" />
				<cc:attributionURL rdf:resource="http://www.rcahms.gov.uk" />
				<cc:attributionName xml:lang="en">RCAHMS</cc:attributionName>
				<dcterms:publisher rdf:resource="http://www.rcahms.gov.uk" />
				<skos:prefLabel xml:lang="en">PINK</skos:prefLabel>
				<dcterms:issued rdf:datatype="http://www.w3.org/2001/XMLSchema#dateTime">2013-07-17T10:08:39</dcterms:issued>
				<skos:broader rdf:resource="http://purl.org/heritagedata/schemes/3/concepts/501987" />
				<skos:scopeNote xml:lang="en">Small square rigged ship with a narrow overhanging stern.</skos:scopeNote>
			</skos:Concept>
		</skos:narrower>
		<skos:narrower rdf:resource="http://purl.org/heritagedata/schemes/3/concepts/501952" />
		<skos:narrower>
			<skos:Concept rdf:about="http://purl.org/heritagedata/schemes/3/concepts/501985">
				<skos:inScheme rdf:resource="http://purl.org/heritagedata/schemes/3" />
				<dcterms:identifier>http://purl.org/heritagedata/schemes/3/concepts/501985</dcterms:identifier>
				<cc:license rdf:resource="http://reference.data.gov.uk/id/open-government-licence" />
				<cc:attributionURL rdf:resource="http://www.rcahms.gov.uk" />
				<cc:attributionName xml:lang="en">RCAHMS</cc:attributionName>
				<dcterms:publisher rdf:resource="http://www.rcahms.gov.uk" />
				<skos:prefLabel xml:lang="en">SNOW</skos:prefLabel>
				<dcterms:issued rdf:datatype="http://www.w3.org/2001/XMLSchema#dateTime">2013-07-17T10:08:39</dcterms:issued>
				<skos:broader rdf:resource="http://purl.org/heritagedata/schemes/3/concepts/501987" />
				<skos:scopeNote xml:lang="en">Two masted merchant vessel, rigged as a brig.</skos:scopeNote>
			</skos:Concept>
		</skos:narrower>
		<skos:broader rdf:resource="http://purl.org/heritagedata/schemes/3/concepts/501969" />
		<skos:scopeNote xml:lang="en">A vessel with a type of rigging where the main driving sails are fixed to yards which lie square to the mast.</skos:scopeNote>
	</skos:Concept>
	<skos:Concept rdf:about="http://purl.org/heritagedata/schemes/3/concepts/501989">
		<skos:inScheme rdf:resource="http://purl.org/heritagedata/schemes/3" />
		<dcterms:identifier>http://purl.org/heritagedata/schemes/3/concepts/501989</dcterms:identifier>
		<cc:license rdf:resource="http://reference.data.gov.uk/id/open-government-licence" />
		<cc:attributionURL rdf:resource="http://www.rcahms.gov.uk" />
		<cc:attributionName xml:lang="en">RCAHMS</cc:attributionName>
		<dcterms:publisher rdf:resource="http://www.rcahms.gov.uk" />
		<skos:prefLabel xml:lang="en">STEAM DRIFTER</skos:prefLabel>
		<dcterms:issued rdf:datatype="http://www.w3.org/2001/XMLSchema#dateTime">2013-07-17T10:08:39</dcterms:issued>
		<skos:narrower>
			<skos:Concept rdf:about="http://purl.org/heritagedata/schemes/3/concepts/501961">
				<skos:inScheme rdf:resource="http://purl.org/heritagedata/schemes/3" />
				<dcterms:identifier>http://purl.org/heritagedata/schemes/3/concepts/501961</dcterms:identifier>
				<cc:license rdf:resource="http://reference.data.gov.uk/id/open-government-licence" />
				<cc:attributionURL rdf:resource="http://www.rcahms.gov.uk" />
				<cc:attributionName xml:lang="en">RCAHMS</cc:attributionName>
				<dcterms:publisher rdf:resource="http://www.rcahms.gov.uk" />
				<skos:prefLabel xml:lang="en">REQUISITIONED STEAM DRIFTER</skos:prefLabel>
				<dcterms:issued rdf:datatype="http://www.w3.org/2001/XMLSchema#dateTime">2013-07-17T10:08:39</dcterms:issued>
				<skos:broader rdf:resource="http://purl.org/heritagedata/schemes/3/concepts/501989" />
				<skos:scopeNote xml:lang="en">A Steam Drifter which has been requisitioned for war service, generally within its local area, with an unchanged crew and with the fitting of only basic armament (if any). Such vessels were typically used for transport and target-towing as well as patrol duties.</skos:scopeNote>
			</skos:Concept>
		</skos:narrower>
		<skos:broader rdf:resource="http://purl.org/heritagedata/schemes/3/concepts/501873" />
		<skos:scopeNote xml:lang="en">A Drifter with integral steam propulsion. Such vessels were long the mainstay of the Scottish inshore fishing industry, supplanting various types of Lugger.</skos:scopeNote>
	</skos:Concept>
	<skos:Concept rdf:about="http://purl.org/heritagedata/schemes/3/concepts/501998">
		<skos:inScheme rdf:resource="http://purl.org/heritagedata/schemes/3" />
		<dcterms:identifier>http://purl.org/heritagedata/schemes/3/concepts/501998</dcterms:identifier>
		<cc:license rdf:resource="http://reference.data.gov.uk/id/open-government-licence" />
		<cc:attributionURL rdf:resource="http://www.rcahms.gov.uk" />
		<cc:attributionName xml:lang="en">RCAHMS</cc:attributionName>
		<dcterms:publisher rdf:resource="http://www.rcahms.gov.uk" />
		<skos:prefLabel xml:lang="en">STEAM TUG</skos:prefLabel>
		<dcterms:issued rdf:datatype="http://www.w3.org/2001/XMLSchema#dateTime">2013-07-17T10:08:39</dcterms:issued>
		<skos:narrower>
			<skos:Concept rdf:about="http://purl.org/heritagedata/schemes/3/concepts/501963">
				<skos:inScheme rdf:resource="http://purl.org/heritagedata/schemes/3" />
				<dcterms:identifier>http://purl.org/heritagedata/schemes/3/concepts/501963</dcterms:identifier>
				<cc:license rdf:resource="http://reference.data.gov.uk/id/open-government-licence" />
				<cc:attributionURL rdf:resource="http://www.rcahms.gov.uk" />
				<cc:attributionName xml:lang="en">RCAHMS</cc:attributionName>
				<dcterms:publisher rdf:resource="http://www.rcahms.gov.uk" />
				<skos:prefLabel xml:lang="en">REQUISITIONED STEAM TUG</skos:prefLabel>
				<dcterms:issued rdf:datatype="http://www.w3.org/2001/XMLSchema#dateTime">2013-07-17T10:08:39</dcterms:issued>
				<skos:broader rdf:resource="http://purl.org/heritagedata/schemes/3/concepts/501998" />
				<skos:scopeNote xml:lang="en">A Steam Tug which has been requisitioned for war service, generally within its local area, with an unchanged crew and with the fitting of only basic armament (if any). Such vessels were used for light transport and fire-fighting as well as towage duties.</skos:scopeNote>
			</skos:Concept>
		</skos:narrower>
		<skos:broader rdf:resource="http://purl.org/heritagedata/schemes/3/concepts/502014" />
		<skos:scopeNote xml:lang="en">A Tug powered by an integral steam engine, which generally transmits its power through a single propellor.</skos:scopeNote>
	</skos:Concept>
	<skos:Concept rdf:about="http://purl.org/heritagedata/schemes/3/concepts/502002">
		<skos:inScheme rdf:resource="http://purl.org/heritagedata/schemes/3" />
		<dcterms:identifier>http://purl.org/heritagedata/schemes/3/concepts/502002</dcterms:identifier>
		<cc:license rdf:resource="http://reference.data.gov.uk/id/open-government-licence" />
		<cc:attributionURL rdf:resource="http://www.rcahms.gov.uk" />
		<cc:attributionName xml:lang="en">RCAHMS</cc:attributionName>
		<dcterms:publisher rdf:resource="http://www.rcahms.gov.uk" />
		<skos:prefLabel xml:lang="en">SUBMARINE</skos:prefLabel>
		<dcterms:issued rdf:datatype="http://www.w3.org/2001/XMLSchema#dateTime">2013-07-17T10:08:39</dcterms:issued>
		<skos:narrower rdf:resource="http://purl.org/heritagedata/schemes/3/concepts/501926" />
		<skos:broader rdf:resource="http://purl.org/heritagedata/schemes/3/concepts/502015" />
		<skos:scopeNote xml:lang="en">A vessel designed to operate below the surface of the sea.</skos:scopeNote>
	</skos:Concept>
	<skos:Concept rdf:about="http://purl.org/heritagedata/schemes/3/concepts/502007">
		<skos:inScheme rdf:resource="http://purl.org/heritagedata/schemes/3" />
		<dcterms:identifier>http://purl.org/heritagedata/schemes/3/concepts/502007</dcterms:identifier>
		<cc:license rdf:resource="http://reference.data.gov.uk/id/open-government-licence" />
		<cc:attributionURL rdf:resource="http://www.rcahms.gov.uk" />
		<cc:attributionName xml:lang="en">RCAHMS</cc:attributionName>
		<dcterms:publisher rdf:resource="http://www.rcahms.gov.uk" />
		<skos:prefLabel xml:lang="en">TANKER</skos:prefLabel>
		<dcterms:issued rdf:datatype="http://www.w3.org/2001/XMLSchema#dateTime">2013-07-17T10:08:39</dcterms:issued>
		<skos:narrower>
			<skos:Concept rdf:about="http://purl.org/heritagedata/schemes/3/concepts/501996">
				<skos:inScheme rdf:resource="http://purl.org/heritagedata/schemes/3" />
				<dcterms:identifier>http://purl.org/heritagedata/schemes/3/concepts/501996</dcterms:identifier>
				<cc:license rdf:resource="http://reference.data.gov.uk/id/open-government-licence" />
				<cc:attributionURL rdf:resource="http://www.rcahms.gov.uk" />
				<cc:attributionName xml:lang="en">RCAHMS</cc:attributionName>
				<dcterms:publisher rdf:resource="http://www.rcahms.gov.uk" />
				<skos:prefLabel xml:lang="en">STEAM TANKER</skos:prefLabel>
				<dcterms:issued rdf:datatype="http://www.w3.org/2001/XMLSchema#dateTime">2013-07-17T10:08:39</dcterms:issued>
				<skos:broader rdf:resource="http://purl.org/heritagedata/schemes/3/concepts/502007" />
				<skos:scopeNote xml:lang="en">A Tanker with integral steam propulsion.</skos:scopeNote>
			</skos:Concept>
		</skos:narrower>
		<skos:broader rdf:resource="http://purl.org/heritagedata/schemes/3/concepts/501857" />
		<skos:scopeNote xml:lang="en">A seagoing vessel built specifically for the bulk carriage of crude oil, petroleum products or chemicals. Such vessels vary considerably in size and form.</skos:scopeNote>
	</skos:Concept>
	<skos:Concept rdf:about="http://purl.org/heritagedata/schemes/3/concepts/502011">
		<skos:inScheme rdf:resource="http://purl.org/heritagedata/schemes/3" />
		<dcterms:identifier>http://purl.org/heritagedata/schemes/3/concepts/502011</dcterms:identifier>
		<cc:license rdf:resource="http://reference.data.gov.uk/id/open-government-licence" />
		<cc:attributionURL rdf:resource="http://www.rcahms.gov.uk" />
		<cc:attributionName xml:lang="en">RCAHMS</cc:attributionName>
		<dcterms:publisher rdf:resource="http://www.rcahms.gov.uk" />
		<skos:prefLabel xml:lang="en">TRANSPORT VESSEL</skos:prefLabel>
		<dcterms:modified rdf:datatype="http://www.w3.org/2001/XMLSchema#dateTime">2011-08-19T09:37:16</dcterms:modified>
		<dcterms:issued rdf:datatype="http://www.w3.org/2001/XMLSchema#dateTime">2013-07-17T10:08:39</dcterms:issued>
		<skos:narrower rdf:resource="http://purl.org/heritagedata/schemes/3/concepts/501857" />
		<skos:broader rdf:resource="http://purl.org/heritagedata/schemes/3/concepts/501925" />
		<skos:scopeNote xml:lang="en">A vessel used for transporting passengers or goods.</skos:scopeNote>
	</skos:Concept>
	<skos:Concept rdf:about="http://purl.org/heritagedata/schemes/3/concepts/502012">
		<skos:inScheme rdf:resource="http://purl.org/heritagedata/schemes/3" />
		<dcterms:identifier>http://purl.org/heritagedata/schemes/3/concepts/502012</dcterms:identifier>
		<cc:license rdf:resource="http://reference.data.gov.uk/id/open-government-licence" />
		<cc:attributionURL rdf:resource="http://www.rcahms.gov.uk" />
		<cc:attributionName xml:lang="en">RCAHMS</cc:attributionName>
		<dcterms:publisher rdf:resource="http://www.rcahms.gov.uk" />
		<skos:prefLabel xml:lang="en">TRAWLER</skos:prefLabel>
		<dcterms:issued rdf:datatype="http://www.w3.org/2001/XMLSchema#dateTime">2013-07-17T10:08:39</dcterms:issued>
		<skos:altLabel xml:lang="en">ADMIRALTY TRAWLER</skos:altLabel>
		<skos:altLabel xml:lang="en">AUXILIARY TRAWLER</skos:altLabel>
		<skos:narrower rdf:resource="http://purl.org/heritagedata/schemes/3/concepts/501938" />
		<skos:narrower>
			<skos:Concept rdf:about="http://purl.org/heritagedata/schemes/3/concepts/501962">
				<skos:inScheme rdf:resource="http://purl.org/heritagedata/schemes/3" />
				<dcterms:identifier>http://purl.org/heritagedata/schemes/3/concepts/501962</dcterms:identifier>
				<cc:license rdf:resource="http://reference.data.gov.uk/id/open-government-licence" />
				<cc:attributionURL rdf:resource="http://www.rcahms.gov.uk" />
				<cc:attributionName xml:lang="en">RCAHMS</cc:attributionName>
				<dcterms:publisher rdf:resource="http://www.rcahms.gov.uk" />
				<skos:prefLabel xml:lang="en">REQUISITIONED STEAM TRAWLER</skos:prefLabel>
				<dcterms:issued rdf:datatype="http://www.w3.org/2001/XMLSchema#dateTime">2013-07-17T10:08:39</dcterms:issued>
				<skos:broader rdf:resource="http://purl.org/heritagedata/schemes/3/concepts/502012" />
				<skos:scopeNote xml:lang="en">A Steam Trawler which has been requisitioned for war service, generally within its local area, with an unchanged crew and with the fitting of only basic armament (if any). Such vessels were used for transport and light towage as well as patrol purposes.</skos:scopeNote>
			</skos:Concept>
		</skos:narrower>
		<skos:narrower>
			<skos:Concept rdf:about="http://purl.org/heritagedata/schemes/3/concepts/501965">
				<skos:inScheme rdf:resource="http://purl.org/heritagedata/schemes/3" />
				<dcterms:identifier>http://purl.org/heritagedata/schemes/3/concepts/501965</dcterms:identifier>
				<cc:license rdf:resource="http://reference.data.gov.uk/id/open-government-licence" />
				<cc:attributionURL rdf:resource="http://www.rcahms.gov.uk" />
				<cc:attributionName xml:lang="en">RCAHMS</cc:attributionName>
				<dcterms:publisher rdf:resource="http://www.rcahms.gov.uk" />
				<skos:prefLabel xml:lang="en">REQUISITIONED TRAWLER</skos:prefLabel>
				<dcterms:issued rdf:datatype="http://www.w3.org/2001/XMLSchema#dateTime">2013-07-17T10:08:39</dcterms:issued>
				<skos:broader rdf:resource="http://purl.org/heritagedata/schemes/3/concepts/502012" />
				<skos:scopeNote xml:lang="en">A Trawler which has been requisitioned for war service, generally within its local area, with an unchanged crew and with the fitting of only basic armament (if any). Such vessels were typically used for transport and target-towing as well as patrol duties.</skos:scopeNote>
			</skos:Concept>
		</skos:narrower>
		<skos:narrower>
			<skos:Concept rdf:about="http://purl.org/heritagedata/schemes/3/concepts/501993">
				<skos:inScheme rdf:resource="http://purl.org/heritagedata/schemes/3" />
				<dcterms:identifier>http://purl.org/heritagedata/schemes/3/concepts/501993</dcterms:identifier>
				<cc:license rdf:resource="http://reference.data.gov.uk/id/open-government-licence" />
				<cc:attributionURL rdf:resource="http://www.rcahms.gov.uk" />
				<cc:attributionName xml:lang="en">RCAHMS</cc:attributionName>
				<dcterms:publisher rdf:resource="http://www.rcahms.gov.uk" />
				<skos:prefLabel xml:lang="en">STEAM PADDLE TRAWLER</skos:prefLabel>
				<dcterms:issued rdf:datatype="http://www.w3.org/2001/XMLSchema#dateTime">2013-07-17T10:08:39</dcterms:issued>
				<skos:broader rdf:resource="http://purl.org/heritagedata/schemes/3/concepts/502012" />
				<skos:scopeNote xml:lang="en">A Trawler powered by an integral steam engine which transmits its power through side-paddles.</skos:scopeNote>
			</skos:Concept>
		</skos:narrower>
		<skos:narrower>
			<skos:Concept rdf:about="http://purl.org/heritagedata/schemes/3/concepts/501997">
				<skos:inScheme rdf:resource="http://purl.org/heritagedata/schemes/3" />
				<dcterms:identifier>http://purl.org/heritagedata/schemes/3/concepts/501997</dcterms:identifier>
				<cc:license rdf:resource="http://reference.data.gov.uk/id/open-government-licence" />
				<cc:attributionURL rdf:resource="http://www.rcahms.gov.uk" />
				<cc:attributionName xml:lang="en">RCAHMS</cc:attributionName>
				<dcterms:publisher rdf:resource="http://www.rcahms.gov.uk" />
				<skos:prefLabel xml:lang="en">STEAM TRAWLER</skos:prefLabel>
				<dcterms:issued rdf:datatype="http://www.w3.org/2001/XMLSchema#dateTime">2013-07-17T10:08:39</dcterms:issued>
				<skos:broader rdf:resource="http://purl.org/heritagedata/schemes/3/concepts/502012" />
				<skos:scopeNote xml:lang="en">A Trawler with integral steam propulsion.</skos:scopeNote>
			</skos:Concept>
		</skos:narrower>
		<skos:broader rdf:resource="http://purl.org/heritagedata/schemes/3/concepts/501889" />
		<skos:scopeNote xml:lang="en">A fishing vessel specially designed to operate and trawl for the catching of bottom lying fish. Use with power where known.</skos:scopeNote>
	</skos:Concept>
	<skos:Concept rdf:about="http://purl.org/heritagedata/schemes/3/concepts/502013">
		<skos:inScheme rdf:resource="http://purl.org/heritagedata/schemes/3" />
		<dcterms:identifier>http://purl.org/heritagedata/schemes/3/concepts/502013</dcterms:identifier>
		<cc:license rdf:resource="http://reference.data.gov.uk/id/open-government-licence" />
		<cc:attributionURL rdf:resource="http://www.rcahms.gov.uk" />
		<cc:attributionName xml:lang="en">RCAHMS</cc:attributionName>
		<dcterms:publisher rdf:resource="http://www.rcahms.gov.uk" />
		<skos:prefLabel xml:lang="en">TRINITY HOUSE VESSEL</skos:prefLabel>
		<dcterms:issued rdf:datatype="http://www.w3.org/2001/XMLSchema#dateTime">2013-07-17T10:08:39</dcterms:issued>
		<skos:narrower>
			<skos:Concept rdf:about="http://purl.org/heritagedata/schemes/3/concepts/501921">
				<skos:inScheme rdf:resource="http://purl.org/heritagedata/schemes/3" />
				<dcterms:identifier>http://purl.org/heritagedata/schemes/3/concepts/501921</dcterms:identifier>
				<cc:license rdf:resource="http://reference.data.gov.uk/id/open-government-licence" />
				<cc:attributionURL rdf:resource="http://www.rcahms.gov.uk" />
				<cc:attributionName xml:lang="en">RCAHMS</cc:attributionName>
				<dcterms:publisher rdf:resource="http://www.rcahms.gov.uk" />
				<skos:prefLabel xml:lang="en">LIGHTSHIP</skos:prefLabel>
				<dcterms:issued rdf:datatype="http://www.w3.org/2001/XMLSchema#dateTime">2013-07-17T10:08:39</dcterms:issued>
				<skos:broader rdf:resource="http://purl.org/heritagedata/schemes/3/concepts/502013" />
				<skos:scopeNote xml:lang="en">Normally an unpowered vessel, moored in places where the construction of a lighthouse is impractical.</skos:scopeNote>
			</skos:Concept>
		</skos:narrower>
		<skos:broader rdf:resource="http://purl.org/heritagedata/schemes/3/concepts/501925" />
		<skos:scopeNote xml:lang="en">Any vessel operated by Trinity house masters and brethren in the maintenance of lighthouses, lightships, buoys and other navigation aids.</skos:scopeNote>
	</skos:Concept>
	<skos:Concept rdf:about="http://purl.org/heritagedata/schemes/3/concepts/502014">
		<skos:inScheme rdf:resource="http://purl.org/heritagedata/schemes/3" />
		<dcterms:identifier>http://purl.org/heritagedata/schemes/3/concepts/502014</dcterms:identifier>
		<cc:license rdf:resource="http://reference.data.gov.uk/id/open-government-licence" />
		<cc:attributionURL rdf:resource="http://www.rcahms.gov.uk" />
		<cc:attributionName xml:lang="en">RCAHMS</cc:attributionName>
		<dcterms:publisher rdf:resource="http://www.rcahms.gov.uk" />
		<skos:prefLabel xml:lang="en">TUG</skos:prefLabel>
		<dcterms:issued rdf:datatype="http://www.w3.org/2001/XMLSchema#dateTime">2013-07-17T10:08:39</dcterms:issued>
		<skos:narrower>
			<skos:Concept rdf:about="http://purl.org/heritagedata/schemes/3/concepts/501994">
				<skos:inScheme rdf:resource="http://purl.org/heritagedata/schemes/3" />
				<dcterms:identifier>http://purl.org/heritagedata/schemes/3/concepts/501994</dcterms:identifier>
				<cc:license rdf:resource="http://reference.data.gov.uk/id/open-government-licence" />
				<cc:attributionURL rdf:resource="http://www.rcahms.gov.uk" />
				<cc:attributionName xml:lang="en">RCAHMS</cc:attributionName>
				<dcterms:publisher rdf:resource="http://www.rcahms.gov.uk" />
				<skos:prefLabel xml:lang="en">STEAM PADDLE TUG</skos:prefLabel>
				<dcterms:issued rdf:datatype="http://www.w3.org/2001/XMLSchema#dateTime">2013-07-17T10:08:39</dcterms:issued>
				<skos:broader rdf:resource="http://purl.org/heritagedata/schemes/3/concepts/502014" />
				<skos:scopeNote xml:lang="en">ATug powered by an integral steam engine which transmits its power through side-paddles.</skos:scopeNote>
			</skos:Concept>
		</skos:narrower>
		<skos:narrower rdf:resource="http://purl.org/heritagedata/schemes/3/concepts/501998" />
		<skos:broader rdf:resource="http://purl.org/heritagedata/schemes/3/concepts/501898" />
		<skos:scopeNote xml:lang="en">A service craft built to provide an independent source of propulsion for other vessels, specifically for those disabled by breakdown, those built as dumb vessels, and for sailing vessels becalmed by lack of wind or short of a crew. Although once propelled by oars or sweeps, steam and later diesel power were adopted at the earliest possible date on grounds of efficiency.
Tugs may be divided into those optimised for manoeuvrability within harbours and those incorporating power for long-distance towing. The former commonly formerly used paddles, but now regularly incorporate specialised power transfer systems (Schneider propellers and Kort nozzles) operating under automatic control. Both types may be fitted with firefighting equipment and/or helicopter platforms</skos:scopeNote>
	</skos:Concept>
	<skos:Concept rdf:about="http://purl.org/heritagedata/schemes/3/concepts/502015">
		<skos:inScheme rdf:resource="http://purl.org/heritagedata/schemes/3" />
		<dcterms:identifier>http://purl.org/heritagedata/schemes/3/concepts/502015</dcterms:identifier>
		<cc:license rdf:resource="http://reference.data.gov.uk/id/open-government-licence" />
		<cc:attributionURL rdf:resource="http://www.rcahms.gov.uk" />
		<cc:attributionName xml:lang="en">RCAHMS</cc:attributionName>
		<dcterms:publisher rdf:resource="http://www.rcahms.gov.uk" />
		<skos:prefLabel xml:lang="en">WARSHIP</skos:prefLabel>
		<dcterms:modified rdf:datatype="http://www.w3.org/2001/XMLSchema#dateTime">2012-12-04T11:48:39</dcterms:modified>
		<dcterms:issued rdf:datatype="http://www.w3.org/2001/XMLSchema#dateTime">2013-07-17T10:08:39</dcterms:issued>
		<skos:narrower>
			<skos:Concept rdf:about="http://purl.org/heritagedata/schemes/3/concepts/501827">
				<skos:inScheme rdf:resource="http://purl.org/heritagedata/schemes/3" />
				<dcterms:identifier>http://purl.org/heritagedata/schemes/3/concepts/501827</dcterms:identifier>
				<cc:license rdf:resource="http://reference.data.gov.uk/id/open-government-licence" />
				<cc:attributionURL rdf:resource="http://www.rcahms.gov.uk" />
				<cc:attributionName xml:lang="en">RCAHMS</cc:attributionName>
				<dcterms:publisher rdf:resource="http://www.rcahms.gov.uk" />
				<skos:prefLabel xml:lang="en">AIRCRAFT CARRIER</skos:prefLabel>
				<dcterms:issued rdf:datatype="http://www.w3.org/2001/XMLSchema#dateTime">2013-07-17T10:08:39</dcterms:issued>
				<skos:broader rdf:resource="http://purl.org/heritagedata/schemes/3/concepts/502015" />
				<skos:scopeNote xml:lang="en">A warship specialised for the carriage of aircraft, and characterised by a flat upper deck for launch and landing while under way. Ships of this vary considerably in role, equipment and size, being usually designed for the operation of a narrow range of aircraft. Seaplane Carriers, which craned aircraft outboard to launch and recover from the sea, may be placed within this category, but not those modern warships and auxiliaries which carry a helicopter as part of a more generalised equipment fit.</skos:scopeNote>
			</skos:Concept>
		</skos:narrower>
		<skos:narrower>
			<skos:Concept rdf:about="http://purl.org/heritagedata/schemes/3/concepts/501844">
				<skos:inScheme rdf:resource="http://purl.org/heritagedata/schemes/3" />
				<dcterms:identifier>http://purl.org/heritagedata/schemes/3/concepts/501844</dcterms:identifier>
				<cc:license rdf:resource="http://reference.data.gov.uk/id/open-government-licence" />
				<cc:attributionURL rdf:resource="http://www.rcahms.gov.uk" />
				<cc:attributionName xml:lang="en">RCAHMS</cc:attributionName>
				<dcterms:publisher rdf:resource="http://www.rcahms.gov.uk" />
				<skos:prefLabel xml:lang="en">BATTLECRUISER</skos:prefLabel>
				<dcterms:issued rdf:datatype="http://www.w3.org/2001/XMLSchema#dateTime">2013-07-17T10:08:39</dcterms:issued>
				<skos:broader rdf:resource="http://purl.org/heritagedata/schemes/3/concepts/502015" />
				<skos:scopeNote xml:lang="en">A specialised armoured large warship built around steam propulsion and heavy guns, optimised for firepower and speed rather than protection. Successor to the Ship of the Line or Line-of-battle Ship of the classic sailing navy: not to be confused with the Battleship</skos:scopeNote>
			</skos:Concept>
		</skos:narrower>
		<skos:narrower>
			<skos:Concept rdf:about="http://purl.org/heritagedata/schemes/3/concepts/501845">
				<skos:inScheme>
					<skos:ConceptScheme rdf:about="http://purl.org/heritagedata/schemes/3">
						<dcterms:identifier>http://purl.org/heritagedata/schemes/3</dcterms:identifier>
						<cc:license rdf:resource="http://reference.data.gov.uk/id/open-government-licence" />
						<cc:attributionURL rdf:resource="http://www.rcahms.gov.uk" />
						<cc:attributionName xml:lang="en">RCAHMS</cc:attributionName>
						<dcterms:title xml:lang="en">Maritime Craft Thesaurus (Scotland)</dcterms:title>
						<rdfs:label xml:lang="en">Maritime Craft Thesaurus (Scotland)</rdfs:label>
						<dcterms:description xml:lang="en">Types of craft that survive as wrecks, or are documented as losses, in Scottish maritime waters.</dcterms:description>
						<dcterms:created rdf:datatype="http://www.w3.org/2001/XMLSchema#dateTime">2007-04-23T18:00:29</dcterms:created>
						<dcterms:modified rdf:datatype="http://www.w3.org/2001/XMLSchema#dateTime">2012-12-04T11:48:39</dcterms:modified>
						<dcterms:publisher rdf:resource="http://www.rcahms.gov.uk" />
						<dcterms:issued rdf:datatype="http://www.w3.org/2001/XMLSchema#dateTime">2013-07-17T10:08:38</dcterms:issued>
						<skos:hasTopConcept rdf:resource="http://purl.org/heritagedata/schemes/3/concepts/501925" />
					</skos:ConceptScheme>
				</skos:inScheme>
				<dcterms:identifier>http://purl.org/heritagedata/schemes/3/concepts/501845</dcterms:identifier>
				<cc:license rdf:resource="http://reference.data.gov.uk/id/open-government-licence" />
				<cc:attributionURL rdf:resource="http://www.rcahms.gov.uk" />
				<cc:attributionName xml:lang="en">RCAHMS</cc:attributionName>
				<dcterms:publisher rdf:resource="http://www.rcahms.gov.uk" />
				<skos:prefLabel xml:lang="en">BATTLESHIP</skos:prefLabel>
				<dcterms:issued rdf:datatype="http://www.w3.org/2001/XMLSchema#dateTime">2013-07-17T10:08:39</dcterms:issued>
				<skos:broader rdf:resource="http://purl.org/heritagedata/schemes/3/concepts/502015" />
				<skos:scopeNote xml:lang="en">A specialised armoured large warship built around steam propulsion and heavy guns, optimised for firepower and protection rather than speed. Successor to the Ship of the Line or Line-of-battle Ship of the classic sailing navy: not to be confused with the Battlecruiser</skos:scopeNote>
			</skos:Concept>
		</skos:narrower>
		<skos:narrower>
			<skos:Concept rdf:about="http://purl.org/heritagedata/schemes/3/concepts/501862">
				<skos:inScheme rdf:resource="http://purl.org/heritagedata/schemes/3" />
				<dcterms:identifier>http://purl.org/heritagedata/schemes/3/concepts/501862</dcterms:identifier>
				<cc:license rdf:resource="http://reference.data.gov.uk/id/open-government-licence" />
				<cc:attributionURL rdf:resource="http://www.rcahms.gov.uk" />
				<cc:attributionName xml:lang="en">RCAHMS</cc:attributionName>
				<dcterms:publisher rdf:resource="http://www.rcahms.gov.uk" />
				<skos:prefLabel xml:lang="en">CORVETTE</skos:prefLabel>
				<dcterms:modified rdf:datatype="http://www.w3.org/2001/XMLSchema#dateTime">2007-04-24T14:35:39</dcterms:modified>
				<dcterms:issued rdf:datatype="http://www.w3.org/2001/XMLSchema#dateTime">2013-07-17T10:08:39</dcterms:issued>
				<skos:broader rdf:resource="http://purl.org/heritagedata/schemes/3/concepts/502015" />
				<skos:scopeNote xml:lang="en">A small general-purpose warship built around diesel, steam or gas turbine propulsion and carrying a range of weaponry, typically optimised for anti-submarine operations. Vessels of this type are now distinguished from Frigates by not carrying a helicopter, Warships of this type have traditionally tended to operate as part of larger formations rather than independently.</skos:scopeNote>
			</skos:Concept>
		</skos:narrower>
		<skos:narrower>
			<skos:Concept rdf:about="http://purl.org/heritagedata/schemes/3/concepts/501864">
				<skos:inScheme rdf:resource="http://purl.org/heritagedata/schemes/3" />
				<dcterms:identifier>http://purl.org/heritagedata/schemes/3/concepts/501864</dcterms:identifier>
				<cc:license rdf:resource="http://reference.data.gov.uk/id/open-government-licence" />
				<cc:attributionURL rdf:resource="http://www.rcahms.gov.uk" />
				<cc:attributionName xml:lang="en">RCAHMS</cc:attributionName>
				<dcterms:publisher rdf:resource="http://www.rcahms.gov.uk" />
				<skos:prefLabel xml:lang="en">CRUISER</skos:prefLabel>
				<dcterms:modified rdf:datatype="http://www.w3.org/2001/XMLSchema#dateTime">2007-04-24T14:36:13</dcterms:modified>
				<dcterms:issued rdf:datatype="http://www.w3.org/2001/XMLSchema#dateTime">2013-07-17T10:08:39</dcterms:issued>
				<skos:broader rdf:resource="http://purl.org/heritagedata/schemes/3/concepts/502015" />
				<skos:scopeNote xml:lang="en">A generalised warship of considerable size built around steam or gas turbine propulsion and carrying a range of weaponry. Vessels of this type have traditionally been the norm in the Royal Navy on account of their ability to operate effectively either independently or as part of a larger formation. In consequence, they have varied widely in size between classes, notably in size, gun calibre and the degree of armour protection. They have rarely been fitted for anti-submarine operations.</skos:scopeNote>
			</skos:Concept>
		</skos:narrower>
		<skos:narrower>
			<skos:Concept rdf:about="http://purl.org/heritagedata/schemes/3/concepts/501870">
				<skos:inScheme rdf:resource="http://purl.org/heritagedata/schemes/3" />
				<dcterms:identifier>http://purl.org/heritagedata/schemes/3/concepts/501870</dcterms:identifier>
				<cc:license rdf:resource="http://reference.data.gov.uk/id/open-government-licence" />
				<cc:attributionURL rdf:resource="http://www.rcahms.gov.uk" />
				<cc:attributionName xml:lang="en">RCAHMS</cc:attributionName>
				<dcterms:publisher rdf:resource="http://www.rcahms.gov.uk" />
				<skos:prefLabel xml:lang="en">DESTROYER</skos:prefLabel>
				<dcterms:modified rdf:datatype="http://www.w3.org/2001/XMLSchema#dateTime">2007-04-24T14:36:43</dcterms:modified>
				<dcterms:issued rdf:datatype="http://www.w3.org/2001/XMLSchema#dateTime">2013-07-17T10:08:39</dcterms:issued>
				<skos:broader rdf:resource="http://purl.org/heritagedata/schemes/3/concepts/502015" />
				<skos:scopeNote xml:lang="en">a medium-sized warship built around steam or gas turbine propulsion and carrying a range of weaponry. Vessels of this type have varied considerably across the 20th century, being originally designed as specialised fast craft with a heavy torpedo armament. In recent years, the term has come to denote a generalised warship designed around a long-range (area defence) anti-aircraft missile system, and carrying a helicopter for anti-submarine operations.Warships of this type have traditionally tended to operate as part of larger formations rather than independently, being similar to Frigates in this respect.</skos:scopeNote>
			</skos:Concept>
		</skos:narrower>
		<skos:narrower rdf:resource="http://purl.org/heritagedata/schemes/3/concepts/501881" />
		<skos:narrower rdf:resource="http://purl.org/heritagedata/schemes/3/concepts/501913" />
		<skos:narrower>
			<skos:Concept rdf:about="http://purl.org/heritagedata/schemes/3/concepts/501927">
				<skos:inScheme rdf:resource="http://purl.org/heritagedata/schemes/3" />
				<dcterms:identifier>http://purl.org/heritagedata/schemes/3/concepts/501927</dcterms:identifier>
				<cc:license rdf:resource="http://reference.data.gov.uk/id/open-government-licence" />
				<cc:attributionURL rdf:resource="http://www.rcahms.gov.uk" />
				<cc:attributionName xml:lang="en">RCAHMS</cc:attributionName>
				<dcterms:publisher rdf:resource="http://www.rcahms.gov.uk" />
				<skos:prefLabel xml:lang="en">MINELAYER</skos:prefLabel>
				<dcterms:issued rdf:datatype="http://www.w3.org/2001/XMLSchema#dateTime">2013-07-17T10:08:39</dcterms:issued>
				<skos:broader rdf:resource="http://purl.org/heritagedata/schemes/3/concepts/502015" />
				<skos:scopeNote xml:lang="en">A specialised warship or naval auxiliary constructed for the transport and laying of mines, which are generally carried on rails laid internally the length and launched through doors at the stern. Three types may be recognised, the most common being the Mine Transport or Exercise Minelayer which is relatively slow, small and unarmed, and is used to lay defensive minefields in waters not subject to enemy threat. Vessels of this type have frequently been converted from merchant service. Fast Minelayers and Submarine Minelayers were used to lay mines covertly in enemy waters; these types are not represented in Scottish waters.</skos:scopeNote>
			</skos:Concept>
		</skos:narrower>
		<skos:narrower>
			<skos:Concept rdf:about="http://purl.org/heritagedata/schemes/3/concepts/501928">
				<skos:inScheme rdf:resource="http://purl.org/heritagedata/schemes/3" />
				<dcterms:identifier>http://purl.org/heritagedata/schemes/3/concepts/501928</dcterms:identifier>
				<cc:license rdf:resource="http://reference.data.gov.uk/id/open-government-licence" />
				<cc:attributionURL rdf:resource="http://www.rcahms.gov.uk" />
				<cc:attributionName xml:lang="en">RCAHMS</cc:attributionName>
				<dcterms:publisher rdf:resource="http://www.rcahms.gov.uk" />
				<skos:prefLabel xml:lang="en">MINESWEEPER</skos:prefLabel>
				<dcterms:issued rdf:datatype="http://www.w3.org/2001/XMLSchema#dateTime">2013-07-17T10:08:39</dcterms:issued>
				<skos:broader rdf:resource="http://purl.org/heritagedata/schemes/3/concepts/502015" />
				<skos:scopeNote xml:lang="en">A vessel designed or adapted to sweep and explode mines laid at sea.</skos:scopeNote>
			</skos:Concept>
		</skos:narrower>
		<skos:narrower>
			<skos:Concept rdf:about="http://purl.org/heritagedata/schemes/3/concepts/501937">
				<skos:inScheme rdf:resource="http://purl.org/heritagedata/schemes/3" />
				<dcterms:identifier>http://purl.org/heritagedata/schemes/3/concepts/501937</dcterms:identifier>
				<cc:license rdf:resource="http://reference.data.gov.uk/id/open-government-licence" />
				<cc:attributionURL rdf:resource="http://www.rcahms.gov.uk" />
				<cc:attributionName xml:lang="en">RCAHMS</cc:attributionName>
				<dcterms:publisher rdf:resource="http://www.rcahms.gov.uk" />
				<skos:prefLabel xml:lang="en">MOTOR TORPEDO BOAT</skos:prefLabel>
				<dcterms:issued rdf:datatype="http://www.w3.org/2001/XMLSchema#dateTime">2013-07-17T10:08:39</dcterms:issued>
				<skos:broader rdf:resource="http://purl.org/heritagedata/schemes/3/concepts/502015" />
				<skos:scopeNote xml:lang="en">A fast but lightweight coastal warship (typically of planing hull form and wooden construction) intended to pose a specialised threat to heavier warships within a restricted range of operation.</skos:scopeNote>
			</skos:Concept>
		</skos:narrower>
		<skos:narrower rdf:resource="http://purl.org/heritagedata/schemes/3/concepts/501979" />
		<skos:narrower rdf:resource="http://purl.org/heritagedata/schemes/3/concepts/502002" />
		<skos:broader rdf:resource="http://purl.org/heritagedata/schemes/3/concepts/501925" />
		<skos:narrower>
			<skos:Concept rdf:about="http://purl.org/heritagedata/schemes/3/concepts/506541">
				<skos:inScheme rdf:resource="http://purl.org/heritagedata/schemes/3" />
				<dcterms:identifier>http://purl.org/heritagedata/schemes/3/concepts/506541</dcterms:identifier>
				<cc:license rdf:resource="http://reference.data.gov.uk/id/open-government-licence" />
				<cc:attributionURL rdf:resource="http://www.rcahms.gov.uk" />
				<cc:attributionName xml:lang="en">RCAHMS</cc:attributionName>
				<dcterms:publisher rdf:resource="http://www.rcahms.gov.uk" />
				<skos:prefLabel xml:lang="en">MOTOR GUN BOAT</skos:prefLabel>
				<dcterms:created rdf:datatype="http://www.w3.org/2001/XMLSchema#dateTime">2012-03-20T09:07:53</dcterms:created>
				<dcterms:modified rdf:datatype="http://www.w3.org/2001/XMLSchema#dateTime">2012-03-20T09:08:25</dcterms:modified>
				<dcterms:issued rdf:datatype="http://www.w3.org/2001/XMLSchema#dateTime">2013-07-17T10:08:39</dcterms:issued>
				<skos:broader rdf:resource="http://purl.org/heritagedata/schemes/3/concepts/502015" />
				<skos:scopeNote xml:lang="en">A specialised fast but lightweight coastal warship (typically of planing hull form and wooden construction) armed with heavy cannon and intended to pose a threat to heavier warships within a restricted range of operation.</skos:scopeNote>
			</skos:Concept>
		</skos:narrower>
		<skos:narrower>
			<skos:Concept rdf:about="http://purl.org/heritagedata/schemes/3/concepts/505901">
				<skos:inScheme rdf:resource="http://purl.org/heritagedata/schemes/3" />
				<dcterms:identifier>http://purl.org/heritagedata/schemes/3/concepts/505901</dcterms:identifier>
				<cc:license rdf:resource="http://reference.data.gov.uk/id/open-government-licence" />
				<cc:attributionURL rdf:resource="http://www.rcahms.gov.uk" />
				<cc:attributionName xml:lang="en">RCAHMS</cc:attributionName>
				<dcterms:publisher rdf:resource="http://www.rcahms.gov.uk" />
				<skos:prefLabel xml:lang="en">ARMED SCHOONER</skos:prefLabel>
				<dcterms:created rdf:datatype="http://www.w3.org/2001/XMLSchema#dateTime">2011-06-14T12:06:16</dcterms:created>
				<dcterms:modified rdf:datatype="http://www.w3.org/2001/XMLSchema#dateTime">2011-06-14T12:07:05</dcterms:modified>
				<dcterms:issued rdf:datatype="http://www.w3.org/2001/XMLSchema#dateTime">2013-07-17T10:08:39</dcterms:issued>
				<skos:broader rdf:resource="http://purl.org/heritagedata/schemes/3/concepts/502015" />
				<skos:scopeNote xml:lang="en">A schooner-rigged vessel armed (typically with about eight guns) as a light warship in commissioned service.</skos:scopeNote>
			</skos:Concept>
		</skos:narrower>
		<skos:narrower rdf:resource="http://purl.org/heritagedata/schemes/3/concepts/503372" />
		<skos:scopeNote xml:lang="en">A ship that is built and primarily intended for war.</skos:scopeNote>
	</skos:Concept>
	<skos:Concept rdf:about="http://purl.org/heritagedata/schemes/3/concepts/502016">
		<skos:inScheme rdf:resource="http://purl.org/heritagedata/schemes/3" />
		<dcterms:identifier>http://purl.org/heritagedata/schemes/3/concepts/502016</dcterms:identifier>
		<cc:license rdf:resource="http://reference.data.gov.uk/id/open-government-licence" />
		<cc:attributionURL rdf:resource="http://www.rcahms.gov.uk" />
		<cc:attributionName xml:lang="en">RCAHMS</cc:attributionName>
		<dcterms:publisher rdf:resource="http://www.rcahms.gov.uk" />
		<skos:prefLabel xml:lang="en">WHALER</skos:prefLabel>
		<dcterms:modified rdf:datatype="http://www.w3.org/2001/XMLSchema#dateTime">2007-04-24T12:08:17</dcterms:modified>
		<dcterms:issued rdf:datatype="http://www.w3.org/2001/XMLSchema#dateTime">2013-07-17T10:08:39</dcterms:issued>
		<skos:broader rdf:resource="http://purl.org/heritagedata/schemes/3/concepts/501889" />
		<skos:related rdf:resource="http://purl.org/heritagedata/schemes/3/concepts/505281" />
		<skos:scopeNote xml:lang="en">This term denotes a specialised vessel of very heavy (ice-resistant) timber construction built to hunt and process whales in Arctic whalers. They were normally rigged as brigs but auxiliary steam engines were commonly fitted. RRS Discovery (in preservation at Dundee) exemplifies the type.
The terms Whaling Ship or Whaling Vessel have also been applied to this class of vessel, which should be differentiated from the larger and whale catchers, factory ships and transport ships of steel construction built for Antarctic whaling in the mid 20th century.
The use of the term to describe a double-banked pulling craft in naval service is inapplicable.</skos:scopeNote>
	</skos:Concept>
	<skos:Concept rdf:about="http://purl.org/heritagedata/schemes/3/concepts/502017">
		<skos:inScheme rdf:resource="http://purl.org/heritagedata/schemes/3" />
		<dcterms:identifier>http://purl.org/heritagedata/schemes/3/concepts/502017</dcterms:identifier>
		<cc:license rdf:resource="http://reference.data.gov.uk/id/open-government-licence" />
		<cc:attributionURL rdf:resource="http://www.rcahms.gov.uk" />
		<cc:attributionName xml:lang="en">RCAHMS</cc:attributionName>
		<dcterms:publisher rdf:resource="http://www.rcahms.gov.uk" />
		<skos:prefLabel xml:lang="en">WHERRY</skos:prefLabel>
		<dcterms:issued rdf:datatype="http://www.w3.org/2001/XMLSchema#dateTime">2013-07-17T10:08:39</dcterms:issued>
		<skos:narrower>
			<skos:Concept rdf:about="http://purl.org/heritagedata/schemes/3/concepts/501999">
				<skos:inScheme rdf:resource="http://purl.org/heritagedata/schemes/3" />
				<dcterms:identifier>http://purl.org/heritagedata/schemes/3/concepts/501999</dcterms:identifier>
				<cc:license rdf:resource="http://reference.data.gov.uk/id/open-government-licence" />
				<cc:attributionURL rdf:resource="http://www.rcahms.gov.uk" />
				<cc:attributionName xml:lang="en">RCAHMS</cc:attributionName>
				<dcterms:publisher rdf:resource="http://www.rcahms.gov.uk" />
				<skos:prefLabel xml:lang="en">STEAM WHERRY</skos:prefLabel>
				<dcterms:issued rdf:datatype="http://www.w3.org/2001/XMLSchema#dateTime">2013-07-17T10:08:39</dcterms:issued>
				<skos:broader rdf:resource="http://purl.org/heritagedata/schemes/3/concepts/502017" />
				<skos:scopeNote xml:lang="en">In the absence of preserved or recorded Scottish examples the usage of this term within Scottish waters remains unclear. It presumably describes a variant of the Wherry having an inbuilt steam engine.</skos:scopeNote>
			</skos:Concept>
		</skos:narrower>
		<skos:broader rdf:resource="http://purl.org/heritagedata/schemes/3/concepts/501968" />
		<skos:scopeNote xml:lang="en">In the absence of preserved or recorded Scottish examples the usage of this term within Scottish waters remains unclear. It probably describes a decked sailing vessel of shallow draught and beamy form used to carry cargo in rivers and estuaries. The term is particularly associated with Eastern England (specifically, the Norfolk Broads) where the type is characterised by having a single mast which carries a large loose-footed gaff mainsail and can be easily lowered to pass under bridges.</skos:scopeNote>
	</skos:Concept>
	<skos:Concept rdf:about="http://purl.org/heritagedata/schemes/3/concepts/502018">
		<skos:inScheme rdf:resource="http://purl.org/heritagedata/schemes/3" />
		<dcterms:identifier>http://purl.org/heritagedata/schemes/3/concepts/502018</dcterms:identifier>
		<cc:license rdf:resource="http://reference.data.gov.uk/id/open-government-licence" />
		<cc:attributionURL rdf:resource="http://www.rcahms.gov.uk" />
		<cc:attributionName xml:lang="en">RCAHMS</cc:attributionName>
		<dcterms:publisher rdf:resource="http://www.rcahms.gov.uk" />
		<skos:prefLabel xml:lang="en">YACHT</skos:prefLabel>
		<dcterms:issued rdf:datatype="http://www.w3.org/2001/XMLSchema#dateTime">2013-07-17T10:08:39</dcterms:issued>
		<skos:narrower>
			<skos:Concept rdf:about="http://purl.org/heritagedata/schemes/3/concepts/501940">
				<skos:inScheme rdf:resource="http://purl.org/heritagedata/schemes/3" />
				<dcterms:identifier>http://purl.org/heritagedata/schemes/3/concepts/501940</dcterms:identifier>
				<cc:license rdf:resource="http://reference.data.gov.uk/id/open-government-licence" />
				<cc:attributionURL rdf:resource="http://www.rcahms.gov.uk" />
				<cc:attributionName xml:lang="en">RCAHMS</cc:attributionName>
				<dcterms:publisher rdf:resource="http://www.rcahms.gov.uk" />
				<skos:prefLabel xml:lang="en">MOTOR YACHT</skos:prefLabel>
				<dcterms:issued rdf:datatype="http://www.w3.org/2001/XMLSchema#dateTime">2013-07-17T10:08:39</dcterms:issued>
				<skos:broader rdf:resource="http://purl.org/heritagedata/schemes/3/concepts/502018" />
				<skos:scopeNote xml:lang="en">A vessel (sometimes of considerable size and sophistication, and usually with onboard accommodation) used for recreation, typically with a paid crew.</skos:scopeNote>
			</skos:Concept>
		</skos:narrower>
		<skos:narrower>
			<skos:Concept rdf:about="http://purl.org/heritagedata/schemes/3/concepts/501964">
				<skos:inScheme rdf:resource="http://purl.org/heritagedata/schemes/3" />
				<dcterms:identifier>http://purl.org/heritagedata/schemes/3/concepts/501964</dcterms:identifier>
				<cc:license rdf:resource="http://reference.data.gov.uk/id/open-government-licence" />
				<cc:attributionURL rdf:resource="http://www.rcahms.gov.uk" />
				<cc:attributionName xml:lang="en">RCAHMS</cc:attributionName>
				<dcterms:publisher rdf:resource="http://www.rcahms.gov.uk" />
				<skos:prefLabel xml:lang="en">REQUISITIONED STEAM YACHT</skos:prefLabel>
				<dcterms:issued rdf:datatype="http://www.w3.org/2001/XMLSchema#dateTime">2013-07-17T10:08:39</dcterms:issued>
				<skos:broader rdf:resource="http://purl.org/heritagedata/schemes/3/concepts/502018" />
				<skos:scopeNote xml:lang="en">A Steam Yacht which has been requisitioned for war service, generally within its local area, with an unchanged crew and with the fitting of only basic armament (if any). Such vessels were used for transport and light towage as well as patrol purposes.</skos:scopeNote>
			</skos:Concept>
		</skos:narrower>
		<skos:narrower>
			<skos:Concept rdf:about="http://purl.org/heritagedata/schemes/3/concepts/502000">
				<skos:inScheme rdf:resource="http://purl.org/heritagedata/schemes/3" />
				<dcterms:identifier>http://purl.org/heritagedata/schemes/3/concepts/502000</dcterms:identifier>
				<cc:license rdf:resource="http://reference.data.gov.uk/id/open-government-licence" />
				<cc:attributionURL rdf:resource="http://www.rcahms.gov.uk" />
				<cc:attributionName xml:lang="en">RCAHMS</cc:attributionName>
				<dcterms:publisher rdf:resource="http://www.rcahms.gov.uk" />
				<skos:prefLabel xml:lang="en">STEAM YACHT</skos:prefLabel>
				<dcterms:issued rdf:datatype="http://www.w3.org/2001/XMLSchema#dateTime">2013-07-17T10:08:39</dcterms:issued>
				<skos:broader rdf:resource="http://purl.org/heritagedata/schemes/3/concepts/502018" />
				<skos:scopeNote xml:lang="en">A vessel (frequently of considerable size and sophistication, and usually with onboard accommodation) used for recreation, typically with a paid crew and most notably by the Edwardian plutocracy.</skos:scopeNote>
			</skos:Concept>
		</skos:narrower>
		<skos:broader rdf:resource="http://purl.org/heritagedata/schemes/3/concepts/501968" />
		<skos:broader rdf:resource="http://purl.org/heritagedata/schemes/3/concepts/501956" />
		<skos:scopeNote xml:lang="en">Any vessel propelled by sail or power and used for pleasure and not plying for hire.</skos:scopeNote>
	</skos:Concept>
	<skos:Concept rdf:about="http://purl.org/heritagedata/schemes/3/concepts/502019">
		<skos:inScheme rdf:resource="http://purl.org/heritagedata/schemes/3" />
		<dcterms:identifier>http://purl.org/heritagedata/schemes/3/concepts/502019</dcterms:identifier>
		<cc:license rdf:resource="http://reference.data.gov.uk/id/open-government-licence" />
		<cc:attributionURL rdf:resource="http://www.rcahms.gov.uk" />
		<cc:attributionName xml:lang="en">RCAHMS</cc:attributionName>
		<dcterms:publisher rdf:resource="http://www.rcahms.gov.uk" />
		<skos:prefLabel xml:lang="en">YAWL</skos:prefLabel>
		<dcterms:issued rdf:datatype="http://www.w3.org/2001/XMLSchema#dateTime">2013-07-17T10:08:39</dcterms:issued>
		<skos:broader rdf:resource="http://purl.org/heritagedata/schemes/3/concepts/501968" />
		<skos:narrower>
			<skos:Concept rdf:about="http://purl.org/heritagedata/schemes/3/concepts/502231">
				<skos:inScheme rdf:resource="http://purl.org/heritagedata/schemes/3" />
				<dcterms:identifier>http://purl.org/heritagedata/schemes/3/concepts/502231</dcterms:identifier>
				<cc:license rdf:resource="http://reference.data.gov.uk/id/open-government-licence" />
				<cc:attributionURL rdf:resource="http://www.rcahms.gov.uk" />
				<cc:attributionName xml:lang="en">RCAHMS</cc:attributionName>
				<dcterms:publisher rdf:resource="http://www.rcahms.gov.uk" />
				<skos:prefLabel xml:lang="en">AUXILIARY YAWL</skos:prefLabel>
				<dcterms:created rdf:datatype="http://www.w3.org/2001/XMLSchema#dateTime">2007-05-17T10:42:06</dcterms:created>
				<dcterms:modified rdf:datatype="http://www.w3.org/2001/XMLSchema#dateTime">2007-05-17T10:42:18</dcterms:modified>
				<dcterms:issued rdf:datatype="http://www.w3.org/2001/XMLSchema#dateTime">2013-07-17T10:08:39</dcterms:issued>
				<skos:broader rdf:resource="http://purl.org/heritagedata/schemes/3/concepts/502019" />
				<skos:scopeNote xml:lang="en">A Yawl having auxiliary steam or diesel propulsion for use in harbour areas, light airs or contrary winds.</skos:scopeNote>
			</skos:Concept>
		</skos:narrower>
		<skos:scopeNote xml:lang="en">A decked sailing vessel, having fore-and-aft sails on both main and mizzen. It is conventionally distinguished from the Ketch by having the mizzen mast stepped aft of the rudder-head.</skos:scopeNote>
	</skos:Concept>
</rdf:RDF>