<?xml version="1.0"?>
<rdf:RDF xmlns:dc="http://purl.org/dc/elements/1.1/" xmlns:owl="http://www.w3.org/2002/07/owl#" xmlns:skosxl="http://www.w3.org/2008/05/skos-xl#" xmlns:rdfs="http://www.w3.org/2000/01/rdf-schema#" xmlns:dcterms="http://purl.org/dc/terms/" xmlns:xsd="http://www.w3.org/2001/XMLSchema#" xmlns:rdf="http://www.w3.org/1999/02/22-rdf-syntax-ns#" xmlns:cc="http://creativecommons.org/ns#" xmlns:skos="http://www.w3.org/2004/02/skos/core#" xml:base="http://stellar/">
	<skos:Concept rdf:about="http://purl.org/heritagedata/schemes/4/concepts/502413">
		<skos:inScheme rdf:resource="http://purl.org/heritagedata/schemes/4" />
		<dcterms:identifier>http://purl.org/heritagedata/schemes/4/concepts/502413</dcterms:identifier>
		<cc:license rdf:resource="http://reference.data.gov.uk/id/open-government-licence" />
		<cc:attributionURL rdf:resource="http://www.rcahms.gov.uk" />
		<cc:attributionName xml:lang="en">RCAHMS</cc:attributionName>
		<dcterms:publisher rdf:resource="http://www.rcahms.gov.uk" />
		<skos:prefLabel xml:lang="en">ENVIRONMENTAL SAMPLING</skos:prefLabel>
		<dcterms:created rdf:datatype="http://www.w3.org/2001/XMLSchema#dateTime">2007-06-01T09:06:16</dcterms:created>
		<dcterms:modified rdf:datatype="http://www.w3.org/2001/XMLSchema#dateTime">2007-06-01T09:09:49</dcterms:modified>
		<dcterms:issued rdf:datatype="http://www.w3.org/2001/XMLSchema#dateTime">2013-07-17T10:08:40</dcterms:issued>
		<skos:narrower>
			<skos:Concept rdf:about="http://purl.org/heritagedata/schemes/4/concepts/502412">
				<skos:inScheme rdf:resource="http://purl.org/heritagedata/schemes/4" />
				<dcterms:identifier>http://purl.org/heritagedata/schemes/4/concepts/502412</dcterms:identifier>
				<cc:license rdf:resource="http://reference.data.gov.uk/id/open-government-licence" />
				<cc:attributionURL rdf:resource="http://www.rcahms.gov.uk" />
				<cc:attributionName xml:lang="en">RCAHMS</cc:attributionName>
				<dcterms:publisher rdf:resource="http://www.rcahms.gov.uk" />
				<skos:prefLabel xml:lang="en">AUGERING SURVEY</skos:prefLabel>
				<dcterms:created rdf:datatype="http://www.w3.org/2001/XMLSchema#dateTime">2007-06-01T09:02:25</dcterms:created>
				<dcterms:modified rdf:datatype="http://www.w3.org/2001/XMLSchema#dateTime">2007-06-01T09:04:28</dcterms:modified>
				<dcterms:issued rdf:datatype="http://www.w3.org/2001/XMLSchema#dateTime">2013-07-17T10:08:40</dcterms:issued>
				<skos:broader rdf:resource="http://purl.org/heritagedata/schemes/4/concepts/502413" />
				<skos:scopeNote xml:lang="en">The systematic evaluation of an area through auger or bore-hole sampling on a transect or grid. Used to determine the depth and character of archaeological and other deposits.</skos:scopeNote>
			</skos:Concept>
		</skos:narrower>
		<skos:broader rdf:resource="http://purl.org/heritagedata/schemes/4/concepts/502346" />
		<skos:narrower>
			<skos:Concept rdf:about="http://purl.org/heritagedata/schemes/4/concepts/502414">
				<skos:inScheme rdf:resource="http://purl.org/heritagedata/schemes/4" />
				<dcterms:identifier>http://purl.org/heritagedata/schemes/4/concepts/502414</dcterms:identifier>
				<cc:license rdf:resource="http://reference.data.gov.uk/id/open-government-licence" />
				<cc:attributionURL rdf:resource="http://www.rcahms.gov.uk" />
				<cc:attributionName xml:lang="en">RCAHMS</cc:attributionName>
				<dcterms:publisher rdf:resource="http://www.rcahms.gov.uk" />
				<skos:prefLabel xml:lang="en">SOIL SAMPLING</skos:prefLabel>
				<dcterms:created rdf:datatype="http://www.w3.org/2001/XMLSchema#dateTime">2007-06-01T09:11:57</dcterms:created>
				<dcterms:modified rdf:datatype="http://www.w3.org/2001/XMLSchema#dateTime">2007-06-01T09:15:22</dcterms:modified>
				<dcterms:issued rdf:datatype="http://www.w3.org/2001/XMLSchema#dateTime">2013-07-17T10:08:40</dcterms:issued>
				<skos:broader rdf:resource="http://purl.org/heritagedata/schemes/4/concepts/502413" />
				<skos:scopeNote xml:lang="en">The removal of a measured quantity of soil for analysis to measure or assess its content or characteristics</skos:scopeNote>
			</skos:Concept>
		</skos:narrower>
		<skos:narrower>
			<skos:Concept rdf:about="http://purl.org/heritagedata/schemes/4/concepts/502415">
				<skos:inScheme rdf:resource="http://purl.org/heritagedata/schemes/4" />
				<dcterms:identifier>http://purl.org/heritagedata/schemes/4/concepts/502415</dcterms:identifier>
				<cc:license rdf:resource="http://reference.data.gov.uk/id/open-government-licence" />
				<cc:attributionURL rdf:resource="http://www.rcahms.gov.uk" />
				<cc:attributionName xml:lang="en">RCAHMS</cc:attributionName>
				<dcterms:publisher rdf:resource="http://www.rcahms.gov.uk" />
				<skos:prefLabel xml:lang="en">BOREHOLE SURVEY</skos:prefLabel>
				<dcterms:created rdf:datatype="http://www.w3.org/2001/XMLSchema#dateTime">2007-06-01T09:15:43</dcterms:created>
				<dcterms:modified rdf:datatype="http://www.w3.org/2001/XMLSchema#dateTime">2007-06-01T09:21:17</dcterms:modified>
				<dcterms:issued rdf:datatype="http://www.w3.org/2001/XMLSchema#dateTime">2013-07-17T10:08:40</dcterms:issued>
				<skos:broader rdf:resource="http://purl.org/heritagedata/schemes/4/concepts/502413" />
				<skos:scopeNote xml:lang="en">Assessment of the depth and character of the subsoil through analysis of a series of samples extracted mechanically from boreholes.</skos:scopeNote>
			</skos:Concept>
		</skos:narrower>
		<skos:narrower>
			<skos:Concept rdf:about="http://purl.org/heritagedata/schemes/4/concepts/503520">
				<skos:inScheme rdf:resource="http://purl.org/heritagedata/schemes/4" />
				<dcterms:identifier>http://purl.org/heritagedata/schemes/4/concepts/503520</dcterms:identifier>
				<cc:license rdf:resource="http://reference.data.gov.uk/id/open-government-licence" />
				<cc:attributionURL rdf:resource="http://www.rcahms.gov.uk" />
				<cc:attributionName xml:lang="en">RCAHMS</cc:attributionName>
				<dcterms:publisher rdf:resource="http://www.rcahms.gov.uk" />
				<skos:prefLabel xml:lang="en">TAPHONOMIC STUDY</skos:prefLabel>
				<dcterms:created rdf:datatype="http://www.w3.org/2001/XMLSchema#dateTime">2008-08-29T10:09:50</dcterms:created>
				<dcterms:modified rdf:datatype="http://www.w3.org/2001/XMLSchema#dateTime">2008-08-29T10:10:20</dcterms:modified>
				<dcterms:issued rdf:datatype="http://www.w3.org/2001/XMLSchema#dateTime">2013-07-17T10:08:40</dcterms:issued>
				<skos:broader rdf:resource="http://purl.org/heritagedata/schemes/4/concepts/502413" />
				<skos:scopeNote xml:lang="en">Study of the processes that bones (animal and or human) have undergone prior to and or following deposition (including - weathering, burning, damage in the form of cut marks or gnaw marks).</skos:scopeNote>
			</skos:Concept>
		</skos:narrower>
		<skos:narrower rdf:resource="http://purl.org/heritagedata/schemes/4/concepts/502709" />
		<skos:narrower rdf:resource="http://purl.org/heritagedata/schemes/4/concepts/502710" />
		<skos:narrower>
			<skos:Concept rdf:about="http://purl.org/heritagedata/schemes/4/concepts/503118">
				<skos:inScheme rdf:resource="http://purl.org/heritagedata/schemes/4" />
				<dcterms:identifier>http://purl.org/heritagedata/schemes/4/concepts/503118</dcterms:identifier>
				<cc:license rdf:resource="http://reference.data.gov.uk/id/open-government-licence" />
				<cc:attributionURL rdf:resource="http://www.rcahms.gov.uk" />
				<cc:attributionName xml:lang="en">RCAHMS</cc:attributionName>
				<dcterms:publisher rdf:resource="http://www.rcahms.gov.uk" />
				<skos:prefLabel xml:lang="en">SOIL MONOLITH SAMPLING</skos:prefLabel>
				<dcterms:created rdf:datatype="http://www.w3.org/2001/XMLSchema#dateTime">2007-12-20T12:38:21</dcterms:created>
				<dcterms:modified rdf:datatype="http://www.w3.org/2001/XMLSchema#dateTime">2007-12-20T12:39:11</dcterms:modified>
				<dcterms:issued rdf:datatype="http://www.w3.org/2001/XMLSchema#dateTime">2013-07-17T10:08:40</dcterms:issued>
				<skos:broader rdf:resource="http://purl.org/heritagedata/schemes/4/concepts/502413" />
				<skos:scopeNote xml:lang="en">The removal of a vertical sample of soil generally using a U-sectioned tin to extract an intact column including distinct layers.</skos:scopeNote>
			</skos:Concept>
		</skos:narrower>
		<skos:narrower rdf:resource="http://purl.org/heritagedata/schemes/4/concepts/503120" />
		<skos:scopeNote xml:lang="en">A range of sampling techniques and analysis used to understand past human use of plants and animals, and how societies interacted with their environment.</skos:scopeNote>
	</skos:Concept>
	<skos:Concept rdf:about="http://purl.org/heritagedata/schemes/4/concepts/506321">
		<skos:inScheme rdf:resource="http://purl.org/heritagedata/schemes/4" />
		<dcterms:identifier>http://purl.org/heritagedata/schemes/4/concepts/506321</dcterms:identifier>
		<cc:license rdf:resource="http://reference.data.gov.uk/id/open-government-licence" />
		<cc:attributionURL rdf:resource="http://www.rcahms.gov.uk" />
		<cc:attributionName xml:lang="en">RCAHMS</cc:attributionName>
		<dcterms:publisher rdf:resource="http://www.rcahms.gov.uk" />
		<skos:prefLabel xml:lang="en">BUILDING NOTICE</skos:prefLabel>
		<dcterms:created rdf:datatype="http://www.w3.org/2001/XMLSchema#dateTime">2011-12-13T14:02:07</dcterms:created>
		<dcterms:modified rdf:datatype="http://www.w3.org/2001/XMLSchema#dateTime">2011-12-13T14:02:32</dcterms:modified>
		<dcterms:issued rdf:datatype="http://www.w3.org/2001/XMLSchema#dateTime">2013-07-17T10:08:40</dcterms:issued>
		<skos:broader rdf:resource="http://purl.org/heritagedata/schemes/4/concepts/502343" />
		<skos:narrower>
			<skos:Concept rdf:about="http://purl.org/heritagedata/schemes/4/concepts/506322">
				<skos:inScheme rdf:resource="http://purl.org/heritagedata/schemes/4" />
				<dcterms:identifier>http://purl.org/heritagedata/schemes/4/concepts/506322</dcterms:identifier>
				<cc:license rdf:resource="http://reference.data.gov.uk/id/open-government-licence" />
				<cc:attributionURL rdf:resource="http://www.rcahms.gov.uk" />
				<cc:attributionName xml:lang="en">RCAHMS</cc:attributionName>
				<dcterms:publisher rdf:resource="http://www.rcahms.gov.uk" />
				<skos:prefLabel xml:lang="en">BUILDING PRESERVATION NOTICE SERVED</skos:prefLabel>
				<dcterms:created rdf:datatype="http://www.w3.org/2001/XMLSchema#dateTime">2011-12-13T14:02:52</dcterms:created>
				<dcterms:modified rdf:datatype="http://www.w3.org/2001/XMLSchema#dateTime">2011-12-13T14:02:52</dcterms:modified>
				<dcterms:issued rdf:datatype="http://www.w3.org/2001/XMLSchema#dateTime">2013-07-17T10:08:40</dcterms:issued>
				<skos:broader rdf:resource="http://purl.org/heritagedata/schemes/4/concepts/506321" />
				<skos:scopeNote xml:lang="en">Type scope note here</skos:scopeNote>
			</skos:Concept>
		</skos:narrower>
		<skos:narrower>
			<skos:Concept rdf:about="http://purl.org/heritagedata/schemes/4/concepts/506323">
				<skos:inScheme rdf:resource="http://purl.org/heritagedata/schemes/4" />
				<dcterms:identifier>http://purl.org/heritagedata/schemes/4/concepts/506323</dcterms:identifier>
				<cc:license rdf:resource="http://reference.data.gov.uk/id/open-government-licence" />
				<cc:attributionURL rdf:resource="http://www.rcahms.gov.uk" />
				<cc:attributionName xml:lang="en">RCAHMS</cc:attributionName>
				<dcterms:publisher rdf:resource="http://www.rcahms.gov.uk" />
				<skos:prefLabel xml:lang="en">COMPULSORY PURCHASE CONSIDERED</skos:prefLabel>
				<dcterms:created rdf:datatype="http://www.w3.org/2001/XMLSchema#dateTime">2011-12-13T14:03:37</dcterms:created>
				<dcterms:modified rdf:datatype="http://www.w3.org/2001/XMLSchema#dateTime">2011-12-13T14:03:55</dcterms:modified>
				<dcterms:issued rdf:datatype="http://www.w3.org/2001/XMLSchema#dateTime">2013-07-17T10:08:40</dcterms:issued>
				<skos:broader rdf:resource="http://purl.org/heritagedata/schemes/4/concepts/506321" />
				<skos:scopeNote xml:lang="en">COMPULSORY PURCHASE CONSIDERED</skos:scopeNote>
			</skos:Concept>
		</skos:narrower>
		<skos:narrower>
			<skos:Concept rdf:about="http://purl.org/heritagedata/schemes/4/concepts/506324">
				<skos:inScheme rdf:resource="http://purl.org/heritagedata/schemes/4" />
				<dcterms:identifier>http://purl.org/heritagedata/schemes/4/concepts/506324</dcterms:identifier>
				<cc:license rdf:resource="http://reference.data.gov.uk/id/open-government-licence" />
				<cc:attributionURL rdf:resource="http://www.rcahms.gov.uk" />
				<cc:attributionName xml:lang="en">RCAHMS</cc:attributionName>
				<dcterms:publisher rdf:resource="http://www.rcahms.gov.uk" />
				<skos:prefLabel xml:lang="en">DANGEROUS BUILDING NOTICE SERVED</skos:prefLabel>
				<dcterms:created rdf:datatype="http://www.w3.org/2001/XMLSchema#dateTime">2011-12-13T14:04:09</dcterms:created>
				<dcterms:modified rdf:datatype="http://www.w3.org/2001/XMLSchema#dateTime">2011-12-13T14:04:14</dcterms:modified>
				<dcterms:issued rdf:datatype="http://www.w3.org/2001/XMLSchema#dateTime">2013-07-17T10:08:40</dcterms:issued>
				<skos:broader rdf:resource="http://purl.org/heritagedata/schemes/4/concepts/506321" />
				<skos:scopeNote xml:lang="en">DANGEROUS BUILDING NOTICE SERVED</skos:scopeNote>
			</skos:Concept>
		</skos:narrower>
		<skos:narrower>
			<skos:Concept rdf:about="http://purl.org/heritagedata/schemes/4/concepts/506325">
				<skos:inScheme rdf:resource="http://purl.org/heritagedata/schemes/4" />
				<dcterms:identifier>http://purl.org/heritagedata/schemes/4/concepts/506325</dcterms:identifier>
				<cc:license rdf:resource="http://reference.data.gov.uk/id/open-government-licence" />
				<cc:attributionURL rdf:resource="http://www.rcahms.gov.uk" />
				<cc:attributionName xml:lang="en">RCAHMS</cc:attributionName>
				<dcterms:publisher rdf:resource="http://www.rcahms.gov.uk" />
				<skos:prefLabel xml:lang="en">DEMOLITION APPLICATION</skos:prefLabel>
				<dcterms:created rdf:datatype="http://www.w3.org/2001/XMLSchema#dateTime">2011-12-13T14:04:36</dcterms:created>
				<dcterms:modified rdf:datatype="http://www.w3.org/2001/XMLSchema#dateTime">2011-12-13T14:04:39</dcterms:modified>
				<dcterms:issued rdf:datatype="http://www.w3.org/2001/XMLSchema#dateTime">2013-07-17T10:08:40</dcterms:issued>
				<skos:broader rdf:resource="http://purl.org/heritagedata/schemes/4/concepts/506321" />
				<skos:scopeNote xml:lang="en">DEMOLITION APPLICATION</skos:scopeNote>
			</skos:Concept>
		</skos:narrower>
		<skos:narrower>
			<skos:Concept rdf:about="http://purl.org/heritagedata/schemes/4/concepts/506326">
				<skos:inScheme rdf:resource="http://purl.org/heritagedata/schemes/4" />
				<dcterms:identifier>http://purl.org/heritagedata/schemes/4/concepts/506326</dcterms:identifier>
				<cc:license rdf:resource="http://reference.data.gov.uk/id/open-government-licence" />
				<cc:attributionURL rdf:resource="http://www.rcahms.gov.uk" />
				<cc:attributionName xml:lang="en">RCAHMS</cc:attributionName>
				<dcterms:publisher rdf:resource="http://www.rcahms.gov.uk" />
				<skos:prefLabel xml:lang="en">REPAIR NOTICE SERVED</skos:prefLabel>
				<dcterms:created rdf:datatype="http://www.w3.org/2001/XMLSchema#dateTime">2011-12-13T14:05:05</dcterms:created>
				<dcterms:modified rdf:datatype="http://www.w3.org/2001/XMLSchema#dateTime">2011-12-13T14:05:08</dcterms:modified>
				<dcterms:issued rdf:datatype="http://www.w3.org/2001/XMLSchema#dateTime">2013-07-17T10:08:40</dcterms:issued>
				<skos:broader rdf:resource="http://purl.org/heritagedata/schemes/4/concepts/506321" />
				<skos:scopeNote xml:lang="en">REPAIR NOTICE SERVED</skos:scopeNote>
			</skos:Concept>
		</skos:narrower>
		<skos:scopeNote xml:lang="en">BUILDING NOTICE</skos:scopeNote>
	</skos:Concept>
	<skos:Concept rdf:about="http://purl.org/heritagedata/schemes/4/concepts/506330">
		<skos:inScheme rdf:resource="http://purl.org/heritagedata/schemes/4" />
		<dcterms:identifier>http://purl.org/heritagedata/schemes/4/concepts/506330</dcterms:identifier>
		<cc:license rdf:resource="http://reference.data.gov.uk/id/open-government-licence" />
		<cc:attributionURL rdf:resource="http://www.rcahms.gov.uk" />
		<cc:attributionName xml:lang="en">RCAHMS</cc:attributionName>
		<dcterms:publisher rdf:resource="http://www.rcahms.gov.uk" />
		<skos:topConceptOf rdf:resource="http://purl.org/heritagedata/schemes/4" />
		<skos:prefLabel xml:lang="en">MANAGEMENT</skos:prefLabel>
		<dcterms:created rdf:datatype="http://www.w3.org/2001/XMLSchema#dateTime">2011-12-13T14:10:04</dcterms:created>
		<dcterms:modified rdf:datatype="http://www.w3.org/2001/XMLSchema#dateTime">2011-12-13T14:12:05</dcterms:modified>
		<dcterms:issued rdf:datatype="http://www.w3.org/2001/XMLSchema#dateTime">2013-07-17T10:08:40</dcterms:issued>
		<skos:narrower rdf:resource="http://purl.org/heritagedata/schemes/4/concepts/506331" />
		<skos:scopeNote xml:lang="en">MANAGEMENT</skos:scopeNote>
	</skos:Concept>
	<skos:Concept rdf:about="http://purl.org/heritagedata/schemes/4/concepts/506331">
		<skos:inScheme rdf:resource="http://purl.org/heritagedata/schemes/4" />
		<dcterms:identifier>http://purl.org/heritagedata/schemes/4/concepts/506331</dcterms:identifier>
		<cc:license rdf:resource="http://reference.data.gov.uk/id/open-government-licence" />
		<cc:attributionURL rdf:resource="http://www.rcahms.gov.uk" />
		<cc:attributionName xml:lang="en">RCAHMS</cc:attributionName>
		<dcterms:publisher rdf:resource="http://www.rcahms.gov.uk" />
		<skos:prefLabel xml:lang="en">SITE MANAGEMENT</skos:prefLabel>
		<dcterms:created rdf:datatype="http://www.w3.org/2001/XMLSchema#dateTime">2011-12-13T14:10:33</dcterms:created>
		<dcterms:modified rdf:datatype="http://www.w3.org/2001/XMLSchema#dateTime">2011-12-13T14:11:57</dcterms:modified>
		<dcterms:issued rdf:datatype="http://www.w3.org/2001/XMLSchema#dateTime">2013-07-17T10:08:40</dcterms:issued>
		<skos:broader rdf:resource="http://purl.org/heritagedata/schemes/4/concepts/506330" />
		<skos:narrower>
			<skos:Concept rdf:about="http://purl.org/heritagedata/schemes/4/concepts/506332">
				<skos:inScheme rdf:resource="http://purl.org/heritagedata/schemes/4" />
				<dcterms:identifier>http://purl.org/heritagedata/schemes/4/concepts/506332</dcterms:identifier>
				<cc:license rdf:resource="http://reference.data.gov.uk/id/open-government-licence" />
				<cc:attributionURL rdf:resource="http://www.rcahms.gov.uk" />
				<cc:attributionName xml:lang="en">RCAHMS</cc:attributionName>
				<dcterms:publisher rdf:resource="http://www.rcahms.gov.uk" />
				<skos:prefLabel xml:lang="en">CHANGE HISTORY</skos:prefLabel>
				<dcterms:created rdf:datatype="http://www.w3.org/2001/XMLSchema#dateTime">2011-12-13T14:10:55</dcterms:created>
				<dcterms:modified rdf:datatype="http://www.w3.org/2001/XMLSchema#dateTime">2011-12-13T14:11:49</dcterms:modified>
				<dcterms:issued rdf:datatype="http://www.w3.org/2001/XMLSchema#dateTime">2013-07-17T10:08:40</dcterms:issued>
				<skos:broader rdf:resource="http://purl.org/heritagedata/schemes/4/concepts/506331" />
				<skos:scopeNote xml:lang="en">CHANGE HISTORY</skos:scopeNote>
			</skos:Concept>
		</skos:narrower>
		<skos:narrower>
			<skos:Concept rdf:about="http://purl.org/heritagedata/schemes/4/concepts/506333">
				<skos:inScheme rdf:resource="http://purl.org/heritagedata/schemes/4" />
				<dcterms:identifier>http://purl.org/heritagedata/schemes/4/concepts/506333</dcterms:identifier>
				<cc:license rdf:resource="http://reference.data.gov.uk/id/open-government-licence" />
				<cc:attributionURL rdf:resource="http://www.rcahms.gov.uk" />
				<cc:attributionName xml:lang="en">RCAHMS</cc:attributionName>
				<dcterms:publisher rdf:resource="http://www.rcahms.gov.uk" />
				<skos:prefLabel xml:lang="en">DEVELOPMENT HISTORY</skos:prefLabel>
				<dcterms:created rdf:datatype="http://www.w3.org/2001/XMLSchema#dateTime">2011-12-13T14:11:20</dcterms:created>
				<dcterms:modified rdf:datatype="http://www.w3.org/2001/XMLSchema#dateTime">2011-12-13T14:11:30</dcterms:modified>
				<dcterms:issued rdf:datatype="http://www.w3.org/2001/XMLSchema#dateTime">2013-07-17T10:08:40</dcterms:issued>
				<skos:broader rdf:resource="http://purl.org/heritagedata/schemes/4/concepts/506331" />
				<skos:scopeNote xml:lang="en">DEVELOPMENT HISTORY</skos:scopeNote>
			</skos:Concept>
		</skos:narrower>
		<skos:scopeNote xml:lang="en">SITE MANAGEMENT</skos:scopeNote>
	</skos:Concept>
	<skos:Concept rdf:about="http://purl.org/heritagedata/schemes/4/concepts/506601">
		<skos:inScheme rdf:resource="http://purl.org/heritagedata/schemes/4" />
		<dcterms:identifier>http://purl.org/heritagedata/schemes/4/concepts/506601</dcterms:identifier>
		<cc:license rdf:resource="http://reference.data.gov.uk/id/open-government-licence" />
		<cc:attributionURL rdf:resource="http://www.rcahms.gov.uk" />
		<cc:attributionName xml:lang="en">RCAHMS</cc:attributionName>
		<dcterms:publisher rdf:resource="http://www.rcahms.gov.uk" />
		<skos:prefLabel xml:lang="en">REMOTE SENSING</skos:prefLabel>
		<dcterms:created rdf:datatype="http://www.w3.org/2001/XMLSchema#dateTime">2012-05-02T09:11:11</dcterms:created>
		<dcterms:modified rdf:datatype="http://www.w3.org/2001/XMLSchema#dateTime">2012-05-02T09:11:23</dcterms:modified>
		<dcterms:issued rdf:datatype="http://www.w3.org/2001/XMLSchema#dateTime">2013-07-17T10:08:40</dcterms:issued>
		<skos:narrower>
			<skos:Concept rdf:about="http://purl.org/heritagedata/schemes/4/concepts/502383">
				<skos:inScheme rdf:resource="http://purl.org/heritagedata/schemes/4" />
				<dcterms:identifier>http://purl.org/heritagedata/schemes/4/concepts/502383</dcterms:identifier>
				<cc:license rdf:resource="http://reference.data.gov.uk/id/open-government-licence" />
				<cc:attributionURL rdf:resource="http://www.rcahms.gov.uk" />
				<cc:attributionName xml:lang="en">RCAHMS</cc:attributionName>
				<dcterms:publisher rdf:resource="http://www.rcahms.gov.uk" />
				<skos:prefLabel xml:lang="en">SIDE SCAN SONAR SURVEY</skos:prefLabel>
				<dcterms:created rdf:datatype="http://www.w3.org/2001/XMLSchema#dateTime">2007-05-31T09:20:23</dcterms:created>
				<dcterms:modified rdf:datatype="http://www.w3.org/2001/XMLSchema#dateTime">2007-05-31T09:25:18</dcterms:modified>
				<dcterms:issued rdf:datatype="http://www.w3.org/2001/XMLSchema#dateTime">2013-07-17T10:08:40</dcterms:issued>
				<skos:broader rdf:resource="http://purl.org/heritagedata/schemes/4/concepts/506601" />
				<skos:scopeNote xml:lang="en">A remote sensing technique used in  underwater archaeology to record objects on the sea or loch bed through the measurement of laterally emitted  and reflected high frequency sound waves.</skos:scopeNote>
			</skos:Concept>
		</skos:narrower>
		<skos:narrower rdf:resource="http://purl.org/heritagedata/schemes/4/concepts/502358" />
		<skos:narrower>
			<skos:Concept rdf:about="http://purl.org/heritagedata/schemes/4/concepts/506461">
				<skos:inScheme rdf:resource="http://purl.org/heritagedata/schemes/4" />
				<dcterms:identifier>http://purl.org/heritagedata/schemes/4/concepts/506461</dcterms:identifier>
				<cc:license rdf:resource="http://reference.data.gov.uk/id/open-government-licence" />
				<cc:attributionURL rdf:resource="http://www.rcahms.gov.uk" />
				<cc:attributionName xml:lang="en">RCAHMS</cc:attributionName>
				<dcterms:publisher rdf:resource="http://www.rcahms.gov.uk" />
				<skos:prefLabel xml:lang="en">SINGLE  BEAM ECHOSOUNDER</skos:prefLabel>
				<dcterms:created rdf:datatype="http://www.w3.org/2001/XMLSchema#dateTime">2012-02-10T16:12:54</dcterms:created>
				<dcterms:modified rdf:datatype="http://www.w3.org/2001/XMLSchema#dateTime">2012-02-10T16:16:35</dcterms:modified>
				<dcterms:issued rdf:datatype="http://www.w3.org/2001/XMLSchema#dateTime">2013-07-17T10:08:40</dcterms:issued>
				<skos:broader rdf:resource="http://purl.org/heritagedata/schemes/4/concepts/506601" />
				<skos:scopeNote xml:lang="en">A remote sensing technique used in  underwater archaeology to record objects on the sea or loch bed through the comparative analysis of soundings produced by transmitting short pulses of acoustic energy  towards the seabed and detecting those pulses reflected.</skos:scopeNote>
			</skos:Concept>
		</skos:narrower>
		<skos:broader rdf:resource="http://purl.org/heritagedata/schemes/4/concepts/502401" />
		<skos:narrower>
			<skos:Concept rdf:about="http://purl.org/heritagedata/schemes/4/concepts/503117">
				<skos:inScheme rdf:resource="http://purl.org/heritagedata/schemes/4" />
				<dcterms:identifier>http://purl.org/heritagedata/schemes/4/concepts/503117</dcterms:identifier>
				<cc:license rdf:resource="http://reference.data.gov.uk/id/open-government-licence" />
				<cc:attributionURL rdf:resource="http://www.rcahms.gov.uk" />
				<cc:attributionName xml:lang="en">RCAHMS</cc:attributionName>
				<dcterms:publisher rdf:resource="http://www.rcahms.gov.uk" />
				<skos:prefLabel xml:lang="en">SUB BOTTOM PROFILING SURVEY</skos:prefLabel>
				<dcterms:created rdf:datatype="http://www.w3.org/2001/XMLSchema#dateTime">2007-12-20T12:33:59</dcterms:created>
				<dcterms:modified rdf:datatype="http://www.w3.org/2001/XMLSchema#dateTime">2007-12-20T12:39:43</dcterms:modified>
				<dcterms:issued rdf:datatype="http://www.w3.org/2001/XMLSchema#dateTime">2013-07-17T10:08:40</dcterms:issued>
				<skos:broader rdf:resource="http://purl.org/heritagedata/schemes/4/concepts/506601" />
				<skos:scopeNote xml:lang="en">A remote sensing technique used to locate and record structures buried within the sea bed through the  emmssion and reflection of high energy low frequency sound waves.</skos:scopeNote>
			</skos:Concept>
		</skos:narrower>
		<skos:narrower>
			<skos:Concept rdf:about="http://purl.org/heritagedata/schemes/4/concepts/503419">
				<skos:inScheme rdf:resource="http://purl.org/heritagedata/schemes/4" />
				<dcterms:identifier>http://purl.org/heritagedata/schemes/4/concepts/503419</dcterms:identifier>
				<cc:license rdf:resource="http://reference.data.gov.uk/id/open-government-licence" />
				<cc:attributionURL rdf:resource="http://www.rcahms.gov.uk" />
				<cc:attributionName xml:lang="en">RCAHMS</cc:attributionName>
				<dcterms:publisher rdf:resource="http://www.rcahms.gov.uk" />
				<skos:prefLabel xml:lang="en">MULTI BEAM SONAR SCAN</skos:prefLabel>
				<dcterms:created rdf:datatype="http://www.w3.org/2001/XMLSchema#dateTime">2008-07-17T11:24:21</dcterms:created>
				<dcterms:modified rdf:datatype="http://www.w3.org/2001/XMLSchema#dateTime">2008-07-17T11:24:30</dcterms:modified>
				<dcterms:issued rdf:datatype="http://www.w3.org/2001/XMLSchema#dateTime">2013-07-17T10:08:40</dcterms:issued>
				<skos:broader rdf:resource="http://purl.org/heritagedata/schemes/4/concepts/506601" />
				<skos:scopeNote xml:lang="en">A remote sensing technique used in  underwater archaeology to record objects on the sea or loch bed through the comparative analysis of reflections received from high frequency sound waves emitted in multiple beams.</skos:scopeNote>
			</skos:Concept>
		</skos:narrower>
		<skos:scopeNote xml:lang="en">Remote sensing techniques.</skos:scopeNote>
	</skos:Concept>
	<skos:Concept rdf:about="http://purl.org/heritagedata/schemes/4/concepts/502339">
		<skos:inScheme rdf:resource="http://purl.org/heritagedata/schemes/4" />
		<dcterms:identifier>http://purl.org/heritagedata/schemes/4/concepts/502339</dcterms:identifier>
		<cc:license rdf:resource="http://reference.data.gov.uk/id/open-government-licence" />
		<cc:attributionURL rdf:resource="http://www.rcahms.gov.uk" />
		<cc:attributionName xml:lang="en">RCAHMS</cc:attributionName>
		<dcterms:publisher rdf:resource="http://www.rcahms.gov.uk" />
		<skos:topConceptOf rdf:resource="http://purl.org/heritagedata/schemes/4" />
		<skos:prefLabel xml:lang="en">OS ANTIQUITY MODELS</skos:prefLabel>
		<dcterms:created rdf:datatype="http://www.w3.org/2001/XMLSchema#dateTime">2007-05-30T09:18:24</dcterms:created>
		<dcterms:modified rdf:datatype="http://www.w3.org/2001/XMLSchema#dateTime">2008-01-07T13:55:40</dcterms:modified>
		<dcterms:issued rdf:datatype="http://www.w3.org/2001/XMLSchema#dateTime">2013-07-17T10:08:40</dcterms:issued>
		<skos:narrower>
			<skos:Concept rdf:about="http://purl.org/heritagedata/schemes/4/concepts/502457">
				<skos:inScheme rdf:resource="http://purl.org/heritagedata/schemes/4" />
				<dcterms:identifier>http://purl.org/heritagedata/schemes/4/concepts/502457</dcterms:identifier>
				<cc:license rdf:resource="http://reference.data.gov.uk/id/open-government-licence" />
				<cc:attributionURL rdf:resource="http://www.rcahms.gov.uk" />
				<cc:attributionName xml:lang="en">RCAHMS</cc:attributionName>
				<dcterms:publisher rdf:resource="http://www.rcahms.gov.uk" />
				<skos:prefLabel xml:lang="en">OS THEMATIC MAPPING</skos:prefLabel>
				<dcterms:created rdf:datatype="http://www.w3.org/2001/XMLSchema#dateTime">2007-06-04T10:37:51</dcterms:created>
				<dcterms:modified rdf:datatype="http://www.w3.org/2001/XMLSchema#dateTime">2007-06-04T10:49:25</dcterms:modified>
				<dcterms:issued rdf:datatype="http://www.w3.org/2001/XMLSchema#dateTime">2013-07-17T10:08:40</dcterms:issued>
				<skos:broader rdf:resource="http://purl.org/heritagedata/schemes/4/concepts/502339" />
				<skos:scopeNote xml:lang="en">Use in conjunction with a specific Project  for the selection and publication of information on a range OS Historical mapping projects including Ancient Britain and Roman Britain.</skos:scopeNote>
			</skos:Concept>
		</skos:narrower>
		<skos:narrower rdf:resource="http://purl.org/heritagedata/schemes/4/concepts/502458" />
		<skos:narrower rdf:resource="http://purl.org/heritagedata/schemes/4/concepts/502459" />
		<skos:narrower>
			<skos:Concept rdf:about="http://purl.org/heritagedata/schemes/4/concepts/502460">
				<skos:inScheme rdf:resource="http://purl.org/heritagedata/schemes/4" />
				<dcterms:identifier>http://purl.org/heritagedata/schemes/4/concepts/502460</dcterms:identifier>
				<cc:license rdf:resource="http://reference.data.gov.uk/id/open-government-licence" />
				<cc:attributionURL rdf:resource="http://www.rcahms.gov.uk" />
				<cc:attributionName xml:lang="en">RCAHMS</cc:attributionName>
				<dcterms:publisher rdf:resource="http://www.rcahms.gov.uk" />
				<skos:prefLabel xml:lang="en">OS 250K STRATEGI MAPPING</skos:prefLabel>
				<dcterms:created rdf:datatype="http://www.w3.org/2001/XMLSchema#dateTime">2007-06-04T10:44:22</dcterms:created>
				<dcterms:modified rdf:datatype="http://www.w3.org/2001/XMLSchema#dateTime">2007-06-05T10:58:55</dcterms:modified>
				<dcterms:issued rdf:datatype="http://www.w3.org/2001/XMLSchema#dateTime">2013-07-17T10:08:40</dcterms:issued>
				<skos:broader rdf:resource="http://purl.org/heritagedata/schemes/4/concepts/502339" />
				<skos:scopeNote xml:lang="en">Use for information published as part of the Heritage and Antiquities theme on OS 1:250,000 scale mapping / Strategi  products.</skos:scopeNote>
			</skos:Concept>
		</skos:narrower>
		<skos:narrower rdf:resource="http://purl.org/heritagedata/schemes/4/concepts/502462" />
		<skos:narrower>
			<skos:Concept rdf:about="http://purl.org/heritagedata/schemes/4/concepts/504780">
				<skos:inScheme rdf:resource="http://purl.org/heritagedata/schemes/4" />
				<dcterms:identifier>http://purl.org/heritagedata/schemes/4/concepts/504780</dcterms:identifier>
				<cc:license rdf:resource="http://reference.data.gov.uk/id/open-government-licence" />
				<cc:attributionURL rdf:resource="http://www.rcahms.gov.uk" />
				<cc:attributionName xml:lang="en">RCAHMS</cc:attributionName>
				<dcterms:publisher rdf:resource="http://www.rcahms.gov.uk" />
				<skos:prefLabel xml:lang="en">OS PAPER MAPS</skos:prefLabel>
				<dcterms:created rdf:datatype="http://www.w3.org/2001/XMLSchema#dateTime">2010-03-19T16:40:56</dcterms:created>
				<dcterms:modified rdf:datatype="http://www.w3.org/2001/XMLSchema#dateTime">2010-03-19T16:42:11</dcterms:modified>
				<dcterms:issued rdf:datatype="http://www.w3.org/2001/XMLSchema#dateTime">2013-07-17T10:08:40</dcterms:issued>
				<skos:broader rdf:resource="http://purl.org/heritagedata/schemes/4/concepts/502339" />
				<skos:scopeNote xml:lang="en">Information depicted on OS paper (chart copy) maps at scales of 1:1250, 1:2,500 or 1:10,000 (10,560).</skos:scopeNote>
			</skos:Concept>
		</skos:narrower>
		<skos:scopeNote xml:lang="en">Used for managing the selection of sites on thematic OS maps. OS ANTIQUITY MODEL events should only be used by staff working on projects directly concerned with the creation or revision of heritage content for publication through the Ordnance Survey.</skos:scopeNote>
	</skos:Concept>
	<skos:Concept rdf:about="http://purl.org/heritagedata/schemes/4/concepts/502348">
		<skos:inScheme rdf:resource="http://purl.org/heritagedata/schemes/4" />
		<dcterms:identifier>http://purl.org/heritagedata/schemes/4/concepts/502348</dcterms:identifier>
		<cc:license rdf:resource="http://reference.data.gov.uk/id/open-government-licence" />
		<cc:attributionURL rdf:resource="http://www.rcahms.gov.uk" />
		<cc:attributionName xml:lang="en">RCAHMS</cc:attributionName>
		<dcterms:publisher rdf:resource="http://www.rcahms.gov.uk" />
		<skos:topConceptOf rdf:resource="http://purl.org/heritagedata/schemes/4" />
		<skos:prefLabel xml:lang="en">DESCRIPTIVE ACCOUNTS</skos:prefLabel>
		<dcterms:created rdf:datatype="http://www.w3.org/2001/XMLSchema#dateTime">2007-05-30T09:19:43</dcterms:created>
		<dcterms:modified rdf:datatype="http://www.w3.org/2001/XMLSchema#dateTime">2007-11-30T10:08:22</dcterms:modified>
		<dcterms:issued rdf:datatype="http://www.w3.org/2001/XMLSchema#dateTime">2013-07-17T10:08:40</dcterms:issued>
		<skos:narrower>
			<skos:Concept rdf:about="http://purl.org/heritagedata/schemes/4/concepts/502434">
				<skos:inScheme rdf:resource="http://purl.org/heritagedata/schemes/4" />
				<dcterms:identifier>http://purl.org/heritagedata/schemes/4/concepts/502434</dcterms:identifier>
				<cc:license rdf:resource="http://reference.data.gov.uk/id/open-government-licence" />
				<cc:attributionURL rdf:resource="http://www.rcahms.gov.uk" />
				<cc:attributionName xml:lang="en">RCAHMS</cc:attributionName>
				<dcterms:publisher rdf:resource="http://www.rcahms.gov.uk" />
				<skos:prefLabel xml:lang="en">RCAHMS NOTE</skos:prefLabel>
				<dcterms:created rdf:datatype="http://www.w3.org/2001/XMLSchema#dateTime">2007-06-01T12:02:00</dcterms:created>
				<dcterms:modified rdf:datatype="http://www.w3.org/2001/XMLSchema#dateTime">2011-10-28T09:20:11</dcterms:modified>
				<dcterms:issued rdf:datatype="http://www.w3.org/2001/XMLSchema#dateTime">2013-07-17T10:08:40</dcterms:issued>
				<skos:broader rdf:resource="http://purl.org/heritagedata/schemes/4/concepts/502348" />
				<skos:scopeNote xml:lang="en">Informal notes from RCAHMS concerning a site and not derived from field visits or inspections or from a published account e.g. Inventory. Text should be accompanied by 'Information from RCAHMS (Initials) DATE YEAR.</skos:scopeNote>
			</skos:Concept>
		</skos:narrower>
		<skos:narrower>
			<skos:Concept rdf:about="http://purl.org/heritagedata/schemes/4/concepts/502502">
				<skos:inScheme rdf:resource="http://purl.org/heritagedata/schemes/4" />
				<dcterms:identifier>http://purl.org/heritagedata/schemes/4/concepts/502502</dcterms:identifier>
				<cc:license rdf:resource="http://reference.data.gov.uk/id/open-government-licence" />
				<cc:attributionURL rdf:resource="http://www.rcahms.gov.uk" />
				<cc:attributionName xml:lang="en">RCAHMS</cc:attributionName>
				<dcterms:publisher rdf:resource="http://www.rcahms.gov.uk" />
				<skos:prefLabel xml:lang="en">ARCHAEOLOGY NOTES</skos:prefLabel>
				<dcterms:created rdf:datatype="http://www.w3.org/2001/XMLSchema#dateTime">2007-06-04T12:44:55</dcterms:created>
				<dcterms:modified rdf:datatype="http://www.w3.org/2001/XMLSchema#dateTime">2007-06-04T13:05:09</dcterms:modified>
				<dcterms:issued rdf:datatype="http://www.w3.org/2001/XMLSchema#dateTime">2013-07-17T10:08:40</dcterms:issued>
				<skos:broader rdf:resource="http://purl.org/heritagedata/schemes/4/concepts/502348" />
				<skos:scopeNote xml:lang="en">Unsorted chronological sequence of text summarising a site record, or reporting on the results of specific blocks of fieldwork.</skos:scopeNote>
			</skos:Concept>
		</skos:narrower>
		<skos:narrower>
			<skos:Concept rdf:about="http://purl.org/heritagedata/schemes/4/concepts/502504">
				<skos:inScheme rdf:resource="http://purl.org/heritagedata/schemes/4" />
				<dcterms:identifier>http://purl.org/heritagedata/schemes/4/concepts/502504</dcterms:identifier>
				<cc:license rdf:resource="http://reference.data.gov.uk/id/open-government-licence" />
				<cc:attributionURL rdf:resource="http://www.rcahms.gov.uk" />
				<cc:attributionName xml:lang="en">RCAHMS</cc:attributionName>
				<dcterms:publisher rdf:resource="http://www.rcahms.gov.uk" />
				<skos:prefLabel xml:lang="en">SUMMARY RECORD</skos:prefLabel>
				<dcterms:created rdf:datatype="http://www.w3.org/2001/XMLSchema#dateTime">2007-06-04T13:05:43</dcterms:created>
				<dcterms:modified rdf:datatype="http://www.w3.org/2001/XMLSchema#dateTime">2007-06-04T13:14:40</dcterms:modified>
				<dcterms:issued rdf:datatype="http://www.w3.org/2001/XMLSchema#dateTime">2013-07-17T10:08:40</dcterms:issued>
				<skos:broader rdf:resource="http://purl.org/heritagedata/schemes/4/concepts/502348" />
				<skos:scopeNote xml:lang="en">A brief account that provides the essential facts about monument or building for the general public. The summary record should act as an introduction to the detailed texts associated with a particular record if these exist.</skos:scopeNote>
			</skos:Concept>
		</skos:narrower>
		<skos:narrower>
			<skos:Concept rdf:about="http://purl.org/heritagedata/schemes/4/concepts/502552">
				<skos:inScheme rdf:resource="http://purl.org/heritagedata/schemes/4" />
				<dcterms:identifier>http://purl.org/heritagedata/schemes/4/concepts/502552</dcterms:identifier>
				<cc:license rdf:resource="http://reference.data.gov.uk/id/open-government-licence" />
				<cc:attributionURL rdf:resource="http://www.rcahms.gov.uk" />
				<cc:attributionName xml:lang="en">RCAHMS</cc:attributionName>
				<dcterms:publisher rdf:resource="http://www.rcahms.gov.uk" />
				<skos:prefLabel xml:lang="en">LINEAR ACCOUNT</skos:prefLabel>
				<dcterms:created rdf:datatype="http://www.w3.org/2001/XMLSchema#dateTime">2007-06-08T08:58:34</dcterms:created>
				<dcterms:modified rdf:datatype="http://www.w3.org/2001/XMLSchema#dateTime">2007-06-08T08:59:34</dcterms:modified>
				<dcterms:issued rdf:datatype="http://www.w3.org/2001/XMLSchema#dateTime">2013-07-17T10:08:40</dcterms:issued>
				<skos:broader rdf:resource="http://purl.org/heritagedata/schemes/4/concepts/502348" />
				<skos:scopeNote xml:lang="en">Summary records describing the history and course of a monument crossing several map-sheets.</skos:scopeNote>
			</skos:Concept>
		</skos:narrower>
		<skos:narrower>
			<skos:Concept rdf:about="http://purl.org/heritagedata/schemes/4/concepts/506422">
				<skos:inScheme rdf:resource="http://purl.org/heritagedata/schemes/4" />
				<dcterms:identifier>http://purl.org/heritagedata/schemes/4/concepts/506422</dcterms:identifier>
				<cc:license rdf:resource="http://reference.data.gov.uk/id/open-government-licence" />
				<cc:attributionURL rdf:resource="http://www.rcahms.gov.uk" />
				<cc:attributionName xml:lang="en">RCAHMS</cc:attributionName>
				<dcterms:publisher rdf:resource="http://www.rcahms.gov.uk" />
				<skos:prefLabel xml:lang="en">GHS NOTE</skos:prefLabel>
				<dcterms:created rdf:datatype="http://www.w3.org/2001/XMLSchema#dateTime">2012-01-10T16:47:33</dcterms:created>
				<dcterms:modified rdf:datatype="http://www.w3.org/2001/XMLSchema#dateTime">2012-01-10T16:48:28</dcterms:modified>
				<dcterms:issued rdf:datatype="http://www.w3.org/2001/XMLSchema#dateTime">2013-07-17T10:08:40</dcterms:issued>
				<skos:broader rdf:resource="http://purl.org/heritagedata/schemes/4/concepts/502348" />
				<skos:scopeNote xml:lang="en">Informal notes from The Garden History Society in Scotland staff concerning a site and not derived from field visits or inspections or from a published account e.g. Inventory. Text should be accompanied by 'Information from The Garden History Society in Scotland (Initials) DATE YEAR.</skos:scopeNote>
			</skos:Concept>
		</skos:narrower>
		<skos:narrower>
			<skos:Concept rdf:about="http://purl.org/heritagedata/schemes/4/concepts/506481">
				<skos:inScheme rdf:resource="http://purl.org/heritagedata/schemes/4" />
				<dcterms:identifier>http://purl.org/heritagedata/schemes/4/concepts/506481</dcterms:identifier>
				<cc:license rdf:resource="http://reference.data.gov.uk/id/open-government-licence" />
				<cc:attributionURL rdf:resource="http://www.rcahms.gov.uk" />
				<cc:attributionName xml:lang="en">RCAHMS</cc:attributionName>
				<dcterms:publisher rdf:resource="http://www.rcahms.gov.uk" />
				<skos:prefLabel xml:lang="en">SRP NOTE</skos:prefLabel>
				<dcterms:created rdf:datatype="http://www.w3.org/2001/XMLSchema#dateTime">2012-02-23T17:07:30</dcterms:created>
				<dcterms:modified rdf:datatype="http://www.w3.org/2001/XMLSchema#dateTime">2012-02-23T17:09:04</dcterms:modified>
				<dcterms:issued rdf:datatype="http://www.w3.org/2001/XMLSchema#dateTime">2013-07-17T10:08:40</dcterms:issued>
				<skos:broader rdf:resource="http://purl.org/heritagedata/schemes/4/concepts/502348" />
				<skos:scopeNote xml:lang="en">Information about a site gathered through the course of the Scotland's Rural Past project.</skos:scopeNote>
			</skos:Concept>
		</skos:narrower>
		<skos:narrower>
			<skos:Concept rdf:about="http://purl.org/heritagedata/schemes/4/concepts/504700">
				<skos:inScheme rdf:resource="http://purl.org/heritagedata/schemes/4" />
				<dcterms:identifier>http://purl.org/heritagedata/schemes/4/concepts/504700</dcterms:identifier>
				<cc:license rdf:resource="http://reference.data.gov.uk/id/open-government-licence" />
				<cc:attributionURL rdf:resource="http://www.rcahms.gov.uk" />
				<cc:attributionName xml:lang="en">RCAHMS</cc:attributionName>
				<dcterms:publisher rdf:resource="http://www.rcahms.gov.uk" />
				<skos:prefLabel xml:lang="en">NTS NOTE</skos:prefLabel>
				<dcterms:created rdf:datatype="http://www.w3.org/2001/XMLSchema#dateTime">2010-01-22T13:53:34</dcterms:created>
				<dcterms:modified rdf:datatype="http://www.w3.org/2001/XMLSchema#dateTime">2010-02-05T09:55:01</dcterms:modified>
				<dcterms:issued rdf:datatype="http://www.w3.org/2001/XMLSchema#dateTime">2013-07-17T10:08:40</dcterms:issued>
				<skos:broader rdf:resource="http://purl.org/heritagedata/schemes/4/concepts/502348" />
				<skos:scopeNote xml:lang="en">Informal notes from National Trust for Scotland staff concerning a site and not derived from field visits or inspections or from a published account e.g. Inventory. Text should be accompanied by 'Information from NTS (Initials) DATE YEAR.</skos:scopeNote>
			</skos:Concept>
		</skos:narrower>
		<skos:narrower>
			<skos:Concept rdf:about="http://purl.org/heritagedata/schemes/4/concepts/506722">
				<skos:inScheme rdf:resource="http://purl.org/heritagedata/schemes/4" />
				<dcterms:identifier>http://purl.org/heritagedata/schemes/4/concepts/506722</dcterms:identifier>
				<cc:license rdf:resource="http://reference.data.gov.uk/id/open-government-licence" />
				<cc:attributionURL rdf:resource="http://www.rcahms.gov.uk" />
				<cc:attributionName xml:lang="en">RCAHMS</cc:attributionName>
				<dcterms:publisher rdf:resource="http://www.rcahms.gov.uk" />
				<skos:prefLabel xml:lang="en">FORMER LOCATION</skos:prefLabel>
				<dcterms:created rdf:datatype="http://www.w3.org/2001/XMLSchema#dateTime">2012-06-27T12:28:40</dcterms:created>
				<dcterms:modified rdf:datatype="http://www.w3.org/2001/XMLSchema#dateTime">2012-06-27T13:28:22</dcterms:modified>
				<dcterms:issued rdf:datatype="http://www.w3.org/2001/XMLSchema#dateTime">2013-07-17T10:08:40</dcterms:issued>
				<skos:broader rdf:resource="http://purl.org/heritagedata/schemes/4/concepts/502348" />
				<skos:scopeNote xml:lang="en">Indicates the former location of a portable antiquity e.g. a pictish symbol stone.</skos:scopeNote>
			</skos:Concept>
		</skos:narrower>
		<skos:narrower>
			<skos:Concept rdf:about="http://purl.org/heritagedata/schemes/4/concepts/503680">
				<skos:inScheme rdf:resource="http://purl.org/heritagedata/schemes/4" />
				<dcterms:identifier>http://purl.org/heritagedata/schemes/4/concepts/503680</dcterms:identifier>
				<cc:license rdf:resource="http://reference.data.gov.uk/id/open-government-licence" />
				<cc:attributionURL rdf:resource="http://www.rcahms.gov.uk" />
				<cc:attributionName xml:lang="en">RCAHMS</cc:attributionName>
				<dcterms:publisher rdf:resource="http://www.rcahms.gov.uk" />
				<skos:prefLabel xml:lang="en">CANCELLATION</skos:prefLabel>
				<dcterms:created rdf:datatype="http://www.w3.org/2001/XMLSchema#dateTime">2008-10-07T11:12:38</dcterms:created>
				<dcterms:modified rdf:datatype="http://www.w3.org/2001/XMLSchema#dateTime">2008-10-07T11:15:37</dcterms:modified>
				<dcterms:issued rdf:datatype="http://www.w3.org/2001/XMLSchema#dateTime">2013-07-17T10:08:40</dcterms:issued>
				<skos:broader rdf:resource="http://purl.org/heritagedata/schemes/4/concepts/502348" />
				<skos:scopeNote xml:lang="en">Use for records which have been cancelled as a result of rationalisation of the database and the removal of duplicate or erroneous entries.</skos:scopeNote>
			</skos:Concept>
		</skos:narrower>
		<skos:narrower>
			<skos:Concept rdf:about="http://purl.org/heritagedata/schemes/4/concepts/503479">
				<skos:inScheme rdf:resource="http://purl.org/heritagedata/schemes/4" />
				<dcterms:identifier>http://purl.org/heritagedata/schemes/4/concepts/503479</dcterms:identifier>
				<cc:license rdf:resource="http://reference.data.gov.uk/id/open-government-licence" />
				<cc:attributionURL rdf:resource="http://www.rcahms.gov.uk" />
				<cc:attributionName xml:lang="en">RCAHMS</cc:attributionName>
				<dcterms:publisher rdf:resource="http://www.rcahms.gov.uk" />
				<skos:prefLabel xml:lang="en">PUBLICATION ACCOUNT</skos:prefLabel>
				<dcterms:created rdf:datatype="http://www.w3.org/2001/XMLSchema#dateTime">2008-08-15T14:12:54</dcterms:created>
				<dcterms:modified rdf:datatype="http://www.w3.org/2001/XMLSchema#dateTime">2008-08-15T15:33:27</dcterms:modified>
				<dcterms:issued rdf:datatype="http://www.w3.org/2001/XMLSchema#dateTime">2013-07-17T10:08:40</dcterms:issued>
				<skos:broader rdf:resource="http://purl.org/heritagedata/schemes/4/concepts/502348" />
				<skos:scopeNote xml:lang="en">Descriptions prepared for publication in articles, books and monographs or on exhibition panels.</skos:scopeNote>
			</skos:Concept>
		</skos:narrower>
		<skos:narrower>
			<skos:Concept rdf:about="http://purl.org/heritagedata/schemes/4/concepts/505441">
				<skos:inScheme rdf:resource="http://purl.org/heritagedata/schemes/4" />
				<dcterms:identifier>http://purl.org/heritagedata/schemes/4/concepts/505441</dcterms:identifier>
				<cc:license rdf:resource="http://reference.data.gov.uk/id/open-government-licence" />
				<cc:attributionURL rdf:resource="http://www.rcahms.gov.uk" />
				<cc:attributionName xml:lang="en">RCAHMS</cc:attributionName>
				<dcterms:publisher rdf:resource="http://www.rcahms.gov.uk" />
				<skos:prefLabel xml:lang="en">ORKNEY SMR NOTE</skos:prefLabel>
				<dcterms:created rdf:datatype="http://www.w3.org/2001/XMLSchema#dateTime">2010-09-21T09:58:14</dcterms:created>
				<dcterms:modified rdf:datatype="http://www.w3.org/2001/XMLSchema#dateTime">2010-09-21T10:01:39</dcterms:modified>
				<dcterms:issued rdf:datatype="http://www.w3.org/2001/XMLSchema#dateTime">2013-07-17T10:08:40</dcterms:issued>
				<skos:broader rdf:resource="http://purl.org/heritagedata/schemes/4/concepts/502348" />
				<skos:scopeNote xml:lang="en">Informal notes from Orkney SMR staff concerning a site and not derived from field visits or inspections or from a published account e.g. Inventory. Text should be accompanied by 'Information from Orkney SMR (Initials) DATE YEAR.</skos:scopeNote>
			</skos:Concept>
		</skos:narrower>
		<skos:narrower>
			<skos:Concept rdf:about="http://purl.org/heritagedata/schemes/4/concepts/505881">
				<skos:inScheme rdf:resource="http://purl.org/heritagedata/schemes/4" />
				<dcterms:identifier>http://purl.org/heritagedata/schemes/4/concepts/505881</dcterms:identifier>
				<cc:license rdf:resource="http://reference.data.gov.uk/id/open-government-licence" />
				<cc:attributionURL rdf:resource="http://www.rcahms.gov.uk" />
				<cc:attributionName xml:lang="en">RCAHMS</cc:attributionName>
				<dcterms:publisher rdf:resource="http://www.rcahms.gov.uk" />
				<skos:prefLabel xml:lang="en">ARCHITECTURE NOTES</skos:prefLabel>
				<dcterms:created rdf:datatype="http://www.w3.org/2001/XMLSchema#dateTime">2011-06-13T14:31:44</dcterms:created>
				<dcterms:modified rdf:datatype="http://www.w3.org/2001/XMLSchema#dateTime">2011-06-13T14:41:10</dcterms:modified>
				<dcterms:issued rdf:datatype="http://www.w3.org/2001/XMLSchema#dateTime">2013-07-17T10:08:40</dcterms:issued>
				<skos:broader rdf:resource="http://purl.org/heritagedata/schemes/4/concepts/502348" />
				<skos:scopeNote xml:lang="en">Unsorted chronological sequence of text summarising a site record, or recording external references.</skos:scopeNote>
			</skos:Concept>
		</skos:narrower>
		<skos:narrower>
			<skos:Concept rdf:about="http://purl.org/heritagedata/schemes/4/concepts/507002">
				<skos:inScheme rdf:resource="http://purl.org/heritagedata/schemes/4" />
				<dcterms:identifier>http://purl.org/heritagedata/schemes/4/concepts/507002</dcterms:identifier>
				<cc:license rdf:resource="http://reference.data.gov.uk/id/open-government-licence" />
				<cc:attributionURL rdf:resource="http://www.rcahms.gov.uk" />
				<cc:attributionName xml:lang="en">RCAHMS</cc:attributionName>
				<dcterms:publisher rdf:resource="http://www.rcahms.gov.uk" />
				<skos:prefLabel xml:lang="en">DCC NOTE</skos:prefLabel>
				<dcterms:created rdf:datatype="http://www.w3.org/2001/XMLSchema#dateTime">2012-08-31T14:43:28</dcterms:created>
				<dcterms:modified rdf:datatype="http://www.w3.org/2001/XMLSchema#dateTime">2012-08-31T14:45:45</dcterms:modified>
				<dcterms:issued rdf:datatype="http://www.w3.org/2001/XMLSchema#dateTime">2013-07-17T10:08:40</dcterms:issued>
				<skos:broader rdf:resource="http://purl.org/heritagedata/schemes/4/concepts/502348" />
				<skos:scopeNote xml:lang="en">Informal notes from Dundee City Council staff concerning a site and not derived from field visits or inspections or from a published account e.g. Inventory. Text should be accompanied by 'Information from Dundee City Council (Initials) DATE YEAR.</skos:scopeNote>
			</skos:Concept>
		</skos:narrower>
		<skos:narrower>
			<skos:Concept rdf:about="http://purl.org/heritagedata/schemes/4/concepts/507003">
				<skos:inScheme rdf:resource="http://purl.org/heritagedata/schemes/4" />
				<dcterms:identifier>http://purl.org/heritagedata/schemes/4/concepts/507003</dcterms:identifier>
				<cc:license rdf:resource="http://reference.data.gov.uk/id/open-government-licence" />
				<cc:attributionURL rdf:resource="http://www.rcahms.gov.uk" />
				<cc:attributionName xml:lang="en">RCAHMS</cc:attributionName>
				<dcterms:publisher rdf:resource="http://www.rcahms.gov.uk" />
				<skos:prefLabel xml:lang="en">EDC NOTE</skos:prefLabel>
				<dcterms:created rdf:datatype="http://www.w3.org/2001/XMLSchema#dateTime">2012-08-31T14:44:36</dcterms:created>
				<dcterms:modified rdf:datatype="http://www.w3.org/2001/XMLSchema#dateTime">2012-08-31T14:46:38</dcterms:modified>
				<dcterms:issued rdf:datatype="http://www.w3.org/2001/XMLSchema#dateTime">2013-07-17T10:08:40</dcterms:issued>
				<skos:broader rdf:resource="http://purl.org/heritagedata/schemes/4/concepts/502348" />
				<skos:scopeNote xml:lang="en">Informal notes from East Dunbartonshire Council staff concerning a site and not derived from field visits or inspections or from a published account e.g. Inventory. Text should be accompanied by 'Information from East Dunbartonshire Council (Initials) DATE YEAR.</skos:scopeNote>
			</skos:Concept>
		</skos:narrower>
		<skos:narrower>
			<skos:Concept rdf:about="http://purl.org/heritagedata/schemes/4/concepts/507062">
				<skos:inScheme rdf:resource="http://purl.org/heritagedata/schemes/4" />
				<dcterms:identifier>http://purl.org/heritagedata/schemes/4/concepts/507062</dcterms:identifier>
				<cc:license rdf:resource="http://reference.data.gov.uk/id/open-government-licence" />
				<cc:attributionURL rdf:resource="http://www.rcahms.gov.uk" />
				<cc:attributionName xml:lang="en">RCAHMS</cc:attributionName>
				<dcterms:publisher rdf:resource="http://www.rcahms.gov.uk" />
				<skos:prefLabel xml:lang="en">TTU NOTE</skos:prefLabel>
				<dcterms:created rdf:datatype="http://www.w3.org/2001/XMLSchema#dateTime">2012-11-12T15:27:39</dcterms:created>
				<dcterms:modified rdf:datatype="http://www.w3.org/2001/XMLSchema#dateTime">2012-11-12T15:35:36</dcterms:modified>
				<dcterms:issued rdf:datatype="http://www.w3.org/2001/XMLSchema#dateTime">2013-07-17T10:08:40</dcterms:issued>
				<skos:broader rdf:resource="http://purl.org/heritagedata/schemes/4/concepts/502348" />
				<skos:scopeNote xml:lang="en">Informal notes from Treasure Trove Unit staff concerning a site and not derived from field visits or inspections or from a published account e.g. Inventory. Text should be accompanied by 'Information from Treasure Trove Unit (Initials) DATE YEAR.</skos:scopeNote>
			</skos:Concept>
		</skos:narrower>
		<skos:narrower>
			<skos:Concept rdf:about="http://purl.org/heritagedata/schemes/4/concepts/507063">
				<skos:inScheme rdf:resource="http://purl.org/heritagedata/schemes/4" />
				<dcterms:identifier>http://purl.org/heritagedata/schemes/4/concepts/507063</dcterms:identifier>
				<cc:license rdf:resource="http://reference.data.gov.uk/id/open-government-licence" />
				<cc:attributionURL rdf:resource="http://www.rcahms.gov.uk" />
				<cc:attributionName xml:lang="en">RCAHMS</cc:attributionName>
				<dcterms:publisher rdf:resource="http://www.rcahms.gov.uk" />
				<skos:prefLabel xml:lang="en">SCA NOTE</skos:prefLabel>
				<dcterms:created rdf:datatype="http://www.w3.org/2001/XMLSchema#dateTime">2012-11-12T15:28:26</dcterms:created>
				<dcterms:modified rdf:datatype="http://www.w3.org/2001/XMLSchema#dateTime">2012-11-12T15:29:51</dcterms:modified>
				<dcterms:issued rdf:datatype="http://www.w3.org/2001/XMLSchema#dateTime">2013-07-17T10:08:40</dcterms:issued>
				<skos:broader rdf:resource="http://purl.org/heritagedata/schemes/4/concepts/502348" />
				<skos:scopeNote xml:lang="en">Informal notes from Scottish Canals staff concerning a site and not derived from field visits or inspections or from a published account e.g. Inventory. Text should be accompanied by 'Information from Scottish Canals (Initials) DATE YEAR.</skos:scopeNote>
			</skos:Concept>
		</skos:narrower>
		<skos:scopeNote xml:lang="en">Covers contextual accounts. Also to be used to store text produced by a variety of HLF projects such as Recording Your Heritage Online, Accessing Scotland's Past and Sir Basil Spence.</skos:scopeNote>
	</skos:Concept>
	<skos:Concept rdf:about="http://purl.org/heritagedata/schemes/4/concepts/502350">
		<skos:inScheme rdf:resource="http://purl.org/heritagedata/schemes/4" />
		<dcterms:identifier>http://purl.org/heritagedata/schemes/4/concepts/502350</dcterms:identifier>
		<cc:license rdf:resource="http://reference.data.gov.uk/id/open-government-licence" />
		<cc:attributionURL rdf:resource="http://www.rcahms.gov.uk" />
		<cc:attributionName xml:lang="en">RCAHMS</cc:attributionName>
		<dcterms:publisher rdf:resource="http://www.rcahms.gov.uk" />
		<skos:topConceptOf rdf:resource="http://purl.org/heritagedata/schemes/4" />
		<skos:prefLabel xml:lang="en">SCIENTIFIC DATING</skos:prefLabel>
		<dcterms:created rdf:datatype="http://www.w3.org/2001/XMLSchema#dateTime">2007-05-30T09:19:56</dcterms:created>
		<dcterms:modified rdf:datatype="http://www.w3.org/2001/XMLSchema#dateTime">2007-11-30T10:23:59</dcterms:modified>
		<dcterms:issued rdf:datatype="http://www.w3.org/2001/XMLSchema#dateTime">2013-07-17T10:08:40</dcterms:issued>
		<skos:narrower>
			<skos:Concept rdf:about="http://purl.org/heritagedata/schemes/4/concepts/502352">
				<skos:inScheme rdf:resource="http://purl.org/heritagedata/schemes/4" />
				<dcterms:identifier>http://purl.org/heritagedata/schemes/4/concepts/502352</dcterms:identifier>
				<cc:license rdf:resource="http://reference.data.gov.uk/id/open-government-licence" />
				<cc:attributionURL rdf:resource="http://www.rcahms.gov.uk" />
				<cc:attributionName xml:lang="en">RCAHMS</cc:attributionName>
				<dcterms:publisher rdf:resource="http://www.rcahms.gov.uk" />
				<skos:prefLabel xml:lang="en">RADIOCARBON DATING</skos:prefLabel>
				<dcterms:created rdf:datatype="http://www.w3.org/2001/XMLSchema#dateTime">2007-05-30T13:30:07</dcterms:created>
				<dcterms:modified rdf:datatype="http://www.w3.org/2001/XMLSchema#dateTime">2007-06-05T13:57:09</dcterms:modified>
				<dcterms:issued rdf:datatype="http://www.w3.org/2001/XMLSchema#dateTime">2013-07-17T10:08:40</dcterms:issued>
				<skos:broader rdf:resource="http://purl.org/heritagedata/schemes/4/concepts/502350" />
				<skos:scopeNote xml:lang="en">Radiocarbon dating measures the rate of decay in the naturally occurring isotope carbon-14 (14C) to determine the approximate age of an organic object.  Uncalibrated (or raw) radiocarbon ages are usually reported in radiocarbon years 'Before Present' (BP), 'Present' being defined as AD 1950. Such raw ages can be calibrated to give calendar dates.</skos:scopeNote>
			</skos:Concept>
		</skos:narrower>
		<skos:narrower>
			<skos:Concept rdf:about="http://purl.org/heritagedata/schemes/4/concepts/502353">
				<skos:inScheme rdf:resource="http://purl.org/heritagedata/schemes/4" />
				<dcterms:identifier>http://purl.org/heritagedata/schemes/4/concepts/502353</dcterms:identifier>
				<cc:license rdf:resource="http://reference.data.gov.uk/id/open-government-licence" />
				<cc:attributionURL rdf:resource="http://www.rcahms.gov.uk" />
				<cc:attributionName xml:lang="en">RCAHMS</cc:attributionName>
				<dcterms:publisher rdf:resource="http://www.rcahms.gov.uk" />
				<skos:prefLabel xml:lang="en">DENDROCHRONOLOGY</skos:prefLabel>
				<dcterms:created rdf:datatype="http://www.w3.org/2001/XMLSchema#dateTime">2007-05-30T13:41:07</dcterms:created>
				<dcterms:modified rdf:datatype="http://www.w3.org/2001/XMLSchema#dateTime">2007-05-30T13:45:10</dcterms:modified>
				<dcterms:issued rdf:datatype="http://www.w3.org/2001/XMLSchema#dateTime">2013-07-17T10:08:40</dcterms:issued>
				<skos:broader rdf:resource="http://purl.org/heritagedata/schemes/4/concepts/502350" />
				<skos:scopeNote xml:lang="en">The scientific analysis of the annual growth rings of trees to determine the absolute age of a piece of timber.</skos:scopeNote>
			</skos:Concept>
		</skos:narrower>
		<skos:narrower>
			<skos:Concept rdf:about="http://purl.org/heritagedata/schemes/4/concepts/502354">
				<skos:inScheme rdf:resource="http://purl.org/heritagedata/schemes/4" />
				<dcterms:identifier>http://purl.org/heritagedata/schemes/4/concepts/502354</dcterms:identifier>
				<cc:license rdf:resource="http://reference.data.gov.uk/id/open-government-licence" />
				<cc:attributionURL rdf:resource="http://www.rcahms.gov.uk" />
				<cc:attributionName xml:lang="en">RCAHMS</cc:attributionName>
				<dcterms:publisher rdf:resource="http://www.rcahms.gov.uk" />
				<skos:prefLabel xml:lang="en">THERMOLUMINESCENCE DATING</skos:prefLabel>
				<dcterms:created rdf:datatype="http://www.w3.org/2001/XMLSchema#dateTime">2007-05-30T13:45:58</dcterms:created>
				<dcterms:modified rdf:datatype="http://www.w3.org/2001/XMLSchema#dateTime">2007-05-30T13:59:03</dcterms:modified>
				<dcterms:issued rdf:datatype="http://www.w3.org/2001/XMLSchema#dateTime">2013-07-17T10:08:40</dcterms:issued>
				<skos:broader rdf:resource="http://purl.org/heritagedata/schemes/4/concepts/502350" />
				<skos:scopeNote xml:lang="en">The determination of a date through the measurement of the absorbed radiation energy in crystals that have either been heated (e.g. ceramics or hearths) or exposed to sunlight (sediments).</skos:scopeNote>
			</skos:Concept>
		</skos:narrower>
		<skos:narrower>
			<skos:Concept rdf:about="http://purl.org/heritagedata/schemes/4/concepts/505341">
				<skos:inScheme rdf:resource="http://purl.org/heritagedata/schemes/4" />
				<dcterms:identifier>http://purl.org/heritagedata/schemes/4/concepts/505341</dcterms:identifier>
				<cc:license rdf:resource="http://reference.data.gov.uk/id/open-government-licence" />
				<cc:attributionURL rdf:resource="http://www.rcahms.gov.uk" />
				<cc:attributionName xml:lang="en">RCAHMS</cc:attributionName>
				<dcterms:publisher rdf:resource="http://www.rcahms.gov.uk" />
				<skos:prefLabel xml:lang="en">ISOTOPE ANALYSIS</skos:prefLabel>
				<dcterms:created rdf:datatype="http://www.w3.org/2001/XMLSchema#dateTime">2010-08-13T10:35:34</dcterms:created>
				<dcterms:modified rdf:datatype="http://www.w3.org/2001/XMLSchema#dateTime">2010-08-13T10:36:38</dcterms:modified>
				<dcterms:issued rdf:datatype="http://www.w3.org/2001/XMLSchema#dateTime">2013-07-17T10:08:40</dcterms:issued>
				<skos:broader rdf:resource="http://purl.org/heritagedata/schemes/4/concepts/502350" />
				<skos:scopeNote xml:lang="en">A technique used for the analysis of bone to identify  information relating to diet and migration. The isotopic signatures of carbon and nitrogen may be used to reconstruct diet and the isotopic signature of oxygen to determine geographic information.</skos:scopeNote>
			</skos:Concept>
		</skos:narrower>
		<skos:scopeNote xml:lang="en">Records the type of method used to obtain dating evidence e.g. radiocarbon dates. In time, additional pages will link to details about specific sample dates.</skos:scopeNote>
	</skos:Concept>
	<skos:Concept rdf:about="http://purl.org/heritagedata/schemes/4/concepts/502349">
		<skos:inScheme rdf:resource="http://purl.org/heritagedata/schemes/4" />
		<dcterms:identifier>http://purl.org/heritagedata/schemes/4/concepts/502349</dcterms:identifier>
		<cc:license rdf:resource="http://reference.data.gov.uk/id/open-government-licence" />
		<cc:attributionURL rdf:resource="http://www.rcahms.gov.uk" />
		<cc:attributionName xml:lang="en">RCAHMS</cc:attributionName>
		<dcterms:publisher rdf:resource="http://www.rcahms.gov.uk" />
		<skos:topConceptOf rdf:resource="http://purl.org/heritagedata/schemes/4" />
		<skos:prefLabel xml:lang="en">SYSTEM UPDATE</skos:prefLabel>
		<dcterms:created rdf:datatype="http://www.w3.org/2001/XMLSchema#dateTime">2007-05-30T09:19:50</dcterms:created>
		<dcterms:modified rdf:datatype="http://www.w3.org/2001/XMLSchema#dateTime">2007-11-30T10:25:03</dcterms:modified>
		<dcterms:issued rdf:datatype="http://www.w3.org/2001/XMLSchema#dateTime">2013-07-17T10:08:40</dcterms:issued>
		<skos:narrower>
			<skos:Concept rdf:about="http://purl.org/heritagedata/schemes/4/concepts/502505">
				<skos:inScheme rdf:resource="http://purl.org/heritagedata/schemes/4" />
				<dcterms:identifier>http://purl.org/heritagedata/schemes/4/concepts/502505</dcterms:identifier>
				<cc:license rdf:resource="http://reference.data.gov.uk/id/open-government-licence" />
				<cc:attributionURL rdf:resource="http://www.rcahms.gov.uk" />
				<cc:attributionName xml:lang="en">RCAHMS</cc:attributionName>
				<dcterms:publisher rdf:resource="http://www.rcahms.gov.uk" />
				<skos:prefLabel xml:lang="en">CREATION EVENT</skos:prefLabel>
				<dcterms:created rdf:datatype="http://www.w3.org/2001/XMLSchema#dateTime">2007-06-04T13:15:28</dcterms:created>
				<dcterms:modified rdf:datatype="http://www.w3.org/2001/XMLSchema#dateTime">2007-06-04T13:16:50</dcterms:modified>
				<dcterms:issued rdf:datatype="http://www.w3.org/2001/XMLSchema#dateTime">2013-07-17T10:08:40</dcterms:issued>
				<skos:broader rdf:resource="http://purl.org/heritagedata/schemes/4/concepts/502349" />
				<skos:scopeNote xml:lang="en">Use for records where no event has been entered once the table has gone live.</skos:scopeNote>
			</skos:Concept>
		</skos:narrower>
		<skos:narrower>
			<skos:Concept rdf:about="http://purl.org/heritagedata/schemes/4/concepts/502506">
				<skos:inScheme rdf:resource="http://purl.org/heritagedata/schemes/4" />
				<dcterms:identifier>http://purl.org/heritagedata/schemes/4/concepts/502506</dcterms:identifier>
				<cc:license rdf:resource="http://reference.data.gov.uk/id/open-government-licence" />
				<cc:attributionURL rdf:resource="http://www.rcahms.gov.uk" />
				<cc:attributionName xml:lang="en">RCAHMS</cc:attributionName>
				<dcterms:publisher rdf:resource="http://www.rcahms.gov.uk" />
				<skos:prefLabel xml:lang="en">NO EVENT</skos:prefLabel>
				<dcterms:created rdf:datatype="http://www.w3.org/2001/XMLSchema#dateTime">2007-06-04T13:17:09</dcterms:created>
				<dcterms:modified rdf:datatype="http://www.w3.org/2001/XMLSchema#dateTime">2007-06-04T13:17:56</dcterms:modified>
				<dcterms:issued rdf:datatype="http://www.w3.org/2001/XMLSchema#dateTime">2013-07-17T10:08:40</dcterms:issued>
				<skos:broader rdf:resource="http://purl.org/heritagedata/schemes/4/concepts/502349" />
				<skos:scopeNote xml:lang="en">Use for records created before Events table was introduced and for which there are no events.</skos:scopeNote>
			</skos:Concept>
		</skos:narrower>
		<skos:narrower>
			<skos:Concept rdf:about="http://purl.org/heritagedata/schemes/4/concepts/502507">
				<skos:inScheme rdf:resource="http://purl.org/heritagedata/schemes/4" />
				<dcterms:identifier>http://purl.org/heritagedata/schemes/4/concepts/502507</dcterms:identifier>
				<cc:license rdf:resource="http://reference.data.gov.uk/id/open-government-licence" />
				<cc:attributionURL rdf:resource="http://www.rcahms.gov.uk" />
				<cc:attributionName xml:lang="en">RCAHMS</cc:attributionName>
				<dcterms:publisher rdf:resource="http://www.rcahms.gov.uk" />
				<skos:prefLabel xml:lang="en">SYSTEM EVENT</skos:prefLabel>
				<dcterms:created rdf:datatype="http://www.w3.org/2001/XMLSchema#dateTime">2007-06-04T13:18:13</dcterms:created>
				<dcterms:modified rdf:datatype="http://www.w3.org/2001/XMLSchema#dateTime">2007-06-04T13:18:47</dcterms:modified>
				<dcterms:issued rdf:datatype="http://www.w3.org/2001/XMLSchema#dateTime">2013-07-17T10:08:40</dcterms:issued>
				<skos:broader rdf:resource="http://purl.org/heritagedata/schemes/4/concepts/502349" />
				<skos:scopeNote xml:lang="en">The record has been updated automatically by the computer.</skos:scopeNote>
			</skos:Concept>
		</skos:narrower>
		<skos:scopeNote xml:lang="en">Events that have occurred within the actual RCAHMS database e.g. data migration.</skos:scopeNote>
	</skos:Concept>
	<skos:Concept rdf:about="http://purl.org/heritagedata/schemes/4/concepts/503057">
		<skos:inScheme rdf:resource="http://purl.org/heritagedata/schemes/4" />
		<dcterms:identifier>http://purl.org/heritagedata/schemes/4/concepts/503057</dcterms:identifier>
		<cc:license rdf:resource="http://reference.data.gov.uk/id/open-government-licence" />
		<cc:attributionURL rdf:resource="http://www.rcahms.gov.uk" />
		<cc:attributionName xml:lang="en">RCAHMS</cc:attributionName>
		<dcterms:publisher rdf:resource="http://www.rcahms.gov.uk" />
		<skos:prefLabel xml:lang="en">SKETCH DRAWING</skos:prefLabel>
		<dcterms:created rdf:datatype="http://www.w3.org/2001/XMLSchema#dateTime">2007-12-17T17:29:27</dcterms:created>
		<dcterms:modified rdf:datatype="http://www.w3.org/2001/XMLSchema#dateTime">2007-12-17T17:31:47</dcterms:modified>
		<dcterms:issued rdf:datatype="http://www.w3.org/2001/XMLSchema#dateTime">2013-07-17T10:08:40</dcterms:issued>
		<skos:broader rdf:resource="http://purl.org/heritagedata/schemes/4/concepts/502362" />
		<skos:broader rdf:resource="http://purl.org/heritagedata/schemes/4/concepts/502432" />
		<skos:scopeNote xml:lang="en">Sketches and other drawings of buildings, monuments or objects. Not made to scale.</skos:scopeNote>
	</skos:Concept>
	<skos:Concept rdf:about="http://purl.org/heritagedata/schemes/4/concepts/503120">
		<skos:inScheme rdf:resource="http://purl.org/heritagedata/schemes/4" />
		<dcterms:identifier>http://purl.org/heritagedata/schemes/4/concepts/503120</dcterms:identifier>
		<cc:license rdf:resource="http://reference.data.gov.uk/id/open-government-licence" />
		<cc:attributionURL rdf:resource="http://www.rcahms.gov.uk" />
		<cc:attributionName xml:lang="en">RCAHMS</cc:attributionName>
		<dcterms:publisher rdf:resource="http://www.rcahms.gov.uk" />
		<skos:prefLabel xml:lang="en">GEOCHEMICAL SURVEY</skos:prefLabel>
		<dcterms:created rdf:datatype="http://www.w3.org/2001/XMLSchema#dateTime">2007-12-20T13:57:25</dcterms:created>
		<dcterms:modified rdf:datatype="http://www.w3.org/2001/XMLSchema#dateTime">2007-12-20T13:58:10</dcterms:modified>
		<dcterms:issued rdf:datatype="http://www.w3.org/2001/XMLSchema#dateTime">2013-07-17T10:08:40</dcterms:issued>
		<skos:narrower>
			<skos:Concept rdf:about="http://purl.org/heritagedata/schemes/4/concepts/504440">
				<skos:inScheme rdf:resource="http://purl.org/heritagedata/schemes/4" />
				<dcterms:identifier>http://purl.org/heritagedata/schemes/4/concepts/504440</dcterms:identifier>
				<cc:license rdf:resource="http://reference.data.gov.uk/id/open-government-licence" />
				<cc:attributionURL rdf:resource="http://www.rcahms.gov.uk" />
				<cc:attributionName xml:lang="en">RCAHMS</cc:attributionName>
				<dcterms:publisher rdf:resource="http://www.rcahms.gov.uk" />
				<skos:prefLabel xml:lang="en">PHOSPHATE SURVEY</skos:prefLabel>
				<dcterms:created rdf:datatype="http://www.w3.org/2001/XMLSchema#dateTime">2009-06-29T15:03:17</dcterms:created>
				<dcterms:modified rdf:datatype="http://www.w3.org/2001/XMLSchema#dateTime">2009-06-29T15:04:57</dcterms:modified>
				<dcterms:issued rdf:datatype="http://www.w3.org/2001/XMLSchema#dateTime">2013-07-17T10:08:40</dcterms:issued>
				<skos:broader rdf:resource="http://purl.org/heritagedata/schemes/4/concepts/503120" />
				<skos:scopeNote xml:lang="en">The systematic collection of soil samples from a defined study area which are then analysed for phosphate. Elevated concentrations of phoshates are a generalised signature of human activity in soils.</skos:scopeNote>
			</skos:Concept>
		</skos:narrower>
		<skos:broader rdf:resource="http://purl.org/heritagedata/schemes/4/concepts/502413" />
		<skos:scopeNote xml:lang="en">the location or identification of areas of past land use by means of the chemical composition of the soil.</skos:scopeNote>
	</skos:Concept>
	<skos:Concept rdf:about="http://purl.org/heritagedata/schemes/4/concepts/502346">
		<skos:inScheme rdf:resource="http://purl.org/heritagedata/schemes/4" />
		<dcterms:identifier>http://purl.org/heritagedata/schemes/4/concepts/502346</dcterms:identifier>
		<cc:license rdf:resource="http://reference.data.gov.uk/id/open-government-licence" />
		<cc:attributionURL rdf:resource="http://www.rcahms.gov.uk" />
		<cc:attributionName xml:lang="en">RCAHMS</cc:attributionName>
		<dcterms:publisher rdf:resource="http://www.rcahms.gov.uk" />
		<skos:topConceptOf rdf:resource="http://purl.org/heritagedata/schemes/4" />
		<skos:prefLabel xml:lang="en">RECORDING</skos:prefLabel>
		<dcterms:created rdf:datatype="http://www.w3.org/2001/XMLSchema#dateTime">2007-05-30T09:19:25</dcterms:created>
		<dcterms:modified rdf:datatype="http://www.w3.org/2001/XMLSchema#dateTime">2008-01-07T10:43:49</dcterms:modified>
		<dcterms:issued rdf:datatype="http://www.w3.org/2001/XMLSchema#dateTime">2013-07-17T10:08:40</dcterms:issued>
		<skos:narrower rdf:resource="http://purl.org/heritagedata/schemes/4/concepts/502402" />
		<skos:narrower rdf:resource="http://purl.org/heritagedata/schemes/4/concepts/502413" />
		<skos:narrower rdf:resource="http://purl.org/heritagedata/schemes/4/concepts/502416" />
		<skos:narrower>
			<skos:Concept rdf:about="http://purl.org/heritagedata/schemes/4/concepts/502551">
				<skos:inScheme rdf:resource="http://purl.org/heritagedata/schemes/4" />
				<dcterms:identifier>http://purl.org/heritagedata/schemes/4/concepts/502551</dcterms:identifier>
				<cc:license rdf:resource="http://reference.data.gov.uk/id/open-government-licence" />
				<cc:attributionURL rdf:resource="http://www.rcahms.gov.uk" />
				<cc:attributionName xml:lang="en">RCAHMS</cc:attributionName>
				<dcterms:publisher rdf:resource="http://www.rcahms.gov.uk" />
				<skos:prefLabel xml:lang="en">DESK BASED ASSESSMENT</skos:prefLabel>
				<dcterms:created rdf:datatype="http://www.w3.org/2001/XMLSchema#dateTime">2007-06-06T09:26:50</dcterms:created>
				<dcterms:modified rdf:datatype="http://www.w3.org/2001/XMLSchema#dateTime">2009-07-15T15:00:46</dcterms:modified>
				<dcterms:issued rdf:datatype="http://www.w3.org/2001/XMLSchema#dateTime">2013-07-17T10:08:40</dcterms:issued>
				<skos:broader rdf:resource="http://purl.org/heritagedata/schemes/4/concepts/502346" />
				<skos:scopeNote xml:lang="en">Systematic search of available heritage databases, analysis of aerial photography,  documentary and cartographic sources normally undertaken as part of an infrastructure development.</skos:scopeNote>
			</skos:Concept>
		</skos:narrower>
		<skos:narrower rdf:resource="http://purl.org/heritagedata/schemes/4/concepts/502401" />
		<skos:narrower>
			<skos:Concept rdf:about="http://purl.org/heritagedata/schemes/4/concepts/505761">
				<skos:inScheme rdf:resource="http://purl.org/heritagedata/schemes/4" />
				<dcterms:identifier>http://purl.org/heritagedata/schemes/4/concepts/505761</dcterms:identifier>
				<cc:license rdf:resource="http://reference.data.gov.uk/id/open-government-licence" />
				<cc:attributionURL rdf:resource="http://www.rcahms.gov.uk" />
				<cc:attributionName xml:lang="en">RCAHMS</cc:attributionName>
				<dcterms:publisher rdf:resource="http://www.rcahms.gov.uk" />
				<skos:prefLabel xml:lang="en">CHARACTERISATION</skos:prefLabel>
				<dcterms:created rdf:datatype="http://www.w3.org/2001/XMLSchema#dateTime">2011-04-19T14:05:54</dcterms:created>
				<dcterms:modified rdf:datatype="http://www.w3.org/2001/XMLSchema#dateTime">2011-06-09T10:18:37</dcterms:modified>
				<dcterms:issued rdf:datatype="http://www.w3.org/2001/XMLSchema#dateTime">2013-07-17T10:08:40</dcterms:issued>
				<skos:broader rdf:resource="http://purl.org/heritagedata/schemes/4/concepts/502346" />
				<skos:scopeNote xml:lang="en">Analysis of the historic environment through desk-based assessment and field visits, resulting in digital map showing a) changing patterns of land use by Category, Type, Period or Relict Period (Historic Landuse Assessment) or b) Areas of Townscape Character defined by historical development, topography and distinctive features which survive to create present character of areas within towns (Urban Survey).</skos:scopeNote>
			</skos:Concept>
		</skos:narrower>
		<skos:scopeNote xml:lang="en">Events that lead to either the initial recognition or definition of a monument or any subsequent work on that site.</skos:scopeNote>
	</skos:Concept>
	<skos:Concept rdf:about="http://purl.org/heritagedata/schemes/4/concepts/504000">
		<skos:inScheme rdf:resource="http://purl.org/heritagedata/schemes/4" />
		<dcterms:identifier>http://purl.org/heritagedata/schemes/4/concepts/504000</dcterms:identifier>
		<cc:license rdf:resource="http://reference.data.gov.uk/id/open-government-licence" />
		<cc:attributionURL rdf:resource="http://www.rcahms.gov.uk" />
		<cc:attributionName xml:lang="en">RCAHMS</cc:attributionName>
		<dcterms:publisher rdf:resource="http://www.rcahms.gov.uk" />
		<skos:topConceptOf rdf:resource="http://purl.org/heritagedata/schemes/4" />
		<skos:prefLabel xml:lang="en">PUBLIC CONTRIBUTION</skos:prefLabel>
		<dcterms:created rdf:datatype="http://www.w3.org/2001/XMLSchema#dateTime">2009-03-04T10:27:23</dcterms:created>
		<dcterms:modified rdf:datatype="http://www.w3.org/2001/XMLSchema#dateTime">2009-03-04T10:27:42</dcterms:modified>
		<dcterms:issued rdf:datatype="http://www.w3.org/2001/XMLSchema#dateTime">2013-07-17T10:08:40</dcterms:issued>
		<skos:narrower>
			<skos:Concept rdf:about="http://purl.org/heritagedata/schemes/4/concepts/504001">
				<skos:inScheme rdf:resource="http://purl.org/heritagedata/schemes/4" />
				<dcterms:identifier>http://purl.org/heritagedata/schemes/4/concepts/504001</dcterms:identifier>
				<cc:license rdf:resource="http://reference.data.gov.uk/id/open-government-licence" />
				<cc:attributionURL rdf:resource="http://www.rcahms.gov.uk" />
				<cc:attributionName xml:lang="en">RCAHMS</cc:attributionName>
				<dcterms:publisher rdf:resource="http://www.rcahms.gov.uk" />
				<skos:prefLabel xml:lang="en">PUBLIC COLLECTION ITEM COMMENT</skos:prefLabel>
				<dcterms:created rdf:datatype="http://www.w3.org/2001/XMLSchema#dateTime">2009-03-04T10:28:25</dcterms:created>
				<dcterms:modified rdf:datatype="http://www.w3.org/2001/XMLSchema#dateTime">2009-03-04T10:28:49</dcterms:modified>
				<dcterms:issued rdf:datatype="http://www.w3.org/2001/XMLSchema#dateTime">2013-07-17T10:08:40</dcterms:issued>
				<skos:broader rdf:resource="http://purl.org/heritagedata/schemes/4/concepts/504000" />
				<skos:scopeNote xml:lang="en">A public comment on Canmore about an RCAHMS image</skos:scopeNote>
			</skos:Concept>
		</skos:narrower>
		<skos:narrower>
			<skos:Concept rdf:about="http://purl.org/heritagedata/schemes/4/concepts/504002">
				<skos:inScheme rdf:resource="http://purl.org/heritagedata/schemes/4" />
				<dcterms:identifier>http://purl.org/heritagedata/schemes/4/concepts/504002</dcterms:identifier>
				<cc:license rdf:resource="http://reference.data.gov.uk/id/open-government-licence" />
				<cc:attributionURL rdf:resource="http://www.rcahms.gov.uk" />
				<cc:attributionName xml:lang="en">RCAHMS</cc:attributionName>
				<dcterms:publisher rdf:resource="http://www.rcahms.gov.uk" />
				<skos:prefLabel xml:lang="en">PUBLIC NON-RCAHMS IMAGE COMMENT</skos:prefLabel>
				<dcterms:created rdf:datatype="http://www.w3.org/2001/XMLSchema#dateTime">2009-03-04T10:29:10</dcterms:created>
				<dcterms:modified rdf:datatype="http://www.w3.org/2001/XMLSchema#dateTime">2009-03-04T10:29:23</dcterms:modified>
				<dcterms:issued rdf:datatype="http://www.w3.org/2001/XMLSchema#dateTime">2013-07-17T10:08:40</dcterms:issued>
				<skos:broader rdf:resource="http://purl.org/heritagedata/schemes/4/concepts/504000" />
				<skos:scopeNote xml:lang="en">A public comment on Canmore about a non-RCAHMS image</skos:scopeNote>
			</skos:Concept>
		</skos:narrower>
		<skos:narrower>
			<skos:Concept rdf:about="http://purl.org/heritagedata/schemes/4/concepts/504003">
				<skos:inScheme rdf:resource="http://purl.org/heritagedata/schemes/4" />
				<dcterms:identifier>http://purl.org/heritagedata/schemes/4/concepts/504003</dcterms:identifier>
				<cc:license rdf:resource="http://reference.data.gov.uk/id/open-government-licence" />
				<cc:attributionURL rdf:resource="http://www.rcahms.gov.uk" />
				<cc:attributionName xml:lang="en">RCAHMS</cc:attributionName>
				<dcterms:publisher rdf:resource="http://www.rcahms.gov.uk" />
				<skos:prefLabel xml:lang="en">PUBLIC SITE COMMENT</skos:prefLabel>
				<dcterms:created rdf:datatype="http://www.w3.org/2001/XMLSchema#dateTime">2009-03-04T10:29:35</dcterms:created>
				<dcterms:modified rdf:datatype="http://www.w3.org/2001/XMLSchema#dateTime">2009-03-04T10:29:49</dcterms:modified>
				<dcterms:issued rdf:datatype="http://www.w3.org/2001/XMLSchema#dateTime">2013-07-17T10:08:40</dcterms:issued>
				<skos:broader rdf:resource="http://purl.org/heritagedata/schemes/4/concepts/504000" />
				<skos:scopeNote xml:lang="en">A public comment on Canmore about an RCAHMS site</skos:scopeNote>
			</skos:Concept>
		</skos:narrower>
		<skos:scopeNote xml:lang="en">Contribution from the public via Canmore</skos:scopeNote>
	</skos:Concept>
	<skos:Concept rdf:about="http://purl.org/heritagedata/schemes/4/concepts/505721">
		<skos:inScheme rdf:resource="http://purl.org/heritagedata/schemes/4" />
		<dcterms:identifier>http://purl.org/heritagedata/schemes/4/concepts/505721</dcterms:identifier>
		<cc:license rdf:resource="http://reference.data.gov.uk/id/open-government-licence" />
		<cc:attributionURL rdf:resource="http://www.rcahms.gov.uk" />
		<cc:attributionName xml:lang="en">RCAHMS</cc:attributionName>
		<dcterms:publisher rdf:resource="http://www.rcahms.gov.uk" />
		<skos:topConceptOf rdf:resource="http://purl.org/heritagedata/schemes/4" />
		<skos:prefLabel xml:lang="en">COLLECTIONS MANAGMENT</skos:prefLabel>
		<dcterms:created rdf:datatype="http://www.w3.org/2001/XMLSchema#dateTime">2011-04-12T15:58:20</dcterms:created>
		<dcterms:modified rdf:datatype="http://www.w3.org/2001/XMLSchema#dateTime">2011-04-12T15:58:20</dcterms:modified>
		<dcterms:issued rdf:datatype="http://www.w3.org/2001/XMLSchema#dateTime">2013-07-17T10:08:40</dcterms:issued>
		<skos:narrower>
			<skos:Concept rdf:about="http://purl.org/heritagedata/schemes/4/concepts/505722">
				<skos:inScheme rdf:resource="http://purl.org/heritagedata/schemes/4" />
				<dcterms:identifier>http://purl.org/heritagedata/schemes/4/concepts/505722</dcterms:identifier>
				<cc:license rdf:resource="http://reference.data.gov.uk/id/open-government-licence" />
				<cc:attributionURL rdf:resource="http://www.rcahms.gov.uk" />
				<cc:attributionName xml:lang="en">RCAHMS</cc:attributionName>
				<dcterms:publisher rdf:resource="http://www.rcahms.gov.uk" />
				<skos:prefLabel xml:lang="en">SPECIAL COLLECTIONS</skos:prefLabel>
				<dcterms:created rdf:datatype="http://www.w3.org/2001/XMLSchema#dateTime">2011-04-12T15:59:31</dcterms:created>
				<dcterms:modified rdf:datatype="http://www.w3.org/2001/XMLSchema#dateTime">2011-04-14T14:42:55</dcterms:modified>
				<dcterms:issued rdf:datatype="http://www.w3.org/2001/XMLSchema#dateTime">2013-07-17T10:08:40</dcterms:issued>
				<skos:broader rdf:resource="http://purl.org/heritagedata/schemes/4/concepts/505721" />
				<skos:scopeNote xml:lang="en">Type scope note here</skos:scopeNote>
			</skos:Concept>
		</skos:narrower>
		<skos:narrower>
			<skos:Concept rdf:about="http://purl.org/heritagedata/schemes/4/concepts/505741">
				<skos:inScheme rdf:resource="http://purl.org/heritagedata/schemes/4" />
				<dcterms:identifier>http://purl.org/heritagedata/schemes/4/concepts/505741</dcterms:identifier>
				<cc:license rdf:resource="http://reference.data.gov.uk/id/open-government-licence" />
				<cc:attributionURL rdf:resource="http://www.rcahms.gov.uk" />
				<cc:attributionName xml:lang="en">RCAHMS</cc:attributionName>
				<dcterms:publisher rdf:resource="http://www.rcahms.gov.uk" />
				<skos:prefLabel xml:lang="en">AUDITS</skos:prefLabel>
				<dcterms:created rdf:datatype="http://www.w3.org/2001/XMLSchema#dateTime">2011-04-14T14:41:44</dcterms:created>
				<dcterms:modified rdf:datatype="http://www.w3.org/2001/XMLSchema#dateTime">2011-04-14T14:42:13</dcterms:modified>
				<dcterms:issued rdf:datatype="http://www.w3.org/2001/XMLSchema#dateTime">2013-07-17T10:08:40</dcterms:issued>
				<skos:broader rdf:resource="http://purl.org/heritagedata/schemes/4/concepts/505721" />
				<skos:scopeNote xml:lang="en">Type scope note here</skos:scopeNote>
			</skos:Concept>
		</skos:narrower>
		<skos:scopeNote xml:lang="en">Type scope note here</skos:scopeNote>
	</skos:Concept>
	<skos:Concept rdf:about="http://purl.org/heritagedata/schemes/4/concepts/502709">
		<skos:inScheme rdf:resource="http://purl.org/heritagedata/schemes/4" />
		<dcterms:identifier>http://purl.org/heritagedata/schemes/4/concepts/502709</dcterms:identifier>
		<cc:license rdf:resource="http://reference.data.gov.uk/id/open-government-licence" />
		<cc:attributionURL rdf:resource="http://www.rcahms.gov.uk" />
		<cc:attributionName xml:lang="en">RCAHMS</cc:attributionName>
		<dcterms:publisher rdf:resource="http://www.rcahms.gov.uk" />
		<skos:prefLabel xml:lang="en">MACROFOSSIL</skos:prefLabel>
		<dcterms:created rdf:datatype="http://www.w3.org/2001/XMLSchema#dateTime">2007-07-13T12:57:12</dcterms:created>
		<dcterms:modified rdf:datatype="http://www.w3.org/2001/XMLSchema#dateTime">2007-07-13T13:02:54</dcterms:modified>
		<dcterms:issued rdf:datatype="http://www.w3.org/2001/XMLSchema#dateTime">2013-07-17T10:08:40</dcterms:issued>
		<skos:broader rdf:resource="http://purl.org/heritagedata/schemes/4/concepts/502413" />
		<skos:narrower>
			<skos:Concept rdf:about="http://purl.org/heritagedata/schemes/4/concepts/502712">
				<skos:inScheme rdf:resource="http://purl.org/heritagedata/schemes/4" />
				<dcterms:identifier>http://purl.org/heritagedata/schemes/4/concepts/502712</dcterms:identifier>
				<cc:license rdf:resource="http://reference.data.gov.uk/id/open-government-licence" />
				<cc:attributionURL rdf:resource="http://www.rcahms.gov.uk" />
				<cc:attributionName xml:lang="en">RCAHMS</cc:attributionName>
				<dcterms:publisher rdf:resource="http://www.rcahms.gov.uk" />
				<skos:prefLabel xml:lang="en">MOLLUSCAN REMAINS</skos:prefLabel>
				<dcterms:created rdf:datatype="http://www.w3.org/2001/XMLSchema#dateTime">2007-07-13T13:11:22</dcterms:created>
				<dcterms:modified rdf:datatype="http://www.w3.org/2001/XMLSchema#dateTime">2007-07-13T13:12:07</dcterms:modified>
				<dcterms:issued rdf:datatype="http://www.w3.org/2001/XMLSchema#dateTime">2013-07-17T10:08:40</dcterms:issued>
				<skos:broader rdf:resource="http://purl.org/heritagedata/schemes/4/concepts/502709" />
				<skos:scopeNote xml:lang="en">The collection, identification and analysis of molluscs (terrestrial / aquatic) from archaeological and other deposits.</skos:scopeNote>
			</skos:Concept>
		</skos:narrower>
		<skos:narrower>
			<skos:Concept rdf:about="http://purl.org/heritagedata/schemes/4/concepts/502713">
				<skos:inScheme rdf:resource="http://purl.org/heritagedata/schemes/4" />
				<dcterms:identifier>http://purl.org/heritagedata/schemes/4/concepts/502713</dcterms:identifier>
				<cc:license rdf:resource="http://reference.data.gov.uk/id/open-government-licence" />
				<cc:attributionURL rdf:resource="http://www.rcahms.gov.uk" />
				<cc:attributionName xml:lang="en">RCAHMS</cc:attributionName>
				<dcterms:publisher rdf:resource="http://www.rcahms.gov.uk" />
				<skos:prefLabel xml:lang="en">ENTOMOLOGICAL REMAINS</skos:prefLabel>
				<dcterms:created rdf:datatype="http://www.w3.org/2001/XMLSchema#dateTime">2007-07-13T13:12:32</dcterms:created>
				<dcterms:modified rdf:datatype="http://www.w3.org/2001/XMLSchema#dateTime">2007-07-13T13:13:03</dcterms:modified>
				<dcterms:issued rdf:datatype="http://www.w3.org/2001/XMLSchema#dateTime">2013-07-17T10:08:40</dcterms:issued>
				<skos:broader rdf:resource="http://purl.org/heritagedata/schemes/4/concepts/502709" />
				<skos:scopeNote xml:lang="en">The collection, identification and analysis of insects from archaeological and other deposits</skos:scopeNote>
			</skos:Concept>
		</skos:narrower>
		<skos:narrower>
			<skos:Concept rdf:about="http://purl.org/heritagedata/schemes/4/concepts/502714">
				<skos:inScheme rdf:resource="http://purl.org/heritagedata/schemes/4" />
				<dcterms:identifier>http://purl.org/heritagedata/schemes/4/concepts/502714</dcterms:identifier>
				<cc:license rdf:resource="http://reference.data.gov.uk/id/open-government-licence" />
				<cc:attributionURL rdf:resource="http://www.rcahms.gov.uk" />
				<cc:attributionName xml:lang="en">RCAHMS</cc:attributionName>
				<dcterms:publisher rdf:resource="http://www.rcahms.gov.uk" />
				<skos:prefLabel xml:lang="en">PLANT REMAINS</skos:prefLabel>
				<dcterms:created rdf:datatype="http://www.w3.org/2001/XMLSchema#dateTime">2007-07-13T13:13:25</dcterms:created>
				<dcterms:modified rdf:datatype="http://www.w3.org/2001/XMLSchema#dateTime">2009-06-29T16:59:05</dcterms:modified>
				<dcterms:issued rdf:datatype="http://www.w3.org/2001/XMLSchema#dateTime">2013-07-17T10:08:40</dcterms:issued>
				<skos:broader rdf:resource="http://purl.org/heritagedata/schemes/4/concepts/502709" />
				<skos:scopeNote xml:lang="en">The collection, identification and analysis of plant macrofossils (seeds, wood, leaves etc) from archaeological and other deposits.</skos:scopeNote>
			</skos:Concept>
		</skos:narrower>
		<skos:scopeNote xml:lang="en">Remains of animal (fauna) or plant (flora), large enough to be examined by the human eye without the aid of a microscope.</skos:scopeNote>
	</skos:Concept>
	<skos:Concept rdf:about="http://purl.org/heritagedata/schemes/4/concepts/502710">
		<skos:inScheme rdf:resource="http://purl.org/heritagedata/schemes/4" />
		<dcterms:identifier>http://purl.org/heritagedata/schemes/4/concepts/502710</dcterms:identifier>
		<cc:license rdf:resource="http://reference.data.gov.uk/id/open-government-licence" />
		<cc:attributionURL rdf:resource="http://www.rcahms.gov.uk" />
		<cc:attributionName xml:lang="en">RCAHMS</cc:attributionName>
		<dcterms:publisher rdf:resource="http://www.rcahms.gov.uk" />
		<skos:prefLabel xml:lang="en">MICROFOSSIL</skos:prefLabel>
		<dcterms:created rdf:datatype="http://www.w3.org/2001/XMLSchema#dateTime">2007-07-13T13:01:43</dcterms:created>
		<dcterms:modified rdf:datatype="http://www.w3.org/2001/XMLSchema#dateTime">2007-07-13T13:02:38</dcterms:modified>
		<dcterms:issued rdf:datatype="http://www.w3.org/2001/XMLSchema#dateTime">2013-07-17T10:08:40</dcterms:issued>
		<skos:narrower>
			<skos:Concept rdf:about="http://purl.org/heritagedata/schemes/4/concepts/502573">
				<skos:inScheme rdf:resource="http://purl.org/heritagedata/schemes/4" />
				<dcterms:identifier>http://purl.org/heritagedata/schemes/4/concepts/502573</dcterms:identifier>
				<cc:license rdf:resource="http://reference.data.gov.uk/id/open-government-licence" />
				<cc:attributionURL rdf:resource="http://www.rcahms.gov.uk" />
				<cc:attributionName xml:lang="en">RCAHMS</cc:attributionName>
				<dcterms:publisher rdf:resource="http://www.rcahms.gov.uk" />
				<skos:prefLabel xml:lang="en">POLLEN ANALYSIS</skos:prefLabel>
				<dcterms:created rdf:datatype="http://www.w3.org/2001/XMLSchema#dateTime">2007-06-08T09:15:15</dcterms:created>
				<dcterms:modified rdf:datatype="http://www.w3.org/2001/XMLSchema#dateTime">2007-06-08T09:19:30</dcterms:modified>
				<dcterms:issued rdf:datatype="http://www.w3.org/2001/XMLSchema#dateTime">2013-07-17T10:08:40</dcterms:issued>
				<skos:broader rdf:resource="http://purl.org/heritagedata/schemes/4/concepts/502710" />
				<skos:scopeNote xml:lang="en">The collection, identification and analysis of pollen from archaeological and other deposits.</skos:scopeNote>
			</skos:Concept>
		</skos:narrower>
		<skos:broader rdf:resource="http://purl.org/heritagedata/schemes/4/concepts/502413" />
		<skos:narrower>
			<skos:Concept rdf:about="http://purl.org/heritagedata/schemes/4/concepts/502711">
				<skos:inScheme rdf:resource="http://purl.org/heritagedata/schemes/4" />
				<dcterms:identifier>http://purl.org/heritagedata/schemes/4/concepts/502711</dcterms:identifier>
				<cc:license rdf:resource="http://reference.data.gov.uk/id/open-government-licence" />
				<cc:attributionURL rdf:resource="http://www.rcahms.gov.uk" />
				<cc:attributionName xml:lang="en">RCAHMS</cc:attributionName>
				<dcterms:publisher rdf:resource="http://www.rcahms.gov.uk" />
				<skos:prefLabel xml:lang="en">DIATOM ANALYSIS</skos:prefLabel>
				<dcterms:created rdf:datatype="http://www.w3.org/2001/XMLSchema#dateTime">2007-07-13T13:03:52</dcterms:created>
				<dcterms:modified rdf:datatype="http://www.w3.org/2001/XMLSchema#dateTime">2007-07-13T13:10:58</dcterms:modified>
				<dcterms:issued rdf:datatype="http://www.w3.org/2001/XMLSchema#dateTime">2013-07-17T10:08:40</dcterms:issued>
				<skos:broader rdf:resource="http://purl.org/heritagedata/schemes/4/concepts/502710" />
				<skos:scopeNote xml:lang="en">The collection, identification and analysis of diatoms from lake or marine deposits.</skos:scopeNote>
			</skos:Concept>
		</skos:narrower>
		<skos:scopeNote xml:lang="en">Remains of animal (fauna) or plant (flora), that cannot be examined by the human eye without aid of a microscope.</skos:scopeNote>
	</skos:Concept>
	<skos:Concept rdf:about="http://purl.org/heritagedata/schemes/4/concepts/502340">
		<skos:inScheme rdf:resource="http://purl.org/heritagedata/schemes/4" />
		<dcterms:identifier>http://purl.org/heritagedata/schemes/4/concepts/502340</dcterms:identifier>
		<cc:license rdf:resource="http://reference.data.gov.uk/id/open-government-licence" />
		<cc:attributionURL rdf:resource="http://www.rcahms.gov.uk" />
		<cc:attributionName xml:lang="en">RCAHMS</cc:attributionName>
		<dcterms:publisher rdf:resource="http://www.rcahms.gov.uk" />
		<skos:topConceptOf rdf:resource="http://purl.org/heritagedata/schemes/4" />
		<skos:prefLabel xml:lang="en">DOCUMENTARY REFERENCE</skos:prefLabel>
		<dcterms:created rdf:datatype="http://www.w3.org/2001/XMLSchema#dateTime">2007-05-30T09:18:26</dcterms:created>
		<dcterms:modified rdf:datatype="http://www.w3.org/2001/XMLSchema#dateTime">2007-11-30T10:12:40</dcterms:modified>
		<dcterms:issued rdf:datatype="http://www.w3.org/2001/XMLSchema#dateTime">2013-07-17T10:08:40</dcterms:issued>
		<skos:narrower>
			<skos:Concept rdf:about="http://purl.org/heritagedata/schemes/4/concepts/502463">
				<skos:inScheme rdf:resource="http://purl.org/heritagedata/schemes/4" />
				<dcterms:identifier>http://purl.org/heritagedata/schemes/4/concepts/502463</dcterms:identifier>
				<cc:license rdf:resource="http://reference.data.gov.uk/id/open-government-licence" />
				<cc:attributionURL rdf:resource="http://www.rcahms.gov.uk" />
				<cc:attributionName xml:lang="en">RCAHMS</cc:attributionName>
				<dcterms:publisher rdf:resource="http://www.rcahms.gov.uk" />
				<skos:prefLabel xml:lang="en">ANTIQUARIAN MAPPING</skos:prefLabel>
				<dcterms:created rdf:datatype="http://www.w3.org/2001/XMLSchema#dateTime">2007-06-04T10:50:28</dcterms:created>
				<dcterms:modified rdf:datatype="http://www.w3.org/2001/XMLSchema#dateTime">2007-06-04T10:53:05</dcterms:modified>
				<dcterms:issued rdf:datatype="http://www.w3.org/2001/XMLSchema#dateTime">2013-07-17T10:08:40</dcterms:issued>
				<skos:broader rdf:resource="http://purl.org/heritagedata/schemes/4/concepts/502340" />
				<skos:scopeNote xml:lang="en">Use for information recorded on Antiquarian maps.</skos:scopeNote>
			</skos:Concept>
		</skos:narrower>
		<skos:narrower rdf:resource="http://purl.org/heritagedata/schemes/4/concepts/502473" />
		<skos:narrower rdf:resource="http://purl.org/heritagedata/schemes/4/concepts/502476" />
		<skos:narrower>
			<skos:Concept rdf:about="http://purl.org/heritagedata/schemes/4/concepts/503760">
				<skos:inScheme rdf:resource="http://purl.org/heritagedata/schemes/4" />
				<dcterms:identifier>http://purl.org/heritagedata/schemes/4/concepts/503760</dcterms:identifier>
				<cc:license rdf:resource="http://reference.data.gov.uk/id/open-government-licence" />
				<cc:attributionURL rdf:resource="http://www.rcahms.gov.uk" />
				<cc:attributionName xml:lang="en">RCAHMS</cc:attributionName>
				<dcterms:publisher rdf:resource="http://www.rcahms.gov.uk" />
				<skos:prefLabel xml:lang="en">EXTERNAL REFERENCE</skos:prefLabel>
				<dcterms:created rdf:datatype="http://www.w3.org/2001/XMLSchema#dateTime">2008-11-24T09:50:46</dcterms:created>
				<dcterms:modified rdf:datatype="http://www.w3.org/2001/XMLSchema#dateTime">2009-08-10T15:48:56</dcterms:modified>
				<dcterms:issued rdf:datatype="http://www.w3.org/2001/XMLSchema#dateTime">2013-07-17T10:08:40</dcterms:issued>
				<skos:broader rdf:resource="http://purl.org/heritagedata/schemes/4/concepts/502340" />
				<skos:scopeNote xml:lang="en">Summary information recorded in archives such as the National Archives of Scotland e.g. EXTERNAL REFERENCE Scottish Records Office 'The Commissioners announce their intention to build 3 new lighthouses'. OR unreferenced information from members of the public e.g. in from Mr Mac of Lerwick.</skos:scopeNote>
			</skos:Concept>
		</skos:narrower>
		<skos:scopeNote xml:lang="en">Summary information recorded in archives such as the National Archives of Scotland and from antiquarian and OS historic mapping.</skos:scopeNote>
	</skos:Concept>
	<skos:Concept rdf:about="http://purl.org/heritagedata/schemes/4/concepts/502342">
		<skos:inScheme rdf:resource="http://purl.org/heritagedata/schemes/4" />
		<dcterms:identifier>http://purl.org/heritagedata/schemes/4/concepts/502342</dcterms:identifier>
		<cc:license rdf:resource="http://reference.data.gov.uk/id/open-government-licence" />
		<cc:attributionURL rdf:resource="http://www.rcahms.gov.uk" />
		<cc:attributionName xml:lang="en">RCAHMS</cc:attributionName>
		<dcterms:publisher rdf:resource="http://www.rcahms.gov.uk" />
		<skos:topConceptOf rdf:resource="http://purl.org/heritagedata/schemes/4" />
		<skos:prefLabel xml:lang="en">CHANGE</skos:prefLabel>
		<dcterms:created rdf:datatype="http://www.w3.org/2001/XMLSchema#dateTime">2007-05-30T09:18:56</dcterms:created>
		<dcterms:modified rdf:datatype="http://www.w3.org/2001/XMLSchema#dateTime">2007-11-30T10:06:38</dcterms:modified>
		<dcterms:issued rdf:datatype="http://www.w3.org/2001/XMLSchema#dateTime">2013-07-17T10:08:40</dcterms:issued>
		<skos:narrower>
			<skos:Concept rdf:about="http://purl.org/heritagedata/schemes/4/concepts/502453">
				<skos:inScheme rdf:resource="http://purl.org/heritagedata/schemes/4" />
				<dcterms:identifier>http://purl.org/heritagedata/schemes/4/concepts/502453</dcterms:identifier>
				<cc:license rdf:resource="http://reference.data.gov.uk/id/open-government-licence" />
				<cc:attributionURL rdf:resource="http://www.rcahms.gov.uk" />
				<cc:attributionName xml:lang="en">RCAHMS</cc:attributionName>
				<dcterms:publisher rdf:resource="http://www.rcahms.gov.uk" />
				<skos:prefLabel xml:lang="en">CHANGE OF USE</skos:prefLabel>
				<dcterms:created rdf:datatype="http://www.w3.org/2001/XMLSchema#dateTime">2007-06-04T10:30:01</dcterms:created>
				<dcterms:modified rdf:datatype="http://www.w3.org/2001/XMLSchema#dateTime">2007-06-04T10:34:43</dcterms:modified>
				<dcterms:issued rdf:datatype="http://www.w3.org/2001/XMLSchema#dateTime">2013-07-17T10:08:40</dcterms:issued>
				<skos:broader rdf:resource="http://purl.org/heritagedata/schemes/4/concepts/502342" />
				<skos:scopeNote xml:lang="en">A subsequent use of a building or monument from that which it was originally designed for, or altered to.</skos:scopeNote>
			</skos:Concept>
		</skos:narrower>
		<skos:narrower>
			<skos:Concept rdf:about="http://purl.org/heritagedata/schemes/4/concepts/502455">
				<skos:inScheme rdf:resource="http://purl.org/heritagedata/schemes/4" />
				<dcterms:identifier>http://purl.org/heritagedata/schemes/4/concepts/502455</dcterms:identifier>
				<cc:license rdf:resource="http://reference.data.gov.uk/id/open-government-licence" />
				<cc:attributionURL rdf:resource="http://www.rcahms.gov.uk" />
				<cc:attributionName xml:lang="en">RCAHMS</cc:attributionName>
				<dcterms:publisher rdf:resource="http://www.rcahms.gov.uk" />
				<skos:prefLabel xml:lang="en">CHANGE OF NAME</skos:prefLabel>
				<dcterms:created rdf:datatype="http://www.w3.org/2001/XMLSchema#dateTime">2007-06-04T10:35:01</dcterms:created>
				<dcterms:modified rdf:datatype="http://www.w3.org/2001/XMLSchema#dateTime">2007-06-04T10:35:28</dcterms:modified>
				<dcterms:issued rdf:datatype="http://www.w3.org/2001/XMLSchema#dateTime">2013-07-17T10:08:40</dcterms:issued>
				<skos:broader rdf:resource="http://purl.org/heritagedata/schemes/4/concepts/502342" />
				<skos:scopeNote xml:lang="en">Where the name of a building or monument has changed from its original appellation.</skos:scopeNote>
			</skos:Concept>
		</skos:narrower>
		<skos:narrower>
			<skos:Concept rdf:about="http://purl.org/heritagedata/schemes/4/concepts/502456">
				<skos:inScheme rdf:resource="http://purl.org/heritagedata/schemes/4" />
				<dcterms:identifier>http://purl.org/heritagedata/schemes/4/concepts/502456</dcterms:identifier>
				<cc:license rdf:resource="http://reference.data.gov.uk/id/open-government-licence" />
				<cc:attributionURL rdf:resource="http://www.rcahms.gov.uk" />
				<cc:attributionName xml:lang="en">RCAHMS</cc:attributionName>
				<dcterms:publisher rdf:resource="http://www.rcahms.gov.uk" />
				<skos:prefLabel xml:lang="en">CHANGE OF CLASSIFICATION</skos:prefLabel>
				<dcterms:created rdf:datatype="http://www.w3.org/2001/XMLSchema#dateTime">2007-06-04T10:35:46</dcterms:created>
				<dcterms:modified rdf:datatype="http://www.w3.org/2001/XMLSchema#dateTime">2007-06-05T11:00:07</dcterms:modified>
				<dcterms:issued rdf:datatype="http://www.w3.org/2001/XMLSchema#dateTime">2013-07-17T10:08:40</dcterms:issued>
				<skos:broader rdf:resource="http://purl.org/heritagedata/schemes/4/concepts/502342" />
				<skos:scopeNote xml:lang="en">Records where the  classification of a record has changed. Classification may change as a result of re-interpretation (in which case there is a related event) or from mapping a non-preferred term to a preferred term in the thesaurus.</skos:scopeNote>
			</skos:Concept>
		</skos:narrower>
		<skos:narrower>
			<skos:Concept rdf:about="http://purl.org/heritagedata/schemes/4/concepts/504760">
				<skos:inScheme rdf:resource="http://purl.org/heritagedata/schemes/4" />
				<dcterms:identifier>http://purl.org/heritagedata/schemes/4/concepts/504760</dcterms:identifier>
				<cc:license rdf:resource="http://reference.data.gov.uk/id/open-government-licence" />
				<cc:attributionURL rdf:resource="http://www.rcahms.gov.uk" />
				<cc:attributionName xml:lang="en">RCAHMS</cc:attributionName>
				<dcterms:publisher rdf:resource="http://www.rcahms.gov.uk" />
				<skos:prefLabel xml:lang="en">CHANGE OF NUMBER</skos:prefLabel>
				<dcterms:created rdf:datatype="http://www.w3.org/2001/XMLSchema#dateTime">2010-03-10T14:46:37</dcterms:created>
				<dcterms:modified rdf:datatype="http://www.w3.org/2001/XMLSchema#dateTime">2010-03-10T14:47:59</dcterms:modified>
				<dcterms:issued rdf:datatype="http://www.w3.org/2001/XMLSchema#dateTime">2013-07-17T10:08:40</dcterms:issued>
				<skos:broader rdf:resource="http://purl.org/heritagedata/schemes/4/concepts/502342" />
				<skos:scopeNote xml:lang="en">Documents the change of site number; for instance if a sub-numbered record has been re-assigned.</skos:scopeNote>
			</skos:Concept>
		</skos:narrower>
		<skos:scopeNote xml:lang="en">Documents the change of name, use or classification of a building or monument.</skos:scopeNote>
	</skos:Concept>
	<skos:Concept rdf:about="http://purl.org/heritagedata/schemes/4/concepts/502343">
		<skos:inScheme rdf:resource="http://purl.org/heritagedata/schemes/4" />
		<dcterms:identifier>http://purl.org/heritagedata/schemes/4/concepts/502343</dcterms:identifier>
		<cc:license rdf:resource="http://reference.data.gov.uk/id/open-government-licence" />
		<cc:attributionURL rdf:resource="http://www.rcahms.gov.uk" />
		<cc:attributionName xml:lang="en">RCAHMS</cc:attributionName>
		<dcterms:publisher rdf:resource="http://www.rcahms.gov.uk" />
		<skos:topConceptOf rdf:resource="http://purl.org/heritagedata/schemes/4" />
		<skos:prefLabel xml:lang="en">BUILDING HISTORY</skos:prefLabel>
		<dcterms:created rdf:datatype="http://www.w3.org/2001/XMLSchema#dateTime">2007-05-30T09:19:01</dcterms:created>
		<dcterms:modified rdf:datatype="http://www.w3.org/2001/XMLSchema#dateTime">2007-11-30T10:00:27</dcterms:modified>
		<dcterms:issued rdf:datatype="http://www.w3.org/2001/XMLSchema#dateTime">2013-07-17T10:08:40</dcterms:issued>
		<skos:narrower rdf:resource="http://purl.org/heritagedata/schemes/4/concepts/502533" />
		<skos:narrower rdf:resource="http://purl.org/heritagedata/schemes/4/concepts/502534" />
		<skos:narrower rdf:resource="http://purl.org/heritagedata/schemes/4/concepts/502535" />
		<skos:narrower rdf:resource="http://purl.org/heritagedata/schemes/4/concepts/506321" />
		<skos:scopeNote xml:lang="en">Events in the life cycle of a building or monument. They specifically relate to the initial design, execution, modification and ultimate destruction of a building or monument.</skos:scopeNote>
	</skos:Concept>
	<skos:Concept rdf:about="http://purl.org/heritagedata/schemes/4/concepts/502358">
		<skos:inScheme rdf:resource="http://purl.org/heritagedata/schemes/4" />
		<dcterms:identifier>http://purl.org/heritagedata/schemes/4/concepts/502358</dcterms:identifier>
		<cc:license rdf:resource="http://reference.data.gov.uk/id/open-government-licence" />
		<cc:attributionURL rdf:resource="http://www.rcahms.gov.uk" />
		<cc:attributionName xml:lang="en">RCAHMS</cc:attributionName>
		<dcterms:publisher rdf:resource="http://www.rcahms.gov.uk" />
		<skos:prefLabel xml:lang="en">GEOPHYSICAL SURVEY</skos:prefLabel>
		<dcterms:created rdf:datatype="http://www.w3.org/2001/XMLSchema#dateTime">2007-05-30T15:00:55</dcterms:created>
		<dcterms:modified rdf:datatype="http://www.w3.org/2001/XMLSchema#dateTime">2007-05-30T15:05:53</dcterms:modified>
		<dcterms:issued rdf:datatype="http://www.w3.org/2001/XMLSchema#dateTime">2013-07-17T10:08:40</dcterms:issued>
		<skos:narrower>
			<skos:Concept rdf:about="http://purl.org/heritagedata/schemes/4/concepts/502409">
				<skos:inScheme rdf:resource="http://purl.org/heritagedata/schemes/4" />
				<dcterms:identifier>http://purl.org/heritagedata/schemes/4/concepts/502409</dcterms:identifier>
				<cc:license rdf:resource="http://reference.data.gov.uk/id/open-government-licence" />
				<cc:attributionURL rdf:resource="http://www.rcahms.gov.uk" />
				<cc:attributionName xml:lang="en">RCAHMS</cc:attributionName>
				<dcterms:publisher rdf:resource="http://www.rcahms.gov.uk" />
				<skos:prefLabel xml:lang="en">METAL DETECTOR SURVEY</skos:prefLabel>
				<dcterms:created rdf:datatype="http://www.w3.org/2001/XMLSchema#dateTime">2007-05-31T16:11:17</dcterms:created>
				<dcterms:modified rdf:datatype="http://www.w3.org/2001/XMLSchema#dateTime">2007-05-31T16:11:40</dcterms:modified>
				<dcterms:issued rdf:datatype="http://www.w3.org/2001/XMLSchema#dateTime">2013-07-17T10:08:40</dcterms:issued>
				<skos:broader rdf:resource="http://purl.org/heritagedata/schemes/4/concepts/502358" />
				<skos:scopeNote xml:lang="en">Systematic metal detector survey usually undertaken as part of a wider archaeological project.</skos:scopeNote>
			</skos:Concept>
		</skos:narrower>
		<skos:narrower>
			<skos:Concept rdf:about="http://purl.org/heritagedata/schemes/4/concepts/502410">
				<skos:inScheme rdf:resource="http://purl.org/heritagedata/schemes/4" />
				<dcterms:identifier>http://purl.org/heritagedata/schemes/4/concepts/502410</dcterms:identifier>
				<cc:license rdf:resource="http://reference.data.gov.uk/id/open-government-licence" />
				<cc:attributionURL rdf:resource="http://www.rcahms.gov.uk" />
				<cc:attributionName xml:lang="en">RCAHMS</cc:attributionName>
				<dcterms:publisher rdf:resource="http://www.rcahms.gov.uk" />
				<skos:prefLabel xml:lang="en">METAL DETECTOR FIND</skos:prefLabel>
				<dcterms:created rdf:datatype="http://www.w3.org/2001/XMLSchema#dateTime">2007-05-31T16:12:15</dcterms:created>
				<dcterms:modified rdf:datatype="http://www.w3.org/2001/XMLSchema#dateTime">2007-05-31T16:13:02</dcterms:modified>
				<dcterms:issued rdf:datatype="http://www.w3.org/2001/XMLSchema#dateTime">2013-07-17T10:08:40</dcterms:issued>
				<skos:broader rdf:resource="http://purl.org/heritagedata/schemes/4/concepts/502358" />
				<skos:scopeNote xml:lang="en">The casual recovery of metal artefacts through the use of a metal detector, usually by an individual or amateur treasure hunting group.</skos:scopeNote>
			</skos:Concept>
		</skos:narrower>
		<skos:broader rdf:resource="http://purl.org/heritagedata/schemes/4/concepts/506601" />
		<skos:narrower>
			<skos:Concept rdf:about="http://purl.org/heritagedata/schemes/4/concepts/502359">
				<skos:inScheme rdf:resource="http://purl.org/heritagedata/schemes/4" />
				<dcterms:identifier>http://purl.org/heritagedata/schemes/4/concepts/502359</dcterms:identifier>
				<cc:license rdf:resource="http://reference.data.gov.uk/id/open-government-licence" />
				<cc:attributionURL rdf:resource="http://www.rcahms.gov.uk" />
				<cc:attributionName xml:lang="en">RCAHMS</cc:attributionName>
				<dcterms:publisher rdf:resource="http://www.rcahms.gov.uk" />
				<skos:prefLabel xml:lang="en">GROUND PENETRATING RADAR</skos:prefLabel>
				<dcterms:created rdf:datatype="http://www.w3.org/2001/XMLSchema#dateTime">2007-05-30T15:07:21</dcterms:created>
				<dcterms:modified rdf:datatype="http://www.w3.org/2001/XMLSchema#dateTime">2007-05-30T15:14:06</dcterms:modified>
				<dcterms:issued rdf:datatype="http://www.w3.org/2001/XMLSchema#dateTime">2013-07-17T10:08:40</dcterms:issued>
				<skos:broader rdf:resource="http://purl.org/heritagedata/schemes/4/concepts/502358" />
				<skos:scopeNote xml:lang="en">A non-invasive technique used to record the location of concealed features through the measurement of reflected radio waves.</skos:scopeNote>
			</skos:Concept>
		</skos:narrower>
		<skos:narrower>
			<skos:Concept rdf:about="http://purl.org/heritagedata/schemes/4/concepts/502361">
				<skos:inScheme rdf:resource="http://purl.org/heritagedata/schemes/4" />
				<dcterms:identifier>http://purl.org/heritagedata/schemes/4/concepts/502361</dcterms:identifier>
				<cc:license rdf:resource="http://reference.data.gov.uk/id/open-government-licence" />
				<cc:attributionURL rdf:resource="http://www.rcahms.gov.uk" />
				<cc:attributionName xml:lang="en">RCAHMS</cc:attributionName>
				<dcterms:publisher rdf:resource="http://www.rcahms.gov.uk" />
				<skos:prefLabel xml:lang="en">UNSPECIFIED GEOPHYSICAL SURVEY TECHNIQUE</skos:prefLabel>
				<dcterms:created rdf:datatype="http://www.w3.org/2001/XMLSchema#dateTime">2007-05-31T09:11:33</dcterms:created>
				<dcterms:modified rdf:datatype="http://www.w3.org/2001/XMLSchema#dateTime">2008-01-08T14:21:50</dcterms:modified>
				<dcterms:issued rdf:datatype="http://www.w3.org/2001/XMLSchema#dateTime">2013-07-17T10:08:40</dcterms:issued>
				<skos:broader rdf:resource="http://purl.org/heritagedata/schemes/4/concepts/502358" />
				<skos:scopeNote xml:lang="en">To be used for geophysical surveys where no methodology has been recorded either by the fieldworker or from events migrated from the University of Glasgow Geophysical Survey database.</skos:scopeNote>
			</skos:Concept>
		</skos:narrower>
		<skos:narrower>
			<skos:Concept rdf:about="http://purl.org/heritagedata/schemes/4/concepts/502380">
				<skos:inScheme rdf:resource="http://purl.org/heritagedata/schemes/4" />
				<dcterms:identifier>http://purl.org/heritagedata/schemes/4/concepts/502380</dcterms:identifier>
				<cc:license rdf:resource="http://reference.data.gov.uk/id/open-government-licence" />
				<cc:attributionURL rdf:resource="http://www.rcahms.gov.uk" />
				<cc:attributionName xml:lang="en">RCAHMS</cc:attributionName>
				<dcterms:publisher rdf:resource="http://www.rcahms.gov.uk" />
				<skos:prefLabel xml:lang="en">SEISMIC</skos:prefLabel>
				<dcterms:created rdf:datatype="http://www.w3.org/2001/XMLSchema#dateTime">2007-05-31T09:15:47</dcterms:created>
				<dcterms:modified rdf:datatype="http://www.w3.org/2001/XMLSchema#dateTime">2007-05-31T09:16:18</dcterms:modified>
				<dcterms:issued rdf:datatype="http://www.w3.org/2001/XMLSchema#dateTime">2013-07-17T10:08:40</dcterms:issued>
				<skos:broader rdf:resource="http://purl.org/heritagedata/schemes/4/concepts/502358" />
				<skos:scopeNote xml:lang="en">Geophysical survey using Seismic techniques</skos:scopeNote>
			</skos:Concept>
		</skos:narrower>
		<skos:narrower>
			<skos:Concept rdf:about="http://purl.org/heritagedata/schemes/4/concepts/502381">
				<skos:inScheme rdf:resource="http://purl.org/heritagedata/schemes/4" />
				<dcterms:identifier>http://purl.org/heritagedata/schemes/4/concepts/502381</dcterms:identifier>
				<cc:license rdf:resource="http://reference.data.gov.uk/id/open-government-licence" />
				<cc:attributionURL rdf:resource="http://www.rcahms.gov.uk" />
				<cc:attributionName xml:lang="en">RCAHMS</cc:attributionName>
				<dcterms:publisher rdf:resource="http://www.rcahms.gov.uk" />
				<skos:prefLabel xml:lang="en">MICROGRAVITY</skos:prefLabel>
				<dcterms:created rdf:datatype="http://www.w3.org/2001/XMLSchema#dateTime">2007-05-31T09:17:06</dcterms:created>
				<dcterms:modified rdf:datatype="http://www.w3.org/2001/XMLSchema#dateTime">2007-05-31T09:17:24</dcterms:modified>
				<dcterms:issued rdf:datatype="http://www.w3.org/2001/XMLSchema#dateTime">2013-07-17T10:08:40</dcterms:issued>
				<skos:broader rdf:resource="http://purl.org/heritagedata/schemes/4/concepts/502358" />
				<skos:scopeNote xml:lang="en">Geophysical survey using Microgravity techniques</skos:scopeNote>
			</skos:Concept>
		</skos:narrower>
		<skos:narrower>
			<skos:Concept rdf:about="http://purl.org/heritagedata/schemes/4/concepts/502382">
				<skos:inScheme rdf:resource="http://purl.org/heritagedata/schemes/4" />
				<dcterms:identifier>http://purl.org/heritagedata/schemes/4/concepts/502382</dcterms:identifier>
				<cc:license rdf:resource="http://reference.data.gov.uk/id/open-government-licence" />
				<cc:attributionURL rdf:resource="http://www.rcahms.gov.uk" />
				<cc:attributionName xml:lang="en">RCAHMS</cc:attributionName>
				<dcterms:publisher rdf:resource="http://www.rcahms.gov.uk" />
				<skos:prefLabel xml:lang="en">MAGNETIC SUSCEPTIBILITY</skos:prefLabel>
				<dcterms:created rdf:datatype="http://www.w3.org/2001/XMLSchema#dateTime">2007-05-31T09:17:50</dcterms:created>
				<dcterms:modified rdf:datatype="http://www.w3.org/2001/XMLSchema#dateTime">2007-05-31T09:19:36</dcterms:modified>
				<dcterms:issued rdf:datatype="http://www.w3.org/2001/XMLSchema#dateTime">2013-07-17T10:08:40</dcterms:issued>
				<skos:broader rdf:resource="http://purl.org/heritagedata/schemes/4/concepts/502358" />
				<skos:scopeNote xml:lang="en">Geophysical survey technique measuring the effect of an artificial electromagnetic field on subsurface and surface features.</skos:scopeNote>
			</skos:Concept>
		</skos:narrower>
		<skos:narrower>
			<skos:Concept rdf:about="http://purl.org/heritagedata/schemes/4/concepts/502384">
				<skos:inScheme rdf:resource="http://purl.org/heritagedata/schemes/4" />
				<dcterms:identifier>http://purl.org/heritagedata/schemes/4/concepts/502384</dcterms:identifier>
				<cc:license rdf:resource="http://reference.data.gov.uk/id/open-government-licence" />
				<cc:attributionURL rdf:resource="http://www.rcahms.gov.uk" />
				<cc:attributionName xml:lang="en">RCAHMS</cc:attributionName>
				<dcterms:publisher rdf:resource="http://www.rcahms.gov.uk" />
				<skos:prefLabel xml:lang="en">MAGNETOMETRY</skos:prefLabel>
				<dcterms:created rdf:datatype="http://www.w3.org/2001/XMLSchema#dateTime">2007-05-31T09:25:45</dcterms:created>
				<dcterms:modified rdf:datatype="http://www.w3.org/2001/XMLSchema#dateTime">2007-06-05T11:27:16</dcterms:modified>
				<dcterms:issued rdf:datatype="http://www.w3.org/2001/XMLSchema#dateTime">2013-07-17T10:08:40</dcterms:issued>
				<skos:broader rdf:resource="http://purl.org/heritagedata/schemes/4/concepts/502358" />
				<skos:scopeNote xml:lang="en">Geophysical survey technique measuring local anomalies in the earth's magnetic field to locate and plot concealed features.</skos:scopeNote>
			</skos:Concept>
		</skos:narrower>
		<skos:narrower>
			<skos:Concept rdf:about="http://purl.org/heritagedata/schemes/4/concepts/502385">
				<skos:inScheme rdf:resource="http://purl.org/heritagedata/schemes/4" />
				<dcterms:identifier>http://purl.org/heritagedata/schemes/4/concepts/502385</dcterms:identifier>
				<cc:license rdf:resource="http://reference.data.gov.uk/id/open-government-licence" />
				<cc:attributionURL rdf:resource="http://www.rcahms.gov.uk" />
				<cc:attributionName xml:lang="en">RCAHMS</cc:attributionName>
				<dcterms:publisher rdf:resource="http://www.rcahms.gov.uk" />
				<skos:prefLabel xml:lang="en">RESISTIVITY</skos:prefLabel>
				<dcterms:created rdf:datatype="http://www.w3.org/2001/XMLSchema#dateTime">2007-05-31T09:28:33</dcterms:created>
				<dcterms:modified rdf:datatype="http://www.w3.org/2001/XMLSchema#dateTime">2007-05-31T09:29:44</dcterms:modified>
				<dcterms:issued rdf:datatype="http://www.w3.org/2001/XMLSchema#dateTime">2013-07-17T10:08:40</dcterms:issued>
				<skos:broader rdf:resource="http://purl.org/heritagedata/schemes/4/concepts/502358" />
				<skos:scopeNote xml:lang="en">Geophysical survey technique measuring differences in electrical resistance to locate and plot buried features.</skos:scopeNote>
			</skos:Concept>
		</skos:narrower>
		<skos:narrower>
			<skos:Concept rdf:about="http://purl.org/heritagedata/schemes/4/concepts/502386">
				<skos:inScheme rdf:resource="http://purl.org/heritagedata/schemes/4" />
				<dcterms:identifier>http://purl.org/heritagedata/schemes/4/concepts/502386</dcterms:identifier>
				<cc:license rdf:resource="http://reference.data.gov.uk/id/open-government-licence" />
				<cc:attributionURL rdf:resource="http://www.rcahms.gov.uk" />
				<cc:attributionName xml:lang="en">RCAHMS</cc:attributionName>
				<dcterms:publisher rdf:resource="http://www.rcahms.gov.uk" />
				<skos:prefLabel xml:lang="en">ELECTROMAGNETIC</skos:prefLabel>
				<dcterms:created rdf:datatype="http://www.w3.org/2001/XMLSchema#dateTime">2007-05-31T09:30:20</dcterms:created>
				<dcterms:modified rdf:datatype="http://www.w3.org/2001/XMLSchema#dateTime">2007-05-31T09:35:27</dcterms:modified>
				<dcterms:issued rdf:datatype="http://www.w3.org/2001/XMLSchema#dateTime">2013-07-17T10:08:40</dcterms:issued>
				<skos:broader rdf:resource="http://purl.org/heritagedata/schemes/4/concepts/502358" />
				<skos:scopeNote xml:lang="en">Geophysical survey techniques measuring the ability of the soil to conduct an electric current. Changes in the rate of conductivity are used to locate and plot buried features.</skos:scopeNote>
			</skos:Concept>
		</skos:narrower>
		<skos:scopeNote xml:lang="en">A range of non-invasive techniques used  to measure the physical characteristics of soils to construct images of buried features.</skos:scopeNote>
	</skos:Concept>
	<skos:Concept rdf:about="http://purl.org/heritagedata/schemes/4/concepts/502388">
		<skos:inScheme rdf:resource="http://purl.org/heritagedata/schemes/4" />
		<dcterms:identifier>http://purl.org/heritagedata/schemes/4/concepts/502388</dcterms:identifier>
		<cc:license rdf:resource="http://reference.data.gov.uk/id/open-government-licence" />
		<cc:attributionURL rdf:resource="http://www.rcahms.gov.uk" />
		<cc:attributionName xml:lang="en">RCAHMS</cc:attributionName>
		<dcterms:publisher rdf:resource="http://www.rcahms.gov.uk" />
		<skos:prefLabel xml:lang="en">AERIAL</skos:prefLabel>
		<dcterms:created rdf:datatype="http://www.w3.org/2001/XMLSchema#dateTime">2007-05-31T09:39:43</dcterms:created>
		<dcterms:modified rdf:datatype="http://www.w3.org/2001/XMLSchema#dateTime">2008-11-19T08:46:28</dcterms:modified>
		<dcterms:issued rdf:datatype="http://www.w3.org/2001/XMLSchema#dateTime">2013-07-17T10:08:40</dcterms:issued>
		<skos:broader rdf:resource="http://purl.org/heritagedata/schemes/4/concepts/502401" />
		<skos:narrower>
			<skos:Concept rdf:about="http://purl.org/heritagedata/schemes/4/concepts/502389">
				<skos:inScheme rdf:resource="http://purl.org/heritagedata/schemes/4" />
				<dcterms:identifier>http://purl.org/heritagedata/schemes/4/concepts/502389</dcterms:identifier>
				<cc:license rdf:resource="http://reference.data.gov.uk/id/open-government-licence" />
				<cc:attributionURL rdf:resource="http://www.rcahms.gov.uk" />
				<cc:attributionName xml:lang="en">RCAHMS</cc:attributionName>
				<dcterms:publisher rdf:resource="http://www.rcahms.gov.uk" />
				<skos:prefLabel xml:lang="en">AERIAL PHOTOGRAPHIC INTERPRETATION</skos:prefLabel>
				<dcterms:created rdf:datatype="http://www.w3.org/2001/XMLSchema#dateTime">2007-05-31T09:42:15</dcterms:created>
				<dcterms:modified rdf:datatype="http://www.w3.org/2001/XMLSchema#dateTime">2007-05-31T09:43:04</dcterms:modified>
				<dcterms:issued rdf:datatype="http://www.w3.org/2001/XMLSchema#dateTime">2013-07-17T10:08:40</dcterms:issued>
				<skos:broader rdf:resource="http://purl.org/heritagedata/schemes/4/concepts/502388" />
				<skos:scopeNote xml:lang="en">The re-interpretation of existing aerial photography excluding transcription work.</skos:scopeNote>
			</skos:Concept>
		</skos:narrower>
		<skos:narrower>
			<skos:Concept rdf:about="http://purl.org/heritagedata/schemes/4/concepts/502390">
				<skos:inScheme rdf:resource="http://purl.org/heritagedata/schemes/4" />
				<dcterms:identifier>http://purl.org/heritagedata/schemes/4/concepts/502390</dcterms:identifier>
				<cc:license rdf:resource="http://reference.data.gov.uk/id/open-government-licence" />
				<cc:attributionURL rdf:resource="http://www.rcahms.gov.uk" />
				<cc:attributionName xml:lang="en">RCAHMS</cc:attributionName>
				<dcterms:publisher rdf:resource="http://www.rcahms.gov.uk" />
				<skos:prefLabel xml:lang="en">AERIAL PHOTOGRAPHY</skos:prefLabel>
				<dcterms:created rdf:datatype="http://www.w3.org/2001/XMLSchema#dateTime">2007-05-31T09:44:50</dcterms:created>
				<dcterms:modified rdf:datatype="http://www.w3.org/2001/XMLSchema#dateTime">2007-06-04T15:16:17</dcterms:modified>
				<dcterms:issued rdf:datatype="http://www.w3.org/2001/XMLSchema#dateTime">2013-07-17T10:08:40</dcterms:issued>
				<skos:broader rdf:resource="http://purl.org/heritagedata/schemes/4/concepts/502388" />
				<skos:scopeNote xml:lang="en">The recording of a monument, building, or wider landscape, through the medium of photography from an aircraft or other airborne vehicle.</skos:scopeNote>
			</skos:Concept>
		</skos:narrower>
		<skos:narrower>
			<skos:Concept rdf:about="http://purl.org/heritagedata/schemes/4/concepts/502391">
				<skos:inScheme rdf:resource="http://purl.org/heritagedata/schemes/4" />
				<dcterms:identifier>http://purl.org/heritagedata/schemes/4/concepts/502391</dcterms:identifier>
				<cc:license rdf:resource="http://reference.data.gov.uk/id/open-government-licence" />
				<cc:attributionURL rdf:resource="http://www.rcahms.gov.uk" />
				<cc:attributionName xml:lang="en">RCAHMS</cc:attributionName>
				<dcterms:publisher rdf:resource="http://www.rcahms.gov.uk" />
				<skos:prefLabel xml:lang="en">AERIAL PHOTOGRAPHIC TRANSCRIPTION</skos:prefLabel>
				<dcterms:created rdf:datatype="http://www.w3.org/2001/XMLSchema#dateTime">2007-05-31T09:49:41</dcterms:created>
				<dcterms:modified rdf:datatype="http://www.w3.org/2001/XMLSchema#dateTime">2007-05-31T09:50:42</dcterms:modified>
				<dcterms:issued rdf:datatype="http://www.w3.org/2001/XMLSchema#dateTime">2013-07-17T10:08:40</dcterms:issued>
				<skos:broader rdf:resource="http://purl.org/heritagedata/schemes/4/concepts/502388" />
				<skos:scopeNote xml:lang="en">The mechanical or manual mapping of archaeological and other features observed from (oblique) aerial photography onto a map base.</skos:scopeNote>
			</skos:Concept>
		</skos:narrower>
		<skos:narrower>
			<skos:Concept rdf:about="http://purl.org/heritagedata/schemes/4/concepts/502392">
				<skos:inScheme rdf:resource="http://purl.org/heritagedata/schemes/4" />
				<dcterms:identifier>http://purl.org/heritagedata/schemes/4/concepts/502392</dcterms:identifier>
				<cc:license rdf:resource="http://reference.data.gov.uk/id/open-government-licence" />
				<cc:attributionURL rdf:resource="http://www.rcahms.gov.uk" />
				<cc:attributionName xml:lang="en">RCAHMS</cc:attributionName>
				<dcterms:publisher rdf:resource="http://www.rcahms.gov.uk" />
				<skos:prefLabel xml:lang="en">INFRARED LINE SCAN</skos:prefLabel>
				<dcterms:created rdf:datatype="http://www.w3.org/2001/XMLSchema#dateTime">2007-05-31T09:51:23</dcterms:created>
				<dcterms:modified rdf:datatype="http://www.w3.org/2001/XMLSchema#dateTime">2009-06-24T17:12:49</dcterms:modified>
				<dcterms:issued rdf:datatype="http://www.w3.org/2001/XMLSchema#dateTime">2013-07-17T10:08:40</dcterms:issued>
				<skos:broader rdf:resource="http://purl.org/heritagedata/schemes/4/concepts/502388" />
				<skos:scopeNote xml:lang="en">The measurement of the differential heat spectrum of both extant and buried features, through the use of infrared signals recorded as video still by RAF aircraft.</skos:scopeNote>
			</skos:Concept>
		</skos:narrower>
		<skos:narrower>
			<skos:Concept rdf:about="http://purl.org/heritagedata/schemes/4/concepts/502393">
				<skos:inScheme rdf:resource="http://purl.org/heritagedata/schemes/4" />
				<dcterms:identifier>http://purl.org/heritagedata/schemes/4/concepts/502393</dcterms:identifier>
				<cc:license rdf:resource="http://reference.data.gov.uk/id/open-government-licence" />
				<cc:attributionURL rdf:resource="http://www.rcahms.gov.uk" />
				<cc:attributionName xml:lang="en">RCAHMS</cc:attributionName>
				<dcterms:publisher rdf:resource="http://www.rcahms.gov.uk" />
				<skos:prefLabel xml:lang="en">INFRARED AERIAL PHOTOGRAPHY</skos:prefLabel>
				<dcterms:created rdf:datatype="http://www.w3.org/2001/XMLSchema#dateTime">2007-05-31T09:55:37</dcterms:created>
				<dcterms:modified rdf:datatype="http://www.w3.org/2001/XMLSchema#dateTime">2009-06-24T17:11:32</dcterms:modified>
				<dcterms:issued rdf:datatype="http://www.w3.org/2001/XMLSchema#dateTime">2013-07-17T10:08:40</dcterms:issued>
				<skos:broader rdf:resource="http://purl.org/heritagedata/schemes/4/concepts/502388" />
				<skos:scopeNote xml:lang="en">The use of infrared sensitive film or sensors for aerial photography that reveals different soil characteristics to normal visible light film.</skos:scopeNote>
			</skos:Concept>
		</skos:narrower>
		<skos:narrower>
			<skos:Concept rdf:about="http://purl.org/heritagedata/schemes/4/concepts/502394">
				<skos:inScheme rdf:resource="http://purl.org/heritagedata/schemes/4" />
				<dcterms:identifier>http://purl.org/heritagedata/schemes/4/concepts/502394</dcterms:identifier>
				<cc:license rdf:resource="http://reference.data.gov.uk/id/open-government-licence" />
				<cc:attributionURL rdf:resource="http://www.rcahms.gov.uk" />
				<cc:attributionName xml:lang="en">RCAHMS</cc:attributionName>
				<dcterms:publisher rdf:resource="http://www.rcahms.gov.uk" />
				<skos:prefLabel xml:lang="en">MULTI SPECTRAL AERIAL PHOTOGRAPHY</skos:prefLabel>
				<dcterms:created rdf:datatype="http://www.w3.org/2001/XMLSchema#dateTime">2007-05-31T10:02:41</dcterms:created>
				<dcterms:modified rdf:datatype="http://www.w3.org/2001/XMLSchema#dateTime">2007-12-20T12:26:52</dcterms:modified>
				<dcterms:issued rdf:datatype="http://www.w3.org/2001/XMLSchema#dateTime">2013-07-17T10:08:40</dcterms:issued>
				<skos:broader rdf:resource="http://purl.org/heritagedata/schemes/4/concepts/502388" />
				<skos:scopeNote xml:lang="en">The use of specialist film or sensors to capture detais visible only at wavelengths outside the normal spectrum.</skos:scopeNote>
			</skos:Concept>
		</skos:narrower>
		<skos:narrower>
			<skos:Concept rdf:about="http://purl.org/heritagedata/schemes/4/concepts/503119">
				<skos:inScheme rdf:resource="http://purl.org/heritagedata/schemes/4" />
				<dcterms:identifier>http://purl.org/heritagedata/schemes/4/concepts/503119</dcterms:identifier>
				<cc:license rdf:resource="http://reference.data.gov.uk/id/open-government-licence" />
				<cc:attributionURL rdf:resource="http://www.rcahms.gov.uk" />
				<cc:attributionName xml:lang="en">RCAHMS</cc:attributionName>
				<dcterms:publisher rdf:resource="http://www.rcahms.gov.uk" />
				<skos:prefLabel xml:lang="en">SATELLITE IMAGERY</skos:prefLabel>
				<dcterms:created rdf:datatype="http://www.w3.org/2001/XMLSchema#dateTime">2007-12-20T12:49:29</dcterms:created>
				<dcterms:modified rdf:datatype="http://www.w3.org/2001/XMLSchema#dateTime">2007-12-20T12:50:26</dcterms:modified>
				<dcterms:issued rdf:datatype="http://www.w3.org/2001/XMLSchema#dateTime">2013-07-17T10:08:40</dcterms:issued>
				<skos:broader rdf:resource="http://purl.org/heritagedata/schemes/4/concepts/502388" />
				<skos:scopeNote xml:lang="en">Identification of heritage features from  images derived from orbiting satellites.</skos:scopeNote>
			</skos:Concept>
		</skos:narrower>
		<skos:narrower>
			<skos:Concept rdf:about="http://purl.org/heritagedata/schemes/4/concepts/504421">
				<skos:inScheme rdf:resource="http://purl.org/heritagedata/schemes/4" />
				<dcterms:identifier>http://purl.org/heritagedata/schemes/4/concepts/504421</dcterms:identifier>
				<cc:license rdf:resource="http://reference.data.gov.uk/id/open-government-licence" />
				<cc:attributionURL rdf:resource="http://www.rcahms.gov.uk" />
				<cc:attributionName xml:lang="en">RCAHMS</cc:attributionName>
				<dcterms:publisher rdf:resource="http://www.rcahms.gov.uk" />
				<skos:prefLabel xml:lang="en">LIDAR SURVEY</skos:prefLabel>
				<dcterms:created rdf:datatype="http://www.w3.org/2001/XMLSchema#dateTime">2009-06-24T17:15:12</dcterms:created>
				<dcterms:modified rdf:datatype="http://www.w3.org/2001/XMLSchema#dateTime">2009-06-24T17:22:46</dcterms:modified>
				<dcterms:issued rdf:datatype="http://www.w3.org/2001/XMLSchema#dateTime">2013-07-17T10:08:40</dcterms:issued>
				<skos:broader rdf:resource="http://purl.org/heritagedata/schemes/4/concepts/502388" />
				<skos:scopeNote xml:lang="en">A remote sensing technique, usually airborne,  that uses laser-driven pulses of light and multispectral cameras to scan and process digital information and produce detailed models of the ground surface including detail obscured by vegetation..</skos:scopeNote>
			</skos:Concept>
		</skos:narrower>
		<skos:scopeNote xml:lang="en">A broad group of events relating to aerial survey including photography, interpretation and transcription work. Use specific term where available.</skos:scopeNote>
	</skos:Concept>
	<skos:Concept rdf:about="http://purl.org/heritagedata/schemes/4/concepts/502395">
		<skos:inScheme rdf:resource="http://purl.org/heritagedata/schemes/4" />
		<dcterms:identifier>http://purl.org/heritagedata/schemes/4/concepts/502395</dcterms:identifier>
		<cc:license rdf:resource="http://reference.data.gov.uk/id/open-government-licence" />
		<cc:attributionURL rdf:resource="http://www.rcahms.gov.uk" />
		<cc:attributionName xml:lang="en">RCAHMS</cc:attributionName>
		<dcterms:publisher rdf:resource="http://www.rcahms.gov.uk" />
		<skos:prefLabel xml:lang="en">ANTIQUARIAN OBSERVATION</skos:prefLabel>
		<dcterms:created rdf:datatype="http://www.w3.org/2001/XMLSchema#dateTime">2007-05-31T10:13:49</dcterms:created>
		<dcterms:modified rdf:datatype="http://www.w3.org/2001/XMLSchema#dateTime">2007-05-31T10:14:28</dcterms:modified>
		<dcterms:issued rdf:datatype="http://www.w3.org/2001/XMLSchema#dateTime">2013-07-17T10:08:40</dcterms:issued>
		<skos:broader rdf:resource="http://purl.org/heritagedata/schemes/4/concepts/502362" />
		<skos:broader rdf:resource="http://purl.org/heritagedata/schemes/4/concepts/502432" />
		<skos:scopeNote xml:lang="en">Observations made by antiquarians and reported through  publication or from unpublished manuscripts.</skos:scopeNote>
	</skos:Concept>
	<skos:Concept rdf:about="http://purl.org/heritagedata/schemes/4/concepts/502396">
		<skos:inScheme rdf:resource="http://purl.org/heritagedata/schemes/4" />
		<dcterms:identifier>http://purl.org/heritagedata/schemes/4/concepts/502396</dcterms:identifier>
		<cc:license rdf:resource="http://reference.data.gov.uk/id/open-government-licence" />
		<cc:attributionURL rdf:resource="http://www.rcahms.gov.uk" />
		<cc:attributionName xml:lang="en">RCAHMS</cc:attributionName>
		<dcterms:publisher rdf:resource="http://www.rcahms.gov.uk" />
		<skos:prefLabel xml:lang="en">ARCHAEOLOGICAL EVALUATION</skos:prefLabel>
		<dcterms:created rdf:datatype="http://www.w3.org/2001/XMLSchema#dateTime">2007-05-31T11:23:32</dcterms:created>
		<dcterms:modified rdf:datatype="http://www.w3.org/2001/XMLSchema#dateTime">2007-05-31T11:30:22</dcterms:modified>
		<dcterms:issued rdf:datatype="http://www.w3.org/2001/XMLSchema#dateTime">2013-07-17T10:08:40</dcterms:issued>
		<skos:broader rdf:resource="http://purl.org/heritagedata/schemes/4/concepts/502416" />
		<skos:related rdf:resource="http://purl.org/heritagedata/schemes/4/concepts/502418" />
		<skos:scopeNote xml:lang="en">An archaeological excavation employing a  sampling strategy (typically 5% or 10% of an area) to evaluate the archaeology of an area usually in advance of a  development.</skos:scopeNote>
	</skos:Concept>
	<skos:Concept rdf:about="http://purl.org/heritagedata/schemes/4/concepts/502399">
		<skos:inScheme rdf:resource="http://purl.org/heritagedata/schemes/4" />
		<dcterms:identifier>http://purl.org/heritagedata/schemes/4/concepts/502399</dcterms:identifier>
		<cc:license rdf:resource="http://reference.data.gov.uk/id/open-government-licence" />
		<cc:attributionURL rdf:resource="http://www.rcahms.gov.uk" />
		<cc:attributionName xml:lang="en">RCAHMS</cc:attributionName>
		<dcterms:publisher rdf:resource="http://www.rcahms.gov.uk" />
		<skos:prefLabel xml:lang="en">FIELD VISIT</skos:prefLabel>
		<dcterms:created rdf:datatype="http://www.w3.org/2001/XMLSchema#dateTime">2007-05-31T11:34:51</dcterms:created>
		<dcterms:modified rdf:datatype="http://www.w3.org/2001/XMLSchema#dateTime">2007-10-29T10:59:55</dcterms:modified>
		<dcterms:issued rdf:datatype="http://www.w3.org/2001/XMLSchema#dateTime">2013-07-17T10:08:40</dcterms:issued>
		<skos:narrower>
			<skos:Concept rdf:about="http://purl.org/heritagedata/schemes/4/concepts/502363">
				<skos:inScheme rdf:resource="http://purl.org/heritagedata/schemes/4" />
				<dcterms:identifier>http://purl.org/heritagedata/schemes/4/concepts/502363</dcterms:identifier>
				<cc:license rdf:resource="http://reference.data.gov.uk/id/open-government-licence" />
				<cc:attributionURL rdf:resource="http://www.rcahms.gov.uk" />
				<cc:attributionName xml:lang="en">RCAHMS</cc:attributionName>
				<dcterms:publisher rdf:resource="http://www.rcahms.gov.uk" />
				<skos:prefLabel xml:lang="en">MEASURED SURVEY</skos:prefLabel>
				<dcterms:created rdf:datatype="http://www.w3.org/2001/XMLSchema#dateTime">2007-05-31T13:09:43</dcterms:created>
				<dcterms:modified rdf:datatype="http://www.w3.org/2001/XMLSchema#dateTime">2010-01-14T15:27:06</dcterms:modified>
				<dcterms:issued rdf:datatype="http://www.w3.org/2001/XMLSchema#dateTime">2013-07-17T10:08:40</dcterms:issued>
				<skos:broader rdf:resource="http://purl.org/heritagedata/schemes/4/concepts/502399" />
				<skos:scopeNote xml:lang="en">The systematic recording of dimensions of an object, monument, building or landscape.</skos:scopeNote>
			</skos:Concept>
		</skos:narrower>
		<skos:narrower>
			<skos:Concept rdf:about="http://purl.org/heritagedata/schemes/4/concepts/502520">
				<skos:inScheme rdf:resource="http://purl.org/heritagedata/schemes/4" />
				<dcterms:identifier>http://purl.org/heritagedata/schemes/4/concepts/502520</dcterms:identifier>
				<cc:license rdf:resource="http://reference.data.gov.uk/id/open-government-licence" />
				<cc:attributionURL rdf:resource="http://www.rcahms.gov.uk" />
				<cc:attributionName xml:lang="en">RCAHMS</cc:attributionName>
				<dcterms:publisher rdf:resource="http://www.rcahms.gov.uk" />
				<skos:prefLabel xml:lang="en">CONDITION SURVEY</skos:prefLabel>
				<dcterms:created rdf:datatype="http://www.w3.org/2001/XMLSchema#dateTime">2007-06-04T14:27:41</dcterms:created>
				<dcterms:modified rdf:datatype="http://www.w3.org/2001/XMLSchema#dateTime">2007-06-04T14:28:51</dcterms:modified>
				<dcterms:issued rdf:datatype="http://www.w3.org/2001/XMLSchema#dateTime">2013-07-17T10:08:40</dcterms:issued>
				<skos:broader rdf:resource="http://purl.org/heritagedata/schemes/4/concepts/502399" />
				<skos:scopeNote xml:lang="en">To be used in association with a field survey visit.</skos:scopeNote>
			</skos:Concept>
		</skos:narrower>
		<skos:broader rdf:resource="http://purl.org/heritagedata/schemes/4/concepts/502432" />
		<skos:broader rdf:resource="http://purl.org/heritagedata/schemes/4/concepts/502362" />
		<skos:scopeNote xml:lang="en">Observations made by an archaeologist, industrial archaeologist or architectural historian (professional or amateur) from a field visit.</skos:scopeNote>
	</skos:Concept>
	<skos:Concept rdf:about="http://purl.org/heritagedata/schemes/4/concepts/502401">
		<skos:inScheme rdf:resource="http://purl.org/heritagedata/schemes/4" />
		<dcterms:identifier>http://purl.org/heritagedata/schemes/4/concepts/502401</dcterms:identifier>
		<cc:license rdf:resource="http://reference.data.gov.uk/id/open-government-licence" />
		<cc:attributionURL rdf:resource="http://www.rcahms.gov.uk" />
		<cc:attributionName xml:lang="en">RCAHMS</cc:attributionName>
		<dcterms:publisher rdf:resource="http://www.rcahms.gov.uk" />
		<skos:prefLabel xml:lang="en">NON INVASIVE TECHNIQUES</skos:prefLabel>
		<dcterms:created rdf:datatype="http://www.w3.org/2001/XMLSchema#dateTime">2007-05-31T11:38:05</dcterms:created>
		<dcterms:modified rdf:datatype="http://www.w3.org/2001/XMLSchema#dateTime">2007-06-05T11:25:49</dcterms:modified>
		<dcterms:issued rdf:datatype="http://www.w3.org/2001/XMLSchema#dateTime">2013-07-17T10:08:40</dcterms:issued>
		<skos:narrower>
			<skos:Concept rdf:about="http://purl.org/heritagedata/schemes/4/concepts/502407">
				<skos:inScheme rdf:resource="http://purl.org/heritagedata/schemes/4" />
				<dcterms:identifier>http://purl.org/heritagedata/schemes/4/concepts/502407</dcterms:identifier>
				<cc:license rdf:resource="http://reference.data.gov.uk/id/open-government-licence" />
				<cc:attributionURL rdf:resource="http://www.rcahms.gov.uk" />
				<cc:attributionName xml:lang="en">RCAHMS</cc:attributionName>
				<dcterms:publisher rdf:resource="http://www.rcahms.gov.uk" />
				<skos:prefLabel xml:lang="en">WIRE SWEEP SURVEY</skos:prefLabel>
				<dcterms:created rdf:datatype="http://www.w3.org/2001/XMLSchema#dateTime">2007-05-31T16:09:19</dcterms:created>
				<dcterms:modified rdf:datatype="http://www.w3.org/2001/XMLSchema#dateTime">2012-05-02T09:16:00</dcterms:modified>
				<dcterms:issued rdf:datatype="http://www.w3.org/2001/XMLSchema#dateTime">2013-07-17T10:08:40</dcterms:issued>
				<skos:broader rdf:resource="http://purl.org/heritagedata/schemes/4/concepts/502401" />
				<skos:scopeNote xml:lang="en">A method of checking the depth of safe water using a single or pairs of survey launches holding minesweeping gear (or a kite otter) to provide a minimum depth above an obstruction.</skos:scopeNote>
			</skos:Concept>
		</skos:narrower>
		<skos:narrower>
			<skos:Concept rdf:about="http://purl.org/heritagedata/schemes/4/concepts/502521">
				<skos:inScheme rdf:resource="http://purl.org/heritagedata/schemes/4" />
				<dcterms:identifier>http://purl.org/heritagedata/schemes/4/concepts/502521</dcterms:identifier>
				<cc:license rdf:resource="http://reference.data.gov.uk/id/open-government-licence" />
				<cc:attributionURL rdf:resource="http://www.rcahms.gov.uk" />
				<cc:attributionName xml:lang="en">RCAHMS</cc:attributionName>
				<dcterms:publisher rdf:resource="http://www.rcahms.gov.uk" />
				<skos:prefLabel xml:lang="en">DIVER INSPECTION</skos:prefLabel>
				<dcterms:created rdf:datatype="http://www.w3.org/2001/XMLSchema#dateTime">2007-06-04T14:29:51</dcterms:created>
				<dcterms:modified rdf:datatype="http://www.w3.org/2001/XMLSchema#dateTime">2012-05-02T09:21:33</dcterms:modified>
				<dcterms:issued rdf:datatype="http://www.w3.org/2001/XMLSchema#dateTime">2013-07-17T10:08:40</dcterms:issued>
				<skos:broader rdf:resource="http://purl.org/heritagedata/schemes/4/concepts/502401" />
				<skos:scopeNote xml:lang="en">An assessment of a known wreck or underwater archaeological site through diving.</skos:scopeNote>
			</skos:Concept>
		</skos:narrower>
		<skos:narrower rdf:resource="http://purl.org/heritagedata/schemes/4/concepts/502388" />
		<skos:narrower rdf:resource="http://purl.org/heritagedata/schemes/4/concepts/502432" />
		<skos:broader rdf:resource="http://purl.org/heritagedata/schemes/4/concepts/502346" />
		<skos:narrower rdf:resource="http://purl.org/heritagedata/schemes/4/concepts/502362" />
		<skos:narrower rdf:resource="http://purl.org/heritagedata/schemes/4/concepts/506601" />
		<skos:scopeNote xml:lang="en">A series of methods that do not involve ground disturbance and are used to survey and record information about archaeological sites, landscapes and the built environment.</skos:scopeNote>
	</skos:Concept>
	<skos:Concept rdf:about="http://purl.org/heritagedata/schemes/4/concepts/502362">
		<skos:inScheme rdf:resource="http://purl.org/heritagedata/schemes/4" />
		<dcterms:identifier>http://purl.org/heritagedata/schemes/4/concepts/502362</dcterms:identifier>
		<cc:license rdf:resource="http://reference.data.gov.uk/id/open-government-licence" />
		<cc:attributionURL rdf:resource="http://www.rcahms.gov.uk" />
		<cc:attributionName xml:lang="en">RCAHMS</cc:attributionName>
		<dcterms:publisher rdf:resource="http://www.rcahms.gov.uk" />
		<skos:prefLabel xml:lang="en">STANDING BUILDING RECORDING</skos:prefLabel>
		<dcterms:created rdf:datatype="http://www.w3.org/2001/XMLSchema#dateTime">2007-05-31T11:43:07</dcterms:created>
		<dcterms:modified rdf:datatype="http://www.w3.org/2001/XMLSchema#dateTime">2007-05-31T11:44:06</dcterms:modified>
		<dcterms:issued rdf:datatype="http://www.w3.org/2001/XMLSchema#dateTime">2013-07-17T10:08:40</dcterms:issued>
		<skos:narrower>
			<skos:Concept rdf:about="http://purl.org/heritagedata/schemes/4/concepts/502366">
				<skos:inScheme rdf:resource="http://purl.org/heritagedata/schemes/4" />
				<dcterms:identifier>http://purl.org/heritagedata/schemes/4/concepts/502366</dcterms:identifier>
				<cc:license rdf:resource="http://reference.data.gov.uk/id/open-government-licence" />
				<cc:attributionURL rdf:resource="http://www.rcahms.gov.uk" />
				<cc:attributionName xml:lang="en">RCAHMS</cc:attributionName>
				<dcterms:publisher rdf:resource="http://www.rcahms.gov.uk" />
				<skos:prefLabel xml:lang="en">OBSERVATION</skos:prefLabel>
				<dcterms:created rdf:datatype="http://www.w3.org/2001/XMLSchema#dateTime">2007-05-31T15:37:22</dcterms:created>
				<dcterms:modified rdf:datatype="http://www.w3.org/2001/XMLSchema#dateTime">2007-05-31T15:37:48</dcterms:modified>
				<dcterms:issued rdf:datatype="http://www.w3.org/2001/XMLSchema#dateTime">2013-07-17T10:08:40</dcterms:issued>
				<skos:broader rdf:resource="http://purl.org/heritagedata/schemes/4/concepts/502362" />
				<skos:scopeNote xml:lang="en">A written account describing the features of a building or monument. Observational detail may include some photography for record purposes</skos:scopeNote>
			</skos:Concept>
		</skos:narrower>
		<skos:narrower rdf:resource="http://purl.org/heritagedata/schemes/4/concepts/502367" />
		<skos:narrower rdf:resource="http://purl.org/heritagedata/schemes/4/concepts/502368" />
		<skos:narrower rdf:resource="http://purl.org/heritagedata/schemes/4/concepts/502395" />
		<skos:narrower rdf:resource="http://purl.org/heritagedata/schemes/4/concepts/502592" />
		<skos:narrower>
			<skos:Concept rdf:about="http://purl.org/heritagedata/schemes/4/concepts/502364">
				<skos:inScheme rdf:resource="http://purl.org/heritagedata/schemes/4" />
				<dcterms:identifier>http://purl.org/heritagedata/schemes/4/concepts/502364</dcterms:identifier>
				<cc:license rdf:resource="http://reference.data.gov.uk/id/open-government-licence" />
				<cc:attributionURL rdf:resource="http://www.rcahms.gov.uk" />
				<cc:attributionName xml:lang="en">RCAHMS</cc:attributionName>
				<dcterms:publisher rdf:resource="http://www.rcahms.gov.uk" />
				<skos:prefLabel xml:lang="en">FABRIC RECORDING</skos:prefLabel>
				<dcterms:created rdf:datatype="http://www.w3.org/2001/XMLSchema#dateTime">2007-05-31T13:10:40</dcterms:created>
				<dcterms:modified rdf:datatype="http://www.w3.org/2001/XMLSchema#dateTime">2007-05-31T15:34:27</dcterms:modified>
				<dcterms:issued rdf:datatype="http://www.w3.org/2001/XMLSchema#dateTime">2013-07-17T10:08:40</dcterms:issued>
				<skos:broader rdf:resource="http://purl.org/heritagedata/schemes/4/concepts/502362" />
				<skos:scopeNote xml:lang="en">The recording and analysis of the fabric of a built feature or building.</skos:scopeNote>
			</skos:Concept>
		</skos:narrower>
		<skos:broader rdf:resource="http://purl.org/heritagedata/schemes/4/concepts/502401" />
		<skos:narrower>
			<skos:Concept rdf:about="http://purl.org/heritagedata/schemes/4/concepts/502365">
				<skos:inScheme rdf:resource="http://purl.org/heritagedata/schemes/4" />
				<dcterms:identifier>http://purl.org/heritagedata/schemes/4/concepts/502365</dcterms:identifier>
				<cc:license rdf:resource="http://reference.data.gov.uk/id/open-government-licence" />
				<cc:attributionURL rdf:resource="http://www.rcahms.gov.uk" />
				<cc:attributionName xml:lang="en">RCAHMS</cc:attributionName>
				<dcterms:publisher rdf:resource="http://www.rcahms.gov.uk" />
				<skos:prefLabel xml:lang="en">PHOTOGRAMMETRIC SURVEY</skos:prefLabel>
				<dcterms:created rdf:datatype="http://www.w3.org/2001/XMLSchema#dateTime">2007-05-31T15:35:07</dcterms:created>
				<dcterms:modified rdf:datatype="http://www.w3.org/2001/XMLSchema#dateTime">2007-05-31T15:36:01</dcterms:modified>
				<dcterms:issued rdf:datatype="http://www.w3.org/2001/XMLSchema#dateTime">2013-07-17T10:08:40</dcterms:issued>
				<skos:broader rdf:resource="http://purl.org/heritagedata/schemes/4/concepts/502362" />
				<skos:scopeNote xml:lang="en">The measurement of a surface (either in elevation or in plan) determined from measurements made in two or more photographic images taken from different positions.</skos:scopeNote>
			</skos:Concept>
		</skos:narrower>
		<skos:narrower rdf:resource="http://purl.org/heritagedata/schemes/4/concepts/502399" />
		<skos:narrower rdf:resource="http://purl.org/heritagedata/schemes/4/concepts/503057" />
		<skos:scopeNote xml:lang="en">The recording of the key features of a building through observation and / or a variety of techniques.</skos:scopeNote>
	</skos:Concept>
	<skos:Concept rdf:about="http://purl.org/heritagedata/schemes/4/concepts/502367">
		<skos:inScheme rdf:resource="http://purl.org/heritagedata/schemes/4" />
		<dcterms:identifier>http://purl.org/heritagedata/schemes/4/concepts/502367</dcterms:identifier>
		<cc:license rdf:resource="http://reference.data.gov.uk/id/open-government-licence" />
		<cc:attributionURL rdf:resource="http://www.rcahms.gov.uk" />
		<cc:attributionName xml:lang="en">RCAHMS</cc:attributionName>
		<dcterms:publisher rdf:resource="http://www.rcahms.gov.uk" />
		<skos:prefLabel xml:lang="en">PHOTOGRAPHIC SURVEY</skos:prefLabel>
		<dcterms:created rdf:datatype="http://www.w3.org/2001/XMLSchema#dateTime">2007-05-31T15:39:06</dcterms:created>
		<dcterms:modified rdf:datatype="http://www.w3.org/2001/XMLSchema#dateTime">2007-06-01T11:02:23</dcterms:modified>
		<dcterms:issued rdf:datatype="http://www.w3.org/2001/XMLSchema#dateTime">2013-07-17T10:08:40</dcterms:issued>
		<skos:broader rdf:resource="http://purl.org/heritagedata/schemes/4/concepts/502362" />
		<skos:broader rdf:resource="http://purl.org/heritagedata/schemes/4/concepts/502432" />
		<skos:scopeNote xml:lang="en">A photographic record of a building or monument carried out as part of a planned programme of recording to create a comprehensive visual record.</skos:scopeNote>
	</skos:Concept>
	<skos:Concept rdf:about="http://purl.org/heritagedata/schemes/4/concepts/502368">
		<skos:inScheme rdf:resource="http://purl.org/heritagedata/schemes/4" />
		<dcterms:identifier>http://purl.org/heritagedata/schemes/4/concepts/502368</dcterms:identifier>
		<cc:license rdf:resource="http://reference.data.gov.uk/id/open-government-licence" />
		<cc:attributionURL rdf:resource="http://www.rcahms.gov.uk" />
		<cc:attributionName xml:lang="en">RCAHMS</cc:attributionName>
		<dcterms:publisher rdf:resource="http://www.rcahms.gov.uk" />
		<skos:prefLabel xml:lang="en">LASER SCANNING</skos:prefLabel>
		<dcterms:created rdf:datatype="http://www.w3.org/2001/XMLSchema#dateTime">2007-05-31T15:40:42</dcterms:created>
		<dcterms:modified rdf:datatype="http://www.w3.org/2001/XMLSchema#dateTime">2007-05-31T15:42:01</dcterms:modified>
		<dcterms:issued rdf:datatype="http://www.w3.org/2001/XMLSchema#dateTime">2013-07-17T10:08:40</dcterms:issued>
		<skos:broader rdf:resource="http://purl.org/heritagedata/schemes/4/concepts/502432" />
		<skos:broader rdf:resource="http://purl.org/heritagedata/schemes/4/concepts/502362" />
		<skos:scopeNote xml:lang="en">The recording of a surface, or surfaces, by laser equipment to create a 3-D model of the target object.</skos:scopeNote>
	</skos:Concept>
	<skos:Concept rdf:about="http://purl.org/heritagedata/schemes/4/concepts/502370">
		<skos:inScheme rdf:resource="http://purl.org/heritagedata/schemes/4" />
		<dcterms:identifier>http://purl.org/heritagedata/schemes/4/concepts/502370</dcterms:identifier>
		<cc:license rdf:resource="http://reference.data.gov.uk/id/open-government-licence" />
		<cc:attributionURL rdf:resource="http://www.rcahms.gov.uk" />
		<cc:attributionName xml:lang="en">RCAHMS</cc:attributionName>
		<dcterms:publisher rdf:resource="http://www.rcahms.gov.uk" />
		<skos:prefLabel xml:lang="en">CONTOUR  SURVEY</skos:prefLabel>
		<dcterms:created rdf:datatype="http://www.w3.org/2001/XMLSchema#dateTime">2007-05-31T15:43:42</dcterms:created>
		<dcterms:modified rdf:datatype="http://www.w3.org/2001/XMLSchema#dateTime">2007-05-31T15:55:43</dcterms:modified>
		<dcterms:issued rdf:datatype="http://www.w3.org/2001/XMLSchema#dateTime">2013-07-17T10:08:40</dcterms:issued>
		<skos:broader rdf:resource="http://purl.org/heritagedata/schemes/4/concepts/502432" />
		<skos:related rdf:resource="http://purl.org/heritagedata/schemes/4/concepts/502371" />
		<skos:scopeNote xml:lang="en">A measured plan of a ground surface mapping points of equal height interpolated to create a contour map of an archaeological site.</skos:scopeNote>
	</skos:Concept>
	<skos:Concept rdf:about="http://purl.org/heritagedata/schemes/4/concepts/502371">
		<skos:inScheme rdf:resource="http://purl.org/heritagedata/schemes/4" />
		<dcterms:identifier>http://purl.org/heritagedata/schemes/4/concepts/502371</dcterms:identifier>
		<cc:license rdf:resource="http://reference.data.gov.uk/id/open-government-licence" />
		<cc:attributionURL rdf:resource="http://www.rcahms.gov.uk" />
		<cc:attributionName xml:lang="en">RCAHMS</cc:attributionName>
		<dcterms:publisher rdf:resource="http://www.rcahms.gov.uk" />
		<skos:prefLabel xml:lang="en">DIGITAL TERRAIN MODEL</skos:prefLabel>
		<dcterms:created rdf:datatype="http://www.w3.org/2001/XMLSchema#dateTime">2007-05-31T15:47:41</dcterms:created>
		<dcterms:modified rdf:datatype="http://www.w3.org/2001/XMLSchema#dateTime">2007-05-31T15:53:28</dcterms:modified>
		<dcterms:issued rdf:datatype="http://www.w3.org/2001/XMLSchema#dateTime">2013-07-17T10:08:40</dcterms:issued>
		<skos:broader rdf:resource="http://purl.org/heritagedata/schemes/4/concepts/502432" />
		<skos:related rdf:resource="http://purl.org/heritagedata/schemes/4/concepts/502370" />
		<skos:scopeNote xml:lang="en">A 3 dimensional representation of  a land-surface created through ground survey or from remote sensing techniques.</skos:scopeNote>
	</skos:Concept>
	<skos:Concept rdf:about="http://purl.org/heritagedata/schemes/4/concepts/502402">
		<skos:inScheme rdf:resource="http://purl.org/heritagedata/schemes/4" />
		<dcterms:identifier>http://purl.org/heritagedata/schemes/4/concepts/502402</dcterms:identifier>
		<cc:license rdf:resource="http://reference.data.gov.uk/id/open-government-licence" />
		<cc:attributionURL rdf:resource="http://www.rcahms.gov.uk" />
		<cc:attributionName xml:lang="en">RCAHMS</cc:attributionName>
		<dcterms:publisher rdf:resource="http://www.rcahms.gov.uk" />
		<skos:prefLabel xml:lang="en">UNDERWATER  ARCHAEOLOGY</skos:prefLabel>
		<dcterms:created rdf:datatype="http://www.w3.org/2001/XMLSchema#dateTime">2007-05-31T15:57:50</dcterms:created>
		<dcterms:modified rdf:datatype="http://www.w3.org/2001/XMLSchema#dateTime">2007-05-31T16:01:51</dcterms:modified>
		<dcterms:issued rdf:datatype="http://www.w3.org/2001/XMLSchema#dateTime">2013-07-17T10:08:40</dcterms:issued>
		<skos:broader rdf:resource="http://purl.org/heritagedata/schemes/4/concepts/502346" />
		<skos:narrower>
			<skos:Concept rdf:about="http://purl.org/heritagedata/schemes/4/concepts/502408">
				<skos:inScheme rdf:resource="http://purl.org/heritagedata/schemes/4" />
				<dcterms:identifier>http://purl.org/heritagedata/schemes/4/concepts/502408</dcterms:identifier>
				<cc:license rdf:resource="http://reference.data.gov.uk/id/open-government-licence" />
				<cc:attributionURL rdf:resource="http://www.rcahms.gov.uk" />
				<cc:attributionName xml:lang="en">RCAHMS</cc:attributionName>
				<dcterms:publisher rdf:resource="http://www.rcahms.gov.uk" />
				<skos:prefLabel xml:lang="en">PRE DISTURBANCE SURVEY</skos:prefLabel>
				<dcterms:created rdf:datatype="http://www.w3.org/2001/XMLSchema#dateTime">2007-05-31T16:10:04</dcterms:created>
				<dcterms:modified rdf:datatype="http://www.w3.org/2001/XMLSchema#dateTime">2007-05-31T16:10:44</dcterms:modified>
				<dcterms:issued rdf:datatype="http://www.w3.org/2001/XMLSchema#dateTime">2013-07-17T10:08:40</dcterms:issued>
				<skos:broader rdf:resource="http://purl.org/heritagedata/schemes/4/concepts/502402" />
				<skos:scopeNote xml:lang="en">The recording of the position of a maritime object. Notes should include a comment on the degree of archaeological veracity.</skos:scopeNote>
			</skos:Concept>
		</skos:narrower>
		<skos:narrower>
			<skos:Concept rdf:about="http://purl.org/heritagedata/schemes/4/concepts/503438">
				<skos:inScheme rdf:resource="http://purl.org/heritagedata/schemes/4" />
				<dcterms:identifier>http://purl.org/heritagedata/schemes/4/concepts/503438</dcterms:identifier>
				<cc:license rdf:resource="http://reference.data.gov.uk/id/open-government-licence" />
				<cc:attributionURL rdf:resource="http://www.rcahms.gov.uk" />
				<cc:attributionName xml:lang="en">RCAHMS</cc:attributionName>
				<dcterms:publisher rdf:resource="http://www.rcahms.gov.uk" />
				<skos:prefLabel xml:lang="en">EVIDENCE OF LOSS</skos:prefLabel>
				<dcterms:created rdf:datatype="http://www.w3.org/2001/XMLSchema#dateTime">2008-07-24T16:05:58</dcterms:created>
				<dcterms:modified rdf:datatype="http://www.w3.org/2001/XMLSchema#dateTime">2009-01-09T16:20:14</dcterms:modified>
				<dcterms:issued rdf:datatype="http://www.w3.org/2001/XMLSchema#dateTime">2013-07-17T10:08:40</dcterms:issued>
				<skos:broader rdf:resource="http://purl.org/heritagedata/schemes/4/concepts/502402" />
				<skos:scopeNote xml:lang="en">This category applies where the discovery of wreckage indicates the prior loss (generally through foundering) of a vessel, possibly at some remove in time and location from those of the discovery of wreckage.</skos:scopeNote>
			</skos:Concept>
		</skos:narrower>
		<skos:scopeNote xml:lang="en">Fieldwork activities associated with the recording of submerged archaeological sites and landscapes  in either freshwater or salt water locations.</skos:scopeNote>
	</skos:Concept>
	<skos:Concept rdf:about="http://purl.org/heritagedata/schemes/4/concepts/502416">
		<skos:inScheme rdf:resource="http://purl.org/heritagedata/schemes/4" />
		<dcterms:identifier>http://purl.org/heritagedata/schemes/4/concepts/502416</dcterms:identifier>
		<cc:license rdf:resource="http://reference.data.gov.uk/id/open-government-licence" />
		<cc:attributionURL rdf:resource="http://www.rcahms.gov.uk" />
		<cc:attributionName xml:lang="en">RCAHMS</cc:attributionName>
		<dcterms:publisher rdf:resource="http://www.rcahms.gov.uk" />
		<skos:prefLabel xml:lang="en">INVASIVE TECHNIQUES</skos:prefLabel>
		<dcterms:created rdf:datatype="http://www.w3.org/2001/XMLSchema#dateTime">2007-06-01T09:22:11</dcterms:created>
		<dcterms:modified rdf:datatype="http://www.w3.org/2001/XMLSchema#dateTime">2007-06-01T09:26:48</dcterms:modified>
		<dcterms:issued rdf:datatype="http://www.w3.org/2001/XMLSchema#dateTime">2013-07-17T10:08:40</dcterms:issued>
		<skos:narrower>
			<skos:Concept rdf:about="http://purl.org/heritagedata/schemes/4/concepts/502369">
				<skos:inScheme rdf:resource="http://purl.org/heritagedata/schemes/4" />
				<dcterms:identifier>http://purl.org/heritagedata/schemes/4/concepts/502369</dcterms:identifier>
				<cc:license rdf:resource="http://reference.data.gov.uk/id/open-government-licence" />
				<cc:attributionURL rdf:resource="http://www.rcahms.gov.uk" />
				<cc:attributionName xml:lang="en">RCAHMS</cc:attributionName>
				<dcterms:publisher rdf:resource="http://www.rcahms.gov.uk" />
				<skos:prefLabel xml:lang="en">TEST PIT SURVEY</skos:prefLabel>
				<dcterms:created rdf:datatype="http://www.w3.org/2001/XMLSchema#dateTime">2007-05-31T15:42:52</dcterms:created>
				<dcterms:modified rdf:datatype="http://www.w3.org/2001/XMLSchema#dateTime">2007-05-31T15:43:23</dcterms:modified>
				<dcterms:issued rdf:datatype="http://www.w3.org/2001/XMLSchema#dateTime">2013-07-17T10:08:40</dcterms:issued>
				<skos:broader rdf:resource="http://purl.org/heritagedata/schemes/4/concepts/502416" />
				<skos:scopeNote xml:lang="en">A sampling strategy, using either regularly placed or randomly spaced pits, undertaken to determine the presence or absence of archaeological features in a given area.</skos:scopeNote>
			</skos:Concept>
		</skos:narrower>
		<skos:narrower>
			<skos:Concept rdf:about="http://purl.org/heritagedata/schemes/4/concepts/502405">
				<skos:inScheme rdf:resource="http://purl.org/heritagedata/schemes/4" />
				<dcterms:identifier>http://purl.org/heritagedata/schemes/4/concepts/502405</dcterms:identifier>
				<cc:license rdf:resource="http://reference.data.gov.uk/id/open-government-licence" />
				<cc:attributionURL rdf:resource="http://www.rcahms.gov.uk" />
				<cc:attributionName xml:lang="en">RCAHMS</cc:attributionName>
				<dcterms:publisher rdf:resource="http://www.rcahms.gov.uk" />
				<skos:prefLabel xml:lang="en">SALVAGE OPERATIONS (MARINE)</skos:prefLabel>
				<dcterms:created rdf:datatype="http://www.w3.org/2001/XMLSchema#dateTime">2007-05-31T16:05:35</dcterms:created>
				<dcterms:modified rdf:datatype="http://www.w3.org/2001/XMLSchema#dateTime">2012-05-02T09:18:52</dcterms:modified>
				<dcterms:issued rdf:datatype="http://www.w3.org/2001/XMLSchema#dateTime">2013-07-17T10:08:40</dcterms:issued>
				<skos:broader rdf:resource="http://purl.org/heritagedata/schemes/4/concepts/502416" />
				<skos:scopeNote xml:lang="en">Diving on vessels for the purpose of recovering artefacts or the fabric of the vessel, either as part of an archaeological investigation or for booty.</skos:scopeNote>
			</skos:Concept>
		</skos:narrower>
		<skos:narrower>
			<skos:Concept rdf:about="http://purl.org/heritagedata/schemes/4/concepts/502406">
				<skos:inScheme rdf:resource="http://purl.org/heritagedata/schemes/4" />
				<dcterms:identifier>http://purl.org/heritagedata/schemes/4/concepts/502406</dcterms:identifier>
				<cc:license rdf:resource="http://reference.data.gov.uk/id/open-government-licence" />
				<cc:attributionURL rdf:resource="http://www.rcahms.gov.uk" />
				<cc:attributionName xml:lang="en">RCAHMS</cc:attributionName>
				<dcterms:publisher rdf:resource="http://www.rcahms.gov.uk" />
				<skos:prefLabel xml:lang="en">SALVAGE RECORD</skos:prefLabel>
				<dcterms:created rdf:datatype="http://www.w3.org/2001/XMLSchema#dateTime">2007-05-31T16:06:31</dcterms:created>
				<dcterms:modified rdf:datatype="http://www.w3.org/2001/XMLSchema#dateTime">2007-05-31T16:08:49</dcterms:modified>
				<dcterms:issued rdf:datatype="http://www.w3.org/2001/XMLSchema#dateTime">2013-07-17T10:08:40</dcterms:issued>
				<skos:broader rdf:resource="http://purl.org/heritagedata/schemes/4/concepts/502416" />
				<skos:scopeNote xml:lang="en">Observations and records made by an archaeologist during periodic visits to a development in contrast to a watching brief where a continuous archaeological presence, with the ability to  suspend work, is maintained on site throughout the ground work.</skos:scopeNote>
			</skos:Concept>
		</skos:narrower>
		<skos:broader rdf:resource="http://purl.org/heritagedata/schemes/4/concepts/502346" />
		<skos:narrower>
			<skos:Concept rdf:about="http://purl.org/heritagedata/schemes/4/concepts/502417">
				<skos:inScheme rdf:resource="http://purl.org/heritagedata/schemes/4" />
				<dcterms:identifier>http://purl.org/heritagedata/schemes/4/concepts/502417</dcterms:identifier>
				<cc:license rdf:resource="http://reference.data.gov.uk/id/open-government-licence" />
				<cc:attributionURL rdf:resource="http://www.rcahms.gov.uk" />
				<cc:attributionName xml:lang="en">RCAHMS</cc:attributionName>
				<dcterms:publisher rdf:resource="http://www.rcahms.gov.uk" />
				<skos:prefLabel xml:lang="en">EXCAVATION</skos:prefLabel>
				<dcterms:created rdf:datatype="http://www.w3.org/2001/XMLSchema#dateTime">2007-06-01T09:30:48</dcterms:created>
				<dcterms:modified rdf:datatype="http://www.w3.org/2001/XMLSchema#dateTime">2007-06-01T09:35:34</dcterms:modified>
				<dcterms:issued rdf:datatype="http://www.w3.org/2001/XMLSchema#dateTime">2013-07-17T10:08:40</dcterms:issued>
				<skos:broader rdf:resource="http://purl.org/heritagedata/schemes/4/concepts/502416" />
				<skos:scopeNote xml:lang="en">The systematic removal of archaeological stratigraphy to reveal and record evidence of past human activity and to establish the relationships between structures, artefacts and other evidence in order to interpret past society.</skos:scopeNote>
			</skos:Concept>
		</skos:narrower>
		<skos:narrower rdf:resource="http://purl.org/heritagedata/schemes/4/concepts/502418" />
		<skos:narrower>
			<skos:Concept rdf:about="http://purl.org/heritagedata/schemes/4/concepts/502419">
				<skos:inScheme rdf:resource="http://purl.org/heritagedata/schemes/4" />
				<dcterms:identifier>http://purl.org/heritagedata/schemes/4/concepts/502419</dcterms:identifier>
				<cc:license rdf:resource="http://reference.data.gov.uk/id/open-government-licence" />
				<cc:attributionURL rdf:resource="http://www.rcahms.gov.uk" />
				<cc:attributionName xml:lang="en">RCAHMS</cc:attributionName>
				<dcterms:publisher rdf:resource="http://www.rcahms.gov.uk" />
				<skos:prefLabel xml:lang="en">WATCHING BRIEF</skos:prefLabel>
				<dcterms:created rdf:datatype="http://www.w3.org/2001/XMLSchema#dateTime">2007-06-01T09:47:45</dcterms:created>
				<dcterms:modified rdf:datatype="http://www.w3.org/2001/XMLSchema#dateTime">2007-06-01T09:54:27</dcterms:modified>
				<dcterms:issued rdf:datatype="http://www.w3.org/2001/XMLSchema#dateTime">2013-07-17T10:08:40</dcterms:issued>
				<skos:broader rdf:resource="http://purl.org/heritagedata/schemes/4/concepts/502416" />
				<skos:scopeNote xml:lang="en">The monitoring by an archaeologist of ground disturbance undertaken for non archaeological purposes usually as a result of a planning condition..</skos:scopeNote>
			</skos:Concept>
		</skos:narrower>
		<skos:narrower>
			<skos:Concept rdf:about="http://purl.org/heritagedata/schemes/4/concepts/502572">
				<skos:inScheme rdf:resource="http://purl.org/heritagedata/schemes/4" />
				<dcterms:identifier>http://purl.org/heritagedata/schemes/4/concepts/502572</dcterms:identifier>
				<cc:license rdf:resource="http://reference.data.gov.uk/id/open-government-licence" />
				<cc:attributionURL rdf:resource="http://www.rcahms.gov.uk" />
				<cc:attributionName xml:lang="en">RCAHMS</cc:attributionName>
				<dcterms:publisher rdf:resource="http://www.rcahms.gov.uk" />
				<skos:prefLabel xml:lang="en">STRIP AND RECORD</skos:prefLabel>
				<dcterms:created rdf:datatype="http://www.w3.org/2001/XMLSchema#dateTime">2007-06-08T09:12:46</dcterms:created>
				<dcterms:modified rdf:datatype="http://www.w3.org/2001/XMLSchema#dateTime">2007-06-08T09:13:59</dcterms:modified>
				<dcterms:issued rdf:datatype="http://www.w3.org/2001/XMLSchema#dateTime">2013-07-17T10:08:40</dcterms:issued>
				<skos:broader rdf:resource="http://purl.org/heritagedata/schemes/4/concepts/502416" />
				<skos:scopeNote xml:lang="en">The removal of a large area of topsoil, usually in advance of a development,  under archaeological supervision, recording, and subsequent whole or part excavation of subsurface features revealed.</skos:scopeNote>
			</skos:Concept>
		</skos:narrower>
		<skos:narrower rdf:resource="http://purl.org/heritagedata/schemes/4/concepts/502396" />
		<skos:scopeNote xml:lang="en">A series of methods used to investigate an archaeological site through ground disturbance.</skos:scopeNote>
	</skos:Concept>
	<skos:Concept rdf:about="http://purl.org/heritagedata/schemes/4/concepts/502418">
		<skos:inScheme rdf:resource="http://purl.org/heritagedata/schemes/4" />
		<dcterms:identifier>http://purl.org/heritagedata/schemes/4/concepts/502418</dcterms:identifier>
		<cc:license rdf:resource="http://reference.data.gov.uk/id/open-government-licence" />
		<cc:attributionURL rdf:resource="http://www.rcahms.gov.uk" />
		<cc:attributionName xml:lang="en">RCAHMS</cc:attributionName>
		<dcterms:publisher rdf:resource="http://www.rcahms.gov.uk" />
		<skos:prefLabel xml:lang="en">TRIAL TRENCH</skos:prefLabel>
		<dcterms:created rdf:datatype="http://www.w3.org/2001/XMLSchema#dateTime">2007-06-01T09:39:08</dcterms:created>
		<dcterms:modified rdf:datatype="http://www.w3.org/2001/XMLSchema#dateTime">2007-06-05T11:25:24</dcterms:modified>
		<dcterms:issued rdf:datatype="http://www.w3.org/2001/XMLSchema#dateTime">2013-07-17T10:08:40</dcterms:issued>
		<skos:broader rdf:resource="http://purl.org/heritagedata/schemes/4/concepts/502416" />
		<skos:related rdf:resource="http://purl.org/heritagedata/schemes/4/concepts/502396" />
		<skos:scopeNote xml:lang="en">The investigation of a site  through the removal of topsoil and subsoil to confirm the absence or presence of archaeological stratigraphy and to determine the  location and character of any features revealed.</skos:scopeNote>
	</skos:Concept>
	<skos:Concept rdf:about="http://purl.org/heritagedata/schemes/4/concepts/502432">
		<skos:inScheme rdf:resource="http://purl.org/heritagedata/schemes/4" />
		<dcterms:identifier>http://purl.org/heritagedata/schemes/4/concepts/502432</dcterms:identifier>
		<cc:license rdf:resource="http://reference.data.gov.uk/id/open-government-licence" />
		<cc:attributionURL rdf:resource="http://www.rcahms.gov.uk" />
		<cc:attributionName xml:lang="en">RCAHMS</cc:attributionName>
		<dcterms:publisher rdf:resource="http://www.rcahms.gov.uk" />
		<skos:prefLabel xml:lang="en">GROUND SURVEY</skos:prefLabel>
		<dcterms:created rdf:datatype="http://www.w3.org/2001/XMLSchema#dateTime">2007-06-01T10:41:42</dcterms:created>
		<dcterms:modified rdf:datatype="http://www.w3.org/2001/XMLSchema#dateTime">2007-06-01T10:42:45</dcterms:modified>
		<dcterms:issued rdf:datatype="http://www.w3.org/2001/XMLSchema#dateTime">2013-07-17T10:08:40</dcterms:issued>
		<skos:narrower rdf:resource="http://purl.org/heritagedata/schemes/4/concepts/502368" />
		<skos:narrower rdf:resource="http://purl.org/heritagedata/schemes/4/concepts/502370" />
		<skos:narrower rdf:resource="http://purl.org/heritagedata/schemes/4/concepts/502371" />
		<skos:narrower rdf:resource="http://purl.org/heritagedata/schemes/4/concepts/502592" />
		<skos:narrower>
			<skos:Concept rdf:about="http://purl.org/heritagedata/schemes/4/concepts/502387">
				<skos:inScheme rdf:resource="http://purl.org/heritagedata/schemes/4" />
				<dcterms:identifier>http://purl.org/heritagedata/schemes/4/concepts/502387</dcterms:identifier>
				<cc:license rdf:resource="http://reference.data.gov.uk/id/open-government-licence" />
				<cc:attributionURL rdf:resource="http://www.rcahms.gov.uk" />
				<cc:attributionName xml:lang="en">RCAHMS</cc:attributionName>
				<dcterms:publisher rdf:resource="http://www.rcahms.gov.uk" />
				<skos:prefLabel xml:lang="en">GEOMORPHOLOGICAL SURVEY</skos:prefLabel>
				<dcterms:created rdf:datatype="http://www.w3.org/2001/XMLSchema#dateTime">2007-05-31T09:35:37</dcterms:created>
				<dcterms:modified rdf:datatype="http://www.w3.org/2001/XMLSchema#dateTime">2007-06-05T11:28:00</dcterms:modified>
				<dcterms:issued rdf:datatype="http://www.w3.org/2001/XMLSchema#dateTime">2013-07-17T10:08:40</dcterms:issued>
				<skos:broader rdf:resource="http://purl.org/heritagedata/schemes/4/concepts/502432" />
				<skos:scopeNote xml:lang="en">Field survey undertaken to record geomorphological features in association with or in the  vicinity of an archaeological site or as part of a wider landscape project.</skos:scopeNote>
			</skos:Concept>
		</skos:narrower>
		<skos:narrower rdf:resource="http://purl.org/heritagedata/schemes/4/concepts/502395" />
		<skos:broader rdf:resource="http://purl.org/heritagedata/schemes/4/concepts/502401" />
		<skos:narrower rdf:resource="http://purl.org/heritagedata/schemes/4/concepts/502367" />
		<skos:narrower rdf:resource="http://purl.org/heritagedata/schemes/4/concepts/502399" />
		<skos:narrower>
			<skos:Concept rdf:about="http://purl.org/heritagedata/schemes/4/concepts/502400">
				<skos:inScheme rdf:resource="http://purl.org/heritagedata/schemes/4" />
				<dcterms:identifier>http://purl.org/heritagedata/schemes/4/concepts/502400</dcterms:identifier>
				<cc:license rdf:resource="http://reference.data.gov.uk/id/open-government-licence" />
				<cc:attributionURL rdf:resource="http://www.rcahms.gov.uk" />
				<cc:attributionName xml:lang="en">RCAHMS</cc:attributionName>
				<dcterms:publisher rdf:resource="http://www.rcahms.gov.uk" />
				<skos:prefLabel xml:lang="en">FIELD WALKING</skos:prefLabel>
				<dcterms:created rdf:datatype="http://www.w3.org/2001/XMLSchema#dateTime">2007-05-31T11:36:34</dcterms:created>
				<dcterms:modified rdf:datatype="http://www.w3.org/2001/XMLSchema#dateTime">2007-05-31T11:37:39</dcterms:modified>
				<dcterms:issued rdf:datatype="http://www.w3.org/2001/XMLSchema#dateTime">2013-07-17T10:08:40</dcterms:issued>
				<skos:broader rdf:resource="http://purl.org/heritagedata/schemes/4/concepts/502432" />
				<skos:scopeNote xml:lang="en">Systematic field walking exercise, organised by grid or transect, aimed at collecting or recording artefacts from a ploughed land surface.</skos:scopeNote>
			</skos:Concept>
		</skos:narrower>
		<skos:narrower rdf:resource="http://purl.org/heritagedata/schemes/4/concepts/503057" />
		<skos:narrower>
			<skos:Concept rdf:about="http://purl.org/heritagedata/schemes/4/concepts/503097">
				<skos:inScheme rdf:resource="http://purl.org/heritagedata/schemes/4" />
				<dcterms:identifier>http://purl.org/heritagedata/schemes/4/concepts/503097</dcterms:identifier>
				<cc:license rdf:resource="http://reference.data.gov.uk/id/open-government-licence" />
				<cc:attributionURL rdf:resource="http://www.rcahms.gov.uk" />
				<cc:attributionName xml:lang="en">RCAHMS</cc:attributionName>
				<dcterms:publisher rdf:resource="http://www.rcahms.gov.uk" />
				<skos:prefLabel xml:lang="en">CASUAL OBSERVATION</skos:prefLabel>
				<dcterms:created rdf:datatype="http://www.w3.org/2001/XMLSchema#dateTime">2007-12-19T09:52:17</dcterms:created>
				<dcterms:modified rdf:datatype="http://www.w3.org/2001/XMLSchema#dateTime">2011-05-20T11:52:51</dcterms:modified>
				<dcterms:issued rdf:datatype="http://www.w3.org/2001/XMLSchema#dateTime">2013-07-17T10:08:40</dcterms:issued>
				<skos:broader rdf:resource="http://purl.org/heritagedata/schemes/4/concepts/502432" />
				<skos:scopeNote xml:lang="en">The unplanned observation of archaeological features.</skos:scopeNote>
			</skos:Concept>
		</skos:narrower>
		<skos:narrower>
			<skos:Concept rdf:about="http://purl.org/heritagedata/schemes/4/concepts/503458">
				<skos:inScheme rdf:resource="http://purl.org/heritagedata/schemes/4" />
				<dcterms:identifier>http://purl.org/heritagedata/schemes/4/concepts/503458</dcterms:identifier>
				<cc:license rdf:resource="http://reference.data.gov.uk/id/open-government-licence" />
				<cc:attributionURL rdf:resource="http://www.rcahms.gov.uk" />
				<cc:attributionName xml:lang="en">RCAHMS</cc:attributionName>
				<dcterms:publisher rdf:resource="http://www.rcahms.gov.uk" />
				<skos:prefLabel xml:lang="en">ARTEFACT RECOVERY</skos:prefLabel>
				<dcterms:created rdf:datatype="http://www.w3.org/2001/XMLSchema#dateTime">2008-07-28T14:01:13</dcterms:created>
				<dcterms:modified rdf:datatype="http://www.w3.org/2001/XMLSchema#dateTime">2008-07-28T14:13:25</dcterms:modified>
				<dcterms:issued rdf:datatype="http://www.w3.org/2001/XMLSchema#dateTime">2013-07-17T10:08:40</dcterms:issued>
				<skos:broader rdf:resource="http://purl.org/heritagedata/schemes/4/concepts/502432" />
				<skos:scopeNote xml:lang="en">The casual recovery of artefacts from the ground surface, usually by an individual or amateur group.</skos:scopeNote>
			</skos:Concept>
		</skos:narrower>
		<skos:scopeNote xml:lang="en">Methods and techniques used to record archaeological sites and landscapes on the ground.</skos:scopeNote>
	</skos:Concept>
	<skos:Concept rdf:about="http://purl.org/heritagedata/schemes/4/concepts/502338">
		<skos:inScheme rdf:resource="http://purl.org/heritagedata/schemes/4" />
		<dcterms:identifier>http://purl.org/heritagedata/schemes/4/concepts/502338</dcterms:identifier>
		<cc:license rdf:resource="http://reference.data.gov.uk/id/open-government-licence" />
		<cc:attributionURL rdf:resource="http://www.rcahms.gov.uk" />
		<cc:attributionName xml:lang="en">RCAHMS</cc:attributionName>
		<dcterms:publisher rdf:resource="http://www.rcahms.gov.uk" />
		<skos:topConceptOf rdf:resource="http://purl.org/heritagedata/schemes/4" />
		<skos:prefLabel xml:lang="en">PROJECT</skos:prefLabel>
		<dcterms:created rdf:datatype="http://www.w3.org/2001/XMLSchema#dateTime">2007-05-30T09:18:04</dcterms:created>
		<dcterms:modified rdf:datatype="http://www.w3.org/2001/XMLSchema#dateTime">2008-01-07T14:05:22</dcterms:modified>
		<dcterms:issued rdf:datatype="http://www.w3.org/2001/XMLSchema#dateTime">2013-07-17T10:08:40</dcterms:issued>
		<skos:narrower>
			<skos:Concept rdf:about="http://purl.org/heritagedata/schemes/4/concepts/505861">
				<skos:inScheme rdf:resource="http://purl.org/heritagedata/schemes/4" />
				<dcterms:identifier>http://purl.org/heritagedata/schemes/4/concepts/505861</dcterms:identifier>
				<cc:license rdf:resource="http://reference.data.gov.uk/id/open-government-licence" />
				<cc:attributionURL rdf:resource="http://www.rcahms.gov.uk" />
				<cc:attributionName xml:lang="en">RCAHMS</cc:attributionName>
				<dcterms:publisher rdf:resource="http://www.rcahms.gov.uk" />
				<skos:prefLabel xml:lang="en">OIC_PROJECT</skos:prefLabel>
				<dcterms:created rdf:datatype="http://www.w3.org/2001/XMLSchema#dateTime">2011-06-07T14:48:07</dcterms:created>
				<dcterms:modified rdf:datatype="http://www.w3.org/2001/XMLSchema#dateTime">2011-06-07T16:17:18</dcterms:modified>
				<dcterms:issued rdf:datatype="http://www.w3.org/2001/XMLSchema#dateTime">2013-07-17T10:08:40</dcterms:issued>
				<skos:broader rdf:resource="http://purl.org/heritagedata/schemes/4/concepts/502338" />
				<skos:scopeNote xml:lang="en">OIC (Orkney Islands Council) Specialist User Recording Environment</skos:scopeNote>
			</skos:Concept>
		</skos:narrower>
		<skos:narrower>
			<skos:Concept rdf:about="http://purl.org/heritagedata/schemes/4/concepts/506421">
				<skos:inScheme rdf:resource="http://purl.org/heritagedata/schemes/4" />
				<dcterms:identifier>http://purl.org/heritagedata/schemes/4/concepts/506421</dcterms:identifier>
				<cc:license rdf:resource="http://reference.data.gov.uk/id/open-government-licence" />
				<cc:attributionURL rdf:resource="http://www.rcahms.gov.uk" />
				<cc:attributionName xml:lang="en">RCAHMS</cc:attributionName>
				<dcterms:publisher rdf:resource="http://www.rcahms.gov.uk" />
				<skos:prefLabel xml:lang="en">GHS PROJECT</skos:prefLabel>
				<dcterms:created rdf:datatype="http://www.w3.org/2001/XMLSchema#dateTime">2012-01-10T16:13:07</dcterms:created>
				<dcterms:modified rdf:datatype="http://www.w3.org/2001/XMLSchema#dateTime">2012-01-10T16:14:20</dcterms:modified>
				<dcterms:issued rdf:datatype="http://www.w3.org/2001/XMLSchema#dateTime">2013-07-17T10:08:40</dcterms:issued>
				<skos:broader rdf:resource="http://purl.org/heritagedata/schemes/4/concepts/502338" />
				<skos:scopeNote xml:lang="en">GHS (The Garden History Society in Scotland) Specialist User Recording Environment</skos:scopeNote>
			</skos:Concept>
		</skos:narrower>
		<skos:narrower>
			<skos:Concept rdf:about="http://purl.org/heritagedata/schemes/4/concepts/505081">
				<skos:inScheme rdf:resource="http://purl.org/heritagedata/schemes/4" />
				<dcterms:identifier>http://purl.org/heritagedata/schemes/4/concepts/505081</dcterms:identifier>
				<cc:license rdf:resource="http://reference.data.gov.uk/id/open-government-licence" />
				<cc:attributionURL rdf:resource="http://www.rcahms.gov.uk" />
				<cc:attributionName xml:lang="en">RCAHMS</cc:attributionName>
				<dcterms:publisher rdf:resource="http://www.rcahms.gov.uk" />
				<skos:prefLabel xml:lang="en">NTS PROJECT</skos:prefLabel>
				<dcterms:created rdf:datatype="http://www.w3.org/2001/XMLSchema#dateTime">2010-07-26T10:57:15</dcterms:created>
				<dcterms:modified rdf:datatype="http://www.w3.org/2001/XMLSchema#dateTime">2010-07-26T10:57:25</dcterms:modified>
				<dcterms:issued rdf:datatype="http://www.w3.org/2001/XMLSchema#dateTime">2013-07-17T10:08:40</dcterms:issued>
				<skos:broader rdf:resource="http://purl.org/heritagedata/schemes/4/concepts/502338" />
				<skos:scopeNote xml:lang="en">NTS (National Trust for Scotland) Specialist User Recording Environment</skos:scopeNote>
			</skos:Concept>
		</skos:narrower>
		<skos:narrower>
			<skos:Concept rdf:about="http://purl.org/heritagedata/schemes/4/concepts/507004">
				<skos:inScheme>
					<skos:ConceptScheme rdf:about="http://purl.org/heritagedata/schemes/4">
						<dcterms:identifier>http://purl.org/heritagedata/schemes/4</dcterms:identifier>
						<cc:license rdf:resource="http://reference.data.gov.uk/id/open-government-licence" />
						<cc:attributionURL rdf:resource="http://www.rcahms.gov.uk" />
						<cc:attributionName xml:lang="en">RCAHMS</cc:attributionName>
						<dcterms:title xml:lang="en">EVENTS (RCAHMS)</dcterms:title>
						<rdfs:label xml:lang="en">EVENTS (RCAHMS)</rdfs:label>
						<dcterms:description xml:lang="en">Events</dcterms:description>
						<dcterms:coverage rdf:resource="http://data.ordnancesurvey.co.uk/id/7000000000041429" />
						<dcterms:created rdf:datatype="http://www.w3.org/2001/XMLSchema#dateTime">2007-05-30T09:15:19</dcterms:created>
						<dcterms:modified rdf:datatype="http://www.w3.org/2001/XMLSchema#dateTime">2008-04-17T10:13:30</dcterms:modified>
						<dcterms:publisher rdf:resource="http://www.rcahms.gov.uk" />
						<dcterms:issued rdf:datatype="http://www.w3.org/2001/XMLSchema#dateTime">2013-07-17T10:08:40</dcterms:issued>
						<skos:hasTopConcept rdf:resource="http://purl.org/heritagedata/schemes/4/concepts/502343" />
						<skos:hasTopConcept rdf:resource="http://purl.org/heritagedata/schemes/4/concepts/502342" />
						<skos:hasTopConcept rdf:resource="http://purl.org/heritagedata/schemes/4/concepts/505721" />
						<skos:hasTopConcept rdf:resource="http://purl.org/heritagedata/schemes/4/concepts/502348" />
						<skos:hasTopConcept rdf:resource="http://purl.org/heritagedata/schemes/4/concepts/502340" />
						<skos:hasTopConcept rdf:resource="http://purl.org/heritagedata/schemes/4/concepts/506330" />
						<skos:hasTopConcept rdf:resource="http://purl.org/heritagedata/schemes/4/concepts/502339" />
						<skos:hasTopConcept rdf:resource="http://purl.org/heritagedata/schemes/4/concepts/502338" />
						<skos:hasTopConcept rdf:resource="http://purl.org/heritagedata/schemes/4/concepts/504000" />
						<skos:hasTopConcept rdf:resource="http://purl.org/heritagedata/schemes/4/concepts/502346" />
						<skos:hasTopConcept rdf:resource="http://purl.org/heritagedata/schemes/4/concepts/502350" />
						<skos:hasTopConcept rdf:resource="http://purl.org/heritagedata/schemes/4/concepts/502349" />
					</skos:ConceptScheme>
				</skos:inScheme>
				<dcterms:identifier>http://purl.org/heritagedata/schemes/4/concepts/507004</dcterms:identifier>
				<cc:license rdf:resource="http://reference.data.gov.uk/id/open-government-licence" />
				<cc:attributionURL rdf:resource="http://www.rcahms.gov.uk" />
				<cc:attributionName xml:lang="en">RCAHMS</cc:attributionName>
				<dcterms:publisher rdf:resource="http://www.rcahms.gov.uk" />
				<skos:prefLabel xml:lang="en">DCC PROJECT</skos:prefLabel>
				<dcterms:created rdf:datatype="http://www.w3.org/2001/XMLSchema#dateTime">2012-08-31T14:47:50</dcterms:created>
				<dcterms:modified rdf:datatype="http://www.w3.org/2001/XMLSchema#dateTime">2012-08-31T14:49:03</dcterms:modified>
				<dcterms:issued rdf:datatype="http://www.w3.org/2001/XMLSchema#dateTime">2013-07-17T10:08:40</dcterms:issued>
				<skos:broader rdf:resource="http://purl.org/heritagedata/schemes/4/concepts/502338" />
				<skos:scopeNote xml:lang="en">DCC (Dundee City Council) Specialist User Recording Environment</skos:scopeNote>
			</skos:Concept>
		</skos:narrower>
		<skos:narrower>
			<skos:Concept rdf:about="http://purl.org/heritagedata/schemes/4/concepts/507005">
				<skos:inScheme rdf:resource="http://purl.org/heritagedata/schemes/4" />
				<dcterms:identifier>http://purl.org/heritagedata/schemes/4/concepts/507005</dcterms:identifier>
				<cc:license rdf:resource="http://reference.data.gov.uk/id/open-government-licence" />
				<cc:attributionURL rdf:resource="http://www.rcahms.gov.uk" />
				<cc:attributionName xml:lang="en">RCAHMS</cc:attributionName>
				<dcterms:publisher rdf:resource="http://www.rcahms.gov.uk" />
				<skos:prefLabel xml:lang="en">EDC PROJECT</skos:prefLabel>
				<dcterms:created rdf:datatype="http://www.w3.org/2001/XMLSchema#dateTime">2012-08-31T14:48:17</dcterms:created>
				<dcterms:modified rdf:datatype="http://www.w3.org/2001/XMLSchema#dateTime">2012-08-31T14:49:47</dcterms:modified>
				<dcterms:issued rdf:datatype="http://www.w3.org/2001/XMLSchema#dateTime">2013-07-17T10:08:40</dcterms:issued>
				<skos:broader rdf:resource="http://purl.org/heritagedata/schemes/4/concepts/502338" />
				<skos:scopeNote xml:lang="en">EDC (East Dunbartonshire Council) Specialist User Recording Environment</skos:scopeNote>
			</skos:Concept>
		</skos:narrower>
		<skos:narrower>
			<skos:Concept rdf:about="http://purl.org/heritagedata/schemes/4/concepts/507064">
				<skos:inScheme rdf:resource="http://purl.org/heritagedata/schemes/4" />
				<dcterms:identifier>http://purl.org/heritagedata/schemes/4/concepts/507064</dcterms:identifier>
				<cc:license rdf:resource="http://reference.data.gov.uk/id/open-government-licence" />
				<cc:attributionURL rdf:resource="http://www.rcahms.gov.uk" />
				<cc:attributionName xml:lang="en">RCAHMS</cc:attributionName>
				<dcterms:publisher rdf:resource="http://www.rcahms.gov.uk" />
				<skos:prefLabel xml:lang="en">TTU PROJECT</skos:prefLabel>
				<dcterms:created rdf:datatype="http://www.w3.org/2001/XMLSchema#dateTime">2012-11-12T15:34:50</dcterms:created>
				<dcterms:modified rdf:datatype="http://www.w3.org/2001/XMLSchema#dateTime">2012-11-12T15:35:10</dcterms:modified>
				<dcterms:issued rdf:datatype="http://www.w3.org/2001/XMLSchema#dateTime">2013-07-17T10:08:40</dcterms:issued>
				<skos:broader rdf:resource="http://purl.org/heritagedata/schemes/4/concepts/502338" />
				<skos:scopeNote xml:lang="en">TTU  (Treasure Trove Unit) Specialist User Recording Environment</skos:scopeNote>
			</skos:Concept>
		</skos:narrower>
		<skos:narrower>
			<skos:Concept rdf:about="http://purl.org/heritagedata/schemes/4/concepts/507065">
				<skos:inScheme rdf:resource="http://purl.org/heritagedata/schemes/4" />
				<dcterms:identifier>http://purl.org/heritagedata/schemes/4/concepts/507065</dcterms:identifier>
				<cc:license rdf:resource="http://reference.data.gov.uk/id/open-government-licence" />
				<cc:attributionURL rdf:resource="http://www.rcahms.gov.uk" />
				<cc:attributionName xml:lang="en">RCAHMS</cc:attributionName>
				<dcterms:publisher rdf:resource="http://www.rcahms.gov.uk" />
				<skos:prefLabel xml:lang="en">SCA PROJECT</skos:prefLabel>
				<dcterms:created rdf:datatype="http://www.w3.org/2001/XMLSchema#dateTime">2012-11-12T15:36:12</dcterms:created>
				<dcterms:modified rdf:datatype="http://www.w3.org/2001/XMLSchema#dateTime">2012-11-12T15:36:51</dcterms:modified>
				<dcterms:issued rdf:datatype="http://www.w3.org/2001/XMLSchema#dateTime">2013-07-17T10:08:40</dcterms:issued>
				<skos:broader rdf:resource="http://purl.org/heritagedata/schemes/4/concepts/502338" />
				<skos:scopeNote xml:lang="en">SCA  (Scottish Canals) Specialist User Recording Environment</skos:scopeNote>
			</skos:Concept>
		</skos:narrower>
		<skos:scopeNote xml:lang="en">A high level grouping  comprising a number of individual but related events relating to one or more archaeological sites or buildings.  A project may relate to fieldwork investigating a particular area or monument type or oblique aerial photography taken over a specific year.  Equally a project may be desk-based, involving the cataloguing of architectural papers.</skos:scopeNote>
	</skos:Concept>
	<skos:Concept rdf:about="http://purl.org/heritagedata/schemes/4/concepts/502458">
		<skos:inScheme rdf:resource="http://purl.org/heritagedata/schemes/4" />
		<dcterms:identifier>http://purl.org/heritagedata/schemes/4/concepts/502458</dcterms:identifier>
		<cc:license rdf:resource="http://reference.data.gov.uk/id/open-government-licence" />
		<cc:attributionURL rdf:resource="http://www.rcahms.gov.uk" />
		<cc:attributionName xml:lang="en">RCAHMS</cc:attributionName>
		<dcterms:publisher rdf:resource="http://www.rcahms.gov.uk" />
		<skos:prefLabel xml:lang="en">OS 50K  LANDRANGER MAPPING</skos:prefLabel>
		<dcterms:created rdf:datatype="http://www.w3.org/2001/XMLSchema#dateTime">2007-06-04T10:40:39</dcterms:created>
		<dcterms:modified rdf:datatype="http://www.w3.org/2001/XMLSchema#dateTime">2007-06-04T10:49:41</dcterms:modified>
		<dcterms:issued rdf:datatype="http://www.w3.org/2001/XMLSchema#dateTime">2013-07-17T10:08:40</dcterms:issued>
		<skos:broader rdf:resource="http://purl.org/heritagedata/schemes/4/concepts/502339" />
		<skos:narrower>
			<skos:Concept rdf:about="http://purl.org/heritagedata/schemes/4/concepts/507262">
				<skos:inScheme rdf:resource="http://purl.org/heritagedata/schemes/4" />
				<dcterms:identifier>http://purl.org/heritagedata/schemes/4/concepts/507262</dcterms:identifier>
				<cc:license rdf:resource="http://reference.data.gov.uk/id/open-government-licence" />
				<cc:attributionURL rdf:resource="http://www.rcahms.gov.uk" />
				<cc:attributionName xml:lang="en">RCAHMS</cc:attributionName>
				<dcterms:publisher rdf:resource="http://www.rcahms.gov.uk" />
				<skos:prefLabel xml:lang="en">OS 50K - NOT REQUESTED</skos:prefLabel>
				<dcterms:created rdf:datatype="http://www.w3.org/2001/XMLSchema#dateTime">2013-01-04T13:05:32</dcterms:created>
				<dcterms:modified rdf:datatype="http://www.w3.org/2001/XMLSchema#dateTime">2013-01-04T13:59:49</dcterms:modified>
				<dcterms:issued rdf:datatype="http://www.w3.org/2001/XMLSchema#dateTime">2013-07-17T10:08:40</dcterms:issued>
				<skos:broader rdf:resource="http://purl.org/heritagedata/schemes/4/concepts/502458" />
				<skos:scopeNote xml:lang="en">Use for noting that an antiquity model, depicted at larger scale (Basic Scale and/or 1:25,000) has not been published at 1:50,000.</skos:scopeNote>
			</skos:Concept>
		</skos:narrower>
		<skos:scopeNote xml:lang="en">Use for information published as part of the Heritage and Antiquities theme on OS 1:50,000 scale mapping / Landranger products.</skos:scopeNote>
	</skos:Concept>
	<skos:Concept rdf:about="http://purl.org/heritagedata/schemes/4/concepts/502459">
		<skos:inScheme rdf:resource="http://purl.org/heritagedata/schemes/4" />
		<dcterms:identifier>http://purl.org/heritagedata/schemes/4/concepts/502459</dcterms:identifier>
		<cc:license rdf:resource="http://reference.data.gov.uk/id/open-government-licence" />
		<cc:attributionURL rdf:resource="http://www.rcahms.gov.uk" />
		<cc:attributionName xml:lang="en">RCAHMS</cc:attributionName>
		<dcterms:publisher rdf:resource="http://www.rcahms.gov.uk" />
		<skos:prefLabel xml:lang="en">OS 25K EXPLORER MAPPING</skos:prefLabel>
		<dcterms:created rdf:datatype="http://www.w3.org/2001/XMLSchema#dateTime">2007-06-04T10:42:24</dcterms:created>
		<dcterms:modified rdf:datatype="http://www.w3.org/2001/XMLSchema#dateTime">2007-06-04T10:43:48</dcterms:modified>
		<dcterms:issued rdf:datatype="http://www.w3.org/2001/XMLSchema#dateTime">2013-07-17T10:08:40</dcterms:issued>
		<skos:broader rdf:resource="http://purl.org/heritagedata/schemes/4/concepts/502339" />
		<skos:narrower>
			<skos:Concept rdf:about="http://purl.org/heritagedata/schemes/4/concepts/507263">
				<skos:inScheme rdf:resource="http://purl.org/heritagedata/schemes/4" />
				<dcterms:identifier>http://purl.org/heritagedata/schemes/4/concepts/507263</dcterms:identifier>
				<cc:license rdf:resource="http://reference.data.gov.uk/id/open-government-licence" />
				<cc:attributionURL rdf:resource="http://www.rcahms.gov.uk" />
				<cc:attributionName xml:lang="en">RCAHMS</cc:attributionName>
				<dcterms:publisher rdf:resource="http://www.rcahms.gov.uk" />
				<skos:prefLabel xml:lang="en">OS 25K - NOT REQUESTED</skos:prefLabel>
				<dcterms:created rdf:datatype="http://www.w3.org/2001/XMLSchema#dateTime">2013-01-04T13:11:25</dcterms:created>
				<dcterms:modified rdf:datatype="http://www.w3.org/2001/XMLSchema#dateTime">2013-01-04T14:00:02</dcterms:modified>
				<dcterms:issued rdf:datatype="http://www.w3.org/2001/XMLSchema#dateTime">2013-07-17T10:08:40</dcterms:issued>
				<skos:broader rdf:resource="http://purl.org/heritagedata/schemes/4/concepts/502459" />
				<skos:scopeNote xml:lang="en">Use for noting that an antiquity model, typically depicted at Basic Scale has not been published at 1:25,000.</skos:scopeNote>
			</skos:Concept>
		</skos:narrower>
		<skos:scopeNote xml:lang="en">Use for information published as part of the Heritage and Antiquities theme on OS 1:25,000 scale mapping / Explorer and related products.</skos:scopeNote>
	</skos:Concept>
	<skos:Concept rdf:about="http://purl.org/heritagedata/schemes/4/concepts/502462">
		<skos:inScheme rdf:resource="http://purl.org/heritagedata/schemes/4" />
		<dcterms:identifier>http://purl.org/heritagedata/schemes/4/concepts/502462</dcterms:identifier>
		<cc:license rdf:resource="http://reference.data.gov.uk/id/open-government-licence" />
		<cc:attributionURL rdf:resource="http://www.rcahms.gov.uk" />
		<cc:attributionName xml:lang="en">RCAHMS</cc:attributionName>
		<dcterms:publisher rdf:resource="http://www.rcahms.gov.uk" />
		<skos:prefLabel xml:lang="en">OS DIGITAL BASIC SCALE MAPPING</skos:prefLabel>
		<dcterms:created rdf:datatype="http://www.w3.org/2001/XMLSchema#dateTime">2007-06-04T10:48:19</dcterms:created>
		<dcterms:modified rdf:datatype="http://www.w3.org/2001/XMLSchema#dateTime">2007-06-04T10:48:59</dcterms:modified>
		<dcterms:issued rdf:datatype="http://www.w3.org/2001/XMLSchema#dateTime">2013-07-17T10:08:40</dcterms:issued>
		<skos:broader rdf:resource="http://purl.org/heritagedata/schemes/4/concepts/502339" />
		<skos:narrower>
			<skos:Concept rdf:about="http://purl.org/heritagedata/schemes/4/concepts/507264">
				<skos:inScheme rdf:resource="http://purl.org/heritagedata/schemes/4" />
				<dcterms:identifier>http://purl.org/heritagedata/schemes/4/concepts/507264</dcterms:identifier>
				<cc:license rdf:resource="http://reference.data.gov.uk/id/open-government-licence" />
				<cc:attributionURL rdf:resource="http://www.rcahms.gov.uk" />
				<cc:attributionName xml:lang="en">RCAHMS</cc:attributionName>
				<dcterms:publisher rdf:resource="http://www.rcahms.gov.uk" />
				<skos:prefLabel xml:lang="en">OS BASIC SCALE NOT REQUESTED</skos:prefLabel>
				<dcterms:created rdf:datatype="http://www.w3.org/2001/XMLSchema#dateTime">2013-01-04T13:13:18</dcterms:created>
				<dcterms:modified rdf:datatype="http://www.w3.org/2001/XMLSchema#dateTime">2013-01-04T13:59:28</dcterms:modified>
				<dcterms:issued rdf:datatype="http://www.w3.org/2001/XMLSchema#dateTime">2013-07-17T10:08:40</dcterms:issued>
				<skos:broader rdf:resource="http://purl.org/heritagedata/schemes/4/concepts/502462" />
				<skos:scopeNote xml:lang="en">Use for noting that an antiquity model, depicted at medium (25k) and/or small scale (50k) has not been previously requested at Basic Scale</skos:scopeNote>
			</skos:Concept>
		</skos:narrower>
		<skos:scopeNote xml:lang="en">Use for information published on OS Basic Scale digital vector mapping.</skos:scopeNote>
	</skos:Concept>
	<skos:Concept rdf:about="http://purl.org/heritagedata/schemes/4/concepts/502473">
		<skos:inScheme rdf:resource="http://purl.org/heritagedata/schemes/4" />
		<dcterms:identifier>http://purl.org/heritagedata/schemes/4/concepts/502473</dcterms:identifier>
		<cc:license rdf:resource="http://reference.data.gov.uk/id/open-government-licence" />
		<cc:attributionURL rdf:resource="http://www.rcahms.gov.uk" />
		<cc:attributionName xml:lang="en">RCAHMS</cc:attributionName>
		<dcterms:publisher rdf:resource="http://www.rcahms.gov.uk" />
		<skos:prefLabel xml:lang="en">REFERENCE</skos:prefLabel>
		<dcterms:created rdf:datatype="http://www.w3.org/2001/XMLSchema#dateTime">2007-06-04T11:25:07</dcterms:created>
		<dcterms:modified rdf:datatype="http://www.w3.org/2001/XMLSchema#dateTime">2009-08-04T15:28:09</dcterms:modified>
		<dcterms:issued rdf:datatype="http://www.w3.org/2001/XMLSchema#dateTime">2013-07-17T10:08:40</dcterms:issued>
		<skos:broader rdf:resource="http://purl.org/heritagedata/schemes/4/concepts/502340" />
		<skos:narrower>
			<skos:Concept rdf:about="http://purl.org/heritagedata/schemes/4/concepts/507042">
				<skos:inScheme rdf:resource="http://purl.org/heritagedata/schemes/4" />
				<dcterms:identifier>http://purl.org/heritagedata/schemes/4/concepts/507042</dcterms:identifier>
				<cc:license rdf:resource="http://reference.data.gov.uk/id/open-government-licence" />
				<cc:attributionURL rdf:resource="http://www.rcahms.gov.uk" />
				<cc:attributionName xml:lang="en">RCAHMS</cc:attributionName>
				<dcterms:publisher rdf:resource="http://www.rcahms.gov.uk" />
				<skos:prefLabel xml:lang="en">SPECIALIST REPORT</skos:prefLabel>
				<dcterms:created rdf:datatype="http://www.w3.org/2001/XMLSchema#dateTime">2012-10-17T10:04:11</dcterms:created>
				<dcterms:modified rdf:datatype="http://www.w3.org/2001/XMLSchema#dateTime">2012-10-17T10:05:18</dcterms:modified>
				<dcterms:issued rdf:datatype="http://www.w3.org/2001/XMLSchema#dateTime">2013-07-17T10:08:40</dcterms:issued>
				<skos:broader rdf:resource="http://purl.org/heritagedata/schemes/4/concepts/502473" />
				<skos:scopeNote xml:lang="en">Information derived from a specialist report (whether published or not) discussing a specific aspect of a site (eg taphonomy) or a particular aspect of the artefact assemblage (eg the pottery or the bone). For general reports, use REFERENCE.</skos:scopeNote>
			</skos:Concept>
		</skos:narrower>
		<skos:scopeNote xml:lang="en">Information derived from documentary sources excluding cartographic products e.g. site descriptions from a number of sources, anything derived from a bibliographic source.</skos:scopeNote>
	</skos:Concept>
	<skos:Concept rdf:about="http://purl.org/heritagedata/schemes/4/concepts/502476">
		<skos:inScheme rdf:resource="http://purl.org/heritagedata/schemes/4" />
		<dcterms:identifier>http://purl.org/heritagedata/schemes/4/concepts/502476</dcterms:identifier>
		<cc:license rdf:resource="http://reference.data.gov.uk/id/open-government-licence" />
		<cc:attributionURL rdf:resource="http://www.rcahms.gov.uk" />
		<cc:attributionName xml:lang="en">RCAHMS</cc:attributionName>
		<dcterms:publisher rdf:resource="http://www.rcahms.gov.uk" />
		<skos:prefLabel xml:lang="en">MARITIME DOCUMENTARY</skos:prefLabel>
		<dcterms:created rdf:datatype="http://www.w3.org/2001/XMLSchema#dateTime">2007-06-04T11:28:35</dcterms:created>
		<dcterms:modified rdf:datatype="http://www.w3.org/2001/XMLSchema#dateTime">2007-06-04T11:29:09</dcterms:modified>
		<dcterms:issued rdf:datatype="http://www.w3.org/2001/XMLSchema#dateTime">2013-07-17T10:08:40</dcterms:issued>
		<skos:broader rdf:resource="http://purl.org/heritagedata/schemes/4/concepts/502340" />
		<skos:narrower>
			<skos:Concept rdf:about="http://purl.org/heritagedata/schemes/4/concepts/502478">
				<skos:inScheme rdf:resource="http://purl.org/heritagedata/schemes/4" />
				<dcterms:identifier>http://purl.org/heritagedata/schemes/4/concepts/502478</dcterms:identifier>
				<cc:license rdf:resource="http://reference.data.gov.uk/id/open-government-licence" />
				<cc:attributionURL rdf:resource="http://www.rcahms.gov.uk" />
				<cc:attributionName xml:lang="en">RCAHMS</cc:attributionName>
				<dcterms:publisher rdf:resource="http://www.rcahms.gov.uk" />
				<skos:prefLabel xml:lang="en">REFIT</skos:prefLabel>
				<dcterms:created rdf:datatype="http://www.w3.org/2001/XMLSchema#dateTime">2007-06-04T11:30:03</dcterms:created>
				<dcterms:modified rdf:datatype="http://www.w3.org/2001/XMLSchema#dateTime">2007-06-04T11:30:52</dcterms:modified>
				<dcterms:issued rdf:datatype="http://www.w3.org/2001/XMLSchema#dateTime">2013-07-17T10:08:40</dcterms:issued>
				<skos:broader rdf:resource="http://purl.org/heritagedata/schemes/4/concepts/502476" />
				<skos:scopeNote xml:lang="en">Documentary references to the act of refitting, or re-rigging, a vessel.</skos:scopeNote>
			</skos:Concept>
		</skos:narrower>
		<skos:narrower>
			<skos:Concept rdf:about="http://purl.org/heritagedata/schemes/4/concepts/502479">
				<skos:inScheme rdf:resource="http://purl.org/heritagedata/schemes/4" />
				<dcterms:identifier>http://purl.org/heritagedata/schemes/4/concepts/502479</dcterms:identifier>
				<cc:license rdf:resource="http://reference.data.gov.uk/id/open-government-licence" />
				<cc:attributionURL rdf:resource="http://www.rcahms.gov.uk" />
				<cc:attributionName xml:lang="en">RCAHMS</cc:attributionName>
				<dcterms:publisher rdf:resource="http://www.rcahms.gov.uk" />
				<skos:prefLabel xml:lang="en">TERTIARY SERVICE</skos:prefLabel>
				<dcterms:created rdf:datatype="http://www.w3.org/2001/XMLSchema#dateTime">2007-06-04T11:31:50</dcterms:created>
				<dcterms:modified rdf:datatype="http://www.w3.org/2001/XMLSchema#dateTime">2007-06-04T11:32:18</dcterms:modified>
				<dcterms:issued rdf:datatype="http://www.w3.org/2001/XMLSchema#dateTime">2013-07-17T10:08:40</dcterms:issued>
				<skos:broader rdf:resource="http://purl.org/heritagedata/schemes/4/concepts/502476" />
				<skos:scopeNote xml:lang="en">The subsequent change of use from a vessel in service, typically for heritage  purposes.  Could include change of name and / or placement in a dry dock or  display context.</skos:scopeNote>
			</skos:Concept>
		</skos:narrower>
		<skos:narrower>
			<skos:Concept rdf:about="http://purl.org/heritagedata/schemes/4/concepts/502480">
				<skos:inScheme rdf:resource="http://purl.org/heritagedata/schemes/4" />
				<dcterms:identifier>http://purl.org/heritagedata/schemes/4/concepts/502480</dcterms:identifier>
				<cc:license rdf:resource="http://reference.data.gov.uk/id/open-government-licence" />
				<cc:attributionURL rdf:resource="http://www.rcahms.gov.uk" />
				<cc:attributionName xml:lang="en">RCAHMS</cc:attributionName>
				<dcterms:publisher rdf:resource="http://www.rcahms.gov.uk" />
				<skos:prefLabel xml:lang="en">SECONDARY SERVICE</skos:prefLabel>
				<dcterms:created rdf:datatype="http://www.w3.org/2001/XMLSchema#dateTime">2007-06-04T11:32:54</dcterms:created>
				<dcterms:modified rdf:datatype="http://www.w3.org/2001/XMLSchema#dateTime">2007-06-04T11:33:09</dcterms:modified>
				<dcterms:issued rdf:datatype="http://www.w3.org/2001/XMLSchema#dateTime">2013-07-17T10:08:40</dcterms:issued>
				<skos:broader rdf:resource="http://purl.org/heritagedata/schemes/4/concepts/502476" />
				<skos:scopeNote xml:lang="en">A subsequent period of use, generally involving conversion and refitting. Possibly involving the change of name.</skos:scopeNote>
			</skos:Concept>
		</skos:narrower>
		<skos:narrower>
			<skos:Concept rdf:about="http://purl.org/heritagedata/schemes/4/concepts/502481">
				<skos:inScheme rdf:resource="http://purl.org/heritagedata/schemes/4" />
				<dcterms:identifier>http://purl.org/heritagedata/schemes/4/concepts/502481</dcterms:identifier>
				<cc:license rdf:resource="http://reference.data.gov.uk/id/open-government-licence" />
				<cc:attributionURL rdf:resource="http://www.rcahms.gov.uk" />
				<cc:attributionName xml:lang="en">RCAHMS</cc:attributionName>
				<dcterms:publisher rdf:resource="http://www.rcahms.gov.uk" />
				<skos:prefLabel xml:lang="en">PRIMARY SERVICE</skos:prefLabel>
				<dcterms:created rdf:datatype="http://www.w3.org/2001/XMLSchema#dateTime">2007-06-04T11:33:34</dcterms:created>
				<dcterms:modified rdf:datatype="http://www.w3.org/2001/XMLSchema#dateTime">2007-06-04T11:34:09</dcterms:modified>
				<dcterms:issued rdf:datatype="http://www.w3.org/2001/XMLSchema#dateTime">2013-07-17T10:08:40</dcterms:issued>
				<skos:broader rdf:resource="http://purl.org/heritagedata/schemes/4/concepts/502476" />
				<skos:scopeNote xml:lang="en">The period of service (or intended period of service)  for which the vessel was originally designed and built for.</skos:scopeNote>
			</skos:Concept>
		</skos:narrower>
		<skos:narrower>
			<skos:Concept rdf:about="http://purl.org/heritagedata/schemes/4/concepts/502482">
				<skos:inScheme rdf:resource="http://purl.org/heritagedata/schemes/4" />
				<dcterms:identifier>http://purl.org/heritagedata/schemes/4/concepts/502482</dcterms:identifier>
				<cc:license rdf:resource="http://reference.data.gov.uk/id/open-government-licence" />
				<cc:attributionURL rdf:resource="http://www.rcahms.gov.uk" />
				<cc:attributionName xml:lang="en">RCAHMS</cc:attributionName>
				<dcterms:publisher rdf:resource="http://www.rcahms.gov.uk" />
				<skos:prefLabel xml:lang="en">NAVIGATIONAL CLEARANCE</skos:prefLabel>
				<dcterms:created rdf:datatype="http://www.w3.org/2001/XMLSchema#dateTime">2007-06-04T11:34:41</dcterms:created>
				<dcterms:modified rdf:datatype="http://www.w3.org/2001/XMLSchema#dateTime">2007-06-04T11:34:52</dcterms:modified>
				<dcterms:issued rdf:datatype="http://www.w3.org/2001/XMLSchema#dateTime">2013-07-17T10:08:40</dcterms:issued>
				<skos:broader rdf:resource="http://purl.org/heritagedata/schemes/4/concepts/502476" />
				<skos:scopeNote xml:lang="en">Removal of masts, funnels and/or superstructure</skos:scopeNote>
			</skos:Concept>
		</skos:narrower>
		<skos:narrower>
			<skos:Concept rdf:about="http://purl.org/heritagedata/schemes/4/concepts/502483">
				<skos:inScheme rdf:resource="http://purl.org/heritagedata/schemes/4" />
				<dcterms:identifier>http://purl.org/heritagedata/schemes/4/concepts/502483</dcterms:identifier>
				<cc:license rdf:resource="http://reference.data.gov.uk/id/open-government-licence" />
				<cc:attributionURL rdf:resource="http://www.rcahms.gov.uk" />
				<cc:attributionName xml:lang="en">RCAHMS</cc:attributionName>
				<dcterms:publisher rdf:resource="http://www.rcahms.gov.uk" />
				<skos:prefLabel xml:lang="en">ENTRY INTO SERVICE</skos:prefLabel>
				<dcterms:created rdf:datatype="http://www.w3.org/2001/XMLSchema#dateTime">2007-06-04T11:35:27</dcterms:created>
				<dcterms:modified rdf:datatype="http://www.w3.org/2001/XMLSchema#dateTime">2007-06-04T11:35:48</dcterms:modified>
				<dcterms:issued rdf:datatype="http://www.w3.org/2001/XMLSchema#dateTime">2013-07-17T10:08:40</dcterms:issued>
				<skos:broader rdf:resource="http://purl.org/heritagedata/schemes/4/concepts/502476" />
				<skos:scopeNote xml:lang="en">Equipment and fittings previously installed and vessel embarks on first, or maiden, voyage.</skos:scopeNote>
			</skos:Concept>
		</skos:narrower>
		<skos:narrower rdf:resource="http://purl.org/heritagedata/schemes/4/concepts/502484" />
		<skos:narrower>
			<skos:Concept rdf:about="http://purl.org/heritagedata/schemes/4/concepts/502490">
				<skos:inScheme rdf:resource="http://purl.org/heritagedata/schemes/4" />
				<dcterms:identifier>http://purl.org/heritagedata/schemes/4/concepts/502490</dcterms:identifier>
				<cc:license rdf:resource="http://reference.data.gov.uk/id/open-government-licence" />
				<cc:attributionURL rdf:resource="http://www.rcahms.gov.uk" />
				<cc:attributionName xml:lang="en">RCAHMS</cc:attributionName>
				<dcterms:publisher rdf:resource="http://www.rcahms.gov.uk" />
				<skos:prefLabel xml:lang="en">RESERVE FLEET LAYING UP</skos:prefLabel>
				<dcterms:created rdf:datatype="http://www.w3.org/2001/XMLSchema#dateTime">2007-06-04T11:44:55</dcterms:created>
				<dcterms:modified rdf:datatype="http://www.w3.org/2001/XMLSchema#dateTime">2007-06-04T11:45:13</dcterms:modified>
				<dcterms:issued rdf:datatype="http://www.w3.org/2001/XMLSchema#dateTime">2013-07-17T10:08:40</dcterms:issued>
				<skos:broader rdf:resource="http://purl.org/heritagedata/schemes/4/concepts/502476" />
				<skos:scopeNote xml:lang="en">Equipment and fittings generally removed, at least in part. Use for warships.</skos:scopeNote>
			</skos:Concept>
		</skos:narrower>
		<skos:narrower>
			<skos:Concept rdf:about="http://purl.org/heritagedata/schemes/4/concepts/502492">
				<skos:inScheme rdf:resource="http://purl.org/heritagedata/schemes/4" />
				<dcterms:identifier>http://purl.org/heritagedata/schemes/4/concepts/502492</dcterms:identifier>
				<cc:license rdf:resource="http://reference.data.gov.uk/id/open-government-licence" />
				<cc:attributionURL rdf:resource="http://www.rcahms.gov.uk" />
				<cc:attributionName xml:lang="en">RCAHMS</cc:attributionName>
				<dcterms:publisher rdf:resource="http://www.rcahms.gov.uk" />
				<skos:prefLabel xml:lang="en">ENVIRONMENTAL CLEANSING</skos:prefLabel>
				<dcterms:created rdf:datatype="http://www.w3.org/2001/XMLSchema#dateTime">2007-06-04T11:47:41</dcterms:created>
				<dcterms:modified rdf:datatype="http://www.w3.org/2001/XMLSchema#dateTime">2007-06-04T11:48:12</dcterms:modified>
				<dcterms:issued rdf:datatype="http://www.w3.org/2001/XMLSchema#dateTime">2013-07-17T10:08:40</dcterms:issued>
				<skos:broader rdf:resource="http://purl.org/heritagedata/schemes/4/concepts/502476" />
				<skos:scopeNote xml:lang="en">The removal of fuel oil and/ or dangerous cargo</skos:scopeNote>
			</skos:Concept>
		</skos:narrower>
		<skos:narrower rdf:resource="http://purl.org/heritagedata/schemes/4/concepts/502493" />
		<skos:narrower>
			<skos:Concept rdf:about="http://purl.org/heritagedata/schemes/4/concepts/502495">
				<skos:inScheme rdf:resource="http://purl.org/heritagedata/schemes/4" />
				<dcterms:identifier>http://purl.org/heritagedata/schemes/4/concepts/502495</dcterms:identifier>
				<cc:license rdf:resource="http://reference.data.gov.uk/id/open-government-licence" />
				<cc:attributionURL rdf:resource="http://www.rcahms.gov.uk" />
				<cc:attributionName xml:lang="en">RCAHMS</cc:attributionName>
				<dcterms:publisher rdf:resource="http://www.rcahms.gov.uk" />
				<skos:prefLabel xml:lang="en">BATTLE</skos:prefLabel>
				<dcterms:created rdf:datatype="http://www.w3.org/2001/XMLSchema#dateTime">2007-06-04T11:53:20</dcterms:created>
				<dcterms:modified rdf:datatype="http://www.w3.org/2001/XMLSchema#dateTime">2007-06-05T13:56:15</dcterms:modified>
				<dcterms:issued rdf:datatype="http://www.w3.org/2001/XMLSchema#dateTime">2013-07-17T10:08:40</dcterms:issued>
				<skos:broader rdf:resource="http://purl.org/heritagedata/schemes/4/concepts/502476" />
				<skos:scopeNote xml:lang="en">The date of a battle a vessel has been involved in.</skos:scopeNote>
			</skos:Concept>
		</skos:narrower>
		<skos:narrower>
			<skos:Concept rdf:about="http://purl.org/heritagedata/schemes/4/concepts/502516">
				<skos:inScheme rdf:resource="http://purl.org/heritagedata/schemes/4" />
				<dcterms:identifier>http://purl.org/heritagedata/schemes/4/concepts/502516</dcterms:identifier>
				<cc:license rdf:resource="http://reference.data.gov.uk/id/open-government-licence" />
				<cc:attributionURL rdf:resource="http://www.rcahms.gov.uk" />
				<cc:attributionName xml:lang="en">RCAHMS</cc:attributionName>
				<dcterms:publisher rdf:resource="http://www.rcahms.gov.uk" />
				<skos:prefLabel xml:lang="en">SCRAPPING</skos:prefLabel>
				<dcterms:created rdf:datatype="http://www.w3.org/2001/XMLSchema#dateTime">2007-06-04T14:21:44</dcterms:created>
				<dcterms:modified rdf:datatype="http://www.w3.org/2001/XMLSchema#dateTime">2007-06-04T14:22:31</dcterms:modified>
				<dcterms:issued rdf:datatype="http://www.w3.org/2001/XMLSchema#dateTime">2013-07-17T10:08:40</dcterms:issued>
				<skos:broader rdf:resource="http://purl.org/heritagedata/schemes/4/concepts/502476" />
				<skos:scopeNote xml:lang="en">The act of scrapping a vessel.</skos:scopeNote>
			</skos:Concept>
		</skos:narrower>
		<skos:narrower>
			<skos:Concept rdf:about="http://purl.org/heritagedata/schemes/4/concepts/502517">
				<skos:inScheme rdf:resource="http://purl.org/heritagedata/schemes/4" />
				<dcterms:identifier>http://purl.org/heritagedata/schemes/4/concepts/502517</dcterms:identifier>
				<cc:license rdf:resource="http://reference.data.gov.uk/id/open-government-licence" />
				<cc:attributionURL rdf:resource="http://www.rcahms.gov.uk" />
				<cc:attributionName xml:lang="en">RCAHMS</cc:attributionName>
				<dcterms:publisher rdf:resource="http://www.rcahms.gov.uk" />
				<skos:prefLabel xml:lang="en">FINAL COLLAPSE</skos:prefLabel>
				<dcterms:created rdf:datatype="http://www.w3.org/2001/XMLSchema#dateTime">2007-06-04T14:23:06</dcterms:created>
				<dcterms:modified rdf:datatype="http://www.w3.org/2001/XMLSchema#dateTime">2007-06-05T11:23:47</dcterms:modified>
				<dcterms:issued rdf:datatype="http://www.w3.org/2001/XMLSchema#dateTime">2013-07-17T10:08:40</dcterms:issued>
				<skos:broader rdf:resource="http://purl.org/heritagedata/schemes/4/concepts/502476" />
				<skos:scopeNote xml:lang="en">Observations that  the structure of a maritime object has disintegrated beyond recognition.  To be used in conjunction with an underwater archaeology recording event where possible.</skos:scopeNote>
			</skos:Concept>
		</skos:narrower>
		<skos:narrower>
			<skos:Concept rdf:about="http://purl.org/heritagedata/schemes/4/concepts/503418">
				<skos:inScheme rdf:resource="http://purl.org/heritagedata/schemes/4" />
				<dcterms:identifier>http://purl.org/heritagedata/schemes/4/concepts/503418</dcterms:identifier>
				<cc:license rdf:resource="http://reference.data.gov.uk/id/open-government-licence" />
				<cc:attributionURL rdf:resource="http://www.rcahms.gov.uk" />
				<cc:attributionName xml:lang="en">RCAHMS</cc:attributionName>
				<dcterms:publisher rdf:resource="http://www.rcahms.gov.uk" />
				<skos:prefLabel xml:lang="en">VESSEL CONSTRUCTION</skos:prefLabel>
				<dcterms:created rdf:datatype="http://www.w3.org/2001/XMLSchema#dateTime">2008-07-17T11:17:25</dcterms:created>
				<dcterms:modified rdf:datatype="http://www.w3.org/2001/XMLSchema#dateTime">2008-10-20T11:05:53</dcterms:modified>
				<dcterms:issued rdf:datatype="http://www.w3.org/2001/XMLSchema#dateTime">2013-07-17T10:08:40</dcterms:issued>
				<skos:broader rdf:resource="http://purl.org/heritagedata/schemes/4/concepts/502476" />
				<skos:scopeNote xml:lang="en">The date a vessel was built.</skos:scopeNote>
			</skos:Concept>
		</skos:narrower>
		<skos:narrower>
			<skos:Concept rdf:about="http://purl.org/heritagedata/schemes/4/concepts/505821">
				<skos:inScheme rdf:resource="http://purl.org/heritagedata/schemes/4" />
				<dcterms:identifier>http://purl.org/heritagedata/schemes/4/concepts/505821</dcterms:identifier>
				<cc:license rdf:resource="http://reference.data.gov.uk/id/open-government-licence" />
				<cc:attributionURL rdf:resource="http://www.rcahms.gov.uk" />
				<cc:attributionName xml:lang="en">RCAHMS</cc:attributionName>
				<dcterms:publisher rdf:resource="http://www.rcahms.gov.uk" />
				<skos:prefLabel xml:lang="en">NAMED LOCATION (NLO)</skos:prefLabel>
				<dcterms:created rdf:datatype="http://www.w3.org/2001/XMLSchema#dateTime">2011-05-18T14:54:53</dcterms:created>
				<dcterms:modified rdf:datatype="http://www.w3.org/2001/XMLSchema#dateTime">2011-05-18T15:11:24</dcterms:modified>
				<dcterms:issued rdf:datatype="http://www.w3.org/2001/XMLSchema#dateTime">2013-07-17T10:08:40</dcterms:issued>
				<skos:broader rdf:resource="http://purl.org/heritagedata/schemes/4/concepts/502476" />
				<skos:scopeNote xml:lang="en">The centre of a diffuse geographical area which has the potential to include many wrecks and downed aircraft as suggested by repeated references to the area within documentary sources. Use for MARITIME sites only.</skos:scopeNote>
			</skos:Concept>
		</skos:narrower>
		<skos:scopeNote xml:lang="en">Documentary events associated with maritime archaeology</skos:scopeNote>
	</skos:Concept>
	<skos:Concept rdf:about="http://purl.org/heritagedata/schemes/4/concepts/502484">
		<skos:inScheme rdf:resource="http://purl.org/heritagedata/schemes/4" />
		<dcterms:identifier>http://purl.org/heritagedata/schemes/4/concepts/502484</dcterms:identifier>
		<cc:license rdf:resource="http://reference.data.gov.uk/id/open-government-licence" />
		<cc:attributionURL rdf:resource="http://www.rcahms.gov.uk" />
		<cc:attributionName xml:lang="en">RCAHMS</cc:attributionName>
		<dcterms:publisher rdf:resource="http://www.rcahms.gov.uk" />
		<skos:prefLabel xml:lang="en">LOSS</skos:prefLabel>
		<dcterms:created rdf:datatype="http://www.w3.org/2001/XMLSchema#dateTime">2007-06-04T11:36:16</dcterms:created>
		<dcterms:modified rdf:datatype="http://www.w3.org/2001/XMLSchema#dateTime">2007-06-05T11:24:11</dcterms:modified>
		<dcterms:issued rdf:datatype="http://www.w3.org/2001/XMLSchema#dateTime">2013-07-17T10:08:40</dcterms:issued>
		<skos:broader rdf:resource="http://purl.org/heritagedata/schemes/4/concepts/502476" />
		<skos:narrower rdf:resource="http://purl.org/heritagedata/schemes/4/concepts/502485" />
		<skos:narrower rdf:resource="http://purl.org/heritagedata/schemes/4/concepts/502486" />
		<skos:narrower>
			<skos:Concept rdf:about="http://purl.org/heritagedata/schemes/4/concepts/502487">
				<skos:inScheme rdf:resource="http://purl.org/heritagedata/schemes/4" />
				<dcterms:identifier>http://purl.org/heritagedata/schemes/4/concepts/502487</dcterms:identifier>
				<cc:license rdf:resource="http://reference.data.gov.uk/id/open-government-licence" />
				<cc:attributionURL rdf:resource="http://www.rcahms.gov.uk" />
				<cc:attributionName xml:lang="en">RCAHMS</cc:attributionName>
				<dcterms:publisher rdf:resource="http://www.rcahms.gov.uk" />
				<skos:prefLabel xml:lang="en">FOUNDERING</skos:prefLabel>
				<dcterms:created rdf:datatype="http://www.w3.org/2001/XMLSchema#dateTime">2007-06-04T11:42:11</dcterms:created>
				<dcterms:modified rdf:datatype="http://www.w3.org/2001/XMLSchema#dateTime">2007-06-04T11:42:50</dcterms:modified>
				<dcterms:issued rdf:datatype="http://www.w3.org/2001/XMLSchema#dateTime">2013-07-17T10:08:40</dcterms:issued>
				<skos:broader rdf:resource="http://purl.org/heritagedata/schemes/4/concepts/502484" />
				<skos:scopeNote xml:lang="en">The date and nature of loss for a particular vessel sunk at sea.</skos:scopeNote>
			</skos:Concept>
		</skos:narrower>
		<skos:narrower rdf:resource="http://purl.org/heritagedata/schemes/4/concepts/502488" />
		<skos:narrower rdf:resource="http://purl.org/heritagedata/schemes/4/concepts/502489" />
		<skos:narrower>
			<skos:Concept rdf:about="http://purl.org/heritagedata/schemes/4/concepts/502491">
				<skos:inScheme rdf:resource="http://purl.org/heritagedata/schemes/4" />
				<dcterms:identifier>http://purl.org/heritagedata/schemes/4/concepts/502491</dcterms:identifier>
				<cc:license rdf:resource="http://reference.data.gov.uk/id/open-government-licence" />
				<cc:attributionURL rdf:resource="http://www.rcahms.gov.uk" />
				<cc:attributionName xml:lang="en">RCAHMS</cc:attributionName>
				<dcterms:publisher rdf:resource="http://www.rcahms.gov.uk" />
				<skos:prefLabel xml:lang="en">IN ORDINARY LAYING UP</skos:prefLabel>
				<dcterms:created rdf:datatype="http://www.w3.org/2001/XMLSchema#dateTime">2007-06-04T11:46:58</dcterms:created>
				<dcterms:modified rdf:datatype="http://www.w3.org/2001/XMLSchema#dateTime">2007-06-04T11:47:15</dcterms:modified>
				<dcterms:issued rdf:datatype="http://www.w3.org/2001/XMLSchema#dateTime">2013-07-17T10:08:40</dcterms:issued>
				<skos:broader rdf:resource="http://purl.org/heritagedata/schemes/4/concepts/502484" />
				<skos:scopeNote xml:lang="en">Equipment and fittings generally removed, at least in part. Use for merchant ships</skos:scopeNote>
			</skos:Concept>
		</skos:narrower>
		<skos:narrower>
			<skos:Concept rdf:about="http://purl.org/heritagedata/schemes/4/concepts/502496">
				<skos:inScheme rdf:resource="http://purl.org/heritagedata/schemes/4" />
				<dcterms:identifier>http://purl.org/heritagedata/schemes/4/concepts/502496</dcterms:identifier>
				<cc:license rdf:resource="http://reference.data.gov.uk/id/open-government-licence" />
				<cc:attributionURL rdf:resource="http://www.rcahms.gov.uk" />
				<cc:attributionName xml:lang="en">RCAHMS</cc:attributionName>
				<dcterms:publisher rdf:resource="http://www.rcahms.gov.uk" />
				<skos:prefLabel xml:lang="en">ABANDONMENT</skos:prefLabel>
				<dcterms:created rdf:datatype="http://www.w3.org/2001/XMLSchema#dateTime">2007-06-04T11:54:05</dcterms:created>
				<dcterms:modified rdf:datatype="http://www.w3.org/2001/XMLSchema#dateTime">2007-06-05T10:29:59</dcterms:modified>
				<dcterms:issued rdf:datatype="http://www.w3.org/2001/XMLSchema#dateTime">2013-07-17T10:08:40</dcterms:issued>
				<skos:broader rdf:resource="http://purl.org/heritagedata/schemes/4/concepts/502484" />
				<skos:scopeNote xml:lang="en">The date a vessel is abandoned, typically inter-tidal on 'mud-berth' and without contents.</skos:scopeNote>
			</skos:Concept>
		</skos:narrower>
		<skos:scopeNote xml:lang="en">The destruction of a vessel through  accidental or deliberate action.</skos:scopeNote>
	</skos:Concept>
	<skos:Concept rdf:about="http://purl.org/heritagedata/schemes/4/concepts/502485">
		<skos:inScheme rdf:resource="http://purl.org/heritagedata/schemes/4" />
		<dcterms:identifier>http://purl.org/heritagedata/schemes/4/concepts/502485</dcterms:identifier>
		<cc:license rdf:resource="http://reference.data.gov.uk/id/open-government-licence" />
		<cc:attributionURL rdf:resource="http://www.rcahms.gov.uk" />
		<cc:attributionName xml:lang="en">RCAHMS</cc:attributionName>
		<dcterms:publisher rdf:resource="http://www.rcahms.gov.uk" />
		<skos:prefLabel xml:lang="en">WAR DAMAGE</skos:prefLabel>
		<dcterms:created rdf:datatype="http://www.w3.org/2001/XMLSchema#dateTime">2007-06-04T11:38:48</dcterms:created>
		<dcterms:modified rdf:datatype="http://www.w3.org/2001/XMLSchema#dateTime">2007-06-05T11:23:14</dcterms:modified>
		<dcterms:issued rdf:datatype="http://www.w3.org/2001/XMLSchema#dateTime">2013-07-17T10:08:40</dcterms:issued>
		<skos:broader rdf:resource="http://purl.org/heritagedata/schemes/4/concepts/502484" />
		<skos:broader rdf:resource="http://purl.org/heritagedata/schemes/4/concepts/502493" />
		<skos:scopeNote xml:lang="en">The date and nature of damage or loss for a particular vessel through military action.</skos:scopeNote>
	</skos:Concept>
	<skos:Concept rdf:about="http://purl.org/heritagedata/schemes/4/concepts/502486">
		<skos:inScheme rdf:resource="http://purl.org/heritagedata/schemes/4" />
		<dcterms:identifier>http://purl.org/heritagedata/schemes/4/concepts/502486</dcterms:identifier>
		<cc:license rdf:resource="http://reference.data.gov.uk/id/open-government-licence" />
		<cc:attributionURL rdf:resource="http://www.rcahms.gov.uk" />
		<cc:attributionName xml:lang="en">RCAHMS</cc:attributionName>
		<dcterms:publisher rdf:resource="http://www.rcahms.gov.uk" />
		<skos:prefLabel xml:lang="en">STRANDING</skos:prefLabel>
		<dcterms:created rdf:datatype="http://www.w3.org/2001/XMLSchema#dateTime">2007-06-04T11:40:13</dcterms:created>
		<dcterms:modified rdf:datatype="http://www.w3.org/2001/XMLSchema#dateTime">2007-06-04T11:53:08</dcterms:modified>
		<dcterms:issued rdf:datatype="http://www.w3.org/2001/XMLSchema#dateTime">2013-07-17T10:08:40</dcterms:issued>
		<skos:broader rdf:resource="http://purl.org/heritagedata/schemes/4/concepts/502484" />
		<skos:broader rdf:resource="http://purl.org/heritagedata/schemes/4/concepts/502493" />
		<skos:scopeNote xml:lang="en">The date and nature of damage or loss for a particular vessel being driven or run ashore.</skos:scopeNote>
	</skos:Concept>
	<skos:Concept rdf:about="http://purl.org/heritagedata/schemes/4/concepts/502488">
		<skos:inScheme rdf:resource="http://purl.org/heritagedata/schemes/4" />
		<dcterms:identifier>http://purl.org/heritagedata/schemes/4/concepts/502488</dcterms:identifier>
		<cc:license rdf:resource="http://reference.data.gov.uk/id/open-government-licence" />
		<cc:attributionURL rdf:resource="http://www.rcahms.gov.uk" />
		<cc:attributionName xml:lang="en">RCAHMS</cc:attributionName>
		<dcterms:publisher rdf:resource="http://www.rcahms.gov.uk" />
		<skos:prefLabel xml:lang="en">FIRE</skos:prefLabel>
		<dcterms:created rdf:datatype="http://www.w3.org/2001/XMLSchema#dateTime">2007-06-04T11:43:19</dcterms:created>
		<dcterms:modified rdf:datatype="http://www.w3.org/2001/XMLSchema#dateTime">2007-06-04T11:51:25</dcterms:modified>
		<dcterms:issued rdf:datatype="http://www.w3.org/2001/XMLSchema#dateTime">2013-07-17T10:08:40</dcterms:issued>
		<skos:broader rdf:resource="http://purl.org/heritagedata/schemes/4/concepts/502484" />
		<skos:broader rdf:resource="http://purl.org/heritagedata/schemes/4/concepts/502493" />
		<skos:scopeNote xml:lang="en">The date and nature of damage or loss for a particular vessel  through fire.</skos:scopeNote>
	</skos:Concept>
	<skos:Concept rdf:about="http://purl.org/heritagedata/schemes/4/concepts/502489">
		<skos:inScheme rdf:resource="http://purl.org/heritagedata/schemes/4" />
		<dcterms:identifier>http://purl.org/heritagedata/schemes/4/concepts/502489</dcterms:identifier>
		<cc:license rdf:resource="http://reference.data.gov.uk/id/open-government-licence" />
		<cc:attributionURL rdf:resource="http://www.rcahms.gov.uk" />
		<cc:attributionName xml:lang="en">RCAHMS</cc:attributionName>
		<dcterms:publisher rdf:resource="http://www.rcahms.gov.uk" />
		<skos:prefLabel xml:lang="en">COLLISION</skos:prefLabel>
		<dcterms:created rdf:datatype="http://www.w3.org/2001/XMLSchema#dateTime">2007-06-04T11:44:01</dcterms:created>
		<dcterms:modified rdf:datatype="http://www.w3.org/2001/XMLSchema#dateTime">2007-06-04T11:51:57</dcterms:modified>
		<dcterms:issued rdf:datatype="http://www.w3.org/2001/XMLSchema#dateTime">2013-07-17T10:08:40</dcterms:issued>
		<skos:broader rdf:resource="http://purl.org/heritagedata/schemes/4/concepts/502484" />
		<skos:broader rdf:resource="http://purl.org/heritagedata/schemes/4/concepts/502493" />
		<skos:scopeNote xml:lang="en">The date and nature of damage or loss for a particular vessel through collision with another vessel.</skos:scopeNote>
	</skos:Concept>
	<skos:Concept rdf:about="http://purl.org/heritagedata/schemes/4/concepts/502493">
		<skos:inScheme rdf:resource="http://purl.org/heritagedata/schemes/4" />
		<dcterms:identifier>http://purl.org/heritagedata/schemes/4/concepts/502493</dcterms:identifier>
		<cc:license rdf:resource="http://reference.data.gov.uk/id/open-government-licence" />
		<cc:attributionURL rdf:resource="http://www.rcahms.gov.uk" />
		<cc:attributionName xml:lang="en">RCAHMS</cc:attributionName>
		<dcterms:publisher rdf:resource="http://www.rcahms.gov.uk" />
		<skos:prefLabel xml:lang="en">DAMAGE</skos:prefLabel>
		<dcterms:created rdf:datatype="http://www.w3.org/2001/XMLSchema#dateTime">2007-06-04T11:48:33</dcterms:created>
		<dcterms:modified rdf:datatype="http://www.w3.org/2001/XMLSchema#dateTime">2007-06-04T11:50:10</dcterms:modified>
		<dcterms:issued rdf:datatype="http://www.w3.org/2001/XMLSchema#dateTime">2013-07-17T10:08:40</dcterms:issued>
		<skos:broader rdf:resource="http://purl.org/heritagedata/schemes/4/concepts/502476" />
		<skos:narrower rdf:resource="http://purl.org/heritagedata/schemes/4/concepts/502488" />
		<skos:narrower rdf:resource="http://purl.org/heritagedata/schemes/4/concepts/502489" />
		<skos:narrower rdf:resource="http://purl.org/heritagedata/schemes/4/concepts/502485" />
		<skos:narrower rdf:resource="http://purl.org/heritagedata/schemes/4/concepts/502486" />
		<skos:scopeNote xml:lang="en">The temporary impairment of a vessel through accidental or activity.</skos:scopeNote>
	</skos:Concept>
	<skos:Concept rdf:about="http://purl.org/heritagedata/schemes/4/concepts/502513">
		<skos:inScheme rdf:resource="http://purl.org/heritagedata/schemes/4" />
		<dcterms:identifier>http://purl.org/heritagedata/schemes/4/concepts/502513</dcterms:identifier>
		<cc:license rdf:resource="http://reference.data.gov.uk/id/open-government-licence" />
		<cc:attributionURL rdf:resource="http://www.rcahms.gov.uk" />
		<cc:attributionName xml:lang="en">RCAHMS</cc:attributionName>
		<dcterms:publisher rdf:resource="http://www.rcahms.gov.uk" />
		<skos:prefLabel xml:lang="en">DESIGN</skos:prefLabel>
		<dcterms:created rdf:datatype="http://www.w3.org/2001/XMLSchema#dateTime">2007-06-04T14:18:59</dcterms:created>
		<dcterms:modified rdf:datatype="http://www.w3.org/2001/XMLSchema#dateTime">2007-06-04T14:19:21</dcterms:modified>
		<dcterms:issued rdf:datatype="http://www.w3.org/2001/XMLSchema#dateTime">2013-07-17T10:08:40</dcterms:issued>
		<skos:broader rdf:resource="http://purl.org/heritagedata/schemes/4/concepts/502534" />
		<skos:narrower>
			<skos:Concept rdf:about="http://purl.org/heritagedata/schemes/4/concepts/502528">
				<skos:inScheme rdf:resource="http://purl.org/heritagedata/schemes/4" />
				<dcterms:identifier>http://purl.org/heritagedata/schemes/4/concepts/502528</dcterms:identifier>
				<cc:license rdf:resource="http://reference.data.gov.uk/id/open-government-licence" />
				<cc:attributionURL rdf:resource="http://www.rcahms.gov.uk" />
				<cc:attributionName xml:lang="en">RCAHMS</cc:attributionName>
				<dcterms:publisher rdf:resource="http://www.rcahms.gov.uk" />
				<skos:prefLabel xml:lang="en">UNEXECUTED</skos:prefLabel>
				<dcterms:created rdf:datatype="http://www.w3.org/2001/XMLSchema#dateTime">2007-06-04T14:36:59</dcterms:created>
				<dcterms:modified rdf:datatype="http://www.w3.org/2001/XMLSchema#dateTime">2007-10-08T16:22:19</dcterms:modified>
				<dcterms:issued rdf:datatype="http://www.w3.org/2001/XMLSchema#dateTime">2013-07-17T10:08:40</dcterms:issued>
				<skos:broader rdf:resource="http://purl.org/heritagedata/schemes/4/concepts/502513" />
				<skos:scopeNote xml:lang="en">Documentation submitted as part of an unsuccessful competition entry, and other unexecuted designs for a building.</skos:scopeNote>
			</skos:Concept>
		</skos:narrower>
		<skos:scopeNote xml:lang="en">Documentation, including plans, drawn up for the construction of a building.</skos:scopeNote>
	</skos:Concept>
	<skos:Concept rdf:about="http://purl.org/heritagedata/schemes/4/concepts/502515">
		<skos:inScheme rdf:resource="http://purl.org/heritagedata/schemes/4" />
		<dcterms:identifier>http://purl.org/heritagedata/schemes/4/concepts/502515</dcterms:identifier>
		<cc:license rdf:resource="http://reference.data.gov.uk/id/open-government-licence" />
		<cc:attributionURL rdf:resource="http://www.rcahms.gov.uk" />
		<cc:attributionName xml:lang="en">RCAHMS</cc:attributionName>
		<dcterms:publisher rdf:resource="http://www.rcahms.gov.uk" />
		<skos:prefLabel xml:lang="en">INCIDENT</skos:prefLabel>
		<dcterms:created rdf:datatype="http://www.w3.org/2001/XMLSchema#dateTime">2007-06-04T14:21:06</dcterms:created>
		<dcterms:modified rdf:datatype="http://www.w3.org/2001/XMLSchema#dateTime">2007-06-04T14:21:26</dcterms:modified>
		<dcterms:issued rdf:datatype="http://www.w3.org/2001/XMLSchema#dateTime">2013-07-17T10:08:40</dcterms:issued>
		<skos:broader rdf:resource="http://purl.org/heritagedata/schemes/4/concepts/502533" />
		<skos:narrower>
			<skos:Concept rdf:about="http://purl.org/heritagedata/schemes/4/concepts/506328">
				<skos:inScheme rdf:resource="http://purl.org/heritagedata/schemes/4" />
				<dcterms:identifier>http://purl.org/heritagedata/schemes/4/concepts/506328</dcterms:identifier>
				<cc:license rdf:resource="http://reference.data.gov.uk/id/open-government-licence" />
				<cc:attributionURL rdf:resource="http://www.rcahms.gov.uk" />
				<cc:attributionName xml:lang="en">RCAHMS</cc:attributionName>
				<dcterms:publisher rdf:resource="http://www.rcahms.gov.uk" />
				<skos:prefLabel xml:lang="en">FIRE DAMAGE</skos:prefLabel>
				<dcterms:created rdf:datatype="http://www.w3.org/2001/XMLSchema#dateTime">2011-12-13T14:07:18</dcterms:created>
				<dcterms:modified rdf:datatype="http://www.w3.org/2001/XMLSchema#dateTime">2011-12-13T14:07:22</dcterms:modified>
				<dcterms:issued rdf:datatype="http://www.w3.org/2001/XMLSchema#dateTime">2013-07-17T10:08:40</dcterms:issued>
				<skos:broader rdf:resource="http://purl.org/heritagedata/schemes/4/concepts/502515" />
				<skos:scopeNote xml:lang="en">FIRE DAMAGE</skos:scopeNote>
			</skos:Concept>
		</skos:narrower>
		<skos:narrower>
			<skos:Concept rdf:about="http://purl.org/heritagedata/schemes/4/concepts/506329">
				<skos:inScheme rdf:resource="http://purl.org/heritagedata/schemes/4" />
				<dcterms:identifier>http://purl.org/heritagedata/schemes/4/concepts/506329</dcterms:identifier>
				<cc:license rdf:resource="http://reference.data.gov.uk/id/open-government-licence" />
				<cc:attributionURL rdf:resource="http://www.rcahms.gov.uk" />
				<cc:attributionName xml:lang="en">RCAHMS</cc:attributionName>
				<dcterms:publisher rdf:resource="http://www.rcahms.gov.uk" />
				<skos:prefLabel xml:lang="en">FLOOD DAMAGE</skos:prefLabel>
				<dcterms:created rdf:datatype="http://www.w3.org/2001/XMLSchema#dateTime">2011-12-13T14:07:49</dcterms:created>
				<dcterms:modified rdf:datatype="http://www.w3.org/2001/XMLSchema#dateTime">2011-12-13T14:07:53</dcterms:modified>
				<dcterms:issued rdf:datatype="http://www.w3.org/2001/XMLSchema#dateTime">2013-07-17T10:08:40</dcterms:issued>
				<skos:broader rdf:resource="http://purl.org/heritagedata/schemes/4/concepts/502515" />
				<skos:scopeNote xml:lang="en">FLOOD DAMAGE</skos:scopeNote>
			</skos:Concept>
		</skos:narrower>
		<skos:scopeNote xml:lang="en">Damage caused to a building through either human or natural causes:. e.g. fire or flood.</skos:scopeNote>
	</skos:Concept>
	<skos:Concept rdf:about="http://purl.org/heritagedata/schemes/4/concepts/502527">
		<skos:inScheme rdf:resource="http://purl.org/heritagedata/schemes/4" />
		<dcterms:identifier>http://purl.org/heritagedata/schemes/4/concepts/502527</dcterms:identifier>
		<cc:license rdf:resource="http://reference.data.gov.uk/id/open-government-licence" />
		<cc:attributionURL rdf:resource="http://www.rcahms.gov.uk" />
		<cc:attributionName xml:lang="en">RCAHMS</cc:attributionName>
		<dcterms:publisher rdf:resource="http://www.rcahms.gov.uk" />
		<skos:prefLabel xml:lang="en">CONSERVATION</skos:prefLabel>
		<dcterms:created rdf:datatype="http://www.w3.org/2001/XMLSchema#dateTime">2007-06-04T14:36:23</dcterms:created>
		<dcterms:modified rdf:datatype="http://www.w3.org/2001/XMLSchema#dateTime">2007-06-05T13:41:39</dcterms:modified>
		<dcterms:issued rdf:datatype="http://www.w3.org/2001/XMLSchema#dateTime">2013-07-17T10:08:40</dcterms:issued>
		<skos:broader rdf:resource="http://purl.org/heritagedata/schemes/4/concepts/502535" />
		<skos:narrower>
			<skos:Concept rdf:about="http://purl.org/heritagedata/schemes/4/concepts/506327">
				<skos:inScheme rdf:resource="http://purl.org/heritagedata/schemes/4" />
				<dcterms:identifier>http://purl.org/heritagedata/schemes/4/concepts/506327</dcterms:identifier>
				<cc:license rdf:resource="http://reference.data.gov.uk/id/open-government-licence" />
				<cc:attributionURL rdf:resource="http://www.rcahms.gov.uk" />
				<cc:attributionName xml:lang="en">RCAHMS</cc:attributionName>
				<dcterms:publisher rdf:resource="http://www.rcahms.gov.uk" />
				<skos:prefLabel xml:lang="en">GRANT AID</skos:prefLabel>
				<dcterms:created rdf:datatype="http://www.w3.org/2001/XMLSchema#dateTime">2011-12-13T14:05:39</dcterms:created>
				<dcterms:modified rdf:datatype="http://www.w3.org/2001/XMLSchema#dateTime">2011-12-13T14:05:43</dcterms:modified>
				<dcterms:issued rdf:datatype="http://www.w3.org/2001/XMLSchema#dateTime">2013-07-17T10:08:40</dcterms:issued>
				<skos:broader rdf:resource="http://purl.org/heritagedata/schemes/4/concepts/502527" />
				<skos:scopeNote xml:lang="en">GRANT AID</skos:scopeNote>
			</skos:Concept>
		</skos:narrower>
		<skos:scopeNote xml:lang="en">Date when conservation work is carried for preservation purposes.</skos:scopeNote>
	</skos:Concept>
	<skos:Concept rdf:about="http://purl.org/heritagedata/schemes/4/concepts/502534">
		<skos:inScheme rdf:resource="http://purl.org/heritagedata/schemes/4" />
		<dcterms:identifier>http://purl.org/heritagedata/schemes/4/concepts/502534</dcterms:identifier>
		<cc:license rdf:resource="http://reference.data.gov.uk/id/open-government-licence" />
		<cc:attributionURL rdf:resource="http://www.rcahms.gov.uk" />
		<cc:attributionName xml:lang="en">RCAHMS</cc:attributionName>
		<dcterms:publisher rdf:resource="http://www.rcahms.gov.uk" />
		<skos:prefLabel xml:lang="en">PRE BUILD</skos:prefLabel>
		<dcterms:created rdf:datatype="http://www.w3.org/2001/XMLSchema#dateTime">2007-06-04T14:45:21</dcterms:created>
		<dcterms:modified rdf:datatype="http://www.w3.org/2001/XMLSchema#dateTime">2007-06-04T14:46:11</dcterms:modified>
		<dcterms:issued rdf:datatype="http://www.w3.org/2001/XMLSchema#dateTime">2013-07-17T10:08:40</dcterms:issued>
		<skos:narrower rdf:resource="http://purl.org/heritagedata/schemes/4/concepts/502513" />
		<skos:narrower>
			<skos:Concept rdf:about="http://purl.org/heritagedata/schemes/4/concepts/502529">
				<skos:inScheme rdf:resource="http://purl.org/heritagedata/schemes/4" />
				<dcterms:identifier>http://purl.org/heritagedata/schemes/4/concepts/502529</dcterms:identifier>
				<cc:license rdf:resource="http://reference.data.gov.uk/id/open-government-licence" />
				<cc:attributionURL rdf:resource="http://www.rcahms.gov.uk" />
				<cc:attributionName xml:lang="en">RCAHMS</cc:attributionName>
				<dcterms:publisher rdf:resource="http://www.rcahms.gov.uk" />
				<skos:prefLabel xml:lang="en">COMMISSION AND CONTRACT</skos:prefLabel>
				<dcterms:created rdf:datatype="http://www.w3.org/2001/XMLSchema#dateTime">2007-06-04T14:37:45</dcterms:created>
				<dcterms:modified rdf:datatype="http://www.w3.org/2001/XMLSchema#dateTime">2008-03-12T14:43:07</dcterms:modified>
				<dcterms:issued rdf:datatype="http://www.w3.org/2001/XMLSchema#dateTime">2013-07-17T10:08:40</dcterms:issued>
				<skos:broader rdf:resource="http://purl.org/heritagedata/schemes/4/concepts/502534" />
				<skos:scopeNote xml:lang="en">Details related to the commissioning of an architectural project and the date the contract for a project was awarded.</skos:scopeNote>
			</skos:Concept>
		</skos:narrower>
		<skos:broader rdf:resource="http://purl.org/heritagedata/schemes/4/concepts/502343" />
		<skos:scopeNote xml:lang="en">Events relating to the commissioning and design of a building. Use more specific term where available.</skos:scopeNote>
	</skos:Concept>
	<skos:Concept rdf:about="http://purl.org/heritagedata/schemes/4/concepts/502533">
		<skos:inScheme rdf:resource="http://purl.org/heritagedata/schemes/4" />
		<dcterms:identifier>http://purl.org/heritagedata/schemes/4/concepts/502533</dcterms:identifier>
		<cc:license rdf:resource="http://reference.data.gov.uk/id/open-government-licence" />
		<cc:attributionURL rdf:resource="http://www.rcahms.gov.uk" />
		<cc:attributionName xml:lang="en">RCAHMS</cc:attributionName>
		<dcterms:publisher rdf:resource="http://www.rcahms.gov.uk" />
		<skos:prefLabel xml:lang="en">DESTRUCTION</skos:prefLabel>
		<dcterms:created rdf:datatype="http://www.w3.org/2001/XMLSchema#dateTime">2007-06-04T14:43:18</dcterms:created>
		<dcterms:modified rdf:datatype="http://www.w3.org/2001/XMLSchema#dateTime">2007-06-04T14:44:09</dcterms:modified>
		<dcterms:issued rdf:datatype="http://www.w3.org/2001/XMLSchema#dateTime">2013-07-17T10:08:40</dcterms:issued>
		<skos:narrower rdf:resource="http://purl.org/heritagedata/schemes/4/concepts/502515" />
		<skos:narrower>
			<skos:Concept rdf:about="http://purl.org/heritagedata/schemes/4/concepts/502522">
				<skos:inScheme rdf:resource="http://purl.org/heritagedata/schemes/4" />
				<dcterms:identifier>http://purl.org/heritagedata/schemes/4/concepts/502522</dcterms:identifier>
				<cc:license rdf:resource="http://reference.data.gov.uk/id/open-government-licence" />
				<cc:attributionURL rdf:resource="http://www.rcahms.gov.uk" />
				<cc:attributionName xml:lang="en">RCAHMS</cc:attributionName>
				<dcterms:publisher rdf:resource="http://www.rcahms.gov.uk" />
				<skos:prefLabel xml:lang="en">PARTIAL DEMOLITION</skos:prefLabel>
				<dcterms:created rdf:datatype="http://www.w3.org/2001/XMLSchema#dateTime">2007-06-04T14:31:10</dcterms:created>
				<dcterms:modified rdf:datatype="http://www.w3.org/2001/XMLSchema#dateTime">2007-06-04T14:31:49</dcterms:modified>
				<dcterms:issued rdf:datatype="http://www.w3.org/2001/XMLSchema#dateTime">2013-07-17T10:08:40</dcterms:issued>
				<skos:broader rdf:resource="http://purl.org/heritagedata/schemes/4/concepts/502533" />
				<skos:scopeNote xml:lang="en">The partial demolition of a building;  e.g. removal of one wing of a Country House.</skos:scopeNote>
			</skos:Concept>
		</skos:narrower>
		<skos:narrower>
			<skos:Concept rdf:about="http://purl.org/heritagedata/schemes/4/concepts/502523">
				<skos:inScheme rdf:resource="http://purl.org/heritagedata/schemes/4" />
				<dcterms:identifier>http://purl.org/heritagedata/schemes/4/concepts/502523</dcterms:identifier>
				<cc:license rdf:resource="http://reference.data.gov.uk/id/open-government-licence" />
				<cc:attributionURL rdf:resource="http://www.rcahms.gov.uk" />
				<cc:attributionName xml:lang="en">RCAHMS</cc:attributionName>
				<dcterms:publisher rdf:resource="http://www.rcahms.gov.uk" />
				<skos:prefLabel xml:lang="en">COMPLETE DEMOLITION</skos:prefLabel>
				<dcterms:created rdf:datatype="http://www.w3.org/2001/XMLSchema#dateTime">2007-06-04T14:32:01</dcterms:created>
				<dcterms:modified rdf:datatype="http://www.w3.org/2001/XMLSchema#dateTime">2007-06-04T14:32:26</dcterms:modified>
				<dcterms:issued rdf:datatype="http://www.w3.org/2001/XMLSchema#dateTime">2013-07-17T10:08:40</dcterms:issued>
				<skos:broader rdf:resource="http://purl.org/heritagedata/schemes/4/concepts/502533" />
				<skos:scopeNote xml:lang="en">The complete demolition of a building.</skos:scopeNote>
			</skos:Concept>
		</skos:narrower>
		<skos:broader rdf:resource="http://purl.org/heritagedata/schemes/4/concepts/502343" />
		<skos:scopeNote xml:lang="en">The partial or complete destruction of a building - use more specific term where possible.</skos:scopeNote>
	</skos:Concept>
	<skos:Concept rdf:about="http://purl.org/heritagedata/schemes/4/concepts/502535">
		<skos:inScheme rdf:resource="http://purl.org/heritagedata/schemes/4" />
		<dcterms:identifier>http://purl.org/heritagedata/schemes/4/concepts/502535</dcterms:identifier>
		<cc:license rdf:resource="http://reference.data.gov.uk/id/open-government-licence" />
		<cc:attributionURL rdf:resource="http://www.rcahms.gov.uk" />
		<cc:attributionName xml:lang="en">RCAHMS</cc:attributionName>
		<dcterms:publisher rdf:resource="http://www.rcahms.gov.uk" />
		<skos:prefLabel xml:lang="en">BUILD</skos:prefLabel>
		<dcterms:created rdf:datatype="http://www.w3.org/2001/XMLSchema#dateTime">2007-06-04T14:48:05</dcterms:created>
		<dcterms:modified rdf:datatype="http://www.w3.org/2001/XMLSchema#dateTime">2007-06-05T11:00:26</dcterms:modified>
		<dcterms:issued rdf:datatype="http://www.w3.org/2001/XMLSchema#dateTime">2013-07-17T10:08:40</dcterms:issued>
		<skos:narrower>
			<skos:Concept rdf:about="http://purl.org/heritagedata/schemes/4/concepts/502519">
				<skos:inScheme rdf:resource="http://purl.org/heritagedata/schemes/4" />
				<dcterms:identifier>http://purl.org/heritagedata/schemes/4/concepts/502519</dcterms:identifier>
				<cc:license rdf:resource="http://reference.data.gov.uk/id/open-government-licence" />
				<cc:attributionURL rdf:resource="http://www.rcahms.gov.uk" />
				<cc:attributionName xml:lang="en">RCAHMS</cc:attributionName>
				<dcterms:publisher rdf:resource="http://www.rcahms.gov.uk" />
				<skos:prefLabel xml:lang="en">DISPLAY</skos:prefLabel>
				<dcterms:created rdf:datatype="http://www.w3.org/2001/XMLSchema#dateTime">2007-06-04T14:25:54</dcterms:created>
				<dcterms:modified rdf:datatype="http://www.w3.org/2001/XMLSchema#dateTime">2008-05-19T11:22:34</dcterms:modified>
				<dcterms:issued rdf:datatype="http://www.w3.org/2001/XMLSchema#dateTime">2013-07-17T10:08:40</dcterms:issued>
				<skos:broader rdf:resource="http://purl.org/heritagedata/schemes/4/concepts/502535" />
				<skos:scopeNote xml:lang="en">The setting out of a building, monument or maritime object for the purposes of public display or recreational diving. This includes temporary exhibitions.</skos:scopeNote>
			</skos:Concept>
		</skos:narrower>
		<skos:narrower>
			<skos:Concept rdf:about="http://purl.org/heritagedata/schemes/4/concepts/502524">
				<skos:inScheme rdf:resource="http://purl.org/heritagedata/schemes/4" />
				<dcterms:identifier>http://purl.org/heritagedata/schemes/4/concepts/502524</dcterms:identifier>
				<cc:license rdf:resource="http://reference.data.gov.uk/id/open-government-licence" />
				<cc:attributionURL rdf:resource="http://www.rcahms.gov.uk" />
				<cc:attributionName xml:lang="en">RCAHMS</cc:attributionName>
				<dcterms:publisher rdf:resource="http://www.rcahms.gov.uk" />
				<skos:prefLabel xml:lang="en">MODIFICATION</skos:prefLabel>
				<dcterms:created rdf:datatype="http://www.w3.org/2001/XMLSchema#dateTime">2007-06-04T14:33:21</dcterms:created>
				<dcterms:modified rdf:datatype="http://www.w3.org/2001/XMLSchema#dateTime">2007-10-08T16:41:31</dcterms:modified>
				<dcterms:issued rdf:datatype="http://www.w3.org/2001/XMLSchema#dateTime">2013-07-17T10:08:40</dcterms:issued>
				<skos:broader rdf:resource="http://purl.org/heritagedata/schemes/4/concepts/502535" />
				<skos:scopeNote xml:lang="en">Alterations to the original fabric of a building that results in a significant enlargement of the structure, and/or change of use.  A related  change of use event record should be created  as a sub-event from the Modification record.  Not to be used for minor alterations to an existing structure.</skos:scopeNote>
			</skos:Concept>
		</skos:narrower>
		<skos:narrower rdf:resource="http://purl.org/heritagedata/schemes/4/concepts/502527" />
		<skos:broader rdf:resource="http://purl.org/heritagedata/schemes/4/concepts/502343" />
		<skos:narrower>
			<skos:Concept rdf:about="http://purl.org/heritagedata/schemes/4/concepts/502526">
				<skos:inScheme rdf:resource="http://purl.org/heritagedata/schemes/4" />
				<dcterms:identifier>http://purl.org/heritagedata/schemes/4/concepts/502526</dcterms:identifier>
				<cc:license rdf:resource="http://reference.data.gov.uk/id/open-government-licence" />
				<cc:attributionURL rdf:resource="http://www.rcahms.gov.uk" />
				<cc:attributionName xml:lang="en">RCAHMS</cc:attributionName>
				<dcterms:publisher rdf:resource="http://www.rcahms.gov.uk" />
				<skos:prefLabel xml:lang="en">CONSTRUCTION</skos:prefLabel>
				<dcterms:created rdf:datatype="http://www.w3.org/2001/XMLSchema#dateTime">2007-06-04T14:35:51</dcterms:created>
				<dcterms:modified rdf:datatype="http://www.w3.org/2001/XMLSchema#dateTime">2007-06-04T14:36:03</dcterms:modified>
				<dcterms:issued rdf:datatype="http://www.w3.org/2001/XMLSchema#dateTime">2013-07-17T10:08:40</dcterms:issued>
				<skos:broader rdf:resource="http://purl.org/heritagedata/schemes/4/concepts/502535" />
				<skos:scopeNote xml:lang="en">The date when the building was built.</skos:scopeNote>
			</skos:Concept>
		</skos:narrower>
		<skos:scopeNote xml:lang="en">Events relating to the initial construction or alteration of a building.</skos:scopeNote>
	</skos:Concept>
	<skos:Concept rdf:about="http://purl.org/heritagedata/schemes/4/concepts/502592">
		<skos:inScheme rdf:resource="http://purl.org/heritagedata/schemes/4" />
		<dcterms:identifier>http://purl.org/heritagedata/schemes/4/concepts/502592</dcterms:identifier>
		<cc:license rdf:resource="http://reference.data.gov.uk/id/open-government-licence" />
		<cc:attributionURL rdf:resource="http://www.rcahms.gov.uk" />
		<cc:attributionName xml:lang="en">RCAHMS</cc:attributionName>
		<dcterms:publisher rdf:resource="http://www.rcahms.gov.uk" />
		<skos:prefLabel xml:lang="en">PHOTOGRAPHIC RECORD</skos:prefLabel>
		<dcterms:created rdf:datatype="http://www.w3.org/2001/XMLSchema#dateTime">2007-06-14T16:19:00</dcterms:created>
		<dcterms:modified rdf:datatype="http://www.w3.org/2001/XMLSchema#dateTime">2007-06-14T16:19:57</dcterms:modified>
		<dcterms:issued rdf:datatype="http://www.w3.org/2001/XMLSchema#dateTime">2013-07-17T10:08:40</dcterms:issued>
		<skos:broader rdf:resource="http://purl.org/heritagedata/schemes/4/concepts/502432" />
		<skos:broader rdf:resource="http://purl.org/heritagedata/schemes/4/concepts/502362" />
		<skos:scopeNote xml:lang="en">Photographs taken during informal visits to sites.  Photography may include those taken by antiquarians, amateur archaeologists or architectural students.  More formal, detailed surveys should be termed 'Photographic Survey'.</skos:scopeNote>
	</skos:Concept>
</rdf:RDF>